<?xml version="1.0"?>
<rdf:RDF xmlns="http://JP_ontology.org/assessment/"
     xml:base="http://JP_ontology.org/assessment/"
     xmlns:owl="http://www.w3.org/2002/07/owl#"
     xmlns:rdf="http://www.w3.org/1999/02/22-rdf-syntax-ns#"
     xmlns:xml="http://www.w3.org/XML/1998/namespace"
     xmlns:xsd="http://www.w3.org/2001/XMLSchema#"
     xmlns:rdfs="http://www.w3.org/2000/01/rdf-schema#"
     xmlns:skos="http://www.w3.org/2004/02/skos/core#"
     xmlns:nis2v="http://JP_ontology.org/nis2v#"
     xmlns:terms="http://purl.org/dc/terms/">
    <owl:Ontology rdf:about="http://JP_ontology.org/assessment/">
        <owl:imports rdf:resource="http://JP_ontology.org/iso27001/"/>
        <owl:imports rdf:resource="http://JP_ontology.org/nis2v/"/>
    </owl:Ontology>
    


    <!-- 
    ///////////////////////////////////////////////////////////////////////////////////////
    //
    // Annotation properties
    //
    ///////////////////////////////////////////////////////////////////////////////////////
     -->


    


    <!-- http://JP_ontology.org/nis2v#hasAnswer -->


    <owl:AnnotationProperty rdf:about="http://JP_ontology.org/nis2v#hasAnswer"/>
    


    <!-- http://JP_ontology.org/nis2v#relatedToControl -->


    <owl:AnnotationProperty rdf:about="http://JP_ontology.org/nis2v#relatedToControl"/>
    


    <!-- http://purl.org/dc/terms/contributor -->


    <owl:AnnotationProperty rdf:about="http://purl.org/dc/terms/contributor"/>
    


    <!-- http://purl.org/dc/terms/created -->


    <owl:AnnotationProperty rdf:about="http://purl.org/dc/terms/created"/>
    


    <!-- http://purl.org/dc/terms/subject -->


    <owl:AnnotationProperty rdf:about="http://purl.org/dc/terms/subject"/>
    


    <!-- http://www.w3.org/2004/02/skos/core#altLabel -->


    <owl:AnnotationProperty rdf:about="http://www.w3.org/2004/02/skos/core#altLabel"/>
    


    <!-- http://www.w3.org/2004/02/skos/core#broader -->


    <owl:AnnotationProperty rdf:about="http://www.w3.org/2004/02/skos/core#broader"/>
    


    <!-- http://www.w3.org/2004/02/skos/core#definition -->


    <owl:AnnotationProperty rdf:about="http://www.w3.org/2004/02/skos/core#definition"/>
    


    <!-- http://www.w3.org/2004/02/skos/core#prefLabel -->


    <owl:AnnotationProperty rdf:about="http://www.w3.org/2004/02/skos/core#prefLabel"/>
    


    <!-- 
    ///////////////////////////////////////////////////////////////////////////////////////
    //
    // Datatypes
    //
    ///////////////////////////////////////////////////////////////////////////////////////
     -->


    


    <!-- http://www.w3.org/2001/XMLSchema#date -->


    <rdfs:Datatype rdf:about="http://www.w3.org/2001/XMLSchema#date"/>
    


    <!-- 
    ///////////////////////////////////////////////////////////////////////////////////////
    //
    // Classes
    //
    ///////////////////////////////////////////////////////////////////////////////////////
     -->


    


    <!-- http://JP_ontology.org/assessment/AssessmentQuestion -->


    <owl:Class rdf:about="http://JP_ontology.org/assessment/AssessmentQuestion">
        <rdfs:subClassOf rdf:resource="http://JP_ontology.org/iso27001/ISOControl270012022"/>
        <terms:contributor>Jenni Parry</terms:contributor>
        <terms:created rdf:datatype="http://www.w3.org/2001/XMLSchema#date">2024-04-18</terms:created>
        <rdfs:isDefinedBy rdf:resource="http://JP_ontology.org/assessment"/>
        <skos:definition xml:lang="en">Represents the set of questions used to perform a gap analysis to assess compliance against ISO 27001:2022 controls and the NIS2 Cybersecurity Measures.</skos:definition>
        <skos:prefLabel xml:lang="en">Assessment Question</skos:prefLabel>
    </owl:Class>
    


    <!-- http://JP_ontology.org/assessment/MCQ.1 -->


    <owl:Class rdf:about="http://JP_ontology.org/assessment/MCQ.1">
        <rdfs:subClassOf rdf:resource="http://JP_ontology.org/assessment/AssessmentQuestion"/>
    </owl:Class>
    


    <!-- http://JP_ontology.org/assessment/MCQ.10.1 -->


    <owl:Class rdf:about="http://JP_ontology.org/assessment/MCQ.10.1">
        <rdfs:subClassOf rdf:resource="http://JP_ontology.org/assessment/AssessmentQuestion"/>
    </owl:Class>
    


    <!-- http://JP_ontology.org/assessment/MCQ.10.2 -->


    <owl:Class rdf:about="http://JP_ontology.org/assessment/MCQ.10.2">
        <rdfs:subClassOf rdf:resource="http://JP_ontology.org/assessment/AssessmentQuestion"/>
    </owl:Class>
    


    <!-- http://JP_ontology.org/assessment/MCQ.100 -->


    <owl:Class rdf:about="http://JP_ontology.org/assessment/MCQ.100">
        <rdfs:subClassOf rdf:resource="http://JP_ontology.org/assessment/AssessmentQuestion"/>
    </owl:Class>
    


    <!-- http://JP_ontology.org/assessment/MCQ.101 -->


    <owl:Class rdf:about="http://JP_ontology.org/assessment/MCQ.101">
        <rdfs:subClassOf rdf:resource="http://JP_ontology.org/assessment/AssessmentQuestion"/>
    </owl:Class>
    


    <!-- http://JP_ontology.org/assessment/MCQ.102 -->


    <owl:Class rdf:about="http://JP_ontology.org/assessment/MCQ.102">
        <rdfs:subClassOf rdf:resource="http://JP_ontology.org/assessment/AssessmentQuestion"/>
    </owl:Class>
    


    <!-- http://JP_ontology.org/assessment/MCQ.103 -->


    <owl:Class rdf:about="http://JP_ontology.org/assessment/MCQ.103">
        <rdfs:subClassOf rdf:resource="http://JP_ontology.org/assessment/AssessmentQuestion"/>
    </owl:Class>
    


    <!-- http://JP_ontology.org/assessment/MCQ.104 -->


    <owl:Class rdf:about="http://JP_ontology.org/assessment/MCQ.104">
        <rdfs:subClassOf rdf:resource="http://JP_ontology.org/assessment/AssessmentQuestion"/>
    </owl:Class>
    


    <!-- http://JP_ontology.org/assessment/MCQ.105.1 -->


    <owl:Class rdf:about="http://JP_ontology.org/assessment/MCQ.105.1">
        <rdfs:subClassOf rdf:resource="http://JP_ontology.org/assessment/AssessmentQuestion"/>
    </owl:Class>
    


    <!-- http://JP_ontology.org/assessment/MCQ.105.2 -->


    <owl:Class rdf:about="http://JP_ontology.org/assessment/MCQ.105.2">
        <rdfs:subClassOf rdf:resource="http://JP_ontology.org/assessment/AssessmentQuestion"/>
    </owl:Class>
    


    <!-- http://JP_ontology.org/assessment/MCQ.105.3 -->


    <owl:Class rdf:about="http://JP_ontology.org/assessment/MCQ.105.3">
        <rdfs:subClassOf rdf:resource="http://JP_ontology.org/assessment/AssessmentQuestion"/>
    </owl:Class>
    


    <!-- http://JP_ontology.org/assessment/MCQ.106.1 -->


    <owl:Class rdf:about="http://JP_ontology.org/assessment/MCQ.106.1">
        <rdfs:subClassOf rdf:resource="http://JP_ontology.org/assessment/AssessmentQuestion"/>
    </owl:Class>
    


    <!-- http://JP_ontology.org/assessment/MCQ.106.2 -->


    <owl:Class rdf:about="http://JP_ontology.org/assessment/MCQ.106.2">
        <rdfs:subClassOf rdf:resource="http://JP_ontology.org/assessment/AssessmentQuestion"/>
    </owl:Class>
    


    <!-- http://JP_ontology.org/assessment/MCQ.107.1 -->


    <owl:Class rdf:about="http://JP_ontology.org/assessment/MCQ.107.1">
        <rdfs:subClassOf rdf:resource="http://JP_ontology.org/assessment/AssessmentQuestion"/>
    </owl:Class>
    


    <!-- http://JP_ontology.org/assessment/MCQ.107.2 -->


    <owl:Class rdf:about="http://JP_ontology.org/assessment/MCQ.107.2">
        <rdfs:subClassOf rdf:resource="http://JP_ontology.org/assessment/AssessmentQuestion"/>
    </owl:Class>
    


    <!-- http://JP_ontology.org/assessment/MCQ.108 -->


    <owl:Class rdf:about="http://JP_ontology.org/assessment/MCQ.108">
        <rdfs:subClassOf rdf:resource="http://JP_ontology.org/assessment/AssessmentQuestion"/>
    </owl:Class>
    


    <!-- http://JP_ontology.org/assessment/MCQ.109 -->


    <owl:Class rdf:about="http://JP_ontology.org/assessment/MCQ.109">
        <rdfs:subClassOf rdf:resource="http://JP_ontology.org/assessment/AssessmentQuestion"/>
    </owl:Class>
    


    <!-- http://JP_ontology.org/assessment/MCQ.11 -->


    <owl:Class rdf:about="http://JP_ontology.org/assessment/MCQ.11">
        <rdfs:subClassOf rdf:resource="http://JP_ontology.org/assessment/AssessmentQuestion"/>
    </owl:Class>
    


    <!-- http://JP_ontology.org/assessment/MCQ.110 -->


    <owl:Class rdf:about="http://JP_ontology.org/assessment/MCQ.110">
        <rdfs:subClassOf rdf:resource="http://JP_ontology.org/assessment/AssessmentQuestion"/>
    </owl:Class>
    


    <!-- http://JP_ontology.org/assessment/MCQ.111 -->


    <owl:Class rdf:about="http://JP_ontology.org/assessment/MCQ.111">
        <rdfs:subClassOf rdf:resource="http://JP_ontology.org/assessment/AssessmentQuestion"/>
    </owl:Class>
    


    <!-- http://JP_ontology.org/assessment/MCQ.112.1 -->


    <owl:Class rdf:about="http://JP_ontology.org/assessment/MCQ.112.1">
        <rdfs:subClassOf rdf:resource="http://JP_ontology.org/assessment/AssessmentQuestion"/>
    </owl:Class>
    


    <!-- http://JP_ontology.org/assessment/MCQ.112.2 -->


    <owl:Class rdf:about="http://JP_ontology.org/assessment/MCQ.112.2">
        <rdfs:subClassOf rdf:resource="http://JP_ontology.org/assessment/AssessmentQuestion"/>
    </owl:Class>
    


    <!-- http://JP_ontology.org/assessment/MCQ.113 -->


    <owl:Class rdf:about="http://JP_ontology.org/assessment/MCQ.113">
        <rdfs:subClassOf rdf:resource="http://JP_ontology.org/assessment/AssessmentQuestion"/>
    </owl:Class>
    


    <!-- http://JP_ontology.org/assessment/MCQ.114 -->


    <owl:Class rdf:about="http://JP_ontology.org/assessment/MCQ.114">
        <rdfs:subClassOf rdf:resource="http://JP_ontology.org/assessment/AssessmentQuestion"/>
    </owl:Class>
    


    <!-- http://JP_ontology.org/assessment/MCQ.115 -->


    <owl:Class rdf:about="http://JP_ontology.org/assessment/MCQ.115">
        <rdfs:subClassOf rdf:resource="http://JP_ontology.org/assessment/AssessmentQuestion"/>
    </owl:Class>
    


    <!-- http://JP_ontology.org/assessment/MCQ.116 -->


    <owl:Class rdf:about="http://JP_ontology.org/assessment/MCQ.116">
        <rdfs:subClassOf rdf:resource="http://JP_ontology.org/assessment/AssessmentQuestion"/>
    </owl:Class>
    


    <!-- http://JP_ontology.org/assessment/MCQ.117 -->


    <owl:Class rdf:about="http://JP_ontology.org/assessment/MCQ.117">
        <rdfs:subClassOf rdf:resource="http://JP_ontology.org/assessment/AssessmentQuestion"/>
    </owl:Class>
    


    <!-- http://JP_ontology.org/assessment/MCQ.118 -->


    <owl:Class rdf:about="http://JP_ontology.org/assessment/MCQ.118">
        <rdfs:subClassOf rdf:resource="http://JP_ontology.org/assessment/AssessmentQuestion"/>
    </owl:Class>
    


    <!-- http://JP_ontology.org/assessment/MCQ.119 -->


    <owl:Class rdf:about="http://JP_ontology.org/assessment/MCQ.119">
        <rdfs:subClassOf rdf:resource="http://JP_ontology.org/assessment/AssessmentQuestion"/>
    </owl:Class>
    


    <!-- http://JP_ontology.org/assessment/MCQ.12 -->


    <owl:Class rdf:about="http://JP_ontology.org/assessment/MCQ.12">
        <rdfs:subClassOf rdf:resource="http://JP_ontology.org/assessment/AssessmentQuestion"/>
    </owl:Class>
    


    <!-- http://JP_ontology.org/assessment/MCQ.120 -->


    <owl:Class rdf:about="http://JP_ontology.org/assessment/MCQ.120">
        <rdfs:subClassOf rdf:resource="http://JP_ontology.org/assessment/AssessmentQuestion"/>
    </owl:Class>
    


    <!-- http://JP_ontology.org/assessment/MCQ.121 -->


    <owl:Class rdf:about="http://JP_ontology.org/assessment/MCQ.121">
        <rdfs:subClassOf rdf:resource="http://JP_ontology.org/assessment/AssessmentQuestion"/>
    </owl:Class>
    


    <!-- http://JP_ontology.org/assessment/MCQ.122 -->


    <owl:Class rdf:about="http://JP_ontology.org/assessment/MCQ.122">
        <rdfs:subClassOf rdf:resource="http://JP_ontology.org/assessment/AssessmentQuestion"/>
    </owl:Class>
    


    <!-- http://JP_ontology.org/assessment/MCQ.123 -->


    <owl:Class rdf:about="http://JP_ontology.org/assessment/MCQ.123">
        <rdfs:subClassOf rdf:resource="http://JP_ontology.org/assessment/AssessmentQuestion"/>
    </owl:Class>
    


    <!-- http://JP_ontology.org/assessment/MCQ.124 -->


    <owl:Class rdf:about="http://JP_ontology.org/assessment/MCQ.124">
        <rdfs:subClassOf rdf:resource="http://JP_ontology.org/assessment/AssessmentQuestion"/>
    </owl:Class>
    


    <!-- http://JP_ontology.org/assessment/MCQ.125 -->


    <owl:Class rdf:about="http://JP_ontology.org/assessment/MCQ.125">
        <rdfs:subClassOf rdf:resource="http://JP_ontology.org/assessment/AssessmentQuestion"/>
    </owl:Class>
    


    <!-- http://JP_ontology.org/assessment/MCQ.126 -->


    <owl:Class rdf:about="http://JP_ontology.org/assessment/MCQ.126">
        <rdfs:subClassOf rdf:resource="http://JP_ontology.org/assessment/AssessmentQuestion"/>
    </owl:Class>
    


    <!-- http://JP_ontology.org/assessment/MCQ.127 -->


    <owl:Class rdf:about="http://JP_ontology.org/assessment/MCQ.127">
        <rdfs:subClassOf rdf:resource="http://JP_ontology.org/assessment/AssessmentQuestion"/>
    </owl:Class>
    


    <!-- http://JP_ontology.org/assessment/MCQ.128 -->


    <owl:Class rdf:about="http://JP_ontology.org/assessment/MCQ.128">
        <rdfs:subClassOf rdf:resource="http://JP_ontology.org/assessment/AssessmentQuestion"/>
    </owl:Class>
    


    <!-- http://JP_ontology.org/assessment/MCQ.129 -->


    <owl:Class rdf:about="http://JP_ontology.org/assessment/MCQ.129">
        <rdfs:subClassOf rdf:resource="http://JP_ontology.org/assessment/AssessmentQuestion"/>
    </owl:Class>
    


    <!-- http://JP_ontology.org/assessment/MCQ.13 -->


    <owl:Class rdf:about="http://JP_ontology.org/assessment/MCQ.13">
        <rdfs:subClassOf rdf:resource="http://JP_ontology.org/assessment/AssessmentQuestion"/>
    </owl:Class>
    


    <!-- http://JP_ontology.org/assessment/MCQ.130 -->


    <owl:Class rdf:about="http://JP_ontology.org/assessment/MCQ.130">
        <rdfs:subClassOf rdf:resource="http://JP_ontology.org/assessment/AssessmentQuestion"/>
    </owl:Class>
    


    <!-- http://JP_ontology.org/assessment/MCQ.14 -->


    <owl:Class rdf:about="http://JP_ontology.org/assessment/MCQ.14">
        <rdfs:subClassOf rdf:resource="http://JP_ontology.org/assessment/AssessmentQuestion"/>
    </owl:Class>
    


    <!-- http://JP_ontology.org/assessment/MCQ.15 -->


    <owl:Class rdf:about="http://JP_ontology.org/assessment/MCQ.15">
        <rdfs:subClassOf rdf:resource="http://JP_ontology.org/assessment/AssessmentQuestion"/>
    </owl:Class>
    


    <!-- http://JP_ontology.org/assessment/MCQ.16 -->


    <owl:Class rdf:about="http://JP_ontology.org/assessment/MCQ.16">
        <rdfs:subClassOf rdf:resource="http://JP_ontology.org/assessment/AssessmentQuestion"/>
    </owl:Class>
    


    <!-- http://JP_ontology.org/assessment/MCQ.17 -->


    <owl:Class rdf:about="http://JP_ontology.org/assessment/MCQ.17">
        <rdfs:subClassOf rdf:resource="http://JP_ontology.org/assessment/AssessmentQuestion"/>
    </owl:Class>
    


    <!-- http://JP_ontology.org/assessment/MCQ.18 -->


    <owl:Class rdf:about="http://JP_ontology.org/assessment/MCQ.18">
        <rdfs:subClassOf rdf:resource="http://JP_ontology.org/assessment/AssessmentQuestion"/>
    </owl:Class>
    


    <!-- http://JP_ontology.org/assessment/MCQ.19 -->


    <owl:Class rdf:about="http://JP_ontology.org/assessment/MCQ.19">
        <rdfs:subClassOf rdf:resource="http://JP_ontology.org/assessment/AssessmentQuestion"/>
    </owl:Class>
    


    <!-- http://JP_ontology.org/assessment/MCQ.2.1 -->


    <owl:Class rdf:about="http://JP_ontology.org/assessment/MCQ.2.1">
        <rdfs:subClassOf rdf:resource="http://JP_ontology.org/assessment/AssessmentQuestion"/>
    </owl:Class>
    


    <!-- http://JP_ontology.org/assessment/MCQ.2.2 -->


    <owl:Class rdf:about="http://JP_ontology.org/assessment/MCQ.2.2">
        <rdfs:subClassOf rdf:resource="http://JP_ontology.org/assessment/AssessmentQuestion"/>
    </owl:Class>
    


    <!-- http://JP_ontology.org/assessment/MCQ.20 -->


    <owl:Class rdf:about="http://JP_ontology.org/assessment/MCQ.20">
        <rdfs:subClassOf rdf:resource="http://JP_ontology.org/assessment/AssessmentQuestion"/>
    </owl:Class>
    


    <!-- http://JP_ontology.org/assessment/MCQ.21 -->


    <owl:Class rdf:about="http://JP_ontology.org/assessment/MCQ.21">
        <rdfs:subClassOf rdf:resource="http://JP_ontology.org/assessment/AssessmentQuestion"/>
    </owl:Class>
    


    <!-- http://JP_ontology.org/assessment/MCQ.22.1 -->


    <owl:Class rdf:about="http://JP_ontology.org/assessment/MCQ.22.1">
        <rdfs:subClassOf rdf:resource="http://JP_ontology.org/assessment/AssessmentQuestion"/>
    </owl:Class>
    


    <!-- http://JP_ontology.org/assessment/MCQ.22.2 -->


    <owl:Class rdf:about="http://JP_ontology.org/assessment/MCQ.22.2">
        <rdfs:subClassOf rdf:resource="http://JP_ontology.org/assessment/AssessmentQuestion"/>
    </owl:Class>
    


    <!-- http://JP_ontology.org/assessment/MCQ.22.3 -->


    <owl:Class rdf:about="http://JP_ontology.org/assessment/MCQ.22.3">
        <rdfs:subClassOf rdf:resource="http://JP_ontology.org/assessment/AssessmentQuestion"/>
    </owl:Class>
    


    <!-- http://JP_ontology.org/assessment/MCQ.22.4 -->


    <owl:Class rdf:about="http://JP_ontology.org/assessment/MCQ.22.4">
        <rdfs:subClassOf rdf:resource="http://JP_ontology.org/assessment/AssessmentQuestion"/>
    </owl:Class>
    


    <!-- http://JP_ontology.org/assessment/MCQ.22.5 -->


    <owl:Class rdf:about="http://JP_ontology.org/assessment/MCQ.22.5">
        <rdfs:subClassOf rdf:resource="http://JP_ontology.org/assessment/AssessmentQuestion"/>
    </owl:Class>
    


    <!-- http://JP_ontology.org/assessment/MCQ.23 -->


    <owl:Class rdf:about="http://JP_ontology.org/assessment/MCQ.23">
        <rdfs:subClassOf rdf:resource="http://JP_ontology.org/assessment/AssessmentQuestion"/>
    </owl:Class>
    


    <!-- http://JP_ontology.org/assessment/MCQ.24 -->


    <owl:Class rdf:about="http://JP_ontology.org/assessment/MCQ.24">
        <rdfs:subClassOf rdf:resource="http://JP_ontology.org/assessment/AssessmentQuestion"/>
    </owl:Class>
    


    <!-- http://JP_ontology.org/assessment/MCQ.25 -->


    <owl:Class rdf:about="http://JP_ontology.org/assessment/MCQ.25">
        <rdfs:subClassOf rdf:resource="http://JP_ontology.org/assessment/AssessmentQuestion"/>
    </owl:Class>
    


    <!-- http://JP_ontology.org/assessment/MCQ.26 -->


    <owl:Class rdf:about="http://JP_ontology.org/assessment/MCQ.26">
        <rdfs:subClassOf rdf:resource="http://JP_ontology.org/assessment/AssessmentQuestion"/>
    </owl:Class>
    


    <!-- http://JP_ontology.org/assessment/MCQ.27 -->


    <owl:Class rdf:about="http://JP_ontology.org/assessment/MCQ.27">
        <rdfs:subClassOf rdf:resource="http://JP_ontology.org/assessment/AssessmentQuestion"/>
    </owl:Class>
    


    <!-- http://JP_ontology.org/assessment/MCQ.28 -->


    <owl:Class rdf:about="http://JP_ontology.org/assessment/MCQ.28">
        <rdfs:subClassOf rdf:resource="http://JP_ontology.org/assessment/AssessmentQuestion"/>
    </owl:Class>
    


    <!-- http://JP_ontology.org/assessment/MCQ.29 -->


    <owl:Class rdf:about="http://JP_ontology.org/assessment/MCQ.29">
        <rdfs:subClassOf rdf:resource="http://JP_ontology.org/assessment/AssessmentQuestion"/>
    </owl:Class>
    


    <!-- http://JP_ontology.org/assessment/MCQ.3.1 -->


    <owl:Class rdf:about="http://JP_ontology.org/assessment/MCQ.3.1">
        <rdfs:subClassOf rdf:resource="http://JP_ontology.org/assessment/AssessmentQuestion"/>
    </owl:Class>
    


    <!-- http://JP_ontology.org/assessment/MCQ.3.2 -->


    <owl:Class rdf:about="http://JP_ontology.org/assessment/MCQ.3.2">
        <rdfs:subClassOf rdf:resource="http://JP_ontology.org/assessment/AssessmentQuestion"/>
    </owl:Class>
    


    <!-- http://JP_ontology.org/assessment/MCQ.30 -->


    <owl:Class rdf:about="http://JP_ontology.org/assessment/MCQ.30">
        <rdfs:subClassOf rdf:resource="http://JP_ontology.org/assessment/AssessmentQuestion"/>
    </owl:Class>
    


    <!-- http://JP_ontology.org/assessment/MCQ.31 -->


    <owl:Class rdf:about="http://JP_ontology.org/assessment/MCQ.31">
        <rdfs:subClassOf rdf:resource="http://JP_ontology.org/assessment/AssessmentQuestion"/>
    </owl:Class>
    


    <!-- http://JP_ontology.org/assessment/MCQ.32 -->


    <owl:Class rdf:about="http://JP_ontology.org/assessment/MCQ.32">
        <rdfs:subClassOf rdf:resource="http://JP_ontology.org/assessment/AssessmentQuestion"/>
    </owl:Class>
    


    <!-- http://JP_ontology.org/assessment/MCQ.33 -->


    <owl:Class rdf:about="http://JP_ontology.org/assessment/MCQ.33">
        <rdfs:subClassOf rdf:resource="http://JP_ontology.org/assessment/AssessmentQuestion"/>
    </owl:Class>
    


    <!-- http://JP_ontology.org/assessment/MCQ.34.1 -->


    <owl:Class rdf:about="http://JP_ontology.org/assessment/MCQ.34.1">
        <rdfs:subClassOf rdf:resource="http://JP_ontology.org/assessment/AssessmentQuestion"/>
    </owl:Class>
    


    <!-- http://JP_ontology.org/assessment/MCQ.34.2 -->


    <owl:Class rdf:about="http://JP_ontology.org/assessment/MCQ.34.2">
        <rdfs:subClassOf rdf:resource="http://JP_ontology.org/assessment/AssessmentQuestion"/>
    </owl:Class>
    


    <!-- http://JP_ontology.org/assessment/MCQ.34.3 -->


    <owl:Class rdf:about="http://JP_ontology.org/assessment/MCQ.34.3">
        <rdfs:subClassOf rdf:resource="http://JP_ontology.org/assessment/AssessmentQuestion"/>
    </owl:Class>
    


    <!-- http://JP_ontology.org/assessment/MCQ.34.4 -->


    <owl:Class rdf:about="http://JP_ontology.org/assessment/MCQ.34.4">
        <rdfs:subClassOf rdf:resource="http://JP_ontology.org/assessment/AssessmentQuestion"/>
    </owl:Class>
    


    <!-- http://JP_ontology.org/assessment/MCQ.35 -->


    <owl:Class rdf:about="http://JP_ontology.org/assessment/MCQ.35">
        <rdfs:subClassOf rdf:resource="http://JP_ontology.org/assessment/AssessmentQuestion"/>
    </owl:Class>
    


    <!-- http://JP_ontology.org/assessment/MCQ.36 -->


    <owl:Class rdf:about="http://JP_ontology.org/assessment/MCQ.36">
        <rdfs:subClassOf rdf:resource="http://JP_ontology.org/assessment/AssessmentQuestion"/>
    </owl:Class>
    


    <!-- http://JP_ontology.org/assessment/MCQ.37 -->


    <owl:Class rdf:about="http://JP_ontology.org/assessment/MCQ.37">
        <rdfs:subClassOf rdf:resource="http://JP_ontology.org/assessment/AssessmentQuestion"/>
    </owl:Class>
    


    <!-- http://JP_ontology.org/assessment/MCQ.38 -->


    <owl:Class rdf:about="http://JP_ontology.org/assessment/MCQ.38">
        <rdfs:subClassOf rdf:resource="http://JP_ontology.org/assessment/AssessmentQuestion"/>
    </owl:Class>
    


    <!-- http://JP_ontology.org/assessment/MCQ.39 -->


    <owl:Class rdf:about="http://JP_ontology.org/assessment/MCQ.39">
        <rdfs:subClassOf rdf:resource="http://JP_ontology.org/assessment/AssessmentQuestion"/>
    </owl:Class>
    


    <!-- http://JP_ontology.org/assessment/MCQ.4.1 -->


    <owl:Class rdf:about="http://JP_ontology.org/assessment/MCQ.4.1">
        <rdfs:subClassOf rdf:resource="http://JP_ontology.org/assessment/AssessmentQuestion"/>
    </owl:Class>
    


    <!-- http://JP_ontology.org/assessment/MCQ.4.2 -->


    <owl:Class rdf:about="http://JP_ontology.org/assessment/MCQ.4.2">
        <rdfs:subClassOf rdf:resource="http://JP_ontology.org/assessment/AssessmentQuestion"/>
    </owl:Class>
    


    <!-- http://JP_ontology.org/assessment/MCQ.4.3 -->


    <owl:Class rdf:about="http://JP_ontology.org/assessment/MCQ.4.3">
        <rdfs:subClassOf rdf:resource="http://JP_ontology.org/assessment/AssessmentQuestion"/>
    </owl:Class>
    


    <!-- http://JP_ontology.org/assessment/MCQ.4.4 -->


    <owl:Class rdf:about="http://JP_ontology.org/assessment/MCQ.4.4">
        <rdfs:subClassOf rdf:resource="http://JP_ontology.org/assessment/AssessmentQuestion"/>
    </owl:Class>
    


    <!-- http://JP_ontology.org/assessment/MCQ.4.5 -->


    <owl:Class rdf:about="http://JP_ontology.org/assessment/MCQ.4.5">
        <rdfs:subClassOf rdf:resource="http://JP_ontology.org/assessment/AssessmentQuestion"/>
    </owl:Class>
    


    <!-- http://JP_ontology.org/assessment/MCQ.4.6 -->


    <owl:Class rdf:about="http://JP_ontology.org/assessment/MCQ.4.6">
        <rdfs:subClassOf rdf:resource="http://JP_ontology.org/assessment/AssessmentQuestion"/>
    </owl:Class>
    


    <!-- http://JP_ontology.org/assessment/MCQ.40 -->


    <owl:Class rdf:about="http://JP_ontology.org/assessment/MCQ.40">
        <rdfs:subClassOf rdf:resource="http://JP_ontology.org/assessment/AssessmentQuestion"/>
    </owl:Class>
    


    <!-- http://JP_ontology.org/assessment/MCQ.41 -->


    <owl:Class rdf:about="http://JP_ontology.org/assessment/MCQ.41">
        <rdfs:subClassOf rdf:resource="http://JP_ontology.org/assessment/AssessmentQuestion"/>
    </owl:Class>
    


    <!-- http://JP_ontology.org/assessment/MCQ.42 -->


    <owl:Class rdf:about="http://JP_ontology.org/assessment/MCQ.42">
        <rdfs:subClassOf rdf:resource="http://JP_ontology.org/assessment/AssessmentQuestion"/>
    </owl:Class>
    


    <!-- http://JP_ontology.org/assessment/MCQ.43 -->


    <owl:Class rdf:about="http://JP_ontology.org/assessment/MCQ.43">
        <rdfs:subClassOf rdf:resource="http://JP_ontology.org/assessment/AssessmentQuestion"/>
    </owl:Class>
    


    <!-- http://JP_ontology.org/assessment/MCQ.44 -->


    <owl:Class rdf:about="http://JP_ontology.org/assessment/MCQ.44">
        <rdfs:subClassOf rdf:resource="http://JP_ontology.org/assessment/AssessmentQuestion"/>
    </owl:Class>
    


    <!-- http://JP_ontology.org/assessment/MCQ.45 -->


    <owl:Class rdf:about="http://JP_ontology.org/assessment/MCQ.45">
        <rdfs:subClassOf rdf:resource="http://JP_ontology.org/assessment/AssessmentQuestion"/>
    </owl:Class>
    


    <!-- http://JP_ontology.org/assessment/MCQ.46 -->


    <owl:Class rdf:about="http://JP_ontology.org/assessment/MCQ.46">
        <rdfs:subClassOf rdf:resource="http://JP_ontology.org/assessment/AssessmentQuestion"/>
    </owl:Class>
    


    <!-- http://JP_ontology.org/assessment/MCQ.47 -->


    <owl:Class rdf:about="http://JP_ontology.org/assessment/MCQ.47">
        <rdfs:subClassOf rdf:resource="http://JP_ontology.org/assessment/AssessmentQuestion"/>
    </owl:Class>
    


    <!-- http://JP_ontology.org/assessment/MCQ.48 -->


    <owl:Class rdf:about="http://JP_ontology.org/assessment/MCQ.48">
        <rdfs:subClassOf rdf:resource="http://JP_ontology.org/assessment/AssessmentQuestion"/>
    </owl:Class>
    


    <!-- http://JP_ontology.org/assessment/MCQ.49.1 -->


    <owl:Class rdf:about="http://JP_ontology.org/assessment/MCQ.49.1">
        <rdfs:subClassOf rdf:resource="http://JP_ontology.org/assessment/AssessmentQuestion"/>
    </owl:Class>
    


    <!-- http://JP_ontology.org/assessment/MCQ.49.2 -->


    <owl:Class rdf:about="http://JP_ontology.org/assessment/MCQ.49.2">
        <rdfs:subClassOf rdf:resource="http://JP_ontology.org/assessment/AssessmentQuestion"/>
    </owl:Class>
    


    <!-- http://JP_ontology.org/assessment/MCQ.49.3 -->


    <owl:Class rdf:about="http://JP_ontology.org/assessment/MCQ.49.3">
        <rdfs:subClassOf rdf:resource="http://JP_ontology.org/assessment/AssessmentQuestion"/>
    </owl:Class>
    


    <!-- http://JP_ontology.org/assessment/MCQ.5.1 -->


    <owl:Class rdf:about="http://JP_ontology.org/assessment/MCQ.5.1">
        <rdfs:subClassOf rdf:resource="http://JP_ontology.org/assessment/AssessmentQuestion"/>
    </owl:Class>
    


    <!-- http://JP_ontology.org/assessment/MCQ.5.2 -->


    <owl:Class rdf:about="http://JP_ontology.org/assessment/MCQ.5.2">
        <rdfs:subClassOf rdf:resource="http://JP_ontology.org/assessment/AssessmentQuestion"/>
    </owl:Class>
    


    <!-- http://JP_ontology.org/assessment/MCQ.5.3 -->


    <owl:Class rdf:about="http://JP_ontology.org/assessment/MCQ.5.3">
        <rdfs:subClassOf rdf:resource="http://JP_ontology.org/assessment/AssessmentQuestion"/>
    </owl:Class>
    


    <!-- http://JP_ontology.org/assessment/MCQ.5.4 -->


    <owl:Class rdf:about="http://JP_ontology.org/assessment/MCQ.5.4">
        <rdfs:subClassOf rdf:resource="http://JP_ontology.org/assessment/AssessmentQuestion"/>
    </owl:Class>
    


    <!-- http://JP_ontology.org/assessment/MCQ.5.5 -->


    <owl:Class rdf:about="http://JP_ontology.org/assessment/MCQ.5.5">
        <rdfs:subClassOf rdf:resource="http://JP_ontology.org/assessment/AssessmentQuestion"/>
    </owl:Class>
    


    <!-- http://JP_ontology.org/assessment/MCQ.5.6 -->


    <owl:Class rdf:about="http://JP_ontology.org/assessment/MCQ.5.6">
        <rdfs:subClassOf rdf:resource="http://JP_ontology.org/assessment/AssessmentQuestion"/>
    </owl:Class>
    


    <!-- http://JP_ontology.org/assessment/MCQ.50 -->


    <owl:Class rdf:about="http://JP_ontology.org/assessment/MCQ.50">
        <rdfs:subClassOf rdf:resource="http://JP_ontology.org/assessment/AssessmentQuestion"/>
    </owl:Class>
    


    <!-- http://JP_ontology.org/assessment/MCQ.51 -->


    <owl:Class rdf:about="http://JP_ontology.org/assessment/MCQ.51">
        <rdfs:subClassOf rdf:resource="http://JP_ontology.org/assessment/AssessmentQuestion"/>
    </owl:Class>
    


    <!-- http://JP_ontology.org/assessment/MCQ.52 -->


    <owl:Class rdf:about="http://JP_ontology.org/assessment/MCQ.52">
        <rdfs:subClassOf rdf:resource="http://JP_ontology.org/assessment/AssessmentQuestion"/>
    </owl:Class>
    


    <!-- http://JP_ontology.org/assessment/MCQ.53 -->


    <owl:Class rdf:about="http://JP_ontology.org/assessment/MCQ.53">
        <rdfs:subClassOf rdf:resource="http://JP_ontology.org/assessment/AssessmentQuestion"/>
    </owl:Class>
    


    <!-- http://JP_ontology.org/assessment/MCQ.54.1 -->


    <owl:Class rdf:about="http://JP_ontology.org/assessment/MCQ.54.1">
        <rdfs:subClassOf rdf:resource="http://JP_ontology.org/assessment/AssessmentQuestion"/>
    </owl:Class>
    


    <!-- http://JP_ontology.org/assessment/MCQ.54.2 -->


    <owl:Class rdf:about="http://JP_ontology.org/assessment/MCQ.54.2">
        <rdfs:subClassOf rdf:resource="http://JP_ontology.org/assessment/AssessmentQuestion"/>
    </owl:Class>
    


    <!-- http://JP_ontology.org/assessment/MCQ.54.3 -->


    <owl:Class rdf:about="http://JP_ontology.org/assessment/MCQ.54.3">
        <rdfs:subClassOf rdf:resource="http://JP_ontology.org/assessment/AssessmentQuestion"/>
    </owl:Class>
    


    <!-- http://JP_ontology.org/assessment/MCQ.54.4 -->


    <owl:Class rdf:about="http://JP_ontology.org/assessment/MCQ.54.4">
        <rdfs:subClassOf rdf:resource="http://JP_ontology.org/assessment/AssessmentQuestion"/>
    </owl:Class>
    


    <!-- http://JP_ontology.org/assessment/MCQ.55.1 -->


    <owl:Class rdf:about="http://JP_ontology.org/assessment/MCQ.55.1">
        <rdfs:subClassOf rdf:resource="http://JP_ontology.org/assessment/AssessmentQuestion"/>
    </owl:Class>
    


    <!-- http://JP_ontology.org/assessment/MCQ.55.2 -->


    <owl:Class rdf:about="http://JP_ontology.org/assessment/MCQ.55.2">
        <rdfs:subClassOf rdf:resource="http://JP_ontology.org/assessment/AssessmentQuestion"/>
    </owl:Class>
    


    <!-- http://JP_ontology.org/assessment/MCQ.55.3 -->


    <owl:Class rdf:about="http://JP_ontology.org/assessment/MCQ.55.3">
        <rdfs:subClassOf rdf:resource="http://JP_ontology.org/assessment/AssessmentQuestion"/>
    </owl:Class>
    


    <!-- http://JP_ontology.org/assessment/MCQ.56.1 -->


    <owl:Class rdf:about="http://JP_ontology.org/assessment/MCQ.56.1">
        <rdfs:subClassOf rdf:resource="http://JP_ontology.org/assessment/AssessmentQuestion"/>
    </owl:Class>
    


    <!-- http://JP_ontology.org/assessment/MCQ.56.2 -->


    <owl:Class rdf:about="http://JP_ontology.org/assessment/MCQ.56.2">
        <rdfs:subClassOf rdf:resource="http://JP_ontology.org/assessment/AssessmentQuestion"/>
    </owl:Class>
    


    <!-- http://JP_ontology.org/assessment/MCQ.56.3 -->


    <owl:Class rdf:about="http://JP_ontology.org/assessment/MCQ.56.3">
        <rdfs:subClassOf rdf:resource="http://JP_ontology.org/assessment/AssessmentQuestion"/>
    </owl:Class>
    


    <!-- http://JP_ontology.org/assessment/MCQ.56.4 -->


    <owl:Class rdf:about="http://JP_ontology.org/assessment/MCQ.56.4">
        <rdfs:subClassOf rdf:resource="http://JP_ontology.org/assessment/AssessmentQuestion"/>
    </owl:Class>
    


    <!-- http://JP_ontology.org/assessment/MCQ.57.1 -->


    <owl:Class rdf:about="http://JP_ontology.org/assessment/MCQ.57.1">
        <rdfs:subClassOf rdf:resource="http://JP_ontology.org/assessment/AssessmentQuestion"/>
    </owl:Class>
    


    <!-- http://JP_ontology.org/assessment/MCQ.57.2 -->


    <owl:Class rdf:about="http://JP_ontology.org/assessment/MCQ.57.2">
        <rdfs:subClassOf rdf:resource="http://JP_ontology.org/assessment/AssessmentQuestion"/>
    </owl:Class>
    


    <!-- http://JP_ontology.org/assessment/MCQ.58 -->


    <owl:Class rdf:about="http://JP_ontology.org/assessment/MCQ.58">
        <rdfs:subClassOf rdf:resource="http://JP_ontology.org/assessment/AssessmentQuestion"/>
    </owl:Class>
    


    <!-- http://JP_ontology.org/assessment/MCQ.59 -->


    <owl:Class rdf:about="http://JP_ontology.org/assessment/MCQ.59">
        <rdfs:subClassOf rdf:resource="http://JP_ontology.org/assessment/AssessmentQuestion"/>
    </owl:Class>
    


    <!-- http://JP_ontology.org/assessment/MCQ.6.1 -->


    <owl:Class rdf:about="http://JP_ontology.org/assessment/MCQ.6.1">
        <rdfs:subClassOf rdf:resource="http://JP_ontology.org/assessment/AssessmentQuestion"/>
    </owl:Class>
    


    <!-- http://JP_ontology.org/assessment/MCQ.6.2 -->


    <owl:Class rdf:about="http://JP_ontology.org/assessment/MCQ.6.2">
        <rdfs:subClassOf rdf:resource="http://JP_ontology.org/assessment/AssessmentQuestion"/>
    </owl:Class>
    


    <!-- http://JP_ontology.org/assessment/MCQ.6.3 -->


    <owl:Class rdf:about="http://JP_ontology.org/assessment/MCQ.6.3">
        <rdfs:subClassOf rdf:resource="http://JP_ontology.org/assessment/AssessmentQuestion"/>
    </owl:Class>
    


    <!-- http://JP_ontology.org/assessment/MCQ.6.4 -->


    <owl:Class rdf:about="http://JP_ontology.org/assessment/MCQ.6.4">
        <rdfs:subClassOf rdf:resource="http://JP_ontology.org/assessment/AssessmentQuestion"/>
    </owl:Class>
    


    <!-- http://JP_ontology.org/assessment/MCQ.60 -->


    <owl:Class rdf:about="http://JP_ontology.org/assessment/MCQ.60">
        <rdfs:subClassOf rdf:resource="http://JP_ontology.org/assessment/AssessmentQuestion"/>
    </owl:Class>
    


    <!-- http://JP_ontology.org/assessment/MCQ.61 -->


    <owl:Class rdf:about="http://JP_ontology.org/assessment/MCQ.61">
        <rdfs:subClassOf rdf:resource="http://JP_ontology.org/assessment/AssessmentQuestion"/>
    </owl:Class>
    


    <!-- http://JP_ontology.org/assessment/MCQ.62 -->


    <owl:Class rdf:about="http://JP_ontology.org/assessment/MCQ.62">
        <rdfs:subClassOf rdf:resource="http://JP_ontology.org/assessment/AssessmentQuestion"/>
    </owl:Class>
    


    <!-- http://JP_ontology.org/assessment/MCQ.63 -->


    <owl:Class rdf:about="http://JP_ontology.org/assessment/MCQ.63">
        <rdfs:subClassOf rdf:resource="http://JP_ontology.org/assessment/AssessmentQuestion"/>
    </owl:Class>
    


    <!-- http://JP_ontology.org/assessment/MCQ.64 -->


    <owl:Class rdf:about="http://JP_ontology.org/assessment/MCQ.64">
        <rdfs:subClassOf rdf:resource="http://JP_ontology.org/assessment/AssessmentQuestion"/>
    </owl:Class>
    


    <!-- http://JP_ontology.org/assessment/MCQ.65 -->


    <owl:Class rdf:about="http://JP_ontology.org/assessment/MCQ.65">
        <rdfs:subClassOf rdf:resource="http://JP_ontology.org/assessment/AssessmentQuestion"/>
    </owl:Class>
    


    <!-- http://JP_ontology.org/assessment/MCQ.66 -->


    <owl:Class rdf:about="http://JP_ontology.org/assessment/MCQ.66">
        <rdfs:subClassOf rdf:resource="http://JP_ontology.org/assessment/AssessmentQuestion"/>
    </owl:Class>
    


    <!-- http://JP_ontology.org/assessment/MCQ.67 -->


    <owl:Class rdf:about="http://JP_ontology.org/assessment/MCQ.67">
        <rdfs:subClassOf rdf:resource="http://JP_ontology.org/assessment/AssessmentQuestion"/>
    </owl:Class>
    


    <!-- http://JP_ontology.org/assessment/MCQ.68 -->


    <owl:Class rdf:about="http://JP_ontology.org/assessment/MCQ.68">
        <rdfs:subClassOf rdf:resource="http://JP_ontology.org/assessment/AssessmentQuestion"/>
    </owl:Class>
    


    <!-- http://JP_ontology.org/assessment/MCQ.69 -->


    <owl:Class rdf:about="http://JP_ontology.org/assessment/MCQ.69">
        <rdfs:subClassOf rdf:resource="http://JP_ontology.org/assessment/AssessmentQuestion"/>
    </owl:Class>
    


    <!-- http://JP_ontology.org/assessment/MCQ.7 -->


    <owl:Class rdf:about="http://JP_ontology.org/assessment/MCQ.7">
        <rdfs:subClassOf rdf:resource="http://JP_ontology.org/assessment/AssessmentQuestion"/>
    </owl:Class>
    


    <!-- http://JP_ontology.org/assessment/MCQ.70.1 -->


    <owl:Class rdf:about="http://JP_ontology.org/assessment/MCQ.70.1">
        <rdfs:subClassOf rdf:resource="http://JP_ontology.org/assessment/AssessmentQuestion"/>
    </owl:Class>
    


    <!-- http://JP_ontology.org/assessment/MCQ.70.2 -->


    <owl:Class rdf:about="http://JP_ontology.org/assessment/MCQ.70.2">
        <rdfs:subClassOf rdf:resource="http://JP_ontology.org/assessment/AssessmentQuestion"/>
    </owl:Class>
    


    <!-- http://JP_ontology.org/assessment/MCQ.70.3 -->


    <owl:Class rdf:about="http://JP_ontology.org/assessment/MCQ.70.3">
        <rdfs:subClassOf rdf:resource="http://JP_ontology.org/assessment/AssessmentQuestion"/>
    </owl:Class>
    


    <!-- http://JP_ontology.org/assessment/MCQ.70.4 -->


    <owl:Class rdf:about="http://JP_ontology.org/assessment/MCQ.70.4">
        <rdfs:subClassOf rdf:resource="http://JP_ontology.org/assessment/AssessmentQuestion"/>
    </owl:Class>
    


    <!-- http://JP_ontology.org/assessment/MCQ.71 -->


    <owl:Class rdf:about="http://JP_ontology.org/assessment/MCQ.71">
        <rdfs:subClassOf rdf:resource="http://JP_ontology.org/assessment/AssessmentQuestion"/>
    </owl:Class>
    


    <!-- http://JP_ontology.org/assessment/MCQ.72 -->


    <owl:Class rdf:about="http://JP_ontology.org/assessment/MCQ.72">
        <rdfs:subClassOf rdf:resource="http://JP_ontology.org/assessment/AssessmentQuestion"/>
    </owl:Class>
    


    <!-- http://JP_ontology.org/assessment/MCQ.73 -->


    <owl:Class rdf:about="http://JP_ontology.org/assessment/MCQ.73">
        <rdfs:subClassOf rdf:resource="http://JP_ontology.org/assessment/AssessmentQuestion"/>
    </owl:Class>
    


    <!-- http://JP_ontology.org/assessment/MCQ.74 -->


    <owl:Class rdf:about="http://JP_ontology.org/assessment/MCQ.74">
        <rdfs:subClassOf rdf:resource="http://JP_ontology.org/assessment/AssessmentQuestion"/>
    </owl:Class>
    


    <!-- http://JP_ontology.org/assessment/MCQ.75.1 -->


    <owl:Class rdf:about="http://JP_ontology.org/assessment/MCQ.75.1">
        <rdfs:subClassOf rdf:resource="http://JP_ontology.org/assessment/AssessmentQuestion"/>
    </owl:Class>
    


    <!-- http://JP_ontology.org/assessment/MCQ.75.2 -->


    <owl:Class rdf:about="http://JP_ontology.org/assessment/MCQ.75.2">
        <rdfs:subClassOf rdf:resource="http://JP_ontology.org/assessment/AssessmentQuestion"/>
    </owl:Class>
    


    <!-- http://JP_ontology.org/assessment/MCQ.76 -->


    <owl:Class rdf:about="http://JP_ontology.org/assessment/MCQ.76">
        <rdfs:subClassOf rdf:resource="http://JP_ontology.org/assessment/AssessmentQuestion"/>
    </owl:Class>
    


    <!-- http://JP_ontology.org/assessment/MCQ.77 -->


    <owl:Class rdf:about="http://JP_ontology.org/assessment/MCQ.77">
        <rdfs:subClassOf rdf:resource="http://JP_ontology.org/assessment/AssessmentQuestion"/>
    </owl:Class>
    


    <!-- http://JP_ontology.org/assessment/MCQ.78 -->


    <owl:Class rdf:about="http://JP_ontology.org/assessment/MCQ.78">
        <rdfs:subClassOf rdf:resource="http://JP_ontology.org/assessment/AssessmentQuestion"/>
    </owl:Class>
    


    <!-- http://JP_ontology.org/assessment/MCQ.79 -->


    <owl:Class rdf:about="http://JP_ontology.org/assessment/MCQ.79">
        <rdfs:subClassOf rdf:resource="http://JP_ontology.org/assessment/AssessmentQuestion"/>
    </owl:Class>
    


    <!-- http://JP_ontology.org/assessment/MCQ.8.1 -->


    <owl:Class rdf:about="http://JP_ontology.org/assessment/MCQ.8.1">
        <rdfs:subClassOf rdf:resource="http://JP_ontology.org/assessment/AssessmentQuestion"/>
    </owl:Class>
    


    <!-- http://JP_ontology.org/assessment/MCQ.8.2 -->


    <owl:Class rdf:about="http://JP_ontology.org/assessment/MCQ.8.2">
        <rdfs:subClassOf rdf:resource="http://JP_ontology.org/assessment/AssessmentQuestion"/>
    </owl:Class>
    


    <!-- http://JP_ontology.org/assessment/MCQ.80 -->


    <owl:Class rdf:about="http://JP_ontology.org/assessment/MCQ.80">
        <rdfs:subClassOf rdf:resource="http://JP_ontology.org/assessment/AssessmentQuestion"/>
    </owl:Class>
    


    <!-- http://JP_ontology.org/assessment/MCQ.81 -->


    <owl:Class rdf:about="http://JP_ontology.org/assessment/MCQ.81">
        <rdfs:subClassOf rdf:resource="http://JP_ontology.org/assessment/AssessmentQuestion"/>
    </owl:Class>
    


    <!-- http://JP_ontology.org/assessment/MCQ.82 -->


    <owl:Class rdf:about="http://JP_ontology.org/assessment/MCQ.82">
        <rdfs:subClassOf rdf:resource="http://JP_ontology.org/assessment/AssessmentQuestion"/>
    </owl:Class>
    


    <!-- http://JP_ontology.org/assessment/MCQ.83 -->


    <owl:Class rdf:about="http://JP_ontology.org/assessment/MCQ.83">
        <rdfs:subClassOf rdf:resource="http://JP_ontology.org/assessment/AssessmentQuestion"/>
    </owl:Class>
    


    <!-- http://JP_ontology.org/assessment/MCQ.84 -->


    <owl:Class rdf:about="http://JP_ontology.org/assessment/MCQ.84">
        <rdfs:subClassOf rdf:resource="http://JP_ontology.org/assessment/AssessmentQuestion"/>
    </owl:Class>
    


    <!-- http://JP_ontology.org/assessment/MCQ.85 -->


    <owl:Class rdf:about="http://JP_ontology.org/assessment/MCQ.85">
        <rdfs:subClassOf rdf:resource="http://JP_ontology.org/assessment/AssessmentQuestion"/>
    </owl:Class>
    


    <!-- http://JP_ontology.org/assessment/MCQ.86 -->


    <owl:Class rdf:about="http://JP_ontology.org/assessment/MCQ.86">
        <rdfs:subClassOf rdf:resource="http://JP_ontology.org/assessment/AssessmentQuestion"/>
    </owl:Class>
    


    <!-- http://JP_ontology.org/assessment/MCQ.87 -->


    <owl:Class rdf:about="http://JP_ontology.org/assessment/MCQ.87">
        <rdfs:subClassOf rdf:resource="http://JP_ontology.org/assessment/AssessmentQuestion"/>
    </owl:Class>
    


    <!-- http://JP_ontology.org/assessment/MCQ.88 -->


    <owl:Class rdf:about="http://JP_ontology.org/assessment/MCQ.88">
        <rdfs:subClassOf rdf:resource="http://JP_ontology.org/assessment/AssessmentQuestion"/>
    </owl:Class>
    


    <!-- http://JP_ontology.org/assessment/MCQ.89 -->


    <owl:Class rdf:about="http://JP_ontology.org/assessment/MCQ.89">
        <rdfs:subClassOf rdf:resource="http://JP_ontology.org/assessment/AssessmentQuestion"/>
    </owl:Class>
    


    <!-- http://JP_ontology.org/assessment/MCQ.9.1 -->


    <owl:Class rdf:about="http://JP_ontology.org/assessment/MCQ.9.1">
        <rdfs:subClassOf rdf:resource="http://JP_ontology.org/assessment/AssessmentQuestion"/>
    </owl:Class>
    


    <!-- http://JP_ontology.org/assessment/MCQ.9.2 -->


    <owl:Class rdf:about="http://JP_ontology.org/assessment/MCQ.9.2">
        <rdfs:subClassOf rdf:resource="http://JP_ontology.org/assessment/AssessmentQuestion"/>
    </owl:Class>
    


    <!-- http://JP_ontology.org/assessment/MCQ.90 -->


    <owl:Class rdf:about="http://JP_ontology.org/assessment/MCQ.90">
        <rdfs:subClassOf rdf:resource="http://JP_ontology.org/assessment/AssessmentQuestion"/>
    </owl:Class>
    


    <!-- http://JP_ontology.org/assessment/MCQ.91.1 -->


    <owl:Class rdf:about="http://JP_ontology.org/assessment/MCQ.91.1">
        <rdfs:subClassOf rdf:resource="http://JP_ontology.org/assessment/AssessmentQuestion"/>
    </owl:Class>
    


    <!-- http://JP_ontology.org/assessment/MCQ.91.2 -->


    <owl:Class rdf:about="http://JP_ontology.org/assessment/MCQ.91.2">
        <rdfs:subClassOf rdf:resource="http://JP_ontology.org/assessment/AssessmentQuestion"/>
    </owl:Class>
    


    <!-- http://JP_ontology.org/assessment/MCQ.92 -->


    <owl:Class rdf:about="http://JP_ontology.org/assessment/MCQ.92">
        <rdfs:subClassOf rdf:resource="http://JP_ontology.org/assessment/AssessmentQuestion"/>
    </owl:Class>
    


    <!-- http://JP_ontology.org/assessment/MCQ.93 -->


    <owl:Class rdf:about="http://JP_ontology.org/assessment/MCQ.93">
        <rdfs:subClassOf rdf:resource="http://JP_ontology.org/assessment/AssessmentQuestion"/>
    </owl:Class>
    


    <!-- http://JP_ontology.org/assessment/MCQ.94 -->


    <owl:Class rdf:about="http://JP_ontology.org/assessment/MCQ.94">
        <rdfs:subClassOf rdf:resource="http://JP_ontology.org/assessment/AssessmentQuestion"/>
    </owl:Class>
    


    <!-- http://JP_ontology.org/assessment/MCQ.95 -->


    <owl:Class rdf:about="http://JP_ontology.org/assessment/MCQ.95">
        <rdfs:subClassOf rdf:resource="http://JP_ontology.org/assessment/AssessmentQuestion"/>
    </owl:Class>
    


    <!-- http://JP_ontology.org/assessment/MCQ.96 -->


    <owl:Class rdf:about="http://JP_ontology.org/assessment/MCQ.96">
        <rdfs:subClassOf rdf:resource="http://JP_ontology.org/assessment/AssessmentQuestion"/>
    </owl:Class>
    


    <!-- http://JP_ontology.org/assessment/MCQ.97 -->


    <owl:Class rdf:about="http://JP_ontology.org/assessment/MCQ.97">
        <rdfs:subClassOf rdf:resource="http://JP_ontology.org/assessment/AssessmentQuestion"/>
    </owl:Class>
    


    <!-- http://JP_ontology.org/assessment/MCQ.98 -->


    <owl:Class rdf:about="http://JP_ontology.org/assessment/MCQ.98">
        <rdfs:subClassOf rdf:resource="http://JP_ontology.org/assessment/AssessmentQuestion"/>
    </owl:Class>
    


    <!-- http://JP_ontology.org/assessment/MCQ.99 -->


    <owl:Class rdf:about="http://JP_ontology.org/assessment/MCQ.99">
        <rdfs:subClassOf rdf:resource="http://JP_ontology.org/assessment/AssessmentQuestion"/>
    </owl:Class>
    


    <!-- http://JP_ontology.org/iso27001/ISOControl270012022 -->


    <owl:Class rdf:about="http://JP_ontology.org/iso27001/ISOControl270012022"/>
    


    <!-- http://www.w3.org/2004/02/skos/core#Concept -->


    <owl:Class rdf:about="http://www.w3.org/2004/02/skos/core#Concept"/>
    


    <!-- 
    ///////////////////////////////////////////////////////////////////////////////////////
    //
    // Individuals
    //
    ///////////////////////////////////////////////////////////////////////////////////////
     -->


    


    <!-- http://JP_ontology.org/assessment/MCQ.1 -->


    <owl:NamedIndividual rdf:about="http://JP_ontology.org/assessment/MCQ.1">
        <rdf:type rdf:resource="http://www.w3.org/2004/02/skos/core#Concept"/>
    </owl:NamedIndividual>
    


    <!-- http://JP_ontology.org/assessment/MCQ.10.1 -->


    <owl:NamedIndividual rdf:about="http://JP_ontology.org/assessment/MCQ.10.1">
        <rdf:type rdf:resource="http://www.w3.org/2004/02/skos/core#Concept"/>
    </owl:NamedIndividual>
    


    <!-- http://JP_ontology.org/assessment/MCQ.10.1AnswerA -->


    <owl:NamedIndividual rdf:about="http://JP_ontology.org/assessment/MCQ.10.1AnswerA">
        <rdf:type rdf:resource="http://JP_ontology.org/assessment/MCQ.10.1"/>
        <skos:altLabel xml:lang="en">(i)</skos:altLabel>
        <skos:definition xml:lang="en">The information security policy and topic-specific policies are not defined, approved by management, published, communicated to, or acknowledged by relevant personnel and interested parties, potentially leading to confusion and lack of awareness regarding security requirements.</skos:definition>
        <skos:prefLabel xml:lang="en">MCQ.10.1 - Not Implemented</skos:prefLabel>
    </owl:NamedIndividual>
    


    <!-- http://JP_ontology.org/assessment/MCQ.10.1AnswerB -->


    <owl:NamedIndividual rdf:about="http://JP_ontology.org/assessment/MCQ.10.1AnswerB">
        <rdf:type rdf:resource="http://JP_ontology.org/assessment/MCQ.10.1"/>
        <skos:altLabel xml:lang="en">(ii)</skos:altLabel>
        <skos:definition xml:lang="en">There are some efforts to define, approve, publish, communicate, and acknowledge the information security policy and topic-specific policies. However, these efforts may be inconsistent or not fully comprehensive across all relevant parties.</skos:definition>
        <skos:prefLabel xml:lang="en">MCQ.10.1 - Partially Implemented</skos:prefLabel>
    </owl:NamedIndividual>
    


    <!-- http://JP_ontology.org/assessment/MCQ.10.1AnswerC -->


    <owl:NamedIndividual rdf:about="http://JP_ontology.org/assessment/MCQ.10.1AnswerC">
        <rdf:type rdf:resource="http://JP_ontology.org/assessment/MCQ.10.1"/>
        <skos:altLabel xml:lang="en">(iii)</skos:altLabel>
        <skos:definition xml:lang="en">The information security policy and topic-specific policies are fully defined, approved by management, published, communicated to, and acknowledged by relevant personnel and interested parties, ensuring widespread awareness and compliance with security requirements.</skos:definition>
        <skos:prefLabel xml:lang="en">MCQ.10.1 - Fully Implemented</skos:prefLabel>
    </owl:NamedIndividual>
    


    <!-- http://JP_ontology.org/assessment/MCQ.10.2 -->


    <owl:NamedIndividual rdf:about="http://JP_ontology.org/assessment/MCQ.10.2">
        <rdf:type rdf:resource="http://www.w3.org/2004/02/skos/core#Concept"/>
    </owl:NamedIndividual>
    


    <!-- http://JP_ontology.org/assessment/MCQ.100 -->


    <owl:NamedIndividual rdf:about="http://JP_ontology.org/assessment/MCQ.100">
        <rdf:type rdf:resource="http://www.w3.org/2004/02/skos/core#Concept"/>
    </owl:NamedIndividual>
    


    <!-- http://JP_ontology.org/assessment/MCQ.101 -->


    <owl:NamedIndividual rdf:about="http://JP_ontology.org/assessment/MCQ.101">
        <rdf:type rdf:resource="http://www.w3.org/2004/02/skos/core#Concept"/>
    </owl:NamedIndividual>
    


    <!-- http://JP_ontology.org/assessment/MCQ.102 -->


    <owl:NamedIndividual rdf:about="http://JP_ontology.org/assessment/MCQ.102">
        <rdf:type rdf:resource="http://www.w3.org/2004/02/skos/core#Concept"/>
    </owl:NamedIndividual>
    


    <!-- http://JP_ontology.org/assessment/MCQ.103 -->


    <owl:NamedIndividual rdf:about="http://JP_ontology.org/assessment/MCQ.103">
        <rdf:type rdf:resource="http://www.w3.org/2004/02/skos/core#Concept"/>
    </owl:NamedIndividual>
    


    <!-- http://JP_ontology.org/assessment/MCQ.104 -->


    <owl:NamedIndividual rdf:about="http://JP_ontology.org/assessment/MCQ.104">
        <rdf:type rdf:resource="http://www.w3.org/2004/02/skos/core#Concept"/>
    </owl:NamedIndividual>
    


    <!-- http://JP_ontology.org/assessment/MCQ.105.1 -->


    <owl:NamedIndividual rdf:about="http://JP_ontology.org/assessment/MCQ.105.1">
        <rdf:type rdf:resource="http://www.w3.org/2004/02/skos/core#Concept"/>
    </owl:NamedIndividual>
    


    <!-- http://JP_ontology.org/assessment/MCQ.105.2 -->


    <owl:NamedIndividual rdf:about="http://JP_ontology.org/assessment/MCQ.105.2">
        <rdf:type rdf:resource="http://www.w3.org/2004/02/skos/core#Concept"/>
    </owl:NamedIndividual>
    


    <!-- http://JP_ontology.org/assessment/MCQ.105.3 -->


    <owl:NamedIndividual rdf:about="http://JP_ontology.org/assessment/MCQ.105.3">
        <rdf:type rdf:resource="http://www.w3.org/2004/02/skos/core#Concept"/>
    </owl:NamedIndividual>
    


    <!-- http://JP_ontology.org/assessment/MCQ.106.1 -->


    <owl:NamedIndividual rdf:about="http://JP_ontology.org/assessment/MCQ.106.1">
        <rdf:type rdf:resource="http://www.w3.org/2004/02/skos/core#Concept"/>
    </owl:NamedIndividual>
    


    <!-- http://JP_ontology.org/assessment/MCQ.106.2 -->


    <owl:NamedIndividual rdf:about="http://JP_ontology.org/assessment/MCQ.106.2">
        <rdf:type rdf:resource="http://www.w3.org/2004/02/skos/core#Concept"/>
    </owl:NamedIndividual>
    


    <!-- http://JP_ontology.org/assessment/MCQ.107.1 -->


    <owl:NamedIndividual rdf:about="http://JP_ontology.org/assessment/MCQ.107.1">
        <rdf:type rdf:resource="http://www.w3.org/2004/02/skos/core#Concept"/>
    </owl:NamedIndividual>
    


    <!-- http://JP_ontology.org/assessment/MCQ.107.2 -->


    <owl:NamedIndividual rdf:about="http://JP_ontology.org/assessment/MCQ.107.2">
        <rdf:type rdf:resource="http://www.w3.org/2004/02/skos/core#Concept"/>
    </owl:NamedIndividual>
    


    <!-- http://JP_ontology.org/assessment/MCQ.108 -->


    <owl:NamedIndividual rdf:about="http://JP_ontology.org/assessment/MCQ.108">
        <rdf:type rdf:resource="http://www.w3.org/2004/02/skos/core#Concept"/>
    </owl:NamedIndividual>
    


    <!-- http://JP_ontology.org/assessment/MCQ.109 -->


    <owl:NamedIndividual rdf:about="http://JP_ontology.org/assessment/MCQ.109">
        <rdf:type rdf:resource="http://www.w3.org/2004/02/skos/core#Concept"/>
    </owl:NamedIndividual>
    


    <!-- http://JP_ontology.org/assessment/MCQ.11 -->


    <owl:NamedIndividual rdf:about="http://JP_ontology.org/assessment/MCQ.11">
        <rdf:type rdf:resource="http://www.w3.org/2004/02/skos/core#Concept"/>
    </owl:NamedIndividual>
    


    <!-- http://JP_ontology.org/assessment/MCQ.110 -->


    <owl:NamedIndividual rdf:about="http://JP_ontology.org/assessment/MCQ.110">
        <rdf:type rdf:resource="http://www.w3.org/2004/02/skos/core#Concept"/>
    </owl:NamedIndividual>
    


    <!-- http://JP_ontology.org/assessment/MCQ.111 -->


    <owl:NamedIndividual rdf:about="http://JP_ontology.org/assessment/MCQ.111">
        <rdf:type rdf:resource="http://www.w3.org/2004/02/skos/core#Concept"/>
    </owl:NamedIndividual>
    


    <!-- http://JP_ontology.org/assessment/MCQ.112.1 -->


    <owl:NamedIndividual rdf:about="http://JP_ontology.org/assessment/MCQ.112.1">
        <rdf:type rdf:resource="http://www.w3.org/2004/02/skos/core#Concept"/>
    </owl:NamedIndividual>
    


    <!-- http://JP_ontology.org/assessment/MCQ.112.2 -->


    <owl:NamedIndividual rdf:about="http://JP_ontology.org/assessment/MCQ.112.2">
        <rdf:type rdf:resource="http://www.w3.org/2004/02/skos/core#Concept"/>
    </owl:NamedIndividual>
    


    <!-- http://JP_ontology.org/assessment/MCQ.113 -->


    <owl:NamedIndividual rdf:about="http://JP_ontology.org/assessment/MCQ.113">
        <rdf:type rdf:resource="http://www.w3.org/2004/02/skos/core#Concept"/>
    </owl:NamedIndividual>
    


    <!-- http://JP_ontology.org/assessment/MCQ.114 -->


    <owl:NamedIndividual rdf:about="http://JP_ontology.org/assessment/MCQ.114">
        <rdf:type rdf:resource="http://www.w3.org/2004/02/skos/core#Concept"/>
    </owl:NamedIndividual>
    


    <!-- http://JP_ontology.org/assessment/MCQ.115 -->


    <owl:NamedIndividual rdf:about="http://JP_ontology.org/assessment/MCQ.115">
        <rdf:type rdf:resource="http://www.w3.org/2004/02/skos/core#Concept"/>
    </owl:NamedIndividual>
    


    <!-- http://JP_ontology.org/assessment/MCQ.116 -->


    <owl:NamedIndividual rdf:about="http://JP_ontology.org/assessment/MCQ.116">
        <rdf:type rdf:resource="http://www.w3.org/2004/02/skos/core#Concept"/>
    </owl:NamedIndividual>
    


    <!-- http://JP_ontology.org/assessment/MCQ.117 -->


    <owl:NamedIndividual rdf:about="http://JP_ontology.org/assessment/MCQ.117">
        <rdf:type rdf:resource="http://www.w3.org/2004/02/skos/core#Concept"/>
    </owl:NamedIndividual>
    


    <!-- http://JP_ontology.org/assessment/MCQ.118 -->


    <owl:NamedIndividual rdf:about="http://JP_ontology.org/assessment/MCQ.118">
        <rdf:type rdf:resource="http://www.w3.org/2004/02/skos/core#Concept"/>
    </owl:NamedIndividual>
    


    <!-- http://JP_ontology.org/assessment/MCQ.119 -->


    <owl:NamedIndividual rdf:about="http://JP_ontology.org/assessment/MCQ.119">
        <rdf:type rdf:resource="http://www.w3.org/2004/02/skos/core#Concept"/>
    </owl:NamedIndividual>
    


    <!-- http://JP_ontology.org/assessment/MCQ.12 -->


    <owl:NamedIndividual rdf:about="http://JP_ontology.org/assessment/MCQ.12">
        <rdf:type rdf:resource="http://www.w3.org/2004/02/skos/core#Concept"/>
    </owl:NamedIndividual>
    


    <!-- http://JP_ontology.org/assessment/MCQ.120 -->


    <owl:NamedIndividual rdf:about="http://JP_ontology.org/assessment/MCQ.120">
        <rdf:type rdf:resource="http://www.w3.org/2004/02/skos/core#Concept"/>
    </owl:NamedIndividual>
    


    <!-- http://JP_ontology.org/assessment/MCQ.121 -->


    <owl:NamedIndividual rdf:about="http://JP_ontology.org/assessment/MCQ.121">
        <rdf:type rdf:resource="http://www.w3.org/2004/02/skos/core#Concept"/>
    </owl:NamedIndividual>
    


    <!-- http://JP_ontology.org/assessment/MCQ.122 -->


    <owl:NamedIndividual rdf:about="http://JP_ontology.org/assessment/MCQ.122">
        <rdf:type rdf:resource="http://www.w3.org/2004/02/skos/core#Concept"/>
    </owl:NamedIndividual>
    


    <!-- http://JP_ontology.org/assessment/MCQ.123 -->


    <owl:NamedIndividual rdf:about="http://JP_ontology.org/assessment/MCQ.123">
        <rdf:type rdf:resource="http://www.w3.org/2004/02/skos/core#Concept"/>
    </owl:NamedIndividual>
    


    <!-- http://JP_ontology.org/assessment/MCQ.124 -->


    <owl:NamedIndividual rdf:about="http://JP_ontology.org/assessment/MCQ.124">
        <rdf:type rdf:resource="http://www.w3.org/2004/02/skos/core#Concept"/>
    </owl:NamedIndividual>
    


    <!-- http://JP_ontology.org/assessment/MCQ.125 -->


    <owl:NamedIndividual rdf:about="http://JP_ontology.org/assessment/MCQ.125">
        <rdf:type rdf:resource="http://www.w3.org/2004/02/skos/core#Concept"/>
    </owl:NamedIndividual>
    


    <!-- http://JP_ontology.org/assessment/MCQ.126 -->


    <owl:NamedIndividual rdf:about="http://JP_ontology.org/assessment/MCQ.126">
        <rdf:type rdf:resource="http://www.w3.org/2004/02/skos/core#Concept"/>
    </owl:NamedIndividual>
    


    <!-- http://JP_ontology.org/assessment/MCQ.127 -->


    <owl:NamedIndividual rdf:about="http://JP_ontology.org/assessment/MCQ.127">
        <rdf:type rdf:resource="http://www.w3.org/2004/02/skos/core#Concept"/>
    </owl:NamedIndividual>
    


    <!-- http://JP_ontology.org/assessment/MCQ.128 -->


    <owl:NamedIndividual rdf:about="http://JP_ontology.org/assessment/MCQ.128">
        <rdf:type rdf:resource="http://www.w3.org/2004/02/skos/core#Concept"/>
    </owl:NamedIndividual>
    


    <!-- http://JP_ontology.org/assessment/MCQ.129 -->


    <owl:NamedIndividual rdf:about="http://JP_ontology.org/assessment/MCQ.129">
        <rdf:type rdf:resource="http://www.w3.org/2004/02/skos/core#Concept"/>
    </owl:NamedIndividual>
    


    <!-- http://JP_ontology.org/assessment/MCQ.13 -->


    <owl:NamedIndividual rdf:about="http://JP_ontology.org/assessment/MCQ.13">
        <rdf:type rdf:resource="http://www.w3.org/2004/02/skos/core#Concept"/>
    </owl:NamedIndividual>
    


    <!-- http://JP_ontology.org/assessment/MCQ.130 -->


    <owl:NamedIndividual rdf:about="http://JP_ontology.org/assessment/MCQ.130">
        <rdf:type rdf:resource="http://www.w3.org/2004/02/skos/core#Concept"/>
    </owl:NamedIndividual>
    


    <!-- http://JP_ontology.org/assessment/MCQ.14 -->


    <owl:NamedIndividual rdf:about="http://JP_ontology.org/assessment/MCQ.14">
        <rdf:type rdf:resource="http://www.w3.org/2004/02/skos/core#Concept"/>
    </owl:NamedIndividual>
    


    <!-- http://JP_ontology.org/assessment/MCQ.15 -->


    <owl:NamedIndividual rdf:about="http://JP_ontology.org/assessment/MCQ.15">
        <rdf:type rdf:resource="http://www.w3.org/2004/02/skos/core#Concept"/>
    </owl:NamedIndividual>
    


    <!-- http://JP_ontology.org/assessment/MCQ.16 -->


    <owl:NamedIndividual rdf:about="http://JP_ontology.org/assessment/MCQ.16">
        <rdf:type rdf:resource="http://www.w3.org/2004/02/skos/core#Concept"/>
    </owl:NamedIndividual>
    


    <!-- http://JP_ontology.org/assessment/MCQ.17 -->


    <owl:NamedIndividual rdf:about="http://JP_ontology.org/assessment/MCQ.17">
        <rdf:type rdf:resource="http://www.w3.org/2004/02/skos/core#Concept"/>
    </owl:NamedIndividual>
    


    <!-- http://JP_ontology.org/assessment/MCQ.18 -->


    <owl:NamedIndividual rdf:about="http://JP_ontology.org/assessment/MCQ.18">
        <rdf:type rdf:resource="http://www.w3.org/2004/02/skos/core#Concept"/>
    </owl:NamedIndividual>
    


    <!-- http://JP_ontology.org/assessment/MCQ.19 -->


    <owl:NamedIndividual rdf:about="http://JP_ontology.org/assessment/MCQ.19">
        <rdf:type rdf:resource="http://www.w3.org/2004/02/skos/core#Concept"/>
    </owl:NamedIndividual>
    


    <!-- http://JP_ontology.org/assessment/MCQ.2.1 -->


    <owl:NamedIndividual rdf:about="http://JP_ontology.org/assessment/MCQ.2.1">
        <rdf:type rdf:resource="http://www.w3.org/2004/02/skos/core#Concept"/>
    </owl:NamedIndividual>
    


    <!-- http://JP_ontology.org/assessment/MCQ.2.2 -->


    <owl:NamedIndividual rdf:about="http://JP_ontology.org/assessment/MCQ.2.2">
        <rdf:type rdf:resource="http://www.w3.org/2004/02/skos/core#Concept"/>
    </owl:NamedIndividual>
    


    <!-- http://JP_ontology.org/assessment/MCQ.20 -->


    <owl:NamedIndividual rdf:about="http://JP_ontology.org/assessment/MCQ.20">
        <rdf:type rdf:resource="http://www.w3.org/2004/02/skos/core#Concept"/>
    </owl:NamedIndividual>
    


    <!-- http://JP_ontology.org/assessment/MCQ.21 -->


    <owl:NamedIndividual rdf:about="http://JP_ontology.org/assessment/MCQ.21">
        <rdf:type rdf:resource="http://www.w3.org/2004/02/skos/core#Concept"/>
    </owl:NamedIndividual>
    


    <!-- http://JP_ontology.org/assessment/MCQ.22.1 -->


    <owl:NamedIndividual rdf:about="http://JP_ontology.org/assessment/MCQ.22.1">
        <rdf:type rdf:resource="http://www.w3.org/2004/02/skos/core#Concept"/>
    </owl:NamedIndividual>
    


    <!-- http://JP_ontology.org/assessment/MCQ.22.2 -->


    <owl:NamedIndividual rdf:about="http://JP_ontology.org/assessment/MCQ.22.2">
        <rdf:type rdf:resource="http://www.w3.org/2004/02/skos/core#Concept"/>
    </owl:NamedIndividual>
    


    <!-- http://JP_ontology.org/assessment/MCQ.22.3 -->


    <owl:NamedIndividual rdf:about="http://JP_ontology.org/assessment/MCQ.22.3">
        <rdf:type rdf:resource="http://www.w3.org/2004/02/skos/core#Concept"/>
    </owl:NamedIndividual>
    


    <!-- http://JP_ontology.org/assessment/MCQ.22.4 -->


    <owl:NamedIndividual rdf:about="http://JP_ontology.org/assessment/MCQ.22.4">
        <rdf:type rdf:resource="http://www.w3.org/2004/02/skos/core#Concept"/>
    </owl:NamedIndividual>
    


    <!-- http://JP_ontology.org/assessment/MCQ.22.5 -->


    <owl:NamedIndividual rdf:about="http://JP_ontology.org/assessment/MCQ.22.5">
        <rdf:type rdf:resource="http://www.w3.org/2004/02/skos/core#Concept"/>
    </owl:NamedIndividual>
    


    <!-- http://JP_ontology.org/assessment/MCQ.23 -->


    <owl:NamedIndividual rdf:about="http://JP_ontology.org/assessment/MCQ.23">
        <rdf:type rdf:resource="http://www.w3.org/2004/02/skos/core#Concept"/>
    </owl:NamedIndividual>
    


    <!-- http://JP_ontology.org/assessment/MCQ.24 -->


    <owl:NamedIndividual rdf:about="http://JP_ontology.org/assessment/MCQ.24">
        <rdf:type rdf:resource="http://www.w3.org/2004/02/skos/core#Concept"/>
    </owl:NamedIndividual>
    


    <!-- http://JP_ontology.org/assessment/MCQ.25 -->


    <owl:NamedIndividual rdf:about="http://JP_ontology.org/assessment/MCQ.25">
        <rdf:type rdf:resource="http://www.w3.org/2004/02/skos/core#Concept"/>
    </owl:NamedIndividual>
    


    <!-- http://JP_ontology.org/assessment/MCQ.26 -->


    <owl:NamedIndividual rdf:about="http://JP_ontology.org/assessment/MCQ.26">
        <rdf:type rdf:resource="http://www.w3.org/2004/02/skos/core#Concept"/>
    </owl:NamedIndividual>
    


    <!-- http://JP_ontology.org/assessment/MCQ.27 -->


    <owl:NamedIndividual rdf:about="http://JP_ontology.org/assessment/MCQ.27">
        <rdf:type rdf:resource="http://www.w3.org/2004/02/skos/core#Concept"/>
    </owl:NamedIndividual>
    


    <!-- http://JP_ontology.org/assessment/MCQ.28 -->


    <owl:NamedIndividual rdf:about="http://JP_ontology.org/assessment/MCQ.28">
        <rdf:type rdf:resource="http://www.w3.org/2004/02/skos/core#Concept"/>
    </owl:NamedIndividual>
    


    <!-- http://JP_ontology.org/assessment/MCQ.29 -->


    <owl:NamedIndividual rdf:about="http://JP_ontology.org/assessment/MCQ.29">
        <rdf:type rdf:resource="http://www.w3.org/2004/02/skos/core#Concept"/>
    </owl:NamedIndividual>
    


    <!-- http://JP_ontology.org/assessment/MCQ.3.1 -->


    <owl:NamedIndividual rdf:about="http://JP_ontology.org/assessment/MCQ.3.1">
        <rdf:type rdf:resource="http://www.w3.org/2004/02/skos/core#Concept"/>
    </owl:NamedIndividual>
    


    <!-- http://JP_ontology.org/assessment/MCQ.3.2 -->


    <owl:NamedIndividual rdf:about="http://JP_ontology.org/assessment/MCQ.3.2">
        <rdf:type rdf:resource="http://www.w3.org/2004/02/skos/core#Concept"/>
    </owl:NamedIndividual>
    


    <!-- http://JP_ontology.org/assessment/MCQ.30 -->


    <owl:NamedIndividual rdf:about="http://JP_ontology.org/assessment/MCQ.30">
        <rdf:type rdf:resource="http://www.w3.org/2004/02/skos/core#Concept"/>
    </owl:NamedIndividual>
    


    <!-- http://JP_ontology.org/assessment/MCQ.31 -->


    <owl:NamedIndividual rdf:about="http://JP_ontology.org/assessment/MCQ.31">
        <rdf:type rdf:resource="http://www.w3.org/2004/02/skos/core#Concept"/>
    </owl:NamedIndividual>
    


    <!-- http://JP_ontology.org/assessment/MCQ.32 -->


    <owl:NamedIndividual rdf:about="http://JP_ontology.org/assessment/MCQ.32">
        <rdf:type rdf:resource="http://www.w3.org/2004/02/skos/core#Concept"/>
    </owl:NamedIndividual>
    


    <!-- http://JP_ontology.org/assessment/MCQ.33 -->


    <owl:NamedIndividual rdf:about="http://JP_ontology.org/assessment/MCQ.33">
        <rdf:type rdf:resource="http://www.w3.org/2004/02/skos/core#Concept"/>
    </owl:NamedIndividual>
    


    <!-- http://JP_ontology.org/assessment/MCQ.34.1 -->


    <owl:NamedIndividual rdf:about="http://JP_ontology.org/assessment/MCQ.34.1">
        <rdf:type rdf:resource="http://www.w3.org/2004/02/skos/core#Concept"/>
    </owl:NamedIndividual>
    


    <!-- http://JP_ontology.org/assessment/MCQ.34.2 -->


    <owl:NamedIndividual rdf:about="http://JP_ontology.org/assessment/MCQ.34.2">
        <rdf:type rdf:resource="http://www.w3.org/2004/02/skos/core#Concept"/>
    </owl:NamedIndividual>
    


    <!-- http://JP_ontology.org/assessment/MCQ.34.3 -->


    <owl:NamedIndividual rdf:about="http://JP_ontology.org/assessment/MCQ.34.3">
        <rdf:type rdf:resource="http://www.w3.org/2004/02/skos/core#Concept"/>
    </owl:NamedIndividual>
    


    <!-- http://JP_ontology.org/assessment/MCQ.34.4 -->


    <owl:NamedIndividual rdf:about="http://JP_ontology.org/assessment/MCQ.34.4">
        <rdf:type rdf:resource="http://www.w3.org/2004/02/skos/core#Concept"/>
    </owl:NamedIndividual>
    


    <!-- http://JP_ontology.org/assessment/MCQ.35 -->


    <owl:NamedIndividual rdf:about="http://JP_ontology.org/assessment/MCQ.35">
        <rdf:type rdf:resource="http://www.w3.org/2004/02/skos/core#Concept"/>
    </owl:NamedIndividual>
    


    <!-- http://JP_ontology.org/assessment/MCQ.36 -->


    <owl:NamedIndividual rdf:about="http://JP_ontology.org/assessment/MCQ.36">
        <rdf:type rdf:resource="http://www.w3.org/2004/02/skos/core#Concept"/>
    </owl:NamedIndividual>
    


    <!-- http://JP_ontology.org/assessment/MCQ.37 -->


    <owl:NamedIndividual rdf:about="http://JP_ontology.org/assessment/MCQ.37">
        <rdf:type rdf:resource="http://www.w3.org/2004/02/skos/core#Concept"/>
    </owl:NamedIndividual>
    


    <!-- http://JP_ontology.org/assessment/MCQ.38 -->


    <owl:NamedIndividual rdf:about="http://JP_ontology.org/assessment/MCQ.38">
        <rdf:type rdf:resource="http://www.w3.org/2004/02/skos/core#Concept"/>
    </owl:NamedIndividual>
    


    <!-- http://JP_ontology.org/assessment/MCQ.39 -->


    <owl:NamedIndividual rdf:about="http://JP_ontology.org/assessment/MCQ.39">
        <rdf:type rdf:resource="http://www.w3.org/2004/02/skos/core#Concept"/>
    </owl:NamedIndividual>
    


    <!-- http://JP_ontology.org/assessment/MCQ.4.1 -->


    <owl:NamedIndividual rdf:about="http://JP_ontology.org/assessment/MCQ.4.1">
        <rdf:type rdf:resource="http://www.w3.org/2004/02/skos/core#Concept"/>
    </owl:NamedIndividual>
    


    <!-- http://JP_ontology.org/assessment/MCQ.4.2 -->


    <owl:NamedIndividual rdf:about="http://JP_ontology.org/assessment/MCQ.4.2">
        <rdf:type rdf:resource="http://www.w3.org/2004/02/skos/core#Concept"/>
    </owl:NamedIndividual>
    


    <!-- http://JP_ontology.org/assessment/MCQ.4.3 -->


    <owl:NamedIndividual rdf:about="http://JP_ontology.org/assessment/MCQ.4.3">
        <rdf:type rdf:resource="http://www.w3.org/2004/02/skos/core#Concept"/>
    </owl:NamedIndividual>
    


    <!-- http://JP_ontology.org/assessment/MCQ.4.4 -->


    <owl:NamedIndividual rdf:about="http://JP_ontology.org/assessment/MCQ.4.4">
        <rdf:type rdf:resource="http://www.w3.org/2004/02/skos/core#Concept"/>
    </owl:NamedIndividual>
    


    <!-- http://JP_ontology.org/assessment/MCQ.4.5 -->


    <owl:NamedIndividual rdf:about="http://JP_ontology.org/assessment/MCQ.4.5">
        <rdf:type rdf:resource="http://www.w3.org/2004/02/skos/core#Concept"/>
    </owl:NamedIndividual>
    


    <!-- http://JP_ontology.org/assessment/MCQ.4.6 -->


    <owl:NamedIndividual rdf:about="http://JP_ontology.org/assessment/MCQ.4.6">
        <rdf:type rdf:resource="http://www.w3.org/2004/02/skos/core#Concept"/>
    </owl:NamedIndividual>
    


    <!-- http://JP_ontology.org/assessment/MCQ.40 -->


    <owl:NamedIndividual rdf:about="http://JP_ontology.org/assessment/MCQ.40">
        <rdf:type rdf:resource="http://www.w3.org/2004/02/skos/core#Concept"/>
    </owl:NamedIndividual>
    


    <!-- http://JP_ontology.org/assessment/MCQ.41 -->


    <owl:NamedIndividual rdf:about="http://JP_ontology.org/assessment/MCQ.41">
        <rdf:type rdf:resource="http://www.w3.org/2004/02/skos/core#Concept"/>
    </owl:NamedIndividual>
    


    <!-- http://JP_ontology.org/assessment/MCQ.42 -->


    <owl:NamedIndividual rdf:about="http://JP_ontology.org/assessment/MCQ.42">
        <rdf:type rdf:resource="http://www.w3.org/2004/02/skos/core#Concept"/>
    </owl:NamedIndividual>
    


    <!-- http://JP_ontology.org/assessment/MCQ.43 -->


    <owl:NamedIndividual rdf:about="http://JP_ontology.org/assessment/MCQ.43">
        <rdf:type rdf:resource="http://www.w3.org/2004/02/skos/core#Concept"/>
    </owl:NamedIndividual>
    


    <!-- http://JP_ontology.org/assessment/MCQ.44 -->


    <owl:NamedIndividual rdf:about="http://JP_ontology.org/assessment/MCQ.44">
        <rdf:type rdf:resource="http://www.w3.org/2004/02/skos/core#Concept"/>
    </owl:NamedIndividual>
    


    <!-- http://JP_ontology.org/assessment/MCQ.45 -->


    <owl:NamedIndividual rdf:about="http://JP_ontology.org/assessment/MCQ.45">
        <rdf:type rdf:resource="http://www.w3.org/2004/02/skos/core#Concept"/>
    </owl:NamedIndividual>
    


    <!-- http://JP_ontology.org/assessment/MCQ.46 -->


    <owl:NamedIndividual rdf:about="http://JP_ontology.org/assessment/MCQ.46">
        <rdf:type rdf:resource="http://www.w3.org/2004/02/skos/core#Concept"/>
    </owl:NamedIndividual>
    


    <!-- http://JP_ontology.org/assessment/MCQ.47 -->


    <owl:NamedIndividual rdf:about="http://JP_ontology.org/assessment/MCQ.47">
        <rdf:type rdf:resource="http://www.w3.org/2004/02/skos/core#Concept"/>
    </owl:NamedIndividual>
    


    <!-- http://JP_ontology.org/assessment/MCQ.48 -->


    <owl:NamedIndividual rdf:about="http://JP_ontology.org/assessment/MCQ.48">
        <rdf:type rdf:resource="http://www.w3.org/2004/02/skos/core#Concept"/>
    </owl:NamedIndividual>
    


    <!-- http://JP_ontology.org/assessment/MCQ.49.1 -->


    <owl:NamedIndividual rdf:about="http://JP_ontology.org/assessment/MCQ.49.1">
        <rdf:type rdf:resource="http://www.w3.org/2004/02/skos/core#Concept"/>
    </owl:NamedIndividual>
    


    <!-- http://JP_ontology.org/assessment/MCQ.49.2 -->


    <owl:NamedIndividual rdf:about="http://JP_ontology.org/assessment/MCQ.49.2">
        <rdf:type rdf:resource="http://www.w3.org/2004/02/skos/core#Concept"/>
    </owl:NamedIndividual>
    


    <!-- http://JP_ontology.org/assessment/MCQ.49.3 -->


    <owl:NamedIndividual rdf:about="http://JP_ontology.org/assessment/MCQ.49.3">
        <rdf:type rdf:resource="http://www.w3.org/2004/02/skos/core#Concept"/>
    </owl:NamedIndividual>
    


    <!-- http://JP_ontology.org/assessment/MCQ.5.1 -->


    <owl:NamedIndividual rdf:about="http://JP_ontology.org/assessment/MCQ.5.1">
        <rdf:type rdf:resource="http://www.w3.org/2004/02/skos/core#Concept"/>
    </owl:NamedIndividual>
    


    <!-- http://JP_ontology.org/assessment/MCQ.5.2 -->


    <owl:NamedIndividual rdf:about="http://JP_ontology.org/assessment/MCQ.5.2">
        <rdf:type rdf:resource="http://www.w3.org/2004/02/skos/core#Concept"/>
    </owl:NamedIndividual>
    


    <!-- http://JP_ontology.org/assessment/MCQ.5.3 -->


    <owl:NamedIndividual rdf:about="http://JP_ontology.org/assessment/MCQ.5.3">
        <rdf:type rdf:resource="http://www.w3.org/2004/02/skos/core#Concept"/>
    </owl:NamedIndividual>
    


    <!-- http://JP_ontology.org/assessment/MCQ.5.4 -->


    <owl:NamedIndividual rdf:about="http://JP_ontology.org/assessment/MCQ.5.4">
        <rdf:type rdf:resource="http://www.w3.org/2004/02/skos/core#Concept"/>
    </owl:NamedIndividual>
    


    <!-- http://JP_ontology.org/assessment/MCQ.5.5 -->


    <owl:NamedIndividual rdf:about="http://JP_ontology.org/assessment/MCQ.5.5">
        <rdf:type rdf:resource="http://www.w3.org/2004/02/skos/core#Concept"/>
    </owl:NamedIndividual>
    


    <!-- http://JP_ontology.org/assessment/MCQ.5.6 -->


    <owl:NamedIndividual rdf:about="http://JP_ontology.org/assessment/MCQ.5.6">
        <rdf:type rdf:resource="http://www.w3.org/2004/02/skos/core#Concept"/>
    </owl:NamedIndividual>
    


    <!-- http://JP_ontology.org/assessment/MCQ.50 -->


    <owl:NamedIndividual rdf:about="http://JP_ontology.org/assessment/MCQ.50">
        <rdf:type rdf:resource="http://www.w3.org/2004/02/skos/core#Concept"/>
    </owl:NamedIndividual>
    


    <!-- http://JP_ontology.org/assessment/MCQ.51 -->


    <owl:NamedIndividual rdf:about="http://JP_ontology.org/assessment/MCQ.51">
        <rdf:type rdf:resource="http://www.w3.org/2004/02/skos/core#Concept"/>
    </owl:NamedIndividual>
    


    <!-- http://JP_ontology.org/assessment/MCQ.52 -->


    <owl:NamedIndividual rdf:about="http://JP_ontology.org/assessment/MCQ.52">
        <rdf:type rdf:resource="http://www.w3.org/2004/02/skos/core#Concept"/>
    </owl:NamedIndividual>
    


    <!-- http://JP_ontology.org/assessment/MCQ.53 -->


    <owl:NamedIndividual rdf:about="http://JP_ontology.org/assessment/MCQ.53">
        <rdf:type rdf:resource="http://www.w3.org/2004/02/skos/core#Concept"/>
    </owl:NamedIndividual>
    


    <!-- http://JP_ontology.org/assessment/MCQ.54.1 -->


    <owl:NamedIndividual rdf:about="http://JP_ontology.org/assessment/MCQ.54.1">
        <rdf:type rdf:resource="http://www.w3.org/2004/02/skos/core#Concept"/>
    </owl:NamedIndividual>
    


    <!-- http://JP_ontology.org/assessment/MCQ.54.2 -->


    <owl:NamedIndividual rdf:about="http://JP_ontology.org/assessment/MCQ.54.2">
        <rdf:type rdf:resource="http://www.w3.org/2004/02/skos/core#Concept"/>
    </owl:NamedIndividual>
    


    <!-- http://JP_ontology.org/assessment/MCQ.54.3 -->


    <owl:NamedIndividual rdf:about="http://JP_ontology.org/assessment/MCQ.54.3">
        <rdf:type rdf:resource="http://www.w3.org/2004/02/skos/core#Concept"/>
    </owl:NamedIndividual>
    


    <!-- http://JP_ontology.org/assessment/MCQ.54.4 -->


    <owl:NamedIndividual rdf:about="http://JP_ontology.org/assessment/MCQ.54.4">
        <rdf:type rdf:resource="http://www.w3.org/2004/02/skos/core#Concept"/>
    </owl:NamedIndividual>
    


    <!-- http://JP_ontology.org/assessment/MCQ.55.1 -->


    <owl:NamedIndividual rdf:about="http://JP_ontology.org/assessment/MCQ.55.1">
        <rdf:type rdf:resource="http://www.w3.org/2004/02/skos/core#Concept"/>
    </owl:NamedIndividual>
    


    <!-- http://JP_ontology.org/assessment/MCQ.55.2 -->


    <owl:NamedIndividual rdf:about="http://JP_ontology.org/assessment/MCQ.55.2">
        <rdf:type rdf:resource="http://www.w3.org/2004/02/skos/core#Concept"/>
    </owl:NamedIndividual>
    


    <!-- http://JP_ontology.org/assessment/MCQ.55.3 -->


    <owl:NamedIndividual rdf:about="http://JP_ontology.org/assessment/MCQ.55.3">
        <rdf:type rdf:resource="http://www.w3.org/2004/02/skos/core#Concept"/>
    </owl:NamedIndividual>
    


    <!-- http://JP_ontology.org/assessment/MCQ.56.1 -->


    <owl:NamedIndividual rdf:about="http://JP_ontology.org/assessment/MCQ.56.1">
        <rdf:type rdf:resource="http://www.w3.org/2004/02/skos/core#Concept"/>
    </owl:NamedIndividual>
    


    <!-- http://JP_ontology.org/assessment/MCQ.56.2 -->


    <owl:NamedIndividual rdf:about="http://JP_ontology.org/assessment/MCQ.56.2">
        <rdf:type rdf:resource="http://www.w3.org/2004/02/skos/core#Concept"/>
    </owl:NamedIndividual>
    


    <!-- http://JP_ontology.org/assessment/MCQ.56.3 -->


    <owl:NamedIndividual rdf:about="http://JP_ontology.org/assessment/MCQ.56.3">
        <rdf:type rdf:resource="http://www.w3.org/2004/02/skos/core#Concept"/>
    </owl:NamedIndividual>
    


    <!-- http://JP_ontology.org/assessment/MCQ.56.4 -->


    <owl:NamedIndividual rdf:about="http://JP_ontology.org/assessment/MCQ.56.4">
        <rdf:type rdf:resource="http://www.w3.org/2004/02/skos/core#Concept"/>
    </owl:NamedIndividual>
    


    <!-- http://JP_ontology.org/assessment/MCQ.57.1 -->


    <owl:NamedIndividual rdf:about="http://JP_ontology.org/assessment/MCQ.57.1">
        <rdf:type rdf:resource="http://www.w3.org/2004/02/skos/core#Concept"/>
    </owl:NamedIndividual>
    


    <!-- http://JP_ontology.org/assessment/MCQ.57.2 -->


    <owl:NamedIndividual rdf:about="http://JP_ontology.org/assessment/MCQ.57.2">
        <rdf:type rdf:resource="http://www.w3.org/2004/02/skos/core#Concept"/>
    </owl:NamedIndividual>
    


    <!-- http://JP_ontology.org/assessment/MCQ.58 -->


    <owl:NamedIndividual rdf:about="http://JP_ontology.org/assessment/MCQ.58">
        <rdf:type rdf:resource="http://www.w3.org/2004/02/skos/core#Concept"/>
    </owl:NamedIndividual>
    


    <!-- http://JP_ontology.org/assessment/MCQ.59 -->


    <owl:NamedIndividual rdf:about="http://JP_ontology.org/assessment/MCQ.59">
        <rdf:type rdf:resource="http://www.w3.org/2004/02/skos/core#Concept"/>
    </owl:NamedIndividual>
    


    <!-- http://JP_ontology.org/assessment/MCQ.6.1 -->


    <owl:NamedIndividual rdf:about="http://JP_ontology.org/assessment/MCQ.6.1">
        <rdf:type rdf:resource="http://www.w3.org/2004/02/skos/core#Concept"/>
    </owl:NamedIndividual>
    


    <!-- http://JP_ontology.org/assessment/MCQ.6.2 -->


    <owl:NamedIndividual rdf:about="http://JP_ontology.org/assessment/MCQ.6.2">
        <rdf:type rdf:resource="http://www.w3.org/2004/02/skos/core#Concept"/>
    </owl:NamedIndividual>
    


    <!-- http://JP_ontology.org/assessment/MCQ.6.3 -->


    <owl:NamedIndividual rdf:about="http://JP_ontology.org/assessment/MCQ.6.3">
        <rdf:type rdf:resource="http://www.w3.org/2004/02/skos/core#Concept"/>
    </owl:NamedIndividual>
    


    <!-- http://JP_ontology.org/assessment/MCQ.6.4 -->


    <owl:NamedIndividual rdf:about="http://JP_ontology.org/assessment/MCQ.6.4">
        <rdf:type rdf:resource="http://www.w3.org/2004/02/skos/core#Concept"/>
    </owl:NamedIndividual>
    


    <!-- http://JP_ontology.org/assessment/MCQ.60 -->


    <owl:NamedIndividual rdf:about="http://JP_ontology.org/assessment/MCQ.60">
        <rdf:type rdf:resource="http://www.w3.org/2004/02/skos/core#Concept"/>
    </owl:NamedIndividual>
    


    <!-- http://JP_ontology.org/assessment/MCQ.61 -->


    <owl:NamedIndividual rdf:about="http://JP_ontology.org/assessment/MCQ.61">
        <rdf:type rdf:resource="http://www.w3.org/2004/02/skos/core#Concept"/>
    </owl:NamedIndividual>
    


    <!-- http://JP_ontology.org/assessment/MCQ.62 -->


    <owl:NamedIndividual rdf:about="http://JP_ontology.org/assessment/MCQ.62">
        <rdf:type rdf:resource="http://www.w3.org/2004/02/skos/core#Concept"/>
    </owl:NamedIndividual>
    


    <!-- http://JP_ontology.org/assessment/MCQ.63 -->


    <owl:NamedIndividual rdf:about="http://JP_ontology.org/assessment/MCQ.63">
        <rdf:type rdf:resource="http://www.w3.org/2004/02/skos/core#Concept"/>
    </owl:NamedIndividual>
    


    <!-- http://JP_ontology.org/assessment/MCQ.64 -->


    <owl:NamedIndividual rdf:about="http://JP_ontology.org/assessment/MCQ.64">
        <rdf:type rdf:resource="http://www.w3.org/2004/02/skos/core#Concept"/>
    </owl:NamedIndividual>
    


    <!-- http://JP_ontology.org/assessment/MCQ.65 -->


    <owl:NamedIndividual rdf:about="http://JP_ontology.org/assessment/MCQ.65">
        <rdf:type rdf:resource="http://www.w3.org/2004/02/skos/core#Concept"/>
    </owl:NamedIndividual>
    


    <!-- http://JP_ontology.org/assessment/MCQ.66 -->


    <owl:NamedIndividual rdf:about="http://JP_ontology.org/assessment/MCQ.66">
        <rdf:type rdf:resource="http://www.w3.org/2004/02/skos/core#Concept"/>
    </owl:NamedIndividual>
    


    <!-- http://JP_ontology.org/assessment/MCQ.67 -->


    <owl:NamedIndividual rdf:about="http://JP_ontology.org/assessment/MCQ.67">
        <rdf:type rdf:resource="http://www.w3.org/2004/02/skos/core#Concept"/>
    </owl:NamedIndividual>
    


    <!-- http://JP_ontology.org/assessment/MCQ.68 -->


    <owl:NamedIndividual rdf:about="http://JP_ontology.org/assessment/MCQ.68">
        <rdf:type rdf:resource="http://www.w3.org/2004/02/skos/core#Concept"/>
    </owl:NamedIndividual>
    


    <!-- http://JP_ontology.org/assessment/MCQ.69 -->


    <owl:NamedIndividual rdf:about="http://JP_ontology.org/assessment/MCQ.69">
        <rdf:type rdf:resource="http://www.w3.org/2004/02/skos/core#Concept"/>
    </owl:NamedIndividual>
    


    <!-- http://JP_ontology.org/assessment/MCQ.7 -->


    <owl:NamedIndividual rdf:about="http://JP_ontology.org/assessment/MCQ.7">
        <rdf:type rdf:resource="http://www.w3.org/2004/02/skos/core#Concept"/>
    </owl:NamedIndividual>
    


    <!-- http://JP_ontology.org/assessment/MCQ.70.1 -->


    <owl:NamedIndividual rdf:about="http://JP_ontology.org/assessment/MCQ.70.1">
        <rdf:type rdf:resource="http://www.w3.org/2004/02/skos/core#Concept"/>
    </owl:NamedIndividual>
    


    <!-- http://JP_ontology.org/assessment/MCQ.70.2 -->


    <owl:NamedIndividual rdf:about="http://JP_ontology.org/assessment/MCQ.70.2">
        <rdf:type rdf:resource="http://www.w3.org/2004/02/skos/core#Concept"/>
    </owl:NamedIndividual>
    


    <!-- http://JP_ontology.org/assessment/MCQ.70.3 -->


    <owl:NamedIndividual rdf:about="http://JP_ontology.org/assessment/MCQ.70.3">
        <rdf:type rdf:resource="http://www.w3.org/2004/02/skos/core#Concept"/>
    </owl:NamedIndividual>
    


    <!-- http://JP_ontology.org/assessment/MCQ.70.4 -->


    <owl:NamedIndividual rdf:about="http://JP_ontology.org/assessment/MCQ.70.4">
        <rdf:type rdf:resource="http://www.w3.org/2004/02/skos/core#Concept"/>
    </owl:NamedIndividual>
    


    <!-- http://JP_ontology.org/assessment/MCQ.71 -->


    <owl:NamedIndividual rdf:about="http://JP_ontology.org/assessment/MCQ.71">
        <rdf:type rdf:resource="http://www.w3.org/2004/02/skos/core#Concept"/>
    </owl:NamedIndividual>
    


    <!-- http://JP_ontology.org/assessment/MCQ.72 -->


    <owl:NamedIndividual rdf:about="http://JP_ontology.org/assessment/MCQ.72">
        <rdf:type rdf:resource="http://www.w3.org/2004/02/skos/core#Concept"/>
    </owl:NamedIndividual>
    


    <!-- http://JP_ontology.org/assessment/MCQ.73 -->


    <owl:NamedIndividual rdf:about="http://JP_ontology.org/assessment/MCQ.73">
        <rdf:type rdf:resource="http://www.w3.org/2004/02/skos/core#Concept"/>
    </owl:NamedIndividual>
    


    <!-- http://JP_ontology.org/assessment/MCQ.74 -->


    <owl:NamedIndividual rdf:about="http://JP_ontology.org/assessment/MCQ.74">
        <rdf:type rdf:resource="http://www.w3.org/2004/02/skos/core#Concept"/>
    </owl:NamedIndividual>
    


    <!-- http://JP_ontology.org/assessment/MCQ.75.1 -->


    <owl:NamedIndividual rdf:about="http://JP_ontology.org/assessment/MCQ.75.1">
        <rdf:type rdf:resource="http://www.w3.org/2004/02/skos/core#Concept"/>
    </owl:NamedIndividual>
    


    <!-- http://JP_ontology.org/assessment/MCQ.75.2 -->


    <owl:NamedIndividual rdf:about="http://JP_ontology.org/assessment/MCQ.75.2">
        <rdf:type rdf:resource="http://www.w3.org/2004/02/skos/core#Concept"/>
    </owl:NamedIndividual>
    


    <!-- http://JP_ontology.org/assessment/MCQ.76 -->


    <owl:NamedIndividual rdf:about="http://JP_ontology.org/assessment/MCQ.76">
        <rdf:type rdf:resource="http://www.w3.org/2004/02/skos/core#Concept"/>
    </owl:NamedIndividual>
    


    <!-- http://JP_ontology.org/assessment/MCQ.77 -->


    <owl:NamedIndividual rdf:about="http://JP_ontology.org/assessment/MCQ.77">
        <rdf:type rdf:resource="http://www.w3.org/2004/02/skos/core#Concept"/>
    </owl:NamedIndividual>
    


    <!-- http://JP_ontology.org/assessment/MCQ.78 -->


    <owl:NamedIndividual rdf:about="http://JP_ontology.org/assessment/MCQ.78">
        <rdf:type rdf:resource="http://www.w3.org/2004/02/skos/core#Concept"/>
    </owl:NamedIndividual>
    


    <!-- http://JP_ontology.org/assessment/MCQ.79 -->


    <owl:NamedIndividual rdf:about="http://JP_ontology.org/assessment/MCQ.79">
        <rdf:type rdf:resource="http://www.w3.org/2004/02/skos/core#Concept"/>
    </owl:NamedIndividual>
    


    <!-- http://JP_ontology.org/assessment/MCQ.8.1 -->


    <owl:NamedIndividual rdf:about="http://JP_ontology.org/assessment/MCQ.8.1">
        <rdf:type rdf:resource="http://www.w3.org/2004/02/skos/core#Concept"/>
    </owl:NamedIndividual>
    


    <!-- http://JP_ontology.org/assessment/MCQ.8.2 -->


    <owl:NamedIndividual rdf:about="http://JP_ontology.org/assessment/MCQ.8.2">
        <rdf:type rdf:resource="http://www.w3.org/2004/02/skos/core#Concept"/>
    </owl:NamedIndividual>
    


    <!-- http://JP_ontology.org/assessment/MCQ.80 -->


    <owl:NamedIndividual rdf:about="http://JP_ontology.org/assessment/MCQ.80">
        <rdf:type rdf:resource="http://www.w3.org/2004/02/skos/core#Concept"/>
    </owl:NamedIndividual>
    


    <!-- http://JP_ontology.org/assessment/MCQ.81 -->


    <owl:NamedIndividual rdf:about="http://JP_ontology.org/assessment/MCQ.81">
        <rdf:type rdf:resource="http://www.w3.org/2004/02/skos/core#Concept"/>
    </owl:NamedIndividual>
    


    <!-- http://JP_ontology.org/assessment/MCQ.82 -->


    <owl:NamedIndividual rdf:about="http://JP_ontology.org/assessment/MCQ.82">
        <rdf:type rdf:resource="http://www.w3.org/2004/02/skos/core#Concept"/>
    </owl:NamedIndividual>
    


    <!-- http://JP_ontology.org/assessment/MCQ.83 -->


    <owl:NamedIndividual rdf:about="http://JP_ontology.org/assessment/MCQ.83">
        <rdf:type rdf:resource="http://www.w3.org/2004/02/skos/core#Concept"/>
    </owl:NamedIndividual>
    


    <!-- http://JP_ontology.org/assessment/MCQ.84 -->


    <owl:NamedIndividual rdf:about="http://JP_ontology.org/assessment/MCQ.84">
        <rdf:type rdf:resource="http://www.w3.org/2004/02/skos/core#Concept"/>
    </owl:NamedIndividual>
    


    <!-- http://JP_ontology.org/assessment/MCQ.85 -->


    <owl:NamedIndividual rdf:about="http://JP_ontology.org/assessment/MCQ.85">
        <rdf:type rdf:resource="http://www.w3.org/2004/02/skos/core#Concept"/>
    </owl:NamedIndividual>
    


    <!-- http://JP_ontology.org/assessment/MCQ.86 -->


    <owl:NamedIndividual rdf:about="http://JP_ontology.org/assessment/MCQ.86">
        <rdf:type rdf:resource="http://www.w3.org/2004/02/skos/core#Concept"/>
    </owl:NamedIndividual>
    


    <!-- http://JP_ontology.org/assessment/MCQ.87 -->


    <owl:NamedIndividual rdf:about="http://JP_ontology.org/assessment/MCQ.87">
        <rdf:type rdf:resource="http://www.w3.org/2004/02/skos/core#Concept"/>
    </owl:NamedIndividual>
    


    <!-- http://JP_ontology.org/assessment/MCQ.88 -->


    <owl:NamedIndividual rdf:about="http://JP_ontology.org/assessment/MCQ.88">
        <rdf:type rdf:resource="http://www.w3.org/2004/02/skos/core#Concept"/>
    </owl:NamedIndividual>
    


    <!-- http://JP_ontology.org/assessment/MCQ.89 -->


    <owl:NamedIndividual rdf:about="http://JP_ontology.org/assessment/MCQ.89">
        <rdf:type rdf:resource="http://www.w3.org/2004/02/skos/core#Concept"/>
    </owl:NamedIndividual>
    


    <!-- http://JP_ontology.org/assessment/MCQ.9.1 -->


    <owl:NamedIndividual rdf:about="http://JP_ontology.org/assessment/MCQ.9.1">
        <rdf:type rdf:resource="http://www.w3.org/2004/02/skos/core#Concept"/>
    </owl:NamedIndividual>
    


    <!-- http://JP_ontology.org/assessment/MCQ.9.2 -->


    <owl:NamedIndividual rdf:about="http://JP_ontology.org/assessment/MCQ.9.2">
        <rdf:type rdf:resource="http://www.w3.org/2004/02/skos/core#Concept"/>
    </owl:NamedIndividual>
    


    <!-- http://JP_ontology.org/assessment/MCQ.90 -->


    <owl:NamedIndividual rdf:about="http://JP_ontology.org/assessment/MCQ.90">
        <rdf:type rdf:resource="http://www.w3.org/2004/02/skos/core#Concept"/>
    </owl:NamedIndividual>
    


    <!-- http://JP_ontology.org/assessment/MCQ.91.1 -->


    <owl:NamedIndividual rdf:about="http://JP_ontology.org/assessment/MCQ.91.1">
        <rdf:type rdf:resource="http://www.w3.org/2004/02/skos/core#Concept"/>
    </owl:NamedIndividual>
    


    <!-- http://JP_ontology.org/assessment/MCQ.91.2 -->


    <owl:NamedIndividual rdf:about="http://JP_ontology.org/assessment/MCQ.91.2">
        <rdf:type rdf:resource="http://www.w3.org/2004/02/skos/core#Concept"/>
    </owl:NamedIndividual>
    


    <!-- http://JP_ontology.org/assessment/MCQ.92 -->


    <owl:NamedIndividual rdf:about="http://JP_ontology.org/assessment/MCQ.92">
        <rdf:type rdf:resource="http://www.w3.org/2004/02/skos/core#Concept"/>
    </owl:NamedIndividual>
    


    <!-- http://JP_ontology.org/assessment/MCQ.93 -->


    <owl:NamedIndividual rdf:about="http://JP_ontology.org/assessment/MCQ.93">
        <rdf:type rdf:resource="http://www.w3.org/2004/02/skos/core#Concept"/>
    </owl:NamedIndividual>
    


    <!-- http://JP_ontology.org/assessment/MCQ.94 -->


    <owl:NamedIndividual rdf:about="http://JP_ontology.org/assessment/MCQ.94">
        <rdf:type rdf:resource="http://www.w3.org/2004/02/skos/core#Concept"/>
    </owl:NamedIndividual>
    


    <!-- http://JP_ontology.org/assessment/MCQ.95 -->


    <owl:NamedIndividual rdf:about="http://JP_ontology.org/assessment/MCQ.95">
        <rdf:type rdf:resource="http://www.w3.org/2004/02/skos/core#Concept"/>
    </owl:NamedIndividual>
    


    <!-- http://JP_ontology.org/assessment/MCQ.96 -->


    <owl:NamedIndividual rdf:about="http://JP_ontology.org/assessment/MCQ.96">
        <rdf:type rdf:resource="http://www.w3.org/2004/02/skos/core#Concept"/>
    </owl:NamedIndividual>
    


    <!-- http://JP_ontology.org/assessment/MCQ.97 -->


    <owl:NamedIndividual rdf:about="http://JP_ontology.org/assessment/MCQ.97">
        <rdf:type rdf:resource="http://www.w3.org/2004/02/skos/core#Concept"/>
    </owl:NamedIndividual>
    


    <!-- http://JP_ontology.org/assessment/MCQ.98 -->


    <owl:NamedIndividual rdf:about="http://JP_ontology.org/assessment/MCQ.98">
        <rdf:type rdf:resource="http://www.w3.org/2004/02/skos/core#Concept"/>
    </owl:NamedIndividual>
    


    <!-- http://JP_ontology.org/assessment/MCQ.99 -->


    <owl:NamedIndividual rdf:about="http://JP_ontology.org/assessment/MCQ.99">
        <rdf:type rdf:resource="http://www.w3.org/2004/02/skos/core#Concept"/>
    </owl:NamedIndividual>
    


    <!-- http://JP_ontology.org/assessment/MCQ10.2AnswerA -->


    <owl:NamedIndividual rdf:about="http://JP_ontology.org/assessment/MCQ10.2AnswerA">
        <rdf:type rdf:resource="http://JP_ontology.org/assessment/MCQ.10.2"/>
        <skos:altLabel xml:lang="en">(i)</skos:altLabel>
        <skos:definition xml:lang="en">The policy is not reviewed at planned intervals or if significant changes occur, potentially leading to outdated or ineffective security measures that do not align with evolving threats and organisational needs.</skos:definition>
        <skos:prefLabel xml:lang="en">MCQ.10.2 - Not Implemented</skos:prefLabel>
    </owl:NamedIndividual>
    


    <!-- http://JP_ontology.org/assessment/MCQ10.2AnswerB -->


    <owl:NamedIndividual rdf:about="http://JP_ontology.org/assessment/MCQ10.2AnswerB">
        <rdf:type rdf:resource="http://JP_ontology.org/assessment/MCQ.10.2"/>
        <skos:altLabel xml:lang="en">(ii)</skos:altLabel>
        <skos:definition xml:lang="en">There are some efforts to review the policy at planned intervals or if significant changes occur. However, these reviews may not be consistently conducted or may lack thoroughness in assessing the policy&apos;s relevance and effectiveness.</skos:definition>
        <skos:prefLabel xml:lang="en">MCQ.10.2 - Partially Implemented</skos:prefLabel>
    </owl:NamedIndividual>
    


    <!-- http://JP_ontology.org/assessment/MCQ10.2AnswerC -->


    <owl:NamedIndividual rdf:about="http://JP_ontology.org/assessment/MCQ10.2AnswerC">
        <rdf:type rdf:resource="http://JP_ontology.org/assessment/MCQ.10.2"/>
        <skos:altLabel xml:lang="en">(iii)</skos:altLabel>
        <skos:definition xml:lang="en">The policy is fully reviewed at planned intervals and if significant changes occur, ensuring that it remains up-to-date, relevant, and aligned with the organisation&apos;s objectives and evolving security landscape.</skos:definition>
        <skos:prefLabel xml:lang="en">MCQ.10.2 - Fully Implemented</skos:prefLabel>
    </owl:NamedIndividual>
    


    <!-- http://JP_ontology.org/assessment/MCQ100AnswerA -->


    <owl:NamedIndividual rdf:about="http://JP_ontology.org/assessment/MCQ100AnswerA">
        <rdf:type rdf:resource="http://JP_ontology.org/assessment/MCQ.100"/>
        <skos:altLabel xml:lang="en">(i)</skos:altLabel>
        <skos:definition xml:lang="en">Data leakage prevention measures are not applied to systems, networks, and other devices that process, store, or transmit sensitive information, leaving the data vulnerable to unauthorized disclosure or leakage.</skos:definition>
        <skos:prefLabel xml:lang="en">MCQ.100 - Not Implemented</skos:prefLabel>
    </owl:NamedIndividual>
    


    <!-- http://JP_ontology.org/assessment/MCQ100AnswerB -->


    <owl:NamedIndividual rdf:about="http://JP_ontology.org/assessment/MCQ100AnswerB">
        <rdf:type rdf:resource="http://JP_ontology.org/assessment/MCQ.100"/>
        <skos:altLabel xml:lang="en">(ii)</skos:altLabel>
        <skos:definition xml:lang="en">There are some efforts to apply data leakage prevention measures to systems, networks, and other devices that handle sensitive information, but the implementation may be inconsistent or not fully comprehensive.</skos:definition>
        <skos:prefLabel xml:lang="en">MCQ.100 - Partially Implemented</skos:prefLabel>
    </owl:NamedIndividual>
    


    <!-- http://JP_ontology.org/assessment/MCQ100AnswerC -->


    <owl:NamedIndividual rdf:about="http://JP_ontology.org/assessment/MCQ100AnswerC">
        <rdf:type rdf:resource="http://JP_ontology.org/assessment/MCQ.100"/>
        <skos:altLabel xml:lang="en">(iii)</skos:altLabel>
        <skos:definition xml:lang="en">Data leakage prevention measures are fully applied to systems, networks, and other devices that process, store, or transmit sensitive information, ensuring protection against unauthorized disclosure or leakage of sensitive data.</skos:definition>
        <skos:prefLabel xml:lang="en">MCQ.100 - Fully Implemented</skos:prefLabel>
    </owl:NamedIndividual>
    


    <!-- http://JP_ontology.org/assessment/MCQ101AnswerA -->


    <owl:NamedIndividual rdf:about="http://JP_ontology.org/assessment/MCQ101AnswerA">
        <rdf:type rdf:resource="http://JP_ontology.org/assessment/MCQ.101"/>
        <skos:altLabel xml:lang="en">(i)</skos:altLabel>
        <skos:definition xml:lang="en">The organisation does not systematically identify or address external and internal issues relevant to its information security management system, leaving it vulnerable to unforeseen challenges.</skos:definition>
        <skos:prefLabel xml:lang="en">MCQ.101 - Not Implemented</skos:prefLabel>
    </owl:NamedIndividual>
    


    <!-- http://JP_ontology.org/assessment/MCQ101AnswerB -->


    <owl:NamedIndividual rdf:about="http://JP_ontology.org/assessment/MCQ101AnswerB">
        <rdf:type rdf:resource="http://JP_ontology.org/assessment/MCQ.101"/>
        <skos:altLabel xml:lang="en">(ii)</skos:altLabel>
        <skos:definition xml:lang="en">Some efforts are made to identify external and internal issues, but the process lacks thoroughness or consistency, resulting in gaps in understanding potential impacts on the information security management system.</skos:definition>
        <skos:prefLabel xml:lang="en">MCQ.101 - Partially Implemented</skos:prefLabel>
    </owl:NamedIndividual>
    


    <!-- http://JP_ontology.org/assessment/MCQ101AnswerC -->


    <owl:NamedIndividual rdf:about="http://JP_ontology.org/assessment/MCQ101AnswerC">
        <rdf:type rdf:resource="http://JP_ontology.org/assessment/MCQ.101"/>
        <skos:altLabel xml:lang="en">(iii)</skos:altLabel>
        <skos:definition xml:lang="en">The organisation actively identifies and assesses both external and internal issues relevant to its information security management system, ensuring a comprehensive understanding of potential impacts and enabling proactive measures to be taken to address them effectively.</skos:definition>
        <skos:prefLabel xml:lang="en">MCQ.101 - Fully Implemented</skos:prefLabel>
    </owl:NamedIndividual>
    


    <!-- http://JP_ontology.org/assessment/MCQ102AnswerA -->


    <owl:NamedIndividual rdf:about="http://JP_ontology.org/assessment/MCQ102AnswerA">
        <rdf:type rdf:resource="http://JP_ontology.org/assessment/MCQ.102"/>
        <skos:altLabel xml:lang="en">(i)</skos:altLabel>
        <skos:definition xml:lang="en">The organisation does not identify interested parties or their requirements, leading to a lack of alignment between the information security management system and stakeholder expectations.</skos:definition>
        <skos:prefLabel xml:lang="en">MCQ.102 - Not Implemented</skos:prefLabel>
    </owl:NamedIndividual>
    


    <!-- http://JP_ontology.org/assessment/MCQ102AnswerB -->


    <owl:NamedIndividual rdf:about="http://JP_ontology.org/assessment/MCQ102AnswerB">
        <rdf:type rdf:resource="http://JP_ontology.org/assessment/MCQ.102"/>
        <skos:altLabel xml:lang="en">(ii)</skos:altLabel>
        <skos:definition xml:lang="en">Some interested parties and their requirements are identified, but there is inconsistency in the process, resulting in gaps in understanding and addressing all relevant requirements.</skos:definition>
        <skos:prefLabel xml:lang="en">MCQ.102 - Partially Implemented</skos:prefLabel>
    </owl:NamedIndividual>
    


    <!-- http://JP_ontology.org/assessment/MCQ102AnswerC -->


    <owl:NamedIndividual rdf:about="http://JP_ontology.org/assessment/MCQ102AnswerC">
        <rdf:type rdf:resource="http://JP_ontology.org/assessment/MCQ.102"/>
        <skos:altLabel xml:lang="en">(iii)</skos:altLabel>
        <skos:definition xml:lang="en">The organisation systematically identifies interested parties, their requirements, and determines which requirements will be addressed through the information security management system, ensuring alignment with stakeholder needs and expectations.</skos:definition>
        <skos:prefLabel xml:lang="en">MCQ.102 - Fully Implemented</skos:prefLabel>
    </owl:NamedIndividual>
    


    <!-- http://JP_ontology.org/assessment/MCQ103AnswerA -->


    <owl:NamedIndividual rdf:about="http://JP_ontology.org/assessment/MCQ103AnswerA">
        <rdf:type rdf:resource="http://JP_ontology.org/assessment/MCQ.103"/>
        <skos:altLabel xml:lang="en">(i)</skos:altLabel>
        <skos:definition xml:lang="en">The organisation does not consider external and internal issues, requirements, or interfaces with other organisations when determining the scope of its ISMS, resulting in an unclear or inadequate scope.</skos:definition>
        <skos:prefLabel xml:lang="en">MCQ.103 - Not Implemented</skos:prefLabel>
    </owl:NamedIndividual>
    


    <!-- http://JP_ontology.org/assessment/MCQ103AnswerB -->


    <owl:NamedIndividual rdf:about="http://JP_ontology.org/assessment/MCQ103AnswerB">
        <rdf:type rdf:resource="http://JP_ontology.org/assessment/MCQ.103"/>
        <skos:altLabel xml:lang="en">(ii)</skos:altLabel>
        <skos:definition xml:lang="en">Some consideration is given to external and internal issues, requirements, and interfaces with other organisations, but there are inconsistencies or gaps in determining the scope, leading to potential ambiguity.</skos:definition>
        <skos:prefLabel xml:lang="en">MCQ.103 - Partially Implemented</skos:prefLabel>
    </owl:NamedIndividual>
    


    <!-- http://JP_ontology.org/assessment/MCQ103AnswerC -->


    <owl:NamedIndividual rdf:about="http://JP_ontology.org/assessment/MCQ103AnswerC">
        <rdf:type rdf:resource="http://JP_ontology.org/assessment/MCQ.103"/>
        <skos:altLabel xml:lang="en">(iii)</skos:altLabel>
        <skos:definition xml:lang="en">The organisation systematically considers external and internal issues, requirements, and interfaces with other organisations when determining the scope of its ISMS, ensuring clarity and alignment with organisational objectives. The scope is documented and readily available for reference.</skos:definition>
        <skos:prefLabel xml:lang="en">MCQ.103 - Fully Implemented</skos:prefLabel>
    </owl:NamedIndividual>
    


    <!-- http://JP_ontology.org/assessment/MCQ104AnswerA -->


    <owl:NamedIndividual rdf:about="http://JP_ontology.org/assessment/MCQ104AnswerA">
        <rdf:type rdf:resource="http://JP_ontology.org/assessment/MCQ.104"/>
        <skos:altLabel xml:lang="en">(i)</skos:altLabel>
        <skos:definition xml:lang="en">The organisation lacks a structured approach to establish, implement, maintain, and improve its ISMS, resulting in inconsistent or ad-hoc security measures that do not meet the requirements outlined in ISO27001.</skos:definition>
        <skos:prefLabel xml:lang="en">MCQ.104 - Not Implemented</skos:prefLabel>
    </owl:NamedIndividual>
    


    <!-- http://JP_ontology.org/assessment/MCQ104AnswerB -->


    <owl:NamedIndividual rdf:about="http://JP_ontology.org/assessment/MCQ104AnswerB">
        <rdf:type rdf:resource="http://JP_ontology.org/assessment/MCQ.104"/>
        <skos:altLabel xml:lang="en">(ii)</skos:altLabel>
        <skos:definition xml:lang="en">Some processes for establishing, implementing, maintaining, and improving the ISMS are in place, but there are inconsistencies or gaps in their execution, leading to partial compliance withISO27001&apos;s requirements.</skos:definition>
        <skos:prefLabel xml:lang="en">MCQ.104 - Partially Implemented</skos:prefLabel>
    </owl:NamedIndividual>
    


    <!-- http://JP_ontology.org/assessment/MCQ104AnswerC -->


    <owl:NamedIndividual rdf:about="http://JP_ontology.org/assessment/MCQ104AnswerC">
        <rdf:type rdf:resource="http://JP_ontology.org/assessment/MCQ.104"/>
        <skos:altLabel xml:lang="en">(iii)</skos:altLabel>
        <skos:definition xml:lang="en">The organisation has robust processes in place to systematically establish, implement, maintain, and continually improve its ISMS in strict accordance with the requirements outlined in ISO27001, ensuring comprehensive security measures are in place and effectively managed.</skos:definition>
        <skos:prefLabel xml:lang="en">MCQ.104 - Fully Implemented</skos:prefLabel>
    </owl:NamedIndividual>
    


    <!-- http://JP_ontology.org/assessment/MCQ105.1AnswerA -->


    <owl:NamedIndividual rdf:about="http://JP_ontology.org/assessment/MCQ105.1AnswerA">
        <rdf:type rdf:resource="http://JP_ontology.org/assessment/MCQ.105.1"/>
        <skos:altLabel xml:lang="en">(i)</skos:altLabel>
        <skos:definition xml:lang="en">Senior management does not ensure the alignment of information security policy and objectives with the organisation&apos;s strategic direction, leading to disjointed goals.</skos:definition>
        <skos:prefLabel xml:lang="en">MCQ.105.1 - Not Implemented</skos:prefLabel>
    </owl:NamedIndividual>
    


    <!-- http://JP_ontology.org/assessment/MCQ105.1AnswerB -->


    <owl:NamedIndividual rdf:about="http://JP_ontology.org/assessment/MCQ105.1AnswerB">
        <rdf:type rdf:resource="http://JP_ontology.org/assessment/MCQ.105.1"/>
        <skos:altLabel xml:lang="en">(ii)</skos:altLabel>
        <skos:definition xml:lang="en">Some efforts are made to align the information security policy and objectives with the organisation&apos;s strategic direction, but there are inconsistencies or gaps in the process.</skos:definition>
        <skos:prefLabel xml:lang="en">MCQ.105.1 - Partially Implemented</skos:prefLabel>
    </owl:NamedIndividual>
    


    <!-- http://JP_ontology.org/assessment/MCQ105.1AnswerC -->


    <owl:NamedIndividual rdf:about="http://JP_ontology.org/assessment/MCQ105.1AnswerC">
        <rdf:type rdf:resource="http://JP_ontology.org/assessment/MCQ.105.1"/>
        <skos:altLabel xml:lang="en">(iii)</skos:altLabel>
        <skos:definition xml:lang="en">Senior management ensures that the information security policy and objectives are fully compatible with the strategic direction of the organisation, ensuring alignment of goals and objectives.</skos:definition>
        <skos:prefLabel xml:lang="en">MCQ.105.1 - Fully Implemented</skos:prefLabel>
    </owl:NamedIndividual>
    


    <!-- http://JP_ontology.org/assessment/MCQ105.2AnswerA -->


    <owl:NamedIndividual rdf:about="http://JP_ontology.org/assessment/MCQ105.2AnswerA">
        <rdf:type rdf:resource="http://JP_ontology.org/assessment/MCQ.105.2"/>
        <skos:altLabel xml:lang="en">(i)</skos:altLabel>
        <skos:definition xml:lang="en">Senior management does not ensure the integration of ISMS requirements into organisational processes, resulting in a lack of alignment between security measures and organisational activities.</skos:definition>
        <skos:prefLabel xml:lang="en">MCQ.105.2 - Not Implemented</skos:prefLabel>
    </owl:NamedIndividual>
    


    <!-- http://JP_ontology.org/assessment/MCQ105.2AnswerB -->


    <owl:NamedIndividual rdf:about="http://JP_ontology.org/assessment/MCQ105.2AnswerB">
        <rdf:type rdf:resource="http://JP_ontology.org/assessment/MCQ.105.2"/>
        <skos:altLabel xml:lang="en">(ii)</skos:altLabel>
        <skos:definition xml:lang="en">Some efforts are made to integrate ISMS requirements into organisational processes, but there are inconsistencies or gaps in the integration process.</skos:definition>
        <skos:prefLabel xml:lang="en">MCQ.105.2 - Partially Implemented</skos:prefLabel>
    </owl:NamedIndividual>
    


    <!-- http://JP_ontology.org/assessment/MCQ105.2AnswerC -->


    <owl:NamedIndividual rdf:about="http://JP_ontology.org/assessment/MCQ105.2AnswerC">
        <rdf:type rdf:resource="http://JP_ontology.org/assessment/MCQ.105.2"/>
        <skos:altLabel xml:lang="en">(iii)</skos:altLabel>
        <skos:definition xml:lang="en">Senior management ensures the seamless integration of ISMS requirements into all organisational processes, ensuring alignment and effectiveness of security measures.</skos:definition>
        <skos:prefLabel xml:lang="en">MCQ.105.2 - Fully Implemented</skos:prefLabel>
    </owl:NamedIndividual>
    


    <!-- http://JP_ontology.org/assessment/MCQ105.3AnswerA -->


    <owl:NamedIndividual rdf:about="http://JP_ontology.org/assessment/MCQ105.3AnswerA">
        <rdf:type rdf:resource="http://JP_ontology.org/assessment/MCQ.105.3"/>
        <skos:altLabel xml:lang="en">(i)</skos:altLabel>
        <skos:definition xml:lang="en">Senior management does not ensure the availability of resources for the ISMS, resulting in resource shortages that hinder effective security management.</skos:definition>
        <skos:prefLabel xml:lang="en">MCQ.105.3 - Not Implemented</skos:prefLabel>
    </owl:NamedIndividual>
    


    <!-- http://JP_ontology.org/assessment/MCQ105.3AnswerB -->


    <owl:NamedIndividual rdf:about="http://JP_ontology.org/assessment/MCQ105.3AnswerB">
        <rdf:type rdf:resource="http://JP_ontology.org/assessment/MCQ.105.3"/>
        <skos:altLabel xml:lang="en">(ii)</skos:altLabel>
        <skos:definition xml:lang="en">Some efforts are made to ensure resource availability for the ISMS, but there are inconsistencies or gaps in resource allocation.</skos:definition>
        <skos:prefLabel xml:lang="en">MCQ.105.3 - Partially Implemented</skos:prefLabel>
    </owl:NamedIndividual>
    


    <!-- http://JP_ontology.org/assessment/MCQ105.3AnswerC -->


    <owl:NamedIndividual rdf:about="http://JP_ontology.org/assessment/MCQ105.3AnswerC">
        <rdf:type rdf:resource="http://JP_ontology.org/assessment/MCQ.105.3"/>
        <skos:altLabel xml:lang="en">(iii)</skos:altLabel>
        <skos:definition xml:lang="en">Senior management ensures that all necessary resources for the ISMS are readily available, ensuring effective implementation and maintenance of security measures.</skos:definition>
        <skos:prefLabel xml:lang="en">MCQ.105.3 - Fully Implemented</skos:prefLabel>
    </owl:NamedIndividual>
    


    <!-- http://JP_ontology.org/assessment/MCQ106.1AnswerA -->


    <owl:NamedIndividual rdf:about="http://JP_ontology.org/assessment/MCQ106.1AnswerA">
        <rdf:type rdf:resource="http://JP_ontology.org/assessment/MCQ.106.1"/>
        <skos:altLabel xml:lang="en">(i)</skos:altLabel>
        <skos:definition xml:lang="en">The organisation does not consider the broader organisational context or the needs and expectations of interested parties when planning for the ISMS, leading to potential disconnects between security measures and organisational objectives.</skos:definition>
        <skos:prefLabel xml:lang="en">MCQ.106.1 - Not Implemented</skos:prefLabel>
    </owl:NamedIndividual>
    


    <!-- http://JP_ontology.org/assessment/MCQ106.1AnswerB -->


    <owl:NamedIndividual rdf:about="http://JP_ontology.org/assessment/MCQ106.1AnswerB">
        <rdf:type rdf:resource="http://JP_ontology.org/assessment/MCQ.106.1"/>
        <skos:altLabel xml:lang="en">(ii)</skos:altLabel>
        <skos:definition xml:lang="en">Some consideration is given to the organisation&apos;s context and the needs and expectations of interested parties when planning for the ISMS, but there are inconsistencies or gaps in addressing risks and opportunities, resulting in partial alignment with ISMS objectives.</skos:definition>
        <skos:prefLabel xml:lang="en">MCQ.106.1 - Partially Implemented</skos:prefLabel>
    </owl:NamedIndividual>
    


    <!-- http://JP_ontology.org/assessment/MCQ106.1AnswerC -->


    <owl:NamedIndividual rdf:about="http://JP_ontology.org/assessment/MCQ106.1AnswerC">
        <rdf:type rdf:resource="http://JP_ontology.org/assessment/MCQ.106.1"/>
        <skos:altLabel xml:lang="en">(iii)</skos:altLabel>
        <skos:definition xml:lang="en">The organisation systematically considers its context and the needs and expectations of interested parties when planning for the ISMS, ensuring that risks and opportunities are identified and addressed to achieve intended outcomes, prevent undesired effects, and promote continual improvement.</skos:definition>
        <skos:prefLabel xml:lang="en">MCQ.106.1 - Fully Implemented</skos:prefLabel>
    </owl:NamedIndividual>
    


    <!-- http://JP_ontology.org/assessment/MCQ106.2AnswerA -->


    <owl:NamedIndividual rdf:about="http://JP_ontology.org/assessment/MCQ106.2AnswerA">
        <rdf:type rdf:resource="http://JP_ontology.org/assessment/MCQ.106.2"/>
        <skos:altLabel xml:lang="en">(i)</skos:altLabel>
        <skos:definition xml:lang="en">The organisation does not plan actions to address identified risks and opportunities for the ISMS, leading to a lack of proactive measures to mitigate potential threats or leverage opportunities for improvement.</skos:definition>
        <skos:prefLabel xml:lang="en">MCQ.106.2 - Not Implemented</skos:prefLabel>
    </owl:NamedIndividual>
    


    <!-- http://JP_ontology.org/assessment/MCQ106.2AnswerB -->


    <owl:NamedIndividual rdf:about="http://JP_ontology.org/assessment/MCQ106.2AnswerB">
        <rdf:type rdf:resource="http://JP_ontology.org/assessment/MCQ.106.2"/>
        <skos:altLabel xml:lang="en">(ii)</skos:altLabel>
        <skos:definition xml:lang="en">Some actions are planned to address identified risks and opportunities, but there are inconsistencies or gaps in implementation and integration into ISMS processes, hindering effectiveness.</skos:definition>
        <skos:prefLabel xml:lang="en">MCQ.106.2 - Partially Implemented</skos:prefLabel>
    </owl:NamedIndividual>
    


    <!-- http://JP_ontology.org/assessment/MCQ106.2AnswerC -->


    <owl:NamedIndividual rdf:about="http://JP_ontology.org/assessment/MCQ106.2AnswerC">
        <rdf:type rdf:resource="http://JP_ontology.org/assessment/MCQ.106.2"/>
        <skos:altLabel xml:lang="en">(iii)</skos:altLabel>
        <skos:definition xml:lang="en">The organisation plans actions to address identified risks and opportunities for the ISMS and integrates them into ISMS processes, ensuring proactive management and continual improvement. Additionally, mechanisms are established to evaluate the effectiveness of these actions.</skos:definition>
        <skos:prefLabel xml:lang="en">MCQ.106.2 - Fully Implemented</skos:prefLabel>
    </owl:NamedIndividual>
    


    <!-- http://JP_ontology.org/assessment/MCQ107.1AnswerA -->


    <owl:NamedIndividual rdf:about="http://JP_ontology.org/assessment/MCQ107.1AnswerA">
        <rdf:type rdf:resource="http://JP_ontology.org/assessment/MCQ.107.1"/>
        <skos:altLabel xml:lang="en">(i)</skos:altLabel>
        <skos:definition xml:lang="en">The organisation does not establish information security objectives consistently across relevant functions and levels, resulting in ambiguity and inconsistency in security goals.</skos:definition>
        <skos:prefLabel xml:lang="en">MCQ.107.1 - Not Implemented</skos:prefLabel>
    </owl:NamedIndividual>
    


    <!-- http://JP_ontology.org/assessment/MCQ107.1AnswerB -->


    <owl:NamedIndividual rdf:about="http://JP_ontology.org/assessment/MCQ107.1AnswerB">
        <rdf:type rdf:resource="http://JP_ontology.org/assessment/MCQ.107.1"/>
        <skos:altLabel xml:lang="en">(ii)</skos:altLabel>
        <skos:definition xml:lang="en">Some effort is made to establish information security objectives, but there are inconsistencies or gaps in their alignment with the information security policy, measurability, and consideration of applicable requirements and risk assessment results.</skos:definition>
        <skos:prefLabel xml:lang="en">MCQ.107.1 - Partially Implemented</skos:prefLabel>
    </owl:NamedIndividual>
    


    <!-- http://JP_ontology.org/assessment/MCQ107.1AnswerC -->


    <owl:NamedIndividual rdf:about="http://JP_ontology.org/assessment/MCQ107.1AnswerC">
        <rdf:type rdf:resource="http://JP_ontology.org/assessment/MCQ.107.1"/>
        <skos:altLabel xml:lang="en">(iii)</skos:altLabel>
        <skos:definition xml:lang="en">The organisation ensures that information security objectives are established consistently across relevant functions and levels. These objectives are aligned with the information security policy, measurable (where practicable), consider applicable requirements and risk assessment results, and are monitored, communicated, updated as needed, and documented.</skos:definition>
        <skos:prefLabel xml:lang="en">MCQ.107.1 - Fully Implemented</skos:prefLabel>
    </owl:NamedIndividual>
    


    <!-- http://JP_ontology.org/assessment/MCQ107.2AnswerA -->


    <owl:NamedIndividual rdf:about="http://JP_ontology.org/assessment/MCQ107.2AnswerA">
        <rdf:type rdf:resource="http://JP_ontology.org/assessment/MCQ.107.2"/>
        <skos:altLabel xml:lang="en">(i)</skos:altLabel>
        <skos:definition xml:lang="en">The organisation lacks a structured approach to planning for the achievement of information security objectives, leading to uncertainty regarding what needs to be done, required resources, responsibilities, timelines, and evaluation methods.</skos:definition>
        <skos:prefLabel xml:lang="en">MCQ.107.2 - Not Implemented</skos:prefLabel>
    </owl:NamedIndividual>
    


    <!-- http://JP_ontology.org/assessment/MCQ107.2AnswerB -->


    <owl:NamedIndividual rdf:about="http://JP_ontology.org/assessment/MCQ107.2AnswerB">
        <rdf:type rdf:resource="http://JP_ontology.org/assessment/MCQ.107.2"/>
        <skos:altLabel xml:lang="en">(ii)</skos:altLabel>
        <skos:definition xml:lang="en">Some planning is done to achieve information security objectives, but there are inconsistencies or gaps in determining actions, resource requirements, responsibilities, timelines, and evaluation methods.</skos:definition>
        <skos:prefLabel xml:lang="en">MCQ.107.2 - Partially Implemented</skos:prefLabel>
    </owl:NamedIndividual>
    


    <!-- http://JP_ontology.org/assessment/MCQ107.2AnswerC -->


    <owl:NamedIndividual rdf:about="http://JP_ontology.org/assessment/MCQ107.2AnswerC">
        <rdf:type rdf:resource="http://JP_ontology.org/assessment/MCQ.107.2"/>
        <skos:altLabel xml:lang="en">(iii)</skos:altLabel>
        <skos:definition xml:lang="en">The organisation systematically plans for the achievement of information security objectives by determining actions, resource requirements, responsibilities, timelines, and evaluation methods, ensuring clarity and effectiveness in implementation and monitoring. Additionally, documented information is retained on the information security objectives.</skos:definition>
        <skos:prefLabel xml:lang="en">MCQ.107.2 - Fully Implemented</skos:prefLabel>
    </owl:NamedIndividual>
    


    <!-- http://JP_ontology.org/assessment/MCQ108AnswerA -->


    <owl:NamedIndividual rdf:about="http://JP_ontology.org/assessment/MCQ108AnswerA">
        <rdf:type rdf:resource="http://JP_ontology.org/assessment/MCQ.108"/>
        <skos:altLabel xml:lang="en">(i)</skos:altLabel>
        <skos:definition xml:lang="en">The organisation does not systematically determine or provide the resources needed for the ISMS, resulting in resource shortages that hinder effective security management.</skos:definition>
        <skos:prefLabel xml:lang="en">MCQ.108 - Not Implemented</skos:prefLabel>
    </owl:NamedIndividual>
    


    <!-- http://JP_ontology.org/assessment/MCQ108AnswerB -->


    <owl:NamedIndividual rdf:about="http://JP_ontology.org/assessment/MCQ108AnswerB">
        <rdf:type rdf:resource="http://JP_ontology.org/assessment/MCQ.108"/>
        <skos:altLabel xml:lang="en">(ii)</skos:altLabel>
        <skos:definition xml:lang="en">Some effort is made to determine and provide resources for the ISMS, but there are inconsistencies or gaps in resource allocation, leading to challenges in maintaining and improving the system.</skos:definition>
        <skos:prefLabel xml:lang="en">MCQ.108 - Partially Implemented</skos:prefLabel>
    </owl:NamedIndividual>
    


    <!-- http://JP_ontology.org/assessment/MCQ108AnswerC -->


    <owl:NamedIndividual rdf:about="http://JP_ontology.org/assessment/MCQ108AnswerC">
        <rdf:type rdf:resource="http://JP_ontology.org/assessment/MCQ.108"/>
        <skos:altLabel xml:lang="en">(iii)</skos:altLabel>
        <skos:definition xml:lang="en">The organisation systematically determines and provides the necessary resources for the establishment, implementation, maintenance, and continual improvement of the ISMS, ensuring effective security management aligned with organisational objectives.</skos:definition>
        <skos:prefLabel xml:lang="en">MCQ.108 - Fully Implemented</skos:prefLabel>
    </owl:NamedIndividual>
    


    <!-- http://JP_ontology.org/assessment/MCQ109AnswerA -->


    <owl:NamedIndividual rdf:about="http://JP_ontology.org/assessment/MCQ109AnswerA">
        <rdf:type rdf:resource="http://JP_ontology.org/assessment/MCQ.109"/>
        <skos:altLabel xml:lang="en">(i)</skos:altLabel>
        <skos:definition xml:lang="en">The organisation lacks systematic control over documented information, leading to its unavailability, unsuitability for use, and inadequate protection from loss of confidentiality, improper use, or loss of integrity.</skos:definition>
        <skos:prefLabel xml:lang="en">MCQ.109 - Not Implemented</skos:prefLabel>
    </owl:NamedIndividual>
    


    <!-- http://JP_ontology.org/assessment/MCQ109AnswerB -->


    <owl:NamedIndividual rdf:about="http://JP_ontology.org/assessment/MCQ109AnswerB">
        <rdf:type rdf:resource="http://JP_ontology.org/assessment/MCQ.109"/>
        <skos:altLabel xml:lang="en">(ii)</skos:altLabel>
        <skos:definition xml:lang="en">Some efforts are made to control documented information, but there are inconsistencies or gaps in activities such as distribution, access, retrieval, use, storage, preservation, change control, retention, and disposition, resulting in potential risks to information security.</skos:definition>
        <skos:prefLabel xml:lang="en">MCQ.109 - Partially Implemented</skos:prefLabel>
    </owl:NamedIndividual>
    


    <!-- http://JP_ontology.org/assessment/MCQ109AnswerC -->


    <owl:NamedIndividual rdf:about="http://JP_ontology.org/assessment/MCQ109AnswerC">
        <rdf:type rdf:resource="http://JP_ontology.org/assessment/MCQ.109"/>
        <skos:altLabel xml:lang="en">(iii)</skos:altLabel>
        <skos:definition xml:lang="en">The organisation systematically controls documented information to ensure its availability, suitability for use, and adequate protection from loss of confidentiality, improper use, or loss of integrity. This includes addressing activities such as distribution, access, retrieval, use, storage, preservation, change control, retention, and disposition, as applicable. Additionally, documented information of external origin necessary for the ISMS is identified and controlled appropriately.</skos:definition>
        <skos:prefLabel xml:lang="en">MCQ.109 - Fully Implemented</skos:prefLabel>
    </owl:NamedIndividual>
    


    <!-- http://JP_ontology.org/assessment/MCQ110AnswerA -->


    <owl:NamedIndividual rdf:about="http://JP_ontology.org/assessment/MCQ110AnswerA">
        <rdf:type rdf:resource="http://JP_ontology.org/assessment/MCQ.110"/>
        <skos:altLabel xml:lang="en">(i)</skos:altLabel>
        <skos:definition xml:lang="en">The organisation lacks criteria for processes and control over them, leading to uncertainty in meeting requirements and implementing actions.</skos:definition>
        <skos:prefLabel xml:lang="en">MCQ.110 - Not Implemented</skos:prefLabel>
    </owl:NamedIndividual>
    


    <!-- http://JP_ontology.org/assessment/MCQ110AnswerB -->


    <owl:NamedIndividual rdf:about="http://JP_ontology.org/assessment/MCQ110AnswerB">
        <rdf:type rdf:resource="http://JP_ontology.org/assessment/MCQ.110"/>
        <skos:altLabel xml:lang="en">(ii)</skos:altLabel>
        <skos:definition xml:lang="en">Some criteria are established for processes, and there is partial control over them. However, there are inconsistencies or gaps in controlling planned changes and reviewing unintended changes, resulting in potential issues in meeting requirements.</skos:definition>
        <skos:prefLabel xml:lang="en">MCQ.110 - Partially Implemented</skos:prefLabel>
    </owl:NamedIndividual>
    


    <!-- http://JP_ontology.org/assessment/MCQ110AnswerC -->


    <owl:NamedIndividual rdf:about="http://JP_ontology.org/assessment/MCQ110AnswerC">
        <rdf:type rdf:resource="http://JP_ontology.org/assessment/MCQ.110"/>
        <skos:altLabel xml:lang="en">(iii)</skos:altLabel>
        <skos:definition xml:lang="en">The organisation establishes criteria for processes and ensures their control. Documented information is available to ensure confidence in process execution. Planned changes are controlled, and consequences of unintended changes are reviewed, with necessary actions taken to mitigate adverse effects. Additionally, externally provided processes, products, or services relevant to the ISMS are controlled.</skos:definition>
        <skos:prefLabel xml:lang="en">MCQ.110 - Fully Implemented</skos:prefLabel>
    </owl:NamedIndividual>
    


    <!-- http://JP_ontology.org/assessment/MCQ111AnswerA -->


    <owl:NamedIndividual rdf:about="http://JP_ontology.org/assessment/MCQ111AnswerA">
        <rdf:type rdf:resource="http://JP_ontology.org/assessment/MCQ.111"/>
        <skos:altLabel xml:lang="en">(i)</skos:altLabel>
        <skos:definition xml:lang="en">Development, testing, and production environments are not separated or adequately secured, leading to potential risks such as unauthorized access or data breaches.</skos:definition>
        <skos:prefLabel xml:lang="en">MCQ.111 - Not Implemented</skos:prefLabel>
    </owl:NamedIndividual>
    


    <!-- http://JP_ontology.org/assessment/MCQ111AnswerB -->


    <owl:NamedIndividual rdf:about="http://JP_ontology.org/assessment/MCQ111AnswerB">
        <rdf:type rdf:resource="http://JP_ontology.org/assessment/MCQ.111"/>
        <skos:altLabel xml:lang="en">(ii)</skos:altLabel>
        <skos:definition xml:lang="en">Some efforts are made to separate and secure development, testing, and production environments, but there are inconsistencies or gaps in implementation, resulting in potential vulnerabilities.</skos:definition>
        <skos:prefLabel xml:lang="en">MCQ.111 - Partially Implemented</skos:prefLabel>
    </owl:NamedIndividual>
    


    <!-- http://JP_ontology.org/assessment/MCQ111AnswerC -->


    <owl:NamedIndividual rdf:about="http://JP_ontology.org/assessment/MCQ111AnswerC">
        <rdf:type rdf:resource="http://JP_ontology.org/assessment/MCQ.111"/>
        <skos:altLabel xml:lang="en">(iii)</skos:altLabel>
        <skos:definition xml:lang="en">The organisation ensures the strict separation and robust security measures for development, testing, and production environments, minimizing risks and ensuring the integrity, confidentiality, and availability of data and systems.</skos:definition>
        <skos:prefLabel xml:lang="en">MCQ.111 - Fully Implemented</skos:prefLabel>
    </owl:NamedIndividual>
    


    <!-- http://JP_ontology.org/assessment/MCQ112.1AnswerA -->


    <owl:NamedIndividual rdf:about="http://JP_ontology.org/assessment/MCQ112.1AnswerA">
        <rdf:type rdf:resource="http://JP_ontology.org/assessment/MCQ.112.1"/>
        <skos:altLabel xml:lang="en">(i)</skos:altLabel>
        <skos:definition xml:lang="en">The organisation lacks determination of what needs to be monitored and measured, methods for monitoring and measurement, and specification of when or by whom monitoring and measurement should be performed, resulting in insufficient evidence of information security performance and ISMS effectiveness.</skos:definition>
        <skos:prefLabel xml:lang="en">MCQ.112.1 - Not Implemented</skos:prefLabel>
    </owl:NamedIndividual>
    


    <!-- http://JP_ontology.org/assessment/MCQ112.1AnswerB -->


    <owl:NamedIndividual rdf:about="http://JP_ontology.org/assessment/MCQ112.1AnswerB">
        <rdf:type rdf:resource="http://JP_ontology.org/assessment/MCQ.112.1"/>
        <skos:altLabel xml:lang="en">(ii)</skos:altLabel>
        <skos:definition xml:lang="en">Some effort is made to determine what needs to be monitored and measured, and methods for monitoring and measurement are partially established. However, there are inconsistencies or gaps in determining when and by whom monitoring and measurement should be performed, leading to incomplete or unreliable evidence of information security performance and ISMS effectiveness.</skos:definition>
        <skos:prefLabel xml:lang="en">MCQ.112.1 - Partially Implemented</skos:prefLabel>
    </owl:NamedIndividual>
    


    <!-- http://JP_ontology.org/assessment/MCQ112.1AnswerC -->


    <owl:NamedIndividual rdf:about="http://JP_ontology.org/assessment/MCQ112.1AnswerC">
        <rdf:type rdf:resource="http://JP_ontology.org/assessment/MCQ.112.1"/>
        <skos:altLabel xml:lang="en">(iii)</skos:altLabel>
        <skos:definition xml:lang="en">The organisation systematically determines what needs to be monitored and measured, establishes methods for monitoring and measurement that produce comparable and reproducible results, specifies when and by whom monitoring and measurement should be performed, and analyzes and evaluates the results.</skos:definition>
        <skos:prefLabel xml:lang="en">MCQ.112.1 - Fully Implemented</skos:prefLabel>
    </owl:NamedIndividual>
    


    <!-- http://JP_ontology.org/assessment/MCQ112.2AnswerA -->


    <owl:NamedIndividual rdf:about="http://JP_ontology.org/assessment/MCQ112.2AnswerA">
        <rdf:type rdf:resource="http://JP_ontology.org/assessment/MCQ.112.2"/>
        <skos:altLabel xml:lang="en">(i)</skos:altLabel>
        <skos:definition xml:lang="en">The organisation lacks a systematic approach to evaluating information security performance and ISMS effectiveness, resulting in a lack of understanding of the system&apos;s performance and effectiveness.</skos:definition>
        <skos:prefLabel xml:lang="en">MCQ.112.2 - Not Implemented</skos:prefLabel>
    </owl:NamedIndividual>
    


    <!-- http://JP_ontology.org/assessment/MCQ112.2AnswerB -->


    <owl:NamedIndividual rdf:about="http://JP_ontology.org/assessment/MCQ112.2AnswerB">
        <rdf:type rdf:resource="http://JP_ontology.org/assessment/MCQ.112.2"/>
        <skos:altLabel xml:lang="en">(ii)</skos:altLabel>
        <skos:definition xml:lang="en">Some effort is made to evaluate information security performance and ISMS effectiveness, but there are inconsistencies or gaps in the evaluation process, leading to limited insights into the system&apos;s performance and effectiveness.</skos:definition>
        <skos:prefLabel xml:lang="en">MCQ.112.2 - Partially Implemented</skos:prefLabel>
    </owl:NamedIndividual>
    


    <!-- http://JP_ontology.org/assessment/MCQ112.2AnswerC -->


    <owl:NamedIndividual rdf:about="http://JP_ontology.org/assessment/MCQ112.2AnswerC">
        <rdf:type rdf:resource="http://JP_ontology.org/assessment/MCQ.112.2"/>
        <skos:altLabel xml:lang="en">(iii)</skos:altLabel>
        <skos:definition xml:lang="en">The organisation systematically evaluates information security performance and ISMS effectiveness, ensuring a comprehensive understanding of the system&apos;s performance and effectiveness.</skos:definition>
        <skos:prefLabel xml:lang="en">MCQ.112.2 - Fully Implemented</skos:prefLabel>
    </owl:NamedIndividual>
    


    <!-- http://JP_ontology.org/assessment/MCQ113AnswerA -->


    <owl:NamedIndividual rdf:about="http://JP_ontology.org/assessment/MCQ113AnswerA">
        <rdf:type rdf:resource="http://JP_ontology.org/assessment/MCQ.113"/>
        <skos:altLabel xml:lang="en">(i)</skos:altLabel>
        <skos:definition xml:lang="en">The organisation does not conduct internal audits at planned intervals to assess conformity to its own requirements and the requirements of relevant documents, nor does it evaluate the effectiveness of ISMS implementation and maintenance.</skos:definition>
        <skos:prefLabel xml:lang="en">MCQ.113 - Not Implemented</skos:prefLabel>
    </owl:NamedIndividual>
    


    <!-- http://JP_ontology.org/assessment/MCQ113AnswerB -->


    <owl:NamedIndividual rdf:about="http://JP_ontology.org/assessment/MCQ113AnswerB">
        <rdf:type rdf:resource="http://JP_ontology.org/assessment/MCQ.113"/>
        <skos:altLabel xml:lang="en">(ii)</skos:altLabel>
        <skos:definition xml:lang="en">Some internal audits are conducted to assess conformity to the organisation&apos;s own requirements and relevant documents, as well as the effectiveness of ISMS implementation and maintenance. However, there are inconsistencies or gaps in the audit process.</skos:definition>
        <skos:prefLabel xml:lang="en">MCQ.113 - Partially Implemented</skos:prefLabel>
    </owl:NamedIndividual>
    


    <!-- http://JP_ontology.org/assessment/MCQ113AnswerC -->


    <owl:NamedIndividual rdf:about="http://JP_ontology.org/assessment/MCQ113AnswerC">
        <rdf:type rdf:resource="http://JP_ontology.org/assessment/MCQ.113"/>
        <skos:altLabel xml:lang="en">(iii)</skos:altLabel>
        <skos:definition xml:lang="en">The organisation conducts internal audits at planned intervals to assess conformity to its own requirements and the requirements of relevant documents, as well as the effectiveness of ISMS implementation and maintenance. This ensures a comprehensive evaluation of the ISMS.</skos:definition>
        <skos:prefLabel xml:lang="en">MCQ.113 - Fully Implemented</skos:prefLabel>
    </owl:NamedIndividual>
    


    <!-- http://JP_ontology.org/assessment/MCQ114AnswerA -->


    <owl:NamedIndividual rdf:about="http://JP_ontology.org/assessment/MCQ114AnswerA">
        <rdf:type rdf:resource="http://JP_ontology.org/assessment/MCQ.114"/>
        <skos:altLabel xml:lang="en">(i)</skos:altLabel>
        <skos:definition xml:lang="en">The organisation lacks a planned, established, implemented, and maintained audit program, including defined frequency, methods, responsibilities, planning requirements, and reporting. Additionally, there is no consideration given to the importance of processes or results of previous audits.</skos:definition>
        <skos:prefLabel xml:lang="en">MCQ.114 - Not Implemented</skos:prefLabel>
    </owl:NamedIndividual>
    


    <!-- http://JP_ontology.org/assessment/MCQ114AnswerB -->


    <owl:NamedIndividual rdf:about="http://JP_ontology.org/assessment/MCQ114AnswerB">
        <rdf:type rdf:resource="http://JP_ontology.org/assessment/MCQ.114"/>
        <skos:altLabel xml:lang="en">(ii)</skos:altLabel>
        <skos:definition xml:lang="en">Some efforts are made to establish an audit program, but there are inconsistencies or gaps in defining frequency, methods, responsibilities, planning requirements, and reporting. There is partial consideration of the importance of processes and results of previous audits.</skos:definition>
        <skos:prefLabel xml:lang="en">MCQ.114 - Partially Implemented</skos:prefLabel>
    </owl:NamedIndividual>
    


    <!-- http://JP_ontology.org/assessment/MCQ114AnswerC -->


    <owl:NamedIndividual rdf:about="http://JP_ontology.org/assessment/MCQ114AnswerC">
        <rdf:type rdf:resource="http://JP_ontology.org/assessment/MCQ.114"/>
        <skos:altLabel xml:lang="en">(iii)</skos:altLabel>
        <skos:definition xml:lang="en">The organisation plans, establishes, implements, and maintains an audit program, including defined frequency, methods, responsibilities, planning requirements, and reporting. Consideration is given to the importance of processes and results of previous audits. Auditors are selected to ensure objectivity and impartiality, and audit results are reported to relevant management. Documented information is available as evidence of the implementation of the audit program and the audit results.</skos:definition>
        <skos:prefLabel xml:lang="en">MCQ.114 - Fully Implemented</skos:prefLabel>
    </owl:NamedIndividual>
    


    <!-- http://JP_ontology.org/assessment/MCQ115AnswerA -->


    <owl:NamedIndividual rdf:about="http://JP_ontology.org/assessment/MCQ115AnswerA">
        <rdf:type rdf:resource="http://JP_ontology.org/assessment/MCQ.115"/>
        <skos:altLabel xml:lang="en">(i)</skos:altLabel>
        <skos:definition xml:lang="en">Senior management does not conduct reviews of the information security management system at planned intervals, leading to uncertainty regarding its suitability, adequacy, and effectiveness.</skos:definition>
        <skos:prefLabel xml:lang="en">MCQ.115 - Not Implemented</skos:prefLabel>
    </owl:NamedIndividual>
    


    <!-- http://JP_ontology.org/assessment/MCQ115AnswerB -->


    <owl:NamedIndividual rdf:about="http://JP_ontology.org/assessment/MCQ115AnswerB">
        <rdf:type rdf:resource="http://JP_ontology.org/assessment/MCQ.115"/>
        <skos:altLabel xml:lang="en">(ii)</skos:altLabel>
        <skos:definition xml:lang="en">Some effort is made by senior management to review the information security management system at planned intervals, but there are inconsistencies or gaps in ensuring its continuing suitability, adequacy, and effectiveness.</skos:definition>
        <skos:prefLabel xml:lang="en">MCQ.115 - Partially Implemented</skos:prefLabel>
    </owl:NamedIndividual>
    


    <!-- http://JP_ontology.org/assessment/MCQ115AnswerC -->


    <owl:NamedIndividual rdf:about="http://JP_ontology.org/assessment/MCQ115AnswerC">
        <rdf:type rdf:resource="http://JP_ontology.org/assessment/MCQ.115"/>
        <skos:altLabel xml:lang="en">(iii)</skos:altLabel>
        <skos:definition xml:lang="en">Senior management systematically conducts reviews of the information security management system at planned intervals, ensuring its continuing suitability, adequacy, and effectiveness. This ensures that the ISMS remains aligned with organisational goals and adapts to changes in the internal and external environment.</skos:definition>
        <skos:prefLabel xml:lang="en">MCQ.115 - Fully Implemented</skos:prefLabel>
    </owl:NamedIndividual>
    


    <!-- http://JP_ontology.org/assessment/MCQ116AnswerA -->


    <owl:NamedIndividual rdf:about="http://JP_ontology.org/assessment/MCQ116AnswerA">
        <rdf:type rdf:resource="http://JP_ontology.org/assessment/MCQ.116"/>
        <skos:altLabel xml:lang="en">(i)</skos:altLabel>
        <skos:definition xml:lang="en">The results of the management review do not include decisions related to continual improvement opportunities or changes to the ISMS, leading to missed opportunities for enhancing information security.</skos:definition>
        <skos:prefLabel xml:lang="en">MCQ.116 - Not Implemented</skos:prefLabel>
    </owl:NamedIndividual>
    


    <!-- http://JP_ontology.org/assessment/MCQ116AnswerB -->


    <owl:NamedIndividual rdf:about="http://JP_ontology.org/assessment/MCQ116AnswerB">
        <rdf:type rdf:resource="http://JP_ontology.org/assessment/MCQ.116"/>
        <skos:altLabel xml:lang="en">(ii)</skos:altLabel>
        <skos:definition xml:lang="en">Some decisions related to continual improvement opportunities and changes to the ISMS are included in the results of the management review, but there are inconsistencies or gaps in the process.</skos:definition>
        <skos:prefLabel xml:lang="en">MCQ.116 - Partially Implemented</skos:prefLabel>
    </owl:NamedIndividual>
    


    <!-- http://JP_ontology.org/assessment/MCQ116AnswerC -->


    <owl:NamedIndividual rdf:about="http://JP_ontology.org/assessment/MCQ116AnswerC">
        <rdf:type rdf:resource="http://JP_ontology.org/assessment/MCQ.116"/>
        <skos:altLabel xml:lang="en">(iii)</skos:altLabel>
        <skos:definition xml:lang="en">The results of the management review include decisions related to continual improvement opportunities and changes to the ISMS. These decisions are systematically considered and documented, ensuring that the ISMS evolves to meet current and future needs effectively.</skos:definition>
        <skos:prefLabel xml:lang="en">MCQ.116 - Fully Implemented</skos:prefLabel>
    </owl:NamedIndividual>
    


    <!-- http://JP_ontology.org/assessment/MCQ117AnswerA -->


    <owl:NamedIndividual rdf:about="http://JP_ontology.org/assessment/MCQ117AnswerA">
        <rdf:type rdf:resource="http://JP_ontology.org/assessment/MCQ.117"/>
        <skos:altLabel xml:lang="en">(i)</skos:altLabel>
        <skos:definition xml:lang="en">The organisation does not have processes in place to continually improve the ISMS, resulting in stagnation and potential vulnerabilities.</skos:definition>
        <skos:prefLabel xml:lang="en">MCQ.117 - Not Implemented</skos:prefLabel>
    </owl:NamedIndividual>
    


    <!-- http://JP_ontology.org/assessment/MCQ117AnswerB -->


    <owl:NamedIndividual rdf:about="http://JP_ontology.org/assessment/MCQ117AnswerB">
        <rdf:type rdf:resource="http://JP_ontology.org/assessment/MCQ.117"/>
        <skos:altLabel xml:lang="en">(ii)</skos:altLabel>
        <skos:definition xml:lang="en">Some efforts are made to improve the ISMS, but there are inconsistencies or gaps in ensuring continual improvement across all aspects of suitability, adequacy, and effectiveness.</skos:definition>
        <skos:prefLabel xml:lang="en">MCQ.117 - Partially Implemented</skos:prefLabel>
    </owl:NamedIndividual>
    


    <!-- http://JP_ontology.org/assessment/MCQ117AnswerC -->


    <owl:NamedIndividual rdf:about="http://JP_ontology.org/assessment/MCQ117AnswerC">
        <rdf:type rdf:resource="http://JP_ontology.org/assessment/MCQ.117"/>
        <skos:altLabel xml:lang="en">(iii)</skos:altLabel>
        <skos:definition xml:lang="en">The organisation has established processes to continually improve the suitability, adequacy, and effectiveness of the ISMS. These processes are systematically implemented and monitored to ensure ongoing enhancement of information security practices.</skos:definition>
        <skos:prefLabel xml:lang="en">MCQ.117 - Fully Implemented</skos:prefLabel>
    </owl:NamedIndividual>
    


    <!-- http://JP_ontology.org/assessment/MCQ118AnswerA -->


    <owl:NamedIndividual rdf:about="http://JP_ontology.org/assessment/MCQ118AnswerA">
        <rdf:type rdf:resource="http://JP_ontology.org/assessment/MCQ.118"/>
        <skos:altLabel xml:lang="en">(i)</skos:altLabel>
        <skos:definition xml:lang="en">The organisation does not have a systematic approach to address nonconformities, leading to ineffective control and correction, and potential recurrence.</skos:definition>
        <skos:prefLabel xml:lang="en">MCQ.118 - Not Implemented</skos:prefLabel>
    </owl:NamedIndividual>
    


    <!-- http://JP_ontology.org/assessment/MCQ118AnswerB -->


    <owl:NamedIndividual rdf:about="http://JP_ontology.org/assessment/MCQ118AnswerB">
        <rdf:type rdf:resource="http://JP_ontology.org/assessment/MCQ.118"/>
        <skos:altLabel xml:lang="en">(ii)</skos:altLabel>
        <skos:definition xml:lang="en">Some actions are taken to address nonconformities, but there are inconsistencies or gaps in evaluating causes, implementing corrective actions, and reviewing effectiveness.</skos:definition>
        <skos:prefLabel xml:lang="en">MCQ.118 - Partially Implemented</skos:prefLabel>
    </owl:NamedIndividual>
    


    <!-- http://JP_ontology.org/assessment/MCQ118AnswerC -->


    <owl:NamedIndividual rdf:about="http://JP_ontology.org/assessment/MCQ118AnswerC">
        <rdf:type rdf:resource="http://JP_ontology.org/assessment/MCQ.118"/>
        <skos:altLabel xml:lang="en">(iii)</skos:altLabel>
        <skos:definition xml:lang="en">The organisation reacts to nonconformities by taking action to control and correct them, addressing consequences, evaluating causes to prevent recurrence, implementing necessary actions, reviewing the effectiveness of corrective actions, and making changes to the ISMS if necessary. Corrective actions are appropriate to the effects of the nonconformities encountered. Documented information is available as evidence of the nature of nonconformities, subsequent actions taken, and the results of corrective actions.</skos:definition>
        <skos:prefLabel xml:lang="en">MCQ.118 - Fully Implemented</skos:prefLabel>
    </owl:NamedIndividual>
    


    <!-- http://JP_ontology.org/assessment/MCQ119AnswerA -->


    <owl:NamedIndividual rdf:about="http://JP_ontology.org/assessment/MCQ119AnswerA">
        <rdf:type rdf:resource="http://JP_ontology.org/assessment/MCQ.119"/>
        <skos:altLabel xml:lang="en">(i)</skos:altLabel>
        <skos:definition xml:lang="en">Management does not require personnel to adhere to information security policies and procedures, leading to inconsistent or inadequate implementation of security measures.</skos:definition>
        <skos:prefLabel xml:lang="en">MCQ.119 - Not Implemented</skos:prefLabel>
    </owl:NamedIndividual>
    


    <!-- http://JP_ontology.org/assessment/MCQ119AnswerB -->


    <owl:NamedIndividual rdf:about="http://JP_ontology.org/assessment/MCQ119AnswerB">
        <rdf:type rdf:resource="http://JP_ontology.org/assessment/MCQ.119"/>
        <skos:altLabel xml:lang="en">(ii)</skos:altLabel>
        <skos:definition xml:lang="en">Some efforts are made by management to require personnel to follow information security policies and procedures, but there are inconsistencies or gaps in enforcement.</skos:definition>
        <skos:prefLabel xml:lang="en">MCQ.119 - Partially Implemented</skos:prefLabel>
    </owl:NamedIndividual>
    


    <!-- http://JP_ontology.org/assessment/MCQ119AnswerC -->


    <owl:NamedIndividual rdf:about="http://JP_ontology.org/assessment/MCQ119AnswerC">
        <rdf:type rdf:resource="http://JP_ontology.org/assessment/MCQ.119"/>
        <skos:altLabel xml:lang="en">(iii)</skos:altLabel>
        <skos:definition xml:lang="en">Management systematically requires all personnel to apply information security in accordance with established policies and procedures. This ensures consistent adherence to security measures across the organisation.</skos:definition>
        <skos:prefLabel xml:lang="en">MCQ.119 - Fully Implemented</skos:prefLabel>
    </owl:NamedIndividual>
    


    <!-- http://JP_ontology.org/assessment/MCQ11AnswerA -->


    <owl:NamedIndividual rdf:about="http://JP_ontology.org/assessment/MCQ11AnswerA">
        <rdf:type rdf:resource="http://JP_ontology.org/assessment/MCQ.11"/>
        <skos:altLabel xml:lang="en">(i)</skos:altLabel>
        <skos:definition xml:lang="en">Roles and responsibilities related to information security are not clearly defined, and there is no formal allocation process based on organisational needs.</skos:definition>
        <skos:prefLabel xml:lang="en">MCQ.11 - Not Implemented</skos:prefLabel>
    </owl:NamedIndividual>
    


    <!-- http://JP_ontology.org/assessment/MCQ11AnswerB -->


    <owl:NamedIndividual rdf:about="http://JP_ontology.org/assessment/MCQ11AnswerB">
        <rdf:type rdf:resource="http://JP_ontology.org/assessment/MCQ.11"/>
        <skos:altLabel xml:lang="en">(ii)</skos:altLabel>
        <skos:definition xml:lang="en">There is a general understanding of information security roles and responsibilities, but they are not consistently defined and allocated according to the organisation&apos;s needs. Some areas may lack clarity or consistency.</skos:definition>
        <skos:prefLabel xml:lang="en">MCQ.11 - Partially Implemented</skos:prefLabel>
    </owl:NamedIndividual>
    


    <!-- http://JP_ontology.org/assessment/MCQ11AnswerC -->


    <owl:NamedIndividual rdf:about="http://JP_ontology.org/assessment/MCQ11AnswerC">
        <rdf:type rdf:resource="http://JP_ontology.org/assessment/MCQ.11"/>
        <skos:altLabel xml:lang="en">(iii)</skos:altLabel>
        <skos:definition xml:lang="en">Clear and comprehensive information security roles and responsibilities are defined and allocated based on the specific needs of the organisation. There are established processes for regularly reviewing and updating these roles to ensure alignment with organisational requirements.</skos:definition>
        <skos:prefLabel xml:lang="en">MCQ.11 - Fully Implemented</skos:prefLabel>
    </owl:NamedIndividual>
    


    <!-- http://JP_ontology.org/assessment/MCQ120AnswerA -->


    <owl:NamedIndividual rdf:about="http://JP_ontology.org/assessment/MCQ120AnswerA">
        <rdf:type rdf:resource="http://JP_ontology.org/assessment/MCQ.120"/>
        <skos:altLabel xml:lang="en">(i)</skos:altLabel>
        <skos:definition xml:lang="en">The organisation lacks procedures for information labeling or does not align them with the adopted information classification scheme, leading to confusion and inconsistency in labeling practices.</skos:definition>
        <skos:prefLabel xml:lang="en">MCQ.120 - Not Implemented</skos:prefLabel>
    </owl:NamedIndividual>
    


    <!-- http://JP_ontology.org/assessment/MCQ120AnswerB -->


    <owl:NamedIndividual rdf:about="http://JP_ontology.org/assessment/MCQ120AnswerB">
        <rdf:type rdf:resource="http://JP_ontology.org/assessment/MCQ.120"/>
        <skos:altLabel xml:lang="en">(ii)</skos:altLabel>
        <skos:definition xml:lang="en">Some procedures for information labeling are developed, but there are inconsistencies or gaps in alignment with the adopted information classification scheme, resulting in limited effectiveness.</skos:definition>
        <skos:prefLabel xml:lang="en">MCQ.120 - Partially Implemented</skos:prefLabel>
    </owl:NamedIndividual>
    


    <!-- http://JP_ontology.org/assessment/MCQ120AnswerC -->


    <owl:NamedIndividual rdf:about="http://JP_ontology.org/assessment/MCQ120AnswerC">
        <rdf:type rdf:resource="http://JP_ontology.org/assessment/MCQ.120"/>
        <skos:altLabel xml:lang="en">(iii)</skos:altLabel>
        <skos:definition xml:lang="en">The organisation systematically develops and implements procedures for information labeling, ensuring alignment with the adopted information classification scheme. This ensures consistent and effective labeling practices across the organisation.</skos:definition>
        <skos:prefLabel xml:lang="en">MCQ.120 - Fully Implemented</skos:prefLabel>
    </owl:NamedIndividual>
    


    <!-- http://JP_ontology.org/assessment/MCQ121AnswerA -->


    <owl:NamedIndividual rdf:about="http://JP_ontology.org/assessment/MCQ121AnswerA">
        <rdf:type rdf:resource="http://JP_ontology.org/assessment/MCQ.121"/>
        <skos:altLabel xml:lang="en">(i)</skos:altLabel>
        <skos:definition xml:lang="en">The organisation lacks change management procedures for information processing facilities and information systems, leading to uncontrolled changes and potential disruptions.</skos:definition>
        <skos:prefLabel xml:lang="en">MCQ.121 - Not Implemented</skos:prefLabel>
    </owl:NamedIndividual>
    


    <!-- http://JP_ontology.org/assessment/MCQ121AnswerB -->


    <owl:NamedIndividual rdf:about="http://JP_ontology.org/assessment/MCQ121AnswerB">
        <rdf:type rdf:resource="http://JP_ontology.org/assessment/MCQ.121"/>
        <skos:altLabel xml:lang="en">(ii)</skos:altLabel>
        <skos:definition xml:lang="en">Some change management procedures are implemented, but there are inconsistencies or gaps in their application to information processing facilities and information systems, resulting in limited effectiveness.</skos:definition>
        <skos:prefLabel xml:lang="en">MCQ.121 - Partially Implemented</skos:prefLabel>
    </owl:NamedIndividual>
    


    <!-- http://JP_ontology.org/assessment/MCQ121AnswerC -->


    <owl:NamedIndividual rdf:about="http://JP_ontology.org/assessment/MCQ121AnswerC">
        <rdf:type rdf:resource="http://JP_ontology.org/assessment/MCQ.121"/>
        <skos:altLabel xml:lang="en">(iii)</skos:altLabel>
        <skos:definition xml:lang="en">The organisation has established change management procedures specifically for information processing facilities and information systems. These procedures ensure that changes are effectively managed, minimizing risks of disruptions and ensuring continuity of operations.</skos:definition>
        <skos:prefLabel xml:lang="en">MCQ.121 - Fully Implemented</skos:prefLabel>
    </owl:NamedIndividual>
    


    <!-- http://JP_ontology.org/assessment/MCQ122AnswerA -->


    <owl:NamedIndividual rdf:about="http://JP_ontology.org/assessment/MCQ122AnswerA">
        <rdf:type rdf:resource="http://JP_ontology.org/assessment/MCQ.122"/>
        <skos:altLabel xml:lang="en">(i)</skos:altLabel>
        <skos:definition xml:lang="en">The organisation lacks a structured approach to planning and agreement between testers and appropriate management for audit tests and assurance activities, leading to ineffective assessment of operational systems.</skos:definition>
        <skos:prefLabel xml:lang="en">MCQ.122 - Not Implemented</skos:prefLabel>
    </owl:NamedIndividual>
    


    <!-- http://JP_ontology.org/assessment/MCQ122AnswerB -->


    <owl:NamedIndividual rdf:about="http://JP_ontology.org/assessment/MCQ122AnswerB">
        <rdf:type rdf:resource="http://JP_ontology.org/assessment/MCQ.122"/>
        <skos:altLabel xml:lang="en">(ii)</skos:altLabel>
        <skos:definition xml:lang="en">Some efforts are made to plan and agree upon audit tests and assurance activities, but there are inconsistencies or gaps in the process, resulting in limited effectiveness in assessing operational systems.</skos:definition>
        <skos:prefLabel xml:lang="en">MCQ.122 - Partially Implemented</skos:prefLabel>
    </owl:NamedIndividual>
    


    <!-- http://JP_ontology.org/assessment/MCQ122AnswerC -->


    <owl:NamedIndividual rdf:about="http://JP_ontology.org/assessment/MCQ122AnswerC">
        <rdf:type rdf:resource="http://JP_ontology.org/assessment/MCQ.122"/>
        <skos:altLabel xml:lang="en">(iii)</skos:altLabel>
        <skos:definition xml:lang="en">The organisation systematically plans and agrees upon audit tests and assurance activities involving the assessment of operational systems between testers and appropriate management. This ensures a structured and coordinated approach, leading to effective assessment and improvement of operational systems.
	</skos:definition>
        <skos:prefLabel xml:lang="en">MCQ.122 - Fully Implemented</skos:prefLabel>
    </owl:NamedIndividual>
    


    <!-- http://JP_ontology.org/assessment/MCQ123AnswerA -->


    <owl:NamedIndividual rdf:about="http://JP_ontology.org/assessment/MCQ123AnswerA">
        <rdf:type rdf:resource="http://JP_ontology.org/assessment/MCQ.123"/>
        <skos:altLabel xml:lang="en">(i)</skos:altLabel>
        <skos:definition xml:lang="en">The organisation lacks procedures to protect intellectual property rights, leading to potential infringement and loss of valuable assets.</skos:definition>
        <skos:prefLabel xml:lang="en">MCQ.123 - Not Implemented</skos:prefLabel>
    </owl:NamedIndividual>
    


    <!-- http://JP_ontology.org/assessment/MCQ123AnswerB -->


    <owl:NamedIndividual rdf:about="http://JP_ontology.org/assessment/MCQ123AnswerB">
        <rdf:type rdf:resource="http://JP_ontology.org/assessment/MCQ.123"/>
        <skos:altLabel xml:lang="en">(ii)</skos:altLabel>
        <skos:definition xml:lang="en">Some procedures are implemented to protect intellectual property rights, but there are inconsistencies or gaps in their effectiveness, potentially leaving intellectual property vulnerable.</skos:definition>
        <skos:prefLabel xml:lang="en">MCQ.123 - Partially Implemented</skos:prefLabel>
    </owl:NamedIndividual>
    


    <!-- http://JP_ontology.org/assessment/MCQ123AnswerC -->


    <owl:NamedIndividual rdf:about="http://JP_ontology.org/assessment/MCQ123AnswerC">
        <rdf:type rdf:resource="http://JP_ontology.org/assessment/MCQ.123"/>
        <skos:altLabel xml:lang="en">(iii)</skos:altLabel>
        <skos:definition xml:lang="en">The organisation has established and implemented appropriate procedures to protect intellectual property rights effectively, safeguarding valuable assets from infringement or unauthorized use.</skos:definition>
        <skos:prefLabel xml:lang="en">MCQ.123 - Fully Implemented</skos:prefLabel>
    </owl:NamedIndividual>
    


    <!-- http://JP_ontology.org/assessment/MCQ124AnswerA -->


    <owl:NamedIndividual rdf:about="http://JP_ontology.org/assessment/MCQ124AnswerA">
        <rdf:type rdf:resource="http://JP_ontology.org/assessment/MCQ.124"/>
        <skos:altLabel xml:lang="en">(i)</skos:altLabel>
        <skos:definition xml:lang="en">The organisation lacks measures to protect records, leading to risks such as loss, destruction, falsification, unauthorized access, and unauthorized release.</skos:definition>
        <skos:prefLabel xml:lang="en">MCQ.124 - Not Implemented</skos:prefLabel>
    </owl:NamedIndividual>
    


    <!-- http://JP_ontology.org/assessment/MCQ124AnswerB -->


    <owl:NamedIndividual rdf:about="http://JP_ontology.org/assessment/MCQ124AnswerB">
        <rdf:type rdf:resource="http://JP_ontology.org/assessment/MCQ.124"/>
        <skos:altLabel xml:lang="en">(ii)</skos:altLabel>
        <skos:definition xml:lang="en">Some measures are in place to protect records, but there are inconsistencies or gaps in ensuring comprehensive protection from risks such as loss, destruction, falsification, unauthorized access, and unauthorized release.</skos:definition>
        <skos:prefLabel xml:lang="en">MCQ.124 - Partially Implemented</skos:prefLabel>
    </owl:NamedIndividual>
    


    <!-- http://JP_ontology.org/assessment/MCQ124AnswerC -->


    <owl:NamedIndividual rdf:about="http://JP_ontology.org/assessment/MCQ124AnswerC">
        <rdf:type rdf:resource="http://JP_ontology.org/assessment/MCQ.124"/>
        <skos:altLabel xml:lang="en">(iii)</skos:altLabel>
        <skos:definition xml:lang="en">The organisation has established and implemented robust measures to protect records effectively from risks such as loss, destruction, falsification, unauthorized access, and unauthorized release, ensuring the integrity and confidentiality of sensitive information.</skos:definition>
        <skos:prefLabel xml:lang="en">MCQ.124 - Fully Implemented</skos:prefLabel>
    </owl:NamedIndividual>
    


    <!-- http://JP_ontology.org/assessment/MCQ125AnswerA -->


    <owl:NamedIndividual rdf:about="http://JP_ontology.org/assessment/MCQ125AnswerA">
        <rdf:type rdf:resource="http://JP_ontology.org/assessment/MCQ.125"/>
        <skos:altLabel xml:lang="en">(i)</skos:altLabel>
        <skos:definition xml:lang="en">The organisation lacks established rules for secure development of software and systems, leading to potential security vulnerabilities.</skos:definition>
        <skos:prefLabel xml:lang="en">MCQ.125 - Not Implemented</skos:prefLabel>
    </owl:NamedIndividual>
    


    <!-- http://JP_ontology.org/assessment/MCQ125AnswerB -->


    <owl:NamedIndividual rdf:about="http://JP_ontology.org/assessment/MCQ125AnswerB">
        <rdf:type rdf:resource="http://JP_ontology.org/assessment/MCQ.125"/>
        <skos:altLabel xml:lang="en">(ii)</skos:altLabel>
        <skos:definition xml:lang="en">Some rules for secure development are established, but there are inconsistencies or gaps in their application, potentially resulting in security risks.</skos:definition>
        <skos:prefLabel xml:lang="en">MCQ.125 - Partially Implemented</skos:prefLabel>
    </owl:NamedIndividual>
    


    <!-- http://JP_ontology.org/assessment/MCQ125AnswerC -->


    <owl:NamedIndividual rdf:about="http://JP_ontology.org/assessment/MCQ125AnswerC">
        <rdf:type rdf:resource="http://JP_ontology.org/assessment/MCQ.125"/>
        <skos:altLabel xml:lang="en">(iii)</skos:altLabel>
        <skos:definition xml:lang="en">The organisation has established and consistently applies rules for the secure development of software and systems, ensuring that security measures are integrated throughout the development lifecycle to mitigate potential vulnerabilities.</skos:definition>
        <skos:prefLabel xml:lang="en">MCQ.125 - Fully Implemented</skos:prefLabel>
    </owl:NamedIndividual>
    


    <!-- http://JP_ontology.org/assessment/MCQ126AnswerA -->


    <owl:NamedIndividual rdf:about="http://JP_ontology.org/assessment/MCQ126AnswerA">
        <rdf:type rdf:resource="http://JP_ontology.org/assessment/MCQ.126"/>
        <skos:altLabel xml:lang="en">(i)</skos:altLabel>
        <skos:definition xml:lang="en">The organisation does not have a process to identify, specify, and approve information security requirements during application development or acquisition, leading to potential security vulnerabilities.</skos:definition>
        <skos:prefLabel xml:lang="en">MCQ.126 - Not Implemented</skos:prefLabel>
    </owl:NamedIndividual>
    


    <!-- http://JP_ontology.org/assessment/MCQ126AnswerB -->


    <owl:NamedIndividual rdf:about="http://JP_ontology.org/assessment/MCQ126AnswerB">
        <rdf:type rdf:resource="http://JP_ontology.org/assessment/MCQ.126"/>
        <skos:altLabel xml:lang="en">(ii)</skos:altLabel>
        <skos:definition xml:lang="en">Some efforts are made to identify, specify, and approve information security requirements, but there are inconsistencies or gaps in the process, potentially resulting in inadequate security measures.</skos:definition>
        <skos:prefLabel xml:lang="en">MCQ.126 - Partially Implemented</skos:prefLabel>
    </owl:NamedIndividual>
    


    <!-- http://JP_ontology.org/assessment/MCQ126AnswerC -->


    <owl:NamedIndividual rdf:about="http://JP_ontology.org/assessment/MCQ126AnswerC">
        <rdf:type rdf:resource="http://JP_ontology.org/assessment/MCQ.126"/>
        <skos:altLabel xml:lang="en">(iii)</skos:altLabel>
        <skos:definition xml:lang="en">The organisation has established and consistently applies a process to identify, specify, and approve information security requirements during application development or acquisition. This ensures that security considerations are integrated into the development or acquisition process to mitigate potential vulnerabilities effectively.

</skos:definition>
        <skos:prefLabel xml:lang="en">MCQ.126 - Fully Implemented</skos:prefLabel>
    </owl:NamedIndividual>
    


    <!-- http://JP_ontology.org/assessment/MCQ127AnswerA -->


    <owl:NamedIndividual rdf:about="http://JP_ontology.org/assessment/MCQ127AnswerA">
        <rdf:type rdf:resource="http://JP_ontology.org/assessment/MCQ.127"/>
        <skos:altLabel xml:lang="en">(i)</skos:altLabel>
        <skos:definition xml:lang="en">The organisation lacks established principles for engineering secure systems and does not document or apply them to information system development activities, leading to potential security vulnerabilities.</skos:definition>
        <skos:prefLabel xml:lang="en">MCQ.127 - Not Implemented</skos:prefLabel>
    </owl:NamedIndividual>
    


    <!-- http://JP_ontology.org/assessment/MCQ127AnswerB -->


    <owl:NamedIndividual rdf:about="http://JP_ontology.org/assessment/MCQ127AnswerB">
        <rdf:type rdf:resource="http://JP_ontology.org/assessment/MCQ.127"/>
        <skos:altLabel xml:lang="en">(ii)</skos:altLabel>
        <skos:definition xml:lang="en">Some principles for engineering secure systems are established, but there are inconsistencies or gaps in their documentation, maintenance, or application to information system development activities.</skos:definition>
        <skos:prefLabel xml:lang="en">MCQ.127 - Partially Implemented</skos:prefLabel>
    </owl:NamedIndividual>
    


    <!-- http://JP_ontology.org/assessment/MCQ127AnswerC -->


    <owl:NamedIndividual rdf:about="http://JP_ontology.org/assessment/MCQ127AnswerC">
        <rdf:type rdf:resource="http://JP_ontology.org/assessment/MCQ.127"/>
        <skos:altLabel xml:lang="en">(iii)</skos:altLabel>
        <skos:definition xml:lang="en">The organisation has established, documented, maintained, and consistently applies principles for engineering secure systems to all information system development activities. This ensures that security is integrated throughout the development process, mitigating potential vulnerabilities effectively.</skos:definition>
        <skos:prefLabel xml:lang="en">MCQ.127 - Fully Implemented</skos:prefLabel>
    </owl:NamedIndividual>
    


    <!-- http://JP_ontology.org/assessment/MCQ128AnswerA -->


    <owl:NamedIndividual rdf:about="http://JP_ontology.org/assessment/MCQ128AnswerA">
        <rdf:type rdf:resource="http://JP_ontology.org/assessment/MCQ.128"/>
        <skos:altLabel xml:lang="en">(i)</skos:altLabel>
        <skos:definition xml:lang="en">The organisation lacks a structured approach to direct, monitor, and review outsourced system development activities, leading to potential risks and inefficiencies.</skos:definition>
        <skos:prefLabel xml:lang="en">MCQ.128 - Not Implemented</skos:prefLabel>
    </owl:NamedIndividual>
    


    <!-- http://JP_ontology.org/assessment/MCQ128AnswerB -->


    <owl:NamedIndividual rdf:about="http://JP_ontology.org/assessment/MCQ128AnswerB">
        <rdf:type rdf:resource="http://JP_ontology.org/assessment/MCQ.128"/>
        <skos:altLabel xml:lang="en">(ii)</skos:altLabel>
        <skos:definition xml:lang="en">Some efforts are made to direct, monitor, and review outsourced system development activities, but there are inconsistencies or gaps in the process, potentially resulting in inadequate oversight.</skos:definition>
        <skos:prefLabel xml:lang="en">MCQ.128 - Partially Implemented</skos:prefLabel>
    </owl:NamedIndividual>
    


    <!-- http://JP_ontology.org/assessment/MCQ128AnswerC -->


    <owl:NamedIndividual rdf:about="http://JP_ontology.org/assessment/MCQ128AnswerC">
        <rdf:type rdf:resource="http://JP_ontology.org/assessment/MCQ.128"/>
        <skos:altLabel xml:lang="en">(iii)</skos:altLabel>
        <skos:definition xml:lang="en">The organisation has established and consistently applies processes to direct, monitor, and review all activities related to outsourced system development. This ensures that outsourced projects are managed effectively and meet security and quality standards.</skos:definition>
        <skos:prefLabel xml:lang="en">MCQ.128 - Fully Implemented</skos:prefLabel>
    </owl:NamedIndividual>
    


    <!-- http://JP_ontology.org/assessment/MCQ129AnswerA -->


    <owl:NamedIndividual rdf:about="http://JP_ontology.org/assessment/MCQ129AnswerA">
        <rdf:type rdf:resource="http://JP_ontology.org/assessment/MCQ.129"/>
        <skos:altLabel xml:lang="en">(i)</skos:altLabel>
        <skos:definition xml:lang="en">The organisation lacks defined security perimeters to protect areas containing information and associated assets, leading to potential unauthorized access and security breaches.</skos:definition>
        <skos:prefLabel xml:lang="en">MCQ.129 - Not Implemented</skos:prefLabel>
    </owl:NamedIndividual>
    


    <!-- http://JP_ontology.org/assessment/MCQ129AnswerB -->


    <owl:NamedIndividual rdf:about="http://JP_ontology.org/assessment/MCQ129AnswerB">
        <rdf:type rdf:resource="http://JP_ontology.org/assessment/MCQ.129"/>
        <skos:altLabel xml:lang="en">(ii)</skos:altLabel>
        <skos:definition xml:lang="en">Some effort is made to define security perimeters, but there are inconsistencies or gaps in their utilization, potentially leaving areas containing information and assets vulnerable.</skos:definition>
        <skos:prefLabel xml:lang="en">MCQ.129 - Partially Implemented</skos:prefLabel>
    </owl:NamedIndividual>
    


    <!-- http://JP_ontology.org/assessment/MCQ129AnswerC -->


    <owl:NamedIndividual rdf:about="http://JP_ontology.org/assessment/MCQ129AnswerC">
        <rdf:type rdf:resource="http://JP_ontology.org/assessment/MCQ.129"/>
        <skos:altLabel xml:lang="en">(iii)</skos:altLabel>
        <skos:definition xml:lang="en">The organisation has clearly defined security perimeters and consistently utilizes them to protect areas containing information and associated assets. This ensures that unauthorized access is prevented, and information security is maintained effectively.</skos:definition>
        <skos:prefLabel xml:lang="en">MCQ.129 - Fully Implemented</skos:prefLabel>
    </owl:NamedIndividual>
    


    <!-- http://JP_ontology.org/assessment/MCQ12AnswerA -->


    <owl:NamedIndividual rdf:about="http://JP_ontology.org/assessment/MCQ12AnswerA">
        <rdf:type rdf:resource="http://JP_ontology.org/assessment/MCQ.12"/>
        <skos:altLabel xml:lang="en">(i)</skos:altLabel>
        <skos:definition xml:lang="en">Management does not enforce the application of information security in accordance with established policies and procedures, resulting in inconsistent adherence across personnel.</skos:definition>
        <skos:prefLabel xml:lang="en">MCQ.12 - Not Implemented</skos:prefLabel>
    </owl:NamedIndividual>
    


    <!-- http://JP_ontology.org/assessment/MCQ12AnswerB -->


    <owl:NamedIndividual rdf:about="http://JP_ontology.org/assessment/MCQ12AnswerB">
        <rdf:type rdf:resource="http://JP_ontology.org/assessment/MCQ.12"/>
        <skos:altLabel xml:lang="en">(ii)</skos:altLabel>
        <skos:definition xml:lang="en">There are some efforts by management to require personnel to apply information security in accordance with established policies and procedures, but enforcement may be inconsistent or lacking in certain areas.</skos:definition>
        <skos:prefLabel xml:lang="en">MCQ.12 - Partially Implemented</skos:prefLabel>
    </owl:NamedIndividual>
    


    <!-- http://JP_ontology.org/assessment/MCQ12AnswerC -->


    <owl:NamedIndividual rdf:about="http://JP_ontology.org/assessment/MCQ12AnswerC">
        <rdf:type rdf:resource="http://JP_ontology.org/assessment/MCQ.12"/>
        <skos:altLabel xml:lang="en">(iii)</skos:altLabel>
        <skos:definition xml:lang="en">Management consistently requires all personnel to apply information security in strict accordance with the established information security policy, topic-specific policies, and procedures of the organisation, ensuring uniform adherence throughout the organisation.</skos:definition>
        <skos:prefLabel xml:lang="en">MCQ.12 - Fully Implemented</skos:prefLabel>
    </owl:NamedIndividual>
    


    <!-- http://JP_ontology.org/assessment/MCQ130AnswerA -->


    <owl:NamedIndividual rdf:about="http://JP_ontology.org/assessment/MCQ130AnswerA">
        <rdf:type rdf:resource="http://JP_ontology.org/assessment/MCQ.130"/>
        <skos:altLabel xml:lang="en">(i)</skos:altLabel>
        <skos:definition xml:lang="en">The organisation lacks proper maintenance procedures for equipment, leading to potential disruptions in availability and compromises to the integrity and confidentiality of information.</skos:definition>
        <skos:prefLabel xml:lang="en">MCQ.130 - Not Implemented</skos:prefLabel>
    </owl:NamedIndividual>
    


    <!-- http://JP_ontology.org/assessment/MCQ130AnswerB -->


    <owl:NamedIndividual rdf:about="http://JP_ontology.org/assessment/MCQ130AnswerB">
        <rdf:type rdf:resource="http://JP_ontology.org/assessment/MCQ.130"/>
        <skos:altLabel xml:lang="en">(ii)</skos:altLabel>
        <skos:definition xml:lang="en">Some maintenance procedures are in place, but there are inconsistencies or gaps in their implementation, potentially resulting in reduced reliability and security of equipment.</skos:definition>
        <skos:prefLabel xml:lang="en">MCQ.130 - Partially Implemented</skos:prefLabel>
    </owl:NamedIndividual>
    


    <!-- http://JP_ontology.org/assessment/MCQ130AnswerC -->


    <owl:NamedIndividual rdf:about="http://JP_ontology.org/assessment/MCQ130AnswerC">
        <rdf:type rdf:resource="http://JP_ontology.org/assessment/MCQ.130"/>
        <skos:altLabel xml:lang="en">(iii)</skos:altLabel>
        <skos:definition xml:lang="en">The organisation has established and consistently follows maintenance procedures to ensure the availability, integrity, and confidentiality of information by maintaining equipment effectively. This ensures that equipment remains reliable and secure, minimizing disruptions and risks to information security.</skos:definition>
        <skos:prefLabel xml:lang="en">MCQ.130 - Fully Implemented</skos:prefLabel>
    </owl:NamedIndividual>
    


    <!-- http://JP_ontology.org/assessment/MCQ13AnswerA -->


    <owl:NamedIndividual rdf:about="http://JP_ontology.org/assessment/MCQ13AnswerA">
        <rdf:type rdf:resource="http://JP_ontology.org/assessment/MCQ.13"/>
        <skos:altLabel>(i)</skos:altLabel>
        <skos:definition xml:lang="en">The organisation does not have established channels or mechanisms for contacting relevant authorities regarding information security matters.</skos:definition>
        <skos:prefLabel>MCQ13. Not Implemented</skos:prefLabel>
    </owl:NamedIndividual>
    


    <!-- http://JP_ontology.org/assessment/MCQ13AnswerB -->


    <owl:NamedIndividual rdf:about="http://JP_ontology.org/assessment/MCQ13AnswerB">
        <rdf:type rdf:resource="http://JP_ontology.org/assessment/MCQ.13"/>
        <skos:altLabel>(ii)</skos:altLabel>
        <skos:definition xml:lang="en">There are ad-hoc or inconsistent efforts to establish and maintain contact with relevant authorities regarding information security matters, but it lacks a formalized or systematic approach.</skos:definition>
        <skos:prefLabel>MCQ13. Partially Implemented</skos:prefLabel>
    </owl:NamedIndividual>
    


    <!-- http://JP_ontology.org/assessment/MCQ13AnswerC -->


    <owl:NamedIndividual rdf:about="http://JP_ontology.org/assessment/MCQ13AnswerC">
        <rdf:type rdf:resource="http://JP_ontology.org/assessment/MCQ.13"/>
        <skos:altLabel>(iii)</skos:altLabel>
        <skos:definition xml:lang="en">The organisation has well-defined processes and established channels for establishing and maintaining regular contact with relevant authorities regarding information security matters, ensuring timely communication and collaboration.</skos:definition>
        <skos:prefLabel>MCQ13. Fully Implemented</skos:prefLabel>
    </owl:NamedIndividual>
    


    <!-- http://JP_ontology.org/assessment/MCQ14AnswerA -->


    <owl:NamedIndividual rdf:about="http://JP_ontology.org/assessment/MCQ14AnswerA">
        <rdf:type rdf:resource="http://JP_ontology.org/assessment/MCQ.14"/>
        <skos:altLabel>(i)</skos:altLabel>
        <skos:definition xml:lang="en">The organisation does not actively engage or maintain contact with special interest groups, security forums, or professional associations relevant to information security.</skos:definition>
        <skos:prefLabel>MCQ14. Not Implemented</skos:prefLabel>
    </owl:NamedIndividual>
    


    <!-- http://JP_ontology.org/assessment/MCQ14AnswerB -->


    <owl:NamedIndividual rdf:about="http://JP_ontology.org/assessment/MCQ14AnswerB">
        <rdf:type rdf:resource="http://JP_ontology.org/assessment/MCQ.14"/>
        <skos:altLabel>(ii)</skos:altLabel>
        <skos:definition xml:lang="en">There are occasional efforts to establish and maintain contact with special interest groups, security forums, or professional associations, but it lacks a consistent or comprehensive approach.</skos:definition>
        <skos:prefLabel>MCQ14. Partially Implemented</skos:prefLabel>
    </owl:NamedIndividual>
    


    <!-- http://JP_ontology.org/assessment/MCQ14AnswerC -->


    <owl:NamedIndividual rdf:about="http://JP_ontology.org/assessment/MCQ14AnswerC">
        <rdf:type rdf:resource="http://JP_ontology.org/assessment/MCQ.14"/>
        <skos:altLabel>(iii)</skos:altLabel>
        <skos:definition xml:lang="en">The organisation has established and maintains regular contact with various special interest groups, security forums, and professional associations relevant to information security, fostering collaboration and knowledge sharing within the industry.</skos:definition>
        <skos:prefLabel>MCQ14. Fully Implemented</skos:prefLabel>
    </owl:NamedIndividual>
    


    <!-- http://JP_ontology.org/assessment/MCQ15AnswerA -->


    <owl:NamedIndividual rdf:about="http://JP_ontology.org/assessment/MCQ15AnswerA">
        <rdf:type rdf:resource="http://JP_ontology.org/assessment/MCQ.15"/>
        <skos:altLabel>(i)</skos:altLabel>
        <skos:definition xml:lang="en">The organisation does not collect or analyse information relating to information security threats to produce threat intelligence.</skos:definition>
        <skos:prefLabel>MCQ15. Not Implemented</skos:prefLabel>
    </owl:NamedIndividual>
    


    <!-- http://JP_ontology.org/assessment/MCQ15AnswerB -->


    <owl:NamedIndividual rdf:about="http://JP_ontology.org/assessment/MCQ15AnswerB">
        <rdf:type rdf:resource="http://JP_ontology.org/assessment/MCQ.15"/>
        <skos:altLabel>(ii)</skos:altLabel>
        <skos:definition xml:lang="en">There are some efforts to collect and analyse information relating to information security threats, but the process may be inconsistent or incomplete in producing comprehensive threat intelligence.</skos:definition>
        <skos:prefLabel>MCQ15. Partially Implemented</skos:prefLabel>
    </owl:NamedIndividual>
    


    <!-- http://JP_ontology.org/assessment/MCQ15AnswerC -->


    <owl:NamedIndividual rdf:about="http://JP_ontology.org/assessment/MCQ15AnswerC">
        <rdf:type rdf:resource="http://JP_ontology.org/assessment/MCQ.15"/>
        <skos:altLabel>(iii)</skos:altLabel>
        <skos:definition xml:lang="en">The organisation consistently collects and analyses information relating to information security threats to produce comprehensive threat intelligence, enabling proactive measures to mitigate potential risks effectively.</skos:definition>
        <skos:prefLabel>MCQ15. Fully Implemented</skos:prefLabel>
    </owl:NamedIndividual>
    


    <!-- http://JP_ontology.org/assessment/MCQ16AnswerA -->


    <owl:NamedIndividual rdf:about="http://JP_ontology.org/assessment/MCQ16AnswerA">
        <rdf:type rdf:resource="http://JP_ontology.org/assessment/MCQ.16"/>
        <skos:altLabel xml:lang="en">(i)</skos:altLabel>
        <skos:definition xml:lang="en">The organisation does not systematically identify, document, or keep up to date with legal, statutory, regulatory, and contractual requirements relevant to information security, nor does it document its approach to meeting these requirements.</skos:definition>
        <skos:prefLabel xml:lang="en">MCQ.16 - Not Implemented</skos:prefLabel>
    </owl:NamedIndividual>
    


    <!-- http://JP_ontology.org/assessment/MCQ16AnswerB -->


    <owl:NamedIndividual rdf:about="http://JP_ontology.org/assessment/MCQ16AnswerB">
        <rdf:type rdf:resource="http://JP_ontology.org/assessment/MCQ.16"/>
        <skos:altLabel xml:lang="en">(ii)</skos:altLabel>
        <skos:definition xml:lang="en">There are some efforts to identify, document, and keep up to date with legal, statutory, regulatory, and contractual requirements relevant to information security, as well as the organisation’s approach to meeting these requirements, but the process may be inconsistent or incomplete.</skos:definition>
        <skos:prefLabel xml:lang="en">MCQ.16 - Partially Implemented</skos:prefLabel>
    </owl:NamedIndividual>
    


    <!-- http://JP_ontology.org/assessment/MCQ16AnswerC -->


    <owl:NamedIndividual rdf:about="http://JP_ontology.org/assessment/MCQ16AnswerC">
        <rdf:type rdf:resource="http://JP_ontology.org/assessment/MCQ.16"/>
        <skos:altLabel xml:lang="en">(iii)</skos:altLabel>
        <skos:definition xml:lang="en">The organisation systematically identifies, documents, and keeps up to date with legal, statutory, regulatory, and contractual requirements relevant to information security, and its approach to meeting these requirements is well-documented and regularly updated, ensuring compliance with applicable laws and regulations.</skos:definition>
        <skos:prefLabel xml:lang="en">MCQ.16 - Fully Implemented</skos:prefLabel>
    </owl:NamedIndividual>
    


    <!-- http://JP_ontology.org/assessment/MCQ17AnswerA -->


    <owl:NamedIndividual rdf:about="http://JP_ontology.org/assessment/MCQ17AnswerA">
        <rdf:type rdf:resource="http://JP_ontology.org/assessment/MCQ.17"/>
        <skos:altLabel>(i)</skos:altLabel>
        <skos:definition xml:lang="en">Operating procedures for information processing facilities are not documented, and there is no system in place to make them available to personnel who require them.</skos:definition>
        <skos:prefLabel>MCQ17. Not Implemented</skos:prefLabel>
    </owl:NamedIndividual>
    


    <!-- http://JP_ontology.org/assessment/MCQ17AnswerB -->


    <owl:NamedIndividual rdf:about="http://JP_ontology.org/assessment/MCQ17AnswerB">
        <rdf:type rdf:resource="http://JP_ontology.org/assessment/MCQ.17"/>
        <skos:altLabel>(ii)</skos:altLabel>
        <skos:definition xml:lang="en">There are some operating procedures for information processing facilities documented, but access to them may be limited or inconsistent for personnel who require them.</skos:definition>
        <skos:prefLabel>MCQ17. Partially Implemented</skos:prefLabel>
    </owl:NamedIndividual>
    


    <!-- http://JP_ontology.org/assessment/MCQ17AnswerC -->


    <owl:NamedIndividual rdf:about="http://JP_ontology.org/assessment/MCQ17AnswerC">
        <rdf:type rdf:resource="http://JP_ontology.org/assessment/MCQ.17"/>
        <skos:altLabel>(iii)</skos:altLabel>
        <skos:definition xml:lang="en">Operating procedures for information processing facilities are comprehensively documented and readily available to all personnel who require them, ensuring efficient and standardized operations across the organisation.</skos:definition>
        <skos:prefLabel>MCQ17. Fully Implemented</skos:prefLabel>
    </owl:NamedIndividual>
    


    <!-- http://JP_ontology.org/assessment/MCQ18AnswerA -->


    <owl:NamedIndividual rdf:about="http://JP_ontology.org/assessment/MCQ18AnswerA">
        <rdf:type rdf:resource="http://JP_ontology.org/assessment/MCQ.18"/>
        <skos:altLabel xml:lang="en">(i)</skos:altLabel>
        <skos:definition xml:lang="en">The organisation lacks defined information security incident management processes, roles, and responsibilities, and there is no communication regarding incident management preparedness.</skos:definition>
        <skos:prefLabel xml:lang="en">MCQ.18 - Not Implemented</skos:prefLabel>
    </owl:NamedIndividual>
    


    <!-- http://JP_ontology.org/assessment/MCQ18AnswerB -->


    <owl:NamedIndividual rdf:about="http://JP_ontology.org/assessment/MCQ18AnswerB">
        <rdf:type rdf:resource="http://JP_ontology.org/assessment/MCQ.18"/>
        <skos:altLabel xml:lang="en">(ii)</skos:altLabel>
        <skos:definition xml:lang="en">There are some efforts to define and establish information security incident management processes, roles, and responsibilities, but communication regarding incident management preparedness may be inconsistent or incomplete.</skos:definition>
        <skos:prefLabel xml:lang="en">MCQ.18 - Partially Implemented</skos:prefLabel>
    </owl:NamedIndividual>
    


    <!-- http://JP_ontology.org/assessment/MCQ18AnswerC -->


    <owl:NamedIndividual rdf:about="http://JP_ontology.org/assessment/MCQ18AnswerC">
        <rdf:type rdf:resource="http://JP_ontology.org/assessment/MCQ.18"/>
        <skos:altLabel xml:lang="en">(iii)</skos:altLabel>
        <skos:definition xml:lang="en">The organisation has clearly defined, established, and communicated information security incident management processes, roles, and responsibilities, ensuring preparedness for managing incidents effectively.</skos:definition>
        <skos:prefLabel xml:lang="en">MCQ.18 - Fully Implemented</skos:prefLabel>
    </owl:NamedIndividual>
    


    <!-- http://JP_ontology.org/assessment/MCQ19AnswerA -->


    <owl:NamedIndividual rdf:about="http://JP_ontology.org/assessment/MCQ19AnswerA">
        <rdf:type rdf:resource="http://JP_ontology.org/assessment/MCQ.19"/>
        <skos:altLabel xml:lang="en">(i)</skos:altLabel>
        <skos:definition xml:lang="en">The organisation lacks a structured process for assessing information security events to determine if they should be categorized as incidents, leading to inconsistencies and potential oversight.</skos:definition>
        <skos:prefLabel xml:lang="en">MCQ.19 - Not Implemented</skos:prefLabel>
    </owl:NamedIndividual>
    


    <!-- http://JP_ontology.org/assessment/MCQ19AnswerB -->


    <owl:NamedIndividual rdf:about="http://JP_ontology.org/assessment/MCQ19AnswerB">
        <rdf:type rdf:resource="http://JP_ontology.org/assessment/MCQ.19"/>
        <skos:altLabel xml:lang="en">(ii)</skos:altLabel>
        <skos:definition xml:lang="en">There are some efforts to assess information security events to determine if they should be categorized as incidents, but the process may be inconsistent or not fully comprehensive.</skos:definition>
        <skos:prefLabel xml:lang="en">MCQ.19 - Partially Implemented</skos:prefLabel>
    </owl:NamedIndividual>
    


    <!-- http://JP_ontology.org/assessment/MCQ19AnswerC -->


    <owl:NamedIndividual rdf:about="http://JP_ontology.org/assessment/MCQ19AnswerC">
        <rdf:type rdf:resource="http://JP_ontology.org/assessment/MCQ.19"/>
        <skos:altLabel xml:lang="en">(iii)</skos:altLabel>
        <skos:definition xml:lang="en">The organisation has a well-defined and systematic process for assessing information security events to determine if they should be categorized as incidents, ensuring prompt and accurate incident identification and response.</skos:definition>
        <skos:prefLabel xml:lang="en">MCQ.19 - Fully Implemented</skos:prefLabel>
    </owl:NamedIndividual>
    


    <!-- http://JP_ontology.org/assessment/MCQ1AnswerA -->


    <owl:NamedIndividual rdf:about="http://JP_ontology.org/assessment/MCQ1AnswerA">
        <rdf:type rdf:resource="http://JP_ontology.org/assessment/MCQ.1"/>
        <skos:altLabel xml:lang="en">(i)</skos:altLabel>
        <skos:definition xml:lang="en">The organisation does not actively identify external and internal issues relevant to its purpose or their potential impact on achieving the intended outcomes of its information security management system.</skos:definition>
        <skos:prefLabel xml:lang="en">MCQ.1 - Not Implemented</skos:prefLabel>
    </owl:NamedIndividual>
    


    <!-- http://JP_ontology.org/assessment/MCQ1AnswerB -->


    <owl:NamedIndividual rdf:about="http://JP_ontology.org/assessment/MCQ1AnswerB">
        <rdf:type rdf:resource="http://JP_ontology.org/assessment/MCQ.1"/>
        <skos:altLabel xml:lang="en">(ii)</skos:altLabel>
        <skos:definition xml:lang="en">There are some efforts to determine external and internal issues relevant to the organisation&apos;s purpose and their impact on achieving the intended outcomes of its information security management system, but the process may be inconsistent or incomplete.</skos:definition>
        <skos:prefLabel xml:lang="en">MCQ.1 - Partially Implemented</skos:prefLabel>
    </owl:NamedIndividual>
    


    <!-- http://JP_ontology.org/assessment/MCQ1AnswerC -->


    <owl:NamedIndividual rdf:about="http://JP_ontology.org/assessment/MCQ1AnswerC">
        <rdf:type rdf:resource="http://JP_ontology.org/assessment/MCQ.1"/>
        <skos:altLabel xml:lang="en">(iii)</skos:altLabel>
        <skos:definition xml:lang="en">The organisation thoroughly identifies external and internal issues relevant to its purpose and assesses their impact on achieving the intended outcomes of its information security management system, ensuring proactive management and alignment with organisational goals.</skos:definition>
        <skos:prefLabel xml:lang="en">MCQ.1 - Fully Implemented</skos:prefLabel>
    </owl:NamedIndividual>
    


    <!-- http://JP_ontology.org/assessment/MCQ2.1AnswerA -->


    <owl:NamedIndividual rdf:about="http://JP_ontology.org/assessment/MCQ2.1AnswerA">
        <rdf:type rdf:resource="http://JP_ontology.org/assessment/MCQ.2.1"/>
        <skos:altLabel xml:lang="en">(i)</skos:altLabel>
        <skos:definition xml:lang="en">Top management does not establish an information security policy appropriate to the organisation&apos;s purpose, nor does it include information security objectives or commit to satisfying applicable requirements related to information security or continually improving the information security management system.</skos:definition>
        <skos:prefLabel xml:lang="en">MCQ.2.1 - Not Implemented</skos:prefLabel>
    </owl:NamedIndividual>
    


    <!-- http://JP_ontology.org/assessment/MCQ2.1AnswerB -->


    <owl:NamedIndividual rdf:about="http://JP_ontology.org/assessment/MCQ2.1AnswerB">
        <rdf:type rdf:resource="http://JP_ontology.org/assessment/MCQ.2.1"/>
        <skos:altLabel xml:lang="en">(ii)</skos:altLabel>
        <skos:definition xml:lang="en">There are some efforts by top management to establish an information security policy appropriate to the organisation&apos;s purpose, and it may include information security objectives or provide a framework for setting them. However, the commitment to satisfying applicable requirements related to information security and continually improving the information security management system may be inconsistent.</skos:definition>
        <skos:prefLabel xml:lang="en">MCQ.2.1 - Partially Implemented</skos:prefLabel>
    </owl:NamedIndividual>
    


    <!-- http://JP_ontology.org/assessment/MCQ2.1AnswerC -->


    <owl:NamedIndividual rdf:about="http://JP_ontology.org/assessment/MCQ2.1AnswerC">
        <rdf:type rdf:resource="http://JP_ontology.org/assessment/MCQ.2.1"/>
        <skos:altLabel xml:lang="en">(iii)</skos:altLabel>
        <skos:definition xml:lang="en">Top management fully establishes an information security policy appropriate to the organisation&apos;s purpose, which includes information security objectives or provides a framework for setting them. Moreover, there is a clear commitment to satisfying applicable requirements related to information security and continually improving the information security management system.</skos:definition>
        <skos:prefLabel xml:lang="en">MCQ.2.1 - Fully Implemented</skos:prefLabel>
    </owl:NamedIndividual>
    


    <!-- http://JP_ontology.org/assessment/MCQ2.2AnswerA -->


    <owl:NamedIndividual rdf:about="http://JP_ontology.org/assessment/MCQ2.2AnswerA">
        <rdf:type rdf:resource="http://JP_ontology.org/assessment/MCQ.2.2"/>
        <skos:altLabel xml:lang="en">(i)</skos:altLabel>
        <skos:definition xml:lang="en">The information security policy is not available as documented information, nor is it communicated within the organisation or made available to interested parties, potentially leading to lack of awareness and understanding of the organisation&apos;s information security objectives</skos:definition>
        <skos:prefLabel xml:lang="en">MCQ.2.2 - Not Implemented</skos:prefLabel>
    </owl:NamedIndividual>
    


    <!-- http://JP_ontology.org/assessment/MCQ2.2AnswerB -->


    <owl:NamedIndividual rdf:about="http://JP_ontology.org/assessment/MCQ2.2AnswerB">
        <rdf:type rdf:resource="http://JP_ontology.org/assessment/MCQ.2.2"/>
        <skos:altLabel xml:lang="en">(ii)</skos:altLabel>
        <skos:definition xml:lang="en">There are some efforts to make the information security policy available as documented information, and it may be communicated within the organisation to some extent. However, it may not be consistently available to interested parties, leading to potential gaps in awareness.</skos:definition>
        <skos:prefLabel xml:lang="en">MCQ.2.2 - Partially Implemented</skos:prefLabel>
    </owl:NamedIndividual>
    


    <!-- http://JP_ontology.org/assessment/MCQ2.2AnswerC -->


    <owl:NamedIndividual rdf:about="http://JP_ontology.org/assessment/MCQ2.2AnswerC">
        <rdf:type rdf:resource="http://JP_ontology.org/assessment/MCQ.2.2"/>
        <skos:altLabel xml:lang="en">(iii)</skos:altLabel>
        <skos:definition xml:lang="en">The information security policy is fully available as documented information, communicated effectively within the organisation, and made available to interested parties as appropriate, ensuring broad awareness and understanding of the organisation&apos;s information security objectives.</skos:definition>
        <skos:prefLabel xml:lang="en">MCQ.2.2 - Fully Implemented</skos:prefLabel>
    </owl:NamedIndividual>
    


    <!-- http://JP_ontology.org/assessment/MCQ20AnswerA -->


    <owl:NamedIndividual rdf:about="http://JP_ontology.org/assessment/MCQ20AnswerA">
        <rdf:type rdf:resource="http://JP_ontology.org/assessment/MCQ.20"/>
        <skos:altLabel xml:lang="en">(i)</skos:altLabel>
        <skos:definition xml:lang="en">Information security incidents are not responded to in accordance with documented procedures, as there are no established guidelines or protocols for incident response.</skos:definition>
        <skos:prefLabel xml:lang="en">MCQ.20 - Not Implemented</skos:prefLabel>
    </owl:NamedIndividual>
    


    <!-- http://JP_ontology.org/assessment/MCQ20AnswerB -->


    <owl:NamedIndividual rdf:about="http://JP_ontology.org/assessment/MCQ20AnswerB">
        <rdf:type rdf:resource="http://JP_ontology.org/assessment/MCQ.20"/>
        <skos:altLabel xml:lang="en">(ii)</skos:altLabel>
        <skos:definition xml:lang="en">There are some efforts to respond to information security incidents in accordance with documented procedures, but adherence to these procedures may be inconsistent or incomplete.</skos:definition>
        <skos:prefLabel xml:lang="en">MCQ.20 - Partially Implemented</skos:prefLabel>
    </owl:NamedIndividual>
    


    <!-- http://JP_ontology.org/assessment/MCQ20AnswerC -->


    <owl:NamedIndividual rdf:about="http://JP_ontology.org/assessment/MCQ20AnswerC">
        <rdf:type rdf:resource="http://JP_ontology.org/assessment/MCQ.20"/>
        <skos:altLabel xml:lang="en">(iii)</skos:altLabel>
        <skos:definition xml:lang="en">Information security incidents are consistently responded to in strict accordance with documented procedures, ensuring a standardized and effective approach to incident response across the organisation.</skos:definition>
        <skos:prefLabel xml:lang="en">MCQ.20 - Fully Implemented</skos:prefLabel>
    </owl:NamedIndividual>
    


    <!-- http://JP_ontology.org/assessment/MCQ21AnswerA -->


    <owl:NamedIndividual rdf:about="http://JP_ontology.org/assessment/MCQ21AnswerA">
        <rdf:type rdf:resource="http://JP_ontology.org/assessment/MCQ.21"/>
        <skos:altLabel xml:lang="en">(i)</skos:altLabel>
        <skos:definition xml:lang="en">Knowledge gained from information security incidents is not systematically utilized to strengthen or improve information security controls, resulting in missed opportunities for enhancement.</skos:definition>
        <skos:prefLabel xml:lang="en">MCQ.21 - Not Implemented</skos:prefLabel>
    </owl:NamedIndividual>
    


    <!-- http://JP_ontology.org/assessment/MCQ21AnswerB -->


    <owl:NamedIndividual rdf:about="http://JP_ontology.org/assessment/MCQ21AnswerB">
        <rdf:type rdf:resource="http://JP_ontology.org/assessment/MCQ.21"/>
        <skos:altLabel xml:lang="en">(ii)</skos:altLabel>
        <skos:definition xml:lang="en">There are some efforts to utilize knowledge gained from information security incidents to strengthen and improve information security controls, but the process may be inconsistent or not fully comprehensive.</skos:definition>
        <skos:prefLabel xml:lang="en">MCQ.21 - Partially Implemented</skos:prefLabel>
    </owl:NamedIndividual>
    


    <!-- http://JP_ontology.org/assessment/MCQ21AnswerC -->


    <owl:NamedIndividual rdf:about="http://JP_ontology.org/assessment/MCQ21AnswerC">
        <rdf:type rdf:resource="http://JP_ontology.org/assessment/MCQ.21"/>
        <skos:altLabel xml:lang="en">(iii)</skos:altLabel>
        <skos:definition xml:lang="en">Knowledge gained from information security incidents is actively and systematically utilized to strengthen and improve information security controls, facilitating continuous enhancement and adaptation to emerging threats.</skos:definition>
        <skos:prefLabel xml:lang="en">MCQ.21 - Fully Implemented</skos:prefLabel>
    </owl:NamedIndividual>
    


    <!-- http://JP_ontology.org/assessment/MCQ22.1AnswerA -->


    <owl:NamedIndividual rdf:about="http://JP_ontology.org/assessment/MCQ22.1AnswerA">
        <rdf:type rdf:resource="http://JP_ontology.org/assessment/MCQ.22.1"/>
        <skos:altLabel xml:lang="en">(i)</skos:altLabel>
        <skos:definition xml:lang="en">Top management does not establish an information security policy appropriate to the purpose of the organisation, potentially leading to a lack of clear direction and guidance in managing information security.</skos:definition>
        <skos:prefLabel xml:lang="en">MCQ.22.1 - Not Implemented</skos:prefLabel>
    </owl:NamedIndividual>
    


    <!-- http://JP_ontology.org/assessment/MCQ22.1AnswerB -->


    <owl:NamedIndividual rdf:about="http://JP_ontology.org/assessment/MCQ22.1AnswerB">
        <rdf:type rdf:resource="http://JP_ontology.org/assessment/MCQ.22.1"/>
        <skos:altLabel xml:lang="en">(ii)</skos:altLabel>
        <skos:definition xml:lang="en">There are some efforts by top management to establish an information security policy appropriate to the purpose of the organisation. However, the policy may not fully align with the organisation&apos;s objectives or may lack specificity.</skos:definition>
        <skos:prefLabel xml:lang="en">MCQ.22.1 - Partially Implemented</skos:prefLabel>
    </owl:NamedIndividual>
    


    <!-- http://JP_ontology.org/assessment/MCQ22.1AnswerC -->


    <owl:NamedIndividual rdf:about="http://JP_ontology.org/assessment/MCQ22.1AnswerC">
        <rdf:type rdf:resource="http://JP_ontology.org/assessment/MCQ.22.1"/>
        <skos:altLabel xml:lang="en">(iii)</skos:altLabel>
        <skos:definition xml:lang="en">Top management has fully established an information security policy that is appropriate to the purpose of the organisation, providing clear direction and guidance in managing information security in alignment with organisational objectives.</skos:definition>
        <skos:prefLabel xml:lang="en">MCQ.22.1 - Fully Implemented</skos:prefLabel>
    </owl:NamedIndividual>
    


    <!-- http://JP_ontology.org/assessment/MCQ22.2AnswerA -->


    <owl:NamedIndividual rdf:about="http://JP_ontology.org/assessment/MCQ22.2AnswerA">
        <rdf:type rdf:resource="http://JP_ontology.org/assessment/MCQ.22.2"/>
        <skos:altLabel xml:lang="en">(i)</skos:altLabel>
        <skos:definition xml:lang="en">The information security policy does not include information security objectives or provide a framework for setting them, potentially leading to ambiguity and lack of direction in achieving security goals.</skos:definition>
        <skos:prefLabel xml:lang="en">MCQ.22.2 - Not Implemented</skos:prefLabel>
    </owl:NamedIndividual>
    


    <!-- http://JP_ontology.org/assessment/MCQ22.2AnswerB -->


    <owl:NamedIndividual rdf:about="http://JP_ontology.org/assessment/MCQ22.2AnswerB">
        <rdf:type rdf:resource="http://JP_ontology.org/assessment/MCQ.22.2"/>
        <skos:altLabel xml:lang="en">(ii)</skos:altLabel>
        <skos:definition xml:lang="en">There are some efforts to include information security objectives in the information security policy or provide a framework for setting them. However, objectives may not be clearly defined or may lack alignment with organisational goals.</skos:definition>
        <skos:prefLabel xml:lang="en">MCQ.22.2 - Partially Implemented</skos:prefLabel>
    </owl:NamedIndividual>
    


    <!-- http://JP_ontology.org/assessment/MCQ22.2AnswerC -->


    <owl:NamedIndividual rdf:about="http://JP_ontology.org/assessment/MCQ22.2AnswerC">
        <rdf:type rdf:resource="http://JP_ontology.org/assessment/MCQ.22.2"/>
        <skos:altLabel xml:lang="en">(iii)</skos:altLabel>
        <skos:definition xml:lang="en">The information security policy fully includes information security objectives or provides a framework for setting them, ensuring alignment with organisational goals and providing clear direction in achieving security objectives.</skos:definition>
        <skos:prefLabel xml:lang="en">MCQ.22.2 - Fully Implemented</skos:prefLabel>
    </owl:NamedIndividual>
    


    <!-- http://JP_ontology.org/assessment/MCQ22.3AnswerA -->


    <owl:NamedIndividual rdf:about="http://JP_ontology.org/assessment/MCQ22.3AnswerA">
        <rdf:type rdf:resource="http://JP_ontology.org/assessment/MCQ.22.3"/>
        <skos:altLabel xml:lang="en">(i)</skos:altLabel>
        <skos:definition xml:lang="en">The information security policy does not include a commitment to satisfy applicable requirements related to information security, potentially leading to non-compliance and increased security risks.</skos:definition>
        <skos:prefLabel xml:lang="en">MCQ.22.3 - Not Implemented</skos:prefLabel>
    </owl:NamedIndividual>
    


    <!-- http://JP_ontology.org/assessment/MCQ22.3AnswerB -->


    <owl:NamedIndividual rdf:about="http://JP_ontology.org/assessment/MCQ22.3AnswerB">
        <rdf:type rdf:resource="http://JP_ontology.org/assessment/MCQ.22.3"/>
        <skos:altLabel xml:lang="en">(ii)</skos:altLabel>
        <skos:definition xml:lang="en">There are some indications in the information security policy of a commitment to satisfy applicable requirements related to information security. However, this commitment may not be clearly articulated or fully comprehensive.</skos:definition>
        <skos:prefLabel xml:lang="en">MCQ.22.3 - Partially Implemented</skos:prefLabel>
    </owl:NamedIndividual>
    


    <!-- http://JP_ontology.org/assessment/MCQ22.3AnswerC -->


    <owl:NamedIndividual rdf:about="http://JP_ontology.org/assessment/MCQ22.3AnswerC">
        <rdf:type rdf:resource="http://JP_ontology.org/assessment/MCQ.22.3"/>
        <skos:altLabel xml:lang="en">(iii)</skos:altLabel>
        <skos:definition xml:lang="en">The information security policy fully includes a commitment to satisfy applicable requirements related to information security, demonstrating the organisation&apos;s commitment to compliance and proactive management of security risks.</skos:definition>
        <skos:prefLabel xml:lang="en">MCQ.22.3 - Fully Implemented</skos:prefLabel>
    </owl:NamedIndividual>
    


    <!-- http://JP_ontology.org/assessment/MCQ22.4AnswerA -->


    <owl:NamedIndividual rdf:about="http://JP_ontology.org/assessment/MCQ22.4AnswerA">
        <rdf:type rdf:resource="http://JP_ontology.org/assessment/MCQ.22.4"/>
        <skos:altLabel xml:lang="en">(i)</skos:altLabel>
        <skos:definition xml:lang="en">The information security policy does not include a commitment to continual improvement of the information security management system, potentially hindering the organisation&apos;s ability to adapt to evolving security threats and challenges.</skos:definition>
        <skos:prefLabel xml:lang="en">MCQ.22.4 - Not Implemented</skos:prefLabel>
    </owl:NamedIndividual>
    


    <!-- http://JP_ontology.org/assessment/MCQ22.4AnswerB -->


    <owl:NamedIndividual rdf:about="http://JP_ontology.org/assessment/MCQ22.4AnswerB">
        <rdf:type rdf:resource="http://JP_ontology.org/assessment/MCQ.22.4"/>
        <skos:altLabel xml:lang="en">(ii)</skos:altLabel>
        <skos:definition xml:lang="en">There are some indications in the information security policy of a commitment to continual improvement of the information security management system. However, this commitment may not be clearly emphasized or fully integrated into organisational processes.</skos:definition>
        <skos:prefLabel xml:lang="en">MCQ.22.4 - Partially Implemented</skos:prefLabel>
    </owl:NamedIndividual>
    


    <!-- http://JP_ontology.org/assessment/MCQ22.4AnswerC -->


    <owl:NamedIndividual rdf:about="http://JP_ontology.org/assessment/MCQ22.4AnswerC">
        <rdf:type rdf:resource="http://JP_ontology.org/assessment/MCQ.22.4"/>
        <skos:altLabel xml:lang="en">(iii)</skos:altLabel>
        <skos:definition xml:lang="en">The information security policy fully includes a commitment to continual improvement of the information security management system, reflecting the organisation&apos;s proactive stance towards enhancing security processes and practices over time.</skos:definition>
        <skos:prefLabel xml:lang="en">MCQ.22.4 - Fully Implemented</skos:prefLabel>
    </owl:NamedIndividual>
    


    <!-- http://JP_ontology.org/assessment/MCQ22.5AnswerA -->


    <owl:NamedIndividual rdf:about="http://JP_ontology.org/assessment/MCQ22.5AnswerA">
        <rdf:type rdf:resource="http://JP_ontology.org/assessment/MCQ.22.5"/>
        <skos:altLabel xml:lang="en">(i)</skos:altLabel>
        <skos:definition xml:lang="en">The information security policy is not available as documented information, communicated within the organisation, or made available to interested parties, potentially leading to confusion and lack of awareness regarding security expectations.</skos:definition>
        <skos:prefLabel xml:lang="en">MCQ.22.5 - Not Implemented</skos:prefLabel>
    </owl:NamedIndividual>
    


    <!-- http://JP_ontology.org/assessment/MCQ22.5AnswerB -->


    <owl:NamedIndividual rdf:about="http://JP_ontology.org/assessment/MCQ22.5AnswerB">
        <rdf:type rdf:resource="http://JP_ontology.org/assessment/MCQ.22.5"/>
        <skos:altLabel xml:lang="en">(ii)</skos:altLabel>
        <skos:definition xml:lang="en">There are some efforts to make the information security policy available as documented information, communicate it within the organisation, and make it available to interested parties. However, these efforts may be inconsistent or not fully comprehensive.</skos:definition>
        <skos:prefLabel xml:lang="en">MCQ.22.5 - Partially Implemented</skos:prefLabel>
    </owl:NamedIndividual>
    


    <!-- http://JP_ontology.org/assessment/MCQ22.5AnswerC -->


    <owl:NamedIndividual rdf:about="http://JP_ontology.org/assessment/MCQ22.5AnswerC">
        <rdf:type rdf:resource="http://JP_ontology.org/assessment/MCQ.22.5"/>
        <skos:altLabel xml:lang="en">(iii)</skos:altLabel>
        <skos:definition xml:lang="en">The information security policy is fully available as documented information, communicated within the organisation, and made available to interested parties as appropriate, ensuring widespread awareness and understanding of security requirements.</skos:definition>
        <skos:prefLabel xml:lang="en">MCQ.22.5 - Fully Implemented</skos:prefLabel>
    </owl:NamedIndividual>
    


    <!-- http://JP_ontology.org/assessment/MCQ23AnswerA -->


    <owl:NamedIndividual rdf:about="http://JP_ontology.org/assessment/MCQ23AnswerA">
        <rdf:type rdf:resource="http://JP_ontology.org/assessment/MCQ.23"/>
        <skos:altLabel xml:lang="en">(i)</skos:altLabel>
        <skos:definition xml:lang="en">The organisation does not provide a mechanism for personnel to report observed or suspected information security events through appropriate channels, hindering timely detection and response to security incidents.</skos:definition>
        <skos:prefLabel xml:lang="en">MCQ.23 - Not Implemented</skos:prefLabel>
    </owl:NamedIndividual>
    


    <!-- http://JP_ontology.org/assessment/MCQ23AnswerB -->


    <owl:NamedIndividual rdf:about="http://JP_ontology.org/assessment/MCQ23AnswerB">
        <rdf:type rdf:resource="http://JP_ontology.org/assessment/MCQ.23"/>
        <skos:altLabel xml:lang="en">(ii)</skos:altLabel>
        <skos:definition xml:lang="en">There are some efforts to provide a mechanism for personnel to report observed or suspected information security events through appropriate channels, but the process may be inconsistent or not fully comprehensive.</skos:definition>
        <skos:prefLabel xml:lang="en">MCQ.23 - Partially Implemented</skos:prefLabel>
    </owl:NamedIndividual>
    


    <!-- http://JP_ontology.org/assessment/MCQ23AnswerC -->


    <owl:NamedIndividual rdf:about="http://JP_ontology.org/assessment/MCQ23AnswerC">
        <rdf:type rdf:resource="http://JP_ontology.org/assessment/MCQ.23"/>
        <skos:altLabel xml:lang="en">(iii)</skos:altLabel>
        <skos:definition xml:lang="en">The organisation has fully implemented a mechanism for personnel to report observed or suspected information security events through appropriate channels in a timely manner, facilitating prompt detection and response to security incidents.</skos:definition>
        <skos:prefLabel xml:lang="en">MCQ.23 - Fully Implemented</skos:prefLabel>
    </owl:NamedIndividual>
    


    <!-- http://JP_ontology.org/assessment/MCQ24AnswerA -->


    <owl:NamedIndividual rdf:about="http://JP_ontology.org/assessment/MCQ24AnswerA">
        <rdf:type rdf:resource="http://JP_ontology.org/assessment/MCQ.24"/>
        <skos:altLabel xml:lang="en">(i)</skos:altLabel>
        <skos:definition xml:lang="en">Logs that record activities, exceptions, faults, and other relevant events are not produced, stored, protected, or analysed, resulting in a lack of visibility into the organisation&apos;s security posture and potential risks.</skos:definition>
        <skos:prefLabel xml:lang="en">MCQ.24 - Not Implemented</skos:prefLabel>
    </owl:NamedIndividual>
    


    <!-- http://JP_ontology.org/assessment/MCQ24AnswerB -->


    <owl:NamedIndividual rdf:about="http://JP_ontology.org/assessment/MCQ24AnswerB">
        <rdf:type rdf:resource="http://JP_ontology.org/assessment/MCQ.24"/>
        <skos:altLabel xml:lang="en">(ii)</skos:altLabel>
        <skos:definition xml:lang="en">There are some efforts to produce, store, protect, and analyse logs that record activities, exceptions, faults, and other relevant events, but the process may be inconsistent or incomplete.</skos:definition>
        <skos:prefLabel xml:lang="en">MCQ.24 - Partially Implemented</skos:prefLabel>
    </owl:NamedIndividual>
    


    <!-- http://JP_ontology.org/assessment/MCQ24AnswerC -->


    <owl:NamedIndividual rdf:about="http://JP_ontology.org/assessment/MCQ24AnswerC">
        <rdf:type rdf:resource="http://JP_ontology.org/assessment/MCQ.24"/>
        <skos:altLabel xml:lang="en">(iii)</skos:altLabel>
        <skos:definition xml:lang="en">Logs that record activities, exceptions, faults, and other relevant events are fully produced, stored, protected, and analysed, providing comprehensive visibility into the organisation&apos;s security posture and enabling proactive management of security events.</skos:definition>
        <skos:prefLabel xml:lang="en">MCQ.24 - Fully Implemented</skos:prefLabel>
    </owl:NamedIndividual>
    


    <!-- http://JP_ontology.org/assessment/MCQ25AnswerA -->


    <owl:NamedIndividual rdf:about="http://JP_ontology.org/assessment/MCQ25AnswerA">
        <rdf:type rdf:resource="http://JP_ontology.org/assessment/MCQ.25"/>
        <skos:altLabel xml:lang="en">(i)</skos:altLabel>
        <skos:definition xml:lang="en">Networks, systems, and applications are not monitored for anomalous behaviour, and there are no processes in place to evaluate potential information security incidents, leaving the organisation vulnerable to undetected threats.</skos:definition>
        <skos:prefLabel xml:lang="en">MCQ.25 - Not Implemented</skos:prefLabel>
    </owl:NamedIndividual>
    


    <!-- http://JP_ontology.org/assessment/MCQ25AnswerB -->


    <owl:NamedIndividual rdf:about="http://JP_ontology.org/assessment/MCQ25AnswerB">
        <rdf:type rdf:resource="http://JP_ontology.org/assessment/MCQ.25"/>
        <skos:altLabel xml:lang="en">(ii)</skos:altLabel>
        <skos:definition xml:lang="en">There are some efforts to monitor networks, systems, and applications for anomalous behaviour, but the process of evaluating potential information security incidents may be inconsistent or incomplete.</skos:definition>
        <skos:prefLabel xml:lang="en">MCQ.25 - Partially Implemented</skos:prefLabel>
    </owl:NamedIndividual>
    


    <!-- http://JP_ontology.org/assessment/MCQ25AnswerC -->


    <owl:NamedIndividual rdf:about="http://JP_ontology.org/assessment/MCQ25AnswerC">
        <rdf:type rdf:resource="http://JP_ontology.org/assessment/MCQ.25"/>
        <skos:altLabel xml:lang="en">(iii)</skos:altLabel>
        <skos:definition xml:lang="en">Networks, systems, and applications are continuously monitored for anomalous behaviour, and appropriate actions are promptly taken to evaluate potential information security incidents, ensuring timely detection and response to security threats.</skos:definition>
        <skos:prefLabel xml:lang="en">MCQ.25 - Fully Implemented</skos:prefLabel>
    </owl:NamedIndividual>
    


    <!-- http://JP_ontology.org/assessment/MCQ26AnswerA -->


    <owl:NamedIndividual rdf:about="http://JP_ontology.org/assessment/MCQ26AnswerA">
        <rdf:type rdf:resource="http://JP_ontology.org/assessment/MCQ.26"/>
        <skos:altLabel>(i)</skos:altLabel>
        <skos:definition xml:lang="en">The clocks of information processing systems used by the organisation are not synchronized to approved time sources, leading to potential discrepancies in timestamps and challenges in correlation of events.</skos:definition>
        <skos:prefLabel>MCQ26. Not Implemented</skos:prefLabel>
    </owl:NamedIndividual>
    


    <!-- http://JP_ontology.org/assessment/MCQ26AnswerB -->


    <owl:NamedIndividual rdf:about="http://JP_ontology.org/assessment/MCQ26AnswerB">
        <rdf:type rdf:resource="http://JP_ontology.org/assessment/MCQ.26"/>
        <skos:altLabel>(ii)</skos:altLabel>
        <skos:definition xml:lang="en">There are some efforts to synchronize the clocks of information processing systems to approved time sources, but the process may be inconsistent or not fully comprehensive.</skos:definition>
        <skos:prefLabel>MCQ26. Partially Implemented</skos:prefLabel>
    </owl:NamedIndividual>
    


    <!-- http://JP_ontology.org/assessment/MCQ26AnswerC -->


    <owl:NamedIndividual rdf:about="http://JP_ontology.org/assessment/MCQ26AnswerC">
        <rdf:type rdf:resource="http://JP_ontology.org/assessment/MCQ.26"/>
        <skos:altLabel>(iii)</skos:altLabel>
        <skos:definition xml:lang="en">The clocks of information processing systems used by the organisation are fully synchronized to approved time sources, ensuring accurate and consistent timestamps for events across the systems.</skos:definition>
        <skos:prefLabel>MCQ26. Fully Implemented</skos:prefLabel>
    </owl:NamedIndividual>
    


    <!-- http://JP_ontology.org/assessment/MCQ27AnswerA -->


    <owl:NamedIndividual rdf:about="http://JP_ontology.org/assessment/MCQ27AnswerA">
        <rdf:type rdf:resource="http://JP_ontology.org/assessment/MCQ.27"/>
        <skos:altLabel xml:lang="en">(i)</skos:altLabel>
        <skos:definition xml:lang="en">The organisation does not have a plan in place to maintain information security at an appropriate level during disruptions, leaving it vulnerable to potential security breaches during such events.</skos:definition>
        <skos:prefLabel xml:lang="en">MCQ.27 - Not Implemented</skos:prefLabel>
    </owl:NamedIndividual>
    


    <!-- http://JP_ontology.org/assessment/MCQ27AnswerB -->


    <owl:NamedIndividual rdf:about="http://JP_ontology.org/assessment/MCQ27AnswerB">
        <rdf:type rdf:resource="http://JP_ontology.org/assessment/MCQ.27"/>
        <skos:altLabel xml:lang="en">(ii)</skos:altLabel>
        <skos:definition xml:lang="en">There are some efforts to plan for maintaining information security during disruptions, but the plan may be incomplete or not fully comprehensive.</skos:definition>
        <skos:prefLabel xml:lang="en">MCQ.27 - Partially Implemented</skos:prefLabel>
    </owl:NamedIndividual>
    


    <!-- http://JP_ontology.org/assessment/MCQ27AnswerC -->


    <owl:NamedIndividual rdf:about="http://JP_ontology.org/assessment/MCQ27AnswerC">
        <rdf:type rdf:resource="http://JP_ontology.org/assessment/MCQ.27"/>
        <skos:altLabel xml:lang="en">(iii)</skos:altLabel>
        <skos:definition xml:lang="en">The organisation has a comprehensive plan in place to maintain information security at an appropriate level during disruptions, ensuring resilience and continuity of operations even in challenging circumstances.</skos:definition>
        <skos:prefLabel xml:lang="en">MCQ.27 - Fully Implemented</skos:prefLabel>
    </owl:NamedIndividual>
    


    <!-- http://JP_ontology.org/assessment/MCQ28AnswerA -->


    <owl:NamedIndividual rdf:about="http://JP_ontology.org/assessment/MCQ28AnswerA">
        <rdf:type rdf:resource="http://JP_ontology.org/assessment/MCQ.28"/>
        <skos:altLabel xml:lang="en">(i)</skos:altLabel>
        <skos:definition xml:lang="en">ICT readiness is not planned, implemented, maintained, or tested based on business continuity objectives and ICT continuity requirements, leaving the organisation vulnerable to disruptions in ICT services during crises.</skos:definition>
        <skos:prefLabel xml:lang="en">MCQ.28 - Not Implemented</skos:prefLabel>
    </owl:NamedIndividual>
    


    <!-- http://JP_ontology.org/assessment/MCQ28AnswerB -->


    <owl:NamedIndividual rdf:about="http://JP_ontology.org/assessment/MCQ28AnswerB">
        <rdf:type rdf:resource="http://JP_ontology.org/assessment/MCQ.28"/>
        <skos:altLabel xml:lang="en">(ii)</skos:altLabel>
        <skos:definition xml:lang="en">There are some efforts to plan, implement, maintain, and test ICT readiness based on business continuity objectives and ICT continuity requirements, but the process may be inconsistent or not fully comprehensive.</skos:definition>
        <skos:prefLabel xml:lang="en">MCQ.28 - Partially Implemented</skos:prefLabel>
    </owl:NamedIndividual>
    


    <!-- http://JP_ontology.org/assessment/MCQ28AnswerC -->


    <owl:NamedIndividual rdf:about="http://JP_ontology.org/assessment/MCQ28AnswerC">
        <rdf:type rdf:resource="http://JP_ontology.org/assessment/MCQ.28"/>
        <skos:altLabel xml:lang="en">(iii)</skos:altLabel>
        <skos:definition xml:lang="en">ICT readiness is fully planned, implemented, maintained, and tested based on business continuity objectives and ICT continuity requirements, ensuring resilience and continuity of ICT services even during crises.</skos:definition>
        <skos:prefLabel xml:lang="en">MCQ.28 - Fully Implemented</skos:prefLabel>
    </owl:NamedIndividual>
    


    <!-- http://JP_ontology.org/assessment/MCQ29AnswerA -->


    <owl:NamedIndividual rdf:about="http://JP_ontology.org/assessment/MCQ29AnswerA">
        <rdf:type rdf:resource="http://JP_ontology.org/assessment/MCQ.29"/>
        <skos:altLabel>(i)</skos:altLabel>
        <skos:definition xml:lang="en">Operating procedures for information processing facilities are not documented, and there is no system in place to make them available to personnel who require them.</skos:definition>
        <skos:prefLabel>MCQ29. Not Implemented</skos:prefLabel>
    </owl:NamedIndividual>
    


    <!-- http://JP_ontology.org/assessment/MCQ29AnswerB -->


    <owl:NamedIndividual rdf:about="http://JP_ontology.org/assessment/MCQ29AnswerB">
        <rdf:type rdf:resource="http://JP_ontology.org/assessment/MCQ.29"/>
        <skos:altLabel>(ii)</skos:altLabel>
        <skos:definition xml:lang="en">There are some operating procedures for information processing facilities documented, but access to them may be limited or inconsistent for personnel who require them.</skos:definition>
        <skos:prefLabel>MCQ29. Partially Implemented</skos:prefLabel>
    </owl:NamedIndividual>
    


    <!-- http://JP_ontology.org/assessment/MCQ29AnswerC -->


    <owl:NamedIndividual rdf:about="http://JP_ontology.org/assessment/MCQ29AnswerC">
        <rdf:type rdf:resource="http://JP_ontology.org/assessment/MCQ.29"/>
        <skos:altLabel>(iii)</skos:altLabel>
        <skos:definition xml:lang="en">Operating procedures for information processing facilities are comprehensively documented and readily available to all personnel who require them, ensuring efficient and standardized operations across the organisation.</skos:definition>
        <skos:prefLabel>MCQ29. Fully Implemented</skos:prefLabel>
    </owl:NamedIndividual>
    


    <!-- http://JP_ontology.org/assessment/MCQ3.1AnswerA -->


    <owl:NamedIndividual rdf:about="http://JP_ontology.org/assessment/MCQ3.1AnswerA">
        <rdf:type rdf:resource="http://JP_ontology.org/assessment/MCQ.3.1"/>
        <skos:altLabel xml:lang="en">(i)</skos:altLabel>
        <skos:definition xml:lang="en">Top management does not ensure that responsibilities and authorities for roles relevant to information security are assigned and communicated within the organisation, potentially leading to confusion and lack of clarity regarding information security responsibilities.</skos:definition>
        <skos:prefLabel xml:lang="en">MCQ.3.1 - Not Implemented</skos:prefLabel>
    </owl:NamedIndividual>
    


    <!-- http://JP_ontology.org/assessment/MCQ3.1AnswerB -->


    <owl:NamedIndividual rdf:about="http://JP_ontology.org/assessment/MCQ3.1AnswerB">
        <rdf:type rdf:resource="http://JP_ontology.org/assessment/MCQ.3.1"/>
        <skos:altLabel xml:lang="en">(ii)</skos:altLabel>
        <skos:definition xml:lang="en">There are some efforts by top management to ensure that responsibilities and authorities for roles relevant to information security are assigned within the organisation. However, communication of these responsibilities may be inconsistent or not fully comprehensive.</skos:definition>
        <skos:prefLabel xml:lang="en">MCQ.3.1 - Partially Implemented</skos:prefLabel>
    </owl:NamedIndividual>
    


    <!-- http://JP_ontology.org/assessment/MCQ3.1AnswerC -->


    <owl:NamedIndividual rdf:about="http://JP_ontology.org/assessment/MCQ3.1AnswerC">
        <rdf:type rdf:resource="http://JP_ontology.org/assessment/MCQ.3.1"/>
        <skos:altLabel xml:lang="en">(iii)</skos:altLabel>
        <skos:definition xml:lang="en">Top management ensures that responsibilities and authorities for roles relevant to information security are assigned and effectively communicated within the organisation, ensuring clear understanding and accountability for information security responsibilities.</skos:definition>
        <skos:prefLabel xml:lang="en">MCQ.3.1 - Fully Implemented</skos:prefLabel>
    </owl:NamedIndividual>
    


    <!-- http://JP_ontology.org/assessment/MCQ3.2AnswerA -->


    <owl:NamedIndividual rdf:about="http://JP_ontology.org/assessment/MCQ3.2AnswerA">
        <rdf:type rdf:resource="http://JP_ontology.org/assessment/MCQ.3.2"/>
        <skos:altLabel xml:lang="en">(i)</skos:altLabel>
        <skos:definition xml:lang="en">Top management does not assign the responsibility and authority for ensuring that the information security management system conforms to its requirements, nor does it designate responsibility for reporting on the performance of the information security management system to top management, potentially leading to a lack of oversight and accountability</skos:definition>
        <skos:prefLabel xml:lang="en">MCQ.3.2 - Not Implemented</skos:prefLabel>
    </owl:NamedIndividual>
    


    <!-- http://JP_ontology.org/assessment/MCQ3.2AnswerB -->


    <owl:NamedIndividual rdf:about="http://JP_ontology.org/assessment/MCQ3.2AnswerB">
        <rdf:type rdf:resource="http://JP_ontology.org/assessment/MCQ.3.2"/>
        <skos:altLabel xml:lang="en">(ii)</skos:altLabel>
        <skos:definition xml:lang="en">There are some efforts by top management to assign the responsibility and authority for ensuring that the information security management system conforms to its requirements, and reporting on its performance to top management. However, the assignment of responsibilities and reporting mechanisms may be inconsistent or not fully comprehensive.</skos:definition>
        <skos:prefLabel xml:lang="en">MCQ.3.2 - Partially Implemented</skos:prefLabel>
    </owl:NamedIndividual>
    


    <!-- http://JP_ontology.org/assessment/MCQ3.2AnswerC -->


    <owl:NamedIndividual rdf:about="http://JP_ontology.org/assessment/MCQ3.2AnswerC">
        <rdf:type rdf:resource="http://JP_ontology.org/assessment/MCQ.3.2"/>
        <skos:altLabel xml:lang="en">(iii)</skos:altLabel>
        <skos:definition xml:lang="en">Top management fully assigns the responsibility and authority for ensuring that the information security management system conforms to its requirements, and designates responsibility for reporting on its performance to top management, ensuring effective oversight and accountability for information security management.</skos:definition>
        <skos:prefLabel xml:lang="en">MCQ.3.2 - Fully Implemented</skos:prefLabel>
    </owl:NamedIndividual>
    


    <!-- http://JP_ontology.org/assessment/MCQ30AnswerA -->


    <owl:NamedIndividual rdf:about="http://JP_ontology.org/assessment/MCQ30AnswerA">
        <rdf:type rdf:resource="http://JP_ontology.org/assessment/MCQ.30"/>
        <skos:altLabel>(i)</skos:altLabel>
        <skos:definition xml:lang="en">Information processing facilities are not protected from power failures and other disruptions caused by failures in supporting utilities, leaving them vulnerable to potential downtime and data loss.</skos:definition>
        <skos:prefLabel>MCQ30. Not Implemented</skos:prefLabel>
    </owl:NamedIndividual>
    


    <!-- http://JP_ontology.org/assessment/MCQ30AnswerB -->


    <owl:NamedIndividual rdf:about="http://JP_ontology.org/assessment/MCQ30AnswerB">
        <rdf:type rdf:resource="http://JP_ontology.org/assessment/MCQ.30"/>
        <skos:altLabel>(ii)</skos:altLabel>
        <skos:definition xml:lang="en">There are some efforts to protect information processing facilities from power failures and other disruptions caused by failures in supporting utilities, but the protection measures may be inconsistent or incomplete.</skos:definition>
        <skos:prefLabel>MCQ30. Partially Implemented</skos:prefLabel>
    </owl:NamedIndividual>
    


    <!-- http://JP_ontology.org/assessment/MCQ30AnswerC -->


    <owl:NamedIndividual rdf:about="http://JP_ontology.org/assessment/MCQ30AnswerC">
        <rdf:type rdf:resource="http://JP_ontology.org/assessment/MCQ.30"/>
        <skos:altLabel>(iii)</skos:altLabel>
        <skos:definition xml:lang="en">Information processing facilities are fully protected from power failures and other disruptions caused by failures in supporting utilities, ensuring uninterrupted operation and data integrity even during utility failures.</skos:definition>
        <skos:prefLabel>MCQ30. Fully Implemented</skos:prefLabel>
    </owl:NamedIndividual>
    


    <!-- http://JP_ontology.org/assessment/MCQ31AnswerA -->


    <owl:NamedIndividual rdf:about="http://JP_ontology.org/assessment/MCQ31AnswerA">
        <rdf:type rdf:resource="http://JP_ontology.org/assessment/MCQ.31"/>
        <skos:altLabel xml:lang="en">(i)</skos:altLabel>
        <skos:definition xml:lang="en">The use of resources is not monitored, and there are no adjustments made in line with current and expected capacity requirements, leading to potential inefficiencies and resource shortages.</skos:definition>
        <skos:prefLabel xml:lang="en">MCQ.31 - Not Implemented</skos:prefLabel>
    </owl:NamedIndividual>
    


    <!-- http://JP_ontology.org/assessment/MCQ31AnswerB -->


    <owl:NamedIndividual rdf:about="http://JP_ontology.org/assessment/MCQ31AnswerB">
        <rdf:type rdf:resource="http://JP_ontology.org/assessment/MCQ.31"/>
        <skos:altLabel xml:lang="en">(ii)</skos:altLabel>
        <skos:definition xml:lang="en">There are some efforts to monitor the use of resources and make adjustments based on current and expected capacity requirements, but the process may be inconsistent or not fully comprehensive.</skos:definition>
        <skos:prefLabel xml:lang="en">MCQ.31 - Partially Implemented</skos:prefLabel>
    </owl:NamedIndividual>
    


    <!-- http://JP_ontology.org/assessment/MCQ31AnswerC -->


    <owl:NamedIndividual rdf:about="http://JP_ontology.org/assessment/MCQ31AnswerC">
        <rdf:type rdf:resource="http://JP_ontology.org/assessment/MCQ.31"/>
        <skos:altLabel xml:lang="en">(iii)</skos:altLabel>
        <skos:definition xml:lang="en">The use of resources is consistently monitored, and adjustments are promptly made in line with current and expected capacity requirements, ensuring optimal resource utilization and performance.</skos:definition>
        <skos:prefLabel xml:lang="en">MCQ.31 - Fully Implemented</skos:prefLabel>
    </owl:NamedIndividual>
    


    <!-- http://JP_ontology.org/assessment/MCQ32AnswerA -->


    <owl:NamedIndividual rdf:about="http://JP_ontology.org/assessment/MCQ32AnswerA">
        <rdf:type rdf:resource="http://JP_ontology.org/assessment/MCQ.32"/>
        <skos:altLabel xml:lang="en">(i)</skos:altLabel>
        <skos:definition xml:lang="en">Backup copies of information, software, and systems are not maintained, and there is no regular testing conducted in accordance with the agreed topic-specific policy on backup, posing risks of data loss and system downtime.</skos:definition>
        <skos:prefLabel xml:lang="en">MCQ.32 - Not Implemented</skos:prefLabel>
    </owl:NamedIndividual>
    


    <!-- http://JP_ontology.org/assessment/MCQ32AnswerB -->


    <owl:NamedIndividual rdf:about="http://JP_ontology.org/assessment/MCQ32AnswerB">
        <rdf:type rdf:resource="http://JP_ontology.org/assessment/MCQ.32"/>
        <skos:altLabel xml:lang="en">(ii)</skos:altLabel>
        <skos:definition xml:lang="en">There are some efforts to maintain backup copies of information, software, and systems, and occasional testing is conducted, but the process may be inconsistent or not fully aligned with the agreed topic-specific policy on backup.</skos:definition>
        <skos:prefLabel xml:lang="en">MCQ.32 - Partially Implemented</skos:prefLabel>
    </owl:NamedIndividual>
    


    <!-- http://JP_ontology.org/assessment/MCQ32AnswerC -->


    <owl:NamedIndividual rdf:about="http://JP_ontology.org/assessment/MCQ32AnswerC">
        <rdf:type rdf:resource="http://JP_ontology.org/assessment/MCQ.32"/>
        <skos:altLabel xml:lang="en">(iii)</skos:altLabel>
        <skos:definition xml:lang="en">Backup copies of information, software, and systems are consistently maintained and regularly tested in accordance with the agreed topic-specific policy on backup, ensuring data integrity and system availability in the event of disruptions.</skos:definition>
        <skos:prefLabel xml:lang="en">MCQ.32 - Fully Implemented</skos:prefLabel>
    </owl:NamedIndividual>
    


    <!-- http://JP_ontology.org/assessment/MCQ33AnswerA -->


    <owl:NamedIndividual rdf:about="http://JP_ontology.org/assessment/MCQ33AnswerA">
        <rdf:type rdf:resource="http://JP_ontology.org/assessment/MCQ.33"/>
        <skos:altLabel>(i)</skos:altLabel>
        <skos:definition xml:lang="en">Information processing facilities lack redundancy and are unable to meet availability requirements, posing risks of downtime and service interruptions.</skos:definition>
        <skos:prefLabel>MCQ33. Not Implemented</skos:prefLabel>
    </owl:NamedIndividual>
    


    <!-- http://JP_ontology.org/assessment/MCQ33AnswerB -->


    <owl:NamedIndividual rdf:about="http://JP_ontology.org/assessment/MCQ33AnswerB">
        <rdf:type rdf:resource="http://JP_ontology.org/assessment/MCQ.33"/>
        <skos:altLabel>(ii)</skos:altLabel>
        <skos:definition xml:lang="en">There are some redundancy measures implemented in information processing facilities, but they may not be sufficient to fully meet availability requirements, leading to potential disruptions in service.</skos:definition>
        <skos:prefLabel>MCQ33. Partially Implemented</skos:prefLabel>
    </owl:NamedIndividual>
    


    <!-- http://JP_ontology.org/assessment/MCQ33AnswerC -->


    <owl:NamedIndividual rdf:about="http://JP_ontology.org/assessment/MCQ33AnswerC">
        <rdf:type rdf:resource="http://JP_ontology.org/assessment/MCQ.33"/>
        <skos:altLabel>(iii)</skos:altLabel>
        <skos:definition xml:lang="en">Information processing facilities are implemented with redundancy measures that are sufficient to meet availability requirements, ensuring continuous operation and minimal downtime.</skos:definition>
        <skos:prefLabel>MCQ33. Fully Implemented</skos:prefLabel>
    </owl:NamedIndividual>
    


    <!-- http://JP_ontology.org/assessment/MCQ34.1AnswerA -->


    <owl:NamedIndividual rdf:about="http://JP_ontology.org/assessment/MCQ34.1AnswerA">
        <rdf:type rdf:resource="http://JP_ontology.org/assessment/MCQ.34.1"/>
        <skos:altLabel xml:lang="en">(i)</skos:altLabel>
        <skos:definition xml:lang="en">The organisation is not planning, implementing, and controlling processes to meet requirements and implement actions by establishing criteria for the processes and implementing control. This lack of control may result in inconsistent or ineffective processes.</skos:definition>
        <skos:prefLabel xml:lang="en">MCQ.34.1 - Not Implemented</skos:prefLabel>
    </owl:NamedIndividual>
    


    <!-- http://JP_ontology.org/assessment/MCQ34.1AnswerB -->


    <owl:NamedIndividual rdf:about="http://JP_ontology.org/assessment/MCQ34.1AnswerB">
        <rdf:type rdf:resource="http://JP_ontology.org/assessment/MCQ.34.1"/>
        <skos:altLabel xml:lang="en">(ii)</skos:altLabel>
        <skos:definition xml:lang="en">There are some efforts by the organisation to plan, implement, and control processes to meet requirements and implement actions by establishing criteria for the processes and implementing control. However, these efforts may be inconsistent or not fully comprehensive.</skos:definition>
        <skos:prefLabel xml:lang="en">MCQ.34.1 - Partially Implemented</skos:prefLabel>
    </owl:NamedIndividual>
    


    <!-- http://JP_ontology.org/assessment/MCQ34.1AnswerC -->


    <owl:NamedIndividual rdf:about="http://JP_ontology.org/assessment/MCQ34.1AnswerC">
        <rdf:type rdf:resource="http://JP_ontology.org/assessment/MCQ.34.1"/>
        <skos:altLabel xml:lang="en">(iii)</skos:altLabel>
        <skos:definition xml:lang="en">The organisation has fully planned, implemented, and controlled processes to meet requirements and implement actions by establishing criteria for the processes and implementing control. This ensures consistent and effective implementation of processes to meet organisational requirements.</skos:definition>
        <skos:prefLabel xml:lang="en">MCQ.34.1 - Fully Implemented</skos:prefLabel>
    </owl:NamedIndividual>
    


    <!-- http://JP_ontology.org/assessment/MCQ34.2AnswerA -->


    <owl:NamedIndividual rdf:about="http://JP_ontology.org/assessment/MCQ34.2AnswerA">
        <rdf:type rdf:resource="http://JP_ontology.org/assessment/MCQ.34.2"/>
        <skos:altLabel xml:lang="en">(i)</skos:altLabel>
        <skos:definition xml:lang="en">Documented information necessary to have confidence that the processes have been carried out as planned is not available, potentially leading to uncertainty and lack of assurance in process implementation.</skos:definition>
        <skos:prefLabel xml:lang="en">MCQ.34.2 - Not Implemented</skos:prefLabel>
    </owl:NamedIndividual>
    


    <!-- http://JP_ontology.org/assessment/MCQ34.2AnswerB -->


    <owl:NamedIndividual rdf:about="http://JP_ontology.org/assessment/MCQ34.2AnswerB">
        <rdf:type rdf:resource="http://JP_ontology.org/assessment/MCQ.34.2"/>
        <skos:altLabel xml:lang="en">(ii)</skos:altLabel>
        <skos:definition xml:lang="en">There are some efforts to make documented information available to the extent necessary to have confidence that the processes have been carried out as planned. However, documentation may be incomplete or not consistently maintained.</skos:definition>
        <skos:prefLabel xml:lang="en">MCQ.34.2 - Partially Implemented</skos:prefLabel>
    </owl:NamedIndividual>
    


    <!-- http://JP_ontology.org/assessment/MCQ34.2AnswerC -->


    <owl:NamedIndividual rdf:about="http://JP_ontology.org/assessment/MCQ34.2AnswerC">
        <rdf:type rdf:resource="http://JP_ontology.org/assessment/MCQ.34.2"/>
        <skos:altLabel xml:lang="en">(iii)</skos:altLabel>
        <skos:definition xml:lang="en">Documented information is fully available to the extent necessary to have confidence that the processes have been carried out as planned, ensuring transparency and accountability in process implementation.</skos:definition>
        <skos:prefLabel xml:lang="en">MCQ.34.2 - Fully Implemented</skos:prefLabel>
    </owl:NamedIndividual>
    


    <!-- http://JP_ontology.org/assessment/MCQ34.3AnswerA -->


    <owl:NamedIndividual rdf:about="http://JP_ontology.org/assessment/MCQ34.3AnswerA">
        <rdf:type rdf:resource="http://JP_ontology.org/assessment/MCQ.34.3"/>
        <skos:altLabel xml:lang="en">(i)</skos:altLabel>
        <skos:definition xml:lang="en">The organisation does not control planned changes and review the consequences of unintended changes, potentially leading to unmanaged risks and adverse effects on operations.</skos:definition>
        <skos:prefLabel xml:lang="en">MCQ.34.3 - Not Implemented</skos:prefLabel>
    </owl:NamedIndividual>
    


    <!-- http://JP_ontology.org/assessment/MCQ34.3AnswerB -->


    <owl:NamedIndividual rdf:about="http://JP_ontology.org/assessment/MCQ34.3AnswerB">
        <rdf:type rdf:resource="http://JP_ontology.org/assessment/MCQ.34.3"/>
        <skos:altLabel xml:lang="en">(ii)</skos:altLabel>
        <skos:definition xml:lang="en">There are some efforts by the organisation to control planned changes and review the consequences of unintended changes. However, these efforts may be inconsistent or not fully comprehensive in mitigating adverse effects.</skos:definition>
        <skos:prefLabel xml:lang="en">MCQ.34.3 - Partially Implemented</skos:prefLabel>
    </owl:NamedIndividual>
    


    <!-- http://JP_ontology.org/assessment/MCQ34.3AnswerC -->


    <owl:NamedIndividual rdf:about="http://JP_ontology.org/assessment/MCQ34.3AnswerC">
        <rdf:type rdf:resource="http://JP_ontology.org/assessment/MCQ.34.3"/>
        <skos:altLabel xml:lang="en">(iii)</skos:altLabel>
        <skos:definition xml:lang="en">The organisation fully controls planned changes and reviews the consequences of unintended changes, taking action to mitigate any adverse effects as necessary, ensuring effective change management and risk mitigation.</skos:definition>
        <skos:prefLabel xml:lang="en">MCQ.34.3 - Fully Implemented</skos:prefLabel>
    </owl:NamedIndividual>
    


    <!-- http://JP_ontology.org/assessment/MCQ34.4AnswerA -->


    <owl:NamedIndividual rdf:about="http://JP_ontology.org/assessment/MCQ34.4AnswerA">
        <rdf:type rdf:resource="http://JP_ontology.org/assessment/MCQ.34.4"/>
        <skos:altLabel xml:lang="en">(i)</skos:altLabel>
        <skos:definition xml:lang="en">The organisation does not ensure that externally provided processes, products, or services relevant to the information security management system are controlled, potentially exposing the organisation to security risks associated with external dependencies.</skos:definition>
        <skos:prefLabel xml:lang="en">MCQ.34.4 - Not Implemented</skos:prefLabel>
    </owl:NamedIndividual>
    


    <!-- http://JP_ontology.org/assessment/MCQ34.4AnswerB -->


    <owl:NamedIndividual rdf:about="http://JP_ontology.org/assessment/MCQ34.4AnswerB">
        <rdf:type rdf:resource="http://JP_ontology.org/assessment/MCQ.34.4"/>
        <skos:altLabel xml:lang="en">(ii)</skos:altLabel>
        <skos:definition xml:lang="en">There are some efforts by the organisation to ensure that externally provided processes, products, or services relevant to the information security management system are controlled. However, these efforts may be inconsistent or not fully comprehensive.</skos:definition>
        <skos:prefLabel xml:lang="en">MCQ.34.4 - Partially Implemented</skos:prefLabel>
    </owl:NamedIndividual>
    


    <!-- http://JP_ontology.org/assessment/MCQ34.4AnswerC -->


    <owl:NamedIndividual rdf:about="http://JP_ontology.org/assessment/MCQ34.4AnswerC">
        <rdf:type rdf:resource="http://JP_ontology.org/assessment/MCQ.34.4"/>
        <skos:altLabel xml:lang="en">(iii)</skos:altLabel>
        <skos:definition xml:lang="en">The organisation fully ensures that externally provided processes, products, or services relevant to the information security management system are controlled, minimizing security risks associated with external dependencies and maintaining the integrity of the management system.</skos:definition>
        <skos:prefLabel xml:lang="en">MCQ.34.4 - Fully Implemented</skos:prefLabel>
    </owl:NamedIndividual>
    


    <!-- http://JP_ontology.org/assessment/MCQ35AnswerA -->


    <owl:NamedIndividual rdf:about="http://JP_ontology.org/assessment/MCQ35AnswerA">
        <rdf:type rdf:resource="http://JP_ontology.org/assessment/MCQ.35"/>
        <skos:altLabel xml:lang="en">(i)</skos:altLabel>
        <skos:definition xml:lang="en">Information security is not integrated into project management, leading to potential security vulnerabilities and risks being overlooked during project implementation.</skos:definition>
        <skos:prefLabel xml:lang="en">MCQ.35 - Not Implemented</skos:prefLabel>
    </owl:NamedIndividual>
    


    <!-- http://JP_ontology.org/assessment/MCQ35AnswerB -->


    <owl:NamedIndividual rdf:about="http://JP_ontology.org/assessment/MCQ35AnswerB">
        <rdf:type rdf:resource="http://JP_ontology.org/assessment/MCQ.35"/>
        <skos:altLabel xml:lang="en">(ii)</skos:altLabel>
        <skos:definition xml:lang="en">There are some efforts to integrate information security into project management, but the integration may be inconsistent or not fully comprehensive across all projects.</skos:definition>
        <skos:prefLabel xml:lang="en">MCQ.35 - Partially Implemented</skos:prefLabel>
    </owl:NamedIndividual>
    


    <!-- http://JP_ontology.org/assessment/MCQ35AnswerC -->


    <owl:NamedIndividual rdf:about="http://JP_ontology.org/assessment/MCQ35AnswerC">
        <rdf:type rdf:resource="http://JP_ontology.org/assessment/MCQ.35"/>
        <skos:altLabel xml:lang="en">(iii)</skos:altLabel>
        <skos:definition xml:lang="en">Information security is fully integrated into project management processes, ensuring that security considerations are addressed throughout the project lifecycle, from initiation to completion.</skos:definition>
        <skos:prefLabel xml:lang="en">MCQ.35 - Fully Implemented</skos:prefLabel>
    </owl:NamedIndividual>
    


    <!-- http://JP_ontology.org/assessment/MCQ36AnswerA -->


    <owl:NamedIndividual rdf:about="http://JP_ontology.org/assessment/MCQ36AnswerA">
        <rdf:type rdf:resource="http://JP_ontology.org/assessment/MCQ.36"/>
        <skos:altLabel xml:lang="en">(i)</skos:altLabel>
        <skos:definition xml:lang="en">Processes and procedures to manage information security risks associated with the use of supplier’s products or services are not defined or implemented, leaving the organisation vulnerable to potential security breaches from third-party sources.</skos:definition>
        <skos:prefLabel xml:lang="en">MCQ.36 - Not Implemented</skos:prefLabel>
    </owl:NamedIndividual>
    


    <!-- http://JP_ontology.org/assessment/MCQ36AnswerB -->


    <owl:NamedIndividual rdf:about="http://JP_ontology.org/assessment/MCQ36AnswerB">
        <rdf:type rdf:resource="http://JP_ontology.org/assessment/MCQ.36"/>
        <skos:altLabel xml:lang="en">(ii)</skos:altLabel>
        <skos:definition xml:lang="en">There are some processes and procedures in place to manage information security risks associated with the use of supplier’s products or services, but they may be incomplete or inconsistently applied</skos:definition>
        <skos:prefLabel xml:lang="en">MCQ.36 - Partially Implemented</skos:prefLabel>
    </owl:NamedIndividual>
    


    <!-- http://JP_ontology.org/assessment/MCQ36AnswerC -->


    <owl:NamedIndividual rdf:about="http://JP_ontology.org/assessment/MCQ36AnswerC">
        <rdf:type rdf:resource="http://JP_ontology.org/assessment/MCQ.36"/>
        <skos:altLabel xml:lang="en">(iii)</skos:altLabel>
        <skos:definition xml:lang="en">Processes and procedures are fully defined and implemented to manage information security risks associated with the use of supplier’s products or services, ensuring thorough assessment and mitigation of potential risks from third-party sources.</skos:definition>
        <skos:prefLabel xml:lang="en">MCQ.36 - Fully Implemented</skos:prefLabel>
    </owl:NamedIndividual>
    


    <!-- http://JP_ontology.org/assessment/MCQ37AnswerA -->


    <owl:NamedIndividual rdf:about="http://JP_ontology.org/assessment/MCQ37AnswerA">
        <rdf:type rdf:resource="http://JP_ontology.org/assessment/MCQ.37"/>
        <skos:altLabel xml:lang="en">(i)</skos:altLabel>
        <skos:definition xml:lang="en">Relevant information security requirements are not established or agreed upon with each supplier based on the type of supplier relationship, leaving the organisation exposed to potential security vulnerabilities from third-party sources.</skos:definition>
        <skos:prefLabel xml:lang="en">MCQ.37 - Not Implemented</skos:prefLabel>
    </owl:NamedIndividual>
    


    <!-- http://JP_ontology.org/assessment/MCQ37AnswerB -->


    <owl:NamedIndividual rdf:about="http://JP_ontology.org/assessment/MCQ37AnswerB">
        <rdf:type rdf:resource="http://JP_ontology.org/assessment/MCQ.37"/>
        <skos:altLabel xml:lang="en">(ii)</skos:altLabel>
        <skos:definition xml:lang="en">There are some efforts to establish and agree upon relevant information security requirements with suppliers based on the type of supplier relationship, but the process may be inconsistent or not fully comprehensive.</skos:definition>
        <skos:prefLabel xml:lang="en">MCQ.37 - Partially Implemented</skos:prefLabel>
    </owl:NamedIndividual>
    


    <!-- http://JP_ontology.org/assessment/MCQ37AnswerC -->


    <owl:NamedIndividual rdf:about="http://JP_ontology.org/assessment/MCQ37AnswerC">
        <rdf:type rdf:resource="http://JP_ontology.org/assessment/MCQ.37"/>
        <skos:altLabel xml:lang="en">(iii)</skos:altLabel>
        <skos:definition xml:lang="en">Relevant information security requirements are fully established and agreed upon with each supplier based on the type of supplier relationship, ensuring alignment with organisational security objectives and mitigation of risks associated with third-party engagements.</skos:definition>
        <skos:prefLabel xml:lang="en">MCQ.37 - Fully Implemented</skos:prefLabel>
    </owl:NamedIndividual>
    


    <!-- http://JP_ontology.org/assessment/MCQ38AnswerA -->


    <owl:NamedIndividual rdf:about="http://JP_ontology.org/assessment/MCQ38AnswerA">
        <rdf:type rdf:resource="http://JP_ontology.org/assessment/MCQ.38"/>
        <skos:altLabel xml:lang="en">(i)</skos:altLabel>
        <skos:definition xml:lang="en">Processes and procedures to manage information security risks associated with the ICT products and services supply chain are not defined or implemented, leaving the organisation vulnerable to potential security breaches from suppliers.</skos:definition>
        <skos:prefLabel xml:lang="en">MCQ.38 - Not Implemented</skos:prefLabel>
    </owl:NamedIndividual>
    


    <!-- http://JP_ontology.org/assessment/MCQ38AnswerB -->


    <owl:NamedIndividual rdf:about="http://JP_ontology.org/assessment/MCQ38AnswerB">
        <rdf:type rdf:resource="http://JP_ontology.org/assessment/MCQ.38"/>
        <skos:altLabel xml:lang="en">(ii)</skos:altLabel>
        <skos:definition xml:lang="en">There are some processes and procedures in place to manage information security risks associated with the ICT products and services supply chain, but they may be incomplete or inconsistently applied.</skos:definition>
        <skos:prefLabel xml:lang="en">MCQ.38 - Partially Implemented</skos:prefLabel>
    </owl:NamedIndividual>
    


    <!-- http://JP_ontology.org/assessment/MCQ38AnswerC -->


    <owl:NamedIndividual rdf:about="http://JP_ontology.org/assessment/MCQ38AnswerC">
        <rdf:type rdf:resource="http://JP_ontology.org/assessment/MCQ.38"/>
        <skos:altLabel xml:lang="en">(iii)</skos:altLabel>
        <skos:definition xml:lang="en">Processes and procedures are fully defined and implemented to manage information security risks associated with the ICT products and services supply chain, ensuring thorough assessment and mitigation of potential risks throughout the supply chain.</skos:definition>
        <skos:prefLabel xml:lang="en">MCQ.38 - Fully Implemented</skos:prefLabel>
    </owl:NamedIndividual>
    


    <!-- http://JP_ontology.org/assessment/MCQ39AnswerA -->


    <owl:NamedIndividual rdf:about="http://JP_ontology.org/assessment/MCQ39AnswerA">
        <rdf:type rdf:resource="http://JP_ontology.org/assessment/MCQ.39"/>
        <skos:altLabel xml:lang="en">(i)</skos:altLabel>
        <skos:definition xml:lang="en">The organisation does not regularly monitor, review, evaluate, or manage change in supplier information security practices and service delivery, potentially exposing the organisation to security risks from suppliers.</skos:definition>
        <skos:prefLabel xml:lang="en">MCQ.39 - Not Implemented</skos:prefLabel>
    </owl:NamedIndividual>
    


    <!-- http://JP_ontology.org/assessment/MCQ39AnswerB -->


    <owl:NamedIndividual rdf:about="http://JP_ontology.org/assessment/MCQ39AnswerB">
        <rdf:type rdf:resource="http://JP_ontology.org/assessment/MCQ.39"/>
        <skos:altLabel xml:lang="en">(ii)</skos:altLabel>
        <skos:definition xml:lang="en">There are some efforts to monitor, review, evaluate, and manage change in supplier information security practices and service delivery, but the process may be inconsistent or not fully comprehensive.</skos:definition>
        <skos:prefLabel xml:lang="en">MCQ.39 - Partially Implemented</skos:prefLabel>
    </owl:NamedIndividual>
    


    <!-- http://JP_ontology.org/assessment/MCQ39AnswerC -->


    <owl:NamedIndividual rdf:about="http://JP_ontology.org/assessment/MCQ39AnswerC">
        <rdf:type rdf:resource="http://JP_ontology.org/assessment/MCQ.39"/>
        <skos:altLabel xml:lang="en">(iii)</skos:altLabel>
        <skos:definition xml:lang="en">The organisation regularly monitors, reviews, evaluates, and manages change in supplier information security practices and service delivery, ensuring ongoing compliance and alignment with organisational security requirements and objectives.</skos:definition>
        <skos:prefLabel xml:lang="en">MCQ.39 - Fully Implemented</skos:prefLabel>
    </owl:NamedIndividual>
    


    <!-- http://JP_ontology.org/assessment/MCQ4.1AnswerA -->


    <owl:NamedIndividual rdf:about="http://JP_ontology.org/assessment/MCQ4.1AnswerA">
        <rdf:type rdf:resource="http://JP_ontology.org/assessment/MCQ.4.1"/>
        <skos:altLabel xml:lang="en">(i)</skos:altLabel>
        <skos:definition xml:lang="en">The organisation does not establish and maintain information security risk criteria, including risk acceptance criteria and criteria for performing information security risk assessments, potentially leading to inconsistent or inadequate risk management practices.</skos:definition>
        <skos:prefLabel xml:lang="en">MCQ.4.1 - Not Implemented</skos:prefLabel>
    </owl:NamedIndividual>
    


    <!-- http://JP_ontology.org/assessment/MCQ4.1AnswerB -->


    <owl:NamedIndividual rdf:about="http://JP_ontology.org/assessment/MCQ4.1AnswerB">
        <rdf:type rdf:resource="http://JP_ontology.org/assessment/MCQ.4.1"/>
        <skos:altLabel xml:lang="en">(ii)</skos:altLabel>
        <skos:definition xml:lang="en">There are some efforts by the organisation to establish and maintain information security risk criteria, including risk acceptance criteria and criteria for performing information security risk assessments. However, these criteria may be inconsistent or not fully comprehensive.</skos:definition>
        <skos:prefLabel xml:lang="en">MCQ.4.1 - Partially Implemented</skos:prefLabel>
    </owl:NamedIndividual>
    


    <!-- http://JP_ontology.org/assessment/MCQ4.1AnswerC -->


    <owl:NamedIndividual rdf:about="http://JP_ontology.org/assessment/MCQ4.1AnswerC">
        <rdf:type rdf:resource="http://JP_ontology.org/assessment/MCQ.4.1"/>
        <skos:altLabel xml:lang="en">(iii)</skos:altLabel>
        <skos:definition xml:lang="en">The organisation fully establishes and maintains information security risk criteria, including clear risk acceptance criteria and criteria for performing information security risk assessments, ensuring consistent and effective risk management practices</skos:definition>
        <skos:prefLabel xml:lang="en">MCQ.4.1 - Fully Implemented</skos:prefLabel>
    </owl:NamedIndividual>
    


    <!-- http://JP_ontology.org/assessment/MCQ4.2AnswerA -->


    <owl:NamedIndividual rdf:about="http://JP_ontology.org/assessment/MCQ4.2AnswerA">
        <rdf:type rdf:resource="http://JP_ontology.org/assessment/MCQ.4.2"/>
        <skos:altLabel xml:lang="en">(i)</skos:altLabel>
        <skos:definition xml:lang="en">The organisation does not ensure that repeated information security risk assessments produce consistent, valid, and comparable results, potentially leading to unreliable risk management decisions.</skos:definition>
        <skos:prefLabel xml:lang="en">MCQ.4.2 - Not Implemented</skos:prefLabel>
    </owl:NamedIndividual>
    


    <!-- http://JP_ontology.org/assessment/MCQ4.2AnswerB -->


    <owl:NamedIndividual rdf:about="http://JP_ontology.org/assessment/MCQ4.2AnswerB">
        <rdf:type rdf:resource="http://JP_ontology.org/assessment/MCQ.4.2"/>
        <skos:altLabel xml:lang="en">(ii)</skos:altLabel>
        <skos:definition xml:lang="en">There are some efforts by the organisation to ensure that repeated information security risk assessments produce consistent, valid, and comparable results. However, the process may be inconsistent or not fully effective.</skos:definition>
        <skos:prefLabel xml:lang="en">MCQ.4.2 - Partially Implemented</skos:prefLabel>
    </owl:NamedIndividual>
    


    <!-- http://JP_ontology.org/assessment/MCQ4.2AnswerC -->


    <owl:NamedIndividual rdf:about="http://JP_ontology.org/assessment/MCQ4.2AnswerC">
        <rdf:type rdf:resource="http://JP_ontology.org/assessment/MCQ.4.2"/>
        <skos:altLabel xml:lang="en">(iii)</skos:altLabel>
        <skos:definition xml:lang="en">The organisation fully ensures that repeated information security risk assessments produce consistent, valid, and comparable results, ensuring reliability and effectiveness in risk management decisions.</skos:definition>
        <skos:prefLabel xml:lang="en">MCQ.4.2 - Fully Implemented</skos:prefLabel>
    </owl:NamedIndividual>
    


    <!-- http://JP_ontology.org/assessment/MCQ4.3AnswerA -->


    <owl:NamedIndividual rdf:about="http://JP_ontology.org/assessment/MCQ4.3AnswerA">
        <rdf:type rdf:resource="http://JP_ontology.org/assessment/MCQ.4.3"/>
        <skos:altLabel xml:lang="en">(i)</skos:altLabel>
        <skos:definition xml:lang="en">The organisation does not effectively identify information security risks, failing to apply the information security risk assessment process to identify risks associated with the loss of confidentiality, integrity, and availability for information within the scope of the information security management system, nor does it consistently identify risk owners.</skos:definition>
        <skos:prefLabel xml:lang="en">MCQ.4.3 - Not Implemented</skos:prefLabel>
    </owl:NamedIndividual>
    


    <!-- http://JP_ontology.org/assessment/MCQ4.3AnswerB -->


    <owl:NamedIndividual rdf:about="http://JP_ontology.org/assessment/MCQ4.3AnswerB">
        <rdf:type rdf:resource="http://JP_ontology.org/assessment/MCQ.4.3"/>
        <skos:altLabel xml:lang="en">(ii)</skos:altLabel>
        <skos:definition xml:lang="en">There are some efforts by the organisation to identify information security risks, including applying the information security risk assessment process to identify risks associated with the loss of confidentiality, integrity, and availability for information within the scope of the information security management system. However, identification of risk owners may be inconsistent or not fully comprehensive.</skos:definition>
        <skos:prefLabel xml:lang="en">MCQ.4.3 - Partially Implemented</skos:prefLabel>
    </owl:NamedIndividual>
    


    <!-- http://JP_ontology.org/assessment/MCQ4.3AnswerC -->


    <owl:NamedIndividual rdf:about="http://JP_ontology.org/assessment/MCQ4.3AnswerC">
        <rdf:type rdf:resource="http://JP_ontology.org/assessment/MCQ.4.3"/>
        <skos:altLabel xml:lang="en">(iii)</skos:altLabel>
        <skos:definition xml:lang="en">The organisation fully identifies information security risks, applying the information security risk assessment process effectively to identify risks associated with the loss of confidentiality, integrity, and availability for information within the scope of the information security management system, and consistently identifies risk owners.</skos:definition>
        <skos:prefLabel xml:lang="en">MCQ.4.3 - Fully Implemented</skos:prefLabel>
    </owl:NamedIndividual>
    


    <!-- http://JP_ontology.org/assessment/MCQ4.4AnswerA -->


    <owl:NamedIndividual rdf:about="http://JP_ontology.org/assessment/MCQ4.4AnswerA">
        <rdf:type rdf:resource="http://JP_ontology.org/assessment/MCQ.4.4"/>
        <skos:altLabel xml:lang="en">(i)</skos:altLabel>
        <skos:definition xml:lang="en">The organisation does not effectively analyse information security risks, failing to assess the potential consequences and realistic likelihood of the occurrence of identified risks, nor does it determine the levels of risk.</skos:definition>
        <skos:prefLabel xml:lang="en">MCQ.4.4 - Not Implemented</skos:prefLabel>
    </owl:NamedIndividual>
    


    <!-- http://JP_ontology.org/assessment/MCQ4.4AnswerB -->


    <owl:NamedIndividual rdf:about="http://JP_ontology.org/assessment/MCQ4.4AnswerB">
        <rdf:type rdf:resource="http://JP_ontology.org/assessment/MCQ.4.4"/>
        <skos:altLabel xml:lang="en">(ii)</skos:altLabel>
        <skos:definition xml:lang="en">There are some efforts by the organisation to analyse information security risks, including assessing the potential consequences and realistic likelihood of the occurrence of identified risks. However, the process may be inconsistent or not fully comprehensive in determining the levels of risk.</skos:definition>
        <skos:prefLabel xml:lang="en">MCQ.4.4 - Partially Implemented</skos:prefLabel>
    </owl:NamedIndividual>
    


    <!-- http://JP_ontology.org/assessment/MCQ4.4AnswerC -->


    <owl:NamedIndividual rdf:about="http://JP_ontology.org/assessment/MCQ4.4AnswerC">
        <rdf:type rdf:resource="http://JP_ontology.org/assessment/MCQ.4.4"/>
        <skos:altLabel xml:lang="en">(iii)</skos:altLabel>
        <skos:definition xml:lang="en">The organisation fully analyses information security risks, effectively assessing the potential consequences and realistic likelihood of the occurrence of identified risks, and determining the levels of risk comprehensively.</skos:definition>
        <skos:prefLabel xml:lang="en">MCQ.4.4 - Fully Implemented</skos:prefLabel>
    </owl:NamedIndividual>
    


    <!-- http://JP_ontology.org/assessment/MCQ4.5AnswerA -->


    <owl:NamedIndividual rdf:about="http://JP_ontology.org/assessment/MCQ4.5AnswerA">
        <rdf:type rdf:resource="http://JP_ontology.org/assessment/MCQ.4.5"/>
        <skos:altLabel xml:lang="en">(i)</skos:altLabel>
        <skos:definition xml:lang="en">The organisation does not effectively evaluate information security risks, failing to compare the results of risk analysis with established risk criteria and prioritize the analysed risks for risk treatment.</skos:definition>
        <skos:prefLabel xml:lang="en">MCQ.4.5 - Not Implemented</skos:prefLabel>
    </owl:NamedIndividual>
    


    <!-- http://JP_ontology.org/assessment/MCQ4.5AnswerB -->


    <owl:NamedIndividual rdf:about="http://JP_ontology.org/assessment/MCQ4.5AnswerB">
        <rdf:type rdf:resource="http://JP_ontology.org/assessment/MCQ.4.5"/>
        <skos:altLabel xml:lang="en">(ii)</skos:altLabel>
        <skos:definition xml:lang="en">There are some efforts by the organisation to evaluate information security risks, including comparing the results of risk analysis with established risk criteria. However, the process may be inconsistent or not fully comprehensive in prioritizing the analysed risks for risk treatment.</skos:definition>
        <skos:prefLabel xml:lang="en">MCQ.4.5 - Partially Implemented</skos:prefLabel>
    </owl:NamedIndividual>
    


    <!-- http://JP_ontology.org/assessment/MCQ4.5AnswerC -->


    <owl:NamedIndividual rdf:about="http://JP_ontology.org/assessment/MCQ4.5AnswerC">
        <rdf:type rdf:resource="http://JP_ontology.org/assessment/MCQ.4.5"/>
        <skos:altLabel xml:lang="en">(iii)</skos:altLabel>
        <skos:definition xml:lang="en">The organisation fully evaluates information security risks, effectively comparing the results of risk analysis with established risk criteria and prioritizing the analysed risks for risk treatment comprehensively.</skos:definition>
        <skos:prefLabel xml:lang="en">MCQ.4.5 - Fully Implemented</skos:prefLabel>
    </owl:NamedIndividual>
    


    <!-- http://JP_ontology.org/assessment/MCQ4.6AnswerA -->


    <owl:NamedIndividual rdf:about="http://JP_ontology.org/assessment/MCQ4.6AnswerA">
        <rdf:type rdf:resource="http://JP_ontology.org/assessment/MCQ.4.6"/>
        <skos:altLabel xml:lang="en">(i)</skos:altLabel>
        <skos:definition xml:lang="en">The organisation does not retain documented information about the information security risk assessment process, potentially leading to difficulties in ensuring accountability and traceability in the risk management process.</skos:definition>
        <skos:prefLabel xml:lang="en">MCQ.4.6 - Not Implemented</skos:prefLabel>
    </owl:NamedIndividual>
    


    <!-- http://JP_ontology.org/assessment/MCQ4.6AnswerB -->


    <owl:NamedIndividual rdf:about="http://JP_ontology.org/assessment/MCQ4.6AnswerB">
        <rdf:type rdf:resource="http://JP_ontology.org/assessment/MCQ.4.6"/>
        <skos:altLabel xml:lang="en">(ii)</skos:altLabel>
        <skos:definition xml:lang="en">There are some efforts by the organisation to retain documented information about the information security risk assessment process. However, the documentation may be incomplete or not consistently maintained.</skos:definition>
        <skos:prefLabel xml:lang="en">MCQ.4.6 - Partially Implemented</skos:prefLabel>
    </owl:NamedIndividual>
    


    <!-- http://JP_ontology.org/assessment/MCQ4.6AnswerC -->


    <owl:NamedIndividual rdf:about="http://JP_ontology.org/assessment/MCQ4.6AnswerC">
        <rdf:type rdf:resource="http://JP_ontology.org/assessment/MCQ.4.6"/>
        <skos:altLabel xml:lang="en">(iii)</skos:altLabel>
        <skos:definition xml:lang="en">The organisation fully retains documented information about the information security risk assessment process, ensuring comprehensive records are maintained to demonstrate accountability and traceability in the risk management process.</skos:definition>
        <skos:prefLabel xml:lang="en">MCQ.4.6 - Fully Implemented</skos:prefLabel>
    </owl:NamedIndividual>
    


    <!-- http://JP_ontology.org/assessment/MCQ40AnswerA -->


    <owl:NamedIndividual rdf:about="http://JP_ontology.org/assessment/MCQ40AnswerA">
        <rdf:type rdf:resource="http://JP_ontology.org/assessment/MCQ.40"/>
        <skos:altLabel xml:lang="en">(i)</skos:altLabel>
        <skos:definition xml:lang="en">Processes for the acquisition, use, management, and exit from cloud services are not established in accordance with the organisation’s information security requirements, posing risks of security breaches and data loss.</skos:definition>
        <skos:prefLabel xml:lang="en">MCQ.40 - Not Implemented</skos:prefLabel>
    </owl:NamedIndividual>
    


    <!-- http://JP_ontology.org/assessment/MCQ40AnswerB -->


    <owl:NamedIndividual rdf:about="http://JP_ontology.org/assessment/MCQ40AnswerB">
        <rdf:type rdf:resource="http://JP_ontology.org/assessment/MCQ.40"/>
        <skos:altLabel xml:lang="en">(ii)</skos:altLabel>
        <skos:definition xml:lang="en">There are some processes established for the acquisition, use, management, and exit from cloud services, but they may not fully align with the organisation’s information security requirements or be consistently applied.</skos:definition>
        <skos:prefLabel xml:lang="en">MCQ.40 - Partially Implemented</skos:prefLabel>
    </owl:NamedIndividual>
    


    <!-- http://JP_ontology.org/assessment/MCQ40AnswerC -->


    <owl:NamedIndividual rdf:about="http://JP_ontology.org/assessment/MCQ40AnswerC">
        <rdf:type rdf:resource="http://JP_ontology.org/assessment/MCQ.40"/>
        <skos:altLabel xml:lang="en">(iii)</skos:altLabel>
        <skos:definition xml:lang="en">Processes are fully established for the acquisition, use, management, and exit from cloud services in accordance with the organisation’s information security requirements, ensuring secure and compliant adoption and operation of cloud services.</skos:definition>
        <skos:prefLabel xml:lang="en">MCQ.40 - Fully Implemented</skos:prefLabel>
    </owl:NamedIndividual>
    


    <!-- http://JP_ontology.org/assessment/MCQ41AnswerA -->


    <owl:NamedIndividual rdf:about="http://JP_ontology.org/assessment/MCQ41AnswerA">
        <rdf:type rdf:resource="http://JP_ontology.org/assessment/MCQ.41"/>
        <skos:altLabel>(i)</skos:altLabel>
        <skos:definition xml:lang="en">Operating procedures for information processing facilities are not documented, and there is no system in place to make them available to personnel who require them.</skos:definition>
        <skos:prefLabel>MCQ41. Not Implemented</skos:prefLabel>
    </owl:NamedIndividual>
    


    <!-- http://JP_ontology.org/assessment/MCQ41AnswerB -->


    <owl:NamedIndividual rdf:about="http://JP_ontology.org/assessment/MCQ41AnswerB">
        <rdf:type rdf:resource="http://JP_ontology.org/assessment/MCQ.41"/>
        <skos:altLabel>(ii)</skos:altLabel>
        <skos:definition xml:lang="en">There are some operating procedures for information processing facilities documented, but access to them may be limited or inconsistent for personnel who require them.</skos:definition>
        <skos:prefLabel>MCQ41. Partially Implemented</skos:prefLabel>
    </owl:NamedIndividual>
    


    <!-- http://JP_ontology.org/assessment/MCQ41AnswerC -->


    <owl:NamedIndividual rdf:about="http://JP_ontology.org/assessment/MCQ41AnswerC">
        <rdf:type rdf:resource="http://JP_ontology.org/assessment/MCQ.41"/>
        <skos:altLabel>(iii)</skos:altLabel>
        <skos:definition xml:lang="en">Operating procedures for information processing facilities are comprehensively documented and readily available to all personnel who require them, ensuring efficient and standardized operations across the organisation.</skos:definition>
        <skos:prefLabel>MCQ41. Fully Implemented</skos:prefLabel>
    </owl:NamedIndividual>
    


    <!-- http://JP_ontology.org/assessment/MCQ42AnswerA -->


    <owl:NamedIndividual rdf:about="http://JP_ontology.org/assessment/MCQ42AnswerA">
        <rdf:type rdf:resource="http://JP_ontology.org/assessment/MCQ.42"/>
        <skos:altLabel xml:lang="en">(i)</skos:altLabel>
        <skos:definition xml:lang="en">The organisation does not acquire information regarding technical vulnerabilities of the information systems in use, evaluate its exposure to such vulnerabilities, or implement appropriate measures, leaving it susceptible to potential security breaches.</skos:definition>
        <skos:prefLabel xml:lang="en">MCQ.42 - Not Implemented</skos:prefLabel>
    </owl:NamedIndividual>
    


    <!-- http://JP_ontology.org/assessment/MCQ42AnswerB -->


    <owl:NamedIndividual rdf:about="http://JP_ontology.org/assessment/MCQ42AnswerB">
        <rdf:type rdf:resource="http://JP_ontology.org/assessment/MCQ.42"/>
        <skos:altLabel xml:lang="en">(ii)</skos:altLabel>
        <skos:definition xml:lang="en">There are some efforts to acquire information regarding technical vulnerabilities and evaluate the organisation’s exposure to such vulnerabilities, but the implementation of appropriate measures may be inconsistent or incomplete.</skos:definition>
        <skos:prefLabel xml:lang="en">MCQ.42 - Partially Implemented</skos:prefLabel>
    </owl:NamedIndividual>
    


    <!-- http://JP_ontology.org/assessment/MCQ42AnswerC -->


    <owl:NamedIndividual rdf:about="http://JP_ontology.org/assessment/MCQ42AnswerC">
        <rdf:type rdf:resource="http://JP_ontology.org/assessment/MCQ.42"/>
        <skos:altLabel xml:lang="en">(iii)</skos:altLabel>
        <skos:definition xml:lang="en">The organisation consistently acquires information regarding technical vulnerabilities of the information systems in use, evaluates its exposure to such vulnerabilities, and implements appropriate measures accordingly, ensuring proactive management of security risks.</skos:definition>
        <skos:prefLabel xml:lang="en">MCQ.42 - Fully Implemented</skos:prefLabel>
    </owl:NamedIndividual>
    


    <!-- http://JP_ontology.org/assessment/MCQ43AnswerA -->


    <owl:NamedIndividual rdf:about="http://JP_ontology.org/assessment/MCQ43AnswerA">
        <rdf:type rdf:resource="http://JP_ontology.org/assessment/MCQ.43"/>
        <skos:altLabel xml:lang="en">(i)</skos:altLabel>
        <skos:definition xml:lang="en">Configurations, including security configurations, of hardware, software, services, and networks are not established, documented, implemented, monitored, or reviewed, leading to potential vulnerabilities and inconsistent security measures.</skos:definition>
        <skos:prefLabel xml:lang="en">MCQ.43 - Not Implemented</skos:prefLabel>
    </owl:NamedIndividual>
    


    <!-- http://JP_ontology.org/assessment/MCQ43AnswerB -->


    <owl:NamedIndividual rdf:about="http://JP_ontology.org/assessment/MCQ43AnswerB">
        <rdf:type rdf:resource="http://JP_ontology.org/assessment/MCQ.43"/>
        <skos:altLabel xml:lang="en">(ii)</skos:altLabel>
        <skos:definition xml:lang="en">There are some efforts to establish, document, implement, monitor, and review configurations, including security configurations, of hardware, software, services, and networks, but the process may be inconsistent or incomplete.</skos:definition>
        <skos:prefLabel xml:lang="en">MCQ.43 - Partially Implemented</skos:prefLabel>
    </owl:NamedIndividual>
    


    <!-- http://JP_ontology.org/assessment/MCQ43AnswerC -->


    <owl:NamedIndividual rdf:about="http://JP_ontology.org/assessment/MCQ43AnswerC">
        <rdf:type rdf:resource="http://JP_ontology.org/assessment/MCQ.43"/>
        <skos:altLabel xml:lang="en">(iii)</skos:altLabel>
        <skos:definition xml:lang="en">Configurations, including security configurations, of hardware, software, services, and networks are fully established, documented, implemented, monitored, and reviewed, ensuring consistent and effective security measures across the organisation.</skos:definition>
        <skos:prefLabel xml:lang="en">MCQ.43 - Fully Implemented</skos:prefLabel>
    </owl:NamedIndividual>
    


    <!-- http://JP_ontology.org/assessment/MCQ44AnswerA -->


    <owl:NamedIndividual rdf:about="http://JP_ontology.org/assessment/MCQ44AnswerA">
        <rdf:type rdf:resource="http://JP_ontology.org/assessment/MCQ.44"/>
        <skos:altLabel xml:lang="en">(i)</skos:altLabel>
        <skos:definition xml:lang="en">Procedures and measures to securely manage software installation on operational systems have not been implemented, potentially leading to unauthorized or insecure software installations.</skos:definition>
        <skos:prefLabel xml:lang="en">MCQ.44 - Not Implemented</skos:prefLabel>
    </owl:NamedIndividual>
    


    <!-- http://JP_ontology.org/assessment/MCQ44AnswerB -->


    <owl:NamedIndividual rdf:about="http://JP_ontology.org/assessment/MCQ44AnswerB">
        <rdf:type rdf:resource="http://JP_ontology.org/assessment/MCQ.44"/>
        <skos:altLabel xml:lang="en">(ii)</skos:altLabel>
        <skos:definition xml:lang="en">There are some procedures and measures in place to securely manage software installation on operational systems, but they may be incomplete or inconsistently applied.</skos:definition>
        <skos:prefLabel xml:lang="en">MCQ.44 - Partially Implemented</skos:prefLabel>
    </owl:NamedIndividual>
    


    <!-- http://JP_ontology.org/assessment/MCQ44AnswerC -->


    <owl:NamedIndividual rdf:about="http://JP_ontology.org/assessment/MCQ44AnswerC">
        <rdf:type rdf:resource="http://JP_ontology.org/assessment/MCQ.44"/>
        <skos:altLabel xml:lang="en">(iii)</skos:altLabel>
        <skos:definition xml:lang="en">Procedures and measures to securely manage software installation on operational systems are fully implemented, ensuring that only authorized and secure software is installed, minimizing security risks.</skos:definition>
        <skos:prefLabel xml:lang="en">MCQ.44 - Fully Implemented</skos:prefLabel>
    </owl:NamedIndividual>
    


    <!-- http://JP_ontology.org/assessment/MCQ45AnswerA -->


    <owl:NamedIndividual rdf:about="http://JP_ontology.org/assessment/MCQ45AnswerA">
        <rdf:type rdf:resource="http://JP_ontology.org/assessment/MCQ.45"/>
        <skos:altLabel xml:lang="en">(i)</skos:altLabel>
        <skos:definition xml:lang="en">Networks and network devices are not secured, managed, or controlled to protect information in systems and applications, leaving the organisation vulnerable to potential security breaches and data compromise.</skos:definition>
        <skos:prefLabel xml:lang="en">MCQ.45 - Not Implemented</skos:prefLabel>
    </owl:NamedIndividual>
    


    <!-- http://JP_ontology.org/assessment/MCQ45AnswerB -->


    <owl:NamedIndividual rdf:about="http://JP_ontology.org/assessment/MCQ45AnswerB">
        <rdf:type rdf:resource="http://JP_ontology.org/assessment/MCQ.45"/>
        <skos:altLabel xml:lang="en">(ii)</skos:altLabel>
        <skos:definition xml:lang="en">There are some efforts to secure, manage, and control networks and network devices to protect information in systems and applications, but the measures may be inconsistent or insufficient in certain areas.</skos:definition>
        <skos:prefLabel xml:lang="en">MCQ.45 - Partially Implemented</skos:prefLabel>
    </owl:NamedIndividual>
    


    <!-- http://JP_ontology.org/assessment/MCQ45AnswerC -->


    <owl:NamedIndividual rdf:about="http://JP_ontology.org/assessment/MCQ45AnswerC">
        <rdf:type rdf:resource="http://JP_ontology.org/assessment/MCQ.45"/>
        <skos:altLabel xml:lang="en">(iii)</skos:altLabel>
        <skos:definition xml:lang="en">Networks and network devices are fully secured, managed, and controlled to protect information in systems and applications, ensuring robust defence against security threats and data breaches.</skos:definition>
        <skos:prefLabel xml:lang="en">MCQ.45 - Fully Implemented</skos:prefLabel>
    </owl:NamedIndividual>
    


    <!-- http://JP_ontology.org/assessment/MCQ46AnswerA -->


    <owl:NamedIndividual rdf:about="http://JP_ontology.org/assessment/MCQ46AnswerA">
        <rdf:type rdf:resource="http://JP_ontology.org/assessment/MCQ.46"/>
        <skos:altLabel xml:lang="en">(i)</skos:altLabel>
        <skos:definition xml:lang="en">Security mechanisms, service levels, and service requirements of network services are not identified, implemented, or monitored, posing risks of security vulnerabilities and service disruptions.</skos:definition>
        <skos:prefLabel xml:lang="en">MCQ.46 - Not Implemented</skos:prefLabel>
    </owl:NamedIndividual>
    


    <!-- http://JP_ontology.org/assessment/MCQ46AnswerB -->


    <owl:NamedIndividual rdf:about="http://JP_ontology.org/assessment/MCQ46AnswerB">
        <rdf:type rdf:resource="http://JP_ontology.org/assessment/MCQ.46"/>
        <skos:altLabel xml:lang="en">(ii)</skos:altLabel>
        <skos:definition xml:lang="en">There are some efforts to identify, implement, and monitor security mechanisms, service levels, and service requirements of network services, but the process may be inconsistent or incomplete.</skos:definition>
        <skos:prefLabel xml:lang="en">MCQ.46 - Partially Implemented</skos:prefLabel>
    </owl:NamedIndividual>
    


    <!-- http://JP_ontology.org/assessment/MCQ46AnswerC -->


    <owl:NamedIndividual rdf:about="http://JP_ontology.org/assessment/MCQ46AnswerC">
        <rdf:type rdf:resource="http://JP_ontology.org/assessment/MCQ.46"/>
        <skos:altLabel xml:lang="en">(iii)</skos:altLabel>
        <skos:definition xml:lang="en">Security mechanisms, service levels, and service requirements of network services are fully identified, implemented, and monitored, ensuring adherence to security standards and optimal performance of network services.</skos:definition>
        <skos:prefLabel xml:lang="en">MCQ.46 - Fully Implemented</skos:prefLabel>
    </owl:NamedIndividual>
    


    <!-- http://JP_ontology.org/assessment/MCQ47AnswerA -->


    <owl:NamedIndividual rdf:about="http://JP_ontology.org/assessment/MCQ47AnswerA">
        <rdf:type rdf:resource="http://JP_ontology.org/assessment/MCQ.47"/>
        <skos:altLabel xml:lang="en">(i)</skos:altLabel>
        <skos:definition xml:lang="en">Segregation is not implemented for groups of information services, users, and information systems within the organisation&apos;s networks, leading to potential risks of unauthorized access and data breaches.</skos:definition>
        <skos:prefLabel xml:lang="en">MCQ.47 - Not Implemented</skos:prefLabel>
    </owl:NamedIndividual>
    


    <!-- http://JP_ontology.org/assessment/MCQ47AnswerB -->


    <owl:NamedIndividual rdf:about="http://JP_ontology.org/assessment/MCQ47AnswerB">
        <rdf:type rdf:resource="http://JP_ontology.org/assessment/MCQ.47"/>
        <skos:altLabel xml:lang="en">(ii)</skos:altLabel>
        <skos:definition xml:lang="en">There are some efforts to implement segregation for groups of information services, users, and information systems within the organisation&apos;s networks, but the implementation may be incomplete or inconsistent.</skos:definition>
        <skos:prefLabel xml:lang="en">MCQ.47 - Partially Implemented</skos:prefLabel>
    </owl:NamedIndividual>
    


    <!-- http://JP_ontology.org/assessment/MCQ47AnswerC -->


    <owl:NamedIndividual rdf:about="http://JP_ontology.org/assessment/MCQ47AnswerC">
        <rdf:type rdf:resource="http://JP_ontology.org/assessment/MCQ.47"/>
        <skos:altLabel xml:lang="en">(iii)</skos:altLabel>
        <skos:definition xml:lang="en">Segregation is fully implemented for groups of information services, users, and information systems within the organisation&apos;s networks, ensuring controlled access and minimizing the impact of security incidents.</skos:definition>
        <skos:prefLabel xml:lang="en">MCQ.47 - Fully Implemented</skos:prefLabel>
    </owl:NamedIndividual>
    


    <!-- http://JP_ontology.org/assessment/MCQ48AnswerA -->


    <owl:NamedIndividual rdf:about="http://JP_ontology.org/assessment/MCQ48AnswerA">
        <rdf:type rdf:resource="http://JP_ontology.org/assessment/MCQ.48"/>
        <skos:altLabel xml:lang="en">(i)</skos:altLabel>
        <skos:definition xml:lang="en">Access to external websites is not managed, exposing the organisation to potential risks from malicious content and cyber threats.</skos:definition>
        <skos:prefLabel xml:lang="en">MCQ.48 - Not Implemented</skos:prefLabel>
    </owl:NamedIndividual>
    


    <!-- http://JP_ontology.org/assessment/MCQ48AnswerB -->


    <owl:NamedIndividual rdf:about="http://JP_ontology.org/assessment/MCQ48AnswerB">
        <rdf:type rdf:resource="http://JP_ontology.org/assessment/MCQ.48"/>
        <skos:altLabel xml:lang="en">(ii)</skos:altLabel>
        <skos:definition xml:lang="en">There are some efforts to manage access to external websites to reduce exposure to malicious content, but the management process may be inconsistent or not fully comprehensive.</skos:definition>
        <skos:prefLabel xml:lang="en">MCQ.48 - Partially Implemented</skos:prefLabel>
    </owl:NamedIndividual>
    


    <!-- http://JP_ontology.org/assessment/MCQ48AnswerC -->


    <owl:NamedIndividual rdf:about="http://JP_ontology.org/assessment/MCQ48AnswerC">
        <rdf:type rdf:resource="http://JP_ontology.org/assessment/MCQ.48"/>
        <skos:altLabel xml:lang="en">(iii)</skos:altLabel>
        <skos:definition xml:lang="en">Access to external websites is fully managed to reduce exposure to malicious content, ensuring proactive protection against cyber threats and maintaining a secure browsing environment for users.</skos:definition>
        <skos:prefLabel xml:lang="en">MCQ.48 - Fully Implemented</skos:prefLabel>
    </owl:NamedIndividual>
    


    <!-- http://JP_ontology.org/assessment/MCQ49.1AnswerA -->


    <owl:NamedIndividual rdf:about="http://JP_ontology.org/assessment/MCQ49.1AnswerA">
        <rdf:type rdf:resource="http://JP_ontology.org/assessment/MCQ.49.1"/>
        <skos:altLabel xml:lang="en">(i)</skos:altLabel>
        <skos:definition xml:lang="en">The organisation does not determine what needs to be monitored and measured, including information security processes and controls, potentially leading to a lack of oversight and inability to assess the effectiveness of security measures.</skos:definition>
        <skos:prefLabel xml:lang="en">MCQ.49.1 - Not Implemented</skos:prefLabel>
    </owl:NamedIndividual>
    


    <!-- http://JP_ontology.org/assessment/MCQ49.1AnswerB -->


    <owl:NamedIndividual rdf:about="http://JP_ontology.org/assessment/MCQ49.1AnswerB">
        <rdf:type rdf:resource="http://JP_ontology.org/assessment/MCQ.49.1"/>
        <skos:altLabel xml:lang="en">(ii)</skos:altLabel>
        <skos:definition xml:lang="en">There are some efforts by the organisation to determine what needs to be monitored and measured, including information security processes and controls. However, this determination may be inconsistent or not fully comprehensive.</skos:definition>
        <skos:prefLabel xml:lang="en">MCQ.49.1 - Partially Implemented</skos:prefLabel>
    </owl:NamedIndividual>
    


    <!-- http://JP_ontology.org/assessment/MCQ49.1AnswerC -->


    <owl:NamedIndividual rdf:about="http://JP_ontology.org/assessment/MCQ49.1AnswerC">
        <rdf:type rdf:resource="http://JP_ontology.org/assessment/MCQ.49.1"/>
        <skos:altLabel xml:lang="en">(iii)</skos:altLabel>
        <skos:definition xml:lang="en">The organisation fully determines what needs to be monitored and measured, including information security processes and controls, ensuring comprehensive oversight and assessment of security measures&apos; effectiveness.</skos:definition>
        <skos:prefLabel xml:lang="en">MCQ.49.1 - Fully Implemented</skos:prefLabel>
    </owl:NamedIndividual>
    


    <!-- http://JP_ontology.org/assessment/MCQ49.2AnswerA -->


    <owl:NamedIndividual rdf:about="http://JP_ontology.org/assessment/MCQ49.2AnswerA">
        <rdf:type rdf:resource="http://JP_ontology.org/assessment/MCQ.49.2"/>
        <skos:altLabel xml:lang="en">(i)</skos:altLabel>
        <skos:definition xml:lang="en">The organisation has not established methods for monitoring, measurement, analysis, and evaluation to ensure valid results. The methods selected may not be capable of producing comparable and reproducible results, potentially leading to unreliable data for decision-making.</skos:definition>
        <skos:prefLabel xml:lang="en">MCQ.49.2 - Not Implemented</skos:prefLabel>
    </owl:NamedIndividual>
    


    <!-- http://JP_ontology.org/assessment/MCQ49.2AnswerB -->


    <owl:NamedIndividual rdf:about="http://JP_ontology.org/assessment/MCQ49.2AnswerB">
        <rdf:type rdf:resource="http://JP_ontology.org/assessment/MCQ.49.2"/>
        <skos:altLabel xml:lang="en">(ii)</skos:altLabel>
        <skos:definition xml:lang="en">There are some efforts by the organisation to establish methods for monitoring, measurement, analysis, and evaluation to ensure valid results. However, these methods may not be consistently applied or capable of producing fully comparable and reproducible results.</skos:definition>
        <skos:prefLabel xml:lang="en">MCQ.49.2 - Partially Implemented</skos:prefLabel>
    </owl:NamedIndividual>
    


    <!-- http://JP_ontology.org/assessment/MCQ49.2AnswerC -->


    <owl:NamedIndividual rdf:about="http://JP_ontology.org/assessment/MCQ49.2AnswerC">
        <rdf:type rdf:resource="http://JP_ontology.org/assessment/MCQ.49.2"/>
        <skos:altLabel xml:lang="en">(iii)</skos:altLabel>
        <skos:definition xml:lang="en">The organisation has fully established methods for monitoring, measurement, analysis, and evaluation to ensure valid results. These methods are carefully selected and capable of producing comparable and reproducible results, ensuring the reliability of data for decision-making purposes.</skos:definition>
        <skos:prefLabel xml:lang="en">MCQ.49.2 - Fully Implemented</skos:prefLabel>
    </owl:NamedIndividual>
    


    <!-- http://JP_ontology.org/assessment/MCQ49.3AnswerA -->


    <owl:NamedIndividual rdf:about="http://JP_ontology.org/assessment/MCQ49.3AnswerA">
        <rdf:type rdf:resource="http://JP_ontology.org/assessment/MCQ.49.3"/>
        <skos:altLabel xml:lang="en">(i)</skos:altLabel>
        <skos:definition xml:lang="en">The organisation does not specify when monitoring and measuring shall be performed, who shall conduct it, and when the results shall be analysed and evaluated, potentially leading to inconsistencies and delays in the assessment of performance.</skos:definition>
        <skos:prefLabel xml:lang="en">MCQ.49.3 - Not Implemented</skos:prefLabel>
    </owl:NamedIndividual>
    


    <!-- http://JP_ontology.org/assessment/MCQ49.3AnswerB -->


    <owl:NamedIndividual rdf:about="http://JP_ontology.org/assessment/MCQ49.3AnswerB">
        <rdf:type rdf:resource="http://JP_ontology.org/assessment/MCQ.49.3"/>
        <skos:altLabel xml:lang="en">(ii)</skos:altLabel>
        <skos:definition xml:lang="en">There are some efforts by the organisation to specify when monitoring and measuring shall be performed, who shall conduct it, and when the results shall be analysed and evaluated. However, these specifications may be incomplete or not consistently followed.</skos:definition>
        <skos:prefLabel xml:lang="en">MCQ.49.3 - Partially Implemented</skos:prefLabel>
    </owl:NamedIndividual>
    


    <!-- http://JP_ontology.org/assessment/MCQ49.3AnswerC -->


    <owl:NamedIndividual rdf:about="http://JP_ontology.org/assessment/MCQ49.3AnswerC">
        <rdf:type rdf:resource="http://JP_ontology.org/assessment/MCQ.49.3"/>
        <skos:altLabel xml:lang="en">(iii)</skos:altLabel>
        <skos:definition xml:lang="en">The organisation fully specifies when monitoring and measuring shall be performed, who shall conduct it, and when the results shall be analysed and evaluated, ensuring consistency and timeliness in performance assessment.</skos:definition>
        <skos:prefLabel xml:lang="en">MCQ.49.3 - Fully Implemented</skos:prefLabel>
    </owl:NamedIndividual>
    


    <!-- http://JP_ontology.org/assessment/MCQ5.1AnswerA -->


    <owl:NamedIndividual rdf:about="http://JP_ontology.org/assessment/MCQ5.1AnswerA">
        <rdf:type rdf:resource="http://JP_ontology.org/assessment/MCQ.5.1"/>
        <skos:altLabel xml:lang="en">(i)</skos:altLabel>
        <skos:definition xml:lang="en">The organisation does not select appropriate information security risk treatment options, potentially leading to ineffective risk mitigation strategies and heightened security risks.</skos:definition>
        <skos:prefLabel xml:lang="en">MCQ.5.1 - Not Implemented</skos:prefLabel>
    </owl:NamedIndividual>
    


    <!-- http://JP_ontology.org/assessment/MCQ5.1AnswerB -->


    <owl:NamedIndividual rdf:about="http://JP_ontology.org/assessment/MCQ5.1AnswerB">
        <rdf:type rdf:resource="http://JP_ontology.org/assessment/MCQ.5.1"/>
        <skos:altLabel xml:lang="en">(ii)</skos:altLabel>
        <skos:definition xml:lang="en">There are some efforts by the organisation to select appropriate information security risk treatment options, considering the results of the risk assessment. However, the process may be inconsistent or not fully comprehensive.</skos:definition>
        <skos:prefLabel xml:lang="en">MCQ.5.1 - Partially Implemented</skos:prefLabel>
    </owl:NamedIndividual>
    


    <!-- http://JP_ontology.org/assessment/MCQ5.1AnswerC -->


    <owl:NamedIndividual rdf:about="http://JP_ontology.org/assessment/MCQ5.1AnswerC">
        <rdf:type rdf:resource="http://JP_ontology.org/assessment/MCQ.5.1"/>
        <skos:altLabel xml:lang="en">(iii)</skos:altLabel>
        <skos:definition xml:lang="en">The organisation fully selects appropriate information security risk treatment options, considering the results of the risk assessment, ensuring effective risk mitigation strategies are implemented to address identified security risks.</skos:definition>
        <skos:prefLabel xml:lang="en">MCQ.5.1 - Fully Implemented</skos:prefLabel>
    </owl:NamedIndividual>
    


    <!-- http://JP_ontology.org/assessment/MCQ5.2AnswerA -->


    <owl:NamedIndividual rdf:about="http://JP_ontology.org/assessment/MCQ5.2AnswerA">
        <rdf:type rdf:resource="http://JP_ontology.org/assessment/MCQ.5.2"/>
        <skos:altLabel xml:lang="en">(i)</skos:altLabel>
        <skos:definition xml:lang="en">The organisation does not determine all necessary controls to implement the chosen information security risk treatment option(s), potentially leaving gaps in the implementation process and compromising the effectiveness of risk mitigation.</skos:definition>
        <skos:prefLabel xml:lang="en">MCQ.5.2 - Not Implemented</skos:prefLabel>
    </owl:NamedIndividual>
    


    <!-- http://JP_ontology.org/assessment/MCQ5.2AnswerB -->


    <owl:NamedIndividual rdf:about="http://JP_ontology.org/assessment/MCQ5.2AnswerB">
        <rdf:type rdf:resource="http://JP_ontology.org/assessment/MCQ.5.2"/>
        <skos:altLabel xml:lang="en">(ii)</skos:altLabel>
        <skos:definition xml:lang="en">There are some efforts by the organisation to determine all necessary controls to implement the chosen information security risk treatment option(s), whether by designing them as required or identifying them from any source. However, the determination process may be inconsistent or not fully comprehensive.</skos:definition>
        <skos:prefLabel xml:lang="en">MCQ.5.2 - Partially Implemented</skos:prefLabel>
    </owl:NamedIndividual>
    


    <!-- http://JP_ontology.org/assessment/MCQ5.2AnswerC -->


    <owl:NamedIndividual rdf:about="http://JP_ontology.org/assessment/MCQ5.2AnswerC">
        <rdf:type rdf:resource="http://JP_ontology.org/assessment/MCQ.5.2"/>
        <skos:altLabel xml:lang="en">(iii)</skos:altLabel>
        <skos:definition xml:lang="en">The organisation fully determines all necessary controls to implement the chosen information security risk treatment option(s), whether by designing them as required or identifying them from any source, ensuring comprehensive coverage in the implementation process.</skos:definition>
        <skos:prefLabel xml:lang="en">MCQ.5.2 - Fully Implemented</skos:prefLabel>
    </owl:NamedIndividual>
    


    <!-- http://JP_ontology.org/assessment/MCQ5.3AnswerA -->


    <owl:NamedIndividual rdf:about="http://JP_ontology.org/assessment/MCQ5.3AnswerA">
        <rdf:type rdf:resource="http://JP_ontology.org/assessment/MCQ.5.3"/>
        <skos:altLabel xml:lang="en">(i)</skos:altLabel>
        <skos:definition xml:lang="en">The organisation does not produce a control of Applicability containing the necessary controls, justification for their inclusion, status of implementation, and reasoning for excluding any controls, potentially leading to ambiguity and lack of transparency in the management of information security controls.</skos:definition>
        <skos:prefLabel xml:lang="en">MCQ.5.3 - Not Implemented</skos:prefLabel>
    </owl:NamedIndividual>
    


    <!-- http://JP_ontology.org/assessment/MCQ5.3AnswerB -->


    <owl:NamedIndividual rdf:about="http://JP_ontology.org/assessment/MCQ5.3AnswerB">
        <rdf:type rdf:resource="http://JP_ontology.org/assessment/MCQ.5.3"/>
        <skos:altLabel xml:lang="en">(ii)</skos:altLabel>
        <skos:definition xml:lang="en">There are some efforts by the organisation to produce a control of Applicability containing the necessary controls, justification for their inclusion, status of implementation, and reasoning for excluding any controls. However, this documentation may be incomplete or inconsistently maintained.</skos:definition>
        <skos:prefLabel xml:lang="en">MCQ.5.3 - Partially Implemented</skos:prefLabel>
    </owl:NamedIndividual>
    


    <!-- http://JP_ontology.org/assessment/MCQ5.3AnswerC -->


    <owl:NamedIndividual rdf:about="http://JP_ontology.org/assessment/MCQ5.3AnswerC">
        <rdf:type rdf:resource="http://JP_ontology.org/assessment/MCQ.5.3"/>
        <skos:altLabel xml:lang="en">(iii)</skos:altLabel>
        <skos:definition xml:lang="en">The organisation fully produces a control of Applicability containing the necessary controls, justification for their inclusion, status of implementation, and reasoning for excluding any controls, ensuring transparency and accountability in the management of information security controls.</skos:definition>
        <skos:prefLabel xml:lang="en">MCQ.5.3 - Fully Implemented</skos:prefLabel>
    </owl:NamedIndividual>
    


    <!-- http://JP_ontology.org/assessment/MCQ5.4AnswerA -->


    <owl:NamedIndividual rdf:about="http://JP_ontology.org/assessment/MCQ5.4AnswerA">
        <rdf:type rdf:resource="http://JP_ontology.org/assessment/MCQ.5.4"/>
        <skos:altLabel xml:lang="en">(i)</skos:altLabel>
        <skos:definition xml:lang="en">The organisation does not formulate an information security risk treatment plan, potentially leaving security risks unaddressed and increasing the likelihood of security incidents.</skos:definition>
        <skos:prefLabel xml:lang="en">MCQ.5.4 - Not Implemented</skos:prefLabel>
    </owl:NamedIndividual>
    


    <!-- http://JP_ontology.org/assessment/MCQ5.4AnswerB -->


    <owl:NamedIndividual rdf:about="http://JP_ontology.org/assessment/MCQ5.4AnswerB">
        <rdf:type rdf:resource="http://JP_ontology.org/assessment/MCQ.5.4"/>
        <skos:altLabel xml:lang="en">(ii)</skos:altLabel>
        <skos:definition xml:lang="en">There are some efforts by the organisation to formulate an information security risk treatment plan. However, the plan may be incomplete or inconsistently applied across different areas of the organisation.</skos:definition>
        <skos:prefLabel xml:lang="en">MCQ.5.4 - Partially Implemented</skos:prefLabel>
    </owl:NamedIndividual>
    


    <!-- http://JP_ontology.org/assessment/MCQ5.4AnswerC -->


    <owl:NamedIndividual rdf:about="http://JP_ontology.org/assessment/MCQ5.4AnswerC">
        <rdf:type rdf:resource="http://JP_ontology.org/assessment/MCQ.5.4"/>
        <skos:altLabel xml:lang="en">(iii)</skos:altLabel>
        <skos:definition xml:lang="en">The organisation fully formulates an information security risk treatment plan, ensuring that all identified risks are adequately addressed and mitigated in a systematic and comprehensive manner.</skos:definition>
        <skos:prefLabel xml:lang="en">MCQ.5.4 - Fully Implemented</skos:prefLabel>
    </owl:NamedIndividual>
    


    <!-- http://JP_ontology.org/assessment/MCQ5.5AnswerA -->


    <owl:NamedIndividual rdf:about="http://JP_ontology.org/assessment/MCQ5.5AnswerA">
        <rdf:type rdf:resource="http://JP_ontology.org/assessment/MCQ.5.5"/>
        <skos:altLabel xml:lang="en">(i)</skos:altLabel>
        <skos:definition xml:lang="en">The organisation does not obtain approval from risk owners for the information security risk treatment plan and acceptance of residual information security risks, potentially leading to misunderstandings and lack of accountability in managing security risks.</skos:definition>
        <skos:prefLabel xml:lang="en">MCQ.5.5 - Not Implemented</skos:prefLabel>
    </owl:NamedIndividual>
    


    <!-- http://JP_ontology.org/assessment/MCQ5.5AnswerB -->


    <owl:NamedIndividual rdf:about="http://JP_ontology.org/assessment/MCQ5.5AnswerB">
        <rdf:type rdf:resource="http://JP_ontology.org/assessment/MCQ.5.5"/>
        <skos:altLabel xml:lang="en">(ii)</skos:altLabel>
        <skos:definition xml:lang="en">There are some efforts by the organisation to obtain approval from risk owners for the information security risk treatment plan and acceptance of residual information security risks. However, these efforts may not be consistently applied or documented.</skos:definition>
        <skos:prefLabel xml:lang="en">MCQ.5.5 - Partially Implemented</skos:prefLabel>
    </owl:NamedIndividual>
    


    <!-- http://JP_ontology.org/assessment/MCQ5.5AnswerC -->


    <owl:NamedIndividual rdf:about="http://JP_ontology.org/assessment/MCQ5.5AnswerC">
        <rdf:type rdf:resource="http://JP_ontology.org/assessment/MCQ.5.5"/>
        <skos:altLabel xml:lang="en">(iii)</skos:altLabel>
        <skos:definition xml:lang="en">The organisation fully obtains approval from risk owners for the information security risk treatment plan and acceptance of residual information security risks, ensuring that all stakeholders are aligned and accountable for managing security risks effectively.</skos:definition>
        <skos:prefLabel xml:lang="en">MCQ.5.5 - Fully Implemented</skos:prefLabel>
    </owl:NamedIndividual>
    


    <!-- http://JP_ontology.org/assessment/MCQ5.6AnswerA -->


    <owl:NamedIndividual rdf:about="http://JP_ontology.org/assessment/MCQ5.6AnswerA">
        <rdf:type rdf:resource="http://JP_ontology.org/assessment/MCQ.5.6"/>
        <skos:altLabel xml:lang="en">(i)</skos:altLabel>
        <skos:definition xml:lang="en">The organisation does not retain documented information about the information security risk treatment process, potentially leading to lack of accountability and transparency in managing security risks.</skos:definition>
        <skos:prefLabel xml:lang="en">MCQ.5.6 - Not Implemented</skos:prefLabel>
    </owl:NamedIndividual>
    


    <!-- http://JP_ontology.org/assessment/MCQ5.6AnswerB -->


    <owl:NamedIndividual rdf:about="http://JP_ontology.org/assessment/MCQ5.6AnswerB">
        <rdf:type rdf:resource="http://JP_ontology.org/assessment/MCQ.5.6"/>
        <skos:altLabel xml:lang="en">(ii)</skos:altLabel>
        <skos:definition xml:lang="en">There are some efforts by the organisation to retain documented information about the information security risk treatment process. However, documentation may be incomplete or inconsistently maintained.</skos:definition>
        <skos:prefLabel xml:lang="en">MCQ.5.6 - Partially Implemented</skos:prefLabel>
    </owl:NamedIndividual>
    


    <!-- http://JP_ontology.org/assessment/MCQ5.6AnswerC -->


    <owl:NamedIndividual rdf:about="http://JP_ontology.org/assessment/MCQ5.6AnswerC">
        <rdf:type rdf:resource="http://JP_ontology.org/assessment/MCQ.5.6"/>
        <skos:altLabel xml:lang="en">(iii)</skos:altLabel>
        <skos:definition xml:lang="en">The organisation fully retains documented information about the information security risk treatment process, ensuring that all steps and decisions taken in the risk treatment process are recorded and accessible for reference and audit purposes.</skos:definition>
        <skos:prefLabel xml:lang="en">MCQ.5.6 - Fully Implemented</skos:prefLabel>
    </owl:NamedIndividual>
    


    <!-- http://JP_ontology.org/assessment/MCQ50AnswerA -->


    <owl:NamedIndividual rdf:about="http://JP_ontology.org/assessment/MCQ50AnswerA">
        <rdf:type rdf:resource="http://JP_ontology.org/assessment/MCQ.50"/>
        <skos:altLabel xml:lang="en">(i)</skos:altLabel>
        <skos:definition xml:lang="en">The organisation is not conducting internal audits at planned intervals to determine conformity to its own requirements and the requirements outlined in the document, risking non-compliance and ineffective implementation of the information security management system.</skos:definition>
        <skos:prefLabel xml:lang="en">MCQ.50 - Not Implemented</skos:prefLabel>
    </owl:NamedIndividual>
    


    <!-- http://JP_ontology.org/assessment/MCQ50AnswerB -->


    <owl:NamedIndividual rdf:about="http://JP_ontology.org/assessment/MCQ50AnswerB">
        <rdf:type rdf:resource="http://JP_ontology.org/assessment/MCQ.50"/>
        <skos:altLabel xml:lang="en">(ii)</skos:altLabel>
        <skos:definition xml:lang="en">There are some efforts to conduct internal audits at planned intervals, but the process may be inconsistent or not fully comprehensive in assessing conformity to both the organisation’s own requirements and the requirements outlined in the document.</skos:definition>
        <skos:prefLabel xml:lang="en">MCQ.50 - Partially Implemented</skos:prefLabel>
    </owl:NamedIndividual>
    


    <!-- http://JP_ontology.org/assessment/MCQ50AnswerC -->


    <owl:NamedIndividual rdf:about="http://JP_ontology.org/assessment/MCQ50AnswerC">
        <rdf:type rdf:resource="http://JP_ontology.org/assessment/MCQ.50"/>
        <skos:altLabel xml:lang="en">(iii)</skos:altLabel>
        <skos:definition xml:lang="en">The organisation conducts internal audits at planned intervals to determine conformity to its own requirements and the requirements outlined in the document, ensuring effective implementation and maintenance of the information security management system.</skos:definition>
        <skos:prefLabel xml:lang="en">MCQ.50 - Fully Implemented</skos:prefLabel>
    </owl:NamedIndividual>
    


    <!-- http://JP_ontology.org/assessment/MCQ51AnswerA -->


    <owl:NamedIndividual rdf:about="http://JP_ontology.org/assessment/MCQ51AnswerA">
        <rdf:type rdf:resource="http://JP_ontology.org/assessment/MCQ.51"/>
        <skos:altLabel xml:lang="en">(i)</skos:altLabel>
        <skos:definition xml:lang="en">Top management is not conducting reviews of the organisation&apos;s information security management system at planned intervals, leading to potential gaps in its suitability, adequacy, and effectiveness.</skos:definition>
        <skos:prefLabel xml:lang="en">MCQ.51 - Not Implemented</skos:prefLabel>
    </owl:NamedIndividual>
    


    <!-- http://JP_ontology.org/assessment/MCQ51AnswerB -->


    <owl:NamedIndividual rdf:about="http://JP_ontology.org/assessment/MCQ51AnswerB">
        <rdf:type rdf:resource="http://JP_ontology.org/assessment/MCQ.51"/>
        <skos:altLabel xml:lang="en">(ii)</skos:altLabel>
        <skos:definition xml:lang="en">There are some efforts by top management to conduct reviews of the organisation&apos;s information security management system at planned intervals, but the process may be inconsistent or not fully comprehensive in assessing suitability, adequacy, and effectiveness.</skos:definition>
        <skos:prefLabel xml:lang="en">MCQ.51 - Partially Implemented</skos:prefLabel>
    </owl:NamedIndividual>
    


    <!-- http://JP_ontology.org/assessment/MCQ51AnswerC -->


    <owl:NamedIndividual rdf:about="http://JP_ontology.org/assessment/MCQ51AnswerC">
        <rdf:type rdf:resource="http://JP_ontology.org/assessment/MCQ.51"/>
        <skos:altLabel xml:lang="en">(iii)</skos:altLabel>
        <skos:definition xml:lang="en">Top management conducts regular reviews of the organisation&apos;s information security management system at planned intervals, ensuring its continuing suitability, adequacy, and effectiveness in addressing security risks and meeting organisational objectives.</skos:definition>
        <skos:prefLabel xml:lang="en">MCQ.51 - Fully Implemented</skos:prefLabel>
    </owl:NamedIndividual>
    


    <!-- http://JP_ontology.org/assessment/MCQ52AnswerA -->


    <owl:NamedIndividual rdf:about="http://JP_ontology.org/assessment/MCQ52AnswerA">
        <rdf:type rdf:resource="http://JP_ontology.org/assessment/MCQ.52"/>
        <skos:altLabel xml:lang="en">(i)</skos:altLabel>
        <skos:definition xml:lang="en">The organisation’s approach to managing information security and its implementation, including people, processes, and technologies, is not reviewed independently at planned intervals or when significant changes occur, potentially leading to outdated or inadequate security measures.</skos:definition>
        <skos:prefLabel xml:lang="en">MCQ.52 - Not Implemented</skos:prefLabel>
    </owl:NamedIndividual>
    


    <!-- http://JP_ontology.org/assessment/MCQ52AnswerB -->


    <owl:NamedIndividual rdf:about="http://JP_ontology.org/assessment/MCQ52AnswerB">
        <rdf:type rdf:resource="http://JP_ontology.org/assessment/MCQ.52"/>
        <skos:altLabel xml:lang="en">(ii)</skos:altLabel>
        <skos:definition xml:lang="en">There are some efforts to review the organisation’s approach to managing information security and its implementation independently at planned intervals or when significant changes occur, but the reviews may be inconsistent or not fully comprehensive.</skos:definition>
        <skos:prefLabel xml:lang="en">MCQ.52 - Partially Implemented</skos:prefLabel>
    </owl:NamedIndividual>
    


    <!-- http://JP_ontology.org/assessment/MCQ52AnswerC -->


    <owl:NamedIndividual rdf:about="http://JP_ontology.org/assessment/MCQ52AnswerC">
        <rdf:type rdf:resource="http://JP_ontology.org/assessment/MCQ.52"/>
        <skos:altLabel xml:lang="en">(iii)</skos:altLabel>
        <skos:definition xml:lang="en">The organisation’s approach to managing information security and its implementation, including people, processes, and technologies, is independently reviewed at planned intervals or when significant changes occur, ensuring ongoing effectiveness and alignment with security objectives.</skos:definition>
        <skos:prefLabel xml:lang="en">MCQ.52 - Fully Implemented</skos:prefLabel>
    </owl:NamedIndividual>
    


    <!-- http://JP_ontology.org/assessment/MCQ53AnswerA -->


    <owl:NamedIndividual rdf:about="http://JP_ontology.org/assessment/MCQ53AnswerA">
        <rdf:type rdf:resource="http://JP_ontology.org/assessment/MCQ.53"/>
        <skos:altLabel xml:lang="en">(i)</skos:altLabel>
        <skos:definition xml:lang="en">Compliance with the organisation’s information security policy, topic-specific policies, rules, and standards is not regularly reviewed, potentially leading to non-compliance and increased security risks.</skos:definition>
        <skos:prefLabel xml:lang="en">MCQ.53 - Not Implemented</skos:prefLabel>
    </owl:NamedIndividual>
    


    <!-- http://JP_ontology.org/assessment/MCQ53AnswerB -->


    <owl:NamedIndividual rdf:about="http://JP_ontology.org/assessment/MCQ53AnswerB">
        <rdf:type rdf:resource="http://JP_ontology.org/assessment/MCQ.53"/>
        <skos:altLabel xml:lang="en">(ii)</skos:altLabel>
        <skos:definition xml:lang="en">There are some efforts to review compliance with the organisation’s information security policy, topic-specific policies, rules, and standards, but the reviews may be inconsistent or not conducted regularly.</skos:definition>
        <skos:prefLabel xml:lang="en">MCQ.53 - Partially Implemented</skos:prefLabel>
    </owl:NamedIndividual>
    


    <!-- http://JP_ontology.org/assessment/MCQ53AnswerC -->


    <owl:NamedIndividual rdf:about="http://JP_ontology.org/assessment/MCQ53AnswerC">
        <rdf:type rdf:resource="http://JP_ontology.org/assessment/MCQ.53"/>
        <skos:altLabel xml:lang="en">(iii)</skos:altLabel>
        <skos:definition xml:lang="en">Compliance with the organisation’s information security policy, topic-specific policies, rules, and standards is regularly reviewed, ensuring adherence to security requirements and prompt identification and resolution of any non-compliance issues.</skos:definition>
        <skos:prefLabel xml:lang="en">MCQ.53 - Fully Implemented</skos:prefLabel>
    </owl:NamedIndividual>
    


    <!-- http://JP_ontology.org/assessment/MCQ54.1AnswerA -->


    <owl:NamedIndividual rdf:about="http://JP_ontology.org/assessment/MCQ54.1AnswerA">
        <rdf:type rdf:resource="http://JP_ontology.org/assessment/MCQ.54.1"/>
        <skos:altLabel>(i)</skos:altLabel>
        <skos:definition xml:lang="en">The organisation does not determine the required competence of individuals performing work under its control that affects its information security performance, potentially leading to gaps in skills and knowledge.</skos:definition>
        <skos:prefLabel>MCQ54.1. Not Implemented</skos:prefLabel>
    </owl:NamedIndividual>
    


    <!-- http://JP_ontology.org/assessment/MCQ54.1AnswerB -->


    <owl:NamedIndividual rdf:about="http://JP_ontology.org/assessment/MCQ54.1AnswerB">
        <rdf:type rdf:resource="http://JP_ontology.org/assessment/MCQ.54.1"/>
        <skos:altLabel>(ii)</skos:altLabel>
        <skos:definition xml:lang="en">There are some efforts to determine the required competence of individuals performing work under its control that affects its information security performance, but the process may be inconsistent or not fully comprehensive.</skos:definition>
        <skos:prefLabel>MCQ54.1. Partially Implemented</skos:prefLabel>
    </owl:NamedIndividual>
    


    <!-- http://JP_ontology.org/assessment/MCQ54.1AnswerC -->


    <owl:NamedIndividual rdf:about="http://JP_ontology.org/assessment/MCQ54.1AnswerC">
        <rdf:type rdf:resource="http://JP_ontology.org/assessment/MCQ.54.1"/>
        <skos:altLabel>(iii)</skos:altLabel>
        <skos:definition xml:lang="en">The organisation fully determines the required competence of individuals performing work under its control that affects its information security performance, ensuring that personnel possess the necessary skills and knowledge to fulfil their roles effectively.</skos:definition>
        <skos:prefLabel>MCQ54.1. Fully Implemented</skos:prefLabel>
    </owl:NamedIndividual>
    


    <!-- http://JP_ontology.org/assessment/MCQ54.2AnswerA -->


    <owl:NamedIndividual rdf:about="http://JP_ontology.org/assessment/MCQ54.2AnswerA">
        <rdf:type rdf:resource="http://JP_ontology.org/assessment/MCQ.54.2"/>
        <skos:altLabel>(i)</skos:altLabel>
        <skos:definition xml:lang="en">The organisation is not ensuring that individuals possess the necessary competence through appropriate education, training, or experience, potentially leading to gaps in skills and knowledge.</skos:definition>
        <skos:prefLabel>MCQ54.2. Not Implemented</skos:prefLabel>
    </owl:NamedIndividual>
    


    <!-- http://JP_ontology.org/assessment/MCQ54.2AnswerB -->


    <owl:NamedIndividual rdf:about="http://JP_ontology.org/assessment/MCQ54.2AnswerB">
        <rdf:type rdf:resource="http://JP_ontology.org/assessment/MCQ.54.2"/>
        <skos:altLabel>(ii)</skos:altLabel>
        <skos:definition xml:lang="en">There are some efforts to ensure that individuals possess the necessary competence through appropriate education, training, or experience, but the process may be inconsistent or not fully comprehensive.</skos:definition>
        <skos:prefLabel>MCQ54.2. Partially Implemented</skos:prefLabel>
    </owl:NamedIndividual>
    


    <!-- http://JP_ontology.org/assessment/MCQ54.2AnswerC -->


    <owl:NamedIndividual rdf:about="http://JP_ontology.org/assessment/MCQ54.2AnswerC">
        <rdf:type rdf:resource="http://JP_ontology.org/assessment/MCQ.54.2"/>
        <skos:altLabel>(iii)</skos:altLabel>
        <skos:definition xml:lang="en">The organisation fully ensures that individuals possess the necessary competence through appropriate education, training, or experience, ensuring that personnel are adequately prepared to fulfil their roles effectively.</skos:definition>
        <skos:prefLabel>MCQ54.2. Fully Implemented</skos:prefLabel>
    </owl:NamedIndividual>
    


    <!-- http://JP_ontology.org/assessment/MCQ54.3AnswerA -->


    <owl:NamedIndividual rdf:about="http://JP_ontology.org/assessment/MCQ54.3AnswerA">
        <rdf:type rdf:resource="http://JP_ontology.org/assessment/MCQ.54.3"/>
        <skos:altLabel>(i)</skos:altLabel>
        <skos:definition xml:lang="en">The organisation is not taking necessary actions to acquire the required competence and is not evaluating the effectiveness of these actions, potentially resulting in inadequately skilled personnel.</skos:definition>
        <skos:prefLabel>MCQ54.3. Not Implemented</skos:prefLabel>
    </owl:NamedIndividual>
    


    <!-- http://JP_ontology.org/assessment/MCQ54.3AnswerB -->


    <owl:NamedIndividual rdf:about="http://JP_ontology.org/assessment/MCQ54.3AnswerB">
        <rdf:type rdf:resource="http://JP_ontology.org/assessment/MCQ.54.3"/>
        <skos:altLabel>(ii)</skos:altLabel>
        <skos:definition xml:lang="en">There are some efforts by the organisation to acquire the required competence and evaluate the effectiveness of these actions, but the process may be inconsistent or not fully comprehensive.</skos:definition>
        <skos:prefLabel>MCQ54.3. Partially Implemented</skos:prefLabel>
    </owl:NamedIndividual>
    


    <!-- http://JP_ontology.org/assessment/MCQ54.3AnswerC -->


    <owl:NamedIndividual rdf:about="http://JP_ontology.org/assessment/MCQ54.3AnswerC">
        <rdf:type rdf:resource="http://JP_ontology.org/assessment/MCQ.54.3"/>
        <skos:altLabel>(iii)</skos:altLabel>
        <skos:definition xml:lang="en">The organisation is taking necessary actions to acquire the required competence and systematically evaluating the effectiveness of these actions, ensuring continuous improvement in the skills and knowledge of its personnel.</skos:definition>
        <skos:prefLabel>MCQ54.3. Fully Implemented</skos:prefLabel>
    </owl:NamedIndividual>
    


    <!-- http://JP_ontology.org/assessment/MCQ54.4AnswerA -->


    <owl:NamedIndividual rdf:about="http://JP_ontology.org/assessment/MCQ54.4AnswerA">
        <rdf:type rdf:resource="http://JP_ontology.org/assessment/MCQ.54.4"/>
        <skos:altLabel>(i)</skos:altLabel>
        <skos:definition xml:lang="en">The organisation is not retaining appropriate documented information as evidence of competence, potentially leading to difficulties in verifying the skills and knowledge of its personnel.</skos:definition>
        <skos:prefLabel>MCQ54.4. Not Implemented</skos:prefLabel>
    </owl:NamedIndividual>
    


    <!-- http://JP_ontology.org/assessment/MCQ54.4AnswerB -->


    <owl:NamedIndividual rdf:about="http://JP_ontology.org/assessment/MCQ54.4AnswerB">
        <rdf:type rdf:resource="http://JP_ontology.org/assessment/MCQ.54.4"/>
        <skos:altLabel>(ii)</skos:altLabel>
        <skos:definition xml:lang="en">There are some efforts by the organisation to retain appropriate documented information as evidence of competence, but the documentation may be incomplete or not consistently maintained.</skos:definition>
        <skos:prefLabel>MCQ54.4. Partially Implemented</skos:prefLabel>
    </owl:NamedIndividual>
    


    <!-- http://JP_ontology.org/assessment/MCQ54.4AnswerC -->


    <owl:NamedIndividual rdf:about="http://JP_ontology.org/assessment/MCQ54.4AnswerC">
        <rdf:type rdf:resource="http://JP_ontology.org/assessment/MCQ.54.4"/>
        <skos:altLabel>(iii)</skos:altLabel>
        <skos:definition xml:lang="en">The organisation is retaining appropriate documented information as evidence of competence, ensuring comprehensive records are maintained to verify the skills and knowledge of its personnel.</skos:definition>
        <skos:prefLabel>MCQ54.4. Fully Implemented</skos:prefLabel>
    </owl:NamedIndividual>
    


    <!-- http://JP_ontology.org/assessment/MCQ55.1AnswerA -->


    <owl:NamedIndividual rdf:about="http://JP_ontology.org/assessment/MCQ55.1AnswerA">
        <rdf:type rdf:resource="http://JP_ontology.org/assessment/MCQ.55.1"/>
        <skos:altLabel xml:lang="en">(i)</skos:altLabel>
        <skos:definition xml:lang="en">Persons doing work under the organisation’s control are not aware of the information security policy, potentially leading to non-compliance and increased security risks.</skos:definition>
        <skos:prefLabel xml:lang="en">MCQ.55.1 - Not Implemented</skos:prefLabel>
    </owl:NamedIndividual>
    


    <!-- http://JP_ontology.org/assessment/MCQ55.1AnswerB -->


    <owl:NamedIndividual rdf:about="http://JP_ontology.org/assessment/MCQ55.1AnswerB">
        <rdf:type rdf:resource="http://JP_ontology.org/assessment/MCQ.55.1"/>
        <skos:altLabel xml:lang="en">(ii)</skos:altLabel>
        <skos:definition xml:lang="en">There are some efforts to make persons doing work under the organisation’s control aware of the information security policy. However, awareness may be inconsistent or not fully comprehensive.</skos:definition>
        <skos:prefLabel xml:lang="en">MCQ.55.1 - Partially Implemented</skos:prefLabel>
    </owl:NamedIndividual>
    


    <!-- http://JP_ontology.org/assessment/MCQ55.1AnswerC -->


    <owl:NamedIndividual rdf:about="http://JP_ontology.org/assessment/MCQ55.1AnswerC">
        <rdf:type rdf:resource="http://JP_ontology.org/assessment/MCQ.55.1"/>
        <skos:altLabel xml:lang="en">(iii)</skos:altLabel>
        <skos:definition xml:lang="en">Persons doing work under the organisation’s control are fully aware of the information security policy, ensuring widespread understanding and adherence to security protocols and procedures.</skos:definition>
        <skos:prefLabel xml:lang="en">MCQ.55.1 - Fully Implemented</skos:prefLabel>
    </owl:NamedIndividual>
    


    <!-- http://JP_ontology.org/assessment/MCQ55.2AnswerA -->


    <owl:NamedIndividual rdf:about="http://JP_ontology.org/assessment/MCQ55.2AnswerA">
        <rdf:type rdf:resource="http://JP_ontology.org/assessment/MCQ.55.2"/>
        <skos:altLabel xml:lang="en">(i)</skos:altLabel>
        <skos:definition xml:lang="en">Persons doing work under the organisation’s control are not aware of their contribution to the effectiveness of the information security management system, nor do they understand the benefits of improved information security performance, potentially leading to decreased motivation and engagement in security efforts.</skos:definition>
        <skos:prefLabel xml:lang="en">MCQ.55.2 - Not Implemented</skos:prefLabel>
    </owl:NamedIndividual>
    


    <!-- http://JP_ontology.org/assessment/MCQ55.2AnswerB -->


    <owl:NamedIndividual rdf:about="http://JP_ontology.org/assessment/MCQ55.2AnswerB">
        <rdf:type rdf:resource="http://JP_ontology.org/assessment/MCQ.55.2"/>
        <skos:altLabel xml:lang="en">(ii)</skos:altLabel>
        <skos:definition xml:lang="en">There are some efforts to make persons doing work under the organisation’s control aware of their contribution to the effectiveness of the information security management system and the benefits of improved information security performance. However, awareness may be inconsistent or not fully comprehensive.</skos:definition>
        <skos:prefLabel xml:lang="en">MCQ.55.2 - Partially Implemented</skos:prefLabel>
    </owl:NamedIndividual>
    


    <!-- http://JP_ontology.org/assessment/MCQ55.2AnswerC -->


    <owl:NamedIndividual rdf:about="http://JP_ontology.org/assessment/MCQ55.2AnswerC">
        <rdf:type rdf:resource="http://JP_ontology.org/assessment/MCQ.55.2"/>
        <skos:altLabel xml:lang="en">(iii)</skos:altLabel>
        <skos:definition xml:lang="en">Persons doing work under the organisation’s control are fully aware of their contribution to the effectiveness of the information security management system and the benefits of improved information security performance, fostering a culture of security awareness and proactive engagement in security initiatives.</skos:definition>
        <skos:prefLabel xml:lang="en">MCQ.55.2 - Fully Implemented</skos:prefLabel>
    </owl:NamedIndividual>
    


    <!-- http://JP_ontology.org/assessment/MCQ55.3AnswerA -->


    <owl:NamedIndividual rdf:about="http://JP_ontology.org/assessment/MCQ55.3AnswerA">
        <rdf:type rdf:resource="http://JP_ontology.org/assessment/MCQ.55.3"/>
        <skos:altLabel xml:lang="en">(i)</skos:altLabel>
        <skos:definition xml:lang="en">Persons doing work under the organisation’s control are not aware of the implications of not conforming with the information security management system requirements, potentially leading to inadvertent non-compliance and increased security risks.</skos:definition>
        <skos:prefLabel xml:lang="en">MCQ.55.3 - Not Implemented</skos:prefLabel>
    </owl:NamedIndividual>
    


    <!-- http://JP_ontology.org/assessment/MCQ55.3AnswerB -->


    <owl:NamedIndividual rdf:about="http://JP_ontology.org/assessment/MCQ55.3AnswerB">
        <rdf:type rdf:resource="http://JP_ontology.org/assessment/MCQ.55.3"/>
        <skos:altLabel xml:lang="en">(ii)</skos:altLabel>
        <skos:definition xml:lang="en">There are some efforts to make persons doing work under the organisation’s control aware of the implications of not conforming with the information security management system requirements. However, awareness may be inconsistent or not fully comprehensive.</skos:definition>
        <skos:prefLabel xml:lang="en">MCQ.55.3 - Partially Implemented</skos:prefLabel>
    </owl:NamedIndividual>
    


    <!-- http://JP_ontology.org/assessment/MCQ55.3AnswerC -->


    <owl:NamedIndividual rdf:about="http://JP_ontology.org/assessment/MCQ55.3AnswerC">
        <rdf:type rdf:resource="http://JP_ontology.org/assessment/MCQ.55.3"/>
        <skos:altLabel xml:lang="en">(iii)</skos:altLabel>
        <skos:definition xml:lang="en">Persons doing work under the organisation’s control are fully aware of the implications of not conforming with the information security management system requirements, fostering a culture of compliance and accountability in information security practices.</skos:definition>
        <skos:prefLabel xml:lang="en">MCQ.55.3 - Fully Implemented</skos:prefLabel>
    </owl:NamedIndividual>
    


    <!-- http://JP_ontology.org/assessment/MCQ56.1AnswerA -->


    <owl:NamedIndividual rdf:about="http://JP_ontology.org/assessment/MCQ56.1AnswerA">
        <rdf:type rdf:resource="http://JP_ontology.org/assessment/MCQ.56.1"/>
        <skos:altLabel xml:lang="en">(i)</skos:altLabel>
        <skos:definition xml:lang="en">The organisation does not determine what information to communicate regarding the information security management system.</skos:definition>
        <skos:prefLabel xml:lang="en">MCQ.56.1 - Not Implemented</skos:prefLabel>
    </owl:NamedIndividual>
    


    <!-- http://JP_ontology.org/assessment/MCQ56.1AnswerB -->


    <owl:NamedIndividual rdf:about="http://JP_ontology.org/assessment/MCQ56.1AnswerB">
        <rdf:type rdf:resource="http://JP_ontology.org/assessment/MCQ.56.1"/>
        <skos:altLabel xml:lang="en">(ii)</skos:altLabel>
        <skos:definition xml:lang="en">The organisation has some understanding of what information to communicate regarding the information security management system, but it may not be comprehensive.</skos:definition>
        <skos:prefLabel xml:lang="en">MCQ.56.1 - Partially Implemented</skos:prefLabel>
    </owl:NamedIndividual>
    


    <!-- http://JP_ontology.org/assessment/MCQ56.1AnswerC -->


    <owl:NamedIndividual rdf:about="http://JP_ontology.org/assessment/MCQ56.1AnswerC">
        <rdf:type rdf:resource="http://JP_ontology.org/assessment/MCQ.56.1"/>
        <skos:altLabel xml:lang="en">(iii)</skos:altLabel>
        <skos:definition xml:lang="en">The organisation has a clear understanding of what information to communicate regarding the information security management system, covering all relevant aspects.</skos:definition>
        <skos:prefLabel xml:lang="en">MCQ.56.1 - Fully Implemented</skos:prefLabel>
    </owl:NamedIndividual>
    


    <!-- http://JP_ontology.org/assessment/MCQ56.2AnswerA -->


    <owl:NamedIndividual rdf:about="http://JP_ontology.org/assessment/MCQ56.2AnswerA">
        <rdf:type rdf:resource="http://JP_ontology.org/assessment/MCQ.56.2"/>
        <skos:altLabel xml:lang="en">(i)</skos:altLabel>
        <skos:definition xml:lang="en">There is no established timing for communication related to the information security management system.</skos:definition>
        <skos:prefLabel xml:lang="en">MCQ.56.2 - Not Implemented</skos:prefLabel>
    </owl:NamedIndividual>
    


    <!-- http://JP_ontology.org/assessment/MCQ56.2AnswerB -->


    <owl:NamedIndividual rdf:about="http://JP_ontology.org/assessment/MCQ56.2AnswerB">
        <rdf:type rdf:resource="http://JP_ontology.org/assessment/MCQ.56.2"/>
        <skos:altLabel xml:lang="en">(ii)</skos:altLabel>
        <skos:definition xml:lang="en">There are some established timings for communication related to the information security management system, but they may not cover all necessary instances.</skos:definition>
        <skos:prefLabel xml:lang="en">MCQ.56.2 - Partially Implemented</skos:prefLabel>
    </owl:NamedIndividual>
    


    <!-- http://JP_ontology.org/assessment/MCQ56.2AnswerC -->


    <owl:NamedIndividual rdf:about="http://JP_ontology.org/assessment/MCQ56.2AnswerC">
        <rdf:type rdf:resource="http://JP_ontology.org/assessment/MCQ.56.2"/>
        <skos:altLabel xml:lang="en">(iii)</skos:altLabel>
        <skos:definition xml:lang="en">There are well-established timings for communication related to the information security management system, ensuring timely dissemination of information.</skos:definition>
        <skos:prefLabel xml:lang="en">MCQ.56.2 - Fully Implemented</skos:prefLabel>
    </owl:NamedIndividual>
    


    <!-- http://JP_ontology.org/assessment/MCQ56.3AnswerA -->


    <owl:NamedIndividual rdf:about="http://JP_ontology.org/assessment/MCQ56.3AnswerA">
        <rdf:type rdf:resource="http://JP_ontology.org/assessment/MCQ.56.3"/>
        <skos:altLabel xml:lang="en">(i)</skos:altLabel>
        <skos:definition xml:lang="en">The organisation lacks clarity on whom to communicate with regarding the information security management system.</skos:definition>
        <skos:prefLabel xml:lang="en">MCQ.56.3 - Not Implemented</skos:prefLabel>
    </owl:NamedIndividual>
    


    <!-- http://JP_ontology.org/assessment/MCQ56.3AnswerB -->


    <owl:NamedIndividual rdf:about="http://JP_ontology.org/assessment/MCQ56.3AnswerB">
        <rdf:type rdf:resource="http://JP_ontology.org/assessment/MCQ.56.3"/>
        <skos:altLabel xml:lang="en">(ii)</skos:altLabel>
        <skos:definition xml:lang="en">The organisation identifies some stakeholders with whom to communicate regarding the information security management system, but there may be gaps in coverage.</skos:definition>
        <skos:prefLabel xml:lang="en">MCQ.56.3 - Partially Implemented</skos:prefLabel>
    </owl:NamedIndividual>
    


    <!-- http://JP_ontology.org/assessment/MCQ56.3AnswerC -->


    <owl:NamedIndividual rdf:about="http://JP_ontology.org/assessment/MCQ56.3AnswerC">
        <rdf:type rdf:resource="http://JP_ontology.org/assessment/MCQ.56.3"/>
        <skos:altLabel xml:lang="en">(iii)</skos:altLabel>
        <skos:definition xml:lang="en">The organisation has identified all relevant stakeholders with whom to communicate regarding the information security management system, ensuring comprehensive coverage.</skos:definition>
        <skos:prefLabel xml:lang="en">MCQ.56.3 - Fully Implemented</skos:prefLabel>
    </owl:NamedIndividual>
    


    <!-- http://JP_ontology.org/assessment/MCQ56.4AnswerA -->


    <owl:NamedIndividual rdf:about="http://JP_ontology.org/assessment/MCQ56.4AnswerA">
        <rdf:type rdf:resource="http://JP_ontology.org/assessment/MCQ.56.4"/>
        <skos:altLabel xml:lang="en">(i)</skos:altLabel>
        <skos:definition xml:lang="en">There are no established methods or protocols for how to communicate information about the information security management system.</skos:definition>
        <skos:prefLabel xml:lang="en">MCQ.56.4 - Not Implemented</skos:prefLabel>
    </owl:NamedIndividual>
    


    <!-- http://JP_ontology.org/assessment/MCQ56.4AnswerB -->


    <owl:NamedIndividual rdf:about="http://JP_ontology.org/assessment/MCQ56.4AnswerB">
        <rdf:type rdf:resource="http://JP_ontology.org/assessment/MCQ.56.4"/>
        <skos:altLabel xml:lang="en">(ii)</skos:altLabel>
        <skos:definition xml:lang="en">There are some established methods or protocols for how to communicate information about the information security management system, but they may not be consistently applied.</skos:definition>
        <skos:prefLabel xml:lang="en">MCQ.56.4 - Partially Implemented</skos:prefLabel>
    </owl:NamedIndividual>
    


    <!-- http://JP_ontology.org/assessment/MCQ56.4AnswerC -->


    <owl:NamedIndividual rdf:about="http://JP_ontology.org/assessment/MCQ56.4AnswerC">
        <rdf:type rdf:resource="http://JP_ontology.org/assessment/MCQ.56.4"/>
        <skos:altLabel xml:lang="en">(iii)</skos:altLabel>
        <skos:definition xml:lang="en">There are established methods and protocols for how to communicate information about the information security management system, ensuring effective and secure communication channels.</skos:definition>
        <skos:prefLabel xml:lang="en">MCQ.56.4 - Fully Implemented</skos:prefLabel>
    </owl:NamedIndividual>
    


    <!-- http://JP_ontology.org/assessment/MCQ57.1AnswerA -->


    <owl:NamedIndividual rdf:about="http://JP_ontology.org/assessment/MCQ57.1AnswerA">
        <rdf:type rdf:resource="http://JP_ontology.org/assessment/MCQ.57.1"/>
        <skos:altLabel xml:lang="en">(i)</skos:altLabel>
        <skos:definition xml:lang="en">Personnel of the organisation and relevant interested parties do not receive appropriate information security awareness, education, and training, leaving them ill-prepared to address security risks and threats.</skos:definition>
        <skos:prefLabel xml:lang="en">MCQ.57.1 - Not Implemented</skos:prefLabel>
    </owl:NamedIndividual>
    


    <!-- http://JP_ontology.org/assessment/MCQ57.1AnswerB -->


    <owl:NamedIndividual rdf:about="http://JP_ontology.org/assessment/MCQ57.1AnswerB">
        <rdf:type rdf:resource="http://JP_ontology.org/assessment/MCQ.57.1"/>
        <skos:altLabel xml:lang="en">(ii)</skos:altLabel>
        <skos:definition xml:lang="en">There are some efforts to provide personnel of the organisation and relevant interested parties with information security awareness, education, and training, but it may be inconsistent or not fully comprehensive.</skos:definition>
        <skos:prefLabel xml:lang="en">MCQ.57.1 - Partially Implemented</skos:prefLabel>
    </owl:NamedIndividual>
    


    <!-- http://JP_ontology.org/assessment/MCQ57.1AnswerC -->


    <owl:NamedIndividual rdf:about="http://JP_ontology.org/assessment/MCQ57.1AnswerC">
        <rdf:type rdf:resource="http://JP_ontology.org/assessment/MCQ.57.1"/>
        <skos:altLabel xml:lang="en">(iii)</skos:altLabel>
        <skos:definition xml:lang="en">Personnel of the organisation and relevant interested parties receive appropriate information security awareness, education, and training, ensuring they are well-equipped to understand and address security risks and threats effectively.</skos:definition>
        <skos:prefLabel xml:lang="en">MCQ.57.1 - Fully Implemented</skos:prefLabel>
    </owl:NamedIndividual>
    


    <!-- http://JP_ontology.org/assessment/MCQ57.2AnswerA -->


    <owl:NamedIndividual rdf:about="http://JP_ontology.org/assessment/MCQ57.2AnswerA">
        <rdf:type rdf:resource="http://JP_ontology.org/assessment/MCQ.57.2"/>
        <skos:altLabel xml:lang="en">(i)</skos:altLabel>
        <skos:definition xml:lang="en">Regular updates of the organisation&apos;s information security policy, topic-specific policies, and procedures relevant to their job function are not provided to personnel of the organisation and relevant interested parties, potentially leading to outdated practices and non-compliance with security standards.</skos:definition>
        <skos:prefLabel xml:lang="en">MCQ.57.2 - Not Implemented</skos:prefLabel>
    </owl:NamedIndividual>
    


    <!-- http://JP_ontology.org/assessment/MCQ57.2AnswerB -->


    <owl:NamedIndividual rdf:about="http://JP_ontology.org/assessment/MCQ57.2AnswerB">
        <rdf:type rdf:resource="http://JP_ontology.org/assessment/MCQ.57.2"/>
        <skos:altLabel xml:lang="en">(ii)</skos:altLabel>
        <skos:definition xml:lang="en">There are some efforts to provide regular updates of the organisation&apos;s information security policy, topic-specific policies, and procedures relevant to their job function to personnel of the organisation and relevant interested parties, but the updates may be inconsistent or not fully comprehensive.</skos:definition>
        <skos:prefLabel xml:lang="en">MCQ.57.2 - Partially Implemented</skos:prefLabel>
    </owl:NamedIndividual>
    


    <!-- http://JP_ontology.org/assessment/MCQ57.2AnswerC -->


    <owl:NamedIndividual rdf:about="http://JP_ontology.org/assessment/MCQ57.2AnswerC">
        <rdf:type rdf:resource="http://JP_ontology.org/assessment/MCQ.57.2"/>
        <skos:altLabel xml:lang="en">(iii)</skos:altLabel>
        <skos:definition xml:lang="en">Regular updates of the organisation&apos;s information security policy, topic-specific policies, and procedures relevant to their job function are fully provided to personnel of the organisation and relevant interested parties, ensuring they are well-informed and compliant with current security standards.</skos:definition>
        <skos:prefLabel xml:lang="en">MCQ.57.2 - Fully Implemented</skos:prefLabel>
    </owl:NamedIndividual>
    


    <!-- http://JP_ontology.org/assessment/MCQ58AnswerA -->


    <owl:NamedIndividual rdf:about="http://JP_ontology.org/assessment/MCQ58AnswerA">
        <rdf:type rdf:resource="http://JP_ontology.org/assessment/MCQ.58"/>
        <skos:altLabel>(i)</skos:altLabel>
        <skos:definition xml:lang="en">Clear desk rules for papers and removable storage media, as well as clear screen rules for information processing facilities, are not defined or appropriately enforced, leading to potential security breaches and unauthorized access to sensitive information.</skos:definition>
        <skos:prefLabel>MCQ58. Not Implemented</skos:prefLabel>
    </owl:NamedIndividual>
    


    <!-- http://JP_ontology.org/assessment/MCQ58AnswerB -->


    <owl:NamedIndividual rdf:about="http://JP_ontology.org/assessment/MCQ58AnswerB">
        <rdf:type rdf:resource="http://JP_ontology.org/assessment/MCQ.58"/>
        <skos:altLabel>(ii)</skos:altLabel>
        <skos:definition xml:lang="en">There are some efforts to define clear desk rules for papers and removable storage media, as well as clear screen rules for information processing facilities, but enforcement may be inconsistent or not fully effective.</skos:definition>
        <skos:prefLabel>MCQ58. Partially Implemented</skos:prefLabel>
    </owl:NamedIndividual>
    


    <!-- http://JP_ontology.org/assessment/MCQ58AnswerC -->


    <owl:NamedIndividual rdf:about="http://JP_ontology.org/assessment/MCQ58AnswerC">
        <rdf:type rdf:resource="http://JP_ontology.org/assessment/MCQ.58"/>
        <skos:altLabel>(iii)</skos:altLabel>
        <skos:definition xml:lang="en">Clear desk rules for papers and removable storage media, as well as clear screen rules for information processing facilities, are defined and appropriately enforced, ensuring the protection of sensitive information and compliance with security policies.</skos:definition>
        <skos:prefLabel>MCQ58. Fully Implemented</skos:prefLabel>
    </owl:NamedIndividual>
    


    <!-- http://JP_ontology.org/assessment/MCQ59AnswerA -->


    <owl:NamedIndividual rdf:about="http://JP_ontology.org/assessment/MCQ59AnswerA">
        <rdf:type rdf:resource="http://JP_ontology.org/assessment/MCQ.59"/>
        <skos:altLabel xml:lang="en">(i)</skos:altLabel>
        <skos:definition xml:lang="en">Rules to control physical and logical access to information and associated assets are not established or implemented, lacking alignment with business and information security requirements.</skos:definition>
        <skos:prefLabel xml:lang="en">MCQ.59 - Not Implemented</skos:prefLabel>
    </owl:NamedIndividual>
    


    <!-- http://JP_ontology.org/assessment/MCQ59AnswerB -->


    <owl:NamedIndividual rdf:about="http://JP_ontology.org/assessment/MCQ59AnswerB">
        <rdf:type rdf:resource="http://JP_ontology.org/assessment/MCQ.59"/>
        <skos:altLabel xml:lang="en">(ii)</skos:altLabel>
        <skos:definition xml:lang="en">There are some rules established to control physical and logical access to information and associated assets, but they may not fully align with both business and information security requirements, leading to potential gaps in access control.</skos:definition>
        <skos:prefLabel xml:lang="en">MCQ.59 - Partially Implemented</skos:prefLabel>
    </owl:NamedIndividual>
    


    <!-- http://JP_ontology.org/assessment/MCQ59AnswerC -->


    <owl:NamedIndividual rdf:about="http://JP_ontology.org/assessment/MCQ59AnswerC">
        <rdf:type rdf:resource="http://JP_ontology.org/assessment/MCQ.59"/>
        <skos:altLabel xml:lang="en">(iii)</skos:altLabel>
        <skos:definition xml:lang="en">Comprehensive rules are established and rigorously implemented to control physical and logical access to information and associated assets, ensuring alignment with both business and information security requirements for effective access control.</skos:definition>
        <skos:prefLabel xml:lang="en">MCQ.59 - Fully Implemented</skos:prefLabel>
    </owl:NamedIndividual>
    


    <!-- http://JP_ontology.org/assessment/MCQ6.1AnswerA -->


    <owl:NamedIndividual rdf:about="http://JP_ontology.org/assessment/MCQ6.1AnswerA">
        <rdf:type rdf:resource="http://JP_ontology.org/assessment/MCQ.6.1"/>
        <skos:altLabel xml:lang="en">(i)</skos:altLabel>
        <skos:definition xml:lang="en">The organisation does not determine what information to communicate regarding the information security management system.</skos:definition>
        <skos:prefLabel xml:lang="en">MCQ.6.1 - Not Implemented</skos:prefLabel>
    </owl:NamedIndividual>
    


    <!-- http://JP_ontology.org/assessment/MCQ6.1AnswerB -->


    <owl:NamedIndividual rdf:about="http://JP_ontology.org/assessment/MCQ6.1AnswerB">
        <rdf:type rdf:resource="http://JP_ontology.org/assessment/MCQ.6.1"/>
        <skos:altLabel xml:lang="en">(ii)</skos:altLabel>
        <skos:definition xml:lang="en">The organisation has some understanding of what information to communicate regarding the information security management system, but it may not be comprehensive.</skos:definition>
        <skos:prefLabel xml:lang="en">MCQ.6.1 - Partially Implemented</skos:prefLabel>
    </owl:NamedIndividual>
    


    <!-- http://JP_ontology.org/assessment/MCQ6.1AnswerC -->


    <owl:NamedIndividual rdf:about="http://JP_ontology.org/assessment/MCQ6.1AnswerC">
        <rdf:type rdf:resource="http://JP_ontology.org/assessment/MCQ.6.1"/>
        <skos:altLabel xml:lang="en">(iii)</skos:altLabel>
        <skos:definition xml:lang="en">The organisation has a clear understanding of what information to communicate regarding the information security management system, covering all relevant aspects.</skos:definition>
        <skos:prefLabel xml:lang="en">MCQ.6.1 - Fully Implemented</skos:prefLabel>
    </owl:NamedIndividual>
    


    <!-- http://JP_ontology.org/assessment/MCQ6.2AnswerA -->


    <owl:NamedIndividual rdf:about="http://JP_ontology.org/assessment/MCQ6.2AnswerA">
        <rdf:type rdf:resource="http://JP_ontology.org/assessment/MCQ.6.2"/>
        <skos:altLabel xml:lang="en">(i)</skos:altLabel>
        <skos:definition xml:lang="en">There is no established timing for communication related to the information security management system.</skos:definition>
        <skos:prefLabel xml:lang="en">MCQ.6.2 - Not Implemented</skos:prefLabel>
    </owl:NamedIndividual>
    


    <!-- http://JP_ontology.org/assessment/MCQ6.2AnswerB -->


    <owl:NamedIndividual rdf:about="http://JP_ontology.org/assessment/MCQ6.2AnswerB">
        <rdf:type rdf:resource="http://JP_ontology.org/assessment/MCQ.6.2"/>
        <skos:altLabel xml:lang="en">(ii)</skos:altLabel>
        <skos:definition xml:lang="en">There are some established timings for communication related to the information security management system, but they may not cover all necessary instances.</skos:definition>
        <skos:prefLabel xml:lang="en">MCQ.6.2 - Partially Implemented</skos:prefLabel>
    </owl:NamedIndividual>
    


    <!-- http://JP_ontology.org/assessment/MCQ6.2AnswerC -->


    <owl:NamedIndividual rdf:about="http://JP_ontology.org/assessment/MCQ6.2AnswerC">
        <rdf:type rdf:resource="http://JP_ontology.org/assessment/MCQ.6.2"/>
        <skos:altLabel xml:lang="en">(iii)</skos:altLabel>
        <skos:definition xml:lang="en">There are well-established timings for communication related to the information security management system, ensuring timely dissemination of information.</skos:definition>
        <skos:prefLabel xml:lang="en">MCQ.6.2 - Fully Implemented</skos:prefLabel>
    </owl:NamedIndividual>
    


    <!-- http://JP_ontology.org/assessment/MCQ6.3AnswerA -->


    <owl:NamedIndividual rdf:about="http://JP_ontology.org/assessment/MCQ6.3AnswerA">
        <rdf:type rdf:resource="http://JP_ontology.org/assessment/MCQ.6.3"/>
        <skos:altLabel xml:lang="en">(i)</skos:altLabel>
        <skos:definition xml:lang="en">The organisation lacks clarity on whom to communicate with regarding the information security management system.</skos:definition>
        <skos:prefLabel xml:lang="en">MCQ.6.3 - Not Implemented</skos:prefLabel>
    </owl:NamedIndividual>
    


    <!-- http://JP_ontology.org/assessment/MCQ6.3AnswerB -->


    <owl:NamedIndividual rdf:about="http://JP_ontology.org/assessment/MCQ6.3AnswerB">
        <rdf:type rdf:resource="http://JP_ontology.org/assessment/MCQ.6.3"/>
        <skos:altLabel xml:lang="en">(ii)</skos:altLabel>
        <skos:definition xml:lang="en">The organisation identifies some stakeholders with whom to communicate regarding the information security management system, but there may be gaps in coverage.</skos:definition>
        <skos:prefLabel xml:lang="en">MCQ.6.3 - Partially Implemented</skos:prefLabel>
    </owl:NamedIndividual>
    


    <!-- http://JP_ontology.org/assessment/MCQ6.3AnswerC -->


    <owl:NamedIndividual rdf:about="http://JP_ontology.org/assessment/MCQ6.3AnswerC">
        <rdf:type rdf:resource="http://JP_ontology.org/assessment/MCQ.6.3"/>
        <skos:altLabel xml:lang="en">(iii)</skos:altLabel>
        <skos:definition xml:lang="en">The organisation has identified all relevant stakeholders with whom to communicate regarding the information security management system, ensuring comprehensive coverage.</skos:definition>
        <skos:prefLabel xml:lang="en">MCQ.6.3 - Fully Implemented</skos:prefLabel>
    </owl:NamedIndividual>
    


    <!-- http://JP_ontology.org/assessment/MCQ6.4AnswerA -->


    <owl:NamedIndividual rdf:about="http://JP_ontology.org/assessment/MCQ6.4AnswerA">
        <rdf:type rdf:resource="http://JP_ontology.org/assessment/MCQ.6.4"/>
        <skos:altLabel xml:lang="en">(i)</skos:altLabel>
        <skos:definition xml:lang="en">There are no established methods or protocols for how to communicate information about the information security management system.</skos:definition>
        <skos:prefLabel xml:lang="en">MCQ.6.4 - Not Implemented</skos:prefLabel>
    </owl:NamedIndividual>
    


    <!-- http://JP_ontology.org/assessment/MCQ6.4AnswerB -->


    <owl:NamedIndividual rdf:about="http://JP_ontology.org/assessment/MCQ6.4AnswerB">
        <rdf:type rdf:resource="http://JP_ontology.org/assessment/MCQ.6.4"/>
        <skos:altLabel xml:lang="en">(ii)</skos:altLabel>
        <skos:definition xml:lang="en">There are some established methods or protocols for how to communicate information about the information security management system, but they may not be consistently applied.</skos:definition>
        <skos:prefLabel xml:lang="en">MCQ.6.4 - Partially Implemented</skos:prefLabel>
    </owl:NamedIndividual>
    


    <!-- http://JP_ontology.org/assessment/MCQ6.4AnswerC -->


    <owl:NamedIndividual rdf:about="http://JP_ontology.org/assessment/MCQ6.4AnswerC">
        <rdf:type rdf:resource="http://JP_ontology.org/assessment/MCQ.6.4"/>
        <skos:altLabel xml:lang="en">(iii)</skos:altLabel>
        <skos:definition xml:lang="en">There are established methods and protocols for how to communicate information about the information security management system, ensuring effective and secure communication channels.</skos:definition>
        <skos:prefLabel xml:lang="en">MCQ.6.4 - Fully Implemented</skos:prefLabel>
    </owl:NamedIndividual>
    


    <!-- http://JP_ontology.org/assessment/MCQ60AnswerA -->


    <owl:NamedIndividual rdf:about="http://JP_ontology.org/assessment/MCQ60AnswerA">
        <rdf:type rdf:resource="http://JP_ontology.org/assessment/MCQ.60"/>
        <skos:altLabel xml:lang="en">(i)</skos:altLabel>
        <skos:definition xml:lang="en">The organisation lacks a structured approach to managing the complete life cycle of identities, leading to inconsistencies and gaps in identity-related processes such as creation, authentication, and termination.</skos:definition>
        <skos:prefLabel xml:lang="en">MCQ.60 - Not Implemented</skos:prefLabel>
    </owl:NamedIndividual>
    


    <!-- http://JP_ontology.org/assessment/MCQ60AnswerB -->


    <owl:NamedIndividual rdf:about="http://JP_ontology.org/assessment/MCQ60AnswerB">
        <rdf:type rdf:resource="http://JP_ontology.org/assessment/MCQ.60"/>
        <skos:altLabel xml:lang="en">(ii)</skos:altLabel>
        <skos:definition xml:lang="en">There are some efforts to manage the complete life cycle of identities, including activities such as creation, authentication, and periodic reviews, but the process may be inconsistent or lacking in certain areas.</skos:definition>
        <skos:prefLabel xml:lang="en">MCQ.60 - Partially Implemented</skos:prefLabel>
    </owl:NamedIndividual>
    


    <!-- http://JP_ontology.org/assessment/MCQ60AnswerC -->


    <owl:NamedIndividual rdf:about="http://JP_ontology.org/assessment/MCQ60AnswerC">
        <rdf:type rdf:resource="http://JP_ontology.org/assessment/MCQ.60"/>
        <skos:altLabel xml:lang="en">(iii)</skos:altLabel>
        <skos:definition xml:lang="en">The organisation has implemented a comprehensive approach to managing the complete life cycle of identities, covering all activities from creation to termination, and ensuring robust oversight and control over identity-related processes.</skos:definition>
        <skos:prefLabel xml:lang="en">MCQ.60 - Fully Implemented</skos:prefLabel>
    </owl:NamedIndividual>
    


    <!-- http://JP_ontology.org/assessment/MCQ61AnswerA -->


    <owl:NamedIndividual rdf:about="http://JP_ontology.org/assessment/MCQ61AnswerA">
        <rdf:type rdf:resource="http://JP_ontology.org/assessment/MCQ.61"/>
        <skos:altLabel xml:lang="en">(i)</skos:altLabel>
        <skos:definition xml:lang="en">There is no management process in place to control the allocation and management of authentication information, and personnel are not advised on the appropriate handling of authentication information.</skos:definition>
        <skos:prefLabel xml:lang="en">MCQ.61 - Not Implemented</skos:prefLabel>
    </owl:NamedIndividual>
    


    <!-- http://JP_ontology.org/assessment/MCQ61AnswerB -->


    <owl:NamedIndividual rdf:about="http://JP_ontology.org/assessment/MCQ61AnswerB">
        <rdf:type rdf:resource="http://JP_ontology.org/assessment/MCQ.61"/>
        <skos:altLabel xml:lang="en">(ii)</skos:altLabel>
        <skos:definition xml:lang="en">There are some efforts to control the allocation and management of authentication information through a management process, but personnel may not consistently receive advice on the appropriate handling of authentication information.</skos:definition>
        <skos:prefLabel xml:lang="en">MCQ.61 - Partially Implemented</skos:prefLabel>
    </owl:NamedIndividual>
    


    <!-- http://JP_ontology.org/assessment/MCQ61AnswerC -->


    <owl:NamedIndividual rdf:about="http://JP_ontology.org/assessment/MCQ61AnswerC">
        <rdf:type rdf:resource="http://JP_ontology.org/assessment/MCQ.61"/>
        <skos:altLabel xml:lang="en">(iii)</skos:altLabel>
        <skos:definition xml:lang="en">The allocation and management of authentication information are controlled by a robust management process, which includes advising personnel on the appropriate handling of authentication information, ensuring secure and effective management of authentication credentials.</skos:definition>
        <skos:prefLabel xml:lang="en">MCQ.61 - Fully Implemented</skos:prefLabel>
    </owl:NamedIndividual>
    


    <!-- http://JP_ontology.org/assessment/MCQ62AnswerA -->


    <owl:NamedIndividual rdf:about="http://JP_ontology.org/assessment/MCQ62AnswerA">
        <rdf:type rdf:resource="http://JP_ontology.org/assessment/MCQ.62"/>
        <skos:altLabel xml:lang="en">(i)</skos:altLabel>
        <skos:definition xml:lang="en">Access rights to information and associated assets are not provisioned, reviewed, modified, or removed in accordance with the organisation’s topic-specific policy and rules for access control, leading to inconsistencies and potential security risks.</skos:definition>
        <skos:prefLabel xml:lang="en">MCQ.62 - Not Implemented</skos:prefLabel>
    </owl:NamedIndividual>
    


    <!-- http://JP_ontology.org/assessment/MCQ62AnswerB -->


    <owl:NamedIndividual rdf:about="http://JP_ontology.org/assessment/MCQ62AnswerB">
        <rdf:type rdf:resource="http://JP_ontology.org/assessment/MCQ.62"/>
        <skos:altLabel xml:lang="en">(ii)</skos:altLabel>
        <skos:definition xml:lang="en">There are some efforts to provision, review, modify, and remove access rights in accordance with the organisation’s topic-specific policy and rules for access control, but the process may be inconsistent or incomplete.</skos:definition>
        <skos:prefLabel xml:lang="en">MCQ.62 - Partially Implemented</skos:prefLabel>
    </owl:NamedIndividual>
    


    <!-- http://JP_ontology.org/assessment/MCQ62AnswerC -->


    <owl:NamedIndividual rdf:about="http://JP_ontology.org/assessment/MCQ62AnswerC">
        <rdf:type rdf:resource="http://JP_ontology.org/assessment/MCQ.62"/>
        <skos:altLabel xml:lang="en">(iii)</skos:altLabel>
        <skos:definition xml:lang="en">Access rights to information and associated assets are provisioned, reviewed, modified, and removed in strict accordance with the organisation’s topic-specific policy and rules for access control, ensuring effective access management and adherence to security requirements.</skos:definition>
        <skos:prefLabel xml:lang="en">MCQ.62 - Fully Implemented</skos:prefLabel>
    </owl:NamedIndividual>
    


    <!-- http://JP_ontology.org/assessment/MCQ63AnswerA -->


    <owl:NamedIndividual rdf:about="http://JP_ontology.org/assessment/MCQ63AnswerA">
        <rdf:type rdf:resource="http://JP_ontology.org/assessment/MCQ.63"/>
        <skos:altLabel xml:lang="en">(i)</skos:altLabel>
        <skos:definition xml:lang="en">The organisation does not acquire information regarding technical vulnerabilities of the information systems in use, evaluate its exposure to such vulnerabilities, or implement appropriate measures, leaving it susceptible to potential security breaches.</skos:definition>
        <skos:prefLabel xml:lang="en">MCQ.63 - Not Implemented</skos:prefLabel>
    </owl:NamedIndividual>
    


    <!-- http://JP_ontology.org/assessment/MCQ63AnswerB -->


    <owl:NamedIndividual rdf:about="http://JP_ontology.org/assessment/MCQ63AnswerB">
        <rdf:type rdf:resource="http://JP_ontology.org/assessment/MCQ.63"/>
        <skos:altLabel xml:lang="en">(ii)</skos:altLabel>
        <skos:definition xml:lang="en">There are some efforts to acquire information regarding technical vulnerabilities and evaluate the organisation’s exposure to such vulnerabilities, but the implementation of appropriate measures may be inconsistent or incomplete.</skos:definition>
        <skos:prefLabel xml:lang="en">MCQ.63 - Partially Implemented</skos:prefLabel>
    </owl:NamedIndividual>
    


    <!-- http://JP_ontology.org/assessment/MCQ63AnswerC -->


    <owl:NamedIndividual rdf:about="http://JP_ontology.org/assessment/MCQ63AnswerC">
        <rdf:type rdf:resource="http://JP_ontology.org/assessment/MCQ.63"/>
        <skos:altLabel xml:lang="en">(iii)</skos:altLabel>
        <skos:definition xml:lang="en">The organisation consistently acquires information regarding technical vulnerabilities of the information systems in use, evaluates its exposure to such vulnerabilities, and implements appropriate measures accordingly, ensuring proactive management of security risks.</skos:definition>
        <skos:prefLabel xml:lang="en">MCQ.63 - Fully Implemented</skos:prefLabel>
    </owl:NamedIndividual>
    


    <!-- http://JP_ontology.org/assessment/MCQ64AnswerA -->


    <owl:NamedIndividual rdf:about="http://JP_ontology.org/assessment/MCQ64AnswerA">
        <rdf:type rdf:resource="http://JP_ontology.org/assessment/MCQ.64"/>
        <skos:altLabel xml:lang="en">(i)</skos:altLabel>
        <skos:definition xml:lang="en">Configurations, including security configurations, of hardware, software, services, and networks are not established, documented, implemented, monitored, or reviewed, leading to potential vulnerabilities and inconsistent security measures.</skos:definition>
        <skos:prefLabel xml:lang="en">MCQ.64 - Not Implemented</skos:prefLabel>
    </owl:NamedIndividual>
    


    <!-- http://JP_ontology.org/assessment/MCQ64AnswerB -->


    <owl:NamedIndividual rdf:about="http://JP_ontology.org/assessment/MCQ64AnswerB">
        <rdf:type rdf:resource="http://JP_ontology.org/assessment/MCQ.64"/>
        <skos:altLabel xml:lang="en">(ii)</skos:altLabel>
        <skos:definition xml:lang="en">There are some efforts to establish, document, implement, monitor, and review configurations, including security configurations, of hardware, software, services, and networks, but the process may be inconsistent or incomplete.</skos:definition>
        <skos:prefLabel xml:lang="en">MCQ.64 - Partially Implemented</skos:prefLabel>
    </owl:NamedIndividual>
    


    <!-- http://JP_ontology.org/assessment/MCQ64AnswerC -->


    <owl:NamedIndividual rdf:about="http://JP_ontology.org/assessment/MCQ64AnswerC">
        <rdf:type rdf:resource="http://JP_ontology.org/assessment/MCQ.64"/>
        <skos:altLabel xml:lang="en">(iii)</skos:altLabel>
        <skos:definition xml:lang="en">Configurations, including security configurations, of hardware, software, services, and networks are fully established, documented, implemented, monitored, and reviewed, ensuring consistent and effective security measures across the organisation.</skos:definition>
        <skos:prefLabel xml:lang="en">MCQ.64 - Fully Implemented</skos:prefLabel>
    </owl:NamedIndividual>
    


    <!-- http://JP_ontology.org/assessment/MCQ65AnswerA -->


    <owl:NamedIndividual rdf:about="http://JP_ontology.org/assessment/MCQ65AnswerA">
        <rdf:type rdf:resource="http://JP_ontology.org/assessment/MCQ.65"/>
        <skos:altLabel xml:lang="en">(i)</skos:altLabel>
        <skos:definition xml:lang="en">Protection against malware is not implemented, and there are no appropriate user awareness measures in place, leaving the organisation vulnerable to malware attacks.</skos:definition>
        <skos:prefLabel xml:lang="en">MCQ.65 - Not Implemented</skos:prefLabel>
    </owl:NamedIndividual>
    


    <!-- http://JP_ontology.org/assessment/MCQ65AnswerB -->


    <owl:NamedIndividual rdf:about="http://JP_ontology.org/assessment/MCQ65AnswerB">
        <rdf:type rdf:resource="http://JP_ontology.org/assessment/MCQ.65"/>
        <skos:altLabel xml:lang="en">(ii)</skos:altLabel>
        <skos:definition xml:lang="en">There are some efforts to implement protection against malware, but user awareness measures may be lacking or insufficient to adequately support the protection against malware.</skos:definition>
        <skos:prefLabel xml:lang="en">MCQ.65 - Partially Implemented</skos:prefLabel>
    </owl:NamedIndividual>
    


    <!-- http://JP_ontology.org/assessment/MCQ65AnswerC -->


    <owl:NamedIndividual rdf:about="http://JP_ontology.org/assessment/MCQ65AnswerC">
        <rdf:type rdf:resource="http://JP_ontology.org/assessment/MCQ.65"/>
        <skos:altLabel xml:lang="en">(iii)</skos:altLabel>
        <skos:definition xml:lang="en">Protection against malware is fully implemented and supported by appropriate user awareness measures, ensuring proactive defence against malware threats and enhancing overall security posture.</skos:definition>
        <skos:prefLabel xml:lang="en">MCQ.65 - Fully Implemented</skos:prefLabel>
    </owl:NamedIndividual>
    


    <!-- http://JP_ontology.org/assessment/MCQ66AnswerA -->


    <owl:NamedIndividual rdf:about="http://JP_ontology.org/assessment/MCQ66AnswerA">
        <rdf:type rdf:resource="http://JP_ontology.org/assessment/MCQ.66"/>
        <skos:altLabel xml:lang="en">(i)</skos:altLabel>
        <skos:definition xml:lang="en">Procedures and measures to securely manage software installation on operational systems have not been implemented, potentially leading to unauthorized or insecure software installations.</skos:definition>
        <skos:prefLabel xml:lang="en">MCQ.66 - Not Implemented</skos:prefLabel>
    </owl:NamedIndividual>
    


    <!-- http://JP_ontology.org/assessment/MCQ66AnswerB -->


    <owl:NamedIndividual rdf:about="http://JP_ontology.org/assessment/MCQ66AnswerB">
        <rdf:type rdf:resource="http://JP_ontology.org/assessment/MCQ.66"/>
        <skos:altLabel xml:lang="en">(ii)</skos:altLabel>
        <skos:definition xml:lang="en">There are some procedures and measures in place to securely manage software installation on operational systems, but they may be incomplete or inconsistently applied.</skos:definition>
        <skos:prefLabel xml:lang="en">MCQ.66 - Partially Implemented</skos:prefLabel>
    </owl:NamedIndividual>
    


    <!-- http://JP_ontology.org/assessment/MCQ66AnswerC -->


    <owl:NamedIndividual rdf:about="http://JP_ontology.org/assessment/MCQ66AnswerC">
        <rdf:type rdf:resource="http://JP_ontology.org/assessment/MCQ.66"/>
        <skos:altLabel xml:lang="en">(iii)</skos:altLabel>
        <skos:definition xml:lang="en">Procedures and measures to securely manage software installation on operational systems are fully implemented, ensuring that only authorized and secure software is installed, minimizing security risks.</skos:definition>
        <skos:prefLabel xml:lang="en">MCQ.66 - Fully Implemented</skos:prefLabel>
    </owl:NamedIndividual>
    


    <!-- http://JP_ontology.org/assessment/MCQ67AnswerA -->


    <owl:NamedIndividual rdf:about="http://JP_ontology.org/assessment/MCQ67AnswerA">
        <rdf:type rdf:resource="http://JP_ontology.org/assessment/MCQ.67"/>
        <skos:altLabel xml:lang="en">(i)</skos:altLabel>
        <skos:definition xml:lang="en">Segregation is not implemented for groups of information services, users, and information systems within the organisation&apos;s networks, leading to potential risks of unauthorized access and data breaches.</skos:definition>
        <skos:prefLabel xml:lang="en">MCQ.67 - Not Implemented</skos:prefLabel>
    </owl:NamedIndividual>
    


    <!-- http://JP_ontology.org/assessment/MCQ67AnswerB -->


    <owl:NamedIndividual rdf:about="http://JP_ontology.org/assessment/MCQ67AnswerB">
        <rdf:type rdf:resource="http://JP_ontology.org/assessment/MCQ.67"/>
        <skos:altLabel xml:lang="en">(ii)</skos:altLabel>
        <skos:definition xml:lang="en">There are some efforts to implement segregation for groups of information services, users, and information systems within the organisation&apos;s networks, but the implementation may be incomplete or inconsistent.</skos:definition>
        <skos:prefLabel xml:lang="en">MCQ.67 - Partially Implemented</skos:prefLabel>
    </owl:NamedIndividual>
    


    <!-- http://JP_ontology.org/assessment/MCQ67AnswerC -->


    <owl:NamedIndividual rdf:about="http://JP_ontology.org/assessment/MCQ67AnswerC">
        <rdf:type rdf:resource="http://JP_ontology.org/assessment/MCQ.67"/>
        <skos:altLabel xml:lang="en">(iii)</skos:altLabel>
        <skos:definition xml:lang="en">Segregation is fully implemented for groups of information services, users, and information systems within the organisation&apos;s networks, ensuring controlled access and minimizing the impact of security incidents.</skos:definition>
        <skos:prefLabel xml:lang="en">MCQ.67 - Fully Implemented</skos:prefLabel>
    </owl:NamedIndividual>
    


    <!-- http://JP_ontology.org/assessment/MCQ68AnswerA -->


    <owl:NamedIndividual rdf:about="http://JP_ontology.org/assessment/MCQ68AnswerA">
        <rdf:type rdf:resource="http://JP_ontology.org/assessment/MCQ.68"/>
        <skos:altLabel>(i)</skos:altLabel>
        <skos:definition xml:lang="en">Operating procedures for information processing facilities are not documented, and there is no system in place to make them available to personnel who require them.</skos:definition>
        <skos:prefLabel>MCQ68. Not Implemented</skos:prefLabel>
    </owl:NamedIndividual>
    


    <!-- http://JP_ontology.org/assessment/MCQ68AnswerB -->


    <owl:NamedIndividual rdf:about="http://JP_ontology.org/assessment/MCQ68AnswerB">
        <rdf:type rdf:resource="http://JP_ontology.org/assessment/MCQ.68"/>
        <skos:altLabel>(ii)</skos:altLabel>
        <skos:definition xml:lang="en">There are some operating procedures for information processing facilities documented, but access to them may be limited or inconsistent for personnel who require them.</skos:definition>
        <skos:prefLabel>MCQ68. Partially Implemented</skos:prefLabel>
    </owl:NamedIndividual>
    


    <!-- http://JP_ontology.org/assessment/MCQ68AnswerC -->


    <owl:NamedIndividual rdf:about="http://JP_ontology.org/assessment/MCQ68AnswerC">
        <rdf:type rdf:resource="http://JP_ontology.org/assessment/MCQ.68"/>
        <skos:altLabel>(iii)</skos:altLabel>
        <skos:definition xml:lang="en">Operating procedures for information processing facilities are comprehensively documented and readily available to all personnel who require them, ensuring efficient and standardized operations across the organisation.</skos:definition>
        <skos:prefLabel>MCQ68. Fully Implemented</skos:prefLabel>
    </owl:NamedIndividual>
    


    <!-- http://JP_ontology.org/assessment/MCQ69AnswerA -->


    <owl:NamedIndividual rdf:about="http://JP_ontology.org/assessment/MCQ69AnswerA">
        <rdf:type rdf:resource="http://JP_ontology.org/assessment/MCQ.69"/>
        <skos:altLabel xml:lang="en">(i)</skos:altLabel>
        <skos:definition xml:lang="en">Rules for the effective use of cryptography, including cryptographic key management, are not defined or implemented, leading to potential vulnerabilities and inadequate protection of sensitive information.</skos:definition>
        <skos:prefLabel xml:lang="en">MCQ.69 - Not Implemented</skos:prefLabel>
    </owl:NamedIndividual>
    


    <!-- http://JP_ontology.org/assessment/MCQ69AnswerB -->


    <owl:NamedIndividual rdf:about="http://JP_ontology.org/assessment/MCQ69AnswerB">
        <rdf:type rdf:resource="http://JP_ontology.org/assessment/MCQ.69"/>
        <skos:altLabel xml:lang="en">(ii)</skos:altLabel>
        <skos:definition xml:lang="en">There are some efforts to define and implement rules for the effective use of cryptography, including cryptographic key management, but the implementation may be inconsistent or incomplete.</skos:definition>
        <skos:prefLabel xml:lang="en">MCQ.69 - Partially Implemented</skos:prefLabel>
    </owl:NamedIndividual>
    


    <!-- http://JP_ontology.org/assessment/MCQ69AnswerC -->


    <owl:NamedIndividual rdf:about="http://JP_ontology.org/assessment/MCQ69AnswerC">
        <rdf:type rdf:resource="http://JP_ontology.org/assessment/MCQ.69"/>
        <skos:altLabel xml:lang="en">(iii)</skos:altLabel>
        <skos:definition xml:lang="en">Rules for the effective use of cryptography, including cryptographic key management, are fully defined and implemented, ensuring secure encryption practices and robust protection of sensitive information.</skos:definition>
        <skos:prefLabel xml:lang="en">MCQ.69 - Fully Implemented</skos:prefLabel>
    </owl:NamedIndividual>
    


    <!-- http://JP_ontology.org/assessment/MCQ70.1AnswerA -->


    <owl:NamedIndividual rdf:about="http://JP_ontology.org/assessment/MCQ70.1AnswerA">
        <rdf:type rdf:resource="http://JP_ontology.org/assessment/MCQ.70.1"/>
        <skos:altLabel>(i)</skos:altLabel>
        <skos:definition xml:lang="en">The organisation does not determine the required competence of individuals performing work under its control that affects its information security performance, potentially leading to gaps in skills and knowledge.</skos:definition>
        <skos:prefLabel>MCQ70.1. Not Implemented</skos:prefLabel>
    </owl:NamedIndividual>
    


    <!-- http://JP_ontology.org/assessment/MCQ70.1AnswerB -->


    <owl:NamedIndividual rdf:about="http://JP_ontology.org/assessment/MCQ70.1AnswerB">
        <rdf:type rdf:resource="http://JP_ontology.org/assessment/MCQ.70.1"/>
        <skos:altLabel>(ii)</skos:altLabel>
        <skos:definition xml:lang="en">There are some efforts to determine the required competence of individuals performing work under its control that affects its information security performance, but the process may be inconsistent or not fully comprehensive.</skos:definition>
        <skos:prefLabel>MCQ70.1. Partially Implemented</skos:prefLabel>
    </owl:NamedIndividual>
    


    <!-- http://JP_ontology.org/assessment/MCQ70.1AnswerC -->


    <owl:NamedIndividual rdf:about="http://JP_ontology.org/assessment/MCQ70.1AnswerC">
        <rdf:type rdf:resource="http://JP_ontology.org/assessment/MCQ.70.1"/>
        <skos:altLabel>(iii)</skos:altLabel>
        <skos:definition xml:lang="en">The organisation fully determines the required competence of individuals performing work under its control that affects its information security performance, ensuring that personnel possess the necessary skills and knowledge to fulfill their roles effectively.</skos:definition>
        <skos:prefLabel>MCQ70.1. Fully Implemented</skos:prefLabel>
    </owl:NamedIndividual>
    


    <!-- http://JP_ontology.org/assessment/MCQ70.2AnswerA -->


    <owl:NamedIndividual rdf:about="http://JP_ontology.org/assessment/MCQ70.2AnswerA">
        <rdf:type rdf:resource="http://JP_ontology.org/assessment/MCQ.70.2"/>
        <skos:altLabel>(i)</skos:altLabel>
        <skos:definition xml:lang="en">The organisation is not ensuring that individuals possess the necessary competence through appropriate education, training, or experience, potentially leading to gaps in skills and knowledge.</skos:definition>
        <skos:prefLabel>MCQ70.2. Not Implemented</skos:prefLabel>
    </owl:NamedIndividual>
    


    <!-- http://JP_ontology.org/assessment/MCQ70.2AnswerB -->


    <owl:NamedIndividual rdf:about="http://JP_ontology.org/assessment/MCQ70.2AnswerB">
        <rdf:type rdf:resource="http://JP_ontology.org/assessment/MCQ.70.2"/>
        <skos:altLabel>(ii)</skos:altLabel>
        <skos:definition xml:lang="en">There are some efforts to ensure that individuals possess the necessary competence through appropriate education, training, or experience, but the process may be inconsistent or not fully comprehensive.</skos:definition>
        <skos:prefLabel>MCQ70.2. Partially Implemented</skos:prefLabel>
    </owl:NamedIndividual>
    


    <!-- http://JP_ontology.org/assessment/MCQ70.2AnswerC -->


    <owl:NamedIndividual rdf:about="http://JP_ontology.org/assessment/MCQ70.2AnswerC">
        <rdf:type rdf:resource="http://JP_ontology.org/assessment/MCQ.70.2"/>
        <skos:altLabel>(iii)</skos:altLabel>
        <skos:definition xml:lang="en">The organisation fully ensures that individuals possess the necessary competence through appropriate education, training, or experience, ensuring that personnel are adequately prepared to fulfill their roles effectively.</skos:definition>
        <skos:prefLabel>MCQ70.2. Fully Implemented</skos:prefLabel>
    </owl:NamedIndividual>
    


    <!-- http://JP_ontology.org/assessment/MCQ70.3AnswerA -->


    <owl:NamedIndividual rdf:about="http://JP_ontology.org/assessment/MCQ70.3AnswerA">
        <rdf:type rdf:resource="http://JP_ontology.org/assessment/MCQ.70.3"/>
        <skos:altLabel>(i)</skos:altLabel>
        <skos:definition xml:lang="en">The organisation is not taking necessary actions to acquire the required competence and is not evaluating the effectiveness of these actions, potentially resulting in inadequately skilled personnel.</skos:definition>
        <skos:prefLabel>MCQ70.3. Not Implemented</skos:prefLabel>
    </owl:NamedIndividual>
    


    <!-- http://JP_ontology.org/assessment/MCQ70.3AnswerB -->


    <owl:NamedIndividual rdf:about="http://JP_ontology.org/assessment/MCQ70.3AnswerB">
        <rdf:type rdf:resource="http://JP_ontology.org/assessment/MCQ.70.3"/>
        <skos:altLabel>(ii)</skos:altLabel>
        <skos:definition xml:lang="en">There are some efforts by the organisation to acquire the required competence and evaluate the effectiveness of these actions, but the process may be inconsistent or not fully comprehensive.</skos:definition>
        <skos:prefLabel>MCQ70.3. Partially Implemented</skos:prefLabel>
    </owl:NamedIndividual>
    


    <!-- http://JP_ontology.org/assessment/MCQ70.3AnswerC -->


    <owl:NamedIndividual rdf:about="http://JP_ontology.org/assessment/MCQ70.3AnswerC">
        <rdf:type rdf:resource="http://JP_ontology.org/assessment/MCQ.70.3"/>
        <skos:altLabel>(iii)</skos:altLabel>
        <skos:definition xml:lang="en">The organisation is taking necessary actions to acquire the required competence and systematically evaluating the effectiveness of these actions, ensuring continuous improvement in the skills and knowledge of its personnel.</skos:definition>
        <skos:prefLabel>MCQ70.3. Fully Implemented</skos:prefLabel>
    </owl:NamedIndividual>
    


    <!-- http://JP_ontology.org/assessment/MCQ70.4AnswerA -->


    <owl:NamedIndividual rdf:about="http://JP_ontology.org/assessment/MCQ70.4AnswerA">
        <rdf:type rdf:resource="http://JP_ontology.org/assessment/MCQ.70.4"/>
        <skos:altLabel>(i)</skos:altLabel>
        <skos:definition xml:lang="en">The organisation is not retaining appropriate documented information as evidence of competence, potentially leading to difficulties in verifying the skills and knowledge of its personnel.</skos:definition>
        <skos:prefLabel>MCQ70.4. Not Implemented</skos:prefLabel>
    </owl:NamedIndividual>
    


    <!-- http://JP_ontology.org/assessment/MCQ70.4AnswerB -->


    <owl:NamedIndividual rdf:about="http://JP_ontology.org/assessment/MCQ70.4AnswerB">
        <rdf:type rdf:resource="http://JP_ontology.org/assessment/MCQ.70.4"/>
        <skos:altLabel>(ii)</skos:altLabel>
        <skos:definition xml:lang="en">There are some efforts by the organisation to retain appropriate documented information as evidence of competence, but the documentation may be incomplete or not consistently maintained.</skos:definition>
        <skos:prefLabel>MCQ70.4. Partially Implemented</skos:prefLabel>
    </owl:NamedIndividual>
    


    <!-- http://JP_ontology.org/assessment/MCQ70.4AnswerC -->


    <owl:NamedIndividual rdf:about="http://JP_ontology.org/assessment/MCQ70.4AnswerC">
        <rdf:type rdf:resource="http://JP_ontology.org/assessment/MCQ.70.4"/>
        <skos:altLabel>(iii)</skos:altLabel>
        <skos:definition xml:lang="en">The organisation is retaining appropriate documented information as evidence of competence, ensuring comprehensive records are maintained to verify the skills and knowledge of its personnel.</skos:definition>
        <skos:prefLabel>MCQ70.4. Fully Implemented</skos:prefLabel>
    </owl:NamedIndividual>
    


    <!-- http://JP_ontology.org/assessment/MCQ71AnswerA -->


    <owl:NamedIndividual rdf:about="http://JP_ontology.org/assessment/MCQ71AnswerA">
        <rdf:type rdf:resource="http://JP_ontology.org/assessment/MCQ.71"/>
        <skos:altLabel xml:lang="en">(i)</skos:altLabel>
        <skos:definition xml:lang="en">Roles and responsibilities related to information security are not clearly defined, and there is no formal allocation process based on organisational needs.</skos:definition>
        <skos:prefLabel xml:lang="en">MCQ.71 - Not Implemented</skos:prefLabel>
    </owl:NamedIndividual>
    


    <!-- http://JP_ontology.org/assessment/MCQ71AnswerB -->


    <owl:NamedIndividual rdf:about="http://JP_ontology.org/assessment/MCQ71AnswerB">
        <rdf:type rdf:resource="http://JP_ontology.org/assessment/MCQ.71"/>
        <skos:altLabel xml:lang="en">(ii)</skos:altLabel>
        <skos:definition xml:lang="en">There is a general understanding of information security roles and responsibilities, but they are not consistently defined and allocated according to the organisation&apos;s needs. Some areas may lack clarity or consistency.</skos:definition>
        <skos:prefLabel xml:lang="en">MCQ.71 - Partially Implemented</skos:prefLabel>
    </owl:NamedIndividual>
    


    <!-- http://JP_ontology.org/assessment/MCQ71AnswerC -->


    <owl:NamedIndividual rdf:about="http://JP_ontology.org/assessment/MCQ71AnswerC">
        <rdf:type rdf:resource="http://JP_ontology.org/assessment/MCQ.71"/>
        <skos:altLabel xml:lang="en">(iii)</skos:altLabel>
        <skos:definition xml:lang="en">Clear and comprehensive information security roles and responsibilities are defined and allocated based on the specific needs of the organisation. There are established processes for regularly reviewing and updating these roles to ensure alignment with organisational requirements.</skos:definition>
        <skos:prefLabel xml:lang="en">MCQ.71 - Fully Implemented</skos:prefLabel>
    </owl:NamedIndividual>
    


    <!-- http://JP_ontology.org/assessment/MCQ72AnswerA -->


    <owl:NamedIndividual rdf:about="http://JP_ontology.org/assessment/MCQ72AnswerA">
        <rdf:type rdf:resource="http://JP_ontology.org/assessment/MCQ.72"/>
        <skos:altLabel>(i)</skos:altLabel>
        <skos:definition xml:lang="en">Conflicting duties and conflicting areas of responsibility are not segregated, potentially leading to conflicts of interest and increased risk of fraud or errors.</skos:definition>
        <skos:prefLabel>MCQ72. Not Implemented</skos:prefLabel>
    </owl:NamedIndividual>
    


    <!-- http://JP_ontology.org/assessment/MCQ72AnswerB -->


    <owl:NamedIndividual rdf:about="http://JP_ontology.org/assessment/MCQ72AnswerB">
        <rdf:type rdf:resource="http://JP_ontology.org/assessment/MCQ.72"/>
        <skos:altLabel>(ii)</skos:altLabel>
        <skos:definition xml:lang="en">There are some efforts to segregate conflicting duties and conflicting areas of responsibility, but the segregation may be incomplete or inconsistently applied.</skos:definition>
        <skos:prefLabel>MCQ72. Partially Implemented</skos:prefLabel>
    </owl:NamedIndividual>
    


    <!-- http://JP_ontology.org/assessment/MCQ72AnswerC -->


    <owl:NamedIndividual rdf:about="http://JP_ontology.org/assessment/MCQ72AnswerC">
        <rdf:type rdf:resource="http://JP_ontology.org/assessment/MCQ.72"/>
        <skos:altLabel>(iii)</skos:altLabel>
        <skos:definition xml:lang="en">Conflicting duties and conflicting areas of responsibility are fully segregated, minimizing the risk of fraud or errors by ensuring appropriate separation of duties and responsibilities.</skos:definition>
        <skos:prefLabel>MCQ72. Fully Implemented</skos:prefLabel>
    </owl:NamedIndividual>
    


    <!-- http://JP_ontology.org/assessment/MCQ73AnswerA -->


    <owl:NamedIndividual rdf:about="http://JP_ontology.org/assessment/MCQ73AnswerA">
        <rdf:type rdf:resource="http://JP_ontology.org/assessment/MCQ.73"/>
        <skos:altLabel>(i)</skos:altLabel>
        <skos:definition xml:lang="en">Background verification checks on candidates prior to joining the organisation and on an ongoing basis are not conducted, neglecting compliance with applicable laws, regulations, and ethics, and failing to adequately assess risks associated with personnel.</skos:definition>
        <skos:prefLabel>MCQ73. Not Implemented</skos:prefLabel>
    </owl:NamedIndividual>
    


    <!-- http://JP_ontology.org/assessment/MCQ73AnswerB -->


    <owl:NamedIndividual rdf:about="http://JP_ontology.org/assessment/MCQ73AnswerB">
        <rdf:type rdf:resource="http://JP_ontology.org/assessment/MCQ.73"/>
        <skos:altLabel>(ii)</skos:altLabel>
        <skos:definition xml:lang="en">There are some efforts to conduct background verification checks on candidates prior to joining the organisation and on an ongoing basis, but the checks may not fully consider applicable laws, regulations, and ethics, or adequately address the perceived risks.</skos:definition>
        <skos:prefLabel>MCQ73. Partially Implemented</skos:prefLabel>
    </owl:NamedIndividual>
    


    <!-- http://JP_ontology.org/assessment/MCQ73AnswerC -->


    <owl:NamedIndividual rdf:about="http://JP_ontology.org/assessment/MCQ73AnswerC">
        <rdf:type rdf:resource="http://JP_ontology.org/assessment/MCQ.73"/>
        <skos:altLabel>(iii)</skos:altLabel>
        <skos:definition xml:lang="en">Background verification checks on all candidates prior to joining the organisation and on an ongoing basis are conducted, ensuring compliance with applicable laws, regulations, and ethics, and proportionality to business requirements and perceived risks.</skos:definition>
        <skos:prefLabel>MCQ73. Fully Implemented</skos:prefLabel>
    </owl:NamedIndividual>
    


    <!-- http://JP_ontology.org/assessment/MCQ74AnswerA -->


    <owl:NamedIndividual rdf:about="http://JP_ontology.org/assessment/MCQ74AnswerA">
        <rdf:type rdf:resource="http://JP_ontology.org/assessment/MCQ.74"/>
        <skos:altLabel>(i)</skos:altLabel>
        <skos:definition xml:lang="en">The employment contractual agreements do not explicitly state the personnel’s and the organisation’s responsibilities for information security, potentially leading to ambiguity and lack of clarity regarding security expectations.</skos:definition>
        <skos:prefLabel>MCQ74. Not Implemented</skos:prefLabel>
    </owl:NamedIndividual>
    


    <!-- http://JP_ontology.org/assessment/MCQ74AnswerB -->


    <owl:NamedIndividual rdf:about="http://JP_ontology.org/assessment/MCQ74AnswerB">
        <rdf:type rdf:resource="http://JP_ontology.org/assessment/MCQ.74"/>
        <skos:altLabel>(ii)</skos:altLabel>
        <skos:definition xml:lang="en">There are some provisions in the employment contractual agreements that state the personnel’s and the organisation’s responsibilities for information security, but the coverage may be inconsistent or incomplete.</skos:definition>
        <skos:prefLabel>MCQ74. Partially Implemented</skos:prefLabel>
    </owl:NamedIndividual>
    


    <!-- http://JP_ontology.org/assessment/MCQ74AnswerC -->


    <owl:NamedIndividual rdf:about="http://JP_ontology.org/assessment/MCQ74AnswerC">
        <rdf:type rdf:resource="http://JP_ontology.org/assessment/MCQ.74"/>
        <skos:altLabel>(iii)</skos:altLabel>
        <skos:definition xml:lang="en">The employment contractual agreements clearly state both the personnel’s and the organisation’s responsibilities for information security, ensuring alignment of expectations and accountability for maintaining security standards.</skos:definition>
        <skos:prefLabel>MCQ74. Fully Implemented</skos:prefLabel>
    </owl:NamedIndividual>
    


    <!-- http://JP_ontology.org/assessment/MCQ75.1AnswerA -->


    <owl:NamedIndividual rdf:about="http://JP_ontology.org/assessment/MCQ75.1AnswerA">
        <rdf:type rdf:resource="http://JP_ontology.org/assessment/MCQ.75.1"/>
        <skos:altLabel xml:lang="en">(i)</skos:altLabel>
        <skos:definition xml:lang="en">Personnel of the organisation and relevant interested parties do not receive appropriate information security awareness, education, and training, leaving them ill-prepared to address security risks and threats.</skos:definition>
        <skos:prefLabel xml:lang="en">MCQ.75.1 - Not Implemented</skos:prefLabel>
    </owl:NamedIndividual>
    


    <!-- http://JP_ontology.org/assessment/MCQ75.1AnswerB -->


    <owl:NamedIndividual rdf:about="http://JP_ontology.org/assessment/MCQ75.1AnswerB">
        <rdf:type rdf:resource="http://JP_ontology.org/assessment/MCQ.75.1"/>
        <skos:altLabel xml:lang="en">(ii)</skos:altLabel>
        <skos:definition xml:lang="en">There are some efforts to provide personnel of the organisation and relevant interested parties with information security awareness, education, and training, but it may be inconsistent or not fully comprehensive.</skos:definition>
        <skos:prefLabel xml:lang="en">MCQ.75.1 - Partially Implemented</skos:prefLabel>
    </owl:NamedIndividual>
    


    <!-- http://JP_ontology.org/assessment/MCQ75.1AnswerC -->


    <owl:NamedIndividual rdf:about="http://JP_ontology.org/assessment/MCQ75.1AnswerC">
        <rdf:type rdf:resource="http://JP_ontology.org/assessment/MCQ.75.1"/>
        <skos:altLabel xml:lang="en">(iii)</skos:altLabel>
        <skos:definition xml:lang="en">Personnel of the organisation and relevant interested parties receive appropriate information security awareness, education, and training, ensuring they are well-equipped to understand and address security risks and threats effectively.</skos:definition>
        <skos:prefLabel xml:lang="en">MCQ.75.1 - Fully Implemented</skos:prefLabel>
    </owl:NamedIndividual>
    


    <!-- http://JP_ontology.org/assessment/MCQ75.2AnswerA -->


    <owl:NamedIndividual rdf:about="http://JP_ontology.org/assessment/MCQ75.2AnswerA">
        <rdf:type rdf:resource="http://JP_ontology.org/assessment/MCQ.75.2"/>
        <skos:altLabel xml:lang="en">(i)</skos:altLabel>
        <skos:definition xml:lang="en">Regular updates of the organisation&apos;s information security policy, topic-specific policies, and procedures relevant to their job function are not provided to personnel of the organisation and relevant interested parties, potentially leading to outdated practices and non-compliance with security standards.</skos:definition>
        <skos:prefLabel xml:lang="en">MCQ.75.2 - Not Implemented</skos:prefLabel>
    </owl:NamedIndividual>
    


    <!-- http://JP_ontology.org/assessment/MCQ75.2AnswerB -->


    <owl:NamedIndividual rdf:about="http://JP_ontology.org/assessment/MCQ75.2AnswerB">
        <rdf:type rdf:resource="http://JP_ontology.org/assessment/MCQ.75.2"/>
        <skos:altLabel xml:lang="en">(ii)</skos:altLabel>
        <skos:definition xml:lang="en">There are some efforts to provide regular updates of the organisation&apos;s information security policy, topic-specific policies, and procedures relevant to their job function to personnel of the organisation and relevant interested parties, but the updates may be inconsistent or not fully comprehensive.</skos:definition>
        <skos:prefLabel xml:lang="en">MCQ.75.2 - Partially Implemented</skos:prefLabel>
    </owl:NamedIndividual>
    


    <!-- http://JP_ontology.org/assessment/MCQ75.2AnswerC -->


    <owl:NamedIndividual rdf:about="http://JP_ontology.org/assessment/MCQ75.2AnswerC">
        <rdf:type rdf:resource="http://JP_ontology.org/assessment/MCQ.75.2"/>
        <skos:altLabel xml:lang="en">(iii)</skos:altLabel>
        <skos:definition xml:lang="en">Regular updates of the organisation&apos;s information security policy, topic-specific policies, and procedures relevant to their job function are fully provided to personnel of the organisation and relevant interested parties, ensuring they are well-informed and compliant with current security standards.</skos:definition>
        <skos:prefLabel xml:lang="en">MCQ.75.2 - Fully Implemented</skos:prefLabel>
    </owl:NamedIndividual>
    


    <!-- http://JP_ontology.org/assessment/MCQ76AnswerA -->


    <owl:NamedIndividual rdf:about="http://JP_ontology.org/assessment/MCQ76AnswerA">
        <rdf:type rdf:resource="http://JP_ontology.org/assessment/MCQ.76"/>
        <skos:altLabel xml:lang="en">(i)</skos:altLabel>
        <skos:definition xml:lang="en">A disciplinary process to take actions against personnel and other relevant interested parties who have committed an information security policy violation is not formalized or communicated, potentially leading to inconsistent responses and inadequate enforcement of security policies.</skos:definition>
        <skos:prefLabel xml:lang="en">MCQ.76 - Not Implemented</skos:prefLabel>
    </owl:NamedIndividual>
    


    <!-- http://JP_ontology.org/assessment/MCQ76AnswerB -->


    <owl:NamedIndividual rdf:about="http://JP_ontology.org/assessment/MCQ76AnswerB">
        <rdf:type rdf:resource="http://JP_ontology.org/assessment/MCQ.76"/>
        <skos:altLabel xml:lang="en">(ii)</skos:altLabel>
        <skos:definition xml:lang="en">There are some elements of a disciplinary process to take actions against personnel and other relevant interested parties who have committed an information security policy violation, but the process may not be fully formalized or effectively communicated.</skos:definition>
        <skos:prefLabel xml:lang="en">MCQ.76 - Partially Implemented</skos:prefLabel>
    </owl:NamedIndividual>
    


    <!-- http://JP_ontology.org/assessment/MCQ76AnswerC -->


    <owl:NamedIndividual rdf:about="http://JP_ontology.org/assessment/MCQ76AnswerC">
        <rdf:type rdf:resource="http://JP_ontology.org/assessment/MCQ.76"/>
        <skos:altLabel xml:lang="en">(iii)</skos:altLabel>
        <skos:definition xml:lang="en">A disciplinary process to take actions against personnel and other relevant interested parties who have committed an information security policy violation is fully formalized and communicated, ensuring consistent enforcement of security policies and accountability for non-compliance.</skos:definition>
        <skos:prefLabel xml:lang="en">MCQ.76 - Fully Implemented</skos:prefLabel>
    </owl:NamedIndividual>
    


    <!-- http://JP_ontology.org/assessment/MCQ77AnswerA -->


    <owl:NamedIndividual rdf:about="http://JP_ontology.org/assessment/MCQ77AnswerA">
        <rdf:type rdf:resource="http://JP_ontology.org/assessment/MCQ.77"/>
        <skos:altLabel>(i)</skos:altLabel>
        <skos:definition xml:lang="en">Information security responsibilities and duties that remain valid after termination or change of employment are not defined, enforced, or communicated, potentially leaving gaps in security measures and continuity.</skos:definition>
        <skos:prefLabel>MCQ77. Not Implemented</skos:prefLabel>
    </owl:NamedIndividual>
    


    <!-- http://JP_ontology.org/assessment/MCQ77AnswerB -->


    <owl:NamedIndividual rdf:about="http://JP_ontology.org/assessment/MCQ77AnswerB">
        <rdf:type rdf:resource="http://JP_ontology.org/assessment/MCQ.77"/>
        <skos:altLabel>(ii)</skos:altLabel>
        <skos:definition xml:lang="en">There are some efforts to define, enforce, and communicate information security responsibilities and duties that remain valid after termination or change of employment, but the process may be inconsistent or incomplete.</skos:definition>
        <skos:prefLabel>MCQ77. Partially Implemented</skos:prefLabel>
    </owl:NamedIndividual>
    


    <!-- http://JP_ontology.org/assessment/MCQ77AnswerC -->


    <owl:NamedIndividual rdf:about="http://JP_ontology.org/assessment/MCQ77AnswerC">
        <rdf:type rdf:resource="http://JP_ontology.org/assessment/MCQ.77"/>
        <skos:altLabel>(iii)</skos:altLabel>
        <skos:definition xml:lang="en">Information security responsibilities and duties that remain valid after termination or change of employment are fully defined, enforced, and communicated to relevant personnel and other interested parties, ensuring continuity and adherence to security measures.</skos:definition>
        <skos:prefLabel>MCQ77. Fully Implemented</skos:prefLabel>
    </owl:NamedIndividual>
    


    <!-- http://JP_ontology.org/assessment/MCQ78AnswerA -->


    <owl:NamedIndividual rdf:about="http://JP_ontology.org/assessment/MCQ78AnswerA">
        <rdf:type rdf:resource="http://JP_ontology.org/assessment/MCQ.78"/>
        <skos:altLabel xml:lang="en">(i)</skos:altLabel>
        <skos:definition xml:lang="en">Confidentiality or non-disclosure agreements reflecting the organisation&apos;s needs for the protection of information are not identified, documented, regularly reviewed, or signed by personnel and other relevant interested parties, potentially exposing sensitive information to unauthorized disclosure.</skos:definition>
        <skos:prefLabel xml:lang="en">MCQ.78 - Not Implemented</skos:prefLabel>
    </owl:NamedIndividual>
    


    <!-- http://JP_ontology.org/assessment/MCQ78AnswerB -->


    <owl:NamedIndividual rdf:about="http://JP_ontology.org/assessment/MCQ78AnswerB">
        <rdf:type rdf:resource="http://JP_ontology.org/assessment/MCQ.78"/>
        <skos:altLabel xml:lang="en">(ii)</skos:altLabel>
        <skos:definition xml:lang="en">There are some efforts to identify, document, regularly review, and sign confidentiality or non-disclosure agreements reflecting the organisation&apos;s needs for the protection of information, but the process may be inconsistent or not fully comprehensive.</skos:definition>
        <skos:prefLabel xml:lang="en">MCQ.78 - Partially Implemented</skos:prefLabel>
    </owl:NamedIndividual>
    


    <!-- http://JP_ontology.org/assessment/MCQ78AnswerC -->


    <owl:NamedIndividual rdf:about="http://JP_ontology.org/assessment/MCQ78AnswerC">
        <rdf:type rdf:resource="http://JP_ontology.org/assessment/MCQ.78"/>
        <skos:altLabel xml:lang="en">(iii)</skos:altLabel>
        <skos:definition xml:lang="en">Confidentiality or non-disclosure agreements reflecting the organisation&apos;s needs for the protection of information are fully identified, documented, regularly reviewed, and signed by personnel and other relevant interested parties, ensuring legal protection and safeguarding of sensitive information.</skos:definition>
        <skos:prefLabel xml:lang="en">MCQ.78 - Fully Implemented</skos:prefLabel>
    </owl:NamedIndividual>
    


    <!-- http://JP_ontology.org/assessment/MCQ79AnswerA -->


    <owl:NamedIndividual rdf:about="http://JP_ontology.org/assessment/MCQ79AnswerA">
        <rdf:type rdf:resource="http://JP_ontology.org/assessment/MCQ.79"/>
        <skos:altLabel xml:lang="en">(i)</skos:altLabel>
        <skos:definition xml:lang="en">Security measures are not implemented when personnel are working remotely, leaving information accessed, processed, or stored outside the organisation’s premises vulnerable to unauthorized access or breaches.</skos:definition>
        <skos:prefLabel xml:lang="en">MCQ.79 - Not Implemented</skos:prefLabel>
    </owl:NamedIndividual>
    


    <!-- http://JP_ontology.org/assessment/MCQ79AnswerB -->


    <owl:NamedIndividual rdf:about="http://JP_ontology.org/assessment/MCQ79AnswerB">
        <rdf:type rdf:resource="http://JP_ontology.org/assessment/MCQ.79"/>
        <skos:altLabel xml:lang="en">(ii)</skos:altLabel>
        <skos:definition xml:lang="en">There are some efforts to implement security measures when personnel are working remotely, but the measures may be inconsistent or not fully comprehensive in protecting information accessed, processed, or stored outside the organisation’s premises.</skos:definition>
        <skos:prefLabel xml:lang="en">MCQ.79 - Partially Implemented</skos:prefLabel>
    </owl:NamedIndividual>
    


    <!-- http://JP_ontology.org/assessment/MCQ79AnswerC -->


    <owl:NamedIndividual rdf:about="http://JP_ontology.org/assessment/MCQ79AnswerC">
        <rdf:type rdf:resource="http://JP_ontology.org/assessment/MCQ.79"/>
        <skos:altLabel xml:lang="en">(iii)</skos:altLabel>
        <skos:definition xml:lang="en">Security measures are fully implemented when personnel are working remotely, ensuring that information accessed, processed, or stored outside the organisation’s premises is adequately protected from unauthorized access or breaches.</skos:definition>
        <skos:prefLabel xml:lang="en">MCQ.79 - Fully Implemented</skos:prefLabel>
    </owl:NamedIndividual>
    


    <!-- http://JP_ontology.org/assessment/MCQ7AnswerA -->


    <owl:NamedIndividual rdf:about="http://JP_ontology.org/assessment/MCQ7AnswerA">
        <rdf:type rdf:resource="http://JP_ontology.org/assessment/MCQ.7"/>
        <skos:altLabel>(i)</skos:altLabel>
        <skos:definition xml:lang="en">Documented information and necessary documentation within the organisations information security management system are not tailored to the organisation&apos;s specific needs, lacking consideration for factors such as size, activities, processes, and personnel competence.</skos:definition>
        <skos:prefLabel>MCQ7. Not Implemented</skos:prefLabel>
    </owl:NamedIndividual>
    


    <!-- http://JP_ontology.org/assessment/MCQ7AnswerB -->


    <owl:NamedIndividual rdf:about="http://JP_ontology.org/assessment/MCQ7AnswerB">
        <rdf:type rdf:resource="http://JP_ontology.org/assessment/MCQ.7"/>
        <skos:altLabel>(ii)</skos:altLabel>
        <skos:definition xml:lang="en">There are some efforts to include documented information and necessary documentation in the organisation&apos;s information security management system according to its needs, but it may not fully account for factors such as size, activities, processes, and personnel competence in all instances.</skos:definition>
        <skos:prefLabel>MCQ7. Partially Implemented</skos:prefLabel>
    </owl:NamedIndividual>
    


    <!-- http://JP_ontology.org/assessment/MCQ7AnswerC -->


    <owl:NamedIndividual rdf:about="http://JP_ontology.org/assessment/MCQ7AnswerC">
        <rdf:type rdf:resource="http://JP_ontology.org/assessment/MCQ.7"/>
        <skos:altLabel>(iii)</skos:altLabel>
        <skos:definition xml:lang="en">Documented information and necessary documentation are comprehensively included in the organisation&apos;s information security management system according to its needs, meticulously considering factors such as size, activities, processes, products, services, complexity of processes, interactions, and personnel competence, ensuring alignment with organisational requirements.</skos:definition>
        <skos:prefLabel>MCQ7. Fully Implemented</skos:prefLabel>
    </owl:NamedIndividual>
    


    <!-- http://JP_ontology.org/assessment/MCQ8.1AnswerA -->


    <owl:NamedIndividual rdf:about="http://JP_ontology.org/assessment/MCQ8.1AnswerA">
        <rdf:type rdf:resource="http://JP_ontology.org/assessment/MCQ.8.1"/>
        <skos:altLabel xml:lang="en">(i)</skos:altLabel>
        <skos:definition xml:lang="en">The organisation does not conduct information security risk assessments at planned intervals or when significant changes are proposed or occur, potentially leaving the organisation vulnerable to evolving threats and vulnerabilities.</skos:definition>
        <skos:prefLabel xml:lang="en">MCQ.8.1 - Not Implemented</skos:prefLabel>
    </owl:NamedIndividual>
    


    <!-- http://JP_ontology.org/assessment/MCQ8.1AnswerB -->


    <owl:NamedIndividual rdf:about="http://JP_ontology.org/assessment/MCQ8.1AnswerB">
        <rdf:type rdf:resource="http://JP_ontology.org/assessment/MCQ.8.1"/>
        <skos:altLabel xml:lang="en">(ii)</skos:altLabel>
        <skos:definition xml:lang="en">There are some efforts by the organisation to conduct information security risk assessments at planned intervals or when significant changes are proposed or occur. However, the process may be inconsistent or not fully comprehensive.</skos:definition>
        <skos:prefLabel xml:lang="en">MCQ.8.1 - Partially Implemented</skos:prefLabel>
    </owl:NamedIndividual>
    


    <!-- http://JP_ontology.org/assessment/MCQ8.1AnswerC -->


    <owl:NamedIndividual rdf:about="http://JP_ontology.org/assessment/MCQ8.1AnswerC">
        <rdf:type rdf:resource="http://JP_ontology.org/assessment/MCQ.8.1"/>
        <skos:altLabel xml:lang="en">(iii)</skos:altLabel>
        <skos:definition xml:lang="en">The organisation fully conducts information security risk assessments at planned intervals or when significant changes are proposed or occur, ensuring proactive risk management and mitigation strategies are in place.</skos:definition>
        <skos:prefLabel xml:lang="en">MCQ.8.1 - Fully Implemented</skos:prefLabel>
    </owl:NamedIndividual>
    


    <!-- http://JP_ontology.org/assessment/MCQ8.2AnswerA -->


    <owl:NamedIndividual rdf:about="http://JP_ontology.org/assessment/MCQ8.2AnswerA">
        <rdf:type rdf:resource="http://JP_ontology.org/assessment/MCQ.8.2"/>
        <skos:altLabel xml:lang="en">(i)</skos:altLabel>
        <skos:definition xml:lang="en">The organisation does not retain documented information of the results of these assessments, potentially leading to a lack of historical data for analysis and decision-making in future assessments.</skos:definition>
        <skos:prefLabel xml:lang="en">MCQ.8.2 - Not Implemented</skos:prefLabel>
    </owl:NamedIndividual>
    


    <!-- http://JP_ontology.org/assessment/MCQ8.2AnswerB -->


    <owl:NamedIndividual rdf:about="http://JP_ontology.org/assessment/MCQ8.2AnswerB">
        <rdf:type rdf:resource="http://JP_ontology.org/assessment/MCQ.8.2"/>
        <skos:altLabel xml:lang="en">(ii)</skos:altLabel>
        <skos:definition xml:lang="en">There are some efforts by the organisation to retain documented information of the results of these assessments. However, the documentation may be incomplete or not consistently maintained.</skos:definition>
        <skos:prefLabel xml:lang="en">MCQ.8.2 - Partially Implemented</skos:prefLabel>
    </owl:NamedIndividual>
    


    <!-- http://JP_ontology.org/assessment/MCQ8.2AnswerC -->


    <owl:NamedIndividual rdf:about="http://JP_ontology.org/assessment/MCQ8.2AnswerC">
        <rdf:type rdf:resource="http://JP_ontology.org/assessment/MCQ.8.2"/>
        <skos:altLabel xml:lang="en">(iii)</skos:altLabel>
        <skos:definition xml:lang="en">The organisation fully retains documented information of the results of these assessments, ensuring comprehensive records are maintained for analysis, decision-making, and reference purposes.</skos:definition>
        <skos:prefLabel xml:lang="en">MCQ.8.2 - Fully Implemented</skos:prefLabel>
    </owl:NamedIndividual>
    


    <!-- http://JP_ontology.org/assessment/MCQ80AnswerA -->


    <owl:NamedIndividual rdf:about="http://JP_ontology.org/assessment/MCQ80AnswerA">
        <rdf:type rdf:resource="http://JP_ontology.org/assessment/MCQ.80"/>
        <skos:altLabel xml:lang="en">(i)</skos:altLabel>
        <skos:definition xml:lang="en">Rules to control physical and logical access to information and associated assets are not established or implemented, lacking alignment with business and information security requirements.</skos:definition>
        <skos:prefLabel xml:lang="en">MCQ.80 - Not Implemented</skos:prefLabel>
    </owl:NamedIndividual>
    


    <!-- http://JP_ontology.org/assessment/MCQ80AnswerB -->


    <owl:NamedIndividual rdf:about="http://JP_ontology.org/assessment/MCQ80AnswerB">
        <rdf:type rdf:resource="http://JP_ontology.org/assessment/MCQ.80"/>
        <skos:altLabel xml:lang="en">(ii)</skos:altLabel>
        <skos:definition xml:lang="en">There are some rules established to control physical and logical access to information and associated assets, but they may not fully align with both business and information security requirements, leading to potential gaps in access control.</skos:definition>
        <skos:prefLabel xml:lang="en">MCQ.80 - Partially Implemented</skos:prefLabel>
    </owl:NamedIndividual>
    


    <!-- http://JP_ontology.org/assessment/MCQ80AnswerC -->


    <owl:NamedIndividual rdf:about="http://JP_ontology.org/assessment/MCQ80AnswerC">
        <rdf:type rdf:resource="http://JP_ontology.org/assessment/MCQ.80"/>
        <skos:altLabel xml:lang="en">(iii)</skos:altLabel>
        <skos:definition xml:lang="en">Comprehensive rules are established and rigorously implemented to control physical and logical access to information and associated assets, ensuring alignment with both business and information security requirements for effective access control.</skos:definition>
        <skos:prefLabel xml:lang="en">MCQ.80 - Fully Implemented</skos:prefLabel>
    </owl:NamedIndividual>
    


    <!-- http://JP_ontology.org/assessment/MCQ81AnswerA -->


    <owl:NamedIndividual rdf:about="http://JP_ontology.org/assessment/MCQ81AnswerA">
        <rdf:type rdf:resource="http://JP_ontology.org/assessment/MCQ.81"/>
        <skos:altLabel xml:lang="en">(i)</skos:altLabel>
        <skos:definition xml:lang="en">The organisation lacks a structured approach to managing the complete life cycle of identities, leading to inconsistencies and gaps in identity-related processes such as creation, authentication, and termination.</skos:definition>
        <skos:prefLabel xml:lang="en">MCQ.81 - Not Implemented</skos:prefLabel>
    </owl:NamedIndividual>
    


    <!-- http://JP_ontology.org/assessment/MCQ81AnswerB -->


    <owl:NamedIndividual rdf:about="http://JP_ontology.org/assessment/MCQ81AnswerB">
        <rdf:type rdf:resource="http://JP_ontology.org/assessment/MCQ.81"/>
        <skos:altLabel xml:lang="en">(ii)</skos:altLabel>
        <skos:definition xml:lang="en">There are some efforts to manage the complete life cycle of identities, including activities such as creation, authentication, and periodic reviews, but the process may be inconsistent or lacking in certain areas.</skos:definition>
        <skos:prefLabel xml:lang="en">MCQ.81 - Partially Implemented</skos:prefLabel>
    </owl:NamedIndividual>
    


    <!-- http://JP_ontology.org/assessment/MCQ81AnswerC -->


    <owl:NamedIndividual rdf:about="http://JP_ontology.org/assessment/MCQ81AnswerC">
        <rdf:type rdf:resource="http://JP_ontology.org/assessment/MCQ.81"/>
        <skos:altLabel xml:lang="en">(iii)</skos:altLabel>
        <skos:definition xml:lang="en">The organisation has implemented a comprehensive approach to managing the complete life cycle of identities, covering all activities from creation to termination, and ensuring robust oversight and control over identity-related processes.</skos:definition>
        <skos:prefLabel xml:lang="en">MCQ.81 - Fully Implemented</skos:prefLabel>
    </owl:NamedIndividual>
    


    <!-- http://JP_ontology.org/assessment/MCQ82AnswerA -->


    <owl:NamedIndividual rdf:about="http://JP_ontology.org/assessment/MCQ82AnswerA">
        <rdf:type rdf:resource="http://JP_ontology.org/assessment/MCQ.82"/>
        <skos:altLabel xml:lang="en">(i)</skos:altLabel>
        <skos:definition xml:lang="en">There is no management process in place to control the allocation and management of authentication information, and personnel are not advised on the appropriate handling of authentication information.</skos:definition>
        <skos:prefLabel xml:lang="en">MCQ.82 - Not Implemented</skos:prefLabel>
    </owl:NamedIndividual>
    


    <!-- http://JP_ontology.org/assessment/MCQ82AnswerB -->


    <owl:NamedIndividual rdf:about="http://JP_ontology.org/assessment/MCQ82AnswerB">
        <rdf:type rdf:resource="http://JP_ontology.org/assessment/MCQ.82"/>
        <skos:altLabel xml:lang="en">(ii)</skos:altLabel>
        <skos:definition xml:lang="en">There are some efforts to control the allocation and management of authentication information through a management process, but personnel may not consistently receive advice on the appropriate handling of authentication information.</skos:definition>
        <skos:prefLabel xml:lang="en">MCQ.82 - Partially Implemented</skos:prefLabel>
    </owl:NamedIndividual>
    


    <!-- http://JP_ontology.org/assessment/MCQ82AnswerC -->


    <owl:NamedIndividual rdf:about="http://JP_ontology.org/assessment/MCQ82AnswerC">
        <rdf:type rdf:resource="http://JP_ontology.org/assessment/MCQ.82"/>
        <skos:altLabel xml:lang="en">(iii)</skos:altLabel>
        <skos:definition xml:lang="en">The allocation and management of authentication information are controlled by a robust management process, which includes advising personnel on the appropriate handling of authentication information, ensuring secure and effective management of authentication credentials.</skos:definition>
        <skos:prefLabel xml:lang="en">MCQ.82 - Fully Implemented</skos:prefLabel>
    </owl:NamedIndividual>
    


    <!-- http://JP_ontology.org/assessment/MCQ83AnswerA -->


    <owl:NamedIndividual rdf:about="http://JP_ontology.org/assessment/MCQ83AnswerA">
        <rdf:type rdf:resource="http://JP_ontology.org/assessment/MCQ.83"/>
        <skos:altLabel xml:lang="en">(i)</skos:altLabel>
        <skos:definition xml:lang="en">Access rights to information and associated assets are not provisioned, reviewed, modified, or removed in accordance with the organisation’s topic-specific policy and rules for access control, leading to inconsistencies and potential security risks.</skos:definition>
        <skos:prefLabel xml:lang="en">MCQ.83 - Not Implemented</skos:prefLabel>
    </owl:NamedIndividual>
    


    <!-- http://JP_ontology.org/assessment/MCQ83AnswerB -->


    <owl:NamedIndividual rdf:about="http://JP_ontology.org/assessment/MCQ83AnswerB">
        <rdf:type rdf:resource="http://JP_ontology.org/assessment/MCQ.83"/>
        <skos:altLabel xml:lang="en">(ii)</skos:altLabel>
        <skos:definition xml:lang="en">There are some efforts to provision, review, modify, and remove access rights in accordance with the organisation’s topic-specific policy and rules for access control, but the process may be inconsistent or incomplete.</skos:definition>
        <skos:prefLabel xml:lang="en">MCQ.83 - Partially Implemented</skos:prefLabel>
    </owl:NamedIndividual>
    


    <!-- http://JP_ontology.org/assessment/MCQ83AnswerC -->


    <owl:NamedIndividual rdf:about="http://JP_ontology.org/assessment/MCQ83AnswerC">
        <rdf:type rdf:resource="http://JP_ontology.org/assessment/MCQ.83"/>
        <skos:altLabel xml:lang="en">(iii)</skos:altLabel>
        <skos:definition xml:lang="en">Access rights to information and associated assets are provisioned, reviewed, modified, and removed in strict accordance with the organisation’s topic-specific policy and rules for access control, ensuring effective access management and adherence to security requirements.</skos:definition>
        <skos:prefLabel xml:lang="en">MCQ.83 - Fully Implemented</skos:prefLabel>
    </owl:NamedIndividual>
    


    <!-- http://JP_ontology.org/assessment/MCQ84AnswerA -->


    <owl:NamedIndividual rdf:about="http://JP_ontology.org/assessment/MCQ84AnswerA">
        <rdf:type rdf:resource="http://JP_ontology.org/assessment/MCQ.84"/>
        <skos:altLabel xml:lang="en">(i)</skos:altLabel>
        <skos:definition xml:lang="en">The allocation and use of privileged access rights are not restricted or managed, potentially leading to unauthorized access to sensitive systems and data.</skos:definition>
        <skos:prefLabel xml:lang="en">MCQ.84 - Not Implemented</skos:prefLabel>
    </owl:NamedIndividual>
    


    <!-- http://JP_ontology.org/assessment/MCQ84AnswerB -->


    <owl:NamedIndividual rdf:about="http://JP_ontology.org/assessment/MCQ84AnswerB">
        <rdf:type rdf:resource="http://JP_ontology.org/assessment/MCQ.84"/>
        <skos:altLabel xml:lang="en">(ii)</skos:altLabel>
        <skos:definition xml:lang="en">There are some efforts to restrict and manage the allocation and use of privileged access rights, but the process may be inconsistent or not fully comprehensive.</skos:definition>
        <skos:prefLabel xml:lang="en">MCQ.84 - Partially Implemented</skos:prefLabel>
    </owl:NamedIndividual>
    


    <!-- http://JP_ontology.org/assessment/MCQ84AnswerC -->


    <owl:NamedIndividual rdf:about="http://JP_ontology.org/assessment/MCQ84AnswerC">
        <rdf:type rdf:resource="http://JP_ontology.org/assessment/MCQ.84"/>
        <skos:altLabel xml:lang="en">(iii)</skos:altLabel>
        <skos:definition xml:lang="en">The allocation and use of privileged access rights are fully restricted and managed, ensuring that only authorized personnel have access to sensitive systems and data, and activities are monitored and audited for compliance.</skos:definition>
        <skos:prefLabel xml:lang="en">MCQ.84 - Fully Implemented</skos:prefLabel>
    </owl:NamedIndividual>
    


    <!-- http://JP_ontology.org/assessment/MCQ85AnswerA -->


    <owl:NamedIndividual rdf:about="http://JP_ontology.org/assessment/MCQ85AnswerA">
        <rdf:type rdf:resource="http://JP_ontology.org/assessment/MCQ.85"/>
        <skos:altLabel xml:lang="en">(i)</skos:altLabel>
        <skos:definition xml:lang="en">Access to information and other associated assets is not restricted in accordance with the established topic-specific policy on access control, potentially leading to unauthorized access and compromise of sensitive assets.</skos:definition>
        <skos:prefLabel xml:lang="en">MCQ.85 - Not Implemented</skos:prefLabel>
    </owl:NamedIndividual>
    


    <!-- http://JP_ontology.org/assessment/MCQ85AnswerB -->


    <owl:NamedIndividual rdf:about="http://JP_ontology.org/assessment/MCQ85AnswerB">
        <rdf:type rdf:resource="http://JP_ontology.org/assessment/MCQ.85"/>
        <skos:altLabel xml:lang="en">(ii)</skos:altLabel>
        <skos:definition xml:lang="en">There are some efforts to restrict access to information and other associated assets in accordance with the established topic-specific policy on access control, but the implementation may be inconsistent or incomplete.</skos:definition>
        <skos:prefLabel xml:lang="en">MCQ.85 - Partially Implemented</skos:prefLabel>
    </owl:NamedIndividual>
    


    <!-- http://JP_ontology.org/assessment/MCQ85AnswerC -->


    <owl:NamedIndividual rdf:about="http://JP_ontology.org/assessment/MCQ85AnswerC">
        <rdf:type rdf:resource="http://JP_ontology.org/assessment/MCQ.85"/>
        <skos:altLabel xml:lang="en">(iii)</skos:altLabel>
        <skos:definition xml:lang="en">Access to information and other associated assets is fully restricted in accordance with the established topic-specific policy on access control, ensuring that access is granted only to authorized individuals based on defined criteria and requirements.</skos:definition>
        <skos:prefLabel xml:lang="en">MCQ.85 - Fully Implemented</skos:prefLabel>
    </owl:NamedIndividual>
    


    <!-- http://JP_ontology.org/assessment/MCQ86AnswerA -->


    <owl:NamedIndividual rdf:about="http://JP_ontology.org/assessment/MCQ86AnswerA">
        <rdf:type rdf:resource="http://JP_ontology.org/assessment/MCQ.86"/>
        <skos:altLabel xml:lang="en">(i)</skos:altLabel>
        <skos:definition xml:lang="en">Read and write access to source code, development tools, and software libraries is not appropriately managed, potentially leading to unauthorized modifications, code leaks, or security breaches.</skos:definition>
        <skos:prefLabel xml:lang="en">MCQ.86 - Not Implemented</skos:prefLabel>
    </owl:NamedIndividual>
    


    <!-- http://JP_ontology.org/assessment/MCQ86AnswerB -->


    <owl:NamedIndividual rdf:about="http://JP_ontology.org/assessment/MCQ86AnswerB">
        <rdf:type rdf:resource="http://JP_ontology.org/assessment/MCQ.86"/>
        <skos:altLabel xml:lang="en">(ii)</skos:altLabel>
        <skos:definition xml:lang="en">There are some efforts to manage read and write access to source code, development tools, and software libraries, but the management may be inconsistent or not fully comprehensive.</skos:definition>
        <skos:prefLabel xml:lang="en">MCQ.86 - Partially Implemented</skos:prefLabel>
    </owl:NamedIndividual>
    


    <!-- http://JP_ontology.org/assessment/MCQ86AnswerC -->


    <owl:NamedIndividual rdf:about="http://JP_ontology.org/assessment/MCQ86AnswerC">
        <rdf:type rdf:resource="http://JP_ontology.org/assessment/MCQ.86"/>
        <skos:altLabel xml:lang="en">(iii)</skos:altLabel>
        <skos:definition xml:lang="en">Read and write access to source code, development tools, and software libraries is fully and appropriately managed, ensuring that access is granted only to authorized personnel and activities are monitored and controlled to prevent unauthorized modifications or breaches.</skos:definition>
        <skos:prefLabel xml:lang="en">MCQ.86 - Fully Implemented</skos:prefLabel>
    </owl:NamedIndividual>
    


    <!-- http://JP_ontology.org/assessment/MCQ87AnswerA -->


    <owl:NamedIndividual rdf:about="http://JP_ontology.org/assessment/MCQ87AnswerA">
        <rdf:type rdf:resource="http://JP_ontology.org/assessment/MCQ.87"/>
        <skos:altLabel xml:lang="en">(i)</skos:altLabel>
        <skos:definition xml:lang="en">Secure authentication technologies and procedures are not implemented based on information access restrictions and the topic-specific policy on access control, resulting in potential vulnerabilities and unauthorized access.</skos:definition>
        <skos:prefLabel xml:lang="en">MCQ.87 - Not Implemented</skos:prefLabel>
    </owl:NamedIndividual>
    


    <!-- http://JP_ontology.org/assessment/MCQ87AnswerB -->


    <owl:NamedIndividual rdf:about="http://JP_ontology.org/assessment/MCQ87AnswerB">
        <rdf:type rdf:resource="http://JP_ontology.org/assessment/MCQ.87"/>
        <skos:altLabel xml:lang="en">(ii)</skos:altLabel>
        <skos:definition xml:lang="en">There are some efforts to implement secure authentication technologies and procedures based on information access restrictions and the topic-specific policy on access control, but the implementation may be incomplete or inconsistent.</skos:definition>
        <skos:prefLabel xml:lang="en">MCQ.87 - Partially Implemented</skos:prefLabel>
    </owl:NamedIndividual>
    


    <!-- http://JP_ontology.org/assessment/MCQ87AnswerC -->


    <owl:NamedIndividual rdf:about="http://JP_ontology.org/assessment/MCQ87AnswerC">
        <rdf:type rdf:resource="http://JP_ontology.org/assessment/MCQ.87"/>
        <skos:altLabel xml:lang="en">(iii)</skos:altLabel>
        <skos:definition xml:lang="en">Secure authentication technologies and procedures are fully implemented based on information access restrictions and the topic-specific policy on access control, ensuring robust access security and compliance with organisational policies.</skos:definition>
        <skos:prefLabel xml:lang="en">MCQ.87 - Fully Implemented</skos:prefLabel>
    </owl:NamedIndividual>
    


    <!-- http://JP_ontology.org/assessment/MCQ88AnswerA -->


    <owl:NamedIndividual rdf:about="http://JP_ontology.org/assessment/MCQ88AnswerA">
        <rdf:type rdf:resource="http://JP_ontology.org/assessment/MCQ.88"/>
        <skos:altLabel xml:lang="en">(i)</skos:altLabel>
        <skos:definition xml:lang="en">The use of utility programs capable of overriding system and application controls is not restricted or tightly controlled, posing risks of unauthorized system modifications or security breaches.</skos:definition>
        <skos:prefLabel xml:lang="en">MCQ.88 - Not Implemented</skos:prefLabel>
    </owl:NamedIndividual>
    


    <!-- http://JP_ontology.org/assessment/MCQ88AnswerB -->


    <owl:NamedIndividual rdf:about="http://JP_ontology.org/assessment/MCQ88AnswerB">
        <rdf:type rdf:resource="http://JP_ontology.org/assessment/MCQ.88"/>
        <skos:altLabel xml:lang="en">(ii)</skos:altLabel>
        <skos:definition xml:lang="en">There are some efforts to restrict and tightly control the use of utility programs capable of overriding system and application controls, but the controls may be inconsistent or not fully comprehensive.</skos:definition>
        <skos:prefLabel xml:lang="en">MCQ.88 - Partially Implemented</skos:prefLabel>
    </owl:NamedIndividual>
    


    <!-- http://JP_ontology.org/assessment/MCQ88AnswerC -->


    <owl:NamedIndividual rdf:about="http://JP_ontology.org/assessment/MCQ88AnswerC">
        <rdf:type rdf:resource="http://JP_ontology.org/assessment/MCQ.88"/>
        <skos:altLabel xml:lang="en">(iii)</skos:altLabel>
        <skos:definition xml:lang="en">The use of utility programs capable of overriding system and application controls is fully restricted and tightly controlled, ensuring that such programs are only used by authorized personnel for legitimate purposes and activities are closely monitored to prevent misuse.</skos:definition>
        <skos:prefLabel xml:lang="en">MCQ.88 - Fully Implemented</skos:prefLabel>
    </owl:NamedIndividual>
    


    <!-- http://JP_ontology.org/assessment/MCQ89AnswerA -->


    <owl:NamedIndividual rdf:about="http://JP_ontology.org/assessment/MCQ89AnswerA">
        <rdf:type rdf:resource="http://JP_ontology.org/assessment/MCQ.89"/>
        <skos:altLabel xml:lang="en">(i)</skos:altLabel>
        <skos:definition xml:lang="en">An inventory of information and other associated assets, including owners, is not developed or maintained, leading to lack of visibility and control over organisational assets.</skos:definition>
        <skos:prefLabel xml:lang="en">MCQ.89 - Not Implemented</skos:prefLabel>
    </owl:NamedIndividual>
    


    <!-- http://JP_ontology.org/assessment/MCQ89AnswerB -->


    <owl:NamedIndividual rdf:about="http://JP_ontology.org/assessment/MCQ89AnswerB">
        <rdf:type rdf:resource="http://JP_ontology.org/assessment/MCQ.89"/>
        <skos:altLabel xml:lang="en">(ii)</skos:altLabel>
        <skos:definition xml:lang="en">There are some efforts to develop and maintain an inventory of information and other associated assets, including owners, but the inventory may be incomplete or not regularly updated.</skos:definition>
        <skos:prefLabel xml:lang="en">MCQ.89 - Partially Implemented</skos:prefLabel>
    </owl:NamedIndividual>
    


    <!-- http://JP_ontology.org/assessment/MCQ89AnswerC -->


    <owl:NamedIndividual rdf:about="http://JP_ontology.org/assessment/MCQ89AnswerC">
        <rdf:type rdf:resource="http://JP_ontology.org/assessment/MCQ.89"/>
        <skos:altLabel xml:lang="en">(iii)</skos:altLabel>
        <skos:definition xml:lang="en">An inventory of information and other associated assets, including owners, is fully developed and maintained, providing comprehensive visibility and control over organisational assets and their ownership.</skos:definition>
        <skos:prefLabel xml:lang="en">MCQ.89 - Fully Implemented</skos:prefLabel>
    </owl:NamedIndividual>
    


    <!-- http://JP_ontology.org/assessment/MCQ9.1AnswerA -->


    <owl:NamedIndividual rdf:about="http://JP_ontology.org/assessment/MCQ9.1AnswerA">
        <rdf:type rdf:resource="http://JP_ontology.org/assessment/MCQ.9.1"/>
        <skos:altLabel xml:lang="en">(i)</skos:altLabel>
        <skos:definition xml:lang="en">The organisation does not implement the information security risk treatment plan, potentially leaving identified risks unaddressed and the organisation vulnerable to security threats.</skos:definition>
        <skos:prefLabel xml:lang="en">MCQ.9.1 - Not Implemented</skos:prefLabel>
    </owl:NamedIndividual>
    


    <!-- http://JP_ontology.org/assessment/MCQ9.1AnswerB -->


    <owl:NamedIndividual rdf:about="http://JP_ontology.org/assessment/MCQ9.1AnswerB">
        <rdf:type rdf:resource="http://JP_ontology.org/assessment/MCQ.9.1"/>
        <skos:altLabel xml:lang="en">(ii)</skos:altLabel>
        <skos:definition xml:lang="en">There are some efforts by the organisation to implement the information security risk treatment plan. However, the implementation may be inconsistent or not fully comprehensive.</skos:definition>
        <skos:prefLabel xml:lang="en">MCQ.9.1 - Partially Implemented</skos:prefLabel>
    </owl:NamedIndividual>
    


    <!-- http://JP_ontology.org/assessment/MCQ9.1AnswerC -->


    <owl:NamedIndividual rdf:about="http://JP_ontology.org/assessment/MCQ9.1AnswerC">
        <rdf:type rdf:resource="http://JP_ontology.org/assessment/MCQ.9.1"/>
        <skos:altLabel xml:lang="en">(iii)</skos:altLabel>
        <skos:definition xml:lang="en">The organisation fully implements the information security risk treatment plan, ensuring that identified risks are addressed effectively and appropriate measures are put in place to mitigate or manage those risks.</skos:definition>
        <skos:prefLabel xml:lang="en">MCQ.9.1 - Fully Implemented</skos:prefLabel>
    </owl:NamedIndividual>
    


    <!-- http://JP_ontology.org/assessment/MCQ9.2AnswerA -->


    <owl:NamedIndividual rdf:about="http://JP_ontology.org/assessment/MCQ9.2AnswerA">
        <rdf:type rdf:resource="http://JP_ontology.org/assessment/MCQ.9.2"/>
        <skos:altLabel xml:lang="en">(i)</skos:altLabel>
        <skos:definition xml:lang="en">The organisation does not retain documented information of the results of the information security risk treatment, potentially leading to a lack of accountability and traceability in the risk management process.</skos:definition>
        <skos:prefLabel xml:lang="en">MCQ.9.2 - Not Implemented</skos:prefLabel>
    </owl:NamedIndividual>
    


    <!-- http://JP_ontology.org/assessment/MCQ9.2AnswerB -->


    <owl:NamedIndividual rdf:about="http://JP_ontology.org/assessment/MCQ9.2AnswerB">
        <rdf:type rdf:resource="http://JP_ontology.org/assessment/MCQ.9.2"/>
        <skos:altLabel xml:lang="en">(ii)</skos:altLabel>
        <skos:definition xml:lang="en">There are some efforts by the organisation to retain documented information of the results of the information security risk treatment. However, the documentation may be incomplete or not consistently maintained.</skos:definition>
        <skos:prefLabel xml:lang="en">MCQ.9.2 - Partially Implemented</skos:prefLabel>
    </owl:NamedIndividual>
    


    <!-- http://JP_ontology.org/assessment/MCQ9.2AnswerC -->


    <owl:NamedIndividual rdf:about="http://JP_ontology.org/assessment/MCQ9.2AnswerC">
        <rdf:type rdf:resource="http://JP_ontology.org/assessment/MCQ.9.2"/>
        <skos:altLabel xml:lang="en">(iii)</skos:altLabel>
        <skos:definition xml:lang="en">The organisation fully retains documented information of the results of the information security risk treatment, ensuring comprehensive records are maintained for analysis, audit, and reference purposes.</skos:definition>
        <skos:prefLabel xml:lang="en">MCQ.9.2 - Fully Implemented</skos:prefLabel>
    </owl:NamedIndividual>
    


    <!-- http://JP_ontology.org/assessment/MCQ90AnswerA -->


    <owl:NamedIndividual rdf:about="http://JP_ontology.org/assessment/MCQ90AnswerA">
        <rdf:type rdf:resource="http://JP_ontology.org/assessment/MCQ.90"/>
        <skos:altLabel xml:lang="en">(i)</skos:altLabel>
        <skos:definition xml:lang="en">Rules for acceptable use and procedures for handling information and other associated assets are not identified, documented, or implemented, potentially leading to misuse or mishandling of sensitive information.</skos:definition>
        <skos:prefLabel xml:lang="en">MCQ.90 - Not Implemented</skos:prefLabel>
    </owl:NamedIndividual>
    


    <!-- http://JP_ontology.org/assessment/MCQ90AnswerB -->


    <owl:NamedIndividual rdf:about="http://JP_ontology.org/assessment/MCQ90AnswerB">
        <rdf:type rdf:resource="http://JP_ontology.org/assessment/MCQ.90"/>
        <skos:altLabel xml:lang="en">(ii)</skos:altLabel>
        <skos:definition xml:lang="en">There are some efforts to identify, document, and implement rules for acceptable use and procedures for handling information and other associated assets, but the documentation may be incomplete or not consistently followed.</skos:definition>
        <skos:prefLabel xml:lang="en">MCQ.90 - Partially Implemented</skos:prefLabel>
    </owl:NamedIndividual>
    


    <!-- http://JP_ontology.org/assessment/MCQ90AnswerC -->


    <owl:NamedIndividual rdf:about="http://JP_ontology.org/assessment/MCQ90AnswerC">
        <rdf:type rdf:resource="http://JP_ontology.org/assessment/MCQ.90"/>
        <skos:altLabel xml:lang="en">(iii)</skos:altLabel>
        <skos:definition xml:lang="en">Rules for acceptable use and procedures for handling information and other associated assets are fully identified, documented, and implemented, ensuring that personnel understand and adhere to appropriate practices for safeguarding sensitive information.</skos:definition>
        <skos:prefLabel xml:lang="en">MCQ.90 - Fully Implemented</skos:prefLabel>
    </owl:NamedIndividual>
    


    <!-- http://JP_ontology.org/assessment/MCQ91.1AnswerA -->


    <owl:NamedIndividual rdf:about="http://JP_ontology.org/assessment/MCQ91.1AnswerA">
        <rdf:type rdf:resource="http://JP_ontology.org/assessment/MCQ.91.1"/>
        <skos:altLabel>(i)</skos:altLabel>
        <skos:definition xml:lang="en">Personnel and other relevant parties are not required to return all of the organisation&apos;s assets in their possession upon the change or termination of their employment, contract, or agreement, potentially resulting in loss of organisational assets and compromised security.</skos:definition>
        <skos:prefLabel>MCQ91.1. Not Implemented</skos:prefLabel>
    </owl:NamedIndividual>
    


    <!-- http://JP_ontology.org/assessment/MCQ91.1AnswerB -->


    <owl:NamedIndividual rdf:about="http://JP_ontology.org/assessment/MCQ91.1AnswerB">
        <rdf:type rdf:resource="http://JP_ontology.org/assessment/MCQ.91.1"/>
        <skos:altLabel>(ii)</skos:altLabel>
        <skos:definition xml:lang="en">There are some requirements for personnel and other relevant parties to return organisation&apos;s assets upon the change or termination of their employment, contract, or agreement, but the process may be inconsistent or not fully enforced.</skos:definition>
        <skos:prefLabel>MCQ91.1. Partially Implemented</skos:prefLabel>
    </owl:NamedIndividual>
    


    <!-- http://JP_ontology.org/assessment/MCQ91.1AnswerC -->


    <owl:NamedIndividual rdf:about="http://JP_ontology.org/assessment/MCQ91.1AnswerC">
        <rdf:type rdf:resource="http://JP_ontology.org/assessment/MCQ.91.1"/>
        <skos:altLabel>(iii)</skos:altLabel>
        <skos:definition xml:lang="en">Personnel and other relevant parties are required to return all of the organisation&apos;s assets in their possession upon the change or termination of their employment, contract, or agreement, ensuring protection of organisational assets and maintaining security measures.</skos:definition>
        <skos:prefLabel>MCQ91.1. Fully Implemented</skos:prefLabel>
    </owl:NamedIndividual>
    


    <!-- http://JP_ontology.org/assessment/MCQ91.2AnswerA -->


    <owl:NamedIndividual rdf:about="http://JP_ontology.org/assessment/MCQ91.2AnswerA">
        <rdf:type rdf:resource="http://JP_ontology.org/assessment/MCQ.91.2"/>
        <skos:altLabel>(i)</skos:altLabel>
        <skos:definition xml:lang="en">Measures to ensure the protection of off-site assets from unauthorized access, theft, damage, or other risks are not implemented, leaving assets vulnerable to security breaches or loss.</skos:definition>
        <skos:prefLabel>MCQ91.2. Not Implemented</skos:prefLabel>
    </owl:NamedIndividual>
    


    <!-- http://JP_ontology.org/assessment/MCQ91.2AnswerB -->


    <owl:NamedIndividual rdf:about="http://JP_ontology.org/assessment/MCQ91.2AnswerB">
        <rdf:type rdf:resource="http://JP_ontology.org/assessment/MCQ.91.2"/>
        <skos:altLabel>(ii)</skos:altLabel>
        <skos:definition xml:lang="en">There are some measures in place to ensure the protection of off-site assets from unauthorized access, theft, damage, or other risks, but the measures may be inconsistent or not fully comprehensive.</skos:definition>
        <skos:prefLabel>MCQ91.2. Partially Implemented</skos:prefLabel>
    </owl:NamedIndividual>
    


    <!-- http://JP_ontology.org/assessment/MCQ91.2AnswerC -->


    <owl:NamedIndividual rdf:about="http://JP_ontology.org/assessment/MCQ91.2AnswerC">
        <rdf:type rdf:resource="http://JP_ontology.org/assessment/MCQ.91.2"/>
        <skos:altLabel>(iii)</skos:altLabel>
        <skos:definition xml:lang="en">Measures to ensure the protection of off-site assets from unauthorized access, theft, damage, or other risks are fully implemented, safeguarding the integrity, confidentiality, and availability of assets even when they are located outside the organisation&apos;s premises.</skos:definition>
        <skos:prefLabel>MCQ91.2. Fully Implemented</skos:prefLabel>
    </owl:NamedIndividual>
    


    <!-- http://JP_ontology.org/assessment/MCQ92AnswerA -->


    <owl:NamedIndividual rdf:about="http://JP_ontology.org/assessment/MCQ92AnswerA">
        <rdf:type rdf:resource="http://JP_ontology.org/assessment/MCQ.92"/>
        <skos:altLabel xml:lang="en">(i)</skos:altLabel>
        <skos:definition xml:lang="en">Storage media are not managed through their life cycle of acquisition, use, transportation, and disposal in accordance with the organisation’s classification scheme and handling requirements, potentially leading to mishandling of sensitive data and security breaches.</skos:definition>
        <skos:prefLabel xml:lang="en">MCQ.92 - Not Implemented</skos:prefLabel>
    </owl:NamedIndividual>
    


    <!-- http://JP_ontology.org/assessment/MCQ92AnswerB -->


    <owl:NamedIndividual rdf:about="http://JP_ontology.org/assessment/MCQ92AnswerB">
        <rdf:type rdf:resource="http://JP_ontology.org/assessment/MCQ.92"/>
        <skos:altLabel xml:lang="en">(ii)</skos:altLabel>
        <skos:definition xml:lang="en">There are some efforts to manage storage media through their life cycle, but the management may be inconsistent or not fully aligned with the organisation’s classification scheme and handling requirements.</skos:definition>
        <skos:prefLabel xml:lang="en">MCQ.92 - Partially Implemented</skos:prefLabel>
    </owl:NamedIndividual>
    


    <!-- http://JP_ontology.org/assessment/MCQ92AnswerC -->


    <owl:NamedIndividual rdf:about="http://JP_ontology.org/assessment/MCQ92AnswerC">
        <rdf:type rdf:resource="http://JP_ontology.org/assessment/MCQ.92"/>
        <skos:altLabel xml:lang="en">(iii)</skos:altLabel>
        <skos:definition xml:lang="en">Storage media are fully managed through their life cycle of acquisition, use, transportation, and disposal in accordance with the organisation’s classification scheme and handling requirements, ensuring proper protection and handling of sensitive data at all stages.</skos:definition>
        <skos:prefLabel xml:lang="en">MCQ.92 - Fully Implemented</skos:prefLabel>
    </owl:NamedIndividual>
    


    <!-- http://JP_ontology.org/assessment/MCQ93AnswerA -->


    <owl:NamedIndividual rdf:about="http://JP_ontology.org/assessment/MCQ93AnswerA">
        <rdf:type rdf:resource="http://JP_ontology.org/assessment/MCQ.93"/>
        <skos:altLabel xml:lang="en">(i)</skos:altLabel>
        <skos:definition xml:lang="en">Items of equipment containing storage media are not verified to ensure that sensitive data and licensed software have been removed or securely overwritten prior to disposal or re-use, potentially resulting in data breaches or unauthorized use of software.</skos:definition>
        <skos:prefLabel xml:lang="en">MCQ.93 - Not Implemented</skos:prefLabel>
    </owl:NamedIndividual>
    


    <!-- http://JP_ontology.org/assessment/MCQ93AnswerB -->


    <owl:NamedIndividual rdf:about="http://JP_ontology.org/assessment/MCQ93AnswerB">
        <rdf:type rdf:resource="http://JP_ontology.org/assessment/MCQ.93"/>
        <skos:altLabel xml:lang="en">(ii)</skos:altLabel>
        <skos:definition xml:lang="en">There are some efforts to verify items of equipment containing storage media, but the verification process may be inconsistent or not fully comprehensive in ensuring the removal of sensitive data and licensed software prior to disposal or re-use.</skos:definition>
        <skos:prefLabel xml:lang="en">MCQ.93 - Partially Implemented</skos:prefLabel>
    </owl:NamedIndividual>
    


    <!-- http://JP_ontology.org/assessment/MCQ93AnswerC -->


    <owl:NamedIndividual rdf:about="http://JP_ontology.org/assessment/MCQ93AnswerC">
        <rdf:type rdf:resource="http://JP_ontology.org/assessment/MCQ.93"/>
        <skos:altLabel xml:lang="en">(iii)</skos:altLabel>
        <skos:definition xml:lang="en">Items of equipment containing storage media are fully verified to ensure that any sensitive data and licensed software have been removed or securely overwritten prior to disposal or re-use, mitigating the risk of data breaches and unauthorized use of software.</skos:definition>
        <skos:prefLabel xml:lang="en">MCQ.93 - Fully Implemented</skos:prefLabel>
    </owl:NamedIndividual>
    


    <!-- http://JP_ontology.org/assessment/MCQ94AnswerA -->


    <owl:NamedIndividual rdf:about="http://JP_ontology.org/assessment/MCQ94AnswerA">
        <rdf:type rdf:resource="http://JP_ontology.org/assessment/MCQ.94"/>
        <skos:altLabel xml:lang="en">(i)</skos:altLabel>
        <skos:definition xml:lang="en">Information stored on, processed by, or accessible via user endpoint devices is not adequately protected, leaving it vulnerable to unauthorized access, theft, or manipulation.</skos:definition>
        <skos:prefLabel xml:lang="en">MCQ.94 - Not Implemented</skos:prefLabel>
    </owl:NamedIndividual>
    


    <!-- http://JP_ontology.org/assessment/MCQ94AnswerB -->


    <owl:NamedIndividual rdf:about="http://JP_ontology.org/assessment/MCQ94AnswerB">
        <rdf:type rdf:resource="http://JP_ontology.org/assessment/MCQ.94"/>
        <skos:altLabel xml:lang="en">(ii)</skos:altLabel>
        <skos:definition xml:lang="en">There are some measures in place to protect information stored on, processed by, or accessible via user endpoint devices, but the protection may be inconsistent or not fully comprehensive.</skos:definition>
        <skos:prefLabel xml:lang="en">MCQ.94 - Partially Implemented</skos:prefLabel>
    </owl:NamedIndividual>
    


    <!-- http://JP_ontology.org/assessment/MCQ94AnswerC -->


    <owl:NamedIndividual rdf:about="http://JP_ontology.org/assessment/MCQ94AnswerC">
        <rdf:type rdf:resource="http://JP_ontology.org/assessment/MCQ.94"/>
        <skos:altLabel xml:lang="en">(iii)</skos:altLabel>
        <skos:definition xml:lang="en">Information stored on, processed by, or accessible via user endpoint devices is fully protected, ensuring confidentiality, integrity, and availability through appropriate security measures and controls.</skos:definition>
        <skos:prefLabel xml:lang="en">MCQ.94 - Fully Implemented</skos:prefLabel>
    </owl:NamedIndividual>
    


    <!-- http://JP_ontology.org/assessment/MCQ95AnswerA -->


    <owl:NamedIndividual rdf:about="http://JP_ontology.org/assessment/MCQ95AnswerA">
        <rdf:type rdf:resource="http://JP_ontology.org/assessment/MCQ.95"/>
        <skos:altLabel xml:lang="en">(i)</skos:altLabel>
        <skos:definition xml:lang="en">Protection against malware is not implemented, and there are no appropriate user awareness measures in place, leaving the organisation vulnerable to malware attacks.</skos:definition>
        <skos:prefLabel xml:lang="en">MCQ.95 - Not Implemented</skos:prefLabel>
    </owl:NamedIndividual>
    


    <!-- http://JP_ontology.org/assessment/MCQ95AnswerB -->


    <owl:NamedIndividual rdf:about="http://JP_ontology.org/assessment/MCQ95AnswerB">
        <rdf:type rdf:resource="http://JP_ontology.org/assessment/MCQ.95"/>
        <skos:altLabel xml:lang="en">(ii)</skos:altLabel>
        <skos:definition xml:lang="en">There are some efforts to implement protection against malware, but user awareness measures may be lacking or insufficient to adequately support the protection against malware.</skos:definition>
        <skos:prefLabel xml:lang="en">MCQ.95 - Partially Implemented</skos:prefLabel>
    </owl:NamedIndividual>
    


    <!-- http://JP_ontology.org/assessment/MCQ95AnswerC -->


    <owl:NamedIndividual rdf:about="http://JP_ontology.org/assessment/MCQ95AnswerC">
        <rdf:type rdf:resource="http://JP_ontology.org/assessment/MCQ.95"/>
        <skos:altLabel xml:lang="en">(iii)</skos:altLabel>
        <skos:definition xml:lang="en">Protection against malware is fully implemented and supported by appropriate user awareness measures, ensuring proactive defense against malware threats and enhancing overall security posture.</skos:definition>
        <skos:prefLabel xml:lang="en">MCQ.95 - Fully Implemented</skos:prefLabel>
    </owl:NamedIndividual>
    


    <!-- http://JP_ontology.org/assessment/MCQ96AnswerA -->


    <owl:NamedIndividual rdf:about="http://JP_ontology.org/assessment/MCQ96AnswerA">
        <rdf:type rdf:resource="http://JP_ontology.org/assessment/MCQ.96"/>
        <skos:altLabel xml:lang="en">(i)</skos:altLabel>
        <skos:definition xml:lang="en">Information transfer rules, procedures, or agreements are not in place for all types of transfer facilities within the organisation and between the organisation and other parties, potentially leading to unsecure or unauthorized transfer of sensitive information.</skos:definition>
        <skos:prefLabel xml:lang="en">MCQ.96 - Not Implemented</skos:prefLabel>
    </owl:NamedIndividual>
    


    <!-- http://JP_ontology.org/assessment/MCQ96AnswerB -->


    <owl:NamedIndividual rdf:about="http://JP_ontology.org/assessment/MCQ96AnswerB">
        <rdf:type rdf:resource="http://JP_ontology.org/assessment/MCQ.96"/>
        <skos:altLabel xml:lang="en">(ii)</skos:altLabel>
        <skos:definition xml:lang="en">There are some efforts to establish information transfer rules, procedures, or agreements, but they may not cover all types of transfer facilities within the organisation and between the organisation and other parties, or the implementation may be inconsistent.</skos:definition>
        <skos:prefLabel xml:lang="en">MCQ.96 - Partially Implemented</skos:prefLabel>
    </owl:NamedIndividual>
    


    <!-- http://JP_ontology.org/assessment/MCQ96AnswerC -->


    <owl:NamedIndividual rdf:about="http://JP_ontology.org/assessment/MCQ96AnswerC">
        <rdf:type rdf:resource="http://JP_ontology.org/assessment/MCQ.96"/>
        <skos:altLabel xml:lang="en">(iii)</skos:altLabel>
        <skos:definition xml:lang="en">Information transfer rules, procedures, or agreements are fully established for all types of transfer facilities within the organisation and between the organisation and other parties, ensuring secure and compliant transfer of information.</skos:definition>
        <skos:prefLabel xml:lang="en">MCQ.96 - Fully Implemented</skos:prefLabel>
    </owl:NamedIndividual>
    


    <!-- http://JP_ontology.org/assessment/MCQ97AnswerA -->


    <owl:NamedIndividual rdf:about="http://JP_ontology.org/assessment/MCQ97AnswerA">
        <rdf:type rdf:resource="http://JP_ontology.org/assessment/MCQ.97"/>
        <skos:altLabel xml:lang="en">(i)</skos:altLabel>
        <skos:definition xml:lang="en">The organisation lacks a structured approach to managing the complete life cycle of identities, leading to inconsistencies and gaps in identity-related processes such as creation, authentication, and termination.</skos:definition>
        <skos:prefLabel xml:lang="en">MCQ.97 - Not Implemented</skos:prefLabel>
    </owl:NamedIndividual>
    


    <!-- http://JP_ontology.org/assessment/MCQ97AnswerB -->


    <owl:NamedIndividual rdf:about="http://JP_ontology.org/assessment/MCQ97AnswerB">
        <rdf:type rdf:resource="http://JP_ontology.org/assessment/MCQ.97"/>
        <skos:altLabel xml:lang="en">(ii)</skos:altLabel>
        <skos:definition xml:lang="en">There are some efforts to manage the complete life cycle of identities, including activities such as creation, authentication, and periodic reviews, but the process may be inconsistent or lacking in certain areas.</skos:definition>
        <skos:prefLabel xml:lang="en">MCQ.97 - Partially Implemented</skos:prefLabel>
    </owl:NamedIndividual>
    


    <!-- http://JP_ontology.org/assessment/MCQ97AnswerC -->


    <owl:NamedIndividual rdf:about="http://JP_ontology.org/assessment/MCQ97AnswerC">
        <rdf:type rdf:resource="http://JP_ontology.org/assessment/MCQ.97"/>
        <skos:altLabel xml:lang="en">(iii)</skos:altLabel>
        <skos:definition xml:lang="en">The organisation has implemented a comprehensive approach to managing the complete life cycle of identities, covering all activities from creation to termination, and ensuring robust oversight and control over identity-related processes.</skos:definition>
        <skos:prefLabel xml:lang="en">MCQ.97 - Fully Implemented</skos:prefLabel>
    </owl:NamedIndividual>
    


    <!-- http://JP_ontology.org/assessment/MCQ98AnswerA -->


    <owl:NamedIndividual rdf:about="http://JP_ontology.org/assessment/MCQ98AnswerA">
        <rdf:type rdf:resource="http://JP_ontology.org/assessment/MCQ.98"/>
        <skos:altLabel xml:lang="en">(i)</skos:altLabel>
        <skos:definition xml:lang="en">There is no management process in place to control the allocation and management of authentication information, and personnel are not advised on the appropriate handling of authentication information.</skos:definition>
        <skos:prefLabel xml:lang="en">MCQ.98 - Not Implemented</skos:prefLabel>
    </owl:NamedIndividual>
    


    <!-- http://JP_ontology.org/assessment/MCQ98AnswerB -->


    <owl:NamedIndividual rdf:about="http://JP_ontology.org/assessment/MCQ98AnswerB">
        <rdf:type rdf:resource="http://JP_ontology.org/assessment/MCQ.98"/>
        <skos:altLabel xml:lang="en">(ii)</skos:altLabel>
        <skos:definition xml:lang="en">There are some efforts to control the allocation and management of authentication information through a management process, but personnel may not consistently receive advice on the appropriate handling of authentication information.</skos:definition>
        <skos:prefLabel xml:lang="en">MCQ.98 - Partially Implemented</skos:prefLabel>
    </owl:NamedIndividual>
    


    <!-- http://JP_ontology.org/assessment/MCQ98AnswerC -->


    <owl:NamedIndividual rdf:about="http://JP_ontology.org/assessment/MCQ98AnswerC">
        <rdf:type rdf:resource="http://JP_ontology.org/assessment/MCQ.98"/>
        <skos:altLabel xml:lang="en">(iii)</skos:altLabel>
        <skos:definition xml:lang="en">The allocation and management of authentication information are controlled by a robust management process, which includes advising personnel on the appropriate handling of authentication information, ensuring secure and effective management of authentication credentials.</skos:definition>
        <skos:prefLabel xml:lang="en">MCQ.98 - Fully Implemented</skos:prefLabel>
    </owl:NamedIndividual>
    


    <!-- http://JP_ontology.org/assessment/MCQ99AnswerA -->


    <owl:NamedIndividual rdf:about="http://JP_ontology.org/assessment/MCQ99AnswerA">
        <rdf:type rdf:resource="http://JP_ontology.org/assessment/MCQ.99"/>
        <skos:altLabel xml:lang="en">(i)</skos:altLabel>
        <skos:definition xml:lang="en">Secure authentication technologies and procedures are not implemented based on information access restrictions and the topic-specific policy on access control, resulting in potential vulnerabilities and unauthorized access.</skos:definition>
        <skos:prefLabel xml:lang="en">MCQ.99 - Not Implemented</skos:prefLabel>
    </owl:NamedIndividual>
    


    <!-- http://JP_ontology.org/assessment/MCQ99AnswerB -->


    <owl:NamedIndividual rdf:about="http://JP_ontology.org/assessment/MCQ99AnswerB">
        <rdf:type rdf:resource="http://JP_ontology.org/assessment/MCQ.99"/>
        <skos:altLabel xml:lang="en">(ii)</skos:altLabel>
        <skos:definition xml:lang="en">There are some efforts to implement secure authentication technologies and procedures based on information access restrictions and the topic-specific policy on access control, but the implementation may be incomplete or inconsistent.</skos:definition>
        <skos:prefLabel xml:lang="en">MCQ.99 - Partially Implemented</skos:prefLabel>
    </owl:NamedIndividual>
    


    <!-- http://JP_ontology.org/assessment/MCQ99AnswerC -->


    <owl:NamedIndividual rdf:about="http://JP_ontology.org/assessment/MCQ99AnswerC">
        <rdf:type rdf:resource="http://JP_ontology.org/assessment/MCQ.99"/>
        <skos:altLabel xml:lang="en">(iii)</skos:altLabel>
        <skos:definition xml:lang="en">Secure authentication technologies and procedures are fully implemented based on information access restrictions and the topic-specific policy on access control, ensuring robust access security and compliance with organisational policies.</skos:definition>
        <skos:prefLabel xml:lang="en">MCQ.99 - Fully Implemented</skos:prefLabel>
    </owl:NamedIndividual>
    


    <!-- 
    ///////////////////////////////////////////////////////////////////////////////////////
    //
    // Annotations
    //
    ///////////////////////////////////////////////////////////////////////////////////////
     -->


    <rdf:Description rdf:about="http://JP_ontology.org/assessment/MCQ.1">
        <nis2v:hasAnswer rdf:resource="http://JP_ontology.org/assessment/MCQ.1AnswerA"/>
        <nis2v:hasAnswer rdf:resource="http://JP_ontology.org/assessment/MCQ.1AnswerB"/>
        <nis2v:hasAnswer rdf:resource="http://JP_ontology.org/assessment/MCQ.1AnswerC"/>
        <nis2v:relatedToControl rdf:resource="http://JP_ontology.org/iso27001/Control4"/>
        <terms:contributor>Jenni Parry</terms:contributor>
        <terms:created rdf:datatype="http://www.w3.org/2001/XMLSchema#date">2024-05-20</terms:created>
        <terms:subject rdf:resource="http://JP_ontology.org/nis2v/Article_21.2a"/>
        <rdfs:isDefinedBy rdf:resource="http://JP_ontology.org/assessment"/>
        <skos:altLabel xml:lang="en">MCQ.1</skos:altLabel>
        <skos:broader rdf:resource="http://JP_ontology.org/assessment/AssessmentQuestion"/>
        <skos:definition xml:lang="en">Does the organisation determine external and internal issues relevant to its purpose and affecting its ability to achieve the intended outcome(s) of its information security management system?</skos:definition>
        <skos:prefLabel xml:lang="en">Multiple Choice Question #1</skos:prefLabel>
    </rdf:Description>
    <rdf:Description rdf:about="http://JP_ontology.org/assessment/MCQ.10.1">
        <nis2v:hasAnswer rdf:resource="http://JP_ontology.org/assessment/MCQ.10.1AnswerA"/>
        <nis2v:hasAnswer rdf:resource="http://JP_ontology.org/assessment/MCQ.10.1AnswerB"/>
        <nis2v:hasAnswer rdf:resource="http://JP_ontology.org/assessment/MCQ.10.1AnswerC"/>
        <nis2v:relatedToControl rdf:resource="http://JP_ontology.org/iso27001/ControlA.5.1"/>
        <terms:contributor>Jenni Parry</terms:contributor>
        <terms:created rdf:datatype="http://www.w3.org/2001/XMLSchema#date">2024-05-20</terms:created>
        <terms:subject rdf:resource="http://JP_ontology.org/nis2v/Article_21.2a"/>
        <rdfs:isDefinedBy rdf:resource="http://JP_ontology.org/assessment"/>
        <skos:altLabel xml:lang="en">MCQ.10.1</skos:altLabel>
        <skos:broader rdf:resource="http://JP_ontology.org/assessment/AssessmentQuestion"/>
        <skos:definition xml:lang="en">Is the information security policy and topic-specific policies defined, approved by management, published, communicated to and acknowledged by relevant personnel and relevant interested parties? </skos:definition>
        <skos:prefLabel xml:lang="en">Multiple Choice Question #10.1</skos:prefLabel>
    </rdf:Description>
    <rdf:Description rdf:about="http://JP_ontology.org/assessment/MCQ.10.2">
        <nis2v:hasAnswer rdf:resource="http://JP_ontology.org/assessment/MCQ.10.2AnswerA"/>
        <nis2v:hasAnswer rdf:resource="http://JP_ontology.org/assessment/MCQ.10.2AnswerB"/>
        <nis2v:hasAnswer rdf:resource="http://JP_ontology.org/assessment/MCQ.10.2AnswerC"/>
        <nis2v:relatedToControl rdf:resource="http://JP_ontology.org/iso27001/ControlA.5.1"/>
        <terms:contributor>Jenni Parry</terms:contributor>
        <terms:created rdf:datatype="http://www.w3.org/2001/XMLSchema#date">2024-05-20</terms:created>
        <terms:subject rdf:resource="http://JP_ontology.org/nis2v/Article_21.2a"/>
        <rdfs:isDefinedBy rdf:resource="http://JP_ontology.org/assessment"/>
        <skos:altLabel xml:lang="en">MCQ.10.2</skos:altLabel>
        <skos:broader rdf:resource="http://JP_ontology.org/assessment/AssessmentQuestion"/>
        <skos:definition xml:lang="en">Is the policy reviewed at planned intervals and if significant changes occur?</skos:definition>
        <skos:prefLabel xml:lang="en">Multiple Choice Question #10.2</skos:prefLabel>
    </rdf:Description>
    <rdf:Description rdf:about="http://JP_ontology.org/assessment/MCQ.100">
        <nis2v:hasAnswer rdf:resource="http://JP_ontology.org/assessment/MCQ.100AnswerA"/>
        <nis2v:hasAnswer rdf:resource="http://JP_ontology.org/assessment/MCQ.100AnswerB"/>
        <nis2v:hasAnswer rdf:resource="http://JP_ontology.org/assessment/MCQ.100AnswerC"/>
        <nis2v:relatedToControl rdf:resource="http://JP_ontology.org/iso27001/ControlA.8.12"/>
        <terms:contributor>Jenni Parry</terms:contributor>
        <terms:created rdf:datatype="http://www.w3.org/2001/XMLSchema#date">2024-05-20</terms:created>
        <terms:subject rdf:resource="http://JP_ontology.org/nis2v/Article_21.2j"/>
        <rdfs:isDefinedBy rdf:resource="http://JP_ontology.org/assessment"/>
        <skos:altLabel xml:lang="en">MCQ.100</skos:altLabel>
        <skos:broader rdf:resource="http://JP_ontology.org/assessment/AssessmentQuestion"/>
        <skos:definition xml:lang="en">Are data leakage prevention measures applied to systems, networks, and any other devices that process, store, or transmit sensitive information?</skos:definition>
        <skos:prefLabel xml:lang="en">Multiple Choice Question #100</skos:prefLabel>
    </rdf:Description>
    <rdf:Description rdf:about="http://JP_ontology.org/assessment/MCQ.101">
        <nis2v:hasAnswer rdf:resource="http://JP_ontology.org/assessment/MCQ.101AnswerA"/>
        <nis2v:hasAnswer rdf:resource="http://JP_ontology.org/assessment/MCQ.101AnswerB"/>
        <nis2v:hasAnswer rdf:resource="http://JP_ontology.org/assessment/MCQ.101AnswerC"/>
        <nis2v:relatedToControl rdf:resource="http://JP_ontology.org/iso27001/Control4.1"/>
        <terms:contributor>Jenni Parry</terms:contributor>
        <terms:created rdf:datatype="http://www.w3.org/2001/XMLSchema#date">2024-05-20</terms:created>
        <terms:subject rdf:resource="http://JP_ontology.org/nis2v/Article_21.2a"/>
        <rdfs:isDefinedBy rdf:resource="http://JP_ontology.org/assessment"/>
        <skos:altLabel xml:lang="en">MCQ.101</skos:altLabel>
        <skos:broader rdf:resource="http://JP_ontology.org/assessment/AssessmentQuestion"/>
        <skos:definition xml:lang="en">How does the organisation address external and internal issues that may impact its ability to achieve the intended outcome(s) of its information security management system?</skos:definition>
        <skos:prefLabel xml:lang="en">Multiple Choice Question #101</skos:prefLabel>
    </rdf:Description>
    <rdf:Description rdf:about="http://JP_ontology.org/assessment/MCQ.102">
        <nis2v:hasAnswer rdf:resource="http://JP_ontology.org/assessment/MCQ.102AnswerA"/>
        <nis2v:hasAnswer rdf:resource="http://JP_ontology.org/assessment/MCQ.102AnswerB"/>
        <nis2v:hasAnswer rdf:resource="http://JP_ontology.org/assessment/MCQ.102AnswerC"/>
        <nis2v:relatedToControl rdf:resource="http://JP_ontology.org/iso27001/Control4.2"/>
        <terms:contributor>Jenni Parry</terms:contributor>
        <terms:created rdf:datatype="http://www.w3.org/2001/XMLSchema#date">2024-05-20</terms:created>
        <terms:subject rdf:resource="http://JP_ontology.org/nis2v/Article_21.2a"/>
        <rdfs:isDefinedBy rdf:resource="http://JP_ontology.org/assessment"/>
        <skos:altLabel xml:lang="en">MCQ.102</skos:altLabel>
        <skos:broader rdf:resource="http://JP_ontology.org/assessment/AssessmentQuestion"/>
        <skos:definition xml:lang="en">How does the organisation determine the interested parties relevant to its information security management system and address their requirements?</skos:definition>
        <skos:prefLabel xml:lang="en">Multiple Choice Question #102</skos:prefLabel>
    </rdf:Description>
    <rdf:Description rdf:about="http://JP_ontology.org/assessment/MCQ.103">
        <nis2v:hasAnswer rdf:resource="http://JP_ontology.org/assessment/MCQ.103AnswerA"/>
        <nis2v:hasAnswer rdf:resource="http://JP_ontology.org/assessment/MCQ.103AnswerB"/>
        <nis2v:hasAnswer rdf:resource="http://JP_ontology.org/assessment/MCQ.103AnswerC"/>
        <nis2v:relatedToControl rdf:resource="http://JP_ontology.org/iso27001/Control4.3"/>
        <terms:contributor>Jenni Parry</terms:contributor>
        <terms:created rdf:datatype="http://www.w3.org/2001/XMLSchema#date">2024-05-20</terms:created>
        <terms:subject rdf:resource="http://JP_ontology.org/nis2v/Article_21.2a"/>
        <rdfs:isDefinedBy rdf:resource="http://JP_ontology.org/assessment"/>
        <skos:altLabel xml:lang="en">MCQ.103</skos:altLabel>
        <skos:broader rdf:resource="http://JP_ontology.org/assessment/AssessmentQuestion"/>
        <skos:definition xml:lang="en">How does the organisation establish the scope of its information security management system (ISMS) while considering various factors?</skos:definition>
        <skos:prefLabel xml:lang="en">Multiple Choice Question #103</skos:prefLabel>
    </rdf:Description>
    <rdf:Description rdf:about="http://JP_ontology.org/assessment/MCQ.104">
        <nis2v:hasAnswer rdf:resource="http://JP_ontology.org/assessment/MCQ.104AnswerA"/>
        <nis2v:hasAnswer rdf:resource="http://JP_ontology.org/assessment/MCQ.104AnswerB"/>
        <nis2v:hasAnswer rdf:resource="http://JP_ontology.org/assessment/MCQ.104AnswerC"/>
        <nis2v:relatedToControl rdf:resource="http://JP_ontology.org/iso27001/Control4.4"/>
        <terms:contributor>Jenni Parry</terms:contributor>
        <terms:created rdf:datatype="http://www.w3.org/2001/XMLSchema#date">2024-05-20</terms:created>
        <terms:subject rdf:resource="http://JP_ontology.org/nis2v/Article_21.2a"/>
        <rdfs:isDefinedBy rdf:resource="http://JP_ontology.org/assessment"/>
        <skos:altLabel xml:lang="en">MCQ.104</skos:altLabel>
        <skos:broader rdf:resource="http://JP_ontology.org/assessment/AssessmentQuestion"/>
        <skos:definition xml:lang="en">How does the organisation ensure the establishment, implementation, maintenance, and continual improvement of its information security management system (ISMS) in alignment with the ISO27001 requirements?</skos:definition>
        <skos:prefLabel xml:lang="en">Multiple Choice Question #104</skos:prefLabel>
    </rdf:Description>
    <rdf:Description rdf:about="http://JP_ontology.org/assessment/MCQ.105.1">
        <nis2v:hasAnswer rdf:resource="http://JP_ontology.org/assessment/MCQ.105.1AnswerA"/>
        <nis2v:hasAnswer rdf:resource="http://JP_ontology.org/assessment/MCQ.105.1AnswerB"/>
        <nis2v:hasAnswer rdf:resource="http://JP_ontology.org/assessment/MCQ.105.1AnswerC"/>
        <nis2v:relatedToControl rdf:resource="http://JP_ontology.org/iso27001/Control5.1"/>
        <terms:contributor>Jenni Parry</terms:contributor>
        <terms:created rdf:datatype="http://www.w3.org/2001/XMLSchema#date">2024-05-20</terms:created>
        <terms:subject rdf:resource="http://JP_ontology.org/nis2v/Article_21.2a"/>
        <rdfs:isDefinedBy rdf:resource="http://JP_ontology.org/assessment"/>
        <skos:altLabel xml:lang="en">MCQ.105.1</skos:altLabel>
        <skos:broader rdf:resource="http://JP_ontology.org/assessment/AssessmentQuestion"/>
        <skos:definition xml:lang="en">How does senior management ensure the information security policy and objectives align with the strategic direction of the organisation?</skos:definition>
        <skos:prefLabel xml:lang="en">Multiple Choice Question #105.1</skos:prefLabel>
    </rdf:Description>
    <rdf:Description rdf:about="http://JP_ontology.org/assessment/MCQ.105.2">
        <nis2v:hasAnswer rdf:resource="http://JP_ontology.org/assessment/MCQ.105.2AnswerA"/>
        <nis2v:hasAnswer rdf:resource="http://JP_ontology.org/assessment/MCQ.105.2AnswerB"/>
        <nis2v:hasAnswer rdf:resource="http://JP_ontology.org/assessment/MCQ.105.2AnswerC"/>
        <nis2v:relatedToControl rdf:resource="http://JP_ontology.org/iso27001/Control5.1"/>
        <terms:contributor>Jenni Parry</terms:contributor>
        <terms:created rdf:datatype="http://www.w3.org/2001/XMLSchema#date">2024-05-20</terms:created>
        <terms:subject rdf:resource="http://JP_ontology.org/nis2v/Article_21.2a"/>
        <rdfs:isDefinedBy rdf:resource="http://JP_ontology.org/assessment"/>
        <skos:altLabel xml:lang="en">MCQ.105.2</skos:altLabel>
        <skos:broader rdf:resource="http://JP_ontology.org/assessment/AssessmentQuestion"/>
        <skos:definition xml:lang="en">How does senior management ensure the integration of information security management system requirements into the organisation’s processes?</skos:definition>
        <skos:prefLabel xml:lang="en">Multiple Choice Question #105.2</skos:prefLabel>
    </rdf:Description>
    <rdf:Description rdf:about="http://JP_ontology.org/assessment/MCQ.105.3">
        <nis2v:hasAnswer rdf:resource="http://JP_ontology.org/assessment/MCQ.105.3AnswerA"/>
        <nis2v:hasAnswer rdf:resource="http://JP_ontology.org/assessment/MCQ.105.3AnswerB"/>
        <nis2v:hasAnswer rdf:resource="http://JP_ontology.org/assessment/MCQ.105.3AnswerC"/>
        <nis2v:relatedToControl rdf:resource="http://JP_ontology.org/iso27001/Control5.1"/>
        <terms:contributor>Jenni Parry</terms:contributor>
        <terms:created rdf:datatype="http://www.w3.org/2001/XMLSchema#date">2024-05-20</terms:created>
        <terms:subject rdf:resource="http://JP_ontology.org/nis2v/Article_21.2a"/>
        <rdfs:isDefinedBy rdf:resource="http://JP_ontology.org/assessment"/>
        <skos:altLabel xml:lang="en">MCQ.105.3</skos:altLabel>
        <skos:broader rdf:resource="http://JP_ontology.org/assessment/AssessmentQuestion"/>
        <skos:definition xml:lang="en">How does senior management ensure that the necessary resources for the information security management system are available?</skos:definition>
        <skos:prefLabel xml:lang="en">Multiple Choice Question #105.3</skos:prefLabel>
    </rdf:Description>
    <rdf:Description rdf:about="http://JP_ontology.org/assessment/MCQ.106.1">
        <nis2v:hasAnswer rdf:resource="http://JP_ontology.org/assessment/MCQ.106.1AnswerA"/>
        <nis2v:hasAnswer rdf:resource="http://JP_ontology.org/assessment/MCQ.106.1AnswerB"/>
        <nis2v:hasAnswer rdf:resource="http://JP_ontology.org/assessment/MCQ.106.1AnswerC"/>
        <nis2v:relatedToControl rdf:resource="http://JP_ontology.org/iso27001/Control6.1."/>
        <terms:contributor>Jenni Parry</terms:contributor>
        <terms:created rdf:datatype="http://www.w3.org/2001/XMLSchema#date">2024-05-20</terms:created>
        <terms:subject rdf:resource="http://JP_ontology.org/nis2v/Article_21.2a"/>
        <rdfs:isDefinedBy rdf:resource="http://JP_ontology.org/assessment"/>
        <skos:altLabel xml:lang="en">MCQ.106.1</skos:altLabel>
        <skos:broader rdf:resource="http://JP_ontology.org/assessment/AssessmentQuestion"/>
        <skos:definition xml:lang="en">When planning for the information security management system, what factors should the organisation consider?</skos:definition>
        <skos:prefLabel xml:lang="en">Multiple Choice Question #106.1</skos:prefLabel>
    </rdf:Description>
    <rdf:Description rdf:about="http://JP_ontology.org/assessment/MCQ.106.2">
        <nis2v:hasAnswer rdf:resource="http://JP_ontology.org/assessment/MCQ.106.2AnswerA"/>
        <nis2v:hasAnswer rdf:resource="http://JP_ontology.org/assessment/MCQ.106.2AnswerB"/>
        <nis2v:hasAnswer rdf:resource="http://JP_ontology.org/assessment/MCQ.106.2AnswerC"/>
        <nis2v:relatedToControl rdf:resource="http://JP_ontology.org/iso27001/Control6.1."/>
        <terms:contributor>Jenni Parry</terms:contributor>
        <terms:created rdf:datatype="http://www.w3.org/2001/XMLSchema#date">2024-05-20</terms:created>
        <terms:subject rdf:resource="http://JP_ontology.org/nis2v/Article_21.2a"/>
        <rdfs:isDefinedBy rdf:resource="http://JP_ontology.org/assessment"/>
        <skos:altLabel xml:lang="en">MCQ.106.2</skos:altLabel>
        <skos:broader rdf:resource="http://JP_ontology.org/assessment/AssessmentQuestion"/>
        <skos:definition xml:lang="en">What actions does the organisation plan regarding the identified risks and opportunities for the information security management system?</skos:definition>
        <skos:prefLabel xml:lang="en">Multiple Choice Question #106.2</skos:prefLabel>
    </rdf:Description>
    <rdf:Description rdf:about="http://JP_ontology.org/assessment/MCQ.107.1">
        <nis2v:hasAnswer rdf:resource="http://JP_ontology.org/assessment/MCQ.107.1AnswerA"/>
        <nis2v:hasAnswer rdf:resource="http://JP_ontology.org/assessment/MCQ.107.1AnswerB"/>
        <nis2v:hasAnswer rdf:resource="http://JP_ontology.org/assessment/MCQ.107.1AnswerC"/>
        <nis2v:relatedToControl rdf:resource="http://JP_ontology.org/iso27001/Control6.2"/>
        <terms:contributor>Jenni Parry</terms:contributor>
        <terms:created rdf:datatype="http://www.w3.org/2001/XMLSchema#date">2024-05-20</terms:created>
        <terms:subject rdf:resource="http://JP_ontology.org/nis2v/Article_21.2a"/>
        <rdfs:isDefinedBy rdf:resource="http://JP_ontology.org/assessment"/>
        <skos:altLabel xml:lang="en">MCQ.107.1</skos:altLabel>
        <skos:broader rdf:resource="http://JP_ontology.org/assessment/AssessmentQuestion"/>
        <skos:definition xml:lang="en">How does the organisation ensure the establishment of information security objectives across relevant functions and levels?</skos:definition>
        <skos:prefLabel xml:lang="en">Multiple Choice Question #107.1</skos:prefLabel>
    </rdf:Description>
    <rdf:Description rdf:about="http://JP_ontology.org/assessment/MCQ.107.2">
        <nis2v:hasAnswer rdf:resource="http://JP_ontology.org/assessment/MCQ.107.2AnswerA"/>
        <nis2v:hasAnswer rdf:resource="http://JP_ontology.org/assessment/MCQ.107.2AnswerB"/>
        <nis2v:hasAnswer rdf:resource="http://JP_ontology.org/assessment/MCQ.107.2AnswerC"/>
        <nis2v:relatedToControl rdf:resource="http://JP_ontology.org/iso27001/Control6.2"/>
        <terms:contributor>Jenni Parry</terms:contributor>
        <terms:created rdf:datatype="http://www.w3.org/2001/XMLSchema#date">2024-05-20</terms:created>
        <terms:subject rdf:resource="http://JP_ontology.org/nis2v/Article_21.2a"/>
        <rdfs:isDefinedBy rdf:resource="http://JP_ontology.org/assessment"/>
        <skos:altLabel xml:lang="en">MCQ.107.2</skos:altLabel>
        <skos:broader rdf:resource="http://JP_ontology.org/assessment/AssessmentQuestion"/>
        <skos:definition xml:lang="en">How does the organisation plan to achieve its information security objectives?</skos:definition>
        <skos:prefLabel xml:lang="en">Multiple Choice Question #107.2</skos:prefLabel>
    </rdf:Description>
    <rdf:Description rdf:about="http://JP_ontology.org/assessment/MCQ.108">
        <nis2v:hasAnswer rdf:resource="http://JP_ontology.org/assessment/MCQ.108AnswerA"/>
        <nis2v:hasAnswer rdf:resource="http://JP_ontology.org/assessment/MCQ.108AnswerB"/>
        <nis2v:hasAnswer rdf:resource="http://JP_ontology.org/assessment/MCQ.108AnswerC"/>
        <nis2v:relatedToControl rdf:resource="http://JP_ontology.org/iso27001/Control7.1"/>
        <terms:contributor>Jenni Parry</terms:contributor>
        <terms:created rdf:datatype="http://www.w3.org/2001/XMLSchema#date">2024-05-20</terms:created>
        <terms:subject rdf:resource="http://JP_ontology.org/nis2v/Article_21.2a"/>
        <rdfs:isDefinedBy rdf:resource="http://JP_ontology.org/assessment"/>
        <skos:altLabel xml:lang="en">MCQ.108</skos:altLabel>
        <skos:broader rdf:resource="http://JP_ontology.org/assessment/AssessmentQuestion"/>
        <skos:definition xml:lang="en">How does the organisation ensure the availability of resources necessary for the establishment, implementation, maintenance, and continual improvement of the information security management system (ISMS)?</skos:definition>
        <skos:prefLabel xml:lang="en">Multiple Choice Question #108</skos:prefLabel>
    </rdf:Description>
    <rdf:Description rdf:about="http://JP_ontology.org/assessment/MCQ.109">
        <nis2v:hasAnswer rdf:resource="http://JP_ontology.org/assessment/MCQ.109AnswerA"/>
        <nis2v:hasAnswer rdf:resource="http://JP_ontology.org/assessment/MCQ.109AnswerB"/>
        <nis2v:hasAnswer rdf:resource="http://JP_ontology.org/assessment/MCQ.109AnswerC"/>
        <nis2v:relatedToControl rdf:resource="http://JP_ontology.org/iso27001/Control7.5.3"/>
        <terms:contributor>Jenni Parry</terms:contributor>
        <terms:created rdf:datatype="http://www.w3.org/2001/XMLSchema#date">2024-05-20</terms:created>
        <terms:subject rdf:resource="http://JP_ontology.org/nis2v/Article_21.2a"/>
        <rdfs:isDefinedBy rdf:resource="http://JP_ontology.org/assessment"/>
        <skos:altLabel xml:lang="en">MCQ.109</skos:altLabel>
        <skos:broader rdf:resource="http://JP_ontology.org/assessment/AssessmentQuestion"/>
        <skos:definition xml:lang="en">How does the organisation ensure the control of documented information required by the information security management system and by relevant documents?</skos:definition>
        <skos:prefLabel xml:lang="en">Multiple Choice Question #109</skos:prefLabel>
    </rdf:Description>
    <rdf:Description rdf:about="http://JP_ontology.org/assessment/MCQ.11">
        <nis2v:hasAnswer rdf:resource="http://JP_ontology.org/assessment/MCQ.11AnswerA"/>
        <nis2v:hasAnswer rdf:resource="http://JP_ontology.org/assessment/MCQ.11AnswerB"/>
        <nis2v:hasAnswer rdf:resource="http://JP_ontology.org/assessment/MCQ.11AnswerC"/>
        <nis2v:relatedToControl rdf:resource="http://JP_ontology.org/iso27001/ControlA.5.2"/>
        <terms:contributor>Jenni Parry</terms:contributor>
        <terms:created rdf:datatype="http://www.w3.org/2001/XMLSchema#date">2024-05-20</terms:created>
        <terms:subject rdf:resource="http://JP_ontology.org/nis2v/Article_21.2a"/>
        <rdfs:isDefinedBy rdf:resource="http://JP_ontology.org/assessment"/>
        <skos:altLabel xml:lang="en">MCQ.11</skos:altLabel>
        <skos:broader rdf:resource="http://JP_ontology.org/assessment/AssessmentQuestion"/>
        <skos:definition xml:lang="en">Are information security roles and responsibilities defined and allocated according to the organisation&apos;s needs?</skos:definition>
        <skos:prefLabel xml:lang="en">Multiple Choice Question #11</skos:prefLabel>
    </rdf:Description>
    <rdf:Description rdf:about="http://JP_ontology.org/assessment/MCQ.110">
        <nis2v:hasAnswer rdf:resource="http://JP_ontology.org/assessment/MCQ.110AnswerA"/>
        <nis2v:hasAnswer rdf:resource="http://JP_ontology.org/assessment/MCQ.110AnswerB"/>
        <nis2v:hasAnswer rdf:resource="http://JP_ontology.org/assessment/MCQ.110AnswerC"/>
        <nis2v:relatedToControl rdf:resource="http://JP_ontology.org/iso27001/Control8.1"/>
        <terms:contributor>Jenni Parry</terms:contributor>
        <terms:created rdf:datatype="http://www.w3.org/2001/XMLSchema#date">2024-05-20</terms:created>
        <terms:subject rdf:resource="http://JP_ontology.org/nis2v/Article_21.2a"/>
        <rdfs:isDefinedBy rdf:resource="http://JP_ontology.org/assessment"/>
        <skos:altLabel xml:lang="en">MCQ.110</skos:altLabel>
        <skos:broader rdf:resource="http://JP_ontology.org/assessment/AssessmentQuestion"/>
        <skos:definition xml:lang="en">How does the organisation ensure the planning, implementation, and control of processes needed to meet requirements?</skos:definition>
        <skos:prefLabel xml:lang="en">Multiple Choice Question #110</skos:prefLabel>
    </rdf:Description>
    <rdf:Description rdf:about="http://JP_ontology.org/assessment/MCQ.111">
        <nis2v:hasAnswer rdf:resource="http://JP_ontology.org/assessment/MCQ.111AnswerA"/>
        <nis2v:hasAnswer rdf:resource="http://JP_ontology.org/assessment/MCQ.111AnswerB"/>
        <nis2v:hasAnswer rdf:resource="http://JP_ontology.org/assessment/MCQ.111AnswerC"/>
        <nis2v:relatedToControl rdf:resource="http://JP_ontology.org/iso27001/ControlA.8.31"/>
        <terms:contributor>Jenni Parry</terms:contributor>
        <terms:created rdf:datatype="http://www.w3.org/2001/XMLSchema#date">2024-05-20</terms:created>
        <terms:subject rdf:resource="http://JP_ontology.org/nis2v/Article_21.2e"/>
        <rdfs:isDefinedBy rdf:resource="http://JP_ontology.org/assessment"/>
        <skos:altLabel xml:lang="en">MCQ.111</skos:altLabel>
        <skos:broader rdf:resource="http://JP_ontology.org/assessment/AssessmentQuestion"/>
        <skos:definition xml:lang="en">How does the organisation ensure the separation and security of development, testing, and production environments?</skos:definition>
        <skos:prefLabel xml:lang="en">Multiple Choice Question #111</skos:prefLabel>
    </rdf:Description>
    <rdf:Description rdf:about="http://JP_ontology.org/assessment/MCQ.112.1">
        <nis2v:hasAnswer rdf:resource="http://JP_ontology.org/assessment/MCQ.112.1AnswerA"/>
        <nis2v:hasAnswer rdf:resource="http://JP_ontology.org/assessment/MCQ.112.1AnswerB"/>
        <nis2v:hasAnswer rdf:resource="http://JP_ontology.org/assessment/MCQ.112.1AnswerC"/>
        <nis2v:relatedToControl rdf:resource="http://JP_ontology.org/iso27001/Control9.1"/>
        <terms:contributor>Jenni Parry</terms:contributor>
        <terms:created rdf:datatype="http://www.w3.org/2001/XMLSchema#date">2024-05-20</terms:created>
        <terms:subject rdf:resource="http://JP_ontology.org/nis2v/Article_21.2f"/>
        <rdfs:isDefinedBy rdf:resource="http://JP_ontology.org/assessment"/>
        <skos:altLabel xml:lang="en">MCQ.112.1</skos:altLabel>
        <skos:broader rdf:resource="http://JP_ontology.org/assessment/AssessmentQuestion"/>
        <skos:definition xml:lang="en">How does the organisation ensure effective monitoring and measurement of information security processes and controls?</skos:definition>
        <skos:prefLabel xml:lang="en">Multiple Choice Question #112.1</skos:prefLabel>
    </rdf:Description>
    <rdf:Description rdf:about="http://JP_ontology.org/assessment/MCQ.112.2">
        <nis2v:hasAnswer rdf:resource="http://JP_ontology.org/assessment/MCQ.112.2AnswerA"/>
        <nis2v:hasAnswer rdf:resource="http://JP_ontology.org/assessment/MCQ.112.2AnswerB"/>
        <nis2v:hasAnswer rdf:resource="http://JP_ontology.org/assessment/MCQ.112.2AnswerC"/>
        <nis2v:relatedToControl rdf:resource="http://JP_ontology.org/iso27001/Control9.1"/>
        <terms:contributor>Jenni Parry</terms:contributor>
        <terms:created rdf:datatype="http://www.w3.org/2001/XMLSchema#date">2024-05-20</terms:created>
        <terms:subject rdf:resource="http://JP_ontology.org/nis2v/Article_21.2f"/>
        <rdfs:isDefinedBy rdf:resource="http://JP_ontology.org/assessment"/>
        <skos:altLabel xml:lang="en">MCQ.112.2</skos:altLabel>
        <skos:broader rdf:resource="http://JP_ontology.org/assessment/AssessmentQuestion"/>
        <skos:definition xml:lang="en">How does the organisation evaluate the information security performance and the effectiveness of the information security management system?</skos:definition>
        <skos:prefLabel xml:lang="en">Multiple Choice Question #112.2</skos:prefLabel>
    </rdf:Description>
    <rdf:Description rdf:about="http://JP_ontology.org/assessment/MCQ.113">
        <nis2v:hasAnswer rdf:resource="http://JP_ontology.org/assessment/MCQ.113AnswerA"/>
        <nis2v:hasAnswer rdf:resource="http://JP_ontology.org/assessment/MCQ.113AnswerB"/>
        <nis2v:hasAnswer rdf:resource="http://JP_ontology.org/assessment/MCQ.113AnswerC"/>
        <nis2v:relatedToControl rdf:resource="http://JP_ontology.org/iso27001/Control9.2"/>
        <terms:contributor>Jenni Parry</terms:contributor>
        <terms:created rdf:datatype="http://www.w3.org/2001/XMLSchema#date">2024-05-20</terms:created>
        <terms:subject rdf:resource="http://JP_ontology.org/nis2v/Article_21.2f"/>
        <rdfs:isDefinedBy rdf:resource="http://JP_ontology.org/assessment"/>
        <skos:altLabel xml:lang="en">MCQ.113</skos:altLabel>
        <skos:broader rdf:resource="http://JP_ontology.org/assessment/AssessmentQuestion"/>
        <skos:definition xml:lang="en">How does the organisation ensure the effectiveness of its information security management system through internal audits?</skos:definition>
        <skos:prefLabel xml:lang="en">Multiple Choice Question #113</skos:prefLabel>
    </rdf:Description>
    <rdf:Description rdf:about="http://JP_ontology.org/assessment/MCQ.114">
        <nis2v:hasAnswer rdf:resource="http://JP_ontology.org/assessment/MCQ.114AnswerA"/>
        <nis2v:hasAnswer rdf:resource="http://JP_ontology.org/assessment/MCQ.114AnswerB"/>
        <nis2v:hasAnswer rdf:resource="http://JP_ontology.org/assessment/MCQ.114AnswerC"/>
        <nis2v:relatedToControl rdf:resource="http://JP_ontology.org/iso27001/Control9.2.2"/>
        <terms:contributor>Jenni Parry</terms:contributor>
        <terms:created rdf:datatype="http://www.w3.org/2001/XMLSchema#date">2024-05-20</terms:created>
        <terms:subject rdf:resource="http://JP_ontology.org/nis2v/Article_21.2f"/>
        <rdfs:isDefinedBy rdf:resource="http://JP_ontology.org/assessment"/>
        <skos:altLabel xml:lang="en">MCQ.114</skos:altLabel>
        <skos:broader rdf:resource="http://JP_ontology.org/assessment/AssessmentQuestion"/>
        <skos:definition xml:lang="en">How does the organisation ensure the effectiveness of its internal audit program?</skos:definition>
        <skos:prefLabel xml:lang="en">Multiple Choice Question #114</skos:prefLabel>
    </rdf:Description>
    <rdf:Description rdf:about="http://JP_ontology.org/assessment/MCQ.115">
        <nis2v:hasAnswer rdf:resource="http://JP_ontology.org/assessment/MCQ.115AnswerA"/>
        <nis2v:hasAnswer rdf:resource="http://JP_ontology.org/assessment/MCQ.115AnswerB"/>
        <nis2v:hasAnswer rdf:resource="http://JP_ontology.org/assessment/MCQ.115AnswerC"/>
        <nis2v:relatedToControl rdf:resource="http://JP_ontology.org/iso27001/Control9.3"/>
        <terms:contributor>Jenni Parry</terms:contributor>
        <terms:created rdf:datatype="http://www.w3.org/2001/XMLSchema#date">2024-05-20</terms:created>
        <terms:subject rdf:resource="http://JP_ontology.org/nis2v/Article_21.2f"/>
        <rdfs:isDefinedBy rdf:resource="http://JP_ontology.org/assessment"/>
        <skos:altLabel xml:lang="en">MCQ.115</skos:altLabel>
        <skos:broader rdf:resource="http://JP_ontology.org/assessment/AssessmentQuestion"/>
        <skos:definition xml:lang="en">How does senior management ensure the ongoing suitability, adequacy, and effectiveness of the organisation&apos;s information security management system?</skos:definition>
        <skos:prefLabel xml:lang="en">Multiple Choice Question #115</skos:prefLabel>
    </rdf:Description>
    <rdf:Description rdf:about="http://JP_ontology.org/assessment/MCQ.116">
        <nis2v:hasAnswer rdf:resource="http://JP_ontology.org/assessment/MCQ.116AnswerA"/>
        <nis2v:hasAnswer rdf:resource="http://JP_ontology.org/assessment/MCQ.116AnswerB"/>
        <nis2v:hasAnswer rdf:resource="http://JP_ontology.org/assessment/MCQ.116AnswerC"/>
        <nis2v:relatedToControl rdf:resource="http://JP_ontology.org/iso27001/Control9.3.3"/>
        <terms:contributor>Jenni Parry</terms:contributor>
        <terms:created rdf:datatype="http://www.w3.org/2001/XMLSchema#date">2024-05-20</terms:created>
        <terms:subject rdf:resource="http://JP_ontology.org/nis2v/Article_21.2f"/>
        <rdfs:isDefinedBy rdf:resource="http://JP_ontology.org/assessment"/>
        <skos:altLabel xml:lang="en">MCQ.116</skos:altLabel>
        <skos:broader rdf:resource="http://JP_ontology.org/assessment/AssessmentQuestion"/>
        <skos:definition xml:lang="en">What decisions are included in the results of the management review of the information security management system?</skos:definition>
        <skos:prefLabel xml:lang="en">Multiple Choice Question #116</skos:prefLabel>
    </rdf:Description>
    <rdf:Description rdf:about="http://JP_ontology.org/assessment/MCQ.117">
        <nis2v:hasAnswer rdf:resource="http://JP_ontology.org/assessment/MCQ.117AnswerA"/>
        <nis2v:hasAnswer rdf:resource="http://JP_ontology.org/assessment/MCQ.117AnswerB"/>
        <nis2v:hasAnswer rdf:resource="http://JP_ontology.org/assessment/MCQ.117AnswerC"/>
        <nis2v:relatedToControl rdf:resource="http://JP_ontology.org/iso27001/Control10.1"/>
        <terms:contributor>Jenni Parry</terms:contributor>
        <terms:created rdf:datatype="http://www.w3.org/2001/XMLSchema#date">2024-05-20</terms:created>
        <terms:subject rdf:resource="http://JP_ontology.org/nis2v/Article_21.2f"/>
        <rdfs:isDefinedBy rdf:resource="http://JP_ontology.org/assessment"/>
        <skos:altLabel xml:lang="en">MCQ.117</skos:altLabel>
        <skos:broader rdf:resource="http://JP_ontology.org/assessment/AssessmentQuestion"/>
        <skos:definition xml:lang="en">How does the organisation ensure the continual improvement of the suitability, adequacy, and effectiveness of the information security management system?</skos:definition>
        <skos:prefLabel xml:lang="en">Multiple Choice Question #117</skos:prefLabel>
    </rdf:Description>
    <rdf:Description rdf:about="http://JP_ontology.org/assessment/MCQ.118">
        <nis2v:hasAnswer rdf:resource="http://JP_ontology.org/assessment/MCQ.118AnswerA"/>
        <nis2v:hasAnswer rdf:resource="http://JP_ontology.org/assessment/MCQ.118AnswerB"/>
        <nis2v:hasAnswer rdf:resource="http://JP_ontology.org/assessment/MCQ.118AnswerC"/>
        <nis2v:relatedToControl rdf:resource="http://JP_ontology.org/iso27001/Control10.2"/>
        <terms:contributor>Jenni Parry</terms:contributor>
        <terms:created rdf:datatype="http://www.w3.org/2001/XMLSchema#date">2024-05-20</terms:created>
        <terms:subject rdf:resource="http://JP_ontology.org/nis2v/Article_21.2f"/>
        <rdfs:isDefinedBy rdf:resource="http://JP_ontology.org/assessment"/>
        <skos:altLabel xml:lang="en">MCQ.118</skos:altLabel>
        <skos:broader rdf:resource="http://JP_ontology.org/assessment/AssessmentQuestion"/>
        <skos:definition xml:lang="en">What steps does the organisation take when a nonconformity occurs within the information security management system?</skos:definition>
        <skos:prefLabel xml:lang="en">Multiple Choice Question #118</skos:prefLabel>
    </rdf:Description>
    <rdf:Description rdf:about="http://JP_ontology.org/assessment/MCQ.119">
        <nis2v:hasAnswer rdf:resource="http://JP_ontology.org/assessment/MCQ.119AnswerA"/>
        <nis2v:hasAnswer rdf:resource="http://JP_ontology.org/assessment/MCQ.119AnswerB"/>
        <nis2v:hasAnswer rdf:resource="http://JP_ontology.org/assessment/MCQ.119AnswerC"/>
        <nis2v:relatedToControl rdf:resource="http://JP_ontology.org/iso27001/ControlA.5.4"/>
        <terms:contributor>Jenni Parry</terms:contributor>
        <terms:created rdf:datatype="http://www.w3.org/2001/XMLSchema#date">2024-05-20</terms:created>
        <terms:subject rdf:resource="http://JP_ontology.org/nis2v/Article_21.2f"/>
        <rdfs:isDefinedBy rdf:resource="http://JP_ontology.org/assessment"/>
        <skos:altLabel xml:lang="en">MCQ.119</skos:altLabel>
        <skos:broader rdf:resource="http://JP_ontology.org/assessment/AssessmentQuestion"/>
        <skos:definition xml:lang="en">How does management ensure that all personnel apply information security in accordance with established policies and procedures?</skos:definition>
        <skos:prefLabel xml:lang="en">Multiple Choice Question #119</skos:prefLabel>
    </rdf:Description>
    <rdf:Description rdf:about="http://JP_ontology.org/assessment/MCQ.12">
        <nis2v:hasAnswer rdf:resource="http://JP_ontology.org/assessment/MCQ.12AnswerA"/>
        <nis2v:hasAnswer rdf:resource="http://JP_ontology.org/assessment/MCQ.12AnswerB"/>
        <nis2v:hasAnswer rdf:resource="http://JP_ontology.org/assessment/MCQ.12AnswerC"/>
        <nis2v:relatedToControl rdf:resource="http://JP_ontology.org/iso27001/ControlA.5.4."/>
        <terms:contributor>Jenni Parry</terms:contributor>
        <terms:created rdf:datatype="http://www.w3.org/2001/XMLSchema#date">2024-05-20</terms:created>
        <terms:subject rdf:resource="http://JP_ontology.org/nis2v/Article_21.2a"/>
        <rdfs:isDefinedBy rdf:resource="http://JP_ontology.org/assessment"/>
        <skos:altLabel xml:lang="en">MCQ.12</skos:altLabel>
        <skos:broader rdf:resource="http://JP_ontology.org/assessment/AssessmentQuestion"/>
        <skos:definition xml:lang="en">Does management require all personnel to apply information security in accordance with the established information security policy, topic-specific policies, and procedures of the organisation?</skos:definition>
        <skos:prefLabel xml:lang="en">Multiple Choice Question #12</skos:prefLabel>
    </rdf:Description>
    <rdf:Description rdf:about="http://JP_ontology.org/assessment/MCQ.120">
        <nis2v:hasAnswer rdf:resource="http://JP_ontology.org/assessment/MCQ.120AnswerA"/>
        <nis2v:hasAnswer rdf:resource="http://JP_ontology.org/assessment/MCQ.120AnswerB"/>
        <nis2v:hasAnswer rdf:resource="http://JP_ontology.org/assessment/MCQ.120AnswerC"/>
        <nis2v:relatedToControl rdf:resource="http://JP_ontology.org/iso27001/ControlA.5.13"/>
        <terms:contributor>Jenni Parry</terms:contributor>
        <terms:created rdf:datatype="http://www.w3.org/2001/XMLSchema#date">2024-05-20</terms:created>
        <terms:subject rdf:resource="http://JP_ontology.org/nis2v/Article_21.2f"/>
        <rdfs:isDefinedBy rdf:resource="http://JP_ontology.org/assessment"/>
        <skos:altLabel xml:lang="en">MCQ.120</skos:altLabel>
        <skos:broader rdf:resource="http://JP_ontology.org/assessment/AssessmentQuestion"/>
        <skos:definition xml:lang="en">How does the organisation ensure the development and implementation of appropriate procedures for information labeling in alignment with the adopted information classification scheme?</skos:definition>
        <skos:prefLabel xml:lang="en">Multiple Choice Question #120</skos:prefLabel>
    </rdf:Description>
    <rdf:Description rdf:about="http://JP_ontology.org/assessment/MCQ.121">
        <nis2v:hasAnswer rdf:resource="http://JP_ontology.org/assessment/MCQ.121AnswerA"/>
        <nis2v:hasAnswer rdf:resource="http://JP_ontology.org/assessment/MCQ.121AnswerB"/>
        <nis2v:hasAnswer rdf:resource="http://JP_ontology.org/assessment/MCQ.121AnswerC"/>
        <nis2v:relatedToControl rdf:resource="http://JP_ontology.org/iso27001/ControlA.8.32"/>
        <terms:contributor>Jenni Parry</terms:contributor>
        <terms:created rdf:datatype="http://www.w3.org/2001/XMLSchema#date">2024-05-20</terms:created>
        <terms:subject rdf:resource="http://JP_ontology.org/nis2v/Article_21.2g"/>
        <rdfs:isDefinedBy rdf:resource="http://JP_ontology.org/assessment"/>
        <skos:altLabel xml:lang="en">MCQ.121</skos:altLabel>
        <skos:broader rdf:resource="http://JP_ontology.org/assessment/AssessmentQuestion"/>
        <skos:definition xml:lang="en">How does the organisation ensure that changes to information processing facilities and information systems are managed effectively?</skos:definition>
        <skos:prefLabel xml:lang="en">Multiple Choice Question #121</skos:prefLabel>
    </rdf:Description>
    <rdf:Description rdf:about="http://JP_ontology.org/assessment/MCQ.122">
        <nis2v:hasAnswer rdf:resource="http://JP_ontology.org/assessment/MCQ.122AnswerA"/>
        <nis2v:hasAnswer rdf:resource="http://JP_ontology.org/assessment/MCQ.122AnswerB"/>
        <nis2v:hasAnswer rdf:resource="http://JP_ontology.org/assessment/MCQ.122AnswerC"/>
        <nis2v:relatedToControl rdf:resource="http://JP_ontology.org/iso27001/ControlA.8.34"/>
        <terms:contributor>Jenni Parry</terms:contributor>
        <terms:created rdf:datatype="http://www.w3.org/2001/XMLSchema#date">2024-05-20</terms:created>
        <terms:subject rdf:resource="http://JP_ontology.org/nis2v/Article_21.2g"/>
        <rdfs:isDefinedBy rdf:resource="http://JP_ontology.org/assessment"/>
        <skos:altLabel xml:lang="en">MCQ.122</skos:altLabel>
        <skos:broader rdf:resource="http://JP_ontology.org/assessment/AssessmentQuestion"/>
        <skos:definition xml:lang="en">How does the organisation ensure that audit tests and other assurance activities involving the assessment of operational systems are effectively planned and agreed upon?</skos:definition>
        <skos:prefLabel xml:lang="en">Multiple Choice Question #122</skos:prefLabel>
    </rdf:Description>
    <rdf:Description rdf:about="http://JP_ontology.org/assessment/MCQ.123">
        <nis2v:hasAnswer rdf:resource="http://JP_ontology.org/assessment/MCQ.123AnswerA"/>
        <nis2v:hasAnswer rdf:resource="http://JP_ontology.org/assessment/MCQ.123AnswerB"/>
        <nis2v:hasAnswer rdf:resource="http://JP_ontology.org/assessment/MCQ.123AnswerC"/>
        <nis2v:relatedToControl rdf:resource="http://JP_ontology.org/iso27001/ControlA.5.32"/>
        <terms:contributor>Jenni Parry</terms:contributor>
        <terms:created rdf:datatype="http://www.w3.org/2001/XMLSchema#date">2024-05-20</terms:created>
        <terms:subject rdf:resource="http://JP_ontology.org/nis2v/Article_21.2g"/>
        <rdfs:isDefinedBy rdf:resource="http://JP_ontology.org/assessment"/>
        <skos:altLabel xml:lang="en">MCQ.123</skos:altLabel>
        <skos:broader rdf:resource="http://JP_ontology.org/assessment/AssessmentQuestion"/>
        <skos:definition xml:lang="en">How does the organisation ensure the protection of intellectual property rights through the implementation of appropriate procedures?</skos:definition>
        <skos:prefLabel xml:lang="en">Multiple Choice Question #123</skos:prefLabel>
    </rdf:Description>
    <rdf:Description rdf:about="http://JP_ontology.org/assessment/MCQ.124">
        <nis2v:hasAnswer rdf:resource="http://JP_ontology.org/assessment/MCQ.124AnswerA"/>
        <nis2v:hasAnswer rdf:resource="http://JP_ontology.org/assessment/MCQ.124AnswerB"/>
        <nis2v:hasAnswer rdf:resource="http://JP_ontology.org/assessment/MCQ.124AnswerC"/>
        <nis2v:relatedToControl rdf:resource="http://JP_ontology.org/iso27001/ControlA.5.33"/>
        <terms:contributor>Jenni Parry</terms:contributor>
        <terms:created rdf:datatype="http://www.w3.org/2001/XMLSchema#date">2024-05-20</terms:created>
        <terms:subject rdf:resource="http://JP_ontology.org/nis2v/Article_21.2g"/>
        <rdfs:isDefinedBy rdf:resource="http://JP_ontology.org/assessment"/>
        <skos:altLabel xml:lang="en">MCQ.124</skos:altLabel>
        <skos:broader rdf:resource="http://JP_ontology.org/assessment/AssessmentQuestion"/>
        <skos:definition xml:lang="en">How does the organisation ensure the protection of records from loss, destruction, falsification, unauthorized access, and unauthorized release?</skos:definition>
        <skos:prefLabel xml:lang="en">Multiple Choice Question #124</skos:prefLabel>
    </rdf:Description>
    <rdf:Description rdf:about="http://JP_ontology.org/assessment/MCQ.125">
        <nis2v:hasAnswer rdf:resource="http://JP_ontology.org/assessment/MCQ.125AnswerA"/>
        <nis2v:hasAnswer rdf:resource="http://JP_ontology.org/assessment/MCQ.125AnswerB"/>
        <nis2v:hasAnswer rdf:resource="http://JP_ontology.org/assessment/MCQ.125AnswerC"/>
        <nis2v:relatedToControl rdf:resource="http://JP_ontology.org/iso27001/ControlA.8.25"/>
        <terms:contributor>Jenni Parry</terms:contributor>
        <terms:created rdf:datatype="http://www.w3.org/2001/XMLSchema#date">2024-05-20</terms:created>
        <terms:subject rdf:resource="http://JP_ontology.org/nis2v/Article_21.2g"/>
        <rdfs:isDefinedBy rdf:resource="http://JP_ontology.org/assessment"/>
        <skos:altLabel xml:lang="en">MCQ.125</skos:altLabel>
        <skos:broader rdf:resource="http://JP_ontology.org/assessment/AssessmentQuestion"/>
        <skos:definition xml:lang="en">How does the organisation ensure the establishment and application of rules for the secure development of software and systems?</skos:definition>
        <skos:prefLabel xml:lang="en">Multiple Choice Question #125</skos:prefLabel>
    </rdf:Description>
    <rdf:Description rdf:about="http://JP_ontology.org/assessment/MCQ.126">
        <nis2v:hasAnswer rdf:resource="http://JP_ontology.org/assessment/MCQ.126AnswerA"/>
        <nis2v:hasAnswer rdf:resource="http://JP_ontology.org/assessment/MCQ.126AnswerB"/>
        <nis2v:hasAnswer rdf:resource="http://JP_ontology.org/assessment/MCQ.126AnswerC"/>
        <nis2v:relatedToControl rdf:resource="http://JP_ontology.org/iso27001/ControlA.8.26"/>
        <terms:contributor>Jenni Parry</terms:contributor>
        <terms:created rdf:datatype="http://www.w3.org/2001/XMLSchema#date">2024-05-20</terms:created>
        <terms:subject rdf:resource="http://JP_ontology.org/nis2v/Article_21.2g"/>
        <rdfs:isDefinedBy rdf:resource="http://JP_ontology.org/assessment"/>
        <skos:altLabel xml:lang="en">MCQ.126</skos:altLabel>
        <skos:broader rdf:resource="http://JP_ontology.org/assessment/AssessmentQuestion"/>
        <skos:definition xml:lang="en">How does the organisation ensure the identification, specification, and approval of information security requirements during the development or acquisition of applications?</skos:definition>
        <skos:prefLabel xml:lang="en">Multiple Choice Question #126</skos:prefLabel>
    </rdf:Description>
    <rdf:Description rdf:about="http://JP_ontology.org/assessment/MCQ.127">
        <nis2v:hasAnswer rdf:resource="http://JP_ontology.org/assessment/MCQ.127AnswerA"/>
        <nis2v:hasAnswer rdf:resource="http://JP_ontology.org/assessment/MCQ.127AnswerB"/>
        <nis2v:hasAnswer rdf:resource="http://JP_ontology.org/assessment/MCQ.127AnswerC"/>
        <nis2v:relatedToControl rdf:resource="http://JP_ontology.org/iso27001/ControlA.8.27"/>
        <terms:contributor>Jenni Parry</terms:contributor>
        <terms:created rdf:datatype="http://www.w3.org/2001/XMLSchema#date">2024-05-20</terms:created>
        <terms:subject rdf:resource="http://JP_ontology.org/nis2v/Article_21.2g"/>
        <rdfs:isDefinedBy rdf:resource="http://JP_ontology.org/assessment"/>
        <skos:altLabel xml:lang="en">MCQ.127</skos:altLabel>
        <skos:broader rdf:resource="http://JP_ontology.org/assessment/AssessmentQuestion"/>
        <skos:definition xml:lang="en">How does the organisation ensure the establishment, documentation, maintenance, and application of principles for engineering secure systems to information system development activities?</skos:definition>
        <skos:prefLabel xml:lang="en">Multiple Choice Question #127</skos:prefLabel>
    </rdf:Description>
    <rdf:Description rdf:about="http://JP_ontology.org/assessment/MCQ.128">
        <nis2v:hasAnswer rdf:resource="http://JP_ontology.org/assessment/MCQ.128AnswerA"/>
        <nis2v:hasAnswer rdf:resource="http://JP_ontology.org/assessment/MCQ.128AnswerB"/>
        <nis2v:hasAnswer rdf:resource="http://JP_ontology.org/assessment/MCQ.128AnswerC"/>
        <nis2v:relatedToControl rdf:resource="http://JP_ontology.org/iso27001/ControlA.8.30"/>
        <terms:contributor>Jenni Parry</terms:contributor>
        <terms:created rdf:datatype="http://www.w3.org/2001/XMLSchema#date">2024-05-20</terms:created>
        <terms:subject rdf:resource="http://JP_ontology.org/nis2v/Article_21.2g"/>
        <rdfs:isDefinedBy rdf:resource="http://JP_ontology.org/assessment"/>
        <skos:altLabel xml:lang="en">MCQ.128</skos:altLabel>
        <skos:broader rdf:resource="http://JP_ontology.org/assessment/AssessmentQuestion"/>
        <skos:definition xml:lang="en">How does the organisation ensure the direction, monitoring, and review of activities related to outsourced system development?</skos:definition>
        <skos:prefLabel xml:lang="en">Multiple Choice Question #128</skos:prefLabel>
    </rdf:Description>
    <rdf:Description rdf:about="http://JP_ontology.org/assessment/MCQ.129">
        <nis2v:hasAnswer rdf:resource="http://JP_ontology.org/assessment/MCQ.129AnswerA"/>
        <nis2v:hasAnswer rdf:resource="http://JP_ontology.org/assessment/MCQ.129AnswerB"/>
        <nis2v:hasAnswer rdf:resource="http://JP_ontology.org/assessment/MCQ.129AnswerC"/>
        <nis2v:relatedToControl rdf:resource="http://JP_ontology.org/iso27001/ControlA.7.1"/>
        <terms:contributor>Jenni Parry</terms:contributor>
        <terms:created rdf:datatype="http://www.w3.org/2001/XMLSchema#date">2024-05-20</terms:created>
        <terms:subject rdf:resource="http://JP_ontology.org/nis2v/Article_21.2i"/>
        <rdfs:isDefinedBy rdf:resource="http://JP_ontology.org/assessment"/>
        <skos:altLabel xml:lang="en">MCQ.129</skos:altLabel>
        <skos:broader rdf:resource="http://JP_ontology.org/assessment/AssessmentQuestion"/>
        <skos:definition xml:lang="en">How does the organisation define and utilize security perimeters to protect areas containing information and associated assets?</skos:definition>
        <skos:prefLabel xml:lang="en">Multiple Choice Question #129</skos:prefLabel>
    </rdf:Description>
    <rdf:Description rdf:about="http://JP_ontology.org/assessment/MCQ.13">
        <nis2v:hasAnswer rdf:resource="http://JP_ontology.org/assessment/MCQ13AnswerA"/>
        <nis2v:hasAnswer rdf:resource="http://JP_ontology.org/assessment/MCQ13AnswerB"/>
        <nis2v:hasAnswer rdf:resource="http://JP_ontology.org/assessment/MCQ13AnswerC"/>
        <nis2v:relatedToControl rdf:resource="http://JP_ontology.org/iso27001/ControlA.5.5"/>
        <terms:contributor>Jenni Parry</terms:contributor>
        <terms:created rdf:datatype="http://www.w3.org/2001/XMLSchema#date">2024-04-17</terms:created>
        <terms:subject rdf:resource="http://JP_ontology.org/nis2v/Article_21.2a"/>
        <rdfs:isDefinedBy rdf:resource="http://JP_ontology.org/assessment"/>
        <skos:altLabel xml:lang="en">MCQ.13</skos:altLabel>
        <skos:broader rdf:resource="http://JP_ontology.org/assessment/AssessmentQuestion"/>
        <skos:definition xml:lang="en">Does the organisation establish and maintain contact with relevant authorities?</skos:definition>
        <skos:prefLabel xml:lang="en">Multiple Choice Question #13</skos:prefLabel>
    </rdf:Description>
    <rdf:Description rdf:about="http://JP_ontology.org/assessment/MCQ.130">
        <nis2v:hasAnswer rdf:resource="http://JP_ontology.org/assessment/MCQ.130AnswerA"/>
        <nis2v:hasAnswer rdf:resource="http://JP_ontology.org/assessment/MCQ.130AnswerB"/>
        <nis2v:hasAnswer rdf:resource="http://JP_ontology.org/assessment/MCQ.130AnswerC"/>
        <nis2v:relatedToControl rdf:resource="http://JP_ontology.org/iso27001/ControlA.7.13"/>
        <terms:contributor>Jenni Parry</terms:contributor>
        <terms:created rdf:datatype="http://www.w3.org/2001/XMLSchema#date">2024-05-20</terms:created>
        <terms:subject rdf:resource="http://JP_ontology.org/nis2v/Article_21.2i"/>
        <rdfs:isDefinedBy rdf:resource="http://JP_ontology.org/assessment"/>
        <skos:altLabel xml:lang="en">MCQ.130</skos:altLabel>
        <skos:broader rdf:resource="http://JP_ontology.org/assessment/AssessmentQuestion"/>
        <skos:definition xml:lang="en">How does the organisation ensure that equipment is maintained correctly to uphold the availability, integrity, and confidentiality of information?</skos:definition>
        <skos:prefLabel xml:lang="en">Multiple Choice Question #130</skos:prefLabel>
    </rdf:Description>
    <rdf:Description rdf:about="http://JP_ontology.org/assessment/MCQ.14">
        <nis2v:hasAnswer rdf:resource="http://JP_ontology.org/assessment/MCQ14AnswerA"/>
        <nis2v:hasAnswer rdf:resource="http://JP_ontology.org/assessment/MCQ14AnswerB"/>
        <nis2v:hasAnswer rdf:resource="http://JP_ontology.org/assessment/MCQ14AnswerC"/>
        <nis2v:relatedToControl rdf:resource="http://JP_ontology.org/iso27001/ControlA.5.6"/>
        <terms:contributor>Jenni Parry</terms:contributor>
        <terms:created rdf:datatype="http://www.w3.org/2001/XMLSchema#date">2024-04-18</terms:created>
        <terms:subject rdf:resource="http://JP_ontology.org/nis2v/Article_21.2a"/>
        <rdfs:isDefinedBy rdf:resource="http://JP_ontology.org/assessment"/>
        <skos:altLabel xml:lang="en">MCQ.14</skos:altLabel>
        <skos:broader rdf:resource="http://JP_ontology.org/assessment/AssessmentQuestion"/>
        <skos:definition xml:lang="en">Does the organisation establish and maintain contact with special interest groups or other specialist security forums and professional associations?</skos:definition>
        <skos:prefLabel xml:lang="en">Multiple Choice Question #14</skos:prefLabel>
    </rdf:Description>
    <rdf:Description rdf:about="http://JP_ontology.org/assessment/MCQ.15">
        <nis2v:hasAnswer rdf:resource="http://JP_ontology.org/assessment/MCQ15AnswerA"/>
        <nis2v:hasAnswer rdf:resource="http://JP_ontology.org/assessment/MCQ15AnswerB"/>
        <nis2v:hasAnswer rdf:resource="http://JP_ontology.org/assessment/MCQ15AnswerC"/>
        <nis2v:relatedToControl rdf:resource="http://JP_ontology.org/iso27001/ControlA.5.7"/>
        <terms:contributor>Jenni Parry</terms:contributor>
        <terms:created rdf:datatype="http://www.w3.org/2001/XMLSchema#date">2024-04-18</terms:created>
        <terms:subject rdf:resource="http://JP_ontology.org/nis2v/Article_21.2a"/>
        <rdfs:isDefinedBy rdf:resource="http://JP_ontology.org/assessment"/>
        <skos:altLabel xml:lang="en">MCQ.15</skos:altLabel>
        <skos:broader rdf:resource="http://JP_ontology.org/assessment/AssessmentQuestion"/>
        <skos:definition xml:lang="en">Is information relating to information security threats collected and analysed to produce threat intelligence?</skos:definition>
        <skos:prefLabel xml:lang="en">Multiple Choice Question #15</skos:prefLabel>
    </rdf:Description>
    <rdf:Description rdf:about="http://JP_ontology.org/assessment/MCQ.16">
        <nis2v:hasAnswer rdf:resource="http://JP_ontology.org/assessment/MCQ.16AnswerA"/>
        <nis2v:hasAnswer rdf:resource="http://JP_ontology.org/assessment/MCQ.16AnswerB"/>
        <nis2v:hasAnswer rdf:resource="http://JP_ontology.org/assessment/MCQ.16AnswerC"/>
        <nis2v:relatedToControl rdf:resource="http://JP_ontology.org/iso27001/ControlA.5.31"/>
        <terms:contributor>Jenni Parry</terms:contributor>
        <terms:created rdf:datatype="http://www.w3.org/2001/XMLSchema#date">2024-05-20</terms:created>
        <terms:subject rdf:resource="http://JP_ontology.org/nis2v/Article_21.2a"/>
        <rdfs:isDefinedBy rdf:resource="http://JP_ontology.org/assessment"/>
        <skos:altLabel xml:lang="en">MCQ.16</skos:altLabel>
        <skos:broader rdf:resource="http://JP_ontology.org/assessment/AssessmentQuestion"/>
        <skos:definition xml:lang="en">Are legal, statutory, regulatory, and contractual requirements relevant to information security, along with the organisation’s approach to meeting these requirements, identified, documented, and kept up to date?</skos:definition>
        <skos:prefLabel xml:lang="en">Multiple Choice Question #16</skos:prefLabel>
    </rdf:Description>
    <rdf:Description rdf:about="http://JP_ontology.org/assessment/MCQ.17">
        <nis2v:hasAnswer rdf:resource="http://JP_ontology.org/assessment/MCQ17AnswerA"/>
        <nis2v:hasAnswer rdf:resource="http://JP_ontology.org/assessment/MCQ17AnswerB"/>
        <nis2v:hasAnswer rdf:resource="http://JP_ontology.org/assessment/MCQ17AnswerC"/>
        <nis2v:relatedToControl rdf:resource="http://JP_ontology.org/iso27001/ControlA.5.37"/>
        <terms:contributor>Jenni Parry</terms:contributor>
        <terms:created rdf:datatype="http://www.w3.org/2001/XMLSchema#date">2024-04-18</terms:created>
        <terms:subject rdf:resource="http://JP_ontology.org/nis2v/Article_21.2a"/>
        <rdfs:isDefinedBy rdf:resource="http://JP_ontology.org/assessment"/>
        <skos:altLabel xml:lang="en">MCQ.17</skos:altLabel>
        <skos:broader rdf:resource="http://JP_ontology.org/assessment/AssessmentQuestion"/>
        <skos:definition xml:lang="en">Are operating procedures for information processing facilities documented and made available to personnel who require them?</skos:definition>
        <skos:prefLabel xml:lang="en">Multiple Choice Question #17</skos:prefLabel>
    </rdf:Description>
    <rdf:Description rdf:about="http://JP_ontology.org/assessment/MCQ.18">
        <nis2v:hasAnswer rdf:resource="http://JP_ontology.org/assessment/MCQ.18AnswerA"/>
        <nis2v:hasAnswer rdf:resource="http://JP_ontology.org/assessment/MCQ.18AnswerB"/>
        <nis2v:hasAnswer rdf:resource="http://JP_ontology.org/assessment/MCQ.18AnswerC"/>
        <nis2v:relatedToControl rdf:resource="http://JP_ontology.org/iso27001/ControlA.5.24"/>
        <terms:contributor>Jenni Parry</terms:contributor>
        <terms:created rdf:datatype="http://www.w3.org/2001/XMLSchema#date">2024-05-20</terms:created>
        <terms:subject rdf:resource="http://JP_ontology.org/nis2v/Article_21.2b"/>
        <rdfs:isDefinedBy rdf:resource="http://JP_ontology.org/assessment"/>
        <skos:altLabel xml:lang="en">MCQ.18</skos:altLabel>
        <skos:broader rdf:resource="http://JP_ontology.org/assessment/AssessmentQuestion"/>
        <skos:definition xml:lang="en">Does the organisation plan and prepare for managing information security incidents by defining, establishing, and communicating information security incident management processes, roles, and responsibilities?</skos:definition>
        <skos:prefLabel xml:lang="en">Multiple Choice Question #18</skos:prefLabel>
    </rdf:Description>
    <rdf:Description rdf:about="http://JP_ontology.org/assessment/MCQ.19">
        <nis2v:hasAnswer rdf:resource="http://JP_ontology.org/assessment/MCQ.19AnswerA"/>
        <nis2v:hasAnswer rdf:resource="http://JP_ontology.org/assessment/MCQ.19AnswerB"/>
        <nis2v:hasAnswer rdf:resource="http://JP_ontology.org/assessment/MCQ.19AnswerC"/>
        <nis2v:relatedToControl rdf:resource="http://JP_ontology.org/iso27001/ControlA.5.25"/>
        <terms:contributor>Jenni Parry</terms:contributor>
        <terms:created rdf:datatype="http://www.w3.org/2001/XMLSchema#date">2024-05-20</terms:created>
        <terms:subject rdf:resource="http://JP_ontology.org/nis2v/Article_21.2b"/>
        <rdfs:isDefinedBy rdf:resource="http://JP_ontology.org/assessment"/>
        <skos:altLabel xml:lang="en">MCQ.19</skos:altLabel>
        <skos:broader rdf:resource="http://JP_ontology.org/assessment/AssessmentQuestion"/>
        <skos:definition xml:lang="en">Does the organisation assess information security events and decide if they are to be categorized as information security incidents?</skos:definition>
        <skos:prefLabel xml:lang="en">Multiple Choice Question #19</skos:prefLabel>
    </rdf:Description>
    <rdf:Description rdf:about="http://JP_ontology.org/assessment/MCQ.2.1">
        <nis2v:hasAnswer rdf:resource="http://JP_ontology.org/assessment/MCQ.2.1AnswerA"/>
        <nis2v:hasAnswer rdf:resource="http://JP_ontology.org/assessment/MCQ.2.1AnswerB"/>
        <nis2v:hasAnswer rdf:resource="http://JP_ontology.org/assessment/MCQ.2.1AnswerC"/>
        <nis2v:relatedToControl rdf:resource="http://JP_ontology.org/iso27001/Control5.2"/>
        <terms:contributor>Jenni Parry</terms:contributor>
        <terms:created rdf:datatype="http://www.w3.org/2001/XMLSchema#date">2024-05-20</terms:created>
        <terms:subject rdf:resource="http://JP_ontology.org/nis2v/Article_21.2a"/>
        <rdfs:isDefinedBy rdf:resource="http://JP_ontology.org/assessment"/>
        <skos:altLabel xml:lang="en">MCQ.2.1</skos:altLabel>
        <skos:broader rdf:resource="http://JP_ontology.org/assessment/AssessmentQuestion"/>
        <skos:definition xml:lang="en">Does top management establish an information security policy that is appropriate to the purpose of the organisation, includes information security objectives or provides a framework for setting them, commits to satisfying applicable requirements related to information security, and commits to continually improving the information security management system? </skos:definition>
        <skos:prefLabel xml:lang="en">Multiple Choice Question #2.1</skos:prefLabel>
    </rdf:Description>
    <rdf:Description rdf:about="http://JP_ontology.org/assessment/MCQ.2.2">
        <nis2v:hasAnswer rdf:resource="http://JP_ontology.org/assessment/MCQ.2.2AnswerA"/>
        <nis2v:hasAnswer rdf:resource="http://JP_ontology.org/assessment/MCQ.2.2AnswerB"/>
        <nis2v:hasAnswer rdf:resource="http://JP_ontology.org/assessment/MCQ.2.2AnswerC"/>
        <nis2v:relatedToControl rdf:resource="http://JP_ontology.org/iso27001/Control5.2"/>
        <terms:contributor>Jenni Parry</terms:contributor>
        <terms:created rdf:datatype="http://www.w3.org/2001/XMLSchema#date">2024-05-20</terms:created>
        <terms:subject rdf:resource="http://JP_ontology.org/nis2v/Article_21.2a"/>
        <rdfs:isDefinedBy rdf:resource="http://JP_ontology.org/assessment"/>
        <skos:altLabel xml:lang="en">MCQ.2.2</skos:altLabel>
        <skos:broader rdf:resource="http://JP_ontology.org/assessment/AssessmentQuestion"/>
        <skos:definition xml:lang="en">Is the information security policy available as documented information, communicated within the organisation, and available to interested parties as appropriate?</skos:definition>
        <skos:prefLabel xml:lang="en">Multiple Choice Question #2.2</skos:prefLabel>
    </rdf:Description>
    <rdf:Description rdf:about="http://JP_ontology.org/assessment/MCQ.20">
        <nis2v:hasAnswer rdf:resource="http://JP_ontology.org/assessment/MCQ.20AnswerA"/>
        <nis2v:hasAnswer rdf:resource="http://JP_ontology.org/assessment/MCQ.20AnswerB"/>
        <nis2v:hasAnswer rdf:resource="http://JP_ontology.org/assessment/MCQ.20AnswerC"/>
        <nis2v:relatedToControl rdf:resource="http://JP_ontology.org/iso27001/ControlA.5.26"/>
        <terms:contributor>Jenni Parry</terms:contributor>
        <terms:created rdf:datatype="http://www.w3.org/2001/XMLSchema#date">2024-05-20</terms:created>
        <terms:subject rdf:resource="http://JP_ontology.org/nis2v/Article_21.2b"/>
        <rdfs:isDefinedBy rdf:resource="http://JP_ontology.org/assessment"/>
        <skos:altLabel xml:lang="en">MCQ.20</skos:altLabel>
        <skos:broader rdf:resource="http://JP_ontology.org/assessment/AssessmentQuestion"/>
        <skos:definition xml:lang="en">Are information security incidents responded to in accordance with the documented procedures?</skos:definition>
        <skos:prefLabel xml:lang="en">Multiple Choice Question #20</skos:prefLabel>
    </rdf:Description>
    <rdf:Description rdf:about="http://JP_ontology.org/assessment/MCQ.21">
        <nis2v:hasAnswer rdf:resource="http://JP_ontology.org/assessment/MCQ.21AnswerA"/>
        <nis2v:hasAnswer rdf:resource="http://JP_ontology.org/assessment/MCQ.21AnswerB"/>
        <nis2v:hasAnswer rdf:resource="http://JP_ontology.org/assessment/MCQ.21AnswerC"/>
        <nis2v:relatedToControl rdf:resource="http://JP_ontology.org/iso27001/ControlA.5.27"/>
        <terms:contributor>Jenni Parry</terms:contributor>
        <terms:created rdf:datatype="http://www.w3.org/2001/XMLSchema#date">2024-05-20</terms:created>
        <terms:subject rdf:resource="http://JP_ontology.org/nis2v/Article_21.2b"/>
        <rdfs:isDefinedBy rdf:resource="http://JP_ontology.org/assessment"/>
        <skos:altLabel xml:lang="en">MCQ.21</skos:altLabel>
        <skos:broader rdf:resource="http://JP_ontology.org/assessment/AssessmentQuestion"/>
        <skos:definition xml:lang="en">Is knowledge gained from information security incidents used to strengthen and improve the information security controls?</skos:definition>
        <skos:prefLabel xml:lang="en">Multiple Choice Question #21</skos:prefLabel>
    </rdf:Description>
    <rdf:Description rdf:about="http://JP_ontology.org/assessment/MCQ.22.1">
        <nis2v:hasAnswer rdf:resource="http://JP_ontology.org/assessment/MCQ.22.1AnswerA"/>
        <nis2v:hasAnswer rdf:resource="http://JP_ontology.org/assessment/MCQ.22.1AnswerB"/>
        <nis2v:hasAnswer rdf:resource="http://JP_ontology.org/assessment/MCQ.22.1AnswerC"/>
        <nis2v:relatedToControl rdf:resource="http://JP_ontology.org/iso27001/ControlA.5.28"/>
        <terms:contributor>Jenni Parry</terms:contributor>
        <terms:created rdf:datatype="http://www.w3.org/2001/XMLSchema#date">2024-05-20</terms:created>
        <terms:subject rdf:resource="http://JP_ontology.org/nis2v/Article_21.2b"/>
        <rdfs:isDefinedBy rdf:resource="http://JP_ontology.org/assessment"/>
        <skos:altLabel xml:lang="en">MCQ.22.1</skos:altLabel>
        <skos:broader rdf:resource="http://JP_ontology.org/assessment/AssessmentQuestion"/>
        <skos:definition xml:lang="en">Does top management establish an information security policy that is appropriate to the purpose of the organisation?</skos:definition>
        <skos:prefLabel xml:lang="en">Multiple Choice Question #22.1</skos:prefLabel>
    </rdf:Description>
    <rdf:Description rdf:about="http://JP_ontology.org/assessment/MCQ.22.2">
        <nis2v:hasAnswer rdf:resource="http://JP_ontology.org/assessment/MCQ.22.2AnswerA"/>
        <nis2v:hasAnswer rdf:resource="http://JP_ontology.org/assessment/MCQ.22.2AnswerB"/>
        <nis2v:hasAnswer rdf:resource="http://JP_ontology.org/assessment/MCQ.22.2AnswerC"/>
        <nis2v:relatedToControl rdf:resource="http://JP_ontology.org/iso27001/ControlA.5.28"/>
        <terms:contributor>Jenni Parry</terms:contributor>
        <terms:created rdf:datatype="http://www.w3.org/2001/XMLSchema#date">2024-05-20</terms:created>
        <terms:subject rdf:resource="http://JP_ontology.org/nis2v/Article_21.2b"/>
        <rdfs:isDefinedBy rdf:resource="http://JP_ontology.org/assessment"/>
        <skos:altLabel xml:lang="en">MCQ.22.2</skos:altLabel>
        <skos:broader rdf:resource="http://JP_ontology.org/assessment/AssessmentQuestion"/>
        <skos:definition xml:lang="en">Does the information security policy include information security objectives or provide a framework for setting them?</skos:definition>
        <skos:prefLabel xml:lang="en">Multiple Choice Question #22.2</skos:prefLabel>
    </rdf:Description>
    <rdf:Description rdf:about="http://JP_ontology.org/assessment/MCQ.22.3">
        <nis2v:hasAnswer rdf:resource="http://JP_ontology.org/assessment/MCQ.22.3AnswerA"/>
        <nis2v:hasAnswer rdf:resource="http://JP_ontology.org/assessment/MCQ.22.3AnswerB"/>
        <nis2v:hasAnswer rdf:resource="http://JP_ontology.org/assessment/MCQ.22.3AnswerC"/>
        <nis2v:relatedToControl rdf:resource="http://JP_ontology.org/iso27001/ControlA.5.28"/>
        <terms:contributor>Jenni Parry</terms:contributor>
        <terms:created rdf:datatype="http://www.w3.org/2001/XMLSchema#date">2024-05-20</terms:created>
        <terms:subject rdf:resource="http://JP_ontology.org/nis2v/Article_21.2b"/>
        <rdfs:isDefinedBy rdf:resource="http://JP_ontology.org/assessment"/>
        <skos:altLabel xml:lang="en">MCQ.22.3</skos:altLabel>
        <skos:broader rdf:resource="http://JP_ontology.org/assessment/AssessmentQuestion"/>
        <skos:definition xml:lang="en">Does the information security policy include a commitment to satisfy applicable requirements related to information security?</skos:definition>
        <skos:prefLabel xml:lang="en">Multiple Choice Question #22.3</skos:prefLabel>
    </rdf:Description>
    <rdf:Description rdf:about="http://JP_ontology.org/assessment/MCQ.22.4">
        <nis2v:hasAnswer rdf:resource="http://JP_ontology.org/assessment/MCQ.22.4AnswerA"/>
        <nis2v:hasAnswer rdf:resource="http://JP_ontology.org/assessment/MCQ.22.4AnswerB"/>
        <nis2v:hasAnswer rdf:resource="http://JP_ontology.org/assessment/MCQ.22.4AnswerC"/>
        <nis2v:relatedToControl rdf:resource="http://JP_ontology.org/iso27001/ControlA.5.28"/>
        <terms:contributor>Jenni Parry</terms:contributor>
        <terms:created rdf:datatype="http://www.w3.org/2001/XMLSchema#date">2024-05-20</terms:created>
        <terms:subject rdf:resource="http://JP_ontology.org/nis2v/Article_21.2b"/>
        <rdfs:isDefinedBy rdf:resource="http://JP_ontology.org/assessment"/>
        <skos:altLabel xml:lang="en">MCQ.22.4</skos:altLabel>
        <skos:broader rdf:resource="http://JP_ontology.org/assessment/AssessmentQuestion"/>
        <skos:definition xml:lang="en">Does the information security policy include a commitment to continual improvement of the information security management system?</skos:definition>
        <skos:prefLabel xml:lang="en">Multiple Choice Question #22.4</skos:prefLabel>
    </rdf:Description>
    <rdf:Description rdf:about="http://JP_ontology.org/assessment/MCQ.22.5">
        <nis2v:hasAnswer rdf:resource="http://JP_ontology.org/assessment/MCQ.22.5AnswerA"/>
        <nis2v:hasAnswer rdf:resource="http://JP_ontology.org/assessment/MCQ.22.5AnswerB"/>
        <nis2v:hasAnswer rdf:resource="http://JP_ontology.org/assessment/MCQ.22.5AnswerC"/>
        <nis2v:relatedToControl rdf:resource="http://JP_ontology.org/iso27001/ControlA.5.28"/>
        <terms:contributor>Jenni Parry</terms:contributor>
        <terms:created rdf:datatype="http://www.w3.org/2001/XMLSchema#date">2024-05-20</terms:created>
        <terms:subject rdf:resource="http://JP_ontology.org/nis2v/Article_21.2b"/>
        <rdfs:isDefinedBy rdf:resource="http://JP_ontology.org/assessment"/>
        <skos:altLabel xml:lang="en">MCQ.22.5</skos:altLabel>
        <skos:broader rdf:resource="http://JP_ontology.org/assessment/AssessmentQuestion"/>
        <skos:definition xml:lang="en">Is the information security policy available as documented information, communicated within the organisation, and available to interested parties, as appropriate?</skos:definition>
        <skos:prefLabel xml:lang="en">Multiple Choice Question #22.5</skos:prefLabel>
    </rdf:Description>
    <rdf:Description rdf:about="http://JP_ontology.org/assessment/MCQ.23">
        <nis2v:hasAnswer rdf:resource="http://JP_ontology.org/assessment/MCQ.23AnswerA"/>
        <nis2v:hasAnswer rdf:resource="http://JP_ontology.org/assessment/MCQ.23AnswerB"/>
        <nis2v:hasAnswer rdf:resource="http://JP_ontology.org/assessment/MCQ.23AnswerC"/>
        <nis2v:relatedToControl rdf:resource="http://JP_ontology.org/iso27001/ControlA.6.8"/>
        <terms:contributor>Jenni Parry</terms:contributor>
        <terms:created rdf:datatype="http://www.w3.org/2001/XMLSchema#date">2024-05-20</terms:created>
        <terms:subject rdf:resource="http://JP_ontology.org/nis2v/Article_21.2b"/>
        <rdfs:isDefinedBy rdf:resource="http://JP_ontology.org/assessment"/>
        <skos:altLabel xml:lang="en">MCQ.23</skos:altLabel>
        <skos:broader rdf:resource="http://JP_ontology.org/assessment/AssessmentQuestion"/>
        <skos:definition xml:lang="en">Does the organisation provide a mechanism for personnel to report observed or suspected information security events through appropriate channels in a timely manner?</skos:definition>
        <skos:prefLabel xml:lang="en">Multiple Choice Question #23</skos:prefLabel>
    </rdf:Description>
    <rdf:Description rdf:about="http://JP_ontology.org/assessment/MCQ.24">
        <nis2v:hasAnswer rdf:resource="http://JP_ontology.org/assessment/MCQ.24AnswerA"/>
        <nis2v:hasAnswer rdf:resource="http://JP_ontology.org/assessment/MCQ.24AnswerB"/>
        <nis2v:hasAnswer rdf:resource="http://JP_ontology.org/assessment/MCQ.24AnswerC"/>
        <nis2v:relatedToControl rdf:resource="http://JP_ontology.org/iso27001/ControlA.8.15"/>
        <terms:contributor>Jenni Parry</terms:contributor>
        <terms:created rdf:datatype="http://www.w3.org/2001/XMLSchema#date">2024-05-20</terms:created>
        <terms:subject rdf:resource="http://JP_ontology.org/nis2v/Article_21.2b"/>
        <rdfs:isDefinedBy rdf:resource="http://JP_ontology.org/assessment"/>
        <skos:altLabel xml:lang="en">MCQ.24</skos:altLabel>
        <skos:broader rdf:resource="http://JP_ontology.org/assessment/AssessmentQuestion"/>
        <skos:definition xml:lang="en">Are logs that record activities, exceptions, faults, and other relevant events produced, stored, protected, and analysed?</skos:definition>
        <skos:prefLabel xml:lang="en">Multiple Choice Question #24</skos:prefLabel>
    </rdf:Description>
    <rdf:Description rdf:about="http://JP_ontology.org/assessment/MCQ.25">
        <nis2v:hasAnswer rdf:resource="http://JP_ontology.org/assessment/MCQ.25AnswerA"/>
        <nis2v:hasAnswer rdf:resource="http://JP_ontology.org/assessment/MCQ.25AnswerB"/>
        <nis2v:hasAnswer rdf:resource="http://JP_ontology.org/assessment/MCQ.25AnswerC"/>
        <nis2v:relatedToControl rdf:resource="http://JP_ontology.org/iso27001/ControlA.8.16"/>
        <terms:contributor>Jenni Parry</terms:contributor>
        <terms:created rdf:datatype="http://www.w3.org/2001/XMLSchema#date">2024-05-20</terms:created>
        <terms:subject rdf:resource="http://JP_ontology.org/nis2v/Article_21.2b"/>
        <rdfs:isDefinedBy rdf:resource="http://JP_ontology.org/assessment"/>
        <skos:altLabel xml:lang="en">MCQ.25</skos:altLabel>
        <skos:broader rdf:resource="http://JP_ontology.org/assessment/AssessmentQuestion"/>
        <skos:definition xml:lang="en">Are networks, systems, and applications monitored for anomalous behaviour, and are appropriate actions taken to evaluate potential information security incidents?</skos:definition>
        <skos:prefLabel xml:lang="en">Multiple Choice Question #25</skos:prefLabel>
    </rdf:Description>
    <rdf:Description rdf:about="http://JP_ontology.org/assessment/MCQ.26">
        <nis2v:hasAnswer rdf:resource="http://JP_ontology.org/assessment/MCQ26AnswerA"/>
        <nis2v:hasAnswer rdf:resource="http://JP_ontology.org/assessment/MCQ26AnswerB"/>
        <nis2v:hasAnswer rdf:resource="http://JP_ontology.org/assessment/MCQ26AnswerC"/>
        <nis2v:relatedToControl rdf:resource="http://JP_ontology.org/iso27001/ControlA.8.17"/>
        <terms:contributor>Jenni Parry</terms:contributor>
        <terms:created rdf:datatype="http://www.w3.org/2001/XMLSchema#date">2024-04-18</terms:created>
        <terms:subject rdf:resource="http://JP_ontology.org/nis2v/Article_21.2b"/>
        <rdfs:isDefinedBy rdf:resource="http://JP_ontology.org/assessment"/>
        <skos:altLabel xml:lang="en">MCQ.26</skos:altLabel>
        <skos:broader rdf:resource="http://JP_ontology.org/assessment/AssessmentQuestion"/>
        <skos:definition xml:lang="en">Are the clocks of information processing systems used by the organisation synchronized to approved time sources?</skos:definition>
        <skos:prefLabel xml:lang="en">Multiple Choice Question #26</skos:prefLabel>
    </rdf:Description>
    <rdf:Description rdf:about="http://JP_ontology.org/assessment/MCQ.27">
        <nis2v:hasAnswer rdf:resource="http://JP_ontology.org/assessment/MCQ.27AnswerA"/>
        <nis2v:hasAnswer rdf:resource="http://JP_ontology.org/assessment/MCQ.27AnswerB"/>
        <nis2v:hasAnswer rdf:resource="http://JP_ontology.org/assessment/MCQ.27AnswerC"/>
        <nis2v:relatedToControl rdf:resource="http://JP_ontology.org/iso27001/ControlA.5.29"/>
        <terms:contributor>Jenni Parry</terms:contributor>
        <terms:created rdf:datatype="http://www.w3.org/2001/XMLSchema#date">2024-05-20</terms:created>
        <terms:subject rdf:resource="http://JP_ontology.org/nis2v/Article_21.2c"/>
        <rdfs:isDefinedBy rdf:resource="http://JP_ontology.org/assessment"/>
        <skos:altLabel xml:lang="en">MCQ.27</skos:altLabel>
        <skos:broader rdf:resource="http://JP_ontology.org/assessment/AssessmentQuestion"/>
        <skos:definition xml:lang="en">Does the organisation plan how to maintain information security at an appropriate level during disruption?</skos:definition>
        <skos:prefLabel xml:lang="en">Multiple Choice Question #27</skos:prefLabel>
    </rdf:Description>
    <rdf:Description rdf:about="http://JP_ontology.org/assessment/MCQ.28">
        <nis2v:hasAnswer rdf:resource="http://JP_ontology.org/assessment/MCQ.28AnswerA"/>
        <nis2v:hasAnswer rdf:resource="http://JP_ontology.org/assessment/MCQ.28AnswerB"/>
        <nis2v:hasAnswer rdf:resource="http://JP_ontology.org/assessment/MCQ.28AnswerC"/>
        <nis2v:relatedToControl rdf:resource="http://JP_ontology.org/iso27001/ControlA.5.30"/>
        <terms:contributor>Jenni Parry</terms:contributor>
        <terms:created rdf:datatype="http://www.w3.org/2001/XMLSchema#date">2024-05-20</terms:created>
        <terms:subject rdf:resource="http://JP_ontology.org/nis2v/Article_21.2c"/>
        <rdfs:isDefinedBy rdf:resource="http://JP_ontology.org/assessment"/>
        <skos:altLabel xml:lang="en">MCQ.28</skos:altLabel>
        <skos:broader rdf:resource="http://JP_ontology.org/assessment/AssessmentQuestion"/>
        <skos:definition xml:lang="en">Is ICT readiness planned, implemented, maintained, and tested based on business continuity objectives and ICT continuity requirements?</skos:definition>
        <skos:prefLabel xml:lang="en">Multiple Choice Question #28</skos:prefLabel>
    </rdf:Description>
    <rdf:Description rdf:about="http://JP_ontology.org/assessment/MCQ.29">
        <nis2v:hasAnswer rdf:resource="http://JP_ontology.org/assessment/MCQ29AnswerA"/>
        <nis2v:hasAnswer rdf:resource="http://JP_ontology.org/assessment/MCQ29AnswerB"/>
        <nis2v:hasAnswer rdf:resource="http://JP_ontology.org/assessment/MCQ29AnswerC"/>
        <nis2v:relatedToControl rdf:resource="http://JP_ontology.org/iso27001/ControlA.5.37"/>
        <terms:contributor>Jenni Parry</terms:contributor>
        <terms:created rdf:datatype="http://www.w3.org/2001/XMLSchema#date">2024-04-18</terms:created>
        <terms:subject rdf:resource="http://JP_ontology.org/nis2v/Article_21.2c"/>
        <rdfs:isDefinedBy rdf:resource="http://JP_ontology.org/assessment"/>
        <skos:altLabel xml:lang="en">MCQ.29</skos:altLabel>
        <skos:broader rdf:resource="http://JP_ontology.org/assessment/AssessmentQuestion"/>
        <skos:definition xml:lang="en">Are operating procedures for information processing facilities documented and made available to personnel who require them?</skos:definition>
        <skos:prefLabel xml:lang="en">Multiple Choice Question #29</skos:prefLabel>
    </rdf:Description>
    <rdf:Description rdf:about="http://JP_ontology.org/assessment/MCQ.3.1">
        <nis2v:hasAnswer rdf:resource="http://JP_ontology.org/assessment/MCQ.3.1AnswerA"/>
        <nis2v:hasAnswer rdf:resource="http://JP_ontology.org/assessment/MCQ.3.1AnswerB"/>
        <nis2v:hasAnswer rdf:resource="http://JP_ontology.org/assessment/MCQ.3.1AnswerC"/>
        <nis2v:relatedToControl rdf:resource="http://JP_ontology.org/iso27001/Control5.3"/>
        <terms:contributor>Jenni Parry</terms:contributor>
        <terms:created rdf:datatype="http://www.w3.org/2001/XMLSchema#date">2024-05-20</terms:created>
        <terms:subject rdf:resource="http://JP_ontology.org/nis2v/Article_21.2a"/>
        <rdfs:isDefinedBy rdf:resource="http://JP_ontology.org/assessment"/>
        <skos:altLabel xml:lang="en">MCQ.3.1</skos:altLabel>
        <skos:broader rdf:resource="http://JP_ontology.org/assessment/AssessmentQuestion"/>
        <skos:definition xml:lang="en">Does top management ensure that responsibilities and authorities for roles relevant to information security are assigned and communicated within the organisation? </skos:definition>
        <skos:prefLabel xml:lang="en">Multiple Choice Question #3.1</skos:prefLabel>
    </rdf:Description>
    <rdf:Description rdf:about="http://JP_ontology.org/assessment/MCQ.3.2">
        <nis2v:hasAnswer rdf:resource="http://JP_ontology.org/assessment/MCQ.3.2AnswerA"/>
        <nis2v:hasAnswer rdf:resource="http://JP_ontology.org/assessment/MCQ.3.2AnswerB"/>
        <nis2v:hasAnswer rdf:resource="http://JP_ontology.org/assessment/MCQ.3.2AnswerC"/>
        <nis2v:relatedToControl rdf:resource="http://JP_ontology.org/iso27001/Control5.3"/>
        <terms:contributor>Jenni Parry</terms:contributor>
        <terms:created rdf:datatype="http://www.w3.org/2001/XMLSchema#date">2024-05-20</terms:created>
        <terms:subject rdf:resource="http://JP_ontology.org/nis2v/Article_21.2a"/>
        <rdfs:isDefinedBy rdf:resource="http://JP_ontology.org/assessment"/>
        <skos:altLabel xml:lang="en">MCQ.3.2</skos:altLabel>
        <skos:broader rdf:resource="http://JP_ontology.org/assessment/AssessmentQuestion"/>
        <skos:definition xml:lang="en">Does top management assign the responsibility and authority for ensuring that the information security management system conforms to its requirements, as well as for reporting on the performance of the information security management system to top management?</skos:definition>
        <skos:prefLabel xml:lang="en">Multiple Choice Question #3.2</skos:prefLabel>
    </rdf:Description>
    <rdf:Description rdf:about="http://JP_ontology.org/assessment/MCQ.30">
        <nis2v:hasAnswer rdf:resource="http://JP_ontology.org/assessment/MCQ30AnswerA"/>
        <nis2v:hasAnswer rdf:resource="http://JP_ontology.org/assessment/MCQ30AnswerB"/>
        <nis2v:hasAnswer rdf:resource="http://JP_ontology.org/assessment/MCQ30AnswerC"/>
        <nis2v:relatedToControl rdf:resource="http://JP_ontology.org/iso27001/ControlA.7.11"/>
        <terms:contributor>Jenni Parry</terms:contributor>
        <terms:created rdf:datatype="http://www.w3.org/2001/XMLSchema#date">2024-04-18</terms:created>
        <terms:subject rdf:resource="http://JP_ontology.org/nis2v/Article_21.2c"/>
        <rdfs:isDefinedBy rdf:resource="http://JP_ontology.org/assessment"/>
        <skos:altLabel xml:lang="en">MCQ.30</skos:altLabel>
        <skos:broader rdf:resource="http://JP_ontology.org/assessment/AssessmentQuestion"/>
        <skos:definition xml:lang="en">Are information processing facilities protected from power failures and other disruptions caused by failures in supporting utilities?</skos:definition>
        <skos:prefLabel xml:lang="en">Multiple Choice Question #30</skos:prefLabel>
    </rdf:Description>
    <rdf:Description rdf:about="http://JP_ontology.org/assessment/MCQ.31">
        <nis2v:hasAnswer rdf:resource="http://JP_ontology.org/assessment/MCQ.31AnswerA"/>
        <nis2v:hasAnswer rdf:resource="http://JP_ontology.org/assessment/MCQ.31AnswerB"/>
        <nis2v:hasAnswer rdf:resource="http://JP_ontology.org/assessment/MCQ.31AnswerC"/>
        <nis2v:relatedToControl rdf:resource="http://JP_ontology.org/iso27001/ControlA.8.6"/>
        <terms:contributor>Jenni Parry</terms:contributor>
        <terms:created rdf:datatype="http://www.w3.org/2001/XMLSchema#date">2024-05-20</terms:created>
        <terms:subject rdf:resource="http://JP_ontology.org/nis2v/Article_21.2c"/>
        <rdfs:isDefinedBy rdf:resource="http://JP_ontology.org/assessment"/>
        <skos:altLabel xml:lang="en">MCQ.31</skos:altLabel>
        <skos:broader rdf:resource="http://JP_ontology.org/assessment/AssessmentQuestion"/>
        <skos:definition xml:lang="en">Is the use of resources monitored and adjusted in line with current and expected capacity requirements?</skos:definition>
        <skos:prefLabel xml:lang="en">Multiple Choice Question #31</skos:prefLabel>
    </rdf:Description>
    <rdf:Description rdf:about="http://JP_ontology.org/assessment/MCQ.32">
        <nis2v:hasAnswer rdf:resource="http://JP_ontology.org/assessment/MCQ.32AnswerA"/>
        <nis2v:hasAnswer rdf:resource="http://JP_ontology.org/assessment/MCQ.32AnswerB"/>
        <nis2v:hasAnswer rdf:resource="http://JP_ontology.org/assessment/MCQ.32AnswerC"/>
        <nis2v:relatedToControl rdf:resource="http://JP_ontology.org/iso27001/ControlA.8.13"/>
        <terms:contributor>Jenni Parry</terms:contributor>
        <terms:created rdf:datatype="http://www.w3.org/2001/XMLSchema#date">2024-05-20</terms:created>
        <terms:subject rdf:resource="http://JP_ontology.org/nis2v/Article_21.2c"/>
        <rdfs:isDefinedBy rdf:resource="http://JP_ontology.org/assessment"/>
        <skos:altLabel xml:lang="en">MCQ.32</skos:altLabel>
        <skos:broader rdf:resource="http://JP_ontology.org/assessment/AssessmentQuestion"/>
        <skos:definition xml:lang="en">Are backup copies of information, software, and systems maintained and regularly tested in accordance with the agreed topic-specific policy on backup?</skos:definition>
        <skos:prefLabel xml:lang="en">Multiple Choice Question #32</skos:prefLabel>
    </rdf:Description>
    <rdf:Description rdf:about="http://JP_ontology.org/assessment/MCQ.33">
        <nis2v:hasAnswer rdf:resource="http://JP_ontology.org/assessment/MCQ33AnswerA"/>
        <nis2v:hasAnswer rdf:resource="http://JP_ontology.org/assessment/MCQ33AnswerB"/>
        <nis2v:hasAnswer rdf:resource="http://JP_ontology.org/assessment/MCQ33AnswerC"/>
        <nis2v:relatedToControl rdf:resource="http://JP_ontology.org/iso27001/ControlA.8.14"/>
        <terms:contributor>Jenni Parry</terms:contributor>
        <terms:created rdf:datatype="http://www.w3.org/2001/XMLSchema#date">2024-04-18</terms:created>
        <terms:subject rdf:resource="http://JP_ontology.org/nis2v/Article_21.2c"/>
        <rdfs:isDefinedBy rdf:resource="http://JP_ontology.org/assessment"/>
        <skos:altLabel xml:lang="en">MCQ.33</skos:altLabel>
        <skos:broader rdf:resource="http://JP_ontology.org/assessment/AssessmentQuestion"/>
        <skos:definition xml:lang="en">Are information processing facilities implemented with redundancy sufficient to meet availability requirements?</skos:definition>
        <skos:prefLabel xml:lang="en">Multiple Choice Question #33</skos:prefLabel>
    </rdf:Description>
    <rdf:Description rdf:about="http://JP_ontology.org/assessment/MCQ.34.1">
        <nis2v:hasAnswer rdf:resource="http://JP_ontology.org/assessment/MCQ.34.1AnswerA"/>
        <nis2v:hasAnswer rdf:resource="http://JP_ontology.org/assessment/MCQ.34.1AnswerB"/>
        <nis2v:hasAnswer rdf:resource="http://JP_ontology.org/assessment/MCQ.34.1AnswerC"/>
        <nis2v:relatedToControl rdf:resource="http://JP_ontology.org/iso27001/Control8.1"/>
        <terms:contributor>Jenni Parry</terms:contributor>
        <terms:created rdf:datatype="http://www.w3.org/2001/XMLSchema#date">2024-05-20</terms:created>
        <terms:subject rdf:resource="http://JP_ontology.org/nis2v/Article_21.2d"/>
        <rdfs:isDefinedBy rdf:resource="http://JP_ontology.org/assessment"/>
        <skos:altLabel xml:lang="en">MCQ.34.1</skos:altLabel>
        <skos:broader rdf:resource="http://JP_ontology.org/assessment/AssessmentQuestion"/>
        <skos:definition xml:lang="en">Is the organisation planning, implementing, and controlling processes to meet requirements and implement actions by establishing criteria for the processes and implementing control in accordance with the established criteria?</skos:definition>
        <skos:prefLabel xml:lang="en">Multiple Choice Question #34.1</skos:prefLabel>
    </rdf:Description>
    <rdf:Description rdf:about="http://JP_ontology.org/assessment/MCQ.34.2">
        <nis2v:hasAnswer rdf:resource="http://JP_ontology.org/assessment/MCQ.34.2AnswerA"/>
        <nis2v:hasAnswer rdf:resource="http://JP_ontology.org/assessment/MCQ.34.2AnswerB"/>
        <nis2v:hasAnswer rdf:resource="http://JP_ontology.org/assessment/MCQ.34.2AnswerC"/>
        <nis2v:relatedToControl rdf:resource="http://JP_ontology.org/iso27001/Control8.1"/>
        <terms:contributor>Jenni Parry</terms:contributor>
        <terms:created rdf:datatype="http://www.w3.org/2001/XMLSchema#date">2024-05-20</terms:created>
        <terms:subject rdf:resource="http://JP_ontology.org/nis2v/Article_21.2d"/>
        <rdfs:isDefinedBy rdf:resource="http://JP_ontology.org/assessment"/>
        <skos:altLabel xml:lang="en">MCQ.34.2</skos:altLabel>
        <skos:broader rdf:resource="http://JP_ontology.org/assessment/AssessmentQuestion"/>
        <skos:definition xml:lang="en">Is documented information available to the extent necessary to have confidence that the processes have been carried out as planned?</skos:definition>
        <skos:prefLabel xml:lang="en">Multiple Choice Question #34.2</skos:prefLabel>
    </rdf:Description>
    <rdf:Description rdf:about="http://JP_ontology.org/assessment/MCQ.34.3">
        <nis2v:hasAnswer rdf:resource="http://JP_ontology.org/assessment/MCQ.34.3AnswerA"/>
        <nis2v:hasAnswer rdf:resource="http://JP_ontology.org/assessment/MCQ.34.3AnswerB"/>
        <nis2v:hasAnswer rdf:resource="http://JP_ontology.org/assessment/MCQ.34.3AnswerC"/>
        <nis2v:relatedToControl rdf:resource="http://JP_ontology.org/iso27001/Control8.1"/>
        <terms:contributor>Jenni Parry</terms:contributor>
        <terms:created rdf:datatype="http://www.w3.org/2001/XMLSchema#date">2024-05-20</terms:created>
        <terms:subject rdf:resource="http://JP_ontology.org/nis2v/Article_21.2d"/>
        <rdfs:isDefinedBy rdf:resource="http://JP_ontology.org/assessment"/>
        <skos:altLabel xml:lang="en">MCQ.34.3</skos:altLabel>
        <skos:broader rdf:resource="http://JP_ontology.org/assessment/AssessmentQuestion"/>
        <skos:definition xml:lang="en">Does the organisation control planned changes and review the consequences of unintended changes, taking action to mitigate any adverse effects as necessary?</skos:definition>
        <skos:prefLabel xml:lang="en">Multiple Choice Question #34.3</skos:prefLabel>
    </rdf:Description>
    <rdf:Description rdf:about="http://JP_ontology.org/assessment/MCQ.34.4">
        <nis2v:hasAnswer rdf:resource="http://JP_ontology.org/assessment/MCQ.34.4AnswerA"/>
        <nis2v:hasAnswer rdf:resource="http://JP_ontology.org/assessment/MCQ.34.4AnswerB"/>
        <nis2v:hasAnswer rdf:resource="http://JP_ontology.org/assessment/MCQ.34.4AnswerC"/>
        <nis2v:relatedToControl rdf:resource="http://JP_ontology.org/iso27001/Control8.1"/>
        <terms:contributor>Jenni Parry</terms:contributor>
        <terms:created rdf:datatype="http://www.w3.org/2001/XMLSchema#date">2024-05-20</terms:created>
        <terms:subject rdf:resource="http://JP_ontology.org/nis2v/Article_21.2d"/>
        <rdfs:isDefinedBy rdf:resource="http://JP_ontology.org/assessment"/>
        <skos:altLabel xml:lang="en">MCQ.34.4</skos:altLabel>
        <skos:broader rdf:resource="http://JP_ontology.org/assessment/AssessmentQuestion"/>
        <skos:definition xml:lang="en">Does the organisation ensure that externally provided processes, products, or services relevant to the information security management system are controlled?</skos:definition>
        <skos:prefLabel xml:lang="en">Multiple Choice Question #34.4</skos:prefLabel>
    </rdf:Description>
    <rdf:Description rdf:about="http://JP_ontology.org/assessment/MCQ.35">
        <nis2v:hasAnswer rdf:resource="http://JP_ontology.org/assessment/MCQ.35AnswerA"/>
        <nis2v:hasAnswer rdf:resource="http://JP_ontology.org/assessment/MCQ.35AnswerB"/>
        <nis2v:hasAnswer rdf:resource="http://JP_ontology.org/assessment/MCQ.35AnswerC"/>
        <nis2v:relatedToControl rdf:resource="http://JP_ontology.org/iso27001/ControlA.5.8"/>
        <terms:contributor>Jenni Parry</terms:contributor>
        <terms:created rdf:datatype="http://www.w3.org/2001/XMLSchema#date">2024-05-20</terms:created>
        <terms:subject rdf:resource="http://JP_ontology.org/nis2v/Article_21.2d"/>
        <rdfs:isDefinedBy rdf:resource="http://JP_ontology.org/assessment"/>
        <skos:altLabel xml:lang="en">MCQ.35</skos:altLabel>
        <skos:broader rdf:resource="http://JP_ontology.org/assessment/AssessmentQuestion"/>
        <skos:definition xml:lang="en">Is information security integrated into project management?</skos:definition>
        <skos:prefLabel xml:lang="en">Multiple Choice Question #35</skos:prefLabel>
    </rdf:Description>
    <rdf:Description rdf:about="http://JP_ontology.org/assessment/MCQ.36">
        <nis2v:hasAnswer rdf:resource="http://JP_ontology.org/assessment/MCQ.36AnswerA"/>
        <nis2v:hasAnswer rdf:resource="http://JP_ontology.org/assessment/MCQ.36AnswerB"/>
        <nis2v:hasAnswer rdf:resource="http://JP_ontology.org/assessment/MCQ.36AnswerC"/>
        <nis2v:relatedToControl rdf:resource="http://JP_ontology.org/iso27001/ControlA.5.19"/>
        <terms:contributor>Jenni Parry</terms:contributor>
        <terms:created rdf:datatype="http://www.w3.org/2001/XMLSchema#date">2024-05-20</terms:created>
        <terms:subject rdf:resource="http://JP_ontology.org/nis2v/Article_21.2d"/>
        <rdfs:isDefinedBy rdf:resource="http://JP_ontology.org/assessment"/>
        <skos:altLabel xml:lang="en">MCQ.36</skos:altLabel>
        <skos:broader rdf:resource="http://JP_ontology.org/assessment/AssessmentQuestion"/>
        <skos:definition xml:lang="en">Are processes and procedures defined and implemented to manage the information security risks associated with the use of supplier’s products or services?</skos:definition>
        <skos:prefLabel xml:lang="en">Multiple Choice Question #36</skos:prefLabel>
    </rdf:Description>
    <rdf:Description rdf:about="http://JP_ontology.org/assessment/MCQ.37">
        <nis2v:hasAnswer rdf:resource="http://JP_ontology.org/assessment/MCQ.37AnswerA"/>
        <nis2v:hasAnswer rdf:resource="http://JP_ontology.org/assessment/MCQ.37AnswerB"/>
        <nis2v:hasAnswer rdf:resource="http://JP_ontology.org/assessment/MCQ.37AnswerC"/>
        <nis2v:relatedToControl rdf:resource="http://JP_ontology.org/iso27001/ControlA.5.20"/>
        <terms:contributor>Jenni Parry</terms:contributor>
        <terms:created rdf:datatype="http://www.w3.org/2001/XMLSchema#date">2024-05-20</terms:created>
        <terms:subject rdf:resource="http://JP_ontology.org/nis2v/Article_21.2d"/>
        <rdfs:isDefinedBy rdf:resource="http://JP_ontology.org/assessment"/>
        <skos:altLabel xml:lang="en">MCQ.37</skos:altLabel>
        <skos:broader rdf:resource="http://JP_ontology.org/assessment/AssessmentQuestion"/>
        <skos:definition xml:lang="en">Are relevant information security requirements established and agreed upon with each supplier based on the type of supplier relationship?</skos:definition>
        <skos:prefLabel xml:lang="en">Multiple Choice Question #37</skos:prefLabel>
    </rdf:Description>
    <rdf:Description rdf:about="http://JP_ontology.org/assessment/MCQ.38">
        <nis2v:hasAnswer rdf:resource="http://JP_ontology.org/assessment/MCQ.38AnswerA"/>
        <nis2v:hasAnswer rdf:resource="http://JP_ontology.org/assessment/MCQ.38AnswerB"/>
        <nis2v:hasAnswer rdf:resource="http://JP_ontology.org/assessment/MCQ.38AnswerC"/>
        <nis2v:relatedToControl rdf:resource="http://JP_ontology.org/iso27001/ControlA.5.21"/>
        <terms:contributor>Jenni Parry</terms:contributor>
        <terms:created rdf:datatype="http://www.w3.org/2001/XMLSchema#date">2024-05-20</terms:created>
        <terms:subject rdf:resource="http://JP_ontology.org/nis2v/Article_21.2d"/>
        <rdfs:isDefinedBy rdf:resource="http://JP_ontology.org/assessment"/>
        <skos:altLabel xml:lang="en">MCQ.38</skos:altLabel>
        <skos:broader rdf:resource="http://JP_ontology.org/assessment/AssessmentQuestion"/>
        <skos:definition xml:lang="en">Are processes and procedures defined and implemented to manage the information security risks associated with the ICT products and services supply chain?</skos:definition>
        <skos:prefLabel xml:lang="en">Multiple Choice Question #38</skos:prefLabel>
    </rdf:Description>
    <rdf:Description rdf:about="http://JP_ontology.org/assessment/MCQ.39">
        <nis2v:hasAnswer rdf:resource="http://JP_ontology.org/assessment/MCQ.39AnswerA"/>
        <nis2v:hasAnswer rdf:resource="http://JP_ontology.org/assessment/MCQ.39AnswerB"/>
        <nis2v:hasAnswer rdf:resource="http://JP_ontology.org/assessment/MCQ.39AnswerC"/>
        <nis2v:relatedToControl rdf:resource="http://JP_ontology.org/iso27001/ControlA.5.22"/>
        <terms:contributor>Jenni Parry</terms:contributor>
        <terms:created rdf:datatype="http://www.w3.org/2001/XMLSchema#date">2024-05-20</terms:created>
        <terms:subject rdf:resource="http://JP_ontology.org/nis2v/Article_21.2d"/>
        <rdfs:isDefinedBy rdf:resource="http://JP_ontology.org/assessment"/>
        <skos:altLabel xml:lang="en">MCQ.39</skos:altLabel>
        <skos:broader rdf:resource="http://JP_ontology.org/assessment/AssessmentQuestion"/>
        <skos:definition xml:lang="en">Is the organisation regularly monitoring, reviewing, evaluating, and managing change in supplier information security practices and service delivery?</skos:definition>
        <skos:prefLabel xml:lang="en">Multiple Choice Question #39</skos:prefLabel>
    </rdf:Description>
    <rdf:Description rdf:about="http://JP_ontology.org/assessment/MCQ.4.1">
        <nis2v:hasAnswer rdf:resource="http://JP_ontology.org/assessment/MCQ.4.1AnswerA"/>
        <nis2v:hasAnswer rdf:resource="http://JP_ontology.org/assessment/MCQ.4.1AnswerB"/>
        <nis2v:hasAnswer rdf:resource="http://JP_ontology.org/assessment/MCQ.4.1AnswerC"/>
        <nis2v:relatedToControl rdf:resource="http://JP_ontology.org/iso27001/Control6.1.2"/>
        <terms:contributor>Jenni Parry</terms:contributor>
        <terms:created rdf:datatype="http://www.w3.org/2001/XMLSchema#date">2024-05-20</terms:created>
        <terms:subject rdf:resource="http://JP_ontology.org/nis2v/Article_21.2a"/>
        <rdfs:isDefinedBy rdf:resource="http://JP_ontology.org/assessment"/>
        <skos:altLabel xml:lang="en">MCQ.4.1</skos:altLabel>
        <skos:broader rdf:resource="http://JP_ontology.org/assessment/AssessmentQuestion"/>
        <skos:definition xml:lang="en">Does the organisation establish and maintain information security risk criteria, including risk acceptance criteria and criteria for performing information security risk assessments?</skos:definition>
        <skos:prefLabel xml:lang="en">Multiple Choice Question #4.1</skos:prefLabel>
    </rdf:Description>
    <rdf:Description rdf:about="http://JP_ontology.org/assessment/MCQ.4.2">
        <nis2v:hasAnswer rdf:resource="http://JP_ontology.org/assessment/MCQ.4.2AnswerA"/>
        <nis2v:hasAnswer rdf:resource="http://JP_ontology.org/assessment/MCQ.4.2AnswerB"/>
        <nis2v:hasAnswer rdf:resource="http://JP_ontology.org/assessment/MCQ.4.2AnswerC"/>
        <nis2v:relatedToControl rdf:resource="http://JP_ontology.org/iso27001/Control6.1.2"/>
        <terms:contributor>Jenni Parry</terms:contributor>
        <terms:created rdf:datatype="http://www.w3.org/2001/XMLSchema#date">2024-05-20</terms:created>
        <terms:subject rdf:resource="http://JP_ontology.org/nis2v/Article_21.2a"/>
        <rdfs:isDefinedBy rdf:resource="http://JP_ontology.org/assessment"/>
        <skos:altLabel xml:lang="en">MCQ.4.2</skos:altLabel>
        <skos:broader rdf:resource="http://JP_ontology.org/assessment/AssessmentQuestion"/>
        <skos:definition xml:lang="en">Does the organisation ensure that repeated information security risk assessments produce consistent, valid, and comparable results?</skos:definition>
        <skos:prefLabel xml:lang="en">Multiple Choice Question #4.2</skos:prefLabel>
    </rdf:Description>
    <rdf:Description rdf:about="http://JP_ontology.org/assessment/MCQ.4.3">
        <nis2v:hasAnswer rdf:resource="http://JP_ontology.org/assessment/MCQ.4.3AnswerA"/>
        <nis2v:hasAnswer rdf:resource="http://JP_ontology.org/assessment/MCQ.4.3AnswerB"/>
        <nis2v:hasAnswer rdf:resource="http://JP_ontology.org/assessment/MCQ.4.3AnswerC"/>
        <nis2v:relatedToControl rdf:resource="http://JP_ontology.org/iso27001/Control6.1.2"/>
        <terms:contributor>Jenni Parry</terms:contributor>
        <terms:created rdf:datatype="http://www.w3.org/2001/XMLSchema#date">2024-05-20</terms:created>
        <terms:subject rdf:resource="http://JP_ontology.org/nis2v/Article_21.2a"/>
        <rdfs:isDefinedBy rdf:resource="http://JP_ontology.org/assessment"/>
        <skos:altLabel xml:lang="en">MCQ.4.3</skos:altLabel>
        <skos:broader rdf:resource="http://JP_ontology.org/assessment/AssessmentQuestion"/>
        <skos:definition xml:lang="en">Does the organisation identify information security risks, including applying the information security risk assessment process to identify risks associated with the loss of confidentiality, integrity, and availability for information within the scope of the information security management system, as well as identifying the risk owners?</skos:definition>
        <skos:prefLabel xml:lang="en">Multiple Choice Question #4.3</skos:prefLabel>
    </rdf:Description>
    <rdf:Description rdf:about="http://JP_ontology.org/assessment/MCQ.4.4">
        <nis2v:hasAnswer rdf:resource="http://JP_ontology.org/assessment/MCQ.4.4AnswerA"/>
        <nis2v:hasAnswer rdf:resource="http://JP_ontology.org/assessment/MCQ.4.4AnswerB"/>
        <nis2v:hasAnswer rdf:resource="http://JP_ontology.org/assessment/MCQ.4.4AnswerC"/>
        <nis2v:relatedToControl rdf:resource="http://JP_ontology.org/iso27001/Control6.1.2"/>
        <terms:contributor>Jenni Parry</terms:contributor>
        <terms:created rdf:datatype="http://www.w3.org/2001/XMLSchema#date">2024-05-20</terms:created>
        <terms:subject rdf:resource="http://JP_ontology.org/nis2v/Article_21.2a"/>
        <rdfs:isDefinedBy rdf:resource="http://JP_ontology.org/assessment"/>
        <skos:altLabel xml:lang="en">MCQ.4.4</skos:altLabel>
        <skos:broader rdf:resource="http://JP_ontology.org/assessment/AssessmentQuestion"/>
        <skos:definition xml:lang="en">Does the organisation analyse information security risks, which involves assessing the potential consequences and realistic likelihood of the occurrence of identified risks, as well as determining the levels of risk?</skos:definition>
        <skos:prefLabel xml:lang="en">Multiple Choice Question #4.4</skos:prefLabel>
    </rdf:Description>
    <rdf:Description rdf:about="http://JP_ontology.org/assessment/MCQ.4.5">
        <nis2v:hasAnswer rdf:resource="http://JP_ontology.org/assessment/MCQ.4.5AnswerA"/>
        <nis2v:hasAnswer rdf:resource="http://JP_ontology.org/assessment/MCQ.4.5AnswerB"/>
        <nis2v:hasAnswer rdf:resource="http://JP_ontology.org/assessment/MCQ.4.5AnswerC"/>
        <nis2v:relatedToControl rdf:resource="http://JP_ontology.org/iso27001/Control6.1.2"/>
        <terms:contributor>Jenni Parry</terms:contributor>
        <terms:created rdf:datatype="http://www.w3.org/2001/XMLSchema#date">2024-05-20</terms:created>
        <terms:subject rdf:resource="http://JP_ontology.org/nis2v/Article_21.2a"/>
        <rdfs:isDefinedBy rdf:resource="http://JP_ontology.org/assessment"/>
        <skos:altLabel xml:lang="en">MCQ.4.5</skos:altLabel>
        <skos:broader rdf:resource="http://JP_ontology.org/assessment/AssessmentQuestion"/>
        <skos:definition xml:lang="en">Does the organisation evaluate information security risks, including comparing the results of risk analysis with established risk criteria and prioritizing the analysed risks for risk treatment?</skos:definition>
        <skos:prefLabel xml:lang="en">Multiple Choice Question #4.5</skos:prefLabel>
    </rdf:Description>
    <rdf:Description rdf:about="http://JP_ontology.org/assessment/MCQ.4.6">
        <nis2v:hasAnswer rdf:resource="http://JP_ontology.org/assessment/MCQ.4.6AnswerA"/>
        <nis2v:hasAnswer rdf:resource="http://JP_ontology.org/assessment/MCQ.4.6AnswerB"/>
        <nis2v:hasAnswer rdf:resource="http://JP_ontology.org/assessment/MCQ.4.6AnswerC"/>
        <nis2v:relatedToControl rdf:resource="http://JP_ontology.org/iso27001/Control6.1.2"/>
        <terms:contributor>Jenni Parry</terms:contributor>
        <terms:created rdf:datatype="http://www.w3.org/2001/XMLSchema#date">2024-05-20</terms:created>
        <terms:subject rdf:resource="http://JP_ontology.org/nis2v/Article_21.2a"/>
        <rdfs:isDefinedBy rdf:resource="http://JP_ontology.org/assessment"/>
        <skos:altLabel xml:lang="en">MCQ.4.6</skos:altLabel>
        <skos:broader rdf:resource="http://JP_ontology.org/assessment/AssessmentQuestion"/>
        <skos:definition xml:lang="en">Does the organisation retain documented information about the information security risk assessment process?</skos:definition>
        <skos:prefLabel xml:lang="en">Multiple Choice Question #4.6</skos:prefLabel>
    </rdf:Description>
    <rdf:Description rdf:about="http://JP_ontology.org/assessment/MCQ.40">
        <nis2v:hasAnswer rdf:resource="http://JP_ontology.org/assessment/MCQ.40AnswerA"/>
        <nis2v:hasAnswer rdf:resource="http://JP_ontology.org/assessment/MCQ.40AnswerB"/>
        <nis2v:hasAnswer rdf:resource="http://JP_ontology.org/assessment/MCQ.40AnswerC"/>
        <nis2v:relatedToControl rdf:resource="http://JP_ontology.org/iso27001/ControlA.5.23"/>
        <terms:contributor>Jenni Parry</terms:contributor>
        <terms:created rdf:datatype="http://www.w3.org/2001/XMLSchema#date">2024-05-20</terms:created>
        <terms:subject rdf:resource="http://JP_ontology.org/nis2v/Article_21.2d"/>
        <rdfs:isDefinedBy rdf:resource="http://JP_ontology.org/assessment"/>
        <skos:altLabel xml:lang="en">MCQ.40</skos:altLabel>
        <skos:broader rdf:resource="http://JP_ontology.org/assessment/AssessmentQuestion"/>
        <skos:definition xml:lang="en">Are processes established for the acquisition, use, management, and exit from cloud services in accordance with the organisation’s information security requirements?</skos:definition>
        <skos:prefLabel xml:lang="en">Multiple Choice Question #40</skos:prefLabel>
    </rdf:Description>
    <rdf:Description rdf:about="http://JP_ontology.org/assessment/MCQ.41">
        <nis2v:hasAnswer rdf:resource="http://JP_ontology.org/assessment/MCQ41AnswerA"/>
        <nis2v:hasAnswer rdf:resource="http://JP_ontology.org/assessment/MCQ41AnswerB"/>
        <nis2v:hasAnswer rdf:resource="http://JP_ontology.org/assessment/MCQ41AnswerC"/>
        <nis2v:relatedToControl rdf:resource="http://JP_ontology.org/iso27001/ControlA.5.37"/>
        <terms:contributor>Jenni Parry</terms:contributor>
        <terms:created rdf:datatype="http://www.w3.org/2001/XMLSchema#date">2024-04-18</terms:created>
        <terms:subject rdf:resource="http://JP_ontology.org/nis2v/Article_21.2e"/>
        <rdfs:isDefinedBy rdf:resource="http://JP_ontology.org/assessment"/>
        <skos:altLabel xml:lang="en">MCQ.41</skos:altLabel>
        <skos:broader rdf:resource="http://JP_ontology.org/assessment/AssessmentQuestion"/>
        <skos:definition xml:lang="en">Are operating procedures for information processing facilities documented and made available to personnel who require them?</skos:definition>
        <skos:prefLabel xml:lang="en">Multiple Choice Question #41</skos:prefLabel>
    </rdf:Description>
    <rdf:Description rdf:about="http://JP_ontology.org/assessment/MCQ.42">
        <nis2v:hasAnswer rdf:resource="http://JP_ontology.org/assessment/MCQ.42AnswerA"/>
        <nis2v:hasAnswer rdf:resource="http://JP_ontology.org/assessment/MCQ.42AnswerB"/>
        <nis2v:hasAnswer rdf:resource="http://JP_ontology.org/assessment/MCQ.42AnswerC"/>
        <nis2v:relatedToControl rdf:resource="http://JP_ontology.org/iso27001/ControlA.8.8"/>
        <terms:contributor>Jenni Parry</terms:contributor>
        <terms:created rdf:datatype="http://www.w3.org/2001/XMLSchema#date">2024-05-20</terms:created>
        <terms:subject rdf:resource="http://JP_ontology.org/nis2v/Article_21.2e"/>
        <rdfs:isDefinedBy rdf:resource="http://JP_ontology.org/assessment"/>
        <skos:altLabel xml:lang="en">MCQ.42</skos:altLabel>
        <skos:broader rdf:resource="http://JP_ontology.org/assessment/AssessmentQuestion"/>
        <skos:definition xml:lang="en">Does the organisation acquire information regarding technical vulnerabilities of the information systems in use, evaluate the organisation’s exposure to such vulnerabilities, and implement appropriate measures accordingly?</skos:definition>
        <skos:prefLabel xml:lang="en">Multiple Choice Question #42</skos:prefLabel>
    </rdf:Description>
    <rdf:Description rdf:about="http://JP_ontology.org/assessment/MCQ.43">
        <nis2v:hasAnswer rdf:resource="http://JP_ontology.org/assessment/MCQ.43AnswerA"/>
        <nis2v:hasAnswer rdf:resource="http://JP_ontology.org/assessment/MCQ.43AnswerB"/>
        <nis2v:hasAnswer rdf:resource="http://JP_ontology.org/assessment/MCQ.43AnswerC"/>
        <nis2v:relatedToControl rdf:resource="http://JP_ontology.org/iso27001/ControlA.8.9"/>
        <terms:contributor>Jenni Parry</terms:contributor>
        <terms:created rdf:datatype="http://www.w3.org/2001/XMLSchema#date">2024-05-20</terms:created>
        <terms:subject rdf:resource="http://JP_ontology.org/nis2v/Article_21.2e"/>
        <rdfs:isDefinedBy rdf:resource="http://JP_ontology.org/assessment"/>
        <skos:altLabel xml:lang="en">MCQ.43</skos:altLabel>
        <skos:broader rdf:resource="http://JP_ontology.org/assessment/AssessmentQuestion"/>
        <skos:definition xml:lang="en">Are configurations, including security configurations, of hardware, software, services, and networks established, documented, implemented, monitored, and reviewed?</skos:definition>
        <skos:prefLabel xml:lang="en">Multiple Choice Question #43</skos:prefLabel>
    </rdf:Description>
    <rdf:Description rdf:about="http://JP_ontology.org/assessment/MCQ.44">
        <nis2v:hasAnswer rdf:resource="http://JP_ontology.org/assessment/MCQ.44AnswerA"/>
        <nis2v:hasAnswer rdf:resource="http://JP_ontology.org/assessment/MCQ.44AnswerB"/>
        <nis2v:hasAnswer rdf:resource="http://JP_ontology.org/assessment/MCQ.44AnswerC"/>
        <nis2v:relatedToControl rdf:resource="http://JP_ontology.org/iso27001/ControlA.8.19"/>
        <terms:contributor>Jenni Parry</terms:contributor>
        <terms:created rdf:datatype="http://www.w3.org/2001/XMLSchema#date">2024-05-20</terms:created>
        <terms:subject rdf:resource="http://JP_ontology.org/nis2v/Article_21.2e"/>
        <rdfs:isDefinedBy rdf:resource="http://JP_ontology.org/assessment"/>
        <skos:altLabel xml:lang="en">MCQ.44</skos:altLabel>
        <skos:broader rdf:resource="http://JP_ontology.org/assessment/AssessmentQuestion"/>
        <skos:definition xml:lang="en">Have procedures and measures been implemented to securely manage software installation on operational systems?</skos:definition>
        <skos:prefLabel xml:lang="en">Multiple Choice Question #44</skos:prefLabel>
    </rdf:Description>
    <rdf:Description rdf:about="http://JP_ontology.org/assessment/MCQ.45">
        <nis2v:hasAnswer rdf:resource="http://JP_ontology.org/assessment/MCQ.45AnswerA"/>
        <nis2v:hasAnswer rdf:resource="http://JP_ontology.org/assessment/MCQ.45AnswerB"/>
        <nis2v:hasAnswer rdf:resource="http://JP_ontology.org/assessment/MCQ.45AnswerC"/>
        <nis2v:relatedToControl rdf:resource="http://JP_ontology.org/iso27001/ControlA.8.20"/>
        <terms:contributor>Jenni Parry</terms:contributor>
        <terms:created rdf:datatype="http://www.w3.org/2001/XMLSchema#date">2024-05-20</terms:created>
        <terms:subject rdf:resource="http://JP_ontology.org/nis2v/Article_21.2e"/>
        <rdfs:isDefinedBy rdf:resource="http://JP_ontology.org/assessment"/>
        <skos:altLabel xml:lang="en">MCQ.45</skos:altLabel>
        <skos:broader rdf:resource="http://JP_ontology.org/assessment/AssessmentQuestion"/>
        <skos:definition xml:lang="en">Are networks and network devices secured, managed, and controlled to protect information in systems and applications?</skos:definition>
        <skos:prefLabel xml:lang="en">Multiple Choice Question #45</skos:prefLabel>
    </rdf:Description>
    <rdf:Description rdf:about="http://JP_ontology.org/assessment/MCQ.46">
        <nis2v:hasAnswer rdf:resource="http://JP_ontology.org/assessment/MCQ.46AnswerA"/>
        <nis2v:hasAnswer rdf:resource="http://JP_ontology.org/assessment/MCQ.46AnswerB"/>
        <nis2v:hasAnswer rdf:resource="http://JP_ontology.org/assessment/MCQ.46AnswerC"/>
        <nis2v:relatedToControl rdf:resource="http://JP_ontology.org/iso27001/ControlA.8.21"/>
        <terms:contributor>Jenni Parry</terms:contributor>
        <terms:created rdf:datatype="http://www.w3.org/2001/XMLSchema#date">2024-05-20</terms:created>
        <terms:subject rdf:resource="http://JP_ontology.org/nis2v/Article_21.2e"/>
        <rdfs:isDefinedBy rdf:resource="http://JP_ontology.org/assessment"/>
        <skos:altLabel xml:lang="en">MCQ.46</skos:altLabel>
        <skos:broader rdf:resource="http://JP_ontology.org/assessment/AssessmentQuestion"/>
        <skos:definition xml:lang="en">Are security mechanisms, service levels, and service requirements of network services identified, implemented, and monitored?</skos:definition>
        <skos:prefLabel xml:lang="en">Multiple Choice Question #46</skos:prefLabel>
    </rdf:Description>
    <rdf:Description rdf:about="http://JP_ontology.org/assessment/MCQ.47">
        <nis2v:hasAnswer rdf:resource="http://JP_ontology.org/assessment/MCQ.47AnswerA"/>
        <nis2v:hasAnswer rdf:resource="http://JP_ontology.org/assessment/MCQ.47AnswerB"/>
        <nis2v:hasAnswer rdf:resource="http://JP_ontology.org/assessment/MCQ.47AnswerC"/>
        <nis2v:relatedToControl rdf:resource="http://JP_ontology.org/iso27001/ControlA.8.22"/>
        <terms:contributor>Jenni Parry</terms:contributor>
        <terms:created rdf:datatype="http://www.w3.org/2001/XMLSchema#date">2024-05-20</terms:created>
        <terms:subject rdf:resource="http://JP_ontology.org/nis2v/Article_21.2e"/>
        <rdfs:isDefinedBy rdf:resource="http://JP_ontology.org/assessment"/>
        <skos:altLabel xml:lang="en">MCQ.47</skos:altLabel>
        <skos:broader rdf:resource="http://JP_ontology.org/assessment/AssessmentQuestion"/>
        <skos:definition xml:lang="en">Is segregation implemented for groups of information services, users, and information systems within the organisation&apos;s networks?</skos:definition>
        <skos:prefLabel xml:lang="en">Multiple Choice Question #47</skos:prefLabel>
    </rdf:Description>
    <rdf:Description rdf:about="http://JP_ontology.org/assessment/MCQ.48">
        <nis2v:hasAnswer rdf:resource="http://JP_ontology.org/assessment/MCQ.48AnswerA"/>
        <nis2v:hasAnswer rdf:resource="http://JP_ontology.org/assessment/MCQ.48AnswerB"/>
        <nis2v:hasAnswer rdf:resource="http://JP_ontology.org/assessment/MCQ.48AnswerC"/>
        <nis2v:relatedToControl rdf:resource="http://JP_ontology.org/iso27001/ControlA.8.23"/>
        <terms:contributor>Jenni Parry</terms:contributor>
        <terms:created rdf:datatype="http://www.w3.org/2001/XMLSchema#date">2024-05-20</terms:created>
        <terms:subject rdf:resource="http://JP_ontology.org/nis2v/Article_21.2e"/>
        <rdfs:isDefinedBy rdf:resource="http://JP_ontology.org/assessment"/>
        <skos:altLabel xml:lang="en">MCQ.48</skos:altLabel>
        <skos:broader rdf:resource="http://JP_ontology.org/assessment/AssessmentQuestion"/>
        <skos:definition xml:lang="en">Is access to external websites managed to reduce exposure to malicious content?</skos:definition>
        <skos:prefLabel xml:lang="en">Multiple Choice Question #48</skos:prefLabel>
    </rdf:Description>
    <rdf:Description rdf:about="http://JP_ontology.org/assessment/MCQ.49.1">
        <nis2v:hasAnswer rdf:resource="http://JP_ontology.org/assessment/MCQ.49.1AnswerA"/>
        <nis2v:hasAnswer rdf:resource="http://JP_ontology.org/assessment/MCQ.49.1AnswerB"/>
        <nis2v:hasAnswer rdf:resource="http://JP_ontology.org/assessment/MCQ.49.1AnswerC"/>
        <nis2v:relatedToControl rdf:resource="http://JP_ontology.org/iso27001/Control9.1"/>
        <terms:contributor>Jenni Parry</terms:contributor>
        <terms:created rdf:datatype="http://www.w3.org/2001/XMLSchema#date">2024-05-20</terms:created>
        <terms:subject rdf:resource="http://JP_ontology.org/nis2v/Article_21.2f"/>
        <rdfs:isDefinedBy rdf:resource="http://JP_ontology.org/assessment"/>
        <skos:altLabel xml:lang="en">MCQ.49.1</skos:altLabel>
        <skos:broader rdf:resource="http://JP_ontology.org/assessment/AssessmentQuestion"/>
        <skos:definition xml:lang="en">Does the organisation determine what needs to be monitored and measured, including information security processes and controls?</skos:definition>
        <skos:prefLabel xml:lang="en">Multiple Choice Question #49.1</skos:prefLabel>
    </rdf:Description>
    <rdf:Description rdf:about="http://JP_ontology.org/assessment/MCQ.49.2">
        <nis2v:hasAnswer rdf:resource="http://JP_ontology.org/assessment/MCQ.49.2AnswerA"/>
        <nis2v:hasAnswer rdf:resource="http://JP_ontology.org/assessment/MCQ.49.2AnswerB"/>
        <nis2v:hasAnswer rdf:resource="http://JP_ontology.org/assessment/MCQ.49.2AnswerC"/>
        <nis2v:relatedToControl rdf:resource="http://JP_ontology.org/iso27001/Control9.1"/>
        <terms:contributor>Jenni Parry</terms:contributor>
        <terms:created rdf:datatype="http://www.w3.org/2001/XMLSchema#date">2024-05-20</terms:created>
        <terms:subject rdf:resource="http://JP_ontology.org/nis2v/Article_21.2f"/>
        <rdfs:isDefinedBy rdf:resource="http://JP_ontology.org/assessment"/>
        <skos:altLabel xml:lang="en">MCQ.49.2</skos:altLabel>
        <skos:broader rdf:resource="http://JP_ontology.org/assessment/AssessmentQuestion"/>
        <skos:definition xml:lang="en">Has the organisation established methods for monitoring, measurement, analysis, and evaluation to ensure valid results, and are these methods selected capable of producing comparable and reproducible results?</skos:definition>
        <skos:prefLabel xml:lang="en">Multiple Choice Question #49.2</skos:prefLabel>
    </rdf:Description>
    <rdf:Description rdf:about="http://JP_ontology.org/assessment/MCQ.49.3">
        <nis2v:hasAnswer rdf:resource="http://JP_ontology.org/assessment/MCQ.49.3AnswerA"/>
        <nis2v:hasAnswer rdf:resource="http://JP_ontology.org/assessment/MCQ.49.3AnswerB"/>
        <nis2v:hasAnswer rdf:resource="http://JP_ontology.org/assessment/MCQ.49.3AnswerC"/>
        <nis2v:relatedToControl rdf:resource="http://JP_ontology.org/iso27001/Control9.1"/>
        <terms:contributor>Jenni Parry</terms:contributor>
        <terms:created rdf:datatype="http://www.w3.org/2001/XMLSchema#date">2024-05-20</terms:created>
        <terms:subject rdf:resource="http://JP_ontology.org/nis2v/Article_21.2f"/>
        <rdfs:isDefinedBy rdf:resource="http://JP_ontology.org/assessment"/>
        <skos:altLabel xml:lang="en">MCQ.49.3</skos:altLabel>
        <skos:broader rdf:resource="http://JP_ontology.org/assessment/AssessmentQuestion"/>
        <skos:definition xml:lang="en">Does the organisation specify when monitoring and measuring shall be performed, who shall conduct it, and when the results shall be analysed and evaluated?</skos:definition>
        <skos:prefLabel xml:lang="en">Multiple Choice Question #49.3</skos:prefLabel>
    </rdf:Description>
    <rdf:Description rdf:about="http://JP_ontology.org/assessment/MCQ.5.1">
        <nis2v:hasAnswer rdf:resource="http://JP_ontology.org/assessment/MCQ.5.1AnswerA"/>
        <nis2v:hasAnswer rdf:resource="http://JP_ontology.org/assessment/MCQ.5.1AnswerB"/>
        <nis2v:hasAnswer rdf:resource="http://JP_ontology.org/assessment/MCQ.5.1AnswerC"/>
        <nis2v:relatedToControl rdf:resource="http://JP_ontology.org/iso27001/Control6.1.3"/>
        <terms:contributor>Jenni Parry</terms:contributor>
        <terms:created rdf:datatype="http://www.w3.org/2001/XMLSchema#date">2024-05-20</terms:created>
        <terms:subject rdf:resource="http://JP_ontology.org/nis2v/Article_21.2a"/>
        <rdfs:isDefinedBy rdf:resource="http://JP_ontology.org/assessment"/>
        <skos:altLabel xml:lang="en">MCQ.5.1</skos:altLabel>
        <skos:broader rdf:resource="http://JP_ontology.org/assessment/AssessmentQuestion"/>
        <skos:definition xml:lang="en">Does the organisation select appropriate information security risk treatment options, considering the results of the risk assessment?</skos:definition>
        <skos:prefLabel xml:lang="en">Multiple Choice Question #5.1</skos:prefLabel>
    </rdf:Description>
    <rdf:Description rdf:about="http://JP_ontology.org/assessment/MCQ.5.2">
        <nis2v:hasAnswer rdf:resource="http://JP_ontology.org/assessment/MCQ.5.2AnswerA"/>
        <nis2v:hasAnswer rdf:resource="http://JP_ontology.org/assessment/MCQ.5.2AnswerB"/>
        <nis2v:hasAnswer rdf:resource="http://JP_ontology.org/assessment/MCQ.5.2AnswerC"/>
        <nis2v:relatedToControl rdf:resource="http://JP_ontology.org/iso27001/Control6.1.3"/>
        <terms:contributor>Jenni Parry</terms:contributor>
        <terms:created rdf:datatype="http://www.w3.org/2001/XMLSchema#date">2024-05-20</terms:created>
        <terms:subject rdf:resource="http://JP_ontology.org/nis2v/Article_21.2a"/>
        <rdfs:isDefinedBy rdf:resource="http://JP_ontology.org/assessment"/>
        <skos:altLabel xml:lang="en">MCQ.5.2</skos:altLabel>
        <skos:broader rdf:resource="http://JP_ontology.org/assessment/AssessmentQuestion"/>
        <skos:definition xml:lang="en">Does the organisation determine all necessary controls to implement the chosen information security risk treatment option(s), whether by designing them as required or identifying them from any source?</skos:definition>
        <skos:prefLabel xml:lang="en">Multiple Choice Question #5.2</skos:prefLabel>
    </rdf:Description>
    <rdf:Description rdf:about="http://JP_ontology.org/assessment/MCQ.5.3">
        <nis2v:hasAnswer rdf:resource="http://JP_ontology.org/assessment/MCQ.5.3AnswerA"/>
        <nis2v:hasAnswer rdf:resource="http://JP_ontology.org/assessment/MCQ.5.3AnswerB"/>
        <nis2v:hasAnswer rdf:resource="http://JP_ontology.org/assessment/MCQ.5.3AnswerC"/>
        <nis2v:relatedToControl rdf:resource="http://JP_ontology.org/iso27001/Control6.1.3"/>
        <terms:contributor>Jenni Parry</terms:contributor>
        <terms:created rdf:datatype="http://www.w3.org/2001/XMLSchema#date">2024-05-20</terms:created>
        <terms:subject rdf:resource="http://JP_ontology.org/nis2v/Article_21.2a"/>
        <rdfs:isDefinedBy rdf:resource="http://JP_ontology.org/assessment"/>
        <skos:altLabel xml:lang="en">MCQ.5.3</skos:altLabel>
        <skos:broader rdf:resource="http://JP_ontology.org/assessment/AssessmentQuestion"/>
        <skos:definition xml:lang="en">Does the organisation produce a control of Applicability containing the necessary controls, justification for their inclusion, status of implementation, and reasoning for excluding any controls?</skos:definition>
        <skos:prefLabel xml:lang="en">Multiple Choice Question #5.3</skos:prefLabel>
    </rdf:Description>
    <rdf:Description rdf:about="http://JP_ontology.org/assessment/MCQ.5.4">
        <nis2v:hasAnswer rdf:resource="http://JP_ontology.org/assessment/MCQ.5.4AnswerA"/>
        <nis2v:hasAnswer rdf:resource="http://JP_ontology.org/assessment/MCQ.5.4AnswerB"/>
        <nis2v:hasAnswer rdf:resource="http://JP_ontology.org/assessment/MCQ.5.4AnswerC"/>
        <nis2v:relatedToControl rdf:resource="http://JP_ontology.org/iso27001/Control6.1.3"/>
        <terms:contributor>Jenni Parry</terms:contributor>
        <terms:created rdf:datatype="http://www.w3.org/2001/XMLSchema#date">2024-05-20</terms:created>
        <terms:subject rdf:resource="http://JP_ontology.org/nis2v/Article_21.2a"/>
        <rdfs:isDefinedBy rdf:resource="http://JP_ontology.org/assessment"/>
        <skos:altLabel xml:lang="en">MCQ.5.4</skos:altLabel>
        <skos:broader rdf:resource="http://JP_ontology.org/assessment/AssessmentQuestion"/>
        <skos:definition xml:lang="en">Does the organisation formulate an information security risk treatment plan?</skos:definition>
        <skos:prefLabel xml:lang="en">Multiple Choice Question #5.4</skos:prefLabel>
    </rdf:Description>
    <rdf:Description rdf:about="http://JP_ontology.org/assessment/MCQ.5.5">
        <nis2v:hasAnswer rdf:resource="http://JP_ontology.org/assessment/MCQ.5.5AnswerA"/>
        <nis2v:hasAnswer rdf:resource="http://JP_ontology.org/assessment/MCQ.5.5AnswerB"/>
        <nis2v:hasAnswer rdf:resource="http://JP_ontology.org/assessment/MCQ.5.5AnswerC"/>
        <nis2v:relatedToControl rdf:resource="http://JP_ontology.org/iso27001/Control6.1.3"/>
        <terms:contributor>Jenni Parry</terms:contributor>
        <terms:created rdf:datatype="http://www.w3.org/2001/XMLSchema#date">2024-05-20</terms:created>
        <terms:subject rdf:resource="http://JP_ontology.org/nis2v/Article_21.2a"/>
        <rdfs:isDefinedBy rdf:resource="http://JP_ontology.org/assessment"/>
        <skos:altLabel xml:lang="en">MCQ.5.5</skos:altLabel>
        <skos:broader rdf:resource="http://JP_ontology.org/assessment/AssessmentQuestion"/>
        <skos:definition xml:lang="en">Does the organisation obtain approval from risk owners for the information security risk treatment plan and acceptance of residual information security risks?</skos:definition>
        <skos:prefLabel xml:lang="en">Multiple Choice Question #5.5</skos:prefLabel>
    </rdf:Description>
    <rdf:Description rdf:about="http://JP_ontology.org/assessment/MCQ.5.6">
        <nis2v:hasAnswer rdf:resource="http://JP_ontology.org/assessment/MCQ.5.6AnswerA"/>
        <nis2v:hasAnswer rdf:resource="http://JP_ontology.org/assessment/MCQ.5.6AnswerB"/>
        <nis2v:hasAnswer rdf:resource="http://JP_ontology.org/assessment/MCQ.5.6AnswerC"/>
        <nis2v:relatedToControl rdf:resource="http://JP_ontology.org/iso27001/Control6.1.3"/>
        <terms:contributor>Jenni Parry</terms:contributor>
        <terms:created rdf:datatype="http://www.w3.org/2001/XMLSchema#date">2024-05-20</terms:created>
        <terms:subject rdf:resource="http://JP_ontology.org/nis2v/Article_21.2a"/>
        <rdfs:isDefinedBy rdf:resource="http://JP_ontology.org/assessment"/>
        <skos:altLabel xml:lang="en">MCQ.5.6</skos:altLabel>
        <skos:broader rdf:resource="http://JP_ontology.org/assessment/AssessmentQuestion"/>
        <skos:definition xml:lang="en">Does the organisation retain documented information about the information security risk treatment process?</skos:definition>
        <skos:prefLabel xml:lang="en">Multiple Choice Question #5.6</skos:prefLabel>
    </rdf:Description>
    <rdf:Description rdf:about="http://JP_ontology.org/assessment/MCQ.50">
        <nis2v:hasAnswer rdf:resource="http://JP_ontology.org/assessment/MCQ.50AnswerA"/>
        <nis2v:hasAnswer rdf:resource="http://JP_ontology.org/assessment/MCQ.50AnswerB"/>
        <nis2v:hasAnswer rdf:resource="http://JP_ontology.org/assessment/MCQ.50AnswerC"/>
        <nis2v:relatedToControl rdf:resource="http://JP_ontology.org/iso27001/Control9.2"/>
        <terms:contributor>Jenni Parry</terms:contributor>
        <terms:created rdf:datatype="http://www.w3.org/2001/XMLSchema#date">2024-05-20</terms:created>
        <terms:subject rdf:resource="http://JP_ontology.org/nis2v/Article_21.2f"/>
        <rdfs:isDefinedBy rdf:resource="http://JP_ontology.org/assessment"/>
        <skos:altLabel xml:lang="en">MCQ.50</skos:altLabel>
        <skos:broader rdf:resource="http://JP_ontology.org/assessment/AssessmentQuestion"/>
        <skos:definition xml:lang="en">Is the organisation conducting internal audits at planned intervals to determine whether the information security management system conforms to both the organisation’s own requirements and the requirements outlined in this document, and whether it is effectively implemented and maintained?</skos:definition>
        <skos:prefLabel xml:lang="en">Multiple Choice Question #50</skos:prefLabel>
    </rdf:Description>
    <rdf:Description rdf:about="http://JP_ontology.org/assessment/MCQ.51">
        <nis2v:hasAnswer rdf:resource="http://JP_ontology.org/assessment/MCQ.51AnswerA"/>
        <nis2v:hasAnswer rdf:resource="http://JP_ontology.org/assessment/MCQ.51AnswerB"/>
        <nis2v:hasAnswer rdf:resource="http://JP_ontology.org/assessment/MCQ.51AnswerC"/>
        <nis2v:relatedToControl rdf:resource="http://JP_ontology.org/iso27001/Control9.3"/>
        <terms:contributor>Jenni Parry</terms:contributor>
        <terms:created rdf:datatype="http://www.w3.org/2001/XMLSchema#date">2024-05-20</terms:created>
        <terms:subject rdf:resource="http://JP_ontology.org/nis2v/Article_21.2f"/>
        <rdfs:isDefinedBy rdf:resource="http://JP_ontology.org/assessment"/>
        <skos:altLabel xml:lang="en">MCQ.51</skos:altLabel>
        <skos:broader rdf:resource="http://JP_ontology.org/assessment/AssessmentQuestion"/>
        <skos:definition xml:lang="en">Is top management conducting reviews of the organisation&apos;s information security management system at planned intervals to ensure its continuing suitability, adequacy, and effectiveness?</skos:definition>
        <skos:prefLabel xml:lang="en">Multiple Choice Question #51</skos:prefLabel>
    </rdf:Description>
    <rdf:Description rdf:about="http://JP_ontology.org/assessment/MCQ.52">
        <nis2v:hasAnswer rdf:resource="http://JP_ontology.org/assessment/MCQ.52AnswerA"/>
        <nis2v:hasAnswer rdf:resource="http://JP_ontology.org/assessment/MCQ.52AnswerB"/>
        <nis2v:hasAnswer rdf:resource="http://JP_ontology.org/assessment/MCQ.52AnswerC"/>
        <nis2v:relatedToControl rdf:resource="http://JP_ontology.org/iso27001/ControlA.5.35"/>
        <terms:contributor>Jenni Parry</terms:contributor>
        <terms:created rdf:datatype="http://www.w3.org/2001/XMLSchema#date">2024-05-20</terms:created>
        <terms:subject rdf:resource="http://JP_ontology.org/nis2v/Article_21.2f"/>
        <rdfs:isDefinedBy rdf:resource="http://JP_ontology.org/assessment"/>
        <skos:altLabel xml:lang="en">MCQ.52</skos:altLabel>
        <skos:broader rdf:resource="http://JP_ontology.org/assessment/AssessmentQuestion"/>
        <skos:definition xml:lang="en">Is the organisation’s approach to managing information security and its implementation, including people, processes, and technologies, reviewed independently at planned intervals or when significant changes occur?</skos:definition>
        <skos:prefLabel xml:lang="en">Multiple Choice Question #52</skos:prefLabel>
    </rdf:Description>
    <rdf:Description rdf:about="http://JP_ontology.org/assessment/MCQ.53">
        <nis2v:hasAnswer rdf:resource="http://JP_ontology.org/assessment/MCQ.53AnswerA"/>
        <nis2v:hasAnswer rdf:resource="http://JP_ontology.org/assessment/MCQ.53AnswerB"/>
        <nis2v:hasAnswer rdf:resource="http://JP_ontology.org/assessment/MCQ.53AnswerC"/>
        <nis2v:relatedToControl rdf:resource="http://JP_ontology.org/iso27001/ControlA.5.36"/>
        <terms:contributor>Jenni Parry</terms:contributor>
        <terms:created rdf:datatype="http://www.w3.org/2001/XMLSchema#date">2024-05-20</terms:created>
        <terms:subject rdf:resource="http://JP_ontology.org/nis2v/Article_21.2f"/>
        <rdfs:isDefinedBy rdf:resource="http://JP_ontology.org/assessment"/>
        <skos:altLabel xml:lang="en">MCQ.53</skos:altLabel>
        <skos:broader rdf:resource="http://JP_ontology.org/assessment/AssessmentQuestion"/>
        <skos:definition xml:lang="en">Is compliance with the organisation’s information security policy, topic-specific policies, rules, and standards regularly reviewed?</skos:definition>
        <skos:prefLabel xml:lang="en">Multiple Choice Question #53</skos:prefLabel>
    </rdf:Description>
    <rdf:Description rdf:about="http://JP_ontology.org/assessment/MCQ.54.1">
        <nis2v:hasAnswer rdf:resource="http://JP_ontology.org/assessment/MCQ54.1AnswerA"/>
        <nis2v:hasAnswer rdf:resource="http://JP_ontology.org/assessment/MCQ54.1AnswerB"/>
        <nis2v:hasAnswer rdf:resource="http://JP_ontology.org/assessment/MCQ54.1AnswerC"/>
        <nis2v:relatedToControl rdf:resource="http://JP_ontology.org/iso27001/Control7.2"/>
        <terms:contributor>Jenni Parry</terms:contributor>
        <terms:created rdf:datatype="http://www.w3.org/2001/XMLSchema#date">2024-04-18</terms:created>
        <terms:subject rdf:resource="http://JP_ontology.org/nis2v/Article_21.2g"/>
        <rdfs:isDefinedBy rdf:resource="http://JP_ontology.org/assessment"/>
        <skos:altLabel xml:lang="en">MCQ.54.1</skos:altLabel>
        <skos:broader rdf:resource="http://JP_ontology.org/assessment/AssessmentQuestion"/>
        <skos:definition xml:lang="en">Is the organisation determining the required competence of individuals performing work under its control that affects its information security performance?</skos:definition>
        <skos:prefLabel xml:lang="en">Multiple Choice Question #54.1</skos:prefLabel>
    </rdf:Description>
    <rdf:Description rdf:about="http://JP_ontology.org/assessment/MCQ.54.2">
        <nis2v:hasAnswer rdf:resource="http://JP_ontology.org/assessment/MCQ54.2AnswerA"/>
        <nis2v:hasAnswer rdf:resource="http://JP_ontology.org/assessment/MCQ54.2AnswerB"/>
        <nis2v:hasAnswer rdf:resource="http://JP_ontology.org/assessment/MCQ54.2AnswerC"/>
        <nis2v:relatedToControl rdf:resource="http://JP_ontology.org/iso27001/Control7.2"/>
        <terms:contributor>Jenni Parry</terms:contributor>
        <terms:created rdf:datatype="http://www.w3.org/2001/XMLSchema#date">2024-04-18</terms:created>
        <terms:subject rdf:resource="http://JP_ontology.org/nis2v/Article_21.2g"/>
        <rdfs:isDefinedBy rdf:resource="http://JP_ontology.org/assessment"/>
        <skos:altLabel xml:lang="en">MCQ.54.2</skos:altLabel>
        <skos:broader rdf:resource="http://JP_ontology.org/assessment/AssessmentQuestion"/>
        <skos:definition xml:lang="en">Is the organisation ensuring that these individuals possess the necessary competence through appropriate education, training, or experience?</skos:definition>
        <skos:prefLabel xml:lang="en">Multiple Choice Question #54.2</skos:prefLabel>
    </rdf:Description>
    <rdf:Description rdf:about="http://JP_ontology.org/assessment/MCQ.54.3">
        <nis2v:hasAnswer rdf:resource="http://JP_ontology.org/assessment/MCQ54.3AnswerA"/>
        <nis2v:hasAnswer rdf:resource="http://JP_ontology.org/assessment/MCQ54.3AnswerB"/>
        <nis2v:hasAnswer rdf:resource="http://JP_ontology.org/assessment/MCQ54.3AnswerC"/>
        <nis2v:relatedToControl rdf:resource="http://JP_ontology.org/iso27001/Control7.2"/>
        <terms:contributor>Jenni Parry</terms:contributor>
        <terms:created rdf:datatype="http://www.w3.org/2001/XMLSchema#date">2024-04-18</terms:created>
        <terms:subject rdf:resource="http://JP_ontology.org/nis2v/Article_21.2g"/>
        <rdfs:isDefinedBy rdf:resource="http://JP_ontology.org/assessment"/>
        <skos:altLabel xml:lang="en">MCQ.54.3</skos:altLabel>
        <skos:broader rdf:resource="http://JP_ontology.org/assessment/AssessmentQuestion"/>
        <skos:definition xml:lang="en">Is the organisation taking necessary actions, where applicable, to acquire the required competence and evaluating the effectiveness of these actions?</skos:definition>
        <skos:prefLabel xml:lang="en">Multiple Choice Question #54.3</skos:prefLabel>
    </rdf:Description>
    <rdf:Description rdf:about="http://JP_ontology.org/assessment/MCQ.54.4">
        <nis2v:hasAnswer rdf:resource="http://JP_ontology.org/assessment/MCQ54.4AnswerA"/>
        <nis2v:hasAnswer rdf:resource="http://JP_ontology.org/assessment/MCQ54.4AnswerB"/>
        <nis2v:hasAnswer rdf:resource="http://JP_ontology.org/assessment/MCQ54.4AnswerC"/>
        <nis2v:relatedToControl rdf:resource="http://JP_ontology.org/iso27001/Control7.2"/>
        <terms:contributor>Jenni Parry</terms:contributor>
        <terms:created rdf:datatype="http://www.w3.org/2001/XMLSchema#date">2024-04-18</terms:created>
        <terms:subject rdf:resource="http://JP_ontology.org/nis2v/Article_21.2g"/>
        <rdfs:isDefinedBy rdf:resource="http://JP_ontology.org/assessment"/>
        <skos:altLabel xml:lang="en">MCQ.54.4</skos:altLabel>
        <skos:broader rdf:resource="http://JP_ontology.org/assessment/AssessmentQuestion"/>
        <skos:definition xml:lang="en">Is the organisation retaining appropriate documented information as evidence of competence?</skos:definition>
        <skos:prefLabel xml:lang="en">Multiple Choice Question #54.4</skos:prefLabel>
    </rdf:Description>
    <rdf:Description rdf:about="http://JP_ontology.org/assessment/MCQ.55.1">
        <nis2v:hasAnswer rdf:resource="http://JP_ontology.org/assessment/MCQ.55.1AnswerA"/>
        <nis2v:hasAnswer rdf:resource="http://JP_ontology.org/assessment/MCQ.55.1AnswerB"/>
        <nis2v:hasAnswer rdf:resource="http://JP_ontology.org/assessment/MCQ.55.1AnswerC"/>
        <nis2v:relatedToControl rdf:resource="http://JP_ontology.org/iso27001/Control7.3"/>
        <terms:contributor>Jenni Parry</terms:contributor>
        <terms:created rdf:datatype="http://www.w3.org/2001/XMLSchema#date">2024-05-20</terms:created>
        <terms:subject rdf:resource="http://JP_ontology.org/nis2v/Article_21.2g"/>
        <rdfs:isDefinedBy rdf:resource="http://JP_ontology.org/assessment"/>
        <skos:altLabel xml:lang="en">MCQ.55.1</skos:altLabel>
        <skos:broader rdf:resource="http://JP_ontology.org/assessment/AssessmentQuestion"/>
        <skos:definition xml:lang="en">Are persons doing work under the organisation’s control aware of the information security policy?</skos:definition>
        <skos:prefLabel xml:lang="en">Multiple Choice Question #55.1</skos:prefLabel>
    </rdf:Description>
    <rdf:Description rdf:about="http://JP_ontology.org/assessment/MCQ.55.2">
        <nis2v:hasAnswer rdf:resource="http://JP_ontology.org/assessment/MCQ.55.2AnswerA"/>
        <nis2v:hasAnswer rdf:resource="http://JP_ontology.org/assessment/MCQ.55.2AnswerB"/>
        <nis2v:hasAnswer rdf:resource="http://JP_ontology.org/assessment/MCQ.55.2AnswerC"/>
        <nis2v:relatedToControl rdf:resource="http://JP_ontology.org/iso27001/Control7.3"/>
        <terms:contributor>Jenni Parry</terms:contributor>
        <terms:created rdf:datatype="http://www.w3.org/2001/XMLSchema#date">2024-05-20</terms:created>
        <terms:subject rdf:resource="http://JP_ontology.org/nis2v/Article_21.2g"/>
        <rdfs:isDefinedBy rdf:resource="http://JP_ontology.org/assessment"/>
        <skos:altLabel xml:lang="en">MCQ.55.2</skos:altLabel>
        <skos:broader rdf:resource="http://JP_ontology.org/assessment/AssessmentQuestion"/>
        <skos:definition xml:lang="en">Are persons doing work under the organisation’s control aware of their contribution to the effectiveness of the information security management system, including the benefits of improved information security performance?</skos:definition>
        <skos:prefLabel xml:lang="en">Multiple Choice Question #55.2</skos:prefLabel>
    </rdf:Description>
    <rdf:Description rdf:about="http://JP_ontology.org/assessment/MCQ.55.3">
        <nis2v:hasAnswer rdf:resource="http://JP_ontology.org/assessment/MCQ.55.3AnswerA"/>
        <nis2v:hasAnswer rdf:resource="http://JP_ontology.org/assessment/MCQ.55.3AnswerB"/>
        <nis2v:hasAnswer rdf:resource="http://JP_ontology.org/assessment/MCQ.55.3AnswerC"/>
        <nis2v:relatedToControl rdf:resource="http://JP_ontology.org/iso27001/Control7.3"/>
        <terms:contributor>Jenni Parry</terms:contributor>
        <terms:created rdf:datatype="http://www.w3.org/2001/XMLSchema#date">2024-05-20</terms:created>
        <terms:subject rdf:resource="http://JP_ontology.org/nis2v/Article_21.2g"/>
        <rdfs:isDefinedBy rdf:resource="http://JP_ontology.org/assessment"/>
        <skos:altLabel xml:lang="en">MCQ.55.3</skos:altLabel>
        <skos:broader rdf:resource="http://JP_ontology.org/assessment/AssessmentQuestion"/>
        <skos:definition xml:lang="en">Are persons doing work under the organisation’s control aware of the implications of not conforming with the information security management system requirements?</skos:definition>
        <skos:prefLabel xml:lang="en">Multiple Choice Question #55.3</skos:prefLabel>
    </rdf:Description>
    <rdf:Description rdf:about="http://JP_ontology.org/assessment/MCQ.56.1">
        <nis2v:hasAnswer rdf:resource="http://JP_ontology.org/assessment/MCQ.56.1AnswerA"/>
        <nis2v:hasAnswer rdf:resource="http://JP_ontology.org/assessment/MCQ.56.1AnswerB"/>
        <nis2v:hasAnswer rdf:resource="http://JP_ontology.org/assessment/MCQ.56.1AnswerC"/>
        <nis2v:relatedToControl rdf:resource="http://JP_ontology.org/iso27001/Control7.4"/>
        <terms:contributor>Jenni Parry</terms:contributor>
        <terms:created rdf:datatype="http://www.w3.org/2001/XMLSchema#date">2024-05-20</terms:created>
        <terms:subject rdf:resource="http://JP_ontology.org/nis2v/Article_21.2g"/>
        <rdfs:isDefinedBy rdf:resource="http://JP_ontology.org/assessment"/>
        <skos:altLabel xml:lang="en">MCQ.56.1</skos:altLabel>
        <skos:broader rdf:resource="http://JP_ontology.org/assessment/AssessmentQuestion"/>
        <skos:definition xml:lang="en">Does the organisation determine what information to communicate relevant to the information security management system?</skos:definition>
        <skos:prefLabel xml:lang="en">Multiple Choice Question #56.1</skos:prefLabel>
    </rdf:Description>
    <rdf:Description rdf:about="http://JP_ontology.org/assessment/MCQ.56.2">
        <nis2v:hasAnswer rdf:resource="http://JP_ontology.org/assessment/MCQ.56.2AnswerA"/>
        <nis2v:hasAnswer rdf:resource="http://JP_ontology.org/assessment/MCQ.56.2AnswerB"/>
        <nis2v:hasAnswer rdf:resource="http://JP_ontology.org/assessment/MCQ.56.2AnswerC"/>
        <nis2v:relatedToControl rdf:resource="http://JP_ontology.org/iso27001/Control7.4"/>
        <terms:contributor>Jenni Parry</terms:contributor>
        <terms:created rdf:datatype="http://www.w3.org/2001/XMLSchema#date">2024-05-20</terms:created>
        <terms:subject rdf:resource="http://JP_ontology.org/nis2v/Article_21.2g"/>
        <rdfs:isDefinedBy rdf:resource="http://JP_ontology.org/assessment"/>
        <skos:altLabel xml:lang="en">MCQ.56.2</skos:altLabel>
        <skos:broader rdf:resource="http://JP_ontology.org/assessment/AssessmentQuestion"/>
        <skos:definition xml:lang="en">Does the organisation determine when to communicate information relevant to the information security management system?</skos:definition>
        <skos:prefLabel xml:lang="en">Multiple Choice Question #56.2</skos:prefLabel>
    </rdf:Description>
    <rdf:Description rdf:about="http://JP_ontology.org/assessment/MCQ.56.3">
        <nis2v:hasAnswer rdf:resource="http://JP_ontology.org/assessment/MCQ.56.3AnswerA"/>
        <nis2v:hasAnswer rdf:resource="http://JP_ontology.org/assessment/MCQ.56.3AnswerB"/>
        <nis2v:hasAnswer rdf:resource="http://JP_ontology.org/assessment/MCQ.56.3AnswerC"/>
        <nis2v:relatedToControl rdf:resource="http://JP_ontology.org/iso27001/Control7.4"/>
        <terms:contributor>Jenni Parry</terms:contributor>
        <terms:created rdf:datatype="http://www.w3.org/2001/XMLSchema#date">2024-05-20</terms:created>
        <terms:subject rdf:resource="http://JP_ontology.org/nis2v/Article_21.2g"/>
        <rdfs:isDefinedBy rdf:resource="http://JP_ontology.org/assessment"/>
        <skos:altLabel xml:lang="en">MCQ.56.3</skos:altLabel>
        <skos:broader rdf:resource="http://JP_ontology.org/assessment/AssessmentQuestion"/>
        <skos:definition xml:lang="en">Does the organisation determine with whom to communicate information relevant to the information security management system?</skos:definition>
        <skos:prefLabel xml:lang="en">Multiple Choice Question #56.3</skos:prefLabel>
    </rdf:Description>
    <rdf:Description rdf:about="http://JP_ontology.org/assessment/MCQ.56.4">
        <nis2v:hasAnswer rdf:resource="http://JP_ontology.org/assessment/MCQ.56.4AnswerA"/>
        <nis2v:hasAnswer rdf:resource="http://JP_ontology.org/assessment/MCQ.56.4AnswerB"/>
        <nis2v:hasAnswer rdf:resource="http://JP_ontology.org/assessment/MCQ.56.4AnswerC"/>
        <nis2v:relatedToControl rdf:resource="http://JP_ontology.org/iso27001/Control7.4"/>
        <terms:contributor>Jenni Parry</terms:contributor>
        <terms:created rdf:datatype="http://www.w3.org/2001/XMLSchema#date">2024-05-20</terms:created>
        <terms:subject rdf:resource="http://JP_ontology.org/nis2v/Article_21.2g"/>
        <rdfs:isDefinedBy rdf:resource="http://JP_ontology.org/assessment"/>
        <skos:altLabel xml:lang="en">MCQ.56.4</skos:altLabel>
        <skos:broader rdf:resource="http://JP_ontology.org/assessment/AssessmentQuestion"/>
        <skos:definition xml:lang="en">Does the organisation determine how to communicate information relevant to the information security management system?</skos:definition>
        <skos:prefLabel xml:lang="en">Multiple Choice Question #56.4</skos:prefLabel>
    </rdf:Description>
    <rdf:Description rdf:about="http://JP_ontology.org/assessment/MCQ.57.1">
        <nis2v:hasAnswer rdf:resource="http://JP_ontology.org/assessment/MCQ.57.1AnswerA"/>
        <nis2v:hasAnswer rdf:resource="http://JP_ontology.org/assessment/MCQ.57.1AnswerB"/>
        <nis2v:hasAnswer rdf:resource="http://JP_ontology.org/assessment/MCQ.57.1AnswerC"/>
        <nis2v:relatedToControl rdf:resource="http://JP_ontology.org/iso27001/ControlA.6.3"/>
        <terms:contributor>Jenni Parry</terms:contributor>
        <terms:created rdf:datatype="http://www.w3.org/2001/XMLSchema#date">2024-05-20</terms:created>
        <terms:subject rdf:resource="http://JP_ontology.org/nis2v/Article_21.2g"/>
        <rdfs:isDefinedBy rdf:resource="http://JP_ontology.org/assessment"/>
        <skos:altLabel xml:lang="en">MCQ.57.1</skos:altLabel>
        <skos:broader rdf:resource="http://JP_ontology.org/assessment/AssessmentQuestion"/>
        <skos:definition xml:lang="en">Do personnel of the organisation and relevant interested parties receive appropriate information security awareness, education, and training?</skos:definition>
        <skos:prefLabel xml:lang="en">Multiple Choice Question #57.1</skos:prefLabel>
    </rdf:Description>
    <rdf:Description rdf:about="http://JP_ontology.org/assessment/MCQ.57.2">
        <nis2v:hasAnswer rdf:resource="http://JP_ontology.org/assessment/MCQ.57.2AnswerA"/>
        <nis2v:hasAnswer rdf:resource="http://JP_ontology.org/assessment/MCQ.57.2AnswerB"/>
        <nis2v:hasAnswer rdf:resource="http://JP_ontology.org/assessment/MCQ.57.2AnswerC"/>
        <nis2v:relatedToControl rdf:resource="http://JP_ontology.org/iso27001/ControlA.6.3"/>
        <terms:contributor>Jenni Parry</terms:contributor>
        <terms:created rdf:datatype="http://www.w3.org/2001/XMLSchema#date">2024-05-20</terms:created>
        <terms:subject rdf:resource="http://JP_ontology.org/nis2v/Article_21.2g"/>
        <rdfs:isDefinedBy rdf:resource="http://JP_ontology.org/assessment"/>
        <skos:altLabel xml:lang="en">MCQ.57.2</skos:altLabel>
        <skos:broader rdf:resource="http://JP_ontology.org/assessment/AssessmentQuestion"/>
        <skos:definition xml:lang="en">Are regular updates of the organisation&apos;s information security policy, topic-specific policies, and procedures relevant to their job function provided to personnel of the organisation and relevant interested parties?</skos:definition>
        <skos:prefLabel xml:lang="en">Multiple Choice Question #57.2</skos:prefLabel>
    </rdf:Description>
    <rdf:Description rdf:about="http://JP_ontology.org/assessment/MCQ.58">
        <nis2v:hasAnswer rdf:resource="http://JP_ontology.org/assessment/MCQ58AnswerA"/>
        <nis2v:hasAnswer rdf:resource="http://JP_ontology.org/assessment/MCQ58AnswerB"/>
        <nis2v:hasAnswer rdf:resource="http://JP_ontology.org/assessment/MCQ58AnswerC"/>
        <nis2v:relatedToControl rdf:resource="http://JP_ontology.org/iso27001/ControlA.7.7"/>
        <terms:contributor>Jenni Parry</terms:contributor>
        <terms:created rdf:datatype="http://www.w3.org/2001/XMLSchema#date">2024-04-18</terms:created>
        <terms:subject rdf:resource="http://JP_ontology.org/nis2v/Article_21.2g"/>
        <rdfs:isDefinedBy rdf:resource="http://JP_ontology.org/assessment"/>
        <skos:altLabel xml:lang="en">MCQ.58</skos:altLabel>
        <skos:broader rdf:resource="http://JP_ontology.org/assessment/AssessmentQuestion"/>
        <skos:definition xml:lang="en">Are clear desk rules for papers and removable storage media, as well as clear screen rules for information processing facilities, defined and appropriately enforced?</skos:definition>
        <skos:prefLabel xml:lang="en">Multiple Choice Question #58</skos:prefLabel>
    </rdf:Description>
    <rdf:Description rdf:about="http://JP_ontology.org/assessment/MCQ.59">
        <nis2v:hasAnswer rdf:resource="http://JP_ontology.org/assessment/MCQ.59AnswerA"/>
        <nis2v:hasAnswer rdf:resource="http://JP_ontology.org/assessment/MCQ.59AnswerB"/>
        <nis2v:hasAnswer rdf:resource="http://JP_ontology.org/assessment/MCQ.59AnswerC"/>
        <nis2v:relatedToControl rdf:resource="http://JP_ontology.org/iso27001/ControlA.5.15"/>
        <terms:contributor>Jenni Parry</terms:contributor>
        <terms:created rdf:datatype="http://www.w3.org/2001/XMLSchema#date">2024-05-20</terms:created>
        <terms:subject rdf:resource="http://JP_ontology.org/nis2v/Article_21.2g"/>
        <rdfs:isDefinedBy rdf:resource="http://JP_ontology.org/assessment"/>
        <skos:altLabel xml:lang="en">MCQ.59</skos:altLabel>
        <skos:broader rdf:resource="http://JP_ontology.org/assessment/AssessmentQuestion"/>
        <skos:definition xml:lang="en">Are rules established and implemented to control physical and logical access to information and other associated assets, based on business and information security requirements?</skos:definition>
        <skos:prefLabel xml:lang="en">Multiple Choice Question #59</skos:prefLabel>
    </rdf:Description>
    <rdf:Description rdf:about="http://JP_ontology.org/assessment/MCQ.6.1">
        <nis2v:hasAnswer rdf:resource="http://JP_ontology.org/assessment/MCQ.6.1AnswerA"/>
        <nis2v:hasAnswer rdf:resource="http://JP_ontology.org/assessment/MCQ.6.1AnswerB"/>
        <nis2v:hasAnswer rdf:resource="http://JP_ontology.org/assessment/MCQ.6.1AnswerC"/>
        <nis2v:relatedToControl rdf:resource="http://JP_ontology.org/iso27001/Control7.4"/>
        <terms:contributor>Jenni Parry</terms:contributor>
        <terms:created rdf:datatype="http://www.w3.org/2001/XMLSchema#date">2024-05-20</terms:created>
        <terms:subject rdf:resource="http://JP_ontology.org/nis2v/Article_21.2a"/>
        <rdfs:isDefinedBy rdf:resource="http://JP_ontology.org/assessment"/>
        <skos:altLabel xml:lang="en">MCQ.6.1</skos:altLabel>
        <skos:broader rdf:resource="http://JP_ontology.org/assessment/AssessmentQuestion"/>
        <skos:definition xml:lang="en">Does the organisation determine what information to communicate relevant to the information security management system?</skos:definition>
        <skos:prefLabel xml:lang="en">Multiple Choice Question #6.1</skos:prefLabel>
    </rdf:Description>
    <rdf:Description rdf:about="http://JP_ontology.org/assessment/MCQ.6.2">
        <nis2v:hasAnswer rdf:resource="http://JP_ontology.org/assessment/MCQ.6.2AnswerA"/>
        <nis2v:hasAnswer rdf:resource="http://JP_ontology.org/assessment/MCQ.6.2AnswerB"/>
        <nis2v:hasAnswer rdf:resource="http://JP_ontology.org/assessment/MCQ.6.2AnswerC"/>
        <nis2v:relatedToControl rdf:resource="http://JP_ontology.org/iso27001/Control7.4"/>
        <terms:contributor>Jenni Parry</terms:contributor>
        <terms:created rdf:datatype="http://www.w3.org/2001/XMLSchema#date">2024-05-20</terms:created>
        <terms:subject rdf:resource="http://JP_ontology.org/nis2v/Article_21.2a"/>
        <rdfs:isDefinedBy rdf:resource="http://JP_ontology.org/assessment"/>
        <skos:altLabel xml:lang="en">MCQ.6.2</skos:altLabel>
        <skos:broader rdf:resource="http://JP_ontology.org/assessment/AssessmentQuestion"/>
        <skos:definition xml:lang="en">Does the organisation determine when to communicate information relevant to the information security management system?</skos:definition>
        <skos:prefLabel xml:lang="en">Multiple Choice Question #6.2</skos:prefLabel>
    </rdf:Description>
    <rdf:Description rdf:about="http://JP_ontology.org/assessment/MCQ.6.3">
        <nis2v:hasAnswer rdf:resource="http://JP_ontology.org/assessment/MCQ.6.3AnswerA"/>
        <nis2v:hasAnswer rdf:resource="http://JP_ontology.org/assessment/MCQ.6.3AnswerB"/>
        <nis2v:hasAnswer rdf:resource="http://JP_ontology.org/assessment/MCQ.6.3AnswerC"/>
        <nis2v:relatedToControl rdf:resource="http://JP_ontology.org/iso27001/Control7.4"/>
        <terms:contributor>Jenni Parry</terms:contributor>
        <terms:created rdf:datatype="http://www.w3.org/2001/XMLSchema#date">2024-05-20</terms:created>
        <terms:subject rdf:resource="http://JP_ontology.org/nis2v/Article_21.2a"/>
        <rdfs:isDefinedBy rdf:resource="http://JP_ontology.org/assessment"/>
        <skos:altLabel xml:lang="en">MCQ.6.3</skos:altLabel>
        <skos:broader rdf:resource="http://JP_ontology.org/assessment/AssessmentQuestion"/>
        <skos:definition xml:lang="en">Does the organisation determine with whom to communicate information relevant to the information security management system?</skos:definition>
        <skos:prefLabel xml:lang="en">Multiple Choice Question #6.3</skos:prefLabel>
    </rdf:Description>
    <rdf:Description rdf:about="http://JP_ontology.org/assessment/MCQ.6.4">
        <nis2v:hasAnswer rdf:resource="http://JP_ontology.org/assessment/MCQ.6.4AnswerA"/>
        <nis2v:hasAnswer rdf:resource="http://JP_ontology.org/assessment/MCQ.6.4AnswerB"/>
        <nis2v:hasAnswer rdf:resource="http://JP_ontology.org/assessment/MCQ.6.4AnswerC"/>
        <nis2v:relatedToControl rdf:resource="http://JP_ontology.org/iso27001/Control7.4"/>
        <terms:contributor>Jenni Parry</terms:contributor>
        <terms:created rdf:datatype="http://www.w3.org/2001/XMLSchema#date">2024-05-20</terms:created>
        <terms:subject rdf:resource="http://JP_ontology.org/nis2v/Article_21.2a"/>
        <rdfs:isDefinedBy rdf:resource="http://JP_ontology.org/assessment"/>
        <skos:altLabel xml:lang="en">MCQ.6.4</skos:altLabel>
        <skos:broader rdf:resource="http://JP_ontology.org/assessment/AssessmentQuestion"/>
        <skos:definition xml:lang="en">Does the organisation determine how to communicate information relevant to the information security management system?</skos:definition>
        <skos:prefLabel xml:lang="en">Multiple Choice Question #6.4</skos:prefLabel>
    </rdf:Description>
    <rdf:Description rdf:about="http://JP_ontology.org/assessment/MCQ.60">
        <nis2v:hasAnswer rdf:resource="http://JP_ontology.org/assessment/MCQ.60AnswerA"/>
        <nis2v:hasAnswer rdf:resource="http://JP_ontology.org/assessment/MCQ.60AnswerB"/>
        <nis2v:hasAnswer rdf:resource="http://JP_ontology.org/assessment/MCQ.60AnswerC"/>
        <nis2v:relatedToControl rdf:resource="http://JP_ontology.org/iso27001/ControlA.5.16"/>
        <terms:contributor>Jenni Parry</terms:contributor>
        <terms:created rdf:datatype="http://www.w3.org/2001/XMLSchema#date">2024-05-20</terms:created>
        <terms:subject rdf:resource="http://JP_ontology.org/nis2v/Article_21.2g"/>
        <rdfs:isDefinedBy rdf:resource="http://JP_ontology.org/assessment"/>
        <skos:altLabel xml:lang="en">MCQ.60</skos:altLabel>
        <skos:broader rdf:resource="http://JP_ontology.org/assessment/AssessmentQuestion"/>
        <skos:definition xml:lang="en">Is the organisation managing the complete life cycle of identities, encompassing activities such as identity creation, authentication, authorization, periodic reviews, modification, and termination, ensuring comprehensive oversight and control over identity-related processes?</skos:definition>
        <skos:prefLabel xml:lang="en">Multiple Choice Question #60</skos:prefLabel>
    </rdf:Description>
    <rdf:Description rdf:about="http://JP_ontology.org/assessment/MCQ.61">
        <nis2v:hasAnswer rdf:resource="http://JP_ontology.org/assessment/MCQ.61AnswerA"/>
        <nis2v:hasAnswer rdf:resource="http://JP_ontology.org/assessment/MCQ.61AnswerB"/>
        <nis2v:hasAnswer rdf:resource="http://JP_ontology.org/assessment/MCQ.61AnswerC"/>
        <nis2v:relatedToControl rdf:resource="http://JP_ontology.org/iso27001/ControlA.5.17"/>
        <terms:contributor>Jenni Parry</terms:contributor>
        <terms:created rdf:datatype="http://www.w3.org/2001/XMLSchema#date">2024-05-20</terms:created>
        <terms:subject rdf:resource="http://JP_ontology.org/nis2v/Article_21.2g"/>
        <rdfs:isDefinedBy rdf:resource="http://JP_ontology.org/assessment"/>
        <skos:altLabel xml:lang="en">MCQ.61</skos:altLabel>
        <skos:broader rdf:resource="http://JP_ontology.org/assessment/AssessmentQuestion"/>
        <skos:definition xml:lang="en">Is the allocation and management of authentication information controlled by a management process, which includes advising personnel on the appropriate handling of authentication information?</skos:definition>
        <skos:prefLabel xml:lang="en">Multiple Choice Question #61</skos:prefLabel>
    </rdf:Description>
    <rdf:Description rdf:about="http://JP_ontology.org/assessment/MCQ.62">
        <nis2v:hasAnswer rdf:resource="http://JP_ontology.org/assessment/MCQ.62AnswerA"/>
        <nis2v:hasAnswer rdf:resource="http://JP_ontology.org/assessment/MCQ.62AnswerB"/>
        <nis2v:hasAnswer rdf:resource="http://JP_ontology.org/assessment/MCQ.62AnswerC"/>
        <nis2v:relatedToControl rdf:resource="http://JP_ontology.org/iso27001/ControlA.5.18"/>
        <terms:contributor>Jenni Parry</terms:contributor>
        <terms:created rdf:datatype="http://www.w3.org/2001/XMLSchema#date">2024-05-20</terms:created>
        <terms:subject rdf:resource="http://JP_ontology.org/nis2v/Article_21.2g"/>
        <rdfs:isDefinedBy rdf:resource="http://JP_ontology.org/assessment"/>
        <skos:altLabel xml:lang="en">MCQ.62</skos:altLabel>
        <skos:broader rdf:resource="http://JP_ontology.org/assessment/AssessmentQuestion"/>
        <skos:definition xml:lang="en">Are access rights to information and other associated assets provisioned, reviewed, modified, and removed in accordance with the organisation’s topic-specific policy and rules for access control?</skos:definition>
        <skos:prefLabel xml:lang="en">Multiple Choice Question #62</skos:prefLabel>
    </rdf:Description>
    <rdf:Description rdf:about="http://JP_ontology.org/assessment/MCQ.63">
        <nis2v:hasAnswer rdf:resource="http://JP_ontology.org/assessment/MCQ.63AnswerA"/>
        <nis2v:hasAnswer rdf:resource="http://JP_ontology.org/assessment/MCQ.63AnswerB"/>
        <nis2v:hasAnswer rdf:resource="http://JP_ontology.org/assessment/MCQ.63AnswerC"/>
        <nis2v:relatedToControl rdf:resource="http://JP_ontology.org/iso27001/ControlA.8.8"/>
        <terms:contributor>Jenni Parry</terms:contributor>
        <terms:created rdf:datatype="http://www.w3.org/2001/XMLSchema#date">2024-05-20</terms:created>
        <terms:subject rdf:resource="http://JP_ontology.org/nis2v/Article_21.2g"/>
        <rdfs:isDefinedBy rdf:resource="http://JP_ontology.org/assessment"/>
        <skos:altLabel xml:lang="en">MCQ.63</skos:altLabel>
        <skos:broader rdf:resource="http://JP_ontology.org/assessment/AssessmentQuestion"/>
        <skos:definition xml:lang="en">Does the organisation acquire information regarding technical vulnerabilities of the information systems in use, evaluate the organisation’s exposure to such vulnerabilities, and implement appropriate measures accordingly?</skos:definition>
        <skos:prefLabel xml:lang="en">Multiple Choice Question #63</skos:prefLabel>
    </rdf:Description>
    <rdf:Description rdf:about="http://JP_ontology.org/assessment/MCQ.64">
        <nis2v:hasAnswer rdf:resource="http://JP_ontology.org/assessment/MCQ.64AnswerA"/>
        <nis2v:hasAnswer rdf:resource="http://JP_ontology.org/assessment/MCQ.64AnswerB"/>
        <nis2v:hasAnswer rdf:resource="http://JP_ontology.org/assessment/MCQ.64AnswerC"/>
        <nis2v:relatedToControl rdf:resource="http://JP_ontology.org/iso27001/ControlA.8.9"/>
        <terms:contributor>Jenni Parry</terms:contributor>
        <terms:created rdf:datatype="http://www.w3.org/2001/XMLSchema#date">2024-05-20</terms:created>
        <terms:subject rdf:resource="http://JP_ontology.org/nis2v/Article_21.2g"/>
        <rdfs:isDefinedBy rdf:resource="http://JP_ontology.org/assessment"/>
        <skos:altLabel xml:lang="en">MCQ.64</skos:altLabel>
        <skos:broader rdf:resource="http://JP_ontology.org/assessment/AssessmentQuestion"/>
        <skos:definition xml:lang="en">Are configurations, including security configurations, of hardware, software, services, and networks established, documented, implemented, monitored, and reviewed?</skos:definition>
        <skos:prefLabel xml:lang="en">Multiple Choice Question #64</skos:prefLabel>
    </rdf:Description>
    <rdf:Description rdf:about="http://JP_ontology.org/assessment/MCQ.65">
        <nis2v:hasAnswer rdf:resource="http://JP_ontology.org/assessment/MCQ.65AnswerA"/>
        <nis2v:hasAnswer rdf:resource="http://JP_ontology.org/assessment/MCQ.65AnswerB"/>
        <nis2v:hasAnswer rdf:resource="http://JP_ontology.org/assessment/MCQ.65AnswerC"/>
        <nis2v:relatedToControl rdf:resource="http://JP_ontology.org/iso27001/ControlA.8.7"/>
        <terms:contributor>Jenni Parry</terms:contributor>
        <terms:created rdf:datatype="http://www.w3.org/2001/XMLSchema#date">2024-05-20</terms:created>
        <terms:subject rdf:resource="http://JP_ontology.org/nis2v/Article_21.2g"/>
        <rdfs:isDefinedBy rdf:resource="http://JP_ontology.org/assessment"/>
        <skos:altLabel xml:lang="en">MCQ.65</skos:altLabel>
        <skos:broader rdf:resource="http://JP_ontology.org/assessment/AssessmentQuestion"/>
        <skos:definition xml:lang="en">Is protection against malware implemented and supported by appropriate user awareness measures?</skos:definition>
        <skos:prefLabel xml:lang="en">Multiple Choice Question #65</skos:prefLabel>
    </rdf:Description>
    <rdf:Description rdf:about="http://JP_ontology.org/assessment/MCQ.66">
        <nis2v:hasAnswer rdf:resource="http://JP_ontology.org/assessment/MCQ.66AnswerA"/>
        <nis2v:hasAnswer rdf:resource="http://JP_ontology.org/assessment/MCQ.66AnswerB"/>
        <nis2v:hasAnswer rdf:resource="http://JP_ontology.org/assessment/MCQ.66AnswerC"/>
        <nis2v:relatedToControl rdf:resource="http://JP_ontology.org/iso27001/ControlA.8.19"/>
        <terms:contributor>Jenni Parry</terms:contributor>
        <terms:created rdf:datatype="http://www.w3.org/2001/XMLSchema#date">2024-05-20</terms:created>
        <terms:subject rdf:resource="http://JP_ontology.org/nis2v/Article_21.2g"/>
        <rdfs:isDefinedBy rdf:resource="http://JP_ontology.org/assessment"/>
        <skos:altLabel xml:lang="en">MCQ.66</skos:altLabel>
        <skos:broader rdf:resource="http://JP_ontology.org/assessment/AssessmentQuestion"/>
        <skos:definition xml:lang="en">Have procedures and measures been implemented to securely manage software installation on operational systems?</skos:definition>
        <skos:prefLabel xml:lang="en">Multiple Choice Question #66</skos:prefLabel>
    </rdf:Description>
    <rdf:Description rdf:about="http://JP_ontology.org/assessment/MCQ.67">
        <nis2v:hasAnswer rdf:resource="http://JP_ontology.org/assessment/MCQ.67AnswerA"/>
        <nis2v:hasAnswer rdf:resource="http://JP_ontology.org/assessment/MCQ.67AnswerB"/>
        <nis2v:hasAnswer rdf:resource="http://JP_ontology.org/assessment/MCQ.67AnswerC"/>
        <nis2v:relatedToControl rdf:resource="http://JP_ontology.org/iso27001/ControlA.8.22"/>
        <terms:contributor>Jenni Parry</terms:contributor>
        <terms:created rdf:datatype="http://www.w3.org/2001/XMLSchema#date">2024-05-20</terms:created>
        <terms:subject rdf:resource="http://JP_ontology.org/nis2v/Article_21.2g"/>
        <rdfs:isDefinedBy rdf:resource="http://JP_ontology.org/assessment"/>
        <skos:altLabel xml:lang="en">MCQ.67</skos:altLabel>
        <skos:broader rdf:resource="http://JP_ontology.org/assessment/AssessmentQuestion"/>
        <skos:definition xml:lang="en">Is segregation implemented for groups of information services, users, and information systems within the organisation&apos;s networks?</skos:definition>
        <skos:prefLabel xml:lang="en">Multiple Choice Question #67</skos:prefLabel>
    </rdf:Description>
    <rdf:Description rdf:about="http://JP_ontology.org/assessment/MCQ.68">
        <nis2v:hasAnswer rdf:resource="http://JP_ontology.org/assessment/MCQ68AnswerA"/>
        <nis2v:hasAnswer rdf:resource="http://JP_ontology.org/assessment/MCQ68AnswerB"/>
        <nis2v:hasAnswer rdf:resource="http://JP_ontology.org/assessment/MCQ68AnswerC"/>
        <nis2v:relatedToControl rdf:resource="http://JP_ontology.org/iso27001/ControlA.5.37"/>
        <terms:contributor>Jenni Parry</terms:contributor>
        <terms:created rdf:datatype="http://www.w3.org/2001/XMLSchema#date">2024-04-18</terms:created>
        <terms:subject rdf:resource="http://JP_ontology.org/nis2v/Article_21.2h"/>
        <rdfs:isDefinedBy rdf:resource="http://JP_ontology.org/assessment"/>
        <skos:altLabel xml:lang="en">MCQ.68</skos:altLabel>
        <skos:broader rdf:resource="http://JP_ontology.org/assessment/AssessmentQuestion"/>
        <skos:definition xml:lang="en">Are operating procedures for information processing facilities documented and made available to personnel who require them?</skos:definition>
        <skos:prefLabel xml:lang="en">Multiple Choice Question #68</skos:prefLabel>
    </rdf:Description>
    <rdf:Description rdf:about="http://JP_ontology.org/assessment/MCQ.69">
        <nis2v:hasAnswer rdf:resource="http://JP_ontology.org/assessment/MCQ.69AnswerA"/>
        <nis2v:hasAnswer rdf:resource="http://JP_ontology.org/assessment/MCQ.69AnswerB"/>
        <nis2v:hasAnswer rdf:resource="http://JP_ontology.org/assessment/MCQ.69AnswerC"/>
        <nis2v:relatedToControl rdf:resource="http://JP_ontology.org/iso27001/ControlA.8.24"/>
        <terms:contributor>Jenni Parry</terms:contributor>
        <terms:created rdf:datatype="http://www.w3.org/2001/XMLSchema#date">2024-05-20</terms:created>
        <terms:subject rdf:resource="http://JP_ontology.org/nis2v/Article_21.2h"/>
        <rdfs:isDefinedBy rdf:resource="http://JP_ontology.org/assessment"/>
        <skos:altLabel xml:lang="en">MCQ.69</skos:altLabel>
        <skos:broader rdf:resource="http://JP_ontology.org/assessment/AssessmentQuestion"/>
        <skos:definition xml:lang="en">Are rules for the effective use of cryptography, including cryptographic key management, defined and implemented?</skos:definition>
        <skos:prefLabel xml:lang="en">Multiple Choice Question #69</skos:prefLabel>
    </rdf:Description>
    <rdf:Description rdf:about="http://JP_ontology.org/assessment/MCQ.7">
        <nis2v:hasAnswer rdf:resource="http://JP_ontology.org/assessment/MCQ7AnswerA"/>
        <nis2v:hasAnswer rdf:resource="http://JP_ontology.org/assessment/MCQ7AnswerB"/>
        <nis2v:hasAnswer rdf:resource="http://JP_ontology.org/assessment/MCQ7AnswerC"/>
        <nis2v:relatedToControl rdf:resource="http://JP_ontology.org/iso27001/Control7.5"/>
        <terms:contributor>Jenni Parry</terms:contributor>
        <terms:created rdf:datatype="http://www.w3.org/2001/XMLSchema#date">2024-04-17</terms:created>
        <terms:subject rdf:resource="http://JP_ontology.org/nis2v/Article_21.2a"/>
        <rdfs:isDefinedBy rdf:resource="http://JP_ontology.org/assessment"/>
        <skos:altLabel xml:lang="en">MCQ.7</skos:altLabel>
        <skos:broader rdf:resource="http://JP_ontology.org/assessment/AssessmentQuestion"/>
        <skos:definition xml:lang="en">Are documented information and additional necessary documentation included in the organisation&apos;s information security management system according to the organisation&apos;s needs, considering factors such as its size, activities, processes, products, services, complexity of processes, interactions, and personnel competence?</skos:definition>
        <skos:prefLabel>Multiple Choice Question #7</skos:prefLabel>
    </rdf:Description>
    <rdf:Description rdf:about="http://JP_ontology.org/assessment/MCQ.70.1">
        <nis2v:hasAnswer rdf:resource="http://JP_ontology.org/assessment/MCQ70.1AnswerA"/>
        <nis2v:hasAnswer rdf:resource="http://JP_ontology.org/assessment/MCQ70.1AnswerB"/>
        <nis2v:hasAnswer rdf:resource="http://JP_ontology.org/assessment/MCQ70.1AnswerC"/>
        <nis2v:relatedToControl rdf:resource="http://JP_ontology.org/iso27001/Control7.2"/>
        <terms:contributor>Jenni Parry</terms:contributor>
        <terms:created rdf:datatype="http://www.w3.org/2001/XMLSchema#date">2024-04-18</terms:created>
        <terms:subject rdf:resource="http://JP_ontology.org/nis2v/Article_21.2i"/>
        <rdfs:isDefinedBy rdf:resource="http://JP_ontology.org/assessment"/>
        <skos:altLabel xml:lang="en">MCQ.70.1</skos:altLabel>
        <skos:broader rdf:resource="http://JP_ontology.org/assessment/AssessmentQuestion"/>
        <skos:definition xml:lang="en">Is the organisation determining the required competence of individuals performing work under its control that affects its information security performance?</skos:definition>
        <skos:prefLabel xml:lang="en">Multiple Choice Question #70.1</skos:prefLabel>
    </rdf:Description>
    <rdf:Description rdf:about="http://JP_ontology.org/assessment/MCQ.70.2">
        <nis2v:hasAnswer rdf:resource="http://JP_ontology.org/assessment/MCQ70.2AnswerA"/>
        <nis2v:hasAnswer rdf:resource="http://JP_ontology.org/assessment/MCQ70.2AnswerB"/>
        <nis2v:hasAnswer rdf:resource="http://JP_ontology.org/assessment/MCQ70.2AnswerC"/>
        <nis2v:relatedToControl rdf:resource="http://JP_ontology.org/iso27001/Control7.2"/>
        <terms:contributor>Jenni Parry</terms:contributor>
        <terms:created rdf:datatype="http://www.w3.org/2001/XMLSchema#date">2024-04-18</terms:created>
        <terms:subject rdf:resource="http://JP_ontology.org/nis2v/Article_21.2i"/>
        <rdfs:isDefinedBy rdf:resource="http://JP_ontology.org/assessment"/>
        <skos:altLabel xml:lang="en">MCQ.70.2</skos:altLabel>
        <skos:broader rdf:resource="http://JP_ontology.org/assessment/AssessmentQuestion"/>
        <skos:definition xml:lang="en">Is the organisation ensuring that these individuals possess the necessary competence through appropriate education, training, or experience?</skos:definition>
        <skos:prefLabel xml:lang="en">Multiple Choice Question #70.2</skos:prefLabel>
    </rdf:Description>
    <rdf:Description rdf:about="http://JP_ontology.org/assessment/MCQ.70.3">
        <nis2v:hasAnswer rdf:resource="http://JP_ontology.org/assessment/MCQ70.3AnswerA"/>
        <nis2v:hasAnswer rdf:resource="http://JP_ontology.org/assessment/MCQ70.3AnswerB"/>
        <nis2v:hasAnswer rdf:resource="http://JP_ontology.org/assessment/MCQ70.3AnswerC"/>
        <nis2v:relatedToControl rdf:resource="http://JP_ontology.org/iso27001/Control7.2"/>
        <terms:contributor>Jenni Parry</terms:contributor>
        <terms:created rdf:datatype="http://www.w3.org/2001/XMLSchema#date">2024-04-18</terms:created>
        <terms:subject rdf:resource="http://JP_ontology.org/nis2v/Article_21.2i"/>
        <rdfs:isDefinedBy rdf:resource="http://JP_ontology.org/assessment"/>
        <skos:altLabel xml:lang="en">MCQ.70.3</skos:altLabel>
        <skos:broader rdf:resource="http://JP_ontology.org/assessment/AssessmentQuestion"/>
        <skos:definition xml:lang="en">Is the organisation taking necessary actions, where applicable, to acquire the required competence and evaluating the effectiveness of these actions?</skos:definition>
        <skos:prefLabel xml:lang="en">Multiple Choice Question #70.3</skos:prefLabel>
    </rdf:Description>
    <rdf:Description rdf:about="http://JP_ontology.org/assessment/MCQ.70.4">
        <nis2v:hasAnswer rdf:resource="http://JP_ontology.org/assessment/MCQ70.4AnswerA"/>
        <nis2v:hasAnswer rdf:resource="http://JP_ontology.org/assessment/MCQ70.4AnswerB"/>
        <nis2v:hasAnswer rdf:resource="http://JP_ontology.org/assessment/MCQ70.4AnswerC"/>
        <nis2v:relatedToControl rdf:resource="http://JP_ontology.org/iso27001/Control7.2"/>
        <terms:contributor>Jenni Parry</terms:contributor>
        <terms:created rdf:datatype="http://www.w3.org/2001/XMLSchema#date">2024-04-18</terms:created>
        <terms:subject rdf:resource="http://JP_ontology.org/nis2v/Article_21.2i"/>
        <rdfs:isDefinedBy rdf:resource="http://JP_ontology.org/assessment"/>
        <skos:altLabel xml:lang="en">MCQ.70.4</skos:altLabel>
        <skos:broader rdf:resource="http://JP_ontology.org/assessment/AssessmentQuestion"/>
        <skos:definition xml:lang="en">Is the organisation retaining appropriate documented information as evidence of competence?</skos:definition>
        <skos:prefLabel xml:lang="en">Multiple Choice Question #70.4</skos:prefLabel>
    </rdf:Description>
    <rdf:Description rdf:about="http://JP_ontology.org/assessment/MCQ.71">
        <nis2v:hasAnswer rdf:resource="http://JP_ontology.org/assessment/MCQ.71AnswerA"/>
        <nis2v:hasAnswer rdf:resource="http://JP_ontology.org/assessment/MCQ.71AnswerB"/>
        <nis2v:hasAnswer rdf:resource="http://JP_ontology.org/assessment/MCQ.71AnswerC"/>
        <nis2v:relatedToControl rdf:resource="http://JP_ontology.org/iso27001/ControlA.5.2"/>
        <terms:contributor>Jenni Parry</terms:contributor>
        <terms:created rdf:datatype="http://www.w3.org/2001/XMLSchema#date">2024-05-20</terms:created>
        <terms:subject rdf:resource="http://JP_ontology.org/nis2v/Article_21.2i"/>
        <rdfs:isDefinedBy rdf:resource="http://JP_ontology.org/assessment"/>
        <skos:altLabel xml:lang="en">MCQ.71</skos:altLabel>
        <skos:broader rdf:resource="http://JP_ontology.org/assessment/AssessmentQuestion"/>
        <skos:definition xml:lang="en">Are information security roles and responsibilities defined and allocated according to the organisation&apos;s needs?</skos:definition>
        <skos:prefLabel xml:lang="en">Multiple Choice Question #71</skos:prefLabel>
    </rdf:Description>
    <rdf:Description rdf:about="http://JP_ontology.org/assessment/MCQ.72">
        <nis2v:hasAnswer rdf:resource="http://JP_ontology.org/assessment/MCQ72AnswerA"/>
        <nis2v:hasAnswer rdf:resource="http://JP_ontology.org/assessment/MCQ72AnswerB"/>
        <nis2v:hasAnswer rdf:resource="http://JP_ontology.org/assessment/MCQ72AnswerC"/>
        <nis2v:relatedToControl rdf:resource="http://JP_ontology.org/iso27001/ControlA.5.3"/>
        <terms:contributor>Jenni Parry</terms:contributor>
        <terms:created rdf:datatype="http://www.w3.org/2001/XMLSchema#date">2024-04-18</terms:created>
        <terms:subject rdf:resource="http://JP_ontology.org/nis2v/Article_21.2i"/>
        <rdfs:isDefinedBy rdf:resource="http://JP_ontology.org/assessment"/>
        <skos:altLabel xml:lang="en">MCQ.72</skos:altLabel>
        <skos:broader rdf:resource="http://JP_ontology.org/assessment/AssessmentQuestion"/>
        <skos:definition xml:lang="en">Are conflicting duties and conflicting areas of responsibility segregated?</skos:definition>
        <skos:prefLabel xml:lang="en">Multiple Choice Question #72</skos:prefLabel>
    </rdf:Description>
    <rdf:Description rdf:about="http://JP_ontology.org/assessment/MCQ.73">
        <nis2v:hasAnswer rdf:resource="http://JP_ontology.org/assessment/MCQ73AnswerA"/>
        <nis2v:hasAnswer rdf:resource="http://JP_ontology.org/assessment/MCQ73AnswerB"/>
        <nis2v:hasAnswer rdf:resource="http://JP_ontology.org/assessment/MCQ73AnswerC"/>
        <nis2v:relatedToControl rdf:resource="http://JP_ontology.org/iso27001/ControlA.6.1"/>
        <terms:contributor>Jenni Parry</terms:contributor>
        <terms:created rdf:datatype="http://www.w3.org/2001/XMLSchema#date">2024-04-18</terms:created>
        <terms:subject rdf:resource="http://JP_ontology.org/nis2v/Article_21.2i"/>
        <rdfs:isDefinedBy rdf:resource="http://JP_ontology.org/assessment"/>
        <skos:altLabel xml:lang="en">MCQ.73</skos:altLabel>
        <skos:broader rdf:resource="http://JP_ontology.org/assessment/AssessmentQuestion"/>
        <skos:definition xml:lang="en">Are background verification checks conducted on all candidates to become personnel prior to joining the organisation and on an ongoing basis, taking into consideration applicable laws, regulations, and ethics, and being proportional to the business requirements, the classification of the information to be accessed, and the perceived risks?</skos:definition>
        <skos:prefLabel xml:lang="en">Multiple Choice Question #73</skos:prefLabel>
    </rdf:Description>
    <rdf:Description rdf:about="http://JP_ontology.org/assessment/MCQ.74">
        <nis2v:hasAnswer rdf:resource="http://JP_ontology.org/assessment/MCQ74AnswerA"/>
        <nis2v:hasAnswer rdf:resource="http://JP_ontology.org/assessment/MCQ74AnswerB"/>
        <nis2v:hasAnswer rdf:resource="http://JP_ontology.org/assessment/MCQ74AnswerC"/>
        <nis2v:relatedToControl rdf:resource="http://JP_ontology.org/iso27001/ControlA.6.2"/>
        <terms:contributor>Jenni Parry</terms:contributor>
        <terms:created rdf:datatype="http://www.w3.org/2001/XMLSchema#date">2024-04-18</terms:created>
        <terms:subject rdf:resource="http://JP_ontology.org/nis2v/Article_21.2i"/>
        <rdfs:isDefinedBy rdf:resource="http://JP_ontology.org/assessment"/>
        <skos:altLabel xml:lang="en">MCQ.74</skos:altLabel>
        <skos:broader rdf:resource="http://JP_ontology.org/assessment/AssessmentQuestion"/>
        <skos:definition xml:lang="en">Do the employment contractual agreements state the personnel’s and the organisation’s responsibilities for information security?</skos:definition>
        <skos:prefLabel xml:lang="en">Multiple Choice Question #74</skos:prefLabel>
    </rdf:Description>
    <rdf:Description rdf:about="http://JP_ontology.org/assessment/MCQ.75.1">
        <nis2v:hasAnswer rdf:resource="http://JP_ontology.org/assessment/MCQ.75.1AnswerA"/>
        <nis2v:hasAnswer rdf:resource="http://JP_ontology.org/assessment/MCQ.75.1AnswerB"/>
        <nis2v:hasAnswer rdf:resource="http://JP_ontology.org/assessment/MCQ.75.1AnswerC"/>
        <nis2v:relatedToControl rdf:resource="http://JP_ontology.org/iso27001/ControlA.6.3"/>
        <terms:contributor>Jenni Parry</terms:contributor>
        <terms:created rdf:datatype="http://www.w3.org/2001/XMLSchema#date">2024-05-20</terms:created>
        <terms:subject rdf:resource="http://JP_ontology.org/nis2v/Article_21.2i"/>
        <rdfs:isDefinedBy rdf:resource="http://JP_ontology.org/assessment"/>
        <skos:altLabel xml:lang="en">MCQ.75.1</skos:altLabel>
        <skos:broader rdf:resource="http://JP_ontology.org/assessment/AssessmentQuestion"/>
        <skos:definition xml:lang="en">Do personnel of the organisation and relevant interested parties receive appropriate information security awareness, education, and training?</skos:definition>
        <skos:prefLabel xml:lang="en">Multiple Choice Question #75.1</skos:prefLabel>
    </rdf:Description>
    <rdf:Description rdf:about="http://JP_ontology.org/assessment/MCQ.75.2">
        <nis2v:hasAnswer rdf:resource="http://JP_ontology.org/assessment/MCQ.75.2AnswerA"/>
        <nis2v:hasAnswer rdf:resource="http://JP_ontology.org/assessment/MCQ.75.2AnswerB"/>
        <nis2v:hasAnswer rdf:resource="http://JP_ontology.org/assessment/MCQ.75.2AnswerC"/>
        <nis2v:relatedToControl rdf:resource="http://JP_ontology.org/iso27001/ControlA.6.3"/>
        <terms:contributor>Jenni Parry</terms:contributor>
        <terms:created rdf:datatype="http://www.w3.org/2001/XMLSchema#date">2024-05-20</terms:created>
        <terms:subject rdf:resource="http://JP_ontology.org/nis2v/Article_21.2i"/>
        <rdfs:isDefinedBy rdf:resource="http://JP_ontology.org/assessment"/>
        <skos:altLabel xml:lang="en">MCQ.75.2</skos:altLabel>
        <skos:broader rdf:resource="http://JP_ontology.org/assessment/AssessmentQuestion"/>
        <skos:definition xml:lang="en">Are regular updates of the organisation&apos;s information security policy, topic-specific policies, and procedures relevant to their job function provided to personnel of the organisation and relevant interested parties?</skos:definition>
        <skos:prefLabel xml:lang="en">Multiple Choice Question #75.2</skos:prefLabel>
    </rdf:Description>
    <rdf:Description rdf:about="http://JP_ontology.org/assessment/MCQ.76">
        <nis2v:hasAnswer rdf:resource="http://JP_ontology.org/assessment/MCQ.76AnswerA"/>
        <nis2v:hasAnswer rdf:resource="http://JP_ontology.org/assessment/MCQ.76AnswerB"/>
        <nis2v:hasAnswer rdf:resource="http://JP_ontology.org/assessment/MCQ.76AnswerC"/>
        <nis2v:relatedToControl rdf:resource="http://JP_ontology.org/iso27001/ControlA.6.4"/>
        <terms:contributor>Jenni Parry</terms:contributor>
        <terms:created rdf:datatype="http://www.w3.org/2001/XMLSchema#date">2024-05-20</terms:created>
        <terms:subject rdf:resource="http://JP_ontology.org/nis2v/Article_21.2i"/>
        <rdfs:isDefinedBy rdf:resource="http://JP_ontology.org/assessment"/>
        <skos:altLabel xml:lang="en">MCQ.76</skos:altLabel>
        <skos:broader rdf:resource="http://JP_ontology.org/assessment/AssessmentQuestion"/>
        <skos:definition xml:lang="en">Is a disciplinary process formalized and communicated to take actions against personnel and other relevant interested parties who have committed an information security policy violation?</skos:definition>
        <skos:prefLabel xml:lang="en">Multiple Choice Question #76</skos:prefLabel>
    </rdf:Description>
    <rdf:Description rdf:about="http://JP_ontology.org/assessment/MCQ.77">
        <nis2v:hasAnswer rdf:resource="http://JP_ontology.org/assessment/MCQ77AnswerA"/>
        <nis2v:hasAnswer rdf:resource="http://JP_ontology.org/assessment/MCQ77AnswerB"/>
        <nis2v:hasAnswer rdf:resource="http://JP_ontology.org/assessment/MCQ77AnswerC"/>
        <nis2v:relatedToControl rdf:resource="http://JP_ontology.org/iso27001/ControlA.6.5"/>
        <terms:contributor>Jenni Parry</terms:contributor>
        <terms:created rdf:datatype="http://www.w3.org/2001/XMLSchema#date">2024-04-18</terms:created>
        <terms:subject rdf:resource="http://JP_ontology.org/nis2v/Article_21.2i"/>
        <rdfs:isDefinedBy rdf:resource="http://JP_ontology.org/assessment"/>
        <skos:altLabel xml:lang="en">MCQ.77</skos:altLabel>
        <skos:broader rdf:resource="http://JP_ontology.org/assessment/AssessmentQuestion"/>
        <skos:definition xml:lang="en">Are information security responsibilities and duties that remain valid after termination or change of employment defined, enforced, and communicated to relevant personnel and other interested parties?</skos:definition>
        <skos:prefLabel xml:lang="en">Multiple Choice Question #77</skos:prefLabel>
    </rdf:Description>
    <rdf:Description rdf:about="http://JP_ontology.org/assessment/MCQ.78">
        <nis2v:hasAnswer rdf:resource="http://JP_ontology.org/assessment/MCQ.78AnswerA"/>
        <nis2v:hasAnswer rdf:resource="http://JP_ontology.org/assessment/MCQ.78AnswerB"/>
        <nis2v:hasAnswer rdf:resource="http://JP_ontology.org/assessment/MCQ.78AnswerC"/>
        <nis2v:relatedToControl rdf:resource="http://JP_ontology.org/iso27001/ControlA.6.6"/>
        <terms:contributor>Jenni Parry</terms:contributor>
        <terms:created rdf:datatype="http://www.w3.org/2001/XMLSchema#date">2024-05-20</terms:created>
        <terms:subject rdf:resource="http://JP_ontology.org/nis2v/Article_21.2i"/>
        <rdfs:isDefinedBy rdf:resource="http://JP_ontology.org/assessment"/>
        <skos:altLabel xml:lang="en">MCQ.78</skos:altLabel>
        <skos:broader rdf:resource="http://JP_ontology.org/assessment/AssessmentQuestion"/>
        <skos:definition xml:lang="en">Are confidentiality or non-disclosure agreements reflecting the organisation&apos;s needs for the protection of information identified, documented, regularly reviewed, and signed by personnel and other relevant interested parties?</skos:definition>
        <skos:prefLabel xml:lang="en">Multiple Choice Question #78</skos:prefLabel>
    </rdf:Description>
    <rdf:Description rdf:about="http://JP_ontology.org/assessment/MCQ.79">
        <nis2v:hasAnswer rdf:resource="http://JP_ontology.org/assessment/MCQ.79AnswerA"/>
        <nis2v:hasAnswer rdf:resource="http://JP_ontology.org/assessment/MCQ.79AnswerB"/>
        <nis2v:hasAnswer rdf:resource="http://JP_ontology.org/assessment/MCQ.79AnswerC"/>
        <nis2v:relatedToControl rdf:resource="http://JP_ontology.org/iso27001/ControlA.6.7"/>
        <terms:contributor>Jenni Parry</terms:contributor>
        <terms:created rdf:datatype="http://www.w3.org/2001/XMLSchema#date">2024-05-20</terms:created>
        <terms:subject rdf:resource="http://JP_ontology.org/nis2v/Article_21.2i"/>
        <rdfs:isDefinedBy rdf:resource="http://JP_ontology.org/assessment"/>
        <skos:altLabel xml:lang="en">MCQ.79</skos:altLabel>
        <skos:broader rdf:resource="http://JP_ontology.org/assessment/AssessmentQuestion"/>
        <skos:definition xml:lang="en">Are security measures implemented when personnel are working remotely to protect information accessed, processed, or stored outside the organisation’s premises?</skos:definition>
        <skos:prefLabel xml:lang="en">Multiple Choice Question #79</skos:prefLabel>
    </rdf:Description>
    <rdf:Description rdf:about="http://JP_ontology.org/assessment/MCQ.8.1">
        <nis2v:hasAnswer rdf:resource="http://JP_ontology.org/assessment/MCQ.8.1AnswerA"/>
        <nis2v:hasAnswer rdf:resource="http://JP_ontology.org/assessment/MCQ.8.1AnswerB"/>
        <nis2v:hasAnswer rdf:resource="http://JP_ontology.org/assessment/MCQ.8.1AnswerC"/>
        <nis2v:relatedToControl rdf:resource="http://JP_ontology.org/iso27001/Control8.2"/>
        <terms:contributor>Jenni Parry</terms:contributor>
        <terms:created rdf:datatype="http://www.w3.org/2001/XMLSchema#date">2024-05-20</terms:created>
        <terms:subject rdf:resource="http://JP_ontology.org/nis2v/Article_21.2a"/>
        <rdfs:isDefinedBy rdf:resource="http://JP_ontology.org/assessment"/>
        <skos:altLabel xml:lang="en">MCQ.8.1</skos:altLabel>
        <skos:broader rdf:resource="http://JP_ontology.org/assessment/AssessmentQuestion"/>
        <skos:definition xml:lang="en">Does the organisation conduct information security risk assessments at planned intervals or when significant changes are proposed or occur? </skos:definition>
        <skos:prefLabel xml:lang="en">Multiple Choice Question #8.1</skos:prefLabel>
    </rdf:Description>
    <rdf:Description rdf:about="http://JP_ontology.org/assessment/MCQ.8.2">
        <nis2v:hasAnswer rdf:resource="http://JP_ontology.org/assessment/MCQ.8.2AnswerA"/>
        <nis2v:hasAnswer rdf:resource="http://JP_ontology.org/assessment/MCQ.8.2AnswerB"/>
        <nis2v:hasAnswer rdf:resource="http://JP_ontology.org/assessment/MCQ.8.2AnswerC"/>
        <nis2v:relatedToControl rdf:resource="http://JP_ontology.org/iso27001/Control8.2"/>
        <terms:contributor>Jenni Parry</terms:contributor>
        <terms:created rdf:datatype="http://www.w3.org/2001/XMLSchema#date">2024-05-20</terms:created>
        <terms:subject rdf:resource="http://JP_ontology.org/nis2v/Article_21.2a"/>
        <rdfs:isDefinedBy rdf:resource="http://JP_ontology.org/assessment"/>
        <skos:altLabel xml:lang="en">MCQ.8.2</skos:altLabel>
        <skos:broader rdf:resource="http://JP_ontology.org/assessment/AssessmentQuestion"/>
        <skos:definition xml:lang="en">Does the organisation retain documented information of the results of these assessments?</skos:definition>
        <skos:prefLabel xml:lang="en">Multiple Choice Question #8.2</skos:prefLabel>
    </rdf:Description>
    <rdf:Description rdf:about="http://JP_ontology.org/assessment/MCQ.80">
        <nis2v:hasAnswer rdf:resource="http://JP_ontology.org/assessment/MCQ.80AnswerA"/>
        <nis2v:hasAnswer rdf:resource="http://JP_ontology.org/assessment/MCQ.80AnswerB"/>
        <nis2v:hasAnswer rdf:resource="http://JP_ontology.org/assessment/MCQ.80AnswerC"/>
        <nis2v:relatedToControl rdf:resource="http://JP_ontology.org/iso27001/ControlA.5.15"/>
        <terms:contributor>Jenni Parry</terms:contributor>
        <terms:created rdf:datatype="http://www.w3.org/2001/XMLSchema#date">2024-05-20</terms:created>
        <terms:subject rdf:resource="http://JP_ontology.org/nis2v/Article_21.2i"/>
        <rdfs:isDefinedBy rdf:resource="http://JP_ontology.org/assessment"/>
        <skos:altLabel xml:lang="en">MCQ.80</skos:altLabel>
        <skos:broader rdf:resource="http://JP_ontology.org/assessment/AssessmentQuestion"/>
        <skos:definition xml:lang="en">Are rules established and implemented to control physical and logical access to information and other associated assets, based on business and information security requirements?</skos:definition>
        <skos:prefLabel xml:lang="en">Multiple Choice Question #80</skos:prefLabel>
    </rdf:Description>
    <rdf:Description rdf:about="http://JP_ontology.org/assessment/MCQ.81">
        <nis2v:hasAnswer rdf:resource="http://JP_ontology.org/assessment/MCQ.81AnswerA"/>
        <nis2v:hasAnswer rdf:resource="http://JP_ontology.org/assessment/MCQ.81AnswerB"/>
        <nis2v:hasAnswer rdf:resource="http://JP_ontology.org/assessment/MCQ.81AnswerC"/>
        <nis2v:relatedToControl rdf:resource="http://JP_ontology.org/iso27001/ControlA.5.16"/>
        <terms:contributor>Jenni Parry</terms:contributor>
        <terms:created rdf:datatype="http://www.w3.org/2001/XMLSchema#date">2024-05-20</terms:created>
        <terms:subject rdf:resource="http://JP_ontology.org/nis2v/Article_21.2i"/>
        <rdfs:isDefinedBy rdf:resource="http://JP_ontology.org/assessment"/>
        <skos:altLabel xml:lang="en">MCQ.81</skos:altLabel>
        <skos:broader rdf:resource="http://JP_ontology.org/assessment/AssessmentQuestion"/>
        <skos:definition xml:lang="en">Is the organisation managing the complete life cycle of identities, encompassing activities such as identity creation, authentication, authorization, periodic reviews, modification, and termination, ensuring comprehensive oversight and control over identity-related processes?</skos:definition>
        <skos:prefLabel xml:lang="en">Multiple Choice Question #81</skos:prefLabel>
    </rdf:Description>
    <rdf:Description rdf:about="http://JP_ontology.org/assessment/MCQ.82">
        <nis2v:hasAnswer rdf:resource="http://JP_ontology.org/assessment/MCQ.82AnswerA"/>
        <nis2v:hasAnswer rdf:resource="http://JP_ontology.org/assessment/MCQ.82AnswerB"/>
        <nis2v:hasAnswer rdf:resource="http://JP_ontology.org/assessment/MCQ.82AnswerC"/>
        <nis2v:relatedToControl rdf:resource="http://JP_ontology.org/iso27001/ControlA.5.17"/>
        <terms:contributor>Jenni Parry</terms:contributor>
        <terms:created rdf:datatype="http://www.w3.org/2001/XMLSchema#date">2024-05-20</terms:created>
        <terms:subject rdf:resource="http://JP_ontology.org/nis2v/Article_21.2i"/>
        <rdfs:isDefinedBy rdf:resource="http://JP_ontology.org/assessment"/>
        <skos:altLabel xml:lang="en">MCQ.82</skos:altLabel>
        <skos:broader rdf:resource="http://JP_ontology.org/assessment/AssessmentQuestion"/>
        <skos:definition xml:lang="en">Is the allocation and management of authentication information controlled by a management process, which includes advising personnel on the appropriate handling of authentication information?</skos:definition>
        <skos:prefLabel xml:lang="en">Multiple Choice Question #82</skos:prefLabel>
    </rdf:Description>
    <rdf:Description rdf:about="http://JP_ontology.org/assessment/MCQ.83">
        <nis2v:hasAnswer rdf:resource="http://JP_ontology.org/assessment/MCQ.83AnswerA"/>
        <nis2v:hasAnswer rdf:resource="http://JP_ontology.org/assessment/MCQ.83AnswerB"/>
        <nis2v:hasAnswer rdf:resource="http://JP_ontology.org/assessment/MCQ.83AnswerC"/>
        <nis2v:relatedToControl rdf:resource="http://JP_ontology.org/iso27001/ControlA.5.18"/>
        <terms:contributor>Jenni Parry</terms:contributor>
        <terms:created rdf:datatype="http://www.w3.org/2001/XMLSchema#date">2024-05-20</terms:created>
        <terms:subject rdf:resource="http://JP_ontology.org/nis2v/Article_21.2i"/>
        <rdfs:isDefinedBy rdf:resource="http://JP_ontology.org/assessment"/>
        <skos:altLabel xml:lang="en">MCQ.83</skos:altLabel>
        <skos:broader rdf:resource="http://JP_ontology.org/assessment/AssessmentQuestion"/>
        <skos:definition xml:lang="en">Are access rights to information and other associated assets provisioned, reviewed, modified, and removed in accordance with the organisation’s topic-specific policy and rules for access control?</skos:definition>
        <skos:prefLabel xml:lang="en">Multiple Choice Question #83</skos:prefLabel>
    </rdf:Description>
    <rdf:Description rdf:about="http://JP_ontology.org/assessment/MCQ.84">
        <nis2v:hasAnswer rdf:resource="http://JP_ontology.org/assessment/MCQ.84AnswerA"/>
        <nis2v:hasAnswer rdf:resource="http://JP_ontology.org/assessment/MCQ.84AnswerB"/>
        <nis2v:hasAnswer rdf:resource="http://JP_ontology.org/assessment/MCQ.84AnswerC"/>
        <nis2v:relatedToControl rdf:resource="http://JP_ontology.org/iso27001/ControlA.8.2"/>
        <terms:contributor>Jenni Parry</terms:contributor>
        <terms:created rdf:datatype="http://www.w3.org/2001/XMLSchema#date">2024-05-20</terms:created>
        <terms:subject rdf:resource="http://JP_ontology.org/nis2v/Article_21.2i"/>
        <rdfs:isDefinedBy rdf:resource="http://JP_ontology.org/assessment"/>
        <skos:altLabel xml:lang="en">MCQ.84</skos:altLabel>
        <skos:broader rdf:resource="http://JP_ontology.org/assessment/AssessmentQuestion"/>
        <skos:definition xml:lang="en">Are the allocation and use of privileged access rights restricted and managed?</skos:definition>
        <skos:prefLabel xml:lang="en">Multiple Choice Question #84</skos:prefLabel>
    </rdf:Description>
    <rdf:Description rdf:about="http://JP_ontology.org/assessment/MCQ.85">
        <nis2v:hasAnswer rdf:resource="http://JP_ontology.org/assessment/MCQ.85AnswerA"/>
        <nis2v:hasAnswer rdf:resource="http://JP_ontology.org/assessment/MCQ.85AnswerB"/>
        <nis2v:hasAnswer rdf:resource="http://JP_ontology.org/assessment/MCQ.85AnswerC"/>
        <nis2v:relatedToControl rdf:resource="http://JP_ontology.org/iso27001/ControlA.8.3"/>
        <terms:contributor>Jenni Parry</terms:contributor>
        <terms:created rdf:datatype="http://www.w3.org/2001/XMLSchema#date">2024-05-20</terms:created>
        <terms:subject rdf:resource="http://JP_ontology.org/nis2v/Article_21.2i"/>
        <rdfs:isDefinedBy rdf:resource="http://JP_ontology.org/assessment"/>
        <skos:altLabel xml:lang="en">MCQ.85</skos:altLabel>
        <skos:broader rdf:resource="http://JP_ontology.org/assessment/AssessmentQuestion"/>
        <skos:definition xml:lang="en">Is access to information and other associated assets restricted in accordance with the established topic-specific policy on access control?</skos:definition>
        <skos:prefLabel xml:lang="en">Multiple Choice Question #85</skos:prefLabel>
    </rdf:Description>
    <rdf:Description rdf:about="http://JP_ontology.org/assessment/MCQ.86">
        <nis2v:hasAnswer rdf:resource="http://JP_ontology.org/assessment/MCQ.86AnswerA"/>
        <nis2v:hasAnswer rdf:resource="http://JP_ontology.org/assessment/MCQ.86AnswerB"/>
        <nis2v:hasAnswer rdf:resource="http://JP_ontology.org/assessment/MCQ.86AnswerC"/>
        <nis2v:relatedToControl rdf:resource="http://JP_ontology.org/iso27001/ControlA.8.4"/>
        <terms:contributor>Jenni Parry</terms:contributor>
        <terms:created rdf:datatype="http://www.w3.org/2001/XMLSchema#date">2024-05-20</terms:created>
        <terms:subject rdf:resource="http://JP_ontology.org/nis2v/Article_21.2i"/>
        <rdfs:isDefinedBy rdf:resource="http://JP_ontology.org/assessment"/>
        <skos:altLabel xml:lang="en">MCQ.86</skos:altLabel>
        <skos:broader rdf:resource="http://JP_ontology.org/assessment/AssessmentQuestion"/>
        <skos:definition xml:lang="en">Is read and write access to source code, development tools, and software libraries appropriately managed?</skos:definition>
        <skos:prefLabel xml:lang="en">Multiple Choice Question #86</skos:prefLabel>
    </rdf:Description>
    <rdf:Description rdf:about="http://JP_ontology.org/assessment/MCQ.87">
        <nis2v:hasAnswer rdf:resource="http://JP_ontology.org/assessment/MCQ.87AnswerA"/>
        <nis2v:hasAnswer rdf:resource="http://JP_ontology.org/assessment/MCQ.87AnswerB"/>
        <nis2v:hasAnswer rdf:resource="http://JP_ontology.org/assessment/MCQ.87AnswerC"/>
        <nis2v:relatedToControl rdf:resource="http://JP_ontology.org/iso27001/ControlA.8.5"/>
        <terms:contributor>Jenni Parry</terms:contributor>
        <terms:created rdf:datatype="http://www.w3.org/2001/XMLSchema#date">2024-05-20</terms:created>
        <terms:subject rdf:resource="http://JP_ontology.org/nis2v/Article_21.2i"/>
        <rdfs:isDefinedBy rdf:resource="http://JP_ontology.org/assessment"/>
        <skos:altLabel xml:lang="en">MCQ.87</skos:altLabel>
        <skos:broader rdf:resource="http://JP_ontology.org/assessment/AssessmentQuestion"/>
        <skos:definition xml:lang="en">Are secure authentication technologies and procedures implemented based on information access restrictions and the topic-specific policy on access control?</skos:definition>
        <skos:prefLabel xml:lang="en">Multiple Choice Question #87</skos:prefLabel>
    </rdf:Description>
    <rdf:Description rdf:about="http://JP_ontology.org/assessment/MCQ.88">
        <nis2v:hasAnswer rdf:resource="http://JP_ontology.org/assessment/MCQ.88AnswerA"/>
        <nis2v:hasAnswer rdf:resource="http://JP_ontology.org/assessment/MCQ.88AnswerB"/>
        <nis2v:hasAnswer rdf:resource="http://JP_ontology.org/assessment/MCQ.88AnswerC"/>
        <nis2v:relatedToControl rdf:resource="http://JP_ontology.org/iso27001/ControlA.8.18"/>
        <terms:contributor>Jenni Parry</terms:contributor>
        <terms:created rdf:datatype="http://www.w3.org/2001/XMLSchema#date">2024-05-20</terms:created>
        <terms:subject rdf:resource="http://JP_ontology.org/nis2v/Article_21.2i"/>
        <rdfs:isDefinedBy rdf:resource="http://JP_ontology.org/assessment"/>
        <skos:altLabel xml:lang="en">MCQ.88</skos:altLabel>
        <skos:broader rdf:resource="http://JP_ontology.org/assessment/AssessmentQuestion"/>
        <skos:definition xml:lang="en">Is the use of utility programs capable of overriding system and application controls restricted and tightly controlled?</skos:definition>
        <skos:prefLabel xml:lang="en">Multiple Choice Question #88</skos:prefLabel>
    </rdf:Description>
    <rdf:Description rdf:about="http://JP_ontology.org/assessment/MCQ.89">
        <nis2v:hasAnswer rdf:resource="http://JP_ontology.org/assessment/MCQ.89AnswerA"/>
        <nis2v:hasAnswer rdf:resource="http://JP_ontology.org/assessment/MCQ.89AnswerB"/>
        <nis2v:hasAnswer rdf:resource="http://JP_ontology.org/assessment/MCQ.89AnswerC"/>
        <nis2v:relatedToControl rdf:resource="http://JP_ontology.org/iso27001/ControlA.5.9"/>
        <terms:contributor>Jenni Parry</terms:contributor>
        <terms:created rdf:datatype="http://www.w3.org/2001/XMLSchema#date">2024-05-20</terms:created>
        <terms:subject rdf:resource="http://JP_ontology.org/nis2v/Article_21.2i"/>
        <rdfs:isDefinedBy rdf:resource="http://JP_ontology.org/assessment"/>
        <skos:altLabel xml:lang="en">MCQ.89</skos:altLabel>
        <skos:broader rdf:resource="http://JP_ontology.org/assessment/AssessmentQuestion"/>
        <skos:definition xml:lang="en">Is an inventory of information and other associated assets, including owners, developed and maintained?</skos:definition>
        <skos:prefLabel xml:lang="en">Multiple Choice Question #89</skos:prefLabel>
    </rdf:Description>
    <rdf:Description rdf:about="http://JP_ontology.org/assessment/MCQ.9.1">
        <nis2v:hasAnswer rdf:resource="http://JP_ontology.org/assessment/MCQ.9.1AnswerA"/>
        <nis2v:hasAnswer rdf:resource="http://JP_ontology.org/assessment/MCQ.9.1AnswerB"/>
        <nis2v:hasAnswer rdf:resource="http://JP_ontology.org/assessment/MCQ.9.1AnswerC"/>
        <nis2v:relatedToControl rdf:resource="http://JP_ontology.org/iso27001/Control8.3"/>
        <terms:contributor>Jenni Parry</terms:contributor>
        <terms:created rdf:datatype="http://www.w3.org/2001/XMLSchema#date">2024-05-20</terms:created>
        <terms:subject rdf:resource="http://JP_ontology.org/nis2v/Article_21.2a"/>
        <rdfs:isDefinedBy rdf:resource="http://JP_ontology.org/assessment"/>
        <skos:altLabel xml:lang="en">MCQ.9.1</skos:altLabel>
        <skos:broader rdf:resource="http://JP_ontology.org/assessment/AssessmentQuestion"/>
        <skos:definition xml:lang="en">Does the organisation implement the information security risk treatment plan? </skos:definition>
        <skos:prefLabel xml:lang="en">Multiple Choice Question #9.1</skos:prefLabel>
    </rdf:Description>
    <rdf:Description rdf:about="http://JP_ontology.org/assessment/MCQ.9.2">
        <nis2v:hasAnswer rdf:resource="http://JP_ontology.org/assessment/MCQ.9.2AnswerA"/>
        <nis2v:hasAnswer rdf:resource="http://JP_ontology.org/assessment/MCQ.9.2AnswerB"/>
        <nis2v:hasAnswer rdf:resource="http://JP_ontology.org/assessment/MCQ.9.2AnswerC"/>
        <nis2v:relatedToControl rdf:resource="http://JP_ontology.org/iso27001/Control8.3"/>
        <terms:contributor>Jenni Parry</terms:contributor>
        <terms:created rdf:datatype="http://www.w3.org/2001/XMLSchema#date">2024-05-20</terms:created>
        <terms:subject rdf:resource="http://JP_ontology.org/nis2v/Article_21.2a"/>
        <rdfs:isDefinedBy rdf:resource="http://JP_ontology.org/assessment"/>
        <skos:altLabel xml:lang="en">MCQ.9.2</skos:altLabel>
        <skos:broader rdf:resource="http://JP_ontology.org/assessment/AssessmentQuestion"/>
        <skos:definition xml:lang="en">Does the organisation retain documented information of the results of the information security risk treatment?</skos:definition>
        <skos:prefLabel xml:lang="en">Multiple Choice Question #9.2</skos:prefLabel>
    </rdf:Description>
    <rdf:Description rdf:about="http://JP_ontology.org/assessment/MCQ.90">
        <nis2v:hasAnswer rdf:resource="http://JP_ontology.org/assessment/MCQ.90AnswerA"/>
        <nis2v:hasAnswer rdf:resource="http://JP_ontology.org/assessment/MCQ.90AnswerB"/>
        <nis2v:hasAnswer rdf:resource="http://JP_ontology.org/assessment/MCQ.90AnswerC"/>
        <nis2v:relatedToControl rdf:resource="http://JP_ontology.org/iso27001/ControlA.5.10"/>
        <terms:contributor>Jenni Parry</terms:contributor>
        <terms:created rdf:datatype="http://www.w3.org/2001/XMLSchema#date">2024-05-20</terms:created>
        <terms:subject rdf:resource="http://JP_ontology.org/nis2v/Article_21.2i"/>
        <rdfs:isDefinedBy rdf:resource="http://JP_ontology.org/assessment"/>
        <skos:altLabel xml:lang="en">MCQ.90</skos:altLabel>
        <skos:broader rdf:resource="http://JP_ontology.org/assessment/AssessmentQuestion"/>
        <skos:definition xml:lang="en">Are rules for acceptable use and procedures for handling information and other associated assets identified, documented, and implemented?</skos:definition>
        <skos:prefLabel xml:lang="en">Multiple Choice Question #90</skos:prefLabel>
    </rdf:Description>
    <rdf:Description rdf:about="http://JP_ontology.org/assessment/MCQ.91.1">
        <nis2v:hasAnswer rdf:resource="http://JP_ontology.org/assessment/MCQ91.1AnswerA"/>
        <nis2v:hasAnswer rdf:resource="http://JP_ontology.org/assessment/MCQ91.1AnswerB"/>
        <nis2v:hasAnswer rdf:resource="http://JP_ontology.org/assessment/MCQ91.1AnswerC"/>
        <nis2v:relatedToControl rdf:resource="http://JP_ontology.org/iso27001/ControlA.5.11"/>
        <terms:contributor>Jenni Parry</terms:contributor>
        <terms:created rdf:datatype="http://www.w3.org/2001/XMLSchema#date">2024-04-18</terms:created>
        <terms:subject rdf:resource="http://JP_ontology.org/nis2v/Article_21.2i"/>
        <rdfs:isDefinedBy rdf:resource="http://JP_ontology.org/assessment"/>
        <skos:altLabel xml:lang="en">MCQ.91.1</skos:altLabel>
        <skos:broader rdf:resource="http://JP_ontology.org/assessment/AssessmentQuestion"/>
        <skos:definition xml:lang="en">Are personnel and other relevant parties required to return all of the organisation&apos;s assets in their possession upon the change or termination of their employment, contract, or agreement?</skos:definition>
        <skos:prefLabel xml:lang="en">Multiple Choice Question #91.1</skos:prefLabel>
    </rdf:Description>
    <rdf:Description rdf:about="http://JP_ontology.org/assessment/MCQ.91.2">
        <nis2v:hasAnswer rdf:resource="http://JP_ontology.org/assessment/MCQ.91.2AnswerA"/>
        <nis2v:hasAnswer rdf:resource="http://JP_ontology.org/assessment/MCQ.91.2AnswerB"/>
        <nis2v:hasAnswer rdf:resource="http://JP_ontology.org/assessment/MCQ.91.2AnswerC"/>
        <nis2v:hasAnswer rdf:resource="http://JP_ontology.org/assessment/MCQ91.2AnswerA"/>
        <nis2v:hasAnswer rdf:resource="http://JP_ontology.org/assessment/MCQ91.2AnswerB"/>
        <nis2v:hasAnswer rdf:resource="http://JP_ontology.org/assessment/MCQ91.2AnswerC"/>
        <nis2v:relatedToControl rdf:resource="http://JP_ontology.org/iso27001/ControlA.7.9"/>
        <terms:contributor>Jenni Parry</terms:contributor>
        <terms:created rdf:datatype="http://www.w3.org/2001/XMLSchema#date">2024-04-18</terms:created>
        <terms:created rdf:datatype="http://www.w3.org/2001/XMLSchema#date">2024-05-20</terms:created>
        <terms:subject rdf:resource="http://JP_ontology.org/nis2v/Article_21.2i"/>
        <terms:subject rdf:resource="http://JP_ontology.org/nis2v/Article__21.2i"/>
        <rdfs:isDefinedBy rdf:resource="http://JP_ontology.org/assessment"/>
        <skos:altLabel xml:lang="en">MCQ.91.2</skos:altLabel>
        <skos:broader rdf:resource="http://JP_ontology.org/assessment/AssessmentQuestion"/>
        <skos:definition xml:lang="en">Are measures implemented to ensure the protection of off-site assets, safeguarding them from unauthorized access, theft, damage, or other risks that may compromise their integrity, confidentiality, or availability?</skos:definition>
        <skos:prefLabel xml:lang="en">Multiple Choice Question #91.2</skos:prefLabel>
    </rdf:Description>
    <rdf:Description rdf:about="http://JP_ontology.org/assessment/MCQ.92">
        <nis2v:hasAnswer rdf:resource="http://JP_ontology.org/assessment/MCQ.92AnswerA"/>
        <nis2v:hasAnswer rdf:resource="http://JP_ontology.org/assessment/MCQ.92AnswerB"/>
        <nis2v:hasAnswer rdf:resource="http://JP_ontology.org/assessment/MCQ.92AnswerC"/>
        <nis2v:relatedToControl rdf:resource="http://JP_ontology.org/iso27001/ControlA.7.10"/>
        <terms:contributor>Jenni Parry</terms:contributor>
        <terms:created rdf:datatype="http://www.w3.org/2001/XMLSchema#date">2024-05-20</terms:created>
        <terms:subject rdf:resource="http://JP_ontology.org/nis2v/Article_21.2i"/>
        <rdfs:isDefinedBy rdf:resource="http://JP_ontology.org/assessment"/>
        <skos:altLabel xml:lang="en">MCQ.92</skos:altLabel>
        <skos:broader rdf:resource="http://JP_ontology.org/assessment/AssessmentQuestion"/>
        <skos:definition xml:lang="en">Is storage media managed through their life cycle of acquisition, use, transportation, and disposal in accordance with the organisation’s classification scheme and handling requirements?</skos:definition>
        <skos:prefLabel xml:lang="en">Multiple Choice Question #92</skos:prefLabel>
    </rdf:Description>
    <rdf:Description rdf:about="http://JP_ontology.org/assessment/MCQ.93">
        <nis2v:hasAnswer rdf:resource="http://JP_ontology.org/assessment/MCQ.93AnswerA"/>
        <nis2v:hasAnswer rdf:resource="http://JP_ontology.org/assessment/MCQ.93AnswerB"/>
        <nis2v:hasAnswer rdf:resource="http://JP_ontology.org/assessment/MCQ.93AnswerC"/>
        <nis2v:relatedToControl rdf:resource="http://JP_ontology.org/iso27001/ControlA.7.14"/>
        <terms:contributor>Jenni Parry</terms:contributor>
        <terms:created rdf:datatype="http://www.w3.org/2001/XMLSchema#date">2024-05-20</terms:created>
        <terms:subject rdf:resource="http://JP_ontology.org/nis2v/Article_21.2i"/>
        <rdfs:isDefinedBy rdf:resource="http://JP_ontology.org/assessment"/>
        <skos:altLabel xml:lang="en">MCQ.93</skos:altLabel>
        <skos:broader rdf:resource="http://JP_ontology.org/assessment/AssessmentQuestion"/>
        <skos:definition xml:lang="en">Are items of equipment containing storage media verified to ensure that any sensitive data and licensed software have been removed or securely overwritten prior to disposal or re-use?</skos:definition>
        <skos:prefLabel xml:lang="en">Multiple Choice Question #93</skos:prefLabel>
    </rdf:Description>
    <rdf:Description rdf:about="http://JP_ontology.org/assessment/MCQ.94">
        <nis2v:hasAnswer rdf:resource="http://JP_ontology.org/assessment/MCQ.94AnswerA"/>
        <nis2v:hasAnswer rdf:resource="http://JP_ontology.org/assessment/MCQ.94AnswerB"/>
        <nis2v:hasAnswer rdf:resource="http://JP_ontology.org/assessment/MCQ.94AnswerC"/>
        <nis2v:relatedToControl rdf:resource="http://JP_ontology.org/iso27001/ControlA.8.1"/>
        <terms:contributor>Jenni Parry</terms:contributor>
        <terms:created rdf:datatype="http://www.w3.org/2001/XMLSchema#date">2024-05-20</terms:created>
        <terms:subject rdf:resource="http://JP_ontology.org/nis2v/Article_21.2i"/>
        <rdfs:isDefinedBy rdf:resource="http://JP_ontology.org/assessment"/>
        <skos:altLabel xml:lang="en">MCQ.94</skos:altLabel>
        <skos:broader rdf:resource="http://JP_ontology.org/assessment/AssessmentQuestion"/>
        <skos:definition xml:lang="en">Is information stored on, processed by, or accessible via user endpoint devices protected?</skos:definition>
        <skos:prefLabel xml:lang="en">Multiple Choice Question #94</skos:prefLabel>
    </rdf:Description>
    <rdf:Description rdf:about="http://JP_ontology.org/assessment/MCQ.95">
        <nis2v:hasAnswer rdf:resource="http://JP_ontology.org/assessment/MCQ.95AnswerA"/>
        <nis2v:hasAnswer rdf:resource="http://JP_ontology.org/assessment/MCQ.95AnswerB"/>
        <nis2v:hasAnswer rdf:resource="http://JP_ontology.org/assessment/MCQ.95AnswerC"/>
        <nis2v:relatedToControl rdf:resource="http://JP_ontology.org/iso27001/ControlA.8.7"/>
        <terms:contributor>Jenni Parry</terms:contributor>
        <terms:created rdf:datatype="http://www.w3.org/2001/XMLSchema#date">2024-05-20</terms:created>
        <terms:subject rdf:resource="http://JP_ontology.org/nis2v/Article_21.2i"/>
        <rdfs:isDefinedBy rdf:resource="http://JP_ontology.org/assessment"/>
        <skos:altLabel xml:lang="en">MCQ.95</skos:altLabel>
        <skos:broader rdf:resource="http://JP_ontology.org/assessment/AssessmentQuestion"/>
        <skos:definition xml:lang="en">Is protection against malware implemented and supported by appropriate user awareness measures?</skos:definition>
        <skos:prefLabel xml:lang="en">Multiple Choice Question #95</skos:prefLabel>
    </rdf:Description>
    <rdf:Description rdf:about="http://JP_ontology.org/assessment/MCQ.96">
        <nis2v:hasAnswer rdf:resource="http://JP_ontology.org/assessment/MCQ.96AnswerA"/>
        <nis2v:hasAnswer rdf:resource="http://JP_ontology.org/assessment/MCQ.96AnswerB"/>
        <nis2v:hasAnswer rdf:resource="http://JP_ontology.org/assessment/MCQ.96AnswerC"/>
        <nis2v:relatedToControl rdf:resource="http://JP_ontology.org/iso27001/ControlA.5.14"/>
        <terms:contributor>Jenni Parry</terms:contributor>
        <terms:created rdf:datatype="http://www.w3.org/2001/XMLSchema#date">2024-05-20</terms:created>
        <terms:subject rdf:resource="http://JP_ontology.org/nis2v/Article_21.2j"/>
        <rdfs:isDefinedBy rdf:resource="http://JP_ontology.org/assessment"/>
        <skos:altLabel xml:lang="en">MCQ.96</skos:altLabel>
        <skos:broader rdf:resource="http://JP_ontology.org/assessment/AssessmentQuestion"/>
        <skos:definition xml:lang="en">Are information transfer rules, procedures, or agreements in place for all types of transfer facilities within the organisation and between the organisation and other parties?</skos:definition>
        <skos:prefLabel xml:lang="en">Multiple Choice Question #96</skos:prefLabel>
    </rdf:Description>
    <rdf:Description rdf:about="http://JP_ontology.org/assessment/MCQ.97">
        <nis2v:hasAnswer rdf:resource="http://JP_ontology.org/assessment/MCQ.97AnswerA"/>
        <nis2v:hasAnswer rdf:resource="http://JP_ontology.org/assessment/MCQ.97AnswerB"/>
        <nis2v:hasAnswer rdf:resource="http://JP_ontology.org/assessment/MCQ.97AnswerC"/>
        <nis2v:relatedToControl rdf:resource="http://JP_ontology.org/iso27001/ControlA.5.16"/>
        <terms:contributor>Jenni Parry</terms:contributor>
        <terms:created rdf:datatype="http://www.w3.org/2001/XMLSchema#date">2024-05-20</terms:created>
        <terms:subject rdf:resource="http://JP_ontology.org/nis2v/Article_21.2j"/>
        <rdfs:isDefinedBy rdf:resource="http://JP_ontology.org/assessment"/>
        <skos:altLabel xml:lang="en">MCQ.97</skos:altLabel>
        <skos:broader rdf:resource="http://JP_ontology.org/assessment/AssessmentQuestion"/>
        <skos:definition xml:lang="en">Is the organisation managing the complete life cycle of identities, encompassing activities such as identity creation, authentication, authorization, periodic reviews, modification, and termination, ensuring comprehensive oversight and control over identity-related processes?</skos:definition>
        <skos:prefLabel xml:lang="en">Multiple Choice Question #97</skos:prefLabel>
    </rdf:Description>
    <rdf:Description rdf:about="http://JP_ontology.org/assessment/MCQ.98">
        <nis2v:hasAnswer rdf:resource="http://JP_ontology.org/assessment/MCQ.98AnswerA"/>
        <nis2v:hasAnswer rdf:resource="http://JP_ontology.org/assessment/MCQ.98AnswerB"/>
        <nis2v:hasAnswer rdf:resource="http://JP_ontology.org/assessment/MCQ.98AnswerC"/>
        <nis2v:relatedToControl rdf:resource="http://JP_ontology.org/iso27001/ControlA.5.17"/>
        <terms:contributor>Jenni Parry</terms:contributor>
        <terms:created rdf:datatype="http://www.w3.org/2001/XMLSchema#date">2024-05-20</terms:created>
        <terms:subject rdf:resource="http://JP_ontology.org/nis2v/Article_21.2j"/>
        <rdfs:isDefinedBy rdf:resource="http://JP_ontology.org/assessment"/>
        <skos:altLabel xml:lang="en">MCQ.98</skos:altLabel>
        <skos:broader rdf:resource="http://JP_ontology.org/assessment/AssessmentQuestion"/>
        <skos:definition xml:lang="en">Is the allocation and management of authentication information controlled by a management process, which includes advising personnel on the appropriate handling of authentication information?</skos:definition>
        <skos:prefLabel xml:lang="en">Multiple Choice Question #98</skos:prefLabel>
    </rdf:Description>
    <rdf:Description rdf:about="http://JP_ontology.org/assessment/MCQ.99">
        <nis2v:hasAnswer rdf:resource="http://JP_ontology.org/assessment/MCQ.99AnswerA"/>
        <nis2v:hasAnswer rdf:resource="http://JP_ontology.org/assessment/MCQ.99AnswerB"/>
        <nis2v:hasAnswer rdf:resource="http://JP_ontology.org/assessment/MCQ.99AnswerC"/>
        <nis2v:relatedToControl rdf:resource="http://JP_ontology.org/iso27001/ControlA.8.5"/>
        <terms:contributor>Jenni Parry</terms:contributor>
        <terms:created rdf:datatype="http://www.w3.org/2001/XMLSchema#date">2024-05-20</terms:created>
        <terms:subject rdf:resource="http://JP_ontology.org/nis2v/Article_21.2j"/>
        <rdfs:isDefinedBy rdf:resource="http://JP_ontology.org/assessment"/>
        <skos:altLabel xml:lang="en">MCQ.99</skos:altLabel>
        <skos:broader rdf:resource="http://JP_ontology.org/assessment/AssessmentQuestion"/>
        <skos:definition xml:lang="en">Are secure authentication technologies and procedures implemented based on information access restrictions and the topic-specific policy on access control?</skos:definition>
        <skos:prefLabel xml:lang="en">Multiple Choice Question #99</skos:prefLabel>
    </rdf:Description>
</rdf:RDF>



<!-- Generated by the OWL API (version 5.1.18) https://github.com/owlcs/owlapi/ -->


