@prefix : <http://JP_ontology.org/nis2v/> .
@prefix owl: <http://www.w3.org/2002/07/owl#> .
@prefix rdf: <http://www.w3.org/1999/02/22-rdf-syntax-ns#> .
@prefix xml: <http://www.w3.org/XML/1998/namespace> .
@prefix xsd: <http://www.w3.org/2001/XMLSchema#> .
@prefix rdfs: <http://www.w3.org/2000/01/rdf-schema#> .
@base <http://JP_ontology.org/nis2v/> .

<http://JP_ontology.org/nis2v/> rdf:type owl:Ontology ;
                                 owl:imports <http://JP_ontology.org/assessment/> ,
                                             <http://JP_ontology.org/iso27001/> ;
                                 <http://purl.org/dc/terms/abstract> "NIS2V Vocabulary extends DPV to describe the NIS2 Cybersecurity risk-management measures (Article 21) mapped against ISO 27001:2022 control framework." ;
                                 <http://purl.org/dc/terms/created> "2024-04-08"^^xsd:date ;
                                 <http://purl.org/dc/terms/creator> "Jenni Parry" ;
                                 <http://purl.org/dc/terms/date> "2024-04-08" ;
                                 <http://purl.org/dc/terms/description> "NIS2V Vocabulary extends DPV to describe the NIS2 Cybersecurity risk-management measures (Article 21) mapped against ISO 27001:2022 control framework." ,
                                                                        "This ontology will extend DPV and utilize it to perform a NIS2 gap analysis against ISO 27001:2022 controls framework (89 controls) and ENISA Minimum Security Measures for Operators of Essential Services (30 controls). Data Privacy Vocabulary (DPV) provides a comprehensive, standardized set of terms to describe GDPR, a number of these terms have been included (SKOS mappings) to describe the NIS2 Cybersecurity risk-management measures." ;
                                 <http://purl.org/dc/terms/extends> <https://w3c.github.io/dpv/dpv/> ;
                                 <http://purl.org/dc/terms/extent> "215" ;
                                 <http://purl.org/dc/terms/format> "application/rdf+xml" ;
                                 <http://purl.org/dc/terms/hasFormat> <https://github.com/Jenni0608/NIS2V-Vocabulary-Repository/blob/main/NIS2V_Vocabulary/nis2v_ontology_final%20-%20v5.rdf> ;
                                 <http://purl.org/dc/terms/identifier> <http://JP_ontology.org/nis2v> ,
                                                                       <https://doi.org/10.5281/zenodo.11620548> ,
                                                                       "https://jenni0608.github.io/NIS2V-Vocabulary-Repository/nis2v_Ontology_Final" ;
                                 <http://purl.org/dc/terms/importedFrom> <http://JP_ontology.org/assessment> ,
                                                                         <http://JP_ontology.org/iso27001> ;
                                 <http://purl.org/dc/terms/language> "en" ;
                                 <http://purl.org/dc/terms/modified> "2024-06-24"^^xsd:date ;
                                 <http://purl.org/dc/terms/publisher> "UCD" ;
                                 <http://purl.org/dc/terms/source> "https://doi.org/10.5281/zenodo.11620548" ;
                                 <http://purl.org/dc/terms/subject> "NIS2, Cybersecurity, ISO 27001, DPV, Risk Management, Ontology" ;
                                 <http://purl.org/dc/terms/title> "NIS2 Vocabulary" ,
                                                                  "nis2v_Ontology_Final.rdf" ;
                                 rdfs:seeAlso :documentation .

#################################################################
#    Annotation properties
#################################################################

###  http://purl.org/dc/terms/abstract
<http://purl.org/dc/terms/abstract> rdf:type owl:AnnotationProperty .


###  http://purl.org/dc/terms/contributor
<http://purl.org/dc/terms/contributor> rdf:type owl:AnnotationProperty .


###  http://purl.org/dc/terms/created
<http://purl.org/dc/terms/created> rdf:type owl:AnnotationProperty .


###  http://purl.org/dc/terms/creator
<http://purl.org/dc/terms/creator> rdf:type owl:AnnotationProperty .


###  http://purl.org/dc/terms/date
<http://purl.org/dc/terms/date> rdf:type owl:AnnotationProperty .


###  http://purl.org/dc/terms/description
<http://purl.org/dc/terms/description> rdf:type owl:AnnotationProperty .


###  http://purl.org/dc/terms/extends
<http://purl.org/dc/terms/extends> rdf:type owl:AnnotationProperty .


###  http://purl.org/dc/terms/extent
<http://purl.org/dc/terms/extent> rdf:type owl:AnnotationProperty .


###  http://purl.org/dc/terms/format
<http://purl.org/dc/terms/format> rdf:type owl:AnnotationProperty .


###  http://purl.org/dc/terms/hasFormat
<http://purl.org/dc/terms/hasFormat> rdf:type owl:AnnotationProperty .


###  http://purl.org/dc/terms/identifier
<http://purl.org/dc/terms/identifier> rdf:type owl:AnnotationProperty .


###  http://purl.org/dc/terms/importedFrom
<http://purl.org/dc/terms/importedFrom> rdf:type owl:AnnotationProperty .


###  http://purl.org/dc/terms/language
<http://purl.org/dc/terms/language> rdf:type owl:AnnotationProperty .


###  http://purl.org/dc/terms/modified
<http://purl.org/dc/terms/modified> rdf:type owl:AnnotationProperty .


###  http://purl.org/dc/terms/publisher
<http://purl.org/dc/terms/publisher> rdf:type owl:AnnotationProperty .


###  http://purl.org/dc/terms/source
<http://purl.org/dc/terms/source> rdf:type owl:AnnotationProperty .


###  http://purl.org/dc/terms/subject
<http://purl.org/dc/terms/subject> rdf:type owl:AnnotationProperty .


###  http://purl.org/dc/terms/title
<http://purl.org/dc/terms/title> rdf:type owl:AnnotationProperty .


###  http://www.w3.org/2004/02/skos/core#altLabel
<http://www.w3.org/2004/02/skos/core#altLabel> rdf:type owl:AnnotationProperty .


###  http://www.w3.org/2004/02/skos/core#broader
<http://www.w3.org/2004/02/skos/core#broader> rdf:type owl:AnnotationProperty .


###  http://www.w3.org/2004/02/skos/core#definition
<http://www.w3.org/2004/02/skos/core#definition> rdf:type owl:AnnotationProperty .


###  http://www.w3.org/2004/02/skos/core#exactMatch
<http://www.w3.org/2004/02/skos/core#exactMatch> rdf:type owl:AnnotationProperty .


###  http://www.w3.org/2004/02/skos/core#narrower
<http://www.w3.org/2004/02/skos/core#narrower> rdf:type owl:AnnotationProperty .


###  http://www.w3.org/2004/02/skos/core#note
<http://www.w3.org/2004/02/skos/core#note> rdf:type owl:AnnotationProperty .


###  http://www.w3.org/2004/02/skos/core#prefLabel
<http://www.w3.org/2004/02/skos/core#prefLabel> rdf:type owl:AnnotationProperty .


###  http://www.w3.org/2004/02/skos/core#related
<http://www.w3.org/2004/02/skos/core#related> rdf:type owl:AnnotationProperty .


#################################################################
#    Datatypes
#################################################################

###  http://www.w3.org/2001/XMLSchema#date
xsd:date rdf:type rdfs:Datatype .


#################################################################
#    Classes
#################################################################

###  http://JP_ontology.org/iso27001/ContextControls
<http://JP_ontology.org/iso27001/ContextControls> rdf:type owl:Class .


###  http://JP_ontology.org/iso27001/ControlOfDocumentedInformation
<http://JP_ontology.org/iso27001/ControlOfDocumentedInformation> rdf:type owl:Class ;
                                                                 rdfs:subClassOf :Article_21.2a ,
                                                                                 :NIS2VTerms .


###  http://JP_ontology.org/iso27001/LeadershipControls
<http://JP_ontology.org/iso27001/LeadershipControls> rdf:type owl:Class .


###  http://JP_ontology.org/iso27001/OperationControls
<http://JP_ontology.org/iso27001/OperationControls> rdf:type owl:Class .


###  http://JP_ontology.org/iso27001/OrganisationalControls
<http://JP_ontology.org/iso27001/OrganisationalControls> rdf:type owl:Class .


###  http://JP_ontology.org/iso27001/PeopleControls
<http://JP_ontology.org/iso27001/PeopleControls> rdf:type owl:Class .


###  http://JP_ontology.org/iso27001/PerformanceEvaluationControls
<http://JP_ontology.org/iso27001/PerformanceEvaluationControls> rdf:type owl:Class .


###  http://JP_ontology.org/iso27001/PhysicalControls
<http://JP_ontology.org/iso27001/PhysicalControls> rdf:type owl:Class .


###  http://JP_ontology.org/iso27001/PlanningControls
<http://JP_ontology.org/iso27001/PlanningControls> rdf:type owl:Class .


###  http://JP_ontology.org/iso27001/SupportControls
<http://JP_ontology.org/iso27001/SupportControls> rdf:type owl:Class .


###  http://JP_ontology.org/iso27001/TechnologicalControls
<http://JP_ontology.org/iso27001/TechnologicalControls> rdf:type owl:Class .


###  http://JP_ontology.org/nis2v/AcceptableUsePolicy
:AcceptableUsePolicy rdf:type owl:Class ;
                     rdfs:subClassOf <http://JP_ontology.org/iso27001/OrganisationalControls> ,
                                     :Article_21.2i ,
                                     :NIS2VTerms .


###  http://JP_ontology.org/nis2v/AccessControlPolicy
:AccessControlPolicy rdf:type owl:Class ;
                     rdfs:subClassOf <http://JP_ontology.org/iso27001/TechnologicalControls> ,
                                     :Article_21.2i ,
                                     :NIS2VTerms .


###  http://JP_ontology.org/nis2v/AccessRightsManagement
:AccessRightsManagement rdf:type owl:Class ;
                        rdfs:subClassOf <http://JP_ontology.org/iso27001/OrganisationalControls> ,
                                        :Article_21.2g ,
                                        :Article_21.2i ,
                                        :NIS2VTerms .


###  http://JP_ontology.org/nis2v/ActivityMonitoring
:ActivityMonitoring rdf:type owl:Class ;
                    rdfs:subClassOf <http://JP_ontology.org/iso27001/TechnologicalControls> ,
                                    :Article_21.2b ,
                                    :NIS2VTerms .


###  http://JP_ontology.org/nis2v/ApplicationSecurityRequirements
:ApplicationSecurityRequirements rdf:type owl:Class ;
                                 rdfs:subClassOf :Article_21.2g ,
                                                 :NIS2VTerms .


###  http://JP_ontology.org/nis2v/Article_21.2a
:Article_21.2a rdf:type owl:Class ;
               rdfs:subClassOf :NIS2CySecMeasures .


###  http://JP_ontology.org/nis2v/Article_21.2b
:Article_21.2b rdf:type owl:Class ;
               rdfs:subClassOf :NIS2CySecMeasures .


###  http://JP_ontology.org/nis2v/Article_21.2c
:Article_21.2c rdf:type owl:Class ;
               rdfs:subClassOf :NIS2CySecMeasures .


###  http://JP_ontology.org/nis2v/Article_21.2d
:Article_21.2d rdf:type owl:Class ;
               rdfs:subClassOf :NIS2CySecMeasures .


###  http://JP_ontology.org/nis2v/Article_21.2e
:Article_21.2e rdf:type owl:Class ;
               rdfs:subClassOf :NIS2CySecMeasures .


###  http://JP_ontology.org/nis2v/Article_21.2f
:Article_21.2f rdf:type owl:Class ;
               rdfs:subClassOf :NIS2CySecMeasures .


###  http://JP_ontology.org/nis2v/Article_21.2g
:Article_21.2g rdf:type owl:Class ;
               rdfs:subClassOf :NIS2CySecMeasures .


###  http://JP_ontology.org/nis2v/Article_21.2h
:Article_21.2h rdf:type owl:Class ;
               rdfs:subClassOf :NIS2CySecMeasures .


###  http://JP_ontology.org/nis2v/Article_21.2i
:Article_21.2i rdf:type owl:Class ;
               rdfs:subClassOf :NIS2CySecMeasures .


###  http://JP_ontology.org/nis2v/Article_21.2j
:Article_21.2j rdf:type owl:Class ;
               rdfs:subClassOf :NIS2CySecMeasures .


###  http://JP_ontology.org/nis2v/AssetManagementProcedures
:AssetManagementProcedures rdf:type owl:Class ;
                           rdfs:subClassOf <http://JP_ontology.org/iso27001/OrganisationalControls> ,
                                           :Article_21.2i ,
                                           :NIS2VTerms .


###  http://JP_ontology.org/nis2v/AuthenticationInformationManagement
:AuthenticationInformationManagement rdf:type owl:Class ;
                                     rdfs:subClassOf <http://JP_ontology.org/iso27001/OrganisationalControls> ,
                                                     :Article_21.2g ,
                                                     :Article_21.2i ,
                                                     :Article_21.2j ,
                                                     :NIS2VTerms .


###  http://JP_ontology.org/nis2v/AwarenessTraining
:AwarenessTraining rdf:type owl:Class ;
                   rdfs:subClassOf <http://JP_ontology.org/iso27001/SupportControls> ,
                                   :Article_21.2g ,
                                   :NIS2VTerms .


###  http://JP_ontology.org/nis2v/BackupManagement
:BackupManagement rdf:type owl:Class ;
                  rdfs:subClassOf <http://JP_ontology.org/iso27001/TechnologicalControls> ,
                                  :Article_21.2c ,
                                  :NIS2VTerms .


###  http://JP_ontology.org/nis2v/Capacitymanagement
:Capacitymanagement rdf:type owl:Class ;
                    rdfs:subClassOf <http://JP_ontology.org/iso27001/TechnologicalControls> ,
                                    :Article_21.2c ,
                                    :NIS2VTerms .


###  http://JP_ontology.org/nis2v/ChangeManagement
:ChangeManagement rdf:type owl:Class ;
                  rdfs:subClassOf :Article_21.2g ,
                                  :NIS2VTerms .


###  http://JP_ontology.org/nis2v/ClearDeskAndClearScreen
:ClearDeskAndClearScreen rdf:type owl:Class ;
                         rdfs:subClassOf :Article_21.2g ,
                                         :NIS2VTerms .


###  http://JP_ontology.org/nis2v/ClockSynchronization
:ClockSynchronization rdf:type owl:Class ;
                      rdfs:subClassOf :Article_21.2b ,
                                      :NIS2VTerms .


###  http://JP_ontology.org/nis2v/CloudServiceManagement
:CloudServiceManagement rdf:type owl:Class ;
                        rdfs:subClassOf <http://JP_ontology.org/iso27001/OrganisationalControls> ,
                                        :Article_21.2d ,
                                        :NIS2VTerms .


###  http://JP_ontology.org/nis2v/Communication
:Communication rdf:type owl:Class ;
               rdfs:subClassOf <http://JP_ontology.org/iso27001/SupportControls> ,
                               :Article_21.2a ,
                               :Article_21.2g ,
                               :NIS2VTerms .


###  http://JP_ontology.org/nis2v/CompetenceManagementForInformationSecurityPersonnel
:CompetenceManagementForInformationSecurityPersonnel rdf:type owl:Class ;
                                                     rdfs:subClassOf :Article_21.2g ,
                                                                     :NIS2VTerms .


###  http://JP_ontology.org/nis2v/ComplianceManagement
:ComplianceManagement rdf:type owl:Class ;
                      rdfs:subClassOf <http://JP_ontology.org/iso27001/OrganisationalControls> ,
                                      :Article_21.2a ,
                                      :NIS2VTerms .


###  http://JP_ontology.org/nis2v/ContactWithAuthorities
:ContactWithAuthorities rdf:type owl:Class ;
                        rdfs:subClassOf :Article_21.2a ,
                                        :NIS2VTerms .


###  http://JP_ontology.org/nis2v/ContactWithSpecialInterestGroups
:ContactWithSpecialInterestGroups rdf:type owl:Class ;
                                  rdfs:subClassOf :Article_21.2a ,
                                                  :NIS2VTerms .


###  http://JP_ontology.org/nis2v/ContextOfTheOrganisation
:ContextOfTheOrganisation rdf:type owl:Class ;
                          rdfs:subClassOf :Article_21.2a ,
                                          :NIS2VTerms .


###  http://JP_ontology.org/nis2v/ContinualImprovement
:ContinualImprovement rdf:type owl:Class ;
                      rdfs:subClassOf :Article_21.2f ,
                                      :NIS2VTerms .


###  http://JP_ontology.org/nis2v/CryptographyPolicy
:CryptographyPolicy rdf:type owl:Class ;
                    rdfs:subClassOf <http://JP_ontology.org/iso27001/TechnologicalControls> ,
                                    :Article_21.2h ,
                                    :NIS2VTerms .


###  http://JP_ontology.org/nis2v/DataLeakagePrevention
:DataLeakagePrevention rdf:type owl:Class ;
                       rdfs:subClassOf <http://JP_ontology.org/iso27001/TechnologicalControls> ,
                                       :Article_21.2j ,
                                       :NIS2VTerms .


###  http://JP_ontology.org/nis2v/DisasterRecoveryProcedures
:DisasterRecoveryProcedures rdf:type owl:Class ;
                            rdfs:subClassOf <http://JP_ontology.org/iso27001/OrganisationalControls> ,
                                            :Article_21.2c ,
                                            :NIS2VTerms .


###  http://JP_ontology.org/nis2v/Disciplinaryprocess
:Disciplinaryprocess rdf:type owl:Class ;
                     rdfs:subClassOf <http://JP_ontology.org/iso27001/PeopleControls> ,
                                     :Article_21.2i ,
                                     :NIS2VTerms .


###  http://JP_ontology.org/nis2v/DocumentedOperatingProcedures
:DocumentedOperatingProcedures rdf:type owl:Class ;
                               rdfs:subClassOf :Article_21.2a ,
                                               :NIS2VTerms .


###  http://JP_ontology.org/nis2v/EndpointDeviceSecurityMeasures
:EndpointDeviceSecurityMeasures rdf:type owl:Class ;
                                rdfs:subClassOf <http://JP_ontology.org/iso27001/TechnologicalControls> ,
                                                :Article_21.2i ,
                                                :NIS2VTerms .


###  http://JP_ontology.org/nis2v/EnforceAccessControl
:EnforceAccessControl rdf:type owl:Class ;
                      rdfs:subClassOf <http://JP_ontology.org/iso27001/OrganisationalControls> ,
                                      :Article_21.2g ,
                                      :Article_21.2i ,
                                      :NIS2VTerms .


###  http://JP_ontology.org/nis2v/EquipmentMaintenance
:EquipmentMaintenance rdf:type owl:Class ;
                      rdfs:subClassOf :Article_21.2g ,
                                      :NIS2VTerms .


###  http://JP_ontology.org/nis2v/EvidenceCollection
:EvidenceCollection rdf:type owl:Class ;
                    rdfs:subClassOf :Article_21.2b ,
                                    :NIS2VTerms .


###  http://JP_ontology.org/nis2v/ExternalWebsiteAccessManagement
:ExternalWebsiteAccessManagement rdf:type owl:Class ;
                                 rdfs:subClassOf <http://JP_ontology.org/iso27001/TechnologicalControls> ,
                                                 :Article_21.2e ,
                                                 :NIS2VTerms .


###  http://JP_ontology.org/nis2v/ICTContinuityManagement
:ICTContinuityManagement rdf:type owl:Class ;
                         rdfs:subClassOf <http://JP_ontology.org/iso27001/OrganisationalControls> ,
                                         :Article_21.2c ,
                                         :NIS2VTerms .


###  http://JP_ontology.org/nis2v/ICTandSupplyChainVigilance
:ICTandSupplyChainVigilance rdf:type owl:Class ;
                            rdfs:subClassOf <http://JP_ontology.org/iso27001/OrganisationalControls> ,
                                            :Article_21.2d ,
                                            :NIS2VTerms .


###  http://JP_ontology.org/nis2v/ISMSDocumentationRequirements
:ISMSDocumentationRequirements rdf:type owl:Class ;
                               rdfs:subClassOf :Article_21.2a ,
                                               :NIS2VTerms .


###  http://JP_ontology.org/nis2v/IdentityManagementMethod
:IdentityManagementMethod rdf:type owl:Class ;
                          rdfs:subClassOf <http://JP_ontology.org/iso27001/OrganisationalControls> ,
                                          :Article_21.2g ,
                                          :Article_21.2i ,
                                          :Article_21.2j ,
                                          :NIS2VTerms .


###  http://JP_ontology.org/nis2v/IncidentKnowledgeApplication
:IncidentKnowledgeApplication rdf:type owl:Class ;
                              rdfs:subClassOf <http://JP_ontology.org/iso27001/OrganisationalControls> ,
                                              :Article_21.2b ,
                                              :NIS2VTerms .


###  http://JP_ontology.org/nis2v/IncidentResponseManagement
:IncidentResponseManagement rdf:type owl:Class ;
                            rdfs:subClassOf <http://JP_ontology.org/iso27001/OrganisationalControls> ,
                                            :Article_21.2b ,
                                            :NIS2VTerms .


###  http://JP_ontology.org/nis2v/IndependentSecurityReview
:IndependentSecurityReview rdf:type owl:Class ;
                           rdfs:subClassOf <http://JP_ontology.org/iso27001/OrganisationalControls> ,
                                           :Article_21.2f ,
                                           :NIS2VTerms .


###  http://JP_ontology.org/nis2v/InformationSecurityAwarenessTraining
:InformationSecurityAwarenessTraining rdf:type owl:Class ;
                                      rdfs:subClassOf <http://JP_ontology.org/iso27001/PeopleControls> ,
                                                      :Article_21.2g ,
                                                      :Article_21.2i ,
                                                      :NIS2VTerms .


###  http://JP_ontology.org/nis2v/InformationSecurityIntergradation
:InformationSecurityIntergradation rdf:type owl:Class ;
                                   rdfs:subClassOf <http://JP_ontology.org/iso27001/OrganisationalControls> ,
                                                   :Article_21.2d ,
                                                   :NIS2VTerms .


###  http://JP_ontology.org/nis2v/InformationSecurityManagementReview
:InformationSecurityManagementReview rdf:type owl:Class ;
                                     rdfs:subClassOf <http://JP_ontology.org/iso27001/PerformanceEvaluationControls> ,
                                                     :Article_21.2f ,
                                                     :NIS2VTerms .


###  http://JP_ontology.org/nis2v/InformationSecurityManagementSystem
:InformationSecurityManagementSystem rdf:type owl:Class ;
                                     rdfs:subClassOf :Article_21.2a ,
                                                     :NIS2VTerms .


###  http://JP_ontology.org/nis2v/InformationSecurityObjectivesandPlanning
:InformationSecurityObjectivesandPlanning rdf:type owl:Class ;
                                          rdfs:subClassOf <http://JP_ontology.org/iso27001/PlanningControls> ,
                                                          :Article_21.2a ,
                                                          :NIS2VTerms .


###  http://JP_ontology.org/nis2v/InformationSecurityPolicy
:InformationSecurityPolicy rdf:type owl:Class ;
                           rdfs:subClassOf <http://JP_ontology.org/iso27001/LeadershipControls> ,
                                           :Article_21.2a ,
                                           :NIS2VTerms .


###  http://JP_ontology.org/nis2v/InformationSecurityPolicyApplication
:InformationSecurityPolicyApplication rdf:type owl:Class ;
                                      rdfs:subClassOf <http://JP_ontology.org/iso27001/OrganisationalControls> ,
                                                      :Article_21.2a ,
                                                      :NIS2VTerms .


###  http://JP_ontology.org/nis2v/InformationSecurityPolicyCompliance
:InformationSecurityPolicyCompliance rdf:type owl:Class ;
                                     rdfs:subClassOf <http://JP_ontology.org/iso27001/OrganisationalControls> ,
                                                     :Article_21.2f ,
                                                     :NIS2VTerms .


###  http://JP_ontology.org/nis2v/InformationSecurityPolicyManagement
:InformationSecurityPolicyManagement rdf:type owl:Class ;
                                     rdfs:subClassOf <http://JP_ontology.org/iso27001/OrganisationalControls> ,
                                                     :Article_21.2a ,
                                                     :NIS2VTerms .


###  http://JP_ontology.org/nis2v/InformationSecurityRiskAssessmentImplementation
:InformationSecurityRiskAssessmentImplementation rdf:type owl:Class ;
                                                 rdfs:subClassOf <http://JP_ontology.org/iso27001/OperationControls> ,
                                                                 :Article_21.2a ,
                                                                 :NIS2VTerms .


###  http://JP_ontology.org/nis2v/InformationSecurityRiskAssessmentProcess
:InformationSecurityRiskAssessmentProcess rdf:type owl:Class ;
                                          rdfs:subClassOf <http://JP_ontology.org/iso27001/PlanningControls> ,
                                                          :Article_21.2a ,
                                                          :NIS2VTerms .


###  http://JP_ontology.org/nis2v/InformationSecurityRiskTreatment
:InformationSecurityRiskTreatment rdf:type owl:Class ;
                                  rdfs:subClassOf <http://JP_ontology.org/iso27001/OperationControls> ,
                                                  :Article_21.2a ,
                                                  :NIS2VTerms .


###  http://JP_ontology.org/nis2v/InformationSecurityRoleDelegation
:InformationSecurityRoleDelegation rdf:type owl:Class ;
                                   rdfs:subClassOf <http://JP_ontology.org/iso27001/LeadershipControls> ,
                                                   :Article_21.2a ,
                                                   :NIS2VTerms .


###  http://JP_ontology.org/nis2v/InformationTransferProtocols
:InformationTransferProtocols rdf:type owl:Class ;
                              rdfs:subClassOf <http://JP_ontology.org/iso27001/OrganisationalControls> ,
                                              :Article_21.2j ,
                                              :NIS2VTerms .


###  http://JP_ontology.org/nis2v/IntellectualPropertyRights
:IntellectualPropertyRights rdf:type owl:Class ;
                            rdfs:subClassOf <http://JP_ontology.org/iso27001/OrganisationalControls> ,
                                            :Article_21.2g ,
                                            :NIS2VTerms .


###  http://JP_ontology.org/nis2v/InternalAudit
:InternalAudit rdf:type owl:Class ;
               rdfs:subClassOf :Article_21.2f ,
                               :NIS2VTerms .


###  http://JP_ontology.org/nis2v/InternalAuditProgramme
:InternalAuditProgramme rdf:type owl:Class ;
                        rdfs:subClassOf :Article_21.2f ,
                                        :NIS2VTerms .


###  http://JP_ontology.org/nis2v/LabellingOfInformation
:LabellingOfInformation rdf:type owl:Class ;
                        rdfs:subClassOf :Article_21.2f ,
                                        :NIS2VTerms .


###  http://JP_ontology.org/nis2v/LeadershipAndCommitment
:LeadershipAndCommitment rdf:type owl:Class ;
                         rdfs:subClassOf :Article_21.2a ,
                                         :NIS2VTerms .


###  http://JP_ontology.org/nis2v/ManagementResponsibilities
:ManagementResponsibilities rdf:type owl:Class ;
                            rdfs:subClassOf :Article_21.2f ,
                                            :NIS2VTerms .


###  http://JP_ontology.org/nis2v/ManagementReviewResults
:ManagementReviewResults rdf:type owl:Class ;
                         rdfs:subClassOf :Article_21.2f ,
                                         :NIS2VTerms .


###  http://JP_ontology.org/nis2v/NIS2CySecMeasures
:NIS2CySecMeasures rdf:type owl:Class .


###  http://JP_ontology.org/nis2v/NIS2VTerms
:NIS2VTerms rdf:type owl:Class .


###  http://JP_ontology.org/nis2v/NeedsAndExpectationsOfInterestedParties
:NeedsAndExpectationsOfInterestedParties rdf:type owl:Class ;
                                         rdfs:subClassOf :Article_21.2a ,
                                                         :NIS2VTerms .


###  http://JP_ontology.org/nis2v/NetworkSecurity
:NetworkSecurity rdf:type owl:Class ;
                 rdfs:subClassOf <http://JP_ontology.org/iso27001/TechnologicalControls> ,
                                 :Article_21.2e ,
                                 :NIS2VTerms .


###  http://JP_ontology.org/nis2v/NetworkServiceSecurityManagement
:NetworkServiceSecurityManagement rdf:type owl:Class ;
                                  rdfs:subClassOf <http://JP_ontology.org/iso27001/TechnologicalControls> ,
                                                  :Article_21.2e ,
                                                  :NIS2VTerms .


###  http://JP_ontology.org/nis2v/NonconformityAndCorrectiveAction
:NonconformityAndCorrectiveAction rdf:type owl:Class ;
                                  rdfs:subClassOf :Article_21.2f ,
                                                  :NIS2VTerms .


###  http://JP_ontology.org/nis2v/OperationalPlanningandControl
:OperationalPlanningandControl rdf:type owl:Class ;
                               rdfs:subClassOf <http://JP_ontology.org/iso27001/OperationControls> ,
                                               :Article_21.2a ,
                                               :Article_21.2d ,
                                               :NIS2VTerms .


###  http://JP_ontology.org/nis2v/OrganisationContext
:OrganisationContext rdf:type owl:Class ;
                     rdfs:subClassOf <http://JP_ontology.org/iso27001/ContextControls> ,
                                     :Article_21.2a ,
                                     :NIS2VTerms .


###  http://JP_ontology.org/nis2v/OutsourcedDevelopment
:OutsourcedDevelopment rdf:type owl:Class ;
                       rdfs:subClassOf :Article_21.2g ,
                                       :NIS2VTerms .


###  http://JP_ontology.org/nis2v/PhysicalSecurityPerimeters
:PhysicalSecurityPerimeters rdf:type owl:Class ;
                            rdfs:subClassOf <http://JP_ontology.org/iso27001/PhysicalControls> ,
                                            :Article_21.2i ,
                                            :NIS2VTerms .


###  http://JP_ontology.org/nis2v/Planning
:Planning rdf:type owl:Class ;
          rdfs:subClassOf :Article_21.2a ,
                          :NIS2VTerms .


###  http://JP_ontology.org/nis2v/PrivilegedAccessManagement
:PrivilegedAccessManagement rdf:type owl:Class ;
                            rdfs:subClassOf <http://JP_ontology.org/iso27001/TechnologicalControls> ,
                                            :Article_21.2i ,
                                            :NIS2VTerms .


###  http://JP_ontology.org/nis2v/ProtectionOfRecords
:ProtectionOfRecords rdf:type owl:Class ;
                     rdfs:subClassOf <http://JP_ontology.org/iso27001/OrganisationalControls> ,
                                     :Article_21.2g ,
                                     :NIS2VTerms .


###  http://JP_ontology.org/nis2v/ProtectionOfSystemsDuringAuditTesting
:ProtectionOfSystemsDuringAuditTesting rdf:type owl:Class ;
                                       rdfs:subClassOf :Article_21.2g ,
                                                       :NIS2VTerms .


###  http://JP_ontology.org/nis2v/Protectionagainstmalware
:Protectionagainstmalware rdf:type owl:Class ;
                          rdfs:subClassOf <http://JP_ontology.org/iso27001/TechnologicalControls> ,
                                          :Article_21.2g ,
                                          :Article_21.2i ,
                                          :NIS2VTerms .


###  http://JP_ontology.org/nis2v/RedundancyOfInformationProcessingFacilities
:RedundancyOfInformationProcessingFacilities rdf:type owl:Class ;
                                             rdfs:subClassOf :Article_21.2c ,
                                                             :NIS2VTerms .


###  http://JP_ontology.org/nis2v/RemoteWorkSecurityProtocols
:RemoteWorkSecurityProtocols rdf:type owl:Class ;
                             rdfs:subClassOf <http://JP_ontology.org/iso27001/PeopleControls> ,
                                             :Article_21.2i ,
                                             :NIS2VTerms .


###  http://JP_ontology.org/nis2v/Resources
:Resources rdf:type owl:Class ;
           rdfs:subClassOf :Article_21.2a ,
                           :NIS2VTerms .


###  http://JP_ontology.org/nis2v/ResponsibilitiesAfterTerminationOrChange
:ResponsibilitiesAfterTerminationOrChange rdf:type owl:Class ;
                                          rdfs:subClassOf :Article_21.2i ,
                                                          :NIS2VTerms .


###  http://JP_ontology.org/nis2v/ReturnOfAssets
:ReturnOfAssets rdf:type owl:Class ;
                rdfs:subClassOf :Article_21.2i ,
                                :NIS2VTerms .


###  http://JP_ontology.org/nis2v/ScopeOfTheISMS
:ScopeOfTheISMS rdf:type owl:Class ;
                rdfs:subClassOf :Article_21.2a ,
                                :NIS2VTerms .


###  http://JP_ontology.org/nis2v/Screening
:Screening rdf:type owl:Class ;
           rdfs:subClassOf :Article_21.2i ,
                           :NIS2VTerms .


###  http://JP_ontology.org/nis2v/SecureAuthenticationImplementation
:SecureAuthenticationImplementation rdf:type owl:Class ;
                                    rdfs:subClassOf <http://JP_ontology.org/iso27001/TechnologicalControls> ,
                                                    :Article_21.2i ,
                                                    :Article_21.2j ,
                                                    :NIS2VTerms .


###  http://JP_ontology.org/nis2v/SecureDevelopmentLifeCycle
:SecureDevelopmentLifeCycle rdf:type owl:Class ;
                            rdfs:subClassOf :Article_21.2g ,
                                            :NIS2VTerms .


###  http://JP_ontology.org/nis2v/SecureSoftwareInstallationManagement
:SecureSoftwareInstallationManagement rdf:type owl:Class ;
                                      rdfs:subClassOf <http://JP_ontology.org/iso27001/TechnologicalControls> ,
                                                      :Article_21.2e ,
                                                      :Article_21.2g ,
                                                      :NIS2VTerms .


###  http://JP_ontology.org/nis2v/SecurityConfigurationOversight
:SecurityConfigurationOversight rdf:type owl:Class ;
                                rdfs:subClassOf <http://JP_ontology.org/iso27001/TechnologicalControls> ,
                                                :Article_21.2e ,
                                                :Article_21.2g ,
                                                :NIS2VTerms .


###  http://JP_ontology.org/nis2v/SecurityEventReportingMechanism
:SecurityEventReportingMechanism rdf:type owl:Class ;
                                 rdfs:subClassOf <http://JP_ontology.org/iso27001/PeopleControls> ,
                                                 :Article_21.2b ,
                                                 :NIS2VTerms .


###  http://JP_ontology.org/nis2v/SecurityIncidentCategorisation
:SecurityIncidentCategorisation rdf:type owl:Class ;
                                rdfs:subClassOf <http://JP_ontology.org/iso27001/OrganisationalControls> ,
                                                :Article_21.2b ,
                                                :NIS2VTerms .


###  http://JP_ontology.org/nis2v/SecurityLoggingandAnalysis
:SecurityLoggingandAnalysis rdf:type owl:Class ;
                            rdfs:subClassOf <http://JP_ontology.org/iso27001/TechnologicalControls> ,
                                            :Article_21.2b ,
                                            :NIS2VTerms .


###  http://JP_ontology.org/nis2v/SecurityOfAssetsOffPremises
:SecurityOfAssetsOffPremises rdf:type owl:Class ;
                             rdfs:subClassOf :Article_21.2i ,
                                             :NIS2VTerms .


###  http://JP_ontology.org/nis2v/SecurityRolesResponsibilityAllocation
:SecurityRolesResponsibilityAllocation rdf:type owl:Class ;
                                       rdfs:subClassOf <http://JP_ontology.org/iso27001/OrganisationalControls> ,
                                                       :Article_21.2a ,
                                                       :Article_21.2i ,
                                                       :NIS2VTerms .


###  http://JP_ontology.org/nis2v/SegregationOfDuties
:SegregationOfDuties rdf:type owl:Class ;
                     rdfs:subClassOf :Article_21.2i ,
                                     :NIS2VTerms .


###  http://JP_ontology.org/nis2v/SegregationOfNetworks
:SegregationOfNetworks rdf:type owl:Class ;
                       rdfs:subClassOf :Article_21.2e ,
                                       :NIS2VTerms .


###  http://JP_ontology.org/nis2v/SeparationOfEnvironments
:SeparationOfEnvironments rdf:type owl:Class ;
                          rdfs:subClassOf :Article_21.2e ,
                                          :NIS2VTerms .


###  http://JP_ontology.org/nis2v/SourceCodeandDevelopmentAccessControl
:SourceCodeandDevelopmentAccessControl rdf:type owl:Class ;
                                       rdfs:subClassOf <http://JP_ontology.org/iso27001/TechnologicalControls> ,
                                                       :Article_21.2i ,
                                                       :NIS2VTerms .


###  http://JP_ontology.org/nis2v/StorageMediaDisposalProtocol
:StorageMediaDisposalProtocol rdf:type owl:Class ;
                              rdfs:subClassOf <http://JP_ontology.org/iso27001/PhysicalControls> ,
                                              :Article_21.2i ,
                                              :NIS2VTerms .


###  http://JP_ontology.org/nis2v/StorageMediaManagement
:StorageMediaManagement rdf:type owl:Class ;
                        rdfs:subClassOf <http://JP_ontology.org/iso27001/PhysicalControls> ,
                                        :Article_21.2i ,
                                        :NIS2VTerms .


###  http://JP_ontology.org/nis2v/SupplierSecurityRequirementsManagement
:SupplierSecurityRequirementsManagement rdf:type owl:Class ;
                                        rdfs:subClassOf <http://JP_ontology.org/iso27001/OrganisationalControls> ,
                                                        :Article_21.2d ,
                                                        :NIS2VTerms .


###  http://JP_ontology.org/nis2v/SupplyChainDiligence
:SupplyChainDiligence rdf:type owl:Class ;
                      rdfs:subClassOf <http://JP_ontology.org/iso27001/OrganisationalControls> ,
                                      :Article_21.2d ,
                                      :NIS2VTerms .


###  http://JP_ontology.org/nis2v/SupportingUtilities
:SupportingUtilities rdf:type owl:Class ;
                     rdfs:subClassOf :Article_21.2c ,
                                     :NIS2VTerms .


###  http://JP_ontology.org/nis2v/TechnicalVulnerabilityManagement
:TechnicalVulnerabilityManagement rdf:type owl:Class ;
                                  rdfs:subClassOf <http://JP_ontology.org/iso27001/TechnologicalControls> ,
                                                  :Article_21.2e ,
                                                  :Article_21.2g ,
                                                  :NIS2VTerms .


###  http://JP_ontology.org/nis2v/TermsAndConditionsOfEmployment
:TermsAndConditionsOfEmployment rdf:type owl:Class ;
                                rdfs:subClassOf :Article_21.2i ,
                                                :NIS2VTerms .


###  http://JP_ontology.org/nis2v/ThirdPartySecurityProcedures
:ThirdPartySecurityProcedures rdf:type owl:Class ;
                              rdfs:subClassOf <http://JP_ontology.org/iso27001/OrganisationalControls> ,
                                              :Article_21.2d ,
                                              :NIS2VTerms .


###  http://JP_ontology.org/nis2v/ThreatIntelligence
:ThreatIntelligence rdf:type owl:Class ;
                    rdfs:subClassOf :Article_21.2a ,
                                    :NIS2VTerms .


###  http://JP_ontology.org/nis2v/UtilityProgramAccessRestrictions
:UtilityProgramAccessRestrictions rdf:type owl:Class ;
                                  rdfs:subClassOf <http://JP_ontology.org/iso27001/TechnologicalControls> ,
                                                  :Article_21.2i ,
                                                  :NIS2VTerms .


###  http://JP_ontology.org/nis2v/Monitoring,Measurement,AnalysisandEvaluation
<http://JP_ontology.org/nis2v/Monitoring,Measurement,AnalysisandEvaluation> rdf:type owl:Class ;
                                                                            rdfs:subClassOf <http://JP_ontology.org/iso27001/PerformanceEvaluationControls> ,
                                                                                            :Article_21.2f ,
                                                                                            :NIS2VTerms .


###  http://JP_ontology.org/nis2v/Non-DisclosureAgreement(NDA)
<http://JP_ontology.org/nis2v/Non-DisclosureAgreement(NDA)> rdf:type owl:Class ;
                                                            rdfs:subClassOf <http://JP_ontology.org/iso27001/PeopleControls> ,
                                                                            :Article_21.2i ,
                                                                            :NIS2VTerms .


###  http://www.w3.org/2004/02/skos/core#Concept
<http://www.w3.org/2004/02/skos/core#Concept> rdf:type owl:Class .


#################################################################
#    Individuals
#################################################################

###  http://JP_ontology.org/iso27001/ControlOfDocumentedInformation
<http://JP_ontology.org/iso27001/ControlOfDocumentedInformation> rdf:type owl:NamedIndividual ,
                                                                          <http://www.w3.org/2004/02/skos/core#Concept> .


###  http://JP_ontology.org/nis2v/AcceptableUsePolicy
:AcceptableUsePolicy rdf:type owl:NamedIndividual ,
                              <http://www.w3.org/2004/02/skos/core#Concept> .


###  http://JP_ontology.org/nis2v/AccessControlPolicy
:AccessControlPolicy rdf:type owl:NamedIndividual ,
                              <http://www.w3.org/2004/02/skos/core#Concept> .


###  http://JP_ontology.org/nis2v/AccessRightsManagement
:AccessRightsManagement rdf:type owl:NamedIndividual ,
                                 <http://www.w3.org/2004/02/skos/core#Concept> .


###  http://JP_ontology.org/nis2v/ActivityMonitoring
:ActivityMonitoring rdf:type owl:NamedIndividual ,
                             <http://www.w3.org/2004/02/skos/core#Concept> .


###  http://JP_ontology.org/nis2v/ApplicationSecurityRequirements
:ApplicationSecurityRequirements rdf:type owl:NamedIndividual ,
                                          <http://www.w3.org/2004/02/skos/core#Concept> .


###  http://JP_ontology.org/nis2v/Article_21.2a
:Article_21.2a rdf:type owl:NamedIndividual ,
                        <http://www.w3.org/2004/02/skos/core#Concept> .


###  http://JP_ontology.org/nis2v/Article_21.2b
:Article_21.2b rdf:type owl:NamedIndividual ,
                        <http://www.w3.org/2004/02/skos/core#Concept> .


###  http://JP_ontology.org/nis2v/Article_21.2c
:Article_21.2c rdf:type owl:NamedIndividual ,
                        <http://www.w3.org/2004/02/skos/core#Concept> .


###  http://JP_ontology.org/nis2v/Article_21.2d
:Article_21.2d rdf:type owl:NamedIndividual ,
                        <http://www.w3.org/2004/02/skos/core#Concept> .


###  http://JP_ontology.org/nis2v/Article_21.2e
:Article_21.2e rdf:type owl:NamedIndividual ,
                        <http://www.w3.org/2004/02/skos/core#Concept> .


###  http://JP_ontology.org/nis2v/Article_21.2f
:Article_21.2f rdf:type owl:NamedIndividual ,
                        <http://www.w3.org/2004/02/skos/core#Concept> .


###  http://JP_ontology.org/nis2v/Article_21.2g
:Article_21.2g rdf:type owl:NamedIndividual ,
                        <http://www.w3.org/2004/02/skos/core#Concept> .


###  http://JP_ontology.org/nis2v/Article_21.2h
:Article_21.2h rdf:type owl:NamedIndividual ,
                        <http://www.w3.org/2004/02/skos/core#Concept> .


###  http://JP_ontology.org/nis2v/Article_21.2i
:Article_21.2i rdf:type owl:NamedIndividual ,
                        <http://www.w3.org/2004/02/skos/core#Concept> .


###  http://JP_ontology.org/nis2v/Article_21.2j
:Article_21.2j rdf:type owl:NamedIndividual ,
                        <http://www.w3.org/2004/02/skos/core#Concept> .


###  http://JP_ontology.org/nis2v/AssetManagementProcedures
:AssetManagementProcedures rdf:type owl:NamedIndividual ,
                                    <http://www.w3.org/2004/02/skos/core#Concept> .


###  http://JP_ontology.org/nis2v/AuthenticationInformationManagement
:AuthenticationInformationManagement rdf:type owl:NamedIndividual ,
                                              <http://www.w3.org/2004/02/skos/core#Concept> .


###  http://JP_ontology.org/nis2v/AwarenessTraining
:AwarenessTraining rdf:type owl:NamedIndividual ,
                            <http://www.w3.org/2004/02/skos/core#Concept> .


###  http://JP_ontology.org/nis2v/BackupManagement
:BackupManagement rdf:type owl:NamedIndividual ,
                           <http://www.w3.org/2004/02/skos/core#Concept> .


###  http://JP_ontology.org/nis2v/Capacitymanagement
:Capacitymanagement rdf:type owl:NamedIndividual ,
                             <http://www.w3.org/2004/02/skos/core#Concept> .


###  http://JP_ontology.org/nis2v/ChangeManagement
:ChangeManagement rdf:type owl:NamedIndividual ,
                           <http://www.w3.org/2004/02/skos/core#Concept> .


###  http://JP_ontology.org/nis2v/ClearDeskAndClearScreen
:ClearDeskAndClearScreen rdf:type owl:NamedIndividual ,
                                  <http://www.w3.org/2004/02/skos/core#Concept> .


###  http://JP_ontology.org/nis2v/ClockSynchronization
:ClockSynchronization rdf:type owl:NamedIndividual ,
                               <http://www.w3.org/2004/02/skos/core#Concept> .


###  http://JP_ontology.org/nis2v/CloudServiceManagement
:CloudServiceManagement rdf:type owl:NamedIndividual ,
                                 <http://www.w3.org/2004/02/skos/core#Concept> .


###  http://JP_ontology.org/nis2v/Communication
:Communication rdf:type owl:NamedIndividual ,
                        <http://www.w3.org/2004/02/skos/core#Concept> .


###  http://JP_ontology.org/nis2v/CompetenceManagementForInformationSecurityPersonnel
:CompetenceManagementForInformationSecurityPersonnel rdf:type owl:NamedIndividual ,
                                                              <http://www.w3.org/2004/02/skos/core#Concept> .


###  http://JP_ontology.org/nis2v/ComplianceManagement
:ComplianceManagement rdf:type owl:NamedIndividual ,
                               <http://www.w3.org/2004/02/skos/core#Concept> .


###  http://JP_ontology.org/nis2v/ContactWithAuthorities
:ContactWithAuthorities rdf:type owl:NamedIndividual ,
                                 <http://www.w3.org/2004/02/skos/core#Concept> .


###  http://JP_ontology.org/nis2v/ContactWithSpecialInterestGroups
:ContactWithSpecialInterestGroups rdf:type owl:NamedIndividual ,
                                           <http://www.w3.org/2004/02/skos/core#Concept> .


###  http://JP_ontology.org/nis2v/ContextOfTheOrganisation
:ContextOfTheOrganisation rdf:type owl:NamedIndividual ,
                                   <http://www.w3.org/2004/02/skos/core#Concept> .


###  http://JP_ontology.org/nis2v/ContinualImprovement
:ContinualImprovement rdf:type owl:NamedIndividual ,
                               <http://www.w3.org/2004/02/skos/core#Concept> .


###  http://JP_ontology.org/nis2v/CryptographyPolicy
:CryptographyPolicy rdf:type owl:NamedIndividual ,
                             <http://www.w3.org/2004/02/skos/core#Concept> .


###  http://JP_ontology.org/nis2v/DataLeakagePrevention
:DataLeakagePrevention rdf:type owl:NamedIndividual ,
                                <http://www.w3.org/2004/02/skos/core#Concept> .


###  http://JP_ontology.org/nis2v/DisasterRecoveryProcedures
:DisasterRecoveryProcedures rdf:type owl:NamedIndividual ,
                                     <http://www.w3.org/2004/02/skos/core#Concept> .


###  http://JP_ontology.org/nis2v/Disciplinaryprocess
:Disciplinaryprocess rdf:type owl:NamedIndividual ,
                              <http://www.w3.org/2004/02/skos/core#Concept> .


###  http://JP_ontology.org/nis2v/DocumentedOperatingProcedures
:DocumentedOperatingProcedures rdf:type owl:NamedIndividual ,
                                        <http://www.w3.org/2004/02/skos/core#Concept> .


###  http://JP_ontology.org/nis2v/EndpointDeviceSecurityMeasures
:EndpointDeviceSecurityMeasures rdf:type owl:NamedIndividual ,
                                         <http://www.w3.org/2004/02/skos/core#Concept> .


###  http://JP_ontology.org/nis2v/EnforceAccessControl
:EnforceAccessControl rdf:type owl:NamedIndividual ,
                               <http://www.w3.org/2004/02/skos/core#Concept> .


###  http://JP_ontology.org/nis2v/EquipmentMaintenance
:EquipmentMaintenance rdf:type owl:NamedIndividual ,
                               <http://www.w3.org/2004/02/skos/core#Concept> .


###  http://JP_ontology.org/nis2v/EvidenceCollection
:EvidenceCollection rdf:type owl:NamedIndividual ,
                             <http://www.w3.org/2004/02/skos/core#Concept> .


###  http://JP_ontology.org/nis2v/ExternalWebsiteAccessManagement
:ExternalWebsiteAccessManagement rdf:type owl:NamedIndividual ,
                                          <http://www.w3.org/2004/02/skos/core#Concept> .


###  http://JP_ontology.org/nis2v/ICTContinuityManagement
:ICTContinuityManagement rdf:type owl:NamedIndividual ,
                                  <http://www.w3.org/2004/02/skos/core#Concept> .


###  http://JP_ontology.org/nis2v/ICTandSupplyChainVigilance
:ICTandSupplyChainVigilance rdf:type owl:NamedIndividual ,
                                     <http://www.w3.org/2004/02/skos/core#Concept> .


###  http://JP_ontology.org/nis2v/ISMSDocumentationRequirements
:ISMSDocumentationRequirements rdf:type owl:NamedIndividual ,
                                        <http://www.w3.org/2004/02/skos/core#Concept> .


###  http://JP_ontology.org/nis2v/IdentityManagementMethod
:IdentityManagementMethod rdf:type owl:NamedIndividual ,
                                   <http://www.w3.org/2004/02/skos/core#Concept> .


###  http://JP_ontology.org/nis2v/IncidentKnowledgeApplication
:IncidentKnowledgeApplication rdf:type owl:NamedIndividual ,
                                       <http://www.w3.org/2004/02/skos/core#Concept> .


###  http://JP_ontology.org/nis2v/IncidentResponseManagement
:IncidentResponseManagement rdf:type owl:NamedIndividual ,
                                     <http://www.w3.org/2004/02/skos/core#Concept> .


###  http://JP_ontology.org/nis2v/IndependentSecurityReview
:IndependentSecurityReview rdf:type owl:NamedIndividual ,
                                    <http://www.w3.org/2004/02/skos/core#Concept> .


###  http://JP_ontology.org/nis2v/InformationSecurityAwarenessTraining
:InformationSecurityAwarenessTraining rdf:type owl:NamedIndividual ,
                                               <http://www.w3.org/2004/02/skos/core#Concept> .


###  http://JP_ontology.org/nis2v/InformationSecurityIntergradation
:InformationSecurityIntergradation rdf:type owl:NamedIndividual ,
                                            <http://www.w3.org/2004/02/skos/core#Concept> .


###  http://JP_ontology.org/nis2v/InformationSecurityManagementReview
:InformationSecurityManagementReview rdf:type owl:NamedIndividual ,
                                              <http://www.w3.org/2004/02/skos/core#Concept> .


###  http://JP_ontology.org/nis2v/InformationSecurityManagementSystem
:InformationSecurityManagementSystem rdf:type owl:NamedIndividual ,
                                              <http://www.w3.org/2004/02/skos/core#Concept> .


###  http://JP_ontology.org/nis2v/InformationSecurityObjectivesandPlanning
:InformationSecurityObjectivesandPlanning rdf:type owl:NamedIndividual ,
                                                   <http://www.w3.org/2004/02/skos/core#Concept> .


###  http://JP_ontology.org/nis2v/InformationSecurityPolicy
:InformationSecurityPolicy rdf:type owl:NamedIndividual ,
                                    <http://www.w3.org/2004/02/skos/core#Concept> .


###  http://JP_ontology.org/nis2v/InformationSecurityPolicyApplication
:InformationSecurityPolicyApplication rdf:type owl:NamedIndividual ,
                                               <http://www.w3.org/2004/02/skos/core#Concept> .


###  http://JP_ontology.org/nis2v/InformationSecurityPolicyCompliance
:InformationSecurityPolicyCompliance rdf:type owl:NamedIndividual ,
                                              <http://www.w3.org/2004/02/skos/core#Concept> .


###  http://JP_ontology.org/nis2v/InformationSecurityPolicyManagement
:InformationSecurityPolicyManagement rdf:type owl:NamedIndividual ,
                                              <http://www.w3.org/2004/02/skos/core#Concept> .


###  http://JP_ontology.org/nis2v/InformationSecurityRiskAssessmentImplementation
:InformationSecurityRiskAssessmentImplementation rdf:type owl:NamedIndividual ,
                                                          <http://www.w3.org/2004/02/skos/core#Concept> .


###  http://JP_ontology.org/nis2v/InformationSecurityRiskAssessmentProcess
:InformationSecurityRiskAssessmentProcess rdf:type owl:NamedIndividual ,
                                                   <http://www.w3.org/2004/02/skos/core#Concept> .


###  http://JP_ontology.org/nis2v/InformationSecurityRiskTreatment
:InformationSecurityRiskTreatment rdf:type owl:NamedIndividual ,
                                           <http://www.w3.org/2004/02/skos/core#Concept> .


###  http://JP_ontology.org/nis2v/InformationSecurityRoleDelegation
:InformationSecurityRoleDelegation rdf:type owl:NamedIndividual ,
                                            <http://www.w3.org/2004/02/skos/core#Concept> .


###  http://JP_ontology.org/nis2v/InformationTransferProtocols
:InformationTransferProtocols rdf:type owl:NamedIndividual ,
                                       <http://www.w3.org/2004/02/skos/core#Concept> .


###  http://JP_ontology.org/nis2v/IntellectualPropertyRights
:IntellectualPropertyRights rdf:type owl:NamedIndividual ,
                                     <http://www.w3.org/2004/02/skos/core#Concept> .


###  http://JP_ontology.org/nis2v/InternalAudit
:InternalAudit rdf:type owl:NamedIndividual ,
                        <http://www.w3.org/2004/02/skos/core#Concept> .


###  http://JP_ontology.org/nis2v/InternalAuditProgramme
:InternalAuditProgramme rdf:type owl:NamedIndividual ,
                                 <http://www.w3.org/2004/02/skos/core#Concept> .


###  http://JP_ontology.org/nis2v/LabellingOfInformation
:LabellingOfInformation rdf:type owl:NamedIndividual ,
                                 <http://www.w3.org/2004/02/skos/core#Concept> .


###  http://JP_ontology.org/nis2v/LeadershipAndCommitment
:LeadershipAndCommitment rdf:type owl:NamedIndividual ,
                                  <http://www.w3.org/2004/02/skos/core#Concept> .


###  http://JP_ontology.org/nis2v/ManagementResponsibilities
:ManagementResponsibilities rdf:type owl:NamedIndividual ,
                                     <http://www.w3.org/2004/02/skos/core#Concept> .


###  http://JP_ontology.org/nis2v/ManagementReviewResults
:ManagementReviewResults rdf:type owl:NamedIndividual ,
                                  <http://www.w3.org/2004/02/skos/core#Concept> .


###  http://JP_ontology.org/nis2v/NIS2CySecMeasures
:NIS2CySecMeasures rdf:type owl:NamedIndividual ,
                            <http://www.w3.org/2004/02/skos/core#Concept> .


###  http://JP_ontology.org/nis2v/NIS2VTerms
:NIS2VTerms rdf:type owl:NamedIndividual ,
                     <http://www.w3.org/2004/02/skos/core#Concept> .


###  http://JP_ontology.org/nis2v/NeedsAndExpectationsOfInterestedParties
:NeedsAndExpectationsOfInterestedParties rdf:type owl:NamedIndividual ,
                                                  <http://www.w3.org/2004/02/skos/core#Concept> .


###  http://JP_ontology.org/nis2v/NetworkSecurity
:NetworkSecurity rdf:type owl:NamedIndividual ,
                          <http://www.w3.org/2004/02/skos/core#Concept> .


###  http://JP_ontology.org/nis2v/NetworkServiceSecurityManagement
:NetworkServiceSecurityManagement rdf:type owl:NamedIndividual ,
                                           <http://www.w3.org/2004/02/skos/core#Concept> .


###  http://JP_ontology.org/nis2v/NonconformityAndCorrectiveAction
:NonconformityAndCorrectiveAction rdf:type owl:NamedIndividual ,
                                           <http://www.w3.org/2004/02/skos/core#Concept> .


###  http://JP_ontology.org/nis2v/OperationalPlanningandControl
:OperationalPlanningandControl rdf:type owl:NamedIndividual ,
                                        <http://www.w3.org/2004/02/skos/core#Concept> .


###  http://JP_ontology.org/nis2v/OrganisationContext
:OrganisationContext rdf:type owl:NamedIndividual ,
                              <http://www.w3.org/2004/02/skos/core#Concept> .


###  http://JP_ontology.org/nis2v/OutsourcedDevelopment
:OutsourcedDevelopment rdf:type owl:NamedIndividual ,
                                <http://www.w3.org/2004/02/skos/core#Concept> .


###  http://JP_ontology.org/nis2v/PhysicalSecurityPerimeters
:PhysicalSecurityPerimeters rdf:type owl:NamedIndividual ,
                                     <http://www.w3.org/2004/02/skos/core#Concept> .


###  http://JP_ontology.org/nis2v/Planning
:Planning rdf:type owl:NamedIndividual ,
                   <http://www.w3.org/2004/02/skos/core#Concept> .


###  http://JP_ontology.org/nis2v/PrivilegedAccessManagement
:PrivilegedAccessManagement rdf:type owl:NamedIndividual ,
                                     <http://www.w3.org/2004/02/skos/core#Concept> .


###  http://JP_ontology.org/nis2v/ProtectionOfRecords
:ProtectionOfRecords rdf:type owl:NamedIndividual ,
                              <http://www.w3.org/2004/02/skos/core#Concept> .


###  http://JP_ontology.org/nis2v/ProtectionOfSystemsDuringAuditTesting
:ProtectionOfSystemsDuringAuditTesting rdf:type owl:NamedIndividual ,
                                                <http://www.w3.org/2004/02/skos/core#Concept> .


###  http://JP_ontology.org/nis2v/Protectionagainstmalware
:Protectionagainstmalware rdf:type owl:NamedIndividual ,
                                   <http://www.w3.org/2004/02/skos/core#Concept> .


###  http://JP_ontology.org/nis2v/RedundancyOfInformationProcessingFacilities
:RedundancyOfInformationProcessingFacilities rdf:type owl:NamedIndividual ,
                                                      <http://www.w3.org/2004/02/skos/core#Concept> .


###  http://JP_ontology.org/nis2v/RemoteWorkSecurityProtocols
:RemoteWorkSecurityProtocols rdf:type owl:NamedIndividual ,
                                      <http://www.w3.org/2004/02/skos/core#Concept> .


###  http://JP_ontology.org/nis2v/Resources
:Resources rdf:type owl:NamedIndividual ,
                    <http://www.w3.org/2004/02/skos/core#Concept> .


###  http://JP_ontology.org/nis2v/ResponsibilitiesAfterTerminationOrChange
:ResponsibilitiesAfterTerminationOrChange rdf:type owl:NamedIndividual ,
                                                   <http://www.w3.org/2004/02/skos/core#Concept> .


###  http://JP_ontology.org/nis2v/ReturnOfAssets
:ReturnOfAssets rdf:type owl:NamedIndividual ,
                         <http://www.w3.org/2004/02/skos/core#Concept> .


###  http://JP_ontology.org/nis2v/ScopeOfTheISMS
:ScopeOfTheISMS rdf:type owl:NamedIndividual ,
                         <http://www.w3.org/2004/02/skos/core#Concept> .


###  http://JP_ontology.org/nis2v/Screening
:Screening rdf:type owl:NamedIndividual ,
                    <http://www.w3.org/2004/02/skos/core#Concept> .


###  http://JP_ontology.org/nis2v/SecureAuthenticationImplementation
:SecureAuthenticationImplementation rdf:type owl:NamedIndividual ,
                                             <http://www.w3.org/2004/02/skos/core#Concept> .


###  http://JP_ontology.org/nis2v/SecureDevelopmentLifeCycle
:SecureDevelopmentLifeCycle rdf:type owl:NamedIndividual ,
                                     <http://www.w3.org/2004/02/skos/core#Concept> .


###  http://JP_ontology.org/nis2v/SecureSoftwareInstallationManagement
:SecureSoftwareInstallationManagement rdf:type owl:NamedIndividual ,
                                               <http://www.w3.org/2004/02/skos/core#Concept> .


###  http://JP_ontology.org/nis2v/SecurityConfigurationOversight
:SecurityConfigurationOversight rdf:type owl:NamedIndividual ,
                                         <http://www.w3.org/2004/02/skos/core#Concept> .


###  http://JP_ontology.org/nis2v/SecurityEventReportingMechanism
:SecurityEventReportingMechanism rdf:type owl:NamedIndividual ,
                                          <http://www.w3.org/2004/02/skos/core#Concept> .


###  http://JP_ontology.org/nis2v/SecurityIncidentCategorisation
:SecurityIncidentCategorisation rdf:type owl:NamedIndividual ,
                                         <http://www.w3.org/2004/02/skos/core#Concept> .


###  http://JP_ontology.org/nis2v/SecurityLoggingandAnalysis
:SecurityLoggingandAnalysis rdf:type owl:NamedIndividual ,
                                     <http://www.w3.org/2004/02/skos/core#Concept> .


###  http://JP_ontology.org/nis2v/SecurityOfAssetsOffPremises
:SecurityOfAssetsOffPremises rdf:type owl:NamedIndividual ,
                                      <http://www.w3.org/2004/02/skos/core#Concept> .


###  http://JP_ontology.org/nis2v/SecurityRolesResponsibilityAllocation
:SecurityRolesResponsibilityAllocation rdf:type owl:NamedIndividual ,
                                                <http://www.w3.org/2004/02/skos/core#Concept> .


###  http://JP_ontology.org/nis2v/SegregationOfDuties
:SegregationOfDuties rdf:type owl:NamedIndividual ,
                              <http://www.w3.org/2004/02/skos/core#Concept> .


###  http://JP_ontology.org/nis2v/SegregationOfNetworks
:SegregationOfNetworks rdf:type owl:NamedIndividual ,
                                <http://www.w3.org/2004/02/skos/core#Concept> .


###  http://JP_ontology.org/nis2v/SeparationOfEnvironments
:SeparationOfEnvironments rdf:type owl:NamedIndividual ,
                                   <http://www.w3.org/2004/02/skos/core#Concept> .


###  http://JP_ontology.org/nis2v/SourceCodeandDevelopmentAccessControl
:SourceCodeandDevelopmentAccessControl rdf:type owl:NamedIndividual ,
                                                <http://www.w3.org/2004/02/skos/core#Concept> .


###  http://JP_ontology.org/nis2v/StorageMediaDisposalProtocol
:StorageMediaDisposalProtocol rdf:type owl:NamedIndividual ,
                                       <http://www.w3.org/2004/02/skos/core#Concept> .


###  http://JP_ontology.org/nis2v/StorageMediaManagement
:StorageMediaManagement rdf:type owl:NamedIndividual ,
                                 <http://www.w3.org/2004/02/skos/core#Concept> .


###  http://JP_ontology.org/nis2v/SupplierSecurityRequirementsManagement
:SupplierSecurityRequirementsManagement rdf:type owl:NamedIndividual ,
                                                 <http://www.w3.org/2004/02/skos/core#Concept> .


###  http://JP_ontology.org/nis2v/SupplyChainDiligence
:SupplyChainDiligence rdf:type owl:NamedIndividual ,
                               <http://www.w3.org/2004/02/skos/core#Concept> .


###  http://JP_ontology.org/nis2v/SupportingUtilities
:SupportingUtilities rdf:type owl:NamedIndividual ,
                              <http://www.w3.org/2004/02/skos/core#Concept> .


###  http://JP_ontology.org/nis2v/TechnicalVulnerabilityManagement
:TechnicalVulnerabilityManagement rdf:type owl:NamedIndividual ,
                                           <http://www.w3.org/2004/02/skos/core#Concept> .


###  http://JP_ontology.org/nis2v/TermsAndConditionsOfEmployment
:TermsAndConditionsOfEmployment rdf:type owl:NamedIndividual ,
                                         <http://www.w3.org/2004/02/skos/core#Concept> .


###  http://JP_ontology.org/nis2v/ThirdPartySecurityProcedures
:ThirdPartySecurityProcedures rdf:type owl:NamedIndividual ,
                                       <http://www.w3.org/2004/02/skos/core#Concept> .


###  http://JP_ontology.org/nis2v/ThreatIntelligence
:ThreatIntelligence rdf:type owl:NamedIndividual ,
                             <http://www.w3.org/2004/02/skos/core#Concept> .


###  http://JP_ontology.org/nis2v/UtilityProgramAccessRestrictions
:UtilityProgramAccessRestrictions rdf:type owl:NamedIndividual ,
                                           <http://www.w3.org/2004/02/skos/core#Concept> .


###  http://JP_ontology.org/nis2v/Monitoring,Measurement,AnalysisandEvaluation
<http://JP_ontology.org/nis2v/Monitoring,Measurement,AnalysisandEvaluation> rdf:type owl:NamedIndividual ,
                                                                                     <http://www.w3.org/2004/02/skos/core#Concept> .


###  http://JP_ontology.org/nis2v/Non-DisclosureAgreement(NDA)
<http://JP_ontology.org/nis2v/Non-DisclosureAgreement(NDA)> rdf:type owl:NamedIndividual ,
                                                                     <http://www.w3.org/2004/02/skos/core#Concept> .


#################################################################
#    Annotations
#################################################################

<http://JP_ontology.org/iso27001/ControlOfDocumentedInformation> <http://purl.org/dc/terms/contributor> "Jenni Parry" ;
                                                                 <http://purl.org/dc/terms/created> "2024-05-01"^^xsd:date ;
                                                                 <http://purl.org/dc/terms/source> "ENISA: Minimum Security Measures for Operators of Essentials Services, https://www.enisa.europa.eu/topics/cybersecurity-policy/nis-directive-new/minimum-security-measures-for-operators-of-essentials-services"@en ;
                                                                 rdfs:isDefinedBy <http://JP_ontology.org/nis2v> ;
                                                                 <http://www.w3.org/2004/02/skos/core#altLabel> "NIS2V Term"@en ;
                                                                 <http://www.w3.org/2004/02/skos/core#definition> "Involves managing the creation, distribution, access, retrieval, retention, and disposal of documents to ensure their accuracy, confidentiality, integrity, and availability as necessary for effective operation and compliance."@en ;
                                                                 <http://www.w3.org/2004/02/skos/core#exactMatch> <http://JP_ontology.org/iso27001/Control7.5.3> ;
                                                                 <http://www.w3.org/2004/02/skos/core#note> "This NIS2V Term aligns with Article 21.2a: Policies on risk analysis and information system security."@en ;
                                                                 <http://www.w3.org/2004/02/skos/core#prefLabel> "Control of Documented Information"@en .


:AcceptableUsePolicy <http://purl.org/dc/terms/contributor> "Jenni Parry" ;
                     <http://purl.org/dc/terms/created> "2024-06-04"^^xsd:date ;
                     <http://purl.org/dc/terms/source> "ISO 27001:2022 Control Framework"@en ;
                     rdfs:isDefinedBy <http://JP_ontology.org/nis2v> ;
                     <http://www.w3.org/2004/02/skos/core#altLabel> "NIS2V Term"@en ;
                     <http://www.w3.org/2004/02/skos/core#definition> "Acceptable Use Policy: Documented rules and procedures governing the appropriate utilisation and handling of information and associated assets within the organisation, implemented to ensure adherence to acceptable use standards."@en ;
                     <http://www.w3.org/2004/02/skos/core#exactMatch> <http://JP_ontology.org/iso27001/ControlA.5.10> ;
                     <http://www.w3.org/2004/02/skos/core#note> "DPV Mapping Coverage: Complex Match"@en ,
                                                                """ISO - DPV Mapping Assumptions / Commentary: Code of Conduct, while also containing rules and guidelines, tends to focus more on ethical behavior, professionalism, and standards of conduct expected from individuals within the organisation. While it may include provisions related to information handling and asset management, its scope is generally narrower compared to organisational policies, as it primarily addresses behavioral expectations.
DPV: A set of rules or procedures outlining the norms and practices for conducting activities
The term Information Security Policy is broader because it encompasses a wider range of rules, guidelines, and procedures related to the management of information security within an organisation.
DPV: Policy regarding security of information"""@en ,
                                                                "This NIS2V Term aligns with Article 21.2 i: Human resources security, access control policies and asset management;"@en ;
                     <http://www.w3.org/2004/02/skos/core#prefLabel> "Acceptable Use Policy"@en ;
                     <http://www.w3.org/2004/02/skos/core#related> <https://w3id.org/dpv#CodeOfConduct> ,
                                                                   <https://w3id.org/dpv#InformationSecurityPolicy> .


:AccessControlPolicy <http://purl.org/dc/terms/contributor> "Jenni Parry" ;
                     <http://purl.org/dc/terms/created> "2024-06-04"^^xsd:date ;
                     <http://purl.org/dc/terms/source> "ISO 27001:2022 Control Framework"@en ;
                     rdfs:isDefinedBy <http://JP_ontology.org/nis2v> ;
                     <http://www.w3.org/2004/02/skos/core#altLabel> "NIS2V Term"@en ;
                     <http://www.w3.org/2004/02/skos/core#broader> <https://w3id.org/dpv#Restrict> ;
                     <http://www.w3.org/2004/02/skos/core#definition> "Access Control Policy: Policy specifying the restrictions and permissions governing access to information and associated assets, in alignment with established topic-specific guidelines on access control."@en ;
                     <http://www.w3.org/2004/02/skos/core#exactMatch> <http://JP_ontology.org/iso27001/ControlA.8.3> ;
                     <http://www.w3.org/2004/02/skos/core#note> "DPV Mapping Coverage: Broader Match"@en ,
                                                                """ISO - DPV Mapping Assumptions / Commentary: Restrict: This term is directly relevant but broad in its application to the control. 
DPV: to apply a restriction on the processing of specific records
The term Restrict broadly covers the action of imposing limitations on access, which is the core requirement of the control. However, without additional context or specificity, it doesn't convey the full scope of implementing access restrictions based on an established access control policy."""@en ,
                                                                "This NIS2V Term aligns with Article 21.2 i: Human resources security, access control policies and asset management;"@en ;
                     <http://www.w3.org/2004/02/skos/core#prefLabel> "Access Control Policy"@en .


:AccessRightsManagement <http://purl.org/dc/terms/contributor> "Jenni Parry" ;
                        <http://purl.org/dc/terms/created> "2024-06-04"^^xsd:date ;
                        <http://purl.org/dc/terms/source> "ISO 27001:2022 Control Framework"@en ;
                        rdfs:isDefinedBy <http://JP_ontology.org/nis2v> ;
                        <http://www.w3.org/2004/02/skos/core#altLabel> "NIS2V Term"@en ;
                        <http://www.w3.org/2004/02/skos/core#definition> "Access Rights Management: Systematic provisioning, review, modification, and removal of access rights based on organisational policies and rules for access control."@en ;
                        <http://www.w3.org/2004/02/skos/core#exactMatch> <http://JP_ontology.org/iso27001/ControlA.5.18> ;
                        <http://www.w3.org/2004/02/skos/core#narrower> <https://w3id.org/dpv#EnforceAccessControl> ;
                        <http://www.w3.org/2004/02/skos/core#note> "DPV Mapping Coverage: Narrower Match"@en ,
                                                                   """ISO - DPV Mapping Assumptions / Commentary: Narrower/Directly Relevant Terms: Enforce Access Control is narrowly focused, detailing aspects of the enforcement and methodology of access control. It is crucial for the implementation of the policy but represent specific components of the broader access rights management process outlined in the control.
DPV: Purposes associated with conducting or enforcing access control as a form of security"""@en ,
                                                                   "This NIS2V Term aligns with Article 21.2 g: Basic computer hygiene practices and cybersecurity training"@en ,
                                                                   "This NIS2V Term aligns with Article 21.2 i: Human resources security, access control policies and asset management;"@en ;
                        <http://www.w3.org/2004/02/skos/core#prefLabel> "Access Rights Management"@en .


:ActivityMonitoring <http://purl.org/dc/terms/contributor> "Jenni Parry" ;
                    <http://purl.org/dc/terms/created> "2024-06-04"^^xsd:date ;
                    <http://purl.org/dc/terms/source> "ISO 27001:2022 Control Framework"@en ;
                    rdfs:isDefinedBy <http://JP_ontology.org/nis2v> ;
                    <http://www.w3.org/2004/02/skos/core#altLabel> "NIS2V Term"@en ;
                    <http://www.w3.org/2004/02/skos/core#definition> "Activity Monitoring: Continuous monitoring of networks, systems, and applications for unusual activities, with steps taken to assess potential security incidents."@en ;
                    <http://www.w3.org/2004/02/skos/core#exactMatch> <http://JP_ontology.org/iso27001/ControlA.8.16> ,
                                                                     <https://w3id.org/dpv#ActivityMonitoring> ;
                    <http://www.w3.org/2004/02/skos/core#note> "DPV Mapping Coverage: Exact Match"@en ,
                                                               """ISO - DPV Mapping Assumptions / Commentary: The ISO control emphasizes the need for monitoring networks, systems, and applications for anomalous behavior to detect potential information security incidents. It focuses on the broader concept of monitoring within incident detection and response.
Activity Monitoring is defined in DPV as Monitoring of activities including assessing whether they have been successfully initiated and completed"""@en ,
                                                               "This NIS2V Term aligns with Article 21.2 b: Incident handling"@en ;
                    <http://www.w3.org/2004/02/skos/core#prefLabel> "Activity Monitoring"@en .


:ApplicationSecurityRequirements <http://purl.org/dc/terms/contributor> "Jenni Parry" ;
                                 <http://purl.org/dc/terms/created> "2024-05-01"^^xsd:date ;
                                 <http://purl.org/dc/terms/source> "ENISA: Minimum Security Measures for Operators of Essentials Services, https://www.enisa.europa.eu/topics/cybersecurity-policy/nis-directive-new/minimum-security-measures-for-operators-of-essentials-services"@en ;
                                 rdfs:isDefinedBy <http://JP_ontology.org/nis2v> ;
                                 <http://www.w3.org/2004/02/skos/core#altLabel> "NIS2V Term"@en ;
                                 <http://www.w3.org/2004/02/skos/core#definition> "Application Security Requirements are specifications and criteria that outline the security features, controls, and behaviors expected from software applications to protect against various threats and vulnerabilities, ensuring the confidentiality, integrity, and availability of data and functionality throughout the application's lifecycle. These requirements typically address authentication, authorization, data encryption, input validation, error handling, logging, and other security considerations specific to the application's context and environment."@en ,
                                                                                  "Secure System Architecture refers to the design and configuration of a system's components, networks, and interfaces in a way that minimizes security risks, protects against threats, and ensures the confidentiality, integrity, and availability of data and services. This includes implementing security controls, segmentation, least privilege access, encryption, and other measures to mitigate vulnerabilities and maintain a resilient and robust architecture."@en ;
                                 <http://www.w3.org/2004/02/skos/core#exactMatch> <http://JP_ontology.org/iso27001/ControlA.8.26> ,
                                                                                  <http://JP_ontology.org/iso27001/ControlA.8.27> ;
                                 <http://www.w3.org/2004/02/skos/core#note> "This NIS2V Term aligns with Article 21.2g: Basic computer hygiene practices and cybersecurity training."@en ;
                                 <http://www.w3.org/2004/02/skos/core#prefLabel> "Application Security Requirements"@en ,
                                                                                 "Secure System Architecture"@en .


:Article_21.2a <http://purl.org/dc/terms/contributor> "Jenni Parry" ;
               <http://purl.org/dc/terms/created> "2024-04-17"^^xsd:date ;
               <http://purl.org/dc/terms/source> "NIS2 Directive, https://eur-lex.europa.eu/eli/dir/2022/2555"@en ;
               rdfs:isDefinedBy <http://JP_ontology.org/nis2v> ;
               <http://www.w3.org/2004/02/skos/core#altLabel> "NIS2 Cybersecurity RiskManagement Measures Article 21.2a"@en ;
               <http://www.w3.org/2004/02/skos/core#broader> :NIS2VTerms ;
               <http://www.w3.org/2004/02/skos/core#definition> "Policies on risk analysis and information system security."@en ;
               <http://www.w3.org/2004/02/skos/core#prefLabel> "Article_21.2a"@en .


:Article_21.2b <http://purl.org/dc/terms/contributor> "Jenni Parry" ;
               <http://purl.org/dc/terms/created> "2024-04-17"^^xsd:date ;
               <http://purl.org/dc/terms/source> "NIS2 Directive, https://eur-lex.europa.eu/eli/dir/2022/2555"@en ;
               rdfs:isDefinedBy <http://JP_ontology.org/nis2v> ;
               <http://www.w3.org/2004/02/skos/core#altLabel> "NIS2 Cybersecurity RiskManagement Measures Article 21.2b"@en ;
               <http://www.w3.org/2004/02/skos/core#broader> :NIS2VTerms ;
               <http://www.w3.org/2004/02/skos/core#definition> "Incident handling, such as the prevention, detection, and response to incidents."@en ;
               <http://www.w3.org/2004/02/skos/core#prefLabel> "Article_21.2b"@en .


:Article_21.2c <http://purl.org/dc/terms/contributor> "Jenni Parry" ;
               <http://purl.org/dc/terms/created> "2024-04-17"^^xsd:date ;
               <http://purl.org/dc/terms/source> "NIS2 Directive, https://eur-lex.europa.eu/eli/dir/2022/2555"@en ;
               rdfs:isDefinedBy <http://JP_ontology.org/nis2v> ;
               <http://www.w3.org/2004/02/skos/core#altLabel> "NIS2 Cybersecurity RiskManagement Measures Article 21.2c"@en ;
               <http://www.w3.org/2004/02/skos/core#broader> :NIS2VTerms ;
               <http://www.w3.org/2004/02/skos/core#definition> "Business continuity management, including backup management, crisis management and disaster recovery."@en ;
               <http://www.w3.org/2004/02/skos/core#prefLabel> "Article_21.2c"@en .


:Article_21.2d <http://purl.org/dc/terms/contributor> "Jenni Parry" ;
               <http://purl.org/dc/terms/created> "2024-04-17"^^xsd:date ;
               <http://purl.org/dc/terms/source> "NIS2 Directive, https://eur-lex.europa.eu/eli/dir/2022/2555"@en ;
               rdfs:isDefinedBy <http://JP_ontology.org/nis2v> ;
               <http://www.w3.org/2004/02/skos/core#altLabel> "NIS2 Cybersecurity RiskManagement Measures Article 21.2d"@en ;
               <http://www.w3.org/2004/02/skos/core#broader> :NIS2VTerms ;
               <http://www.w3.org/2004/02/skos/core#definition> "Supply chain security including security-related aspects concerning the relationships between each entity and its suppliers or service providers."@en ;
               <http://www.w3.org/2004/02/skos/core#prefLabel> "Article_21.2d"@en .


:Article_21.2e <http://purl.org/dc/terms/contributor> "Jenni Parry" ;
               <http://purl.org/dc/terms/created> "2024-04-17"^^xsd:date ;
               <http://purl.org/dc/terms/source> "NIS2 Directive, https://eur-lex.europa.eu/eli/dir/2022/2555"@en ;
               rdfs:isDefinedBy <http://JP_ontology.org/nis2v> ;
               <http://www.w3.org/2004/02/skos/core#altLabel> "NIS2 Cybersecurity RiskManagement Measures Article 21.2e"@en ;
               <http://www.w3.org/2004/02/skos/core#broader> :NIS2VTerms ;
               <http://www.w3.org/2004/02/skos/core#definition> "Security in network and information systems acquisition, development and maintenance, including vulnerability handling and disclosure."@en ;
               <http://www.w3.org/2004/02/skos/core#prefLabel> "Article_21.2e"@en .


:Article_21.2f <http://purl.org/dc/terms/contributor> "Jenni Parry" ;
               <http://purl.org/dc/terms/created> "2024-04-17"^^xsd:date ;
               <http://purl.org/dc/terms/source> "NIS2 Directive, https://eur-lex.europa.eu/eli/dir/2022/2555"@en ;
               rdfs:isDefinedBy <http://JP_ontology.org/nis2v> ;
               <http://www.w3.org/2004/02/skos/core#altLabel> "NIS2 Cybersecurity RiskManagement Measures Article 21.2f"@en ;
               <http://www.w3.org/2004/02/skos/core#broader> :NIS2VTerms ;
               <http://www.w3.org/2004/02/skos/core#definition> "Policies and procedures (including testing and auditing) to assess the effectiveness of cybersecurity risk management measures."@en ;
               <http://www.w3.org/2004/02/skos/core#prefLabel> "Article_21.2f"@en .


:Article_21.2g <http://purl.org/dc/terms/contributor> "Jenni Parry" ;
               <http://purl.org/dc/terms/created> "2024-04-17"^^xsd:date ;
               <http://purl.org/dc/terms/source> "NIS2 Directive, https://eur-lex.europa.eu/eli/dir/2022/2555"@en ;
               rdfs:isDefinedBy <http://JP_ontology.org/nis2v> ;
               <http://www.w3.org/2004/02/skos/core#altLabel> "NIS2 Cybersecurity RiskManagement Measures Article 21.2g"@en ;
               <http://www.w3.org/2004/02/skos/core#broader> :NIS2VTerms ;
               <http://www.w3.org/2004/02/skos/core#definition> "Basic cyber hygiene practices and cybersecurity training."@en ;
               <http://www.w3.org/2004/02/skos/core#prefLabel> "Article_21.2g"@en .


:Article_21.2h <http://purl.org/dc/terms/contributor> "Jenni Parry" ;
               <http://purl.org/dc/terms/created> "2024-04-17"^^xsd:date ;
               <http://purl.org/dc/terms/source> "NIS2 Directive, https://eur-lex.europa.eu/eli/dir/2022/2555"@en ;
               rdfs:isDefinedBy <http://JP_ontology.org/nis2v> ;
               <http://www.w3.org/2004/02/skos/core#altLabel> "NIS2 Cybersecurity RiskManagement Measures Article 21.2h"@en ;
               <http://www.w3.org/2004/02/skos/core#broader> :NIS2VTerms ;
               <http://www.w3.org/2004/02/skos/core#definition> "Policies and procedures regarding the use of cryptography and, where appropriate, encryption."@en ;
               <http://www.w3.org/2004/02/skos/core#prefLabel> "Article_21.2h"@en .


:Article_21.2i <http://purl.org/dc/terms/contributor> "Jenni Parry" ;
               <http://purl.org/dc/terms/created> "2024-04-17"^^xsd:date ;
               <http://purl.org/dc/terms/source> "NIS2 Directive, https://eur-lex.europa.eu/eli/dir/2022/2555"@en ;
               rdfs:isDefinedBy <http://JP_ontology.org/nis2v> ;
               <http://www.w3.org/2004/02/skos/core#altLabel> "NIS2 Cybersecurity RiskManagement Measures Article 21.2i"@en ;
               <http://www.w3.org/2004/02/skos/core#broader> :NIS2VTerms ;
               <http://www.w3.org/2004/02/skos/core#definition> "Human resources security, access control policies and asset management."@en ;
               <http://www.w3.org/2004/02/skos/core#prefLabel> "Article_21.2i"@en .


:Article_21.2j <http://purl.org/dc/terms/contributor> "Jenni Parry" ;
               <http://purl.org/dc/terms/created> "2024-04-17"^^xsd:date ;
               <http://purl.org/dc/terms/source> "NIS2 Directive, https://eur-lex.europa.eu/eli/dir/2022/2555"@en ;
               rdfs:isDefinedBy <http://JP_ontology.org/nis2v> ;
               <http://www.w3.org/2004/02/skos/core#altLabel> "NIS2 Cybersecurity RiskManagement Measures Article 21.2j"@en ;
               <http://www.w3.org/2004/02/skos/core#broader> :NIS2VTerms ;
               <http://www.w3.org/2004/02/skos/core#definition> "Multi-factor authentication or continuous authentication solutions, secured voice, video and text communications and secured emergency communication systems within the entity, where appropriate."@en ;
               <http://www.w3.org/2004/02/skos/core#prefLabel> "Article_21.2j"@en .


:AssetManagementProcedures <http://purl.org/dc/terms/contributor> "Jenni Parry" ;
                           <http://purl.org/dc/terms/created> "2024-06-04"^^xsd:date ;
                           <http://purl.org/dc/terms/source> "ISO 27001:2022 Control Framework"@en ;
                           rdfs:isDefinedBy <http://JP_ontology.org/nis2v> ;
                           <http://www.w3.org/2004/02/skos/core#altLabel> "NIS2V Term"@en ;
                           <http://www.w3.org/2004/02/skos/core#definition> "Asset Management Procedures: Processes and practices implemented by an organisation to effectively identify, categorize, track, and manage its physical and digital assets throughout their lifecycle, including acquisition, deployment, utilization, maintenance, and disposal, with the aim of maximizing value, minimizing loss, and ensuring compliance with relevant policies and regulations."@en ;
                           <http://www.w3.org/2004/02/skos/core#exactMatch> <http://JP_ontology.org/iso27001/ControlA.5.9> ,
                                                                            <https://w3id.org/dpv#AssetManagementProcedures> ;
                           <http://www.w3.org/2004/02/skos/core#note> "DPV Mapping Coverage: Exact Match"@en ,
                                                                      "ISO - DPV Mapping Assumptions / Commentary: The term Asset Management Procedures is directly relevant and specific to the ISO control. The control emphasizes the development and maintenance of an inventory of information and associated assets, including ownership information. This inventory is essential for managing and safeguarding organisational assets effectively."@en ,
                                                                      "This NIS2V Term aligns with Article 21.2 i: Human resources security, access control policies and asset management;"@en ;
                           <http://www.w3.org/2004/02/skos/core#prefLabel> "Asset Management Procedures"@en .


:AuthenticationInformationManagement <http://purl.org/dc/terms/contributor> "Jenni Parry" ;
                                     <http://purl.org/dc/terms/created> "2024-06-05"^^xsd:date ;
                                     <http://purl.org/dc/terms/source> "ISO 27001:2022 Control Framework"@en ;
                                     rdfs:isDefinedBy <http://JP_ontology.org/nis2v> ;
                                     <http://www.w3.org/2004/02/skos/core#altLabel> "NIS2V Term"@en ;
                                     <http://www.w3.org/2004/02/skos/core#definition> "Authentication Information Management: Supervised allocation and handling of authentication credentials, with guidance provided to personnel on secure practices."@en ;
                                     <http://www.w3.org/2004/02/skos/core#exactMatch> <http://JP_ontology.org/iso27001/ControlA.5.17> ;
                                     <http://www.w3.org/2004/02/skos/core#note> "This NIS2V Term aligns with Article 21.2 g: Basic computer hygiene practices and cybersecurity training"@en ,
                                                                                "This NIS2V Term aligns with Article 21.2 i: Human resources security, access control policies and asset management;"@en ,
                                                                                "This NIS2V Term aligns with Article 21.2 j: The use of multi-factor authentication or continuous authentication solutions, secured voice, video and text communications and secured emergency communications systems within the entity, where appropriate"@en ;
                                     <http://www.w3.org/2004/02/skos/core#prefLabel> "Authentication Information Management"@en .


:AwarenessTraining <http://purl.org/dc/terms/contributor> "Jenni Parry" ;
                   <http://purl.org/dc/terms/created> "2024-06-04"^^xsd:date ;
                   <http://purl.org/dc/terms/source> "ISO 27001:2022 Control Framework"@en ;
                   rdfs:isDefinedBy <http://JP_ontology.org/nis2v> ;
                   <http://www.w3.org/2004/02/skos/core#altLabel> "NIS2V Term"@en ;
                   <http://www.w3.org/2004/02/skos/core#definition> "Awareness Training: Training provided to individuals working under the organisation's control to ensure awareness of the information security policy, their role in enhancing information security management system effectiveness, and the consequences of non-conformance with system requirements."@en ;
                   <http://www.w3.org/2004/02/skos/core#exactMatch> <http://JP_ontology.org/iso27001/Control7.3> ;
                   <http://www.w3.org/2004/02/skos/core#note> "DPV Mapping Coverage: Complex Match"@en ,
                                                              """ISO - DPV Mapping Assumptions / Commentary: The ISO control outlines the awareness requirements for individuals working under the organisation's control regarding information security policies, their contributions to the information security management system, and the implications of non-conformance.
Each term listed represents a specific aspect or method of increasing awareness within the organisation, focusing on training related to information security.
While these terms are relevant to increasing awareness, they represent narrower aspects within the broader context of organisational awareness of information security policies and management system requirements.
Cybersecurity Training - DPV: Training methods related to cybersecurity
Security Knowledge Training - DPV: Training intended to increase knowledge regarding security
Data Protection Training - DPV: Training intended to increase knowledge regarding data protection"""@en ,
                                                              "This NIS2V Term aligns with Article 21.2 g: Basic computer hygiene practices and cybersecurity training"@en ;
                   <http://www.w3.org/2004/02/skos/core#prefLabel> "Awareness Training"@en ;
                   <http://www.w3.org/2004/02/skos/core#related> <https://w3id.org/dpv#CybersecurityTraining> ,
                                                                 <https://w3id.org/dpv#DataProtectionTraining> ,
                                                                 <https://w3id.org/dpv#SecurityKnowledgeTraining> .


:BackupManagement <http://purl.org/dc/terms/contributor> "Jenni Parry" ;
                  <http://purl.org/dc/terms/created> "2024-06-04"^^xsd:date ;
                  <http://purl.org/dc/terms/source> "ISO 27001:2022 Control Framework"@en ;
                  rdfs:isDefinedBy <http://JP_ontology.org/nis2v> ;
                  <http://www.w3.org/2004/02/skos/core#altLabel> "NIS2V Term"@en ;
                  <http://www.w3.org/2004/02/skos/core#definition> "Backup Management: Regular maintenance and testing of backup copies of information, software, and systems, as stipulated by specific backup policies."@en ;
                  <http://www.w3.org/2004/02/skos/core#exactMatch> <http://JP_ontology.org/iso27001/ControlA.8.13> ;
                  <http://www.w3.org/2004/02/skos/core#narrower> <https://w3id.org/dpv#DataBackupProtocols> ;
                  <http://www.w3.org/2004/02/skos/core#note> "DPV Mapping Coverage: Narrower Match"@en ,
                                                             """ISO - DPV Mapping Assumptions / Commentary: The ISO control emphasizes the need for maintaining and regularly testing backup copies of information, software, and systems in accordance with the agreed backup policy. It focuses on the broader concept of backup management within information security practices. Data Backup Protocols is a narrower concept.
DPV: Protocols or plans for backing up of data"""@en ,
                                                             "This NIS2V Term aligns with Article 21.2 c: Business continuity, such as backup management and disaster recovery, and crisis management"@en ;
                  <http://www.w3.org/2004/02/skos/core#prefLabel> "Backup Management"@en .


:Capacitymanagement <http://purl.org/dc/terms/contributor> "Jenni Parry" ;
                    <http://purl.org/dc/terms/created> "2024-06-04"^^xsd:date ;
                    <http://purl.org/dc/terms/source> "ISO 27001:2022 Control Framework"@en ;
                    rdfs:isDefinedBy <http://JP_ontology.org/nis2v> ;
                    <http://www.w3.org/2004/02/skos/core#altLabel> "NIS2V Term"@en ;
                    <http://www.w3.org/2004/02/skos/core#definition> "Capacity management: The process of planning and controlling IT resources to meet current and future demands."@en ;
                    <http://www.w3.org/2004/02/skos/core#exactMatch> <http://JP_ontology.org/iso27001/ControlA.8.6> ;
                    <http://www.w3.org/2004/02/skos/core#narrower> <https://w3id.org/dpv#ActivityMonitoring> ;
                    <http://www.w3.org/2004/02/skos/core#note> "DPV Mapping Coverage: Narrower Match"@en ,
                                                               """ISO - DPV Mapping Assumptions / Commentary: This term relates to monitoring activities within the organisation. However, in this specific context, they may not directly address the aspect of monitoring resource usage in line with capacity requirements.
DPV: Monitoring of activities including assessing whether they have been successfully initiated and completed"""@en ,
                                                               "This NIS2V Term aligns with Article 21.2 c: Business continuity, such as backup management and disaster recovery, and crisis management"@en ;
                    <http://www.w3.org/2004/02/skos/core#prefLabel> "Capacity management"@en .


:ChangeManagement <http://purl.org/dc/terms/contributor> "Jenni Parry" ;
                  <http://purl.org/dc/terms/created> "2024-05-01"^^xsd:date ;
                  <http://purl.org/dc/terms/source> "ENISA: Minimum Security Measures for Operators of Essentials Services, https://www.enisa.europa.eu/topics/cybersecurity-policy/nis-directive-new/minimum-security-measures-for-operators-of-essentials-services"@en ;
                  rdfs:isDefinedBy <http://JP_ontology.org/nis2v> ;
                  <http://www.w3.org/2004/02/skos/core#altLabel> "NIS2V Term"@en ;
                  <http://www.w3.org/2004/02/skos/core#definition> "Change Management is a systematic approach to planning, implementing, and managing changes to processes, technologies, systems, or organisational structures within an organisation, aiming to minimize disruption, mitigate risks, and maximize benefits while ensuring effective communication, stakeholder engagement, and adoption of the changes."@en ;
                  <http://www.w3.org/2004/02/skos/core#exactMatch> <http://JP_ontology.org/iso27001/ControlA.8.32> ;
                  <http://www.w3.org/2004/02/skos/core#note> "This NIS2V Term aligns with Article 21.2g: Basic computer hygiene practices and cybersecurity training."@en ;
                  <http://www.w3.org/2004/02/skos/core#prefLabel> "Change Management"@en .


:ClearDeskAndClearScreen <http://purl.org/dc/terms/contributor> "Jenni Parry" ;
                         <http://purl.org/dc/terms/created> "2024-04-17"^^xsd:date ;
                         <http://purl.org/dc/terms/source> "ISO 27001:2022 Control Framework"@en ;
                         rdfs:isDefinedBy <http://JP_ontology.org/nis2v> ;
                         <http://www.w3.org/2004/02/skos/core#altLabel> "NIS2V Term"@en ;
                         <http://www.w3.org/2004/02/skos/core#definition> "The Clear Desk and Clear Screen practices are individual components of the Workplace Security Policy, each with their specific focussecuring physical items in the workspace and electronic information displayed on screens, respectively."@en ;
                         <http://www.w3.org/2004/02/skos/core#exactMatch> <http://JP_ontology.org/iso27001/ControlA.7.7> ;
                         <http://www.w3.org/2004/02/skos/core#note> "This NIS2V Term aligns with Article 21.2g: Basic cyber hygiene practices and cybersecurity training."@en ;
                         <http://www.w3.org/2004/02/skos/core#prefLabel> "Clear Desk and Clear Screen"@en .


:ClockSynchronization <http://purl.org/dc/terms/contributor> "Jenni Parry" ;
                      <http://purl.org/dc/terms/created> "2024-04-15"^^xsd:date ;
                      <http://purl.org/dc/terms/source> "ISO 27001:2022 Control Framework"@en ;
                      rdfs:isDefinedBy <http://JP_ontology.org/nis2v> ;
                      <http://www.w3.org/2004/02/skos/core#altLabel> "NIS2V Term"@en ;
                      <http://www.w3.org/2004/02/skos/core#definition> "The process of coordinating timekeeping among different systems to ensure the same time reference is used."@en ;
                      <http://www.w3.org/2004/02/skos/core#exactMatch> <http://JP_ontology.org/iso27001/ControlA.8.17> ;
                      <http://www.w3.org/2004/02/skos/core#note> "This NIS2V Term aligns with Article 21.2b: Incident handling, such as the prevention, detection, and response to incidents."@en ;
                      <http://www.w3.org/2004/02/skos/core#prefLabel> "Clock Synchronization"@en .


:CloudServiceManagement <http://purl.org/dc/terms/contributor> "Jenni Parry" ;
                        <http://purl.org/dc/terms/created> "2024-04-26"^^xsd:date ,
                                                           "2024-05-01"^^xsd:date ;
                        <http://purl.org/dc/terms/source> "ENISA: Minimum Security Measures for Operators of Essentials Services, https://www.enisa.europa.eu/topics/cybersecurity-policy/nis-directive-new/minimum-security-measures-for-operators-of-essentials-services"@en ,
                                                          "ISO 27001:2022 Control Framework"@en ;
                        rdfs:isDefinedBy <http://JP_ontology.org/nis2v> ;
                        <http://www.w3.org/2004/02/skos/core#altLabel> "NIS2V Term"@en ;
                        <http://www.w3.org/2004/02/skos/core#definition> "Establishment of processes for acquiring, using, managing, and exiting cloud services, aligned with the organisation's information security standards."@en ;
                        <http://www.w3.org/2004/02/skos/core#exactMatch> <http://JP_ontology.org/iso27001/ControlA.5.23> ;
                        <http://www.w3.org/2004/02/skos/core#note> "This NIS2V Term aligns with Article 21.2d: Supply chain security including security-related aspects concerning the relationships between each entity and its suppliers or service providers."@en ,
                                                                   "This NIS2V Term aligns with NIS2 Article 21.2d: Supply chain security, including security-related aspects concerning the relationships between each entity and its direct suppliers or service providers"@en ;
                        <http://www.w3.org/2004/02/skos/core#prefLabel> "Cloud Service Management"@en .


:Communication <http://purl.org/dc/terms/contributor> "Jenni Parry" ;
               <http://purl.org/dc/terms/created> "2024-04-26"^^xsd:date ;
               <http://purl.org/dc/terms/source> "ISO 27001:2022 Control Framework"@en ;
               rdfs:isDefinedBy <http://JP_ontology.org/nis2v> ;
               <http://www.w3.org/2004/02/skos/core#altLabel> "NIS2V Term"@en ;
               <http://www.w3.org/2004/02/skos/core#definition> "The organization is required to evaluate and manage all aspects of communications related to the information security management system, encompassing content, timing, audience, and methods."@en ;
               <http://www.w3.org/2004/02/skos/core#exactMatch> <http://JP_ontology.org/iso27001/Control7.4> ;
               <http://www.w3.org/2004/02/skos/core#note> "This NIS2V Term aligns with Article 21.2g: Basic cyber hygiene practices and cybersecurity training."@en ;
               <http://www.w3.org/2004/02/skos/core#prefLabel> "Communication"@en .


:CompetenceManagementForInformationSecurityPersonnel <http://purl.org/dc/terms/contributor> "Jenni Parry" ;
                                                     <http://purl.org/dc/terms/created> "2024-04-17"^^xsd:date ;
                                                     <http://purl.org/dc/terms/source> "ISO 27001:2022 Control Framework"@en ;
                                                     rdfs:isDefinedBy <http://JP_ontology.org/nis2v> ;
                                                     <http://www.w3.org/2004/02/skos/core#altLabel> "NIS2V Term"@en ;
                                                     <http://www.w3.org/2004/02/skos/core#broader> :Article_21.2i ;
                                                     <http://www.w3.org/2004/02/skos/core#definition> "The process of ensuring that personnel responsible for information security possess and maintain the necessary skills, knowledge, and abilities to perform their roles effectively. This includes ongoing training, certification, and performance evaluation."@en ;
                                                     <http://www.w3.org/2004/02/skos/core#exactMatch> <http://JP_ontology.org/iso27001/Control7.2> ;
                                                     <http://www.w3.org/2004/02/skos/core#note> "This NIS2V Term aligns with Article 21.2g: Basic cyber hygiene practices and cybersecurity training and Article21.2i: Human resources security, access control policies and asset management."@en ;
                                                     <http://www.w3.org/2004/02/skos/core#prefLabel> "Competence Management for Information Security Personnel"@en .


:ComplianceManagement <http://purl.org/dc/terms/contributor> "Jenni Parry" ;
                      <http://purl.org/dc/terms/created> "2024-06-04"^^xsd:date ;
                      <http://purl.org/dc/terms/source> "ISO 27001:2022 Control Framework"@en ;
                      rdfs:isDefinedBy <http://JP_ontology.org/nis2v> ;
                      <http://www.w3.org/2004/02/skos/core#altLabel> "NIS2V Term"@en ;
                      <http://www.w3.org/2004/02/skos/core#definition> "Compliance Management: Identification, documentation, and ongoing updating of legal, statutory, regulatory, and contractual information security requirements, aligned with organisational compliance strategies."@en ;
                      <http://www.w3.org/2004/02/skos/core#exactMatch> <http://JP_ontology.org/iso27001/ControlA.5.31> ;
                      <http://www.w3.org/2004/02/skos/core#narrower> <https://w3id.org/dpv#ContractualTerms> ;
                      <http://www.w3.org/2004/02/skos/core#note> "DPV Mapping Coverage: Narrower Match"@en ,
                                                                 """ISO - DPV Mapping Assumptions / Commentary: Contractual Terms: This term directly relates to the contractual requirements part of the control statement. It refers to the specific conditions and stipulations outlined in contracts that an organisation must adhere to. While it's directly relevant to one aspect of the control, it doesn't cover the legal, statutory, or regulatory requirements.
DPV: Contractual terms governing data handling within or with an entity"""@en ,
                                                                 "This NIS2V Term aligns with Article 21.2 a: Policies on risk analysis and information system security"@en ;
                      <http://www.w3.org/2004/02/skos/core#prefLabel> "Compliance Management"@en .


:ContactWithAuthorities <http://purl.org/dc/terms/contributor> "Jenni Parry" ;
                        <http://purl.org/dc/terms/created> "2024-04-24"^^xsd:date ;
                        <http://purl.org/dc/terms/source> "ISO 27001:2022 Control Framework"@en ;
                        rdfs:isDefinedBy <http://JP_ontology.org/nis2v> ;
                        <http://www.w3.org/2004/02/skos/core#altLabel> "NIS2V Term"@en ;
                        <http://www.w3.org/2004/02/skos/core#definition> "Contact with Authorities: Involves interactions between individuals, organisations, or entities and government or regulatory bodies for various purposes such as compliance, reporting, or seeking permissions."@en ;
                        <http://www.w3.org/2004/02/skos/core#exactMatch> <http://JP_ontology.org/iso27001/ControlA.5.5> ;
                        <http://www.w3.org/2004/02/skos/core#note> "This NIS2V Term aligns with Article 21.2a: Policies on risk analysis and information system security."@en ;
                        <http://www.w3.org/2004/02/skos/core#prefLabel> "Contact with Authorities"@en .


:ContactWithSpecialInterestGroups <http://purl.org/dc/terms/contributor> "Jenni Parry" ;
                                  <http://purl.org/dc/terms/created> "2024-04-24"^^xsd:date ;
                                  <http://purl.org/dc/terms/source> "ISO 27001:2022 Control Framework"@en ;
                                  rdfs:isDefinedBy <http://JP_ontology.org/nis2v> ;
                                  <http://www.w3.org/2004/02/skos/core#altLabel> "NIS2V Term"@en ;
                                  <http://www.w3.org/2004/02/skos/core#definition> "Contact with special interest groups: Refers to interactions between individuals, organisations, or entities and advocacy groups or organisations that represent specific causes, industries, or interests, often to influence policy, regulations, or public opinion."@en ;
                                  <http://www.w3.org/2004/02/skos/core#exactMatch> <http://JP_ontology.org/iso27001/ControlA.5.6> ;
                                  <http://www.w3.org/2004/02/skos/core#note> "This NIS2V Term aligns with Article 21.2a: Policies on risk analysis and information system security."@en ;
                                  <http://www.w3.org/2004/02/skos/core#prefLabel> "Contact with Special Interest Groups"@en .


:ContextOfTheOrganisation <http://purl.org/dc/terms/contributor> "Jenni Parry" ;
                          <http://purl.org/dc/terms/created> "2024-04-24"^^xsd:date ;
                          <http://purl.org/dc/terms/source> "ISO 27001:2022 Control Framework"@en ;
                          rdfs:isDefinedBy <http://JP_ontology.org/nis2v> ;
                          <http://www.w3.org/2004/02/skos/core#altLabel> "NIS2V Term"@en ;
                          <http://www.w3.org/2004/02/skos/core#definition> "Context of the Organisation: Refers to the internal and external factors that influence an organisation's strategic decisions and operations."@en ;
                          <http://www.w3.org/2004/02/skos/core#exactMatch> <http://JP_ontology.org/iso27001/Control4> ;
                          <http://www.w3.org/2004/02/skos/core#note> "This NIS2V Term aligns with Article 21.2a: Policies on risk analysis and information system security."@en ;
                          <http://www.w3.org/2004/02/skos/core#prefLabel> "Context of the Organisation"@en .


:ContinualImprovement <http://purl.org/dc/terms/contributor> "Jenni Parry" ;
                      <http://purl.org/dc/terms/created> "2024-05-01"^^xsd:date ;
                      <http://purl.org/dc/terms/source> "ENISA: Minimum Security Measures for Operators of Essentials Services, https://www.enisa.europa.eu/topics/cybersecurity-policy/nis-directive-new/minimum-security-measures-for-operators-of-essentials-services"@en ;
                      rdfs:isDefinedBy <http://JP_ontology.org/nis2v> ;
                      <http://www.w3.org/2004/02/skos/core#altLabel> "NIS2V Term"@en ;
                      <http://www.w3.org/2004/02/skos/core#definition> "The ongoing process of enhancing an organisation's performance, processes, products, or services through systematic and incremental changes."@en ;
                      <http://www.w3.org/2004/02/skos/core#exactMatch> <http://JP_ontology.org/iso27001/Control10.1> ;
                      <http://www.w3.org/2004/02/skos/core#note> "This NIS2V Term aligns with Article 21.2f: Policies and procedures to assess the effectiveness of cybersecurity risk management measures."@en ;
                      <http://www.w3.org/2004/02/skos/core#prefLabel> "Continual Improvement"@en .


:CryptographyPolicy <http://purl.org/dc/terms/contributor> "Jenni Parry" ;
                    <http://purl.org/dc/terms/created> "2024-06-04"^^xsd:date ;
                    <http://purl.org/dc/terms/source> "ISO 27001:2022 Control Framework"@en ;
                    rdfs:isDefinedBy <http://JP_ontology.org/nis2v> ;
                    <http://www.w3.org/2004/02/skos/core#altLabel> "NIS2V Term"@en ;
                    <http://www.w3.org/2004/02/skos/core#definition> "Cryptography Policy: Establishment and enforcement of rules governing the effective utilisation of cryptography within the organisation, encompassing cryptographic key management and implementation guidelines."@en ;
                    <http://www.w3.org/2004/02/skos/core#exactMatch> <http://JP_ontology.org/iso27001/ControlA.8.24> ;
                    <http://www.w3.org/2004/02/skos/core#note> "DPV Mapping Coverage: Complex Match"@en ,
                                                               """ISO - DPV Mapping Assumptions / Commentary: The ISO control focuses on defining and implementing rules for the effective use of cryptography and cryptographic key management. BroaderMatch: Cryptographic Methods offer a broader overview of the field, covering the range of techniques and processes that the defined rules for effective use of cryptography would govern.
DPV: Use of cryptographic methods to perform tasks
Directly Aligned: Cryptographic Key Management is directly aligned with part of the control's emphasis, specifically addressing the management aspect of cryptographic practices.
DPV: Management of cryptographic keys, including their generation, storage, assessment, and safekeeping."""@en ,
                                                               "This NIS2V Term aligns with Article 21.2 h: Policies and procedures regarding the use of cryptography and, where appropriate, encryption"@en ;
                    <http://www.w3.org/2004/02/skos/core#prefLabel> "Cryptography Policy"@en ;
                    <http://www.w3.org/2004/02/skos/core#related> <https://w3id.org/dpv#CryptographicKeyManagement> ,
                                                                  <https://w3id.org/dpv#CryptographicMethods> .


:DataLeakagePrevention <http://purl.org/dc/terms/contributor> "Jenni Parry" ;
                       <http://purl.org/dc/terms/created> "2024-06-04"^^xsd:date ;
                       <http://purl.org/dc/terms/source> "ISO 27001:2022 Control Framework"@en ;
                       rdfs:isDefinedBy <http://JP_ontology.org/nis2v> ;
                       <http://www.w3.org/2004/02/skos/core#altLabel> "NIS2V Term"@en ;
                       <http://www.w3.org/2004/02/skos/core#broader> <https://w3id.org/dpv#DataSecurityManagement> ;
                       <http://www.w3.org/2004/02/skos/core#definition> "Data Leakage Prevention: A set of practices aimed at ensuring sensitive data is not lost, misused, or accessed by unauthorized users."@en ;
                       <http://www.w3.org/2004/02/skos/core#exactMatch> <http://JP_ontology.org/iso27001/ControlA.8.12> ;
                       <http://www.w3.org/2004/02/skos/core#note> "DPV Mapping Coverage: Broader Match"@en ,
                                                                  """ISO - DPV Mapping Assumptions / Commentary: This ISO Control focuses on preventing the unauthorised disclosure of sensitive information. It's a narrower focus within the broader context of Data Security Management.
DPV: Measures associated with management of data security."""@en ,
                                                                  "This NIS2V Term aligns with Article 21.2 j: The use of multi-factor authentication or continuous authentication solutions, secured voice, video and text communications and secured emergency communications systems within the entity, where appropriate"@en ;
                       <http://www.w3.org/2004/02/skos/core#prefLabel> "Data Leakage Prevention  "@en .


:DisasterRecoveryProcedures <http://purl.org/dc/terms/contributor> "Jenni Parry" ;
                            <http://purl.org/dc/terms/created> "2024-06-04"^^xsd:date ;
                            <http://purl.org/dc/terms/source> "ISO 27001:2022 Control Framework"@en ;
                            rdfs:isDefinedBy <http://JP_ontology.org/nis2v> ;
                            <http://www.w3.org/2004/02/skos/core#altLabel> "NIS2V Term"@en ;
                            <http://www.w3.org/2004/02/skos/core#definition> "Disaster Recovery Procedures: Strategic planning by the organisation to uphold information security standards during periods of disruption."@en ;
                            <http://www.w3.org/2004/02/skos/core#exactMatch> <http://JP_ontology.org/iso27001/ControlA.5.29> ,
                                                                             <https://w3id.org/dpv#DisasterRecoveryProcedures> ;
                            <http://www.w3.org/2004/02/skos/core#note> "DPV Mapping Coverage: Exact Match"@en ,
                                                                       "ISO - DPV Mapping Assumptions / Commentary: The ISO control focuses on maintaining information security at an appropriate level during disruption. This DPV term is defined as Procedures related to management of disasters and recovery"@en ,
                                                                       "This NIS2V Term aligns with Article 21.2 c: Business continuity, such as backup management and disaster recovery, and crisis management"@en ;
                            <http://www.w3.org/2004/02/skos/core#prefLabel> "Disaster Recovery Procedures"@en .


:Disciplinaryprocess <http://purl.org/dc/terms/contributor> "Jenni Parry" ;
                     <http://purl.org/dc/terms/created> "2024-06-04"^^xsd:date ;
                     <http://purl.org/dc/terms/source> "ISO 27001:2022 Control Framework"@en ;
                     rdfs:isDefinedBy <http://JP_ontology.org/nis2v> ;
                     <http://www.w3.org/2004/02/skos/core#altLabel> "NIS2V Term"@en ;
                     <http://www.w3.org/2004/02/skos/core#definition> "Disciplinary process: Procedures for dealing with violations of rules or policies within an organisation."@en ;
                     <http://www.w3.org/2004/02/skos/core#exactMatch> <http://JP_ontology.org/iso27001/ControlA.6.4> ;
                     <http://www.w3.org/2004/02/skos/core#narrower> <https://w3id.org/dpv#CodeOfConduct> ;
                     <http://www.w3.org/2004/02/skos/core#note> "DPV Mapping Coverage: Narrower Match"@en ,
                                                                """ISO - DPV Mapping Assumptions / Commentary: The ISO control is a broader concept encompassing the establishment and communication of disciplinary procedures for violations of information security policies, which may include the code of conduct and information security policy.
DPV: A set of rules or procedures outlining the norms and practices for conducting activities"""@en ,
                                                                "This NIS2V Term aligns with Article 21.2 i: Human resources security, access control policies and asset management;"@en ;
                     <http://www.w3.org/2004/02/skos/core#prefLabel> "Disciplinary process"@en .


:DocumentedOperatingProcedures <http://purl.org/dc/terms/contributor> "Jenni Parry" ;
                               <http://purl.org/dc/terms/created> "2024-04-15"^^xsd:date ;
                               <http://purl.org/dc/terms/source> "ISO 27001:2022 Control Framework"@en ;
                               rdfs:isDefinedBy <http://JP_ontology.org/nis2v> ;
                               <http://www.w3.org/2004/02/skos/core#altLabel> "NIS2V Term"@en ;
                               <http://www.w3.org/2004/02/skos/core#broader> :Article_21.2c ,
                                                                             :Article_21.2e ,
                                                                             :Article_21.2h ;
                               <http://www.w3.org/2004/02/skos/core#definition> "Documented Operating Procedures: Written instructions detailing the step-by-step processes and protocols to be followed in carrying out specific tasks or activities within an organisation."@en ;
                               <http://www.w3.org/2004/02/skos/core#exactMatch> <http://JP_ontology.org/iso27001/ControlA.5.37> ;
                               <http://www.w3.org/2004/02/skos/core#note> "This NIS2V Term aligns with Article 21.2a: Policies on risk analysis and information system security, Article 21.2c: Business continuity management, including backup management, crisis management and disaster recovery, Article 21.2e: Basic cyber hygiene practices and cybersecurity training, and Article 21.2h: Policies and procedures regarding the use of cryptography and, where appropriate, encryption."@en ;
                               <http://www.w3.org/2004/02/skos/core#prefLabel> "Documented Operating Procedures"@en .


:EndpointDeviceSecurityMeasures <http://purl.org/dc/terms/contributor> "Jenni Parry" ;
                                <http://purl.org/dc/terms/created> "2024-06-04"^^xsd:date ;
                                <http://purl.org/dc/terms/source> "ISO 27001:2022 Control Framework"@en ;
                                rdfs:isDefinedBy <http://JP_ontology.org/nis2v> ;
                                <http://www.w3.org/2004/02/skos/core#altLabel> "NIS2V Term"@en ;
                                <http://www.w3.org/2004/02/skos/core#definition> "Endpoint Device Security Measures: Protection mechanisms implemented to safeguard information stored on, processed by, or accessible via user endpoint devices."@en ;
                                <http://www.w3.org/2004/02/skos/core#exactMatch> <http://JP_ontology.org/iso27001/ControlA.8.1> ;
                                <http://www.w3.org/2004/02/skos/core#note> "DPV Mapping Coverage: Complex Match"@en ,
                                                                           """ISO - DPV Mapping Assumptions / Commentary: The ISO control emphasizes the need to protect information stored on, processed by, or accessible via user endpoint devices. It highlights the importance of safeguarding data on these devices from unauthorized access, modification, or disclosure.
File System Security is a narrower term that focus on specific aspects of data protection within endpoint devices. 
DPV: Security implemented over a file system
Operating System Security is a narrower term that addresses security measures implemented at the operating system level of user endpoint devices. 
DPV: Security implemented at or through operating systems"""@en ,
                                                                           "This NIS2V Term aligns with Article 21.2 i: Human resources security, access control policies and asset management;"@en ;
                                <http://www.w3.org/2004/02/skos/core#prefLabel> "Endpoint Device Security Measures"@en ;
                                <http://www.w3.org/2004/02/skos/core#related> <https://w3id.org/dpv#FileSystemSecurity> ,
                                                                              <https://w3id.org/dpv#OperatingSystemSecurity> .


:EnforceAccessControl <http://purl.org/dc/terms/contributor> "Jenni Parry" ;
                      <http://purl.org/dc/terms/created> "2024-06-04"^^xsd:date ;
                      <http://purl.org/dc/terms/source> "ISO 27001:2022 Control Framework"@en ;
                      rdfs:isDefinedBy <http://JP_ontology.org/nis2v> ;
                      <http://www.w3.org/2004/02/skos/core#altLabel> "NIS2V Term"@en ;
                      <http://www.w3.org/2004/02/skos/core#definition> "Access Control Regulation: Establishment and enforcement of rules for physical and logical access to information, aligning with business and security needs."@en ;
                      <http://www.w3.org/2004/02/skos/core#exactMatch> <http://JP_ontology.org/iso27001/ControlA.5.15> ,
                                                                       <https://w3id.org/dpv#EnforceAccessControl> ;
                      <http://www.w3.org/2004/02/skos/core#note> "DPV Mapping Coverage: Exact Match"@en ,
                                                                 "ISO - DPV Mapping Assumptions / Commentary: Enforce Access Control defines the purposes associated with conducting or enforcing access control as a form of security"@en ,
                                                                 "This NIS2V Term aligns with Article 21.2 g: Basic computer hygiene practices and cybersecurity training"@en ,
                                                                 "This NIS2V Term aligns with Article 21.2 i: Human resources security, access control policies and asset management;"@en ;
                      <http://www.w3.org/2004/02/skos/core#prefLabel> "Enforce Access Control"@en .


:EquipmentMaintenance <http://purl.org/dc/terms/contributor> "Jenni Parry" ;
                      <http://purl.org/dc/terms/created> "2024-05-01"^^xsd:date ;
                      <http://purl.org/dc/terms/source> "ENISA: Minimum Security Measures for Operators of Essentials Services, https://www.enisa.europa.eu/topics/cybersecurity-policy/nis-directive-new/minimum-security-measures-for-operators-of-essentials-services"@en ;
                      rdfs:isDefinedBy <http://JP_ontology.org/nis2v> ;
                      <http://www.w3.org/2004/02/skos/core#altLabel> "NIS2V Term"@en ;
                      <http://www.w3.org/2004/02/skos/core#definition> "Equipment Maintenance involves the regular upkeep, inspection, servicing, and repair of physical assets, machinery, tools, and devices within an organisation to ensure their proper functioning, reliability, and longevity. This includes preventive maintenance tasks, such as cleaning, lubrication, calibration, and replacement of worn-out parts, as well as reactive maintenance to address unexpected failures or malfunctions promptly. Effective equipment maintenance programs help minimize downtime, reduce costs, and extend the lifespan of equipment."@en ;
                      <http://www.w3.org/2004/02/skos/core#exactMatch> <http://JP_ontology.org/iso27001/ControlA.7.13> ;
                      <http://www.w3.org/2004/02/skos/core#note> "This NIS2V Term aligns with Article 21.2i: Human resources security, access control policies and asset management."@en ;
                      <http://www.w3.org/2004/02/skos/core#prefLabel> "Equipment Maintenance"@en .


:EvidenceCollection <http://purl.org/dc/terms/contributor> "Jenni Parry" ;
                    <http://purl.org/dc/terms/created> "2024-05-01"^^xsd:date ;
                    <http://purl.org/dc/terms/source> "ENISA: Minimum Security Measures for Operators of Essentials Services, https://www.enisa.europa.eu/topics/cybersecurity-policy/nis-directive-new/minimum-security-measures-for-operators-of-essentials-services"@en ;
                    rdfs:isDefinedBy <http://JP_ontology.org/nis2v> ;
                    <http://www.w3.org/2004/02/skos/core#altLabel> "NIS2V Term"@en ;
                    <http://www.w3.org/2004/02/skos/core#definition> "The process of gathering, preserving, and documenting digital or physical evidence relevant to an investigation or legal proceeding."@en ;
                    <http://www.w3.org/2004/02/skos/core#exactMatch> <http://JP_ontology.org/iso27001/ControlA.5.28> ;
                    <http://www.w3.org/2004/02/skos/core#note> "This NIS2V Term aligns with NIS2 Article 21.2b: Incident handling, specifically related to the prevention, detection, and response to incidents."@en ;
                    <http://www.w3.org/2004/02/skos/core#prefLabel> "Evidence Collection"@en .


:ExternalWebsiteAccessManagement <http://purl.org/dc/terms/contributor> "Jenni Parry" ;
                                 <http://purl.org/dc/terms/created> "2024-06-04"^^xsd:date ;
                                 <http://purl.org/dc/terms/source> "ISO 27001:2022 Control Framework"@en ;
                                 rdfs:isDefinedBy <http://JP_ontology.org/nis2v> ;
                                 <http://www.w3.org/2004/02/skos/core#altLabel> "NIS2V Term"@en ;
                                 <http://www.w3.org/2004/02/skos/core#definition> "External Website Access Management: Management of access to external websites to minimize the risk of exposure to malicious content."@en ;
                                 <http://www.w3.org/2004/02/skos/core#exactMatch> <http://JP_ontology.org/iso27001/ControlA.8.23> ;
                                 <http://www.w3.org/2004/02/skos/core#narrower> <https://w3id.org/dpv#WebSecurityProtocols> ;
                                 <http://www.w3.org/2004/02/skos/core#note> "DPV Mapping Coverage: Narrower Match"@en ,
                                                                            """ISO - DPV Mapping Assumptions / Commentary: Web Security Protocols is a narrower term that directly contributes to achieving the control's objective by focusing on the secure transmission of data over the web. It's essential but represents only a part of the broader strategy required to manage access to external websites effectively.
DPV: Security implemented at or over web-based protocols"""@en ,
                                                                            "This NIS2V Term aligns with Article 21.2 e: Security in network and information systems acquisition, development and maintenance, including vulnerability handling and disclosure"@en ;
                                 <http://www.w3.org/2004/02/skos/core#prefLabel> "External Website Access Management"@en .


:ICTContinuityManagement <http://purl.org/dc/terms/contributor> "Jenni Parry" ;
                         <http://purl.org/dc/terms/created> "2024-06-04"^^xsd:date ;
                         <http://purl.org/dc/terms/source> "ISO 27001:2022 Control Framework"@en ;
                         rdfs:isDefinedBy <http://JP_ontology.org/nis2v> ;
                         <http://www.w3.org/2004/02/skos/core#altLabel> "NIS2V Term"@en ;
                         <http://www.w3.org/2004/02/skos/core#broader> <https://w3id.org/dpv#DisasterRecoveryProcedures> ;
                         <http://www.w3.org/2004/02/skos/core#definition> "ICT Continuity Management: Planning, implementation, maintenance, and testing of ICT readiness to meet business continuity objectives and specific ICT continuity needs."@en ;
                         <http://www.w3.org/2004/02/skos/core#exactMatch> <http://JP_ontology.org/iso27001/ControlA.5.30> ;
                         <http://www.w3.org/2004/02/skos/core#note> "DPV Mapping Coverage: Broader Match"@en ,
                                                                    "ISO - DPV Mapping Assumptions / Commentary: The ISO control is a broader concept encompassing the planning, implementation, maintenance, and testing of ICT readiness, which may include disaster recovery procedures as part of the overall readiness plan."@en ,
                                                                    "This NIS2V Term aligns with Article 21.2 c: Business continuity, such as backup management and disaster recovery, and crisis management"@en ;
                         <http://www.w3.org/2004/02/skos/core#prefLabel> "ICT Continuity Management"@en .


:ICTandSupplyChainVigilance <http://purl.org/dc/terms/contributor> "Jenni Parry" ;
                            <http://purl.org/dc/terms/created> "2024-06-04"^^xsd:date ;
                            <http://purl.org/dc/terms/source> "ISO 27001:2022 Control Framework"@en ;
                            rdfs:isDefinedBy <http://JP_ontology.org/nis2v> ;
                            <http://www.w3.org/2004/02/skos/core#altLabel> "NIS2V Term"@en ;
                            <http://www.w3.org/2004/02/skos/core#definition> "ICT and Supply Chain Vigilance: The ongoing monitoring and proactive oversight of Information and Communication Technology (ICT) products and services within the supply chain to identify and mitigate potential security risks or vulnerabilities."@en ;
                            <http://www.w3.org/2004/02/skos/core#exactMatch> <http://JP_ontology.org/iso27001/ControlA.5.21> ;
                            <http://www.w3.org/2004/02/skos/core#note> "DPV Mapping Coverage: Complex Match"@en ,
                                                                       """ISO - DPV Mapping Assumptions / Commentary: Linking these DPV terms with clear relationships can accurately capture the essence of the control. The broader terms provide the context and framework, while the more specific terms like Risk Mitigation Measure, Third Party Contract, and Vendor Management detail the operational execution of supply chain risk management.
Broad Frameworks: Organisation Risk Management process sets the overarching framework for risk management activities, including those for the ICT supply chain.
DPV: Purposes associated with managing risk for organisation's activities
Critical Components: Vendor Management is essential for the practical aspects of managing supply chain risks, focusing on the relationships with suppliers and the contractual mechanisms to control risks.
DPV: Purposes associated with manage orders, payment, evaluation, and prospecting related to vendors"""@en ,
                                                                       "This NIS2V Term aligns with Article 21.2 d: Supply chain security, including security-related aspects concerning the relationships between each entity and its direct suppliers or service providers "@en ;
                            <http://www.w3.org/2004/02/skos/core#prefLabel> "ICT and Supply Chain Vigilance"@en ;
                            <http://www.w3.org/2004/02/skos/core#related> <https://w3id.org/dpv#OrganisationRiskManagement> ,
                                                                          <https://w3id.org/dpv#VendorManagement> .


:ISMSDocumentationRequirements <http://purl.org/dc/terms/contributor> "Jenni Parry" ;
                               <http://purl.org/dc/terms/created> "2024-04-15"^^xsd:date ;
                               <http://purl.org/dc/terms/source> "ISO 27001:2022 Control Framework"@en ;
                               rdfs:isDefinedBy <http://JP_ontology.org/nis2v> ;
                               <http://www.w3.org/2004/02/skos/core#altLabel> "NIS2V Term"@en ;
                               <http://www.w3.org/2004/02/skos/core#definition> "ISMS Documentation Requirements: This refers to adhering to the specific documentation needs mandated by an Information Security Management System (ISMS). This includes policies, procedures, and records that demonstrate the ISMS is designed, implemented, and maintained according to the standards (like ISO/IEC 27001)."@en ;
                               <http://www.w3.org/2004/02/skos/core#exactMatch> <http://JP_ontology.org/iso27001/Control7.5> ;
                               <http://www.w3.org/2004/02/skos/core#note> "This NIS2V Term aligns with Article 21.2a: Policies on risk analysis and information system security."@en ;
                               <http://www.w3.org/2004/02/skos/core#prefLabel> "ISMS Documentation Requirements"@en .


:IdentityManagementMethod <http://purl.org/dc/terms/contributor> "Jenni Parry" ;
                          <http://purl.org/dc/terms/created> "2024-06-04"^^xsd:date ;
                          <http://purl.org/dc/terms/source> "ISO 27001:2022 Control Framework"@en ;
                          rdfs:isDefinedBy <http://JP_ontology.org/nis2v> ;
                          <http://www.w3.org/2004/02/skos/core#altLabel> "NIS2V Term"@en ;
                          <http://www.w3.org/2004/02/skos/core#definition> "Identity Lifecycle Management: Comprehensive management of user identities throughout their entire lifecycle within the organisation."@en ;
                          <http://www.w3.org/2004/02/skos/core#exactMatch> <http://JP_ontology.org/iso27001/ControlA.5.16> ,
                                                                           <https://w3id.org/dpv#IdentityManagementMethod> ;
                          <http://www.w3.org/2004/02/skos/core#note> "DPV Mapping Coverage: Exact Match"@en ,
                                                                     "ISO - DPV Mapping Assumptions / Commentary: Identity Management Method covers the overall process. DPV defines it as the management of identity and identity-based processes."@en ,
                                                                     "This NIS2V Term aligns with Article 21.2 g: Basic computer hygiene practices and cybersecurity training"@en ,
                                                                     "This NIS2V Term aligns with Article 21.2 i: Human resources security, access control policies and asset management;"@en ,
                                                                     "This NIS2V Term aligns with Article 21.2 j: The use of multi-factor authentication or continuous authentication solutions, secured voice, video and text communications and secured emergency communications systems within the entity, where appropriate"@en ;
                          <http://www.w3.org/2004/02/skos/core#prefLabel> "Identity Management Method"@en .


:IncidentKnowledgeApplication <http://purl.org/dc/terms/contributor> "Jenni Parry" ;
                              <http://purl.org/dc/terms/created> "2024-06-05"^^xsd:date ;
                              <http://purl.org/dc/terms/source> "ISO 27001:2022 Control Framework"@en ;
                              rdfs:isDefinedBy <http://JP_ontology.org/nis2v> ;
                              <http://www.w3.org/2004/02/skos/core#altLabel> "NIS2V Term"@en ;
                              <http://www.w3.org/2004/02/skos/core#definition> "Incident Knowledge Application: utilisation of insights from security incidents to enhance and refine information security controls."@en ;
                              <http://www.w3.org/2004/02/skos/core#exactMatch> <http://JP_ontology.org/iso27001/ControlA.5.27> ;
                              <http://www.w3.org/2004/02/skos/core#note> "This NIS2V Term aligns with Article 21.2 b: Incident handling"@en ;
                              <http://www.w3.org/2004/02/skos/core#prefLabel> "Incident Knowledge Application"@en .


:IncidentResponseManagement <http://purl.org/dc/terms/contributor> "Jenni Parry" ;
                            <http://purl.org/dc/terms/created> "2024-06-04"^^xsd:date ;
                            <http://purl.org/dc/terms/source> "ISO 27001:2022 Control Framework"@en ;
                            rdfs:isDefinedBy <http://JP_ontology.org/nis2v> ;
                            <http://www.w3.org/2004/02/skos/core#altLabel> "NIS2V Term"@en ;
                            <http://www.w3.org/2004/02/skos/core#broader> <https://w3id.org/dpv#IncidentManagementProcedures> ;
                            <http://www.w3.org/2004/02/skos/core#definition> "Incident Response Management: Handling of information security incidents following established and documented procedures."@en ;
                            <http://www.w3.org/2004/02/skos/core#exactMatch> <http://JP_ontology.org/iso27001/ControlA.5.26> ;
                            <http://www.w3.org/2004/02/skos/core#note> "DPV Mapping Coverage: Broader Match"@en ,
                                                                       """ISO - DPV Mapping Assumptions / Commentary: Incident Management Procedures is a broader term than the ISO control as it encompassing various procedures and protocols related to managing incidents.
DPV: Procedures related to management of incidents"""@en ,
                                                                       "This NIS2V Term aligns with Article 21.2 b: Incident handling"@en ;
                            <http://www.w3.org/2004/02/skos/core#prefLabel> "Incident Response Management"@en .


:IndependentSecurityReview <http://purl.org/dc/terms/contributor> "Jenni Parry" ;
                           <http://purl.org/dc/terms/created> "2024-06-04"^^xsd:date ;
                           <http://purl.org/dc/terms/source> "ISO 27001:2022 Control Framework"@en ;
                           rdfs:isDefinedBy <http://JP_ontology.org/nis2v> ;
                           <http://www.w3.org/2004/02/skos/core#altLabel> "NIS2V Term"@en ;
                           <http://www.w3.org/2004/02/skos/core#definition> "Independent Security Review: Regular independent reviews of the organisation's information security management, encompassing people, processes, and technologies, especially after significant changes."@en ;
                           <http://www.w3.org/2004/02/skos/core#exactMatch> <http://JP_ontology.org/iso27001/ControlA.5.35> ;
                           <http://www.w3.org/2004/02/skos/core#note> "DPV Mapping Coverage: Complex Match"@en ,
                                                                      """ISO - DPV Mapping Assumptions / Commentary: The ISO control is a broader concept encompassing the independent review process of the organisation's information security management approach, which may include various methods such as penetration testing and cybersecurity assessment.
Penetration Testing Methods - DPV: Use of penetration testing to identify weaknesses and vulnerabilities through simulations
Cybersecurity Assessment - DPV: Assessment of cybersecurity capabilities in terms of vulnerabilities and effectiveness of controls"""@en ,
                                                                      "This NIS2V Term aligns with Article 21.2 f: Policies and procedures to assess the effectiveness of cybersecurity risk management measures"@en ;
                           <http://www.w3.org/2004/02/skos/core#prefLabel> "Independent Security Review"@en ;
                           <http://www.w3.org/2004/02/skos/core#related> <https://w3id.org/dpv#CybersecurityAssessment> ,
                                                                         <https://w3id.org/dpv#PenetrationTestingMethods> .


:InformationSecurityAwarenessTraining <http://purl.org/dc/terms/contributor> "Jenni Parry" ;
                                      <http://purl.org/dc/terms/created> "2024-06-04"^^xsd:date ;
                                      <http://purl.org/dc/terms/source> "ISO 27001:2022 Control Framework"@en ;
                                      rdfs:isDefinedBy <http://JP_ontology.org/nis2v> ;
                                      <http://www.w3.org/2004/02/skos/core#altLabel> "NIS2V Term"@en ;
                                      <http://www.w3.org/2004/02/skos/core#definition> "Information Security Awareness Training: Provision of security awareness, education, and training to personnel and relevant parties, including updates on security policies and procedures related to their roles."@en ;
                                      <http://www.w3.org/2004/02/skos/core#exactMatch> <http://JP_ontology.org/iso27001/ControlA.6.3> ;
                                      <http://www.w3.org/2004/02/skos/core#note> "DPV Mapping Coverage: Complex Match"@en ,
                                                                                 """ISO - DPV Mapping Assumptions / Commentary: The ISO control is a broader concept encompassing the provision of various types of training and awareness programs related to information security.
While these terms are relevant to increasing awareness, they represent narrower aspects within the broader context of organisational awareness of information security policies and management system requirements.
Cybersecurity Training - DPV: Training methods related to cybersecurity
Security Knowledge Training - DPV: Training intended to increase knowledge regarding security
Data Protection Training - DPV: Training intended to increase knowledge regarding data protection"""@en ,
                                                                                 "This NIS2V Term aligns with Article 21.2 g: Basic computer hygiene practices and cybersecurity training"@en ,
                                                                                 "This NIS2V Term aligns with Article 21.2 i: Human resources security, access control policies and asset management;"@en ;
                                      <http://www.w3.org/2004/02/skos/core#prefLabel> "Information Security Awareness Training"@en ;
                                      <http://www.w3.org/2004/02/skos/core#related> <https://w3id.org/dpv#CybersecurityTraining> ,
                                                                                    <https://w3id.org/dpv#DataProtectionTraining> ,
                                                                                    <https://w3id.org/dpv#SecurityKnowledgeTraining> .


:InformationSecurityIntergradation <http://purl.org/dc/terms/contributor> "Jenni Parry" ;
                                   <http://purl.org/dc/terms/created> "2024-06-05"^^xsd:date ;
                                   <http://purl.org/dc/terms/source> "ISO 27001:2022 Control Framework"@en ;
                                   rdfs:isDefinedBy <http://JP_ontology.org/nis2v> ;
                                   <http://www.w3.org/2004/02/skos/core#altLabel> "NIS2V Term"@en ;
                                   <http://www.w3.org/2004/02/skos/core#definition> "Information Security Intergradation: Information Security Integration: Embedding data protection practices into the fabric of an organisation's processes and projects."@en ;
                                   <http://www.w3.org/2004/02/skos/core#exactMatch> <http://JP_ontology.org/iso27001/ControlA.5.8> ;
                                   <http://www.w3.org/2004/02/skos/core#note> "This NIS2V Term aligns with Article 21.2 d: Supply chain security, including security-related aspects concerning the relationships between each entity and its direct suppliers or service providers "@en ;
                                   <http://www.w3.org/2004/02/skos/core#prefLabel> "Information Security Intergradation"@en .


:InformationSecurityManagementReview <http://purl.org/dc/terms/contributor> "Jenni Parry" ;
                                     <http://purl.org/dc/terms/created> "2024-06-04"^^xsd:date ;
                                     <http://purl.org/dc/terms/source> "ISO 27001:2022 Control Framework"@en ;
                                     rdfs:isDefinedBy <http://JP_ontology.org/nis2v> ;
                                     <http://www.w3.org/2004/02/skos/core#altLabel> "NIS2V Term"@en ;
                                     <http://www.w3.org/2004/02/skos/core#definition> "Information Security Management Review: Periodic reviews by top management to assess the suitability, adequacy, and effectiveness of the organisation's information security management system."@en ;
                                     <http://www.w3.org/2004/02/skos/core#exactMatch> <http://JP_ontology.org/iso27001/Control9.3> ;
                                     <http://www.w3.org/2004/02/skos/core#narrower> <https://w3id.org/dpv#ReviewProcedure> ;
                                     <http://www.w3.org/2004/02/skos/core#note> "DPV Mapping Coverage: Narrower Match"@en ,
                                                                                """ISO - DPV Mapping Assumptions / Commentary: The ISO control is a broader concept.
DPV: a procedure or process that reviews the correctness and validity of other procedures and policies e.g. to ensure continued validity, adequacy for intended purposes, and conformance of processes with findings"""@en ,
                                                                                "This NIS2V Term aligns with Article 21.2 f: Policies and procedures to assess the effectiveness of cybersecurity risk management measures"@en ;
                                     <http://www.w3.org/2004/02/skos/core#prefLabel> "Information Security Management Review"@en .


:InformationSecurityManagementSystem <http://purl.org/dc/terms/contributor> "Jenni Parry" ;
                                     <http://purl.org/dc/terms/created> "2024-05-01"^^xsd:date ;
                                     <http://purl.org/dc/terms/source> "ENISA: Minimum Security Measures for Operators of Essentials Services, https://www.enisa.europa.eu/topics/cybersecurity-policy/nis-directive-new/minimum-security-measures-for-operators-of-essentials-services"@en ;
                                     rdfs:isDefinedBy <http://JP_ontology.org/nis2v> ;
                                     <http://www.w3.org/2004/02/skos/core#altLabel> "NIS2V Term"@en ;
                                     <http://www.w3.org/2004/02/skos/core#definition> "A systematic approach to managing sensitive company information, ensuring its confidentiality, integrity, and availability."@en ;
                                     <http://www.w3.org/2004/02/skos/core#exactMatch> <http://JP_ontology.org/iso27001/Control4.4> ;
                                     <http://www.w3.org/2004/02/skos/core#note> "This NIS2V Term aligns with Article 21.2a: Policies on risk analysis and information system security."@en ;
                                     <http://www.w3.org/2004/02/skos/core#prefLabel> "Information Security Management System"@en .


:InformationSecurityObjectivesandPlanning <http://purl.org/dc/terms/contributor> "Jenni Parry" ;
                                          <http://purl.org/dc/terms/created> "2024-06-05"^^xsd:date ;
                                          <http://purl.org/dc/terms/source> "ISO 27001:2022 Control Framework"@en ;
                                          rdfs:isDefinedBy <http://JP_ontology.org/nis2v> ;
                                          <http://www.w3.org/2004/02/skos/core#altLabel> "NIS2V Term"@en ;
                                          <http://www.w3.org/2004/02/skos/core#definition> "Information Security Objectives and Planning involve defining specific goals and strategies for managing and improving information security within an organisation, including identifying risks, implementing controls, and allocating resources to mitigate threats and vulnerabilities."@en ;
                                          <http://www.w3.org/2004/02/skos/core#exactMatch> <http://JP_ontology.org/iso27001/Control6.2> ;
                                          <http://www.w3.org/2004/02/skos/core#note> "This NIS2V Term aligns with Article 21.2 a: Policies on risk analysis and information system security"@en ;
                                          <http://www.w3.org/2004/02/skos/core#prefLabel> "Information Security Objectives and Planning"@en .


:InformationSecurityPolicy <http://purl.org/dc/terms/contributor> "Jenni Parry" ;
                           <http://purl.org/dc/terms/created> "2024-06-05"^^xsd:date ;
                           <http://purl.org/dc/terms/source> "ISO 27001:2022 Control Framework"@en ;
                           rdfs:isDefinedBy <http://JP_ontology.org/nis2v> ;
                           <http://www.w3.org/2004/02/skos/core#altLabel> "NIS2V Term"@en ;
                           <http://www.w3.org/2004/02/skos/core#definition> "Information Security Policy: A set of documented guidelines, rules, and procedures established by an organisation to ensure the confidentiality, integrity, and availability of its information assets, as well as to define the responsibilities of employees and users regarding information security."@en ;
                           <http://www.w3.org/2004/02/skos/core#exactMatch> <http://JP_ontology.org/iso27001/Control5.2> ,
                                                                            <https://w3id.org/dpv#InformationSecurityPolicy> ;
                           <http://www.w3.org/2004/02/skos/core#note> "DPV Mapping Coverage: Exact Match"@en ,
                                                                      "ISO - DPV Mapping Assumptions / Commentary: The term Information Security Policy is an exact match for the control statement, as it directly corresponds to the requirements for establishing, documenting, communicating, and improving an information security policy. DPV: Policy regarding security of information"@en ,
                                                                      "This NIS2V Term aligns with Article 21.2 a: Policies on risk analysis and information system security"@en ;
                           <http://www.w3.org/2004/02/skos/core#prefLabel> "Information Security Policy"@en .


:InformationSecurityPolicyApplication <http://purl.org/dc/terms/contributor> "Jenni Parry" ;
                                      <http://purl.org/dc/terms/created> "2024-06-04"^^xsd:date ;
                                      <http://purl.org/dc/terms/source> "ISO 27001:2022 Control Framework"@en ;
                                      rdfs:isDefinedBy <http://JP_ontology.org/nis2v> ;
                                      <http://www.w3.org/2004/02/skos/core#altLabel> "NIS2V Term"@en ;
                                      <http://www.w3.org/2004/02/skos/core#definition> "Information Security Policy Application: Enforcement of adherence to information security policies and procedures by all personnel as mandated by management."@en ;
                                      <http://www.w3.org/2004/02/skos/core#exactMatch> <http://JP_ontology.org/iso27001/ControlA.5.4> ;
                                      <http://www.w3.org/2004/02/skos/core#narrower> <https://w3id.org/dpv#InformationSecurityPolicy> ;
                                      <http://www.w3.org/2004/02/skos/core#note> "DPV Mapping Coverage: Narrower Match"@en ,
                                                                                 """ISO - DPV Mapping Assumptions / Commentary: Information Security Policy could be considered a narrower concept compared to ISO control. It represents a specific policy focused on guiding personnel on information security practices within the organisation.
DPV: Policy regarding security of information"""@en ,
                                                                                 "This NIS2V Term aligns with Article 21.2 a: Policies on risk analysis and information system security"@en ;
                                      <http://www.w3.org/2004/02/skos/core#prefLabel> "Information Security Policy Application"@en .


:InformationSecurityPolicyCompliance <http://purl.org/dc/terms/contributor> "Jenni Parry" ;
                                     <http://purl.org/dc/terms/created> "2024-06-04"^^xsd:date ;
                                     <http://purl.org/dc/terms/source> "ISO 27001:2022 Control Framework"@en ;
                                     rdfs:isDefinedBy <http://JP_ontology.org/nis2v> ;
                                     <http://www.w3.org/2004/02/skos/core#altLabel> "NIS2V Term"@en ;
                                     <http://www.w3.org/2004/02/skos/core#definition> "Information Security Policy Compliance: Adherence to the rules, guidelines, and directives outlined in an organisation's information security policy to ensure the confidentiality, integrity, and availability of information assets and systems."@en ;
                                     <http://www.w3.org/2004/02/skos/core#exactMatch> <http://JP_ontology.org/iso27001/ControlA.5.36> ;
                                     <http://www.w3.org/2004/02/skos/core#narrower> <https://w3id.org/dpv#ComplianceMonitoring> ;
                                     <http://www.w3.org/2004/02/skos/core#note> "DPV Mapping Coverage: Narrower Match"@en ,
                                                                                """ISO - DPV Mapping Assumptions / Commentary: The ISO control outlines the requirements of the compliance review process. Compliance Monitoring directly supports the control's requirement to regularly review compliance with the organisation's information security frameworks.
Compliance Monitoring - DPV: Monitoring of compliance (e.g. internal policy, regulations)"""@en ,
                                                                                "This NIS2V Term aligns with Article 21.2 f: Policies and procedures to assess the effectiveness of cybersecurity risk management measures"@en ;
                                     <http://www.w3.org/2004/02/skos/core#prefLabel> "Information Security Policy Compliance"@en .


:InformationSecurityPolicyManagement <http://purl.org/dc/terms/contributor> "Jenni Parry" ;
                                     <http://purl.org/dc/terms/created> "2024-06-04"^^xsd:date ;
                                     <http://purl.org/dc/terms/source> "ISO 27001:2022 Control Framework"@en ;
                                     rdfs:isDefinedBy <http://JP_ontology.org/nis2v> ;
                                     <http://www.w3.org/2004/02/skos/core#altLabel> "NIS2V Term"@en ;
                                     <http://www.w3.org/2004/02/skos/core#definition> "Information Security Policy Management: Information security and related policies are established, endorsed, and circulated by management, including regular reviews and updates."@en ;
                                     <http://www.w3.org/2004/02/skos/core#exactMatch> <http://JP_ontology.org/iso27001/ControlA.5.1> ,
                                                                                      <https://w3id.org/dpv#InformationSecurityPolicy> ;
                                     <http://www.w3.org/2004/02/skos/core#note> "DPV Mapping Coverage: Exact Match"@en ,
                                                                                """ISO - DPV Mapping Assumptions / Commentary: The control outlines the process for defining, approving, publishing, communicating, acknowledging, and reviewing information security policies and topic-specific policies within an organisation.
Information Security Policy is a specific type of policy that focuses specifically on the management of information security within an organisation. It outlines the organisation's approach to protecting its information assets, including guidelines for data handling, access controls, incident response, etc.
DPV: Policy regarding security of information"""@en ,
                                                                                "This NIS2V Term aligns with Article 21.2 a: Policies on risk analysis and information system security"@en ;
                                     <http://www.w3.org/2004/02/skos/core#prefLabel> "Information Security Policy Management"@en .


:InformationSecurityRiskAssessmentImplementation <http://purl.org/dc/terms/contributor> "Jenni Parry" ;
                                                 <http://purl.org/dc/terms/created> "2024-06-04"^^xsd:date ;
                                                 <http://purl.org/dc/terms/source> "ISO 27001:2022 Control Framework"@en ;
                                                 rdfs:isDefinedBy <http://JP_ontology.org/nis2v> ;
                                                 <http://www.w3.org/2004/02/skos/core#altLabel> "NIS2V Term"@en ;
                                                 <http://www.w3.org/2004/02/skos/core#definition> "Information Security Risk Assessment Implementation: The implementation of Information Security Risk Assessments involves conducting them at planned intervals or in response to significant changes that could impact security, and retaining documented results of these assessments, thus ensuring the organization remains agile and responsive to emerging threats."@en ;
                                                 <http://www.w3.org/2004/02/skos/core#exactMatch> <http://JP_ontology.org/iso27001/Control8.2> ,
                                                                                                  <https://w3id.org/dpv#RiskAssessment> ;
                                                 <http://www.w3.org/2004/02/skos/core#note> "DPV Mapping Coverage: Exact Match"@en ,
                                                                                            """ISO - DPV Mapping Assumptions / Commentary: Risk Assessment is an exact match for the core activity described in the control statement. This term directly corresponds to the requirement for conducting risk assessments in accordance with established criteria and documenting those assessments.
Risk Assessment - DPV: Assessment involving identification, analysis, and evaluation of risk"""@en ,
                                                                                            "This NIS2V Term aligns with Article 21.2 a: Policies on risk analysis and information system security"@en ;
                                                 <http://www.w3.org/2004/02/skos/core#prefLabel> "Information Security Risk Assessment Implementation"@en .


:InformationSecurityRiskAssessmentProcess <http://purl.org/dc/terms/contributor> "Jenni Parry" ;
                                          <http://purl.org/dc/terms/created> "2024-04-26"^^xsd:date ;
                                          <http://purl.org/dc/terms/source> "ISO 27001:2022 Control Framework"@en ;
                                          rdfs:isDefinedBy <http://JP_ontology.org/nis2v> ;
                                          <http://www.w3.org/2004/02/skos/core#altLabel> "NIS2V Term"@en ;
                                          <http://www.w3.org/2004/02/skos/core#definition> "The information security risk assessment process includes establishing clear criteria for accepting risks, ensuring assessments are consistent and valid, identifying risks related to the loss of confidentiality, integrity, and availability, analyzing these risks to assess their consequences and likelihood, and evaluating them against established criteria to prioritize treatment."@en ;
                                          <http://www.w3.org/2004/02/skos/core#exactMatch> <http://JP_ontology.org/iso27001/Control6.1.2> ;
                                          <http://www.w3.org/2004/02/skos/core#note> "This NIS2V Term aligns with Article 21.2a: Policies on risk analysis and information system security."@en ;
                                          <http://www.w3.org/2004/02/skos/core#prefLabel> "Information Security Risk Assessment Process"@en .


:InformationSecurityRiskTreatment <http://purl.org/dc/terms/contributor> "Jenni Parry" ;
                                  <http://purl.org/dc/terms/created> "2024-06-04"^^xsd:date ;
                                  <http://purl.org/dc/terms/source> "ISO 27001:2022 Control Framework"@en ;
                                  rdfs:isDefinedBy <http://JP_ontology.org/nis2v> ;
                                  <http://www.w3.org/2004/02/skos/core#altLabel> "NIS2V Term"@en ;
                                  <http://www.w3.org/2004/02/skos/core#definition> "Risk Treatment: This involves selecting and applying one or more options for modifying risks, which can include avoiding, reducing, transferring, or retaining risk."@en ;
                                  <http://www.w3.org/2004/02/skos/core#exactMatch> <http://JP_ontology.org/iso27001/Control8.3> ;
                                  <http://www.w3.org/2004/02/skos/core#narrower> <https://w3id.org/dpv#RiskMitigationMeasure> ;
                                  <http://www.w3.org/2004/02/skos/core#note> "DPV Mapping Coverage: Narrower Match"@en ,
                                                                             """ISO - DPV Mapping Assumptions / Commentary: Risk Mitigation Measure is a narrower match with ISO control. It represents specific actions or measures taken to reduce the impact or likelihood of identified risks, which would typically be part of a broader risk treatment plan or risk management strategy.
DPV: Measures intended to mitigate, minimise, or prevent risk."""@en ,
                                                                             "This NIS2V Term aligns with Article 21.2 a: Policies on risk analysis and information system security"@en ;
                                  <http://www.w3.org/2004/02/skos/core#prefLabel> "Information Security Risk Treatment"@en .


:InformationSecurityRoleDelegation <http://purl.org/dc/terms/contributor> "Jenni Parry" ;
                                   <http://purl.org/dc/terms/created> "2024-06-05"^^xsd:date ;
                                   <http://purl.org/dc/terms/source> "ISO 27001:2022 Control Framework"@en ;
                                   rdfs:isDefinedBy <http://JP_ontology.org/nis2v> ;
                                   <http://www.w3.org/2004/02/skos/core#altLabel> "NIS2V Term"@en ;
                                   <http://www.w3.org/2004/02/skos/core#definition> "Information Security Role Delegation: Top management assigns and communicates responsibilities for information security roles, ensuring the ISMS adheres to standards and reporting on its performance."@en ;
                                   <http://www.w3.org/2004/02/skos/core#exactMatch> <http://JP_ontology.org/iso27001/Control5.3> ;
                                   <http://www.w3.org/2004/02/skos/core#note> "This NIS2V Term aligns with Article 21.2 a: Policies on risk analysis and information system security"@en ;
                                   <http://www.w3.org/2004/02/skos/core#prefLabel> "Information Security Role Delegation"@en .


:InformationTransferProtocols <http://purl.org/dc/terms/contributor> "Jenni Parry" ;
                              <http://purl.org/dc/terms/created> "2024-06-04"^^xsd:date ;
                              <http://purl.org/dc/terms/source> "ISO 27001:2022 Control Framework"@en ;
                              rdfs:isDefinedBy <http://JP_ontology.org/nis2v> ;
                              <http://www.w3.org/2004/02/skos/core#altLabel> "NIS2V Term"@en ;
                              <http://www.w3.org/2004/02/skos/core#definition> "Information Transfer Protocols: Established rules, procedures, or agreements governing the transfer of information across all types of transfer facilities within the organisation and between the organisation and external parties."@en ;
                              <http://www.w3.org/2004/02/skos/core#exactMatch> <http://JP_ontology.org/iso27001/ControlA.5.14> ;
                              <http://www.w3.org/2004/02/skos/core#narrower> <https://w3id.org/dpv#SafeguardForDataTransfer> ;
                              <http://www.w3.org/2004/02/skos/core#note> "DPV Mapping Coverage: Narrower Match"@en ,
                                                                         """ISO - DPV Mapping Assumptions / Commentary: The control statement focuses on the establishment of rules, procedures, or agreements for all types of information transfer within and between organisations.
Narrower/Directly Relevant: Safeguard for Data Transfer directly address specific aspects of securing information transfers, fitting into the broader requirement for establishing secure transfer mechanisms.
DPV: Represents a safeguard used for data transfer. Can include technical or organisational measures."""@en ,
                                                                         "This NIS2V Term aligns with Article 21.2 j: The use of multi-factor authentication or continuous authentication solutions, secured voice, video and text communications and secured emergency communications systems within the entity, where appropriate"@en ;
                              <http://www.w3.org/2004/02/skos/core#prefLabel> "Information Transfer Protocols"@en .


:IntellectualPropertyRights <http://purl.org/dc/terms/contributor> "Jenni Parry" ;
                            <http://purl.org/dc/terms/created> "2024-06-04"^^xsd:date ;
                            <http://purl.org/dc/terms/source> "ISO 27001:2022 Control Framework"@en ;
                            rdfs:isDefinedBy <http://JP_ontology.org/nis2v> ;
                            <http://www.w3.org/2004/02/skos/core#altLabel> "NIS2V Term"@en ;
                            <http://www.w3.org/2004/02/skos/core#definition> "Intellectual Property Rights (IPR) refer to legal rights that protect creations of the human mind or intellect, such as inventions, literary and artistic works, designs, symbols, names, and images, granting exclusive rights to creators or owners to use, reproduce, and profit from their intellectual creations for a specified period, thus encouraging innovation and creativity while providing incentives for investment in research and development."@en ;
                            <http://www.w3.org/2004/02/skos/core#exactMatch> <http://JP_ontology.org/iso27001/ControlA.5.32> ,
                                                                             <https://w3id.org/dpv#IPRManagement> ;
                            <http://www.w3.org/2004/02/skos/core#note> "DPV Mapping Coverage: Exact Match"@en ,
                                                                       "ISO - DPV Mapping Assumptions / Commentary: The ISO control requires suitable procedures to safeguard intellectual property rights, this would be covered in the management of Intellectual Property Rights (i.e. provides the means to identify and safeguard and enforce)."@en ,
                                                                       "This NIS2V Term aligns with Article 21.2 g: Basic computer hygiene practices and cybersecurity training"@en ;
                            <http://www.w3.org/2004/02/skos/core#prefLabel> "Intellectual Property Rights"@en .


:InternalAudit <http://purl.org/dc/terms/contributor> "Jenni Parry" ;
               <http://purl.org/dc/terms/created> "2024-05-01"^^xsd:date ;
               <http://purl.org/dc/terms/source> "ISO 27001:2022 Control Framework"@en ;
               rdfs:isDefinedBy <http://JP_ontology.org/nis2v> ;
               <http://www.w3.org/2004/02/skos/core#altLabel> "NIS2V Term"@en ;
               <http://www.w3.org/2004/02/skos/core#definition> "Refers to an independent and objective examination of an organisation's activities, processes, controls, and systems conducted by internal auditors to assess compliance, effectiveness, and efficiency and to provide recommendations for improvement."@en ;
               <http://www.w3.org/2004/02/skos/core#exactMatch> <http://JP_ontology.org/iso27001/Control9.2> ;
               <http://www.w3.org/2004/02/skos/core#note> "This NIS2V Term aligns with Article 21.2f: Policies and procedures to assess the effectiveness of cybersecurity risk management measures."@en ;
               <http://www.w3.org/2004/02/skos/core#prefLabel> "Internal Audit"@en .


:InternalAuditProgramme <http://purl.org/dc/terms/contributor> "Jenni Parry" ;
                        <http://purl.org/dc/terms/created> "2024-05-01"^^xsd:date ;
                        <http://purl.org/dc/terms/source> "ENISA: Minimum Security Measures for Operators of Essentials Services, https://www.enisa.europa.eu/topics/cybersecurity-policy/nis-directive-new/minimum-security-measures-for-operators-of-essentials-services"@en ;
                        rdfs:isDefinedBy <http://JP_ontology.org/nis2v> ;
                        <http://www.w3.org/2004/02/skos/core#altLabel> "NIS2V Term"@en ;
                        <http://www.w3.org/2004/02/skos/core#definition> "Outlines the schedule, scope, and objectives of internal audit activities within an organisation, including resource allocation and identification of audit criteria."@en ;
                        <http://www.w3.org/2004/02/skos/core#exactMatch> <http://JP_ontology.org/iso27001/Control9.2.2> ;
                        <http://www.w3.org/2004/02/skos/core#note> "This NIS2V Term aligns with Article 21.2f: Policies and procedures to assess the effectiveness of cybersecurity risk management measures."@en ;
                        <http://www.w3.org/2004/02/skos/core#prefLabel> "Internal Audit Programme"@en .


:LabellingOfInformation <http://purl.org/dc/terms/contributor> "Jenni Parry" ;
                        <http://purl.org/dc/terms/created> "2024-05-01"^^xsd:date ;
                        <http://purl.org/dc/terms/source> "ENISA: Minimum Security Measures for Operators of Essentials Services, https://www.enisa.europa.eu/topics/cybersecurity-policy/nis-directive-new/minimum-security-measures-for-operators-of-essentials-services"@en ;
                        rdfs:isDefinedBy <http://JP_ontology.org/nis2v> ;
                        <http://www.w3.org/2004/02/skos/core#altLabel> "NIS2V Term"@en ;
                        <http://www.w3.org/2004/02/skos/core#definition> "Labelling of Information involves the process of categorizing, marking, or tagging data or documents with appropriate labels or identifiers to indicate their sensitivity, classification level, access restrictions, or handling requirements, helping to ensure confidentiality, integrity, and proper management of information assets.."@en ;
                        <http://www.w3.org/2004/02/skos/core#exactMatch> <http://JP_ontology.org/iso27001/ControlA.5.13> ;
                        <http://www.w3.org/2004/02/skos/core#note> "This NIS2V Term aligns with Article 21.2f: Policies and procedures to assess the effectiveness of cybersecurity risk management measures."@en ;
                        <http://www.w3.org/2004/02/skos/core#prefLabel> "Labelling of Information"@en .


:LeadershipAndCommitment <http://purl.org/dc/terms/contributor> "Jenni Parry" ;
                         <http://purl.org/dc/terms/created> "2024-05-01"^^xsd:date ;
                         <http://purl.org/dc/terms/source> "ENISA: Minimum Security Measures for Operators of Essentials Services, https://www.enisa.europa.eu/topics/cybersecurity-policy/nis-directive-new/minimum-security-measures-for-operators-of-essentials-services"@en ;
                         rdfs:isDefinedBy <http://JP_ontology.org/nis2v> ;
                         <http://www.w3.org/2004/02/skos/core#altLabel> "NIS2V Term"@en ;
                         <http://www.w3.org/2004/02/skos/core#definition> "Refers to the top management's active involvement, support, and dedication to establishing and maintaining an effective management system."@en ;
                         <http://www.w3.org/2004/02/skos/core#exactMatch> <http://JP_ontology.org/iso27001/Control5.1> ;
                         <http://www.w3.org/2004/02/skos/core#note> "This NIS2V Term aligns with Article 21.2a: Policies on risk analysis and information system security."@en ;
                         <http://www.w3.org/2004/02/skos/core#prefLabel> "Leadership and Commitment"@en .


:ManagementResponsibilities <http://purl.org/dc/terms/contributor> "Jenni Parry" ;
                            <http://purl.org/dc/terms/created> "2024-05-01"^^xsd:date ;
                            <http://purl.org/dc/terms/source> "ENISA: Minimum Security Measures for Operators of Essentials Services, https://www.enisa.europa.eu/topics/cybersecurity-policy/nis-directive-new/minimum-security-measures-for-operators-of-essentials-services"@en ;
                            rdfs:isDefinedBy <http://JP_ontology.org/nis2v> ;
                            <http://www.w3.org/2004/02/skos/core#altLabel> "NIS2V Term"@en ;
                            <http://www.w3.org/2004/02/skos/core#definition> "Refers to the duties, obligations, and roles assigned to top management within an organisation, including establishing policies and ensuring compliance."@en ;
                            <http://www.w3.org/2004/02/skos/core#exactMatch> <http://JP_ontology.org/iso27001/ControlA.5.4> ;
                            <http://www.w3.org/2004/02/skos/core#note> "This NIS2V Term aligns with Article 21.2f: Policies and procedures to assess the effectiveness of cybersecurity risk management measures."@en ;
                            <http://www.w3.org/2004/02/skos/core#prefLabel> "Management Responsibilities"@en .


:ManagementReviewResults <http://purl.org/dc/terms/contributor> "Jenni Parry" ;
                         <http://purl.org/dc/terms/created> "2024-05-01"^^xsd:date ;
                         <http://purl.org/dc/terms/source> "ENISA: Minimum Security Measures for Operators of Essentials Services, https://www.enisa.europa.eu/topics/cybersecurity-policy/nis-directive-new/minimum-security-measures-for-operators-of-essentials-services"@en ;
                         rdfs:isDefinedBy <http://JP_ontology.org/nis2v> ;
                         <http://www.w3.org/2004/02/skos/core#altLabel> "NIS2V Term"@en ;
                         <http://www.w3.org/2004/02/skos/core#definition> "Refers to the outcomes, findings, conclusions, and actions resulting from the management review process, including decisions regarding improvements and strategic changes."@en ;
                         <http://www.w3.org/2004/02/skos/core#exactMatch> <http://JP_ontology.org/iso27001/Control9.3.3> ;
                         <http://www.w3.org/2004/02/skos/core#note> "This NIS2V Term aligns with Article 21.2f: Policies and procedures to assess the effectiveness of cybersecurity risk management measures."@en ;
                         <http://www.w3.org/2004/02/skos/core#prefLabel> "Management Review Results"@en .


:NIS2CySecMeasures <http://purl.org/dc/terms/contributor> "Jenni Parry" ;
                   <http://purl.org/dc/terms/created> "2024-04-18"^^xsd:date ;
                   rdfs:isDefinedBy <http://JP_ontology.org/nis2v> ;
                   <http://www.w3.org/2004/02/skos/core#altLabel> "NIS2 Cybersecurity Risk-Management Measures (Article 21)"@en ;
                   <http://www.w3.org/2004/02/skos/core#definition> "Represents the cybersecurity measures outlined in NIS2, specifically those related to risk management as per Article 21."@en ;
                   <http://www.w3.org/2004/02/skos/core#prefLabel> "NIS2 CySec Measures"@en .


:NIS2VTerms <http://purl.org/dc/terms/contributor> "Jenni Parry" ;
            <http://purl.org/dc/terms/created> "2024-04-18"^^xsd:date ;
            rdfs:isDefinedBy <http://JP_ontology.org/nis2v> ;
            <http://www.w3.org/2004/02/skos/core#altLabel> "NIS2 Cybersecurity Risk-Management Measures (Article 21)"@en ;
            <http://www.w3.org/2004/02/skos/core#definition> "Represents the cybersecurity measures outlined in NIS2, specifically those related to risk management as per Article 21."@en ;
            <http://www.w3.org/2004/02/skos/core#prefLabel> "NIS2V Terms"@en .


:NeedsAndExpectationsOfInterestedParties <http://purl.org/dc/terms/contributor> "Jenni Parry" ;
                                         <http://purl.org/dc/terms/created> "2024-05-01"^^xsd:date ;
                                         <http://purl.org/dc/terms/source> "ENISA: Minimum Security Measures for Operators of Essentials Services, https://www.enisa.europa.eu/topics/cybersecurity-policy/nis-directive-new/minimum-security-measures-for-operators-of-essentials-services"@en ;
                                         rdfs:isDefinedBy <http://JP_ontology.org/nis2v> ;
                                         <http://www.w3.org/2004/02/skos/core#altLabel> "NIS2V Term"@en ;
                                         <http://www.w3.org/2004/02/skos/core#definition> "Refers to the requirements, desires, and anticipated outcomes of individuals or groups who have a vested interest in an organisation's activities, products, or services."@en ;
                                         <http://www.w3.org/2004/02/skos/core#exactMatch> <http://JP_ontology.org/iso27001/Control4.2> ;
                                         <http://www.w3.org/2004/02/skos/core#note> "This NIS2V Term aligns with Article 21.2a: Policies on risk analysis and information system security."@en ;
                                         <http://www.w3.org/2004/02/skos/core#prefLabel> "Needs and Expectations of Interested Parties"@en .


:NetworkSecurity <http://purl.org/dc/terms/contributor> "Jenni Parry" ;
                 <http://purl.org/dc/terms/created> "2024-06-04"^^xsd:date ;
                 <http://purl.org/dc/terms/source> "ISO 27001:2022 Control Framework"@en ;
                 rdfs:isDefinedBy <http://JP_ontology.org/nis2v> ;
                 <http://www.w3.org/2004/02/skos/core#altLabel> "NIS2V Term"@en ;
                 <http://www.w3.org/2004/02/skos/core#definition> "Network Security: The protection of computer networks and their infrastructure from unauthorized access, misuse, modification, or denial of service through the implementation of various security measures such as firewalls, intrusion detection systems, and encryption protocols."@en ;
                 <http://www.w3.org/2004/02/skos/core#exactMatch> <http://JP_ontology.org/iso27001/ControlA.8.20> ;
                 <http://www.w3.org/2004/02/skos/core#narrower> <https://w3id.org/dpv#NetworkSecurityProtocols> ;
                 <http://www.w3.org/2004/02/skos/core#note> "DPV Mapping Coverage: Narrower Match"@en ,
                                                            """ISO - DPV Mapping Assumptions / Commentary: Directly Relevant: Network Security Protocols is closely aligned with the control's requirements for securing networks and network devices. It covers essential aspects of protecting information as it is transmitted across networks, making it a direct match for part of the control's focus.
DPV: Security implemented at or over networks protocols"""@en ,
                                                            "This NIS2V Term aligns with Article 21.2 e: Security in network and information systems acquisition, development and maintenance, including vulnerability handling and disclosure"@en ;
                 <http://www.w3.org/2004/02/skos/core#prefLabel> "Network Security"@en .


:NetworkServiceSecurityManagement <http://purl.org/dc/terms/contributor> "Jenni Parry" ;
                                  <http://purl.org/dc/terms/created> "2024-06-04"^^xsd:date ;
                                  <http://purl.org/dc/terms/source> "ISO 27001:2022 Control Framework"@en ;
                                  rdfs:isDefinedBy <http://JP_ontology.org/nis2v> ;
                                  <http://www.w3.org/2004/02/skos/core#altLabel> "NIS2V Term"@en ;
                                  <http://www.w3.org/2004/02/skos/core#definition> "Network Service Security Management: Identification, implementation, and monitoring of security mechanisms, service levels, and requirements for network services."@en ;
                                  <http://www.w3.org/2004/02/skos/core#exactMatch> <http://JP_ontology.org/iso27001/ControlA.8.21> ;
                                  <http://www.w3.org/2004/02/skos/core#narrower> <https://w3id.org/dpv#NetworkSecurityProtocols> ;
                                  <http://www.w3.org/2004/02/skos/core#note> "DPV Mapping Coverage: Narrower Match"@en ,
                                                                             """ISO - DPV Mapping Assumptions / Commentary: The ISO control addresses a broader scope of actions related to the identification, implementation, and monitoring of security mechanisms, service levels, and service requirements for network services. It includes ensuring the security, performance, and functionality of network services.
Network Security Protocols refers specifically to the protocols and standards used to secure network communication and data transmission. While it is an essential component of ensuring network security, it represents a narrower aspect within the broader context of the ISO control.
DPV: Security implemented at or over networks protocols"""@en ,
                                                                             "This NIS2V Term aligns with Article 21.2 e: Security in network and information systems acquisition, development and maintenance, including vulnerability handling and disclosure"@en ;
                                  <http://www.w3.org/2004/02/skos/core#prefLabel> "Network Service Security Management"@en .


:NonconformityAndCorrectiveAction <http://purl.org/dc/terms/contributor> "Jenni Parry" ;
                                  <http://purl.org/dc/terms/created> "2024-05-01"^^xsd:date ;
                                  <http://purl.org/dc/terms/source> "ENISA: Minimum Security Measures for Operators of Essentials Services, https://www.enisa.europa.eu/topics/cybersecurity-policy/nis-directive-new/minimum-security-measures-for-operators-of-essentials-services"@en ;
                                  rdfs:isDefinedBy <http://JP_ontology.org/nis2v> ;
                                  <http://www.w3.org/2004/02/skos/core#altLabel> "NIS2V Term"@en ;
                                  <http://www.w3.org/2004/02/skos/core#definition> "Involves identifying instances where products, processes, or services do not meet specified requirements, and implementing corrective measures."@en ;
                                  <http://www.w3.org/2004/02/skos/core#exactMatch> <http://JP_ontology.org/iso27001/Control10.2> ;
                                  <http://www.w3.org/2004/02/skos/core#note> "This NIS2V Term aligns with Article 21.2f: Policies and procedures to assess the effectiveness of cybersecurity risk management measures."@en ;
                                  <http://www.w3.org/2004/02/skos/core#prefLabel> "Nonconformity and Corrective Action"@en .


:OperationalPlanningandControl <http://purl.org/dc/terms/contributor> "Jenni Parry" ;
                               <http://purl.org/dc/terms/created> "2024-06-04"^^xsd:date ;
                               <http://purl.org/dc/terms/source> "ISO 27001:2022 Control Framework"@en ;
                               rdfs:isDefinedBy <http://JP_ontology.org/nis2v> ;
                               <http://www.w3.org/2004/02/skos/core#altLabel> "NIS2V Term"@en ;
                               <http://www.w3.org/2004/02/skos/core#broader> <https://w3id.org/dpv#GovernanceProcedures> ;
                               <http://www.w3.org/2004/02/skos/core#definition> "Operational Planning and Control: Strategic management of processes to meet specific requirements, including establishing criteria, controlling process execution, managing changes, and overseeing external processes relevant to information security."@en ;
                               <http://www.w3.org/2004/02/skos/core#exactMatch> <http://JP_ontology.org/iso27001/Control8.1> ;
                               <http://www.w3.org/2004/02/skos/core#note> "DPV Mapping Coverage: Broader Match"@en ,
                                                                          "ISO - DPV Mapping Assumptions / Commentary: Governance Procedures: This term is broadly applicable to the control statement. Governance procedures likely include the planning, implementing, controlling, and reviewing processes as part of ensuring that information security management system requirements are met. This term could encompass the establishment of criteria for processes and their control, making it a good match for the overarching requirements of the control."@en ,
                                                                          "This NIS2V Term aligns with Article 21.2 a: Policies on risk analysis and information system security"@en ,
                                                                          "This NIS2V Term aligns with Article 21.2 d: Supply chain security, including security-related aspects concerning the relationships between each entity and its direct suppliers or service providers "@en ;
                               <http://www.w3.org/2004/02/skos/core#prefLabel> "Operational Planning and Control"@en .


:OrganisationContext <http://purl.org/dc/terms/contributor> "Jenni Parry" ;
                     <http://purl.org/dc/terms/created> "2024-06-04"^^xsd:date ;
                     <http://purl.org/dc/terms/source> "ISO 27001:2022 Control Framework"@en ;
                     rdfs:isDefinedBy <http://JP_ontology.org/nis2v> ;
                     <http://www.w3.org/2004/02/skos/core#altLabel> "NIS2V Term"@en ;
                     <http://www.w3.org/2004/02/skos/core#definition> "Organisational Context encompasses the internal and external factors that shape an organisation's structure, culture, strategies, and decision-making processes, including its industry, market, stakeholders, and regulatory environment."@en ;
                     <http://www.w3.org/2004/02/skos/core#exactMatch> <http://JP_ontology.org/iso27001/Control4.1> ;
                     <http://www.w3.org/2004/02/skos/core#narrower> <https://w3id.org/dpv#OrganisationGovernance> ;
                     <http://www.w3.org/2004/02/skos/core#note> "DPV Mapping Coverage: Narrower Match"@en ,
                                                                """ISO - DPV Mapping Assumptions / Commentary: The ISO Control emphasizes the need for the organisation to identify external and internal issues relevant to its purpose and their impact on its information security management system. 
Organisation Governance is a narrower term that specifically relates to the processes and procedures involved in governing the organisation.
DPV: Purposes associated with conducting activities and functions for governance of an organisation"""@en ,
                                                                "This NIS2V Term aligns with Article 21.2 a: Policies on risk analysis and information system security"@en ;
                     <http://www.w3.org/2004/02/skos/core#prefLabel> "Organisation Context"@en .


:OutsourcedDevelopment <http://purl.org/dc/terms/contributor> "Jenni Parry" ;
                       <http://purl.org/dc/terms/created> "2024-05-01"^^xsd:date ;
                       <http://purl.org/dc/terms/source> "ENISA: Minimum Security Measures for Operators of Essentials Services, https://www.enisa.europa.eu/topics/cybersecurity-policy/nis-directive-new/minimum-security-measures-for-operators-of-essentials-services"@en ;
                       rdfs:isDefinedBy <http://JP_ontology.org/nis2v> ;
                       <http://www.w3.org/2004/02/skos/core#altLabel> "NIS2V Term"@en ;
                       <http://www.w3.org/2004/02/skos/core#definition> "Outsourced Development involves engaging external parties, such as third-party vendors or contractors, to undertake various stages of the software development lifecycle, including design, coding, testing, and maintenance, instead of relying solely on in-house resources. This approach can offer cost efficiencies, access to specialized skills, and scalability, but requires careful management to ensure quality, security, and compliance with requirements and standards."@en ;
                       <http://www.w3.org/2004/02/skos/core#exactMatch> <http://JP_ontology.org/iso27001/ControlA.8.30> ;
                       <http://www.w3.org/2004/02/skos/core#note> "This NIS2V Term aligns with Article 21.2g: Basic computer hygiene practices and cybersecurity training."@en ;
                       <http://www.w3.org/2004/02/skos/core#prefLabel> "Outsourced Development"@en .


:PhysicalSecurityPerimeters <http://purl.org/dc/terms/contributor> "Jenni Parry" ;
                            <http://purl.org/dc/terms/created> "2024-06-04"^^xsd:date ;
                            <http://purl.org/dc/terms/source> "ISO 27001:2022 Control Framework"@en ;
                            rdfs:isDefinedBy <http://JP_ontology.org/nis2v> ;
                            <http://www.w3.org/2004/02/skos/core#altLabel> "NIS2V Term"@en ;
                            <http://www.w3.org/2004/02/skos/core#definition> "Physical Security Perimeters are physical barriers or boundaries established to control access to sensitive or restricted areas within a facility, premises, or site, aiming to prevent unauthorized entry, protect assets, and ensure the safety and security of personnel, equipment, and information. These perimeters may include fences, gates, walls, checkpoints, access control systems, surveillance cameras, and other security measures designed to deter and detect intrusions or unauthorized activities."@en ;
                            <http://www.w3.org/2004/02/skos/core#exactMatch> <http://JP_ontology.org/iso27001/ControlA.7.1> ;
                            <http://www.w3.org/2004/02/skos/core#narrower> <https://w3id.org/dpv#PhysicalAccessControlMethod> ;
                            <http://www.w3.org/2004/02/skos/core#note> "DPV Mapping Coverage: Narrower Match"@en ,
                                                                       """ISO - DPV Mapping Assumptions / Commentary: Narrower Match: Physical access control methods are an essential to manage and monitor the security perimeters.
DPV: Access control applied for physical access e.g. premises or equipment"""@en ,
                                                                       "This NIS2V Term aligns with Article 21.2 i: Human resources security, access control policies and asset management;"@en ;
                            <http://www.w3.org/2004/02/skos/core#prefLabel> "Physical Security Perimeters"@en .


:Planning <http://purl.org/dc/terms/contributor> "Jenni Parry" ;
          <http://purl.org/dc/terms/created> "2024-05-01"^^xsd:date ;
          <http://purl.org/dc/terms/source> "ENISA: Minimum Security Measures for Operators of Essentials Services, https://www.enisa.europa.eu/topics/cybersecurity-policy/nis-directive-new/minimum-security-measures-for-operators-of-essentials-services"@en ;
          rdfs:isDefinedBy <http://JP_ontology.org/nis2v> ;
          <http://www.w3.org/2004/02/skos/core#altLabel> "NIS2V Term"@en ;
          <http://www.w3.org/2004/02/skos/core#definition> "Involves the process of setting objectives and determining the actions and resources required to achieve them, typically encompassing strategic, tactical, and operational planning activities."@en ;
          <http://www.w3.org/2004/02/skos/core#exactMatch> <http://JP_ontology.org/iso27001/Control6.1> ;
          <http://www.w3.org/2004/02/skos/core#note> "This NIS2V Term aligns with Article 21.2a: Policies on risk analysis and information system security."@en ;
          <http://www.w3.org/2004/02/skos/core#prefLabel> "Planning"@en .


:PrivilegedAccessManagement <http://purl.org/dc/terms/contributor> "Jenni Parry" ;
                            <http://purl.org/dc/terms/created> "2024-06-04"^^xsd:date ;
                            <http://purl.org/dc/terms/source> "ISO 27001:2022 Control Framework"@en ;
                            rdfs:isDefinedBy <http://JP_ontology.org/nis2v> ;
                            <http://www.w3.org/2004/02/skos/core#altLabel> "NIS2V Term"@en ;
                            <http://www.w3.org/2004/02/skos/core#definition> "Privileged Access Management: Regulation and management of the allocation and utilization of privileged access rights within the organisation to ensure restriction and proper handling."@en ;
                            <http://www.w3.org/2004/02/skos/core#exactMatch> <http://JP_ontology.org/iso27001/ControlA.8.2> ;
                            <http://www.w3.org/2004/02/skos/core#note> "DPV Mapping Coverage: Complex Match"@en ,
                                                                       """ISO - DPV Mapping Assumptions / Commentary: This control covers the allocation, use and restriction of privileged access rights. Access Control Method is narrower as it refers to the specific techniques or mechanisms used to control access to resources within a system.
DPV: Methods which restrict access to a place or resource
Security Role Procedures is also narrower as it specifically pertains to the procedures and guidelines governing security roles and their associated access rights within an organisation.
DPV: Procedures related to security roles"""@en ,
                                                                       "This NIS2V Term aligns with Article 21.2 i: Human resources security, access control policies and asset management;"@en ;
                            <http://www.w3.org/2004/02/skos/core#prefLabel> "Privileged Access Management"@en ;
                            <http://www.w3.org/2004/02/skos/core#related> <https://w3id.org/dpv#AccessControlMethod> ,
                                                                          <https://w3id.org/dpv#SecurityRoleProcedures> .


:ProtectionOfRecords <http://purl.org/dc/terms/contributor> "Jenni Parry" ;
                     <http://purl.org/dc/terms/created> "2024-06-04"^^xsd:date ;
                     <http://purl.org/dc/terms/source> "ISO 27001:2022 Control Framework"@en ;
                     rdfs:isDefinedBy <http://JP_ontology.org/nis2v> ;
                     <http://www.w3.org/2004/02/skos/core#altLabel> "NIS2V Term"@en ;
                     <http://www.w3.org/2004/02/skos/core#definition> "Protection of Records involves measures taken to safeguard the confidentiality, integrity, and availability of organisational records, ensuring their protection against unauthorized access, alteration, loss, or destruction, and facilitating their accurate retrieval, retention, and disposal in compliance with legal, regulatory, and business requirements."@en ;
                     <http://www.w3.org/2004/02/skos/core#exactMatch> <http://JP_ontology.org/iso27001/ControlA.5.33> ,
                                                                      <https://w3id.org/dpv#RecordManagement> ;
                     <http://www.w3.org/2004/02/skos/core#note> "DPV Mapping Coverage: Exact Match"@en ,
                                                                "ISO - DPV Mapping Assumptions / Commentary: The purposes associated with Record Management cover the overall management creation, storage, and use which means the records are safeguarded against loss."@en ,
                                                                "This NIS2V Term aligns with Article 21.2 g: Basic computer hygiene practices and cybersecurity training"@en ;
                     <http://www.w3.org/2004/02/skos/core#prefLabel> "Protection of Records"@en .


:ProtectionOfSystemsDuringAuditTesting <http://purl.org/dc/terms/contributor> "Jenni Parry" ;
                                       <http://purl.org/dc/terms/created> "2024-05-01"^^xsd:date ;
                                       <http://purl.org/dc/terms/source> "ENISA: Minimum Security Measures for Operators of Essentials Services, https://www.enisa.europa.eu/topics/cybersecurity-policy/nis-directive-new/minimum-security-measures-for-operators-of-essentials-services"@en ;
                                       rdfs:isDefinedBy <http://JP_ontology.org/nis2v> ;
                                       <http://www.w3.org/2004/02/skos/core#altLabel> "NIS2V Term"@en ;
                                       <http://www.w3.org/2004/02/skos/core#definition> "Protection of Systems During Audit Testing involves implementing measures to safeguard the integrity, confidentiality, and availability of information systems and data while conducting audit activities, ensuring that testing processes do not inadvertently compromise the security or functionality of critical systems or sensitive information."@en ;
                                       <http://www.w3.org/2004/02/skos/core#exactMatch> <http://JP_ontology.org/iso27001/ControlA.8.34> ;
                                       <http://www.w3.org/2004/02/skos/core#note> "This NIS2V Term aligns with Article 21.2g: Basic computer hygiene practices and cybersecurity training."@en ;
                                       <http://www.w3.org/2004/02/skos/core#prefLabel> "Protection of Systems During Audit Testing"@en .


:Protectionagainstmalware <http://purl.org/dc/terms/contributor> "Jenni Parry" ;
                          <http://purl.org/dc/terms/created> "2024-06-04"^^xsd:date ;
                          <http://purl.org/dc/terms/source> "ISO 27001:2022 Control Framework"@en ;
                          rdfs:isDefinedBy <http://JP_ontology.org/nis2v> ;
                          <http://www.w3.org/2004/02/skos/core#altLabel> "NIS2V Term"@en ;
                          <http://www.w3.org/2004/02/skos/core#definition> "Protection against malware: Measures and strategies implemented to defend computer systems, networks, and devices from malicious software."@en ;
                          <http://www.w3.org/2004/02/skos/core#exactMatch> <http://JP_ontology.org/iso27001/ControlA.8.7> ;
                          <http://www.w3.org/2004/02/skos/core#note> "DPV Mapping Coverage: Complex Match"@en ,
                                                                     """ISO - DPV Mapping Assumptions / Commentary: The ISO control emphasizes the implementation of protection against malware, supported by appropriate user awareness. It focuses on the specific aspect of ensuring users are aware of the risks associated with malware and how to mitigate them.
Cybersecurity Training and Security Knowledge Training are narrower concepts. Both terms refer to training programs aimed at educating users about cybersecurity practices, including malware prevention, detection, and response. They focus on enhancing users' knowledge and skills related to cybersecurity. However Cybersecurity Training might be slightly more inclusive as it often covers a broader range of cybersecurity topics beyond just malware protection.
Cybersecurity Training - DPV: Training methods related to cybersecurity
Security Knowledge Training - DPV: Training intended to increase knowledge regarding security"""@en ,
                                                                     "This NIS2V Term aligns with Article 21.2 g: Basic computer hygiene practices and cybersecurity training"@en ,
                                                                     "This NIS2V Term aligns with Article 21.2 i: Human resources security, access control policies and asset management;"@en ;
                          <http://www.w3.org/2004/02/skos/core#prefLabel> "Protection against malware"@en ;
                          <http://www.w3.org/2004/02/skos/core#related> <https://w3id.org/dpv#CybersecurityTraining> ,
                                                                        <https://w3id.org/dpv#SecurityKnowledgeTraining> .


:RedundancyOfInformationProcessingFacilities <http://purl.org/dc/terms/contributor> "Jenni Parry" ;
                                             <http://purl.org/dc/terms/created> "2024-04-15"^^xsd:date ;
                                             <http://purl.org/dc/terms/source> "ISO 27001:2022 Control Framework"@en ;
                                             rdfs:isDefinedBy <http://JP_ontology.org/nis2v> ;
                                             <http://www.w3.org/2004/02/skos/core#altLabel> "NIS2V Term"@en ;
                                             <http://www.w3.org/2004/02/skos/core#definition> "Implementing multiple systems or components to provide backup in case one fails."@en ;
                                             <http://www.w3.org/2004/02/skos/core#exactMatch> <http://JP_ontology.org/iso27001/ControlA.8.14> ;
                                             <http://www.w3.org/2004/02/skos/core#note> "This NIS2V Term aligns with Article 21.2c: Business continuity management, including backup management, crisis management and disaster recovery."@en ;
                                             <http://www.w3.org/2004/02/skos/core#prefLabel> "Redundancy of Information Processing Facilities"@en .


:RemoteWorkSecurityProtocols <http://purl.org/dc/terms/contributor> "Jenni Parry" ;
                             <http://purl.org/dc/terms/created> "2024-06-05"^^xsd:date ;
                             <http://purl.org/dc/terms/source> "ISO 27001:2022 Control Framework"@en ;
                             rdfs:isDefinedBy <http://JP_ontology.org/nis2v> ;
                             <http://www.w3.org/2004/02/skos/core#altLabel> "NIS2V Term"@en ;
                             <http://www.w3.org/2004/02/skos/core#definition> "Remote Work Security Protocols: Implementation of security measures to safeguard information accessed, processed, or stored outside the organisation's premises during remote work scenarios."@en ;
                             <http://www.w3.org/2004/02/skos/core#exactMatch> <http://JP_ontology.org/iso27001/ControlA.6.7> ;
                             <http://www.w3.org/2004/02/skos/core#note> "This NIS2V Term aligns with Article 21.2 i: Human resources security, access control policies and asset management;"@en ;
                             <http://www.w3.org/2004/02/skos/core#prefLabel> "Remote Work Security Protocols"@en .


:Resources <http://purl.org/dc/terms/contributor> "Jenni Parry" ;
           <http://purl.org/dc/terms/created> "2024-05-01"^^xsd:date ;
           <http://purl.org/dc/terms/source> "ENISA: Minimum Security Measures for Operators of Essentials Services, https://www.enisa.europa.eu/topics/cybersecurity-policy/nis-directive-new/minimum-security-measures-for-operators-of-essentials-services"@en ;
           rdfs:isDefinedBy <http://JP_ontology.org/nis2v> ;
           <http://www.w3.org/2004/02/skos/core#altLabel> "NIS2V Term"@en ;
           <http://www.w3.org/2004/02/skos/core#definition> "Encompasses the personnel, infrastructure, finances, technologies, and other assets available to support an organisation's operations, projects, and objectives."@en ;
           <http://www.w3.org/2004/02/skos/core#exactMatch> <http://JP_ontology.org/iso27001/Control7.1> ;
           <http://www.w3.org/2004/02/skos/core#note> "This NIS2V Term aligns with Article 21.2a: Policies on risk analysis and information system security."@en ;
           <http://www.w3.org/2004/02/skos/core#prefLabel> "Resources"@en .


:ResponsibilitiesAfterTerminationOrChange <http://purl.org/dc/terms/contributor> "Jenni Parry" ;
                                          <http://purl.org/dc/terms/created> "2024-04-17"^^xsd:date ;
                                          <http://purl.org/dc/terms/source> "ISO 27001:2022 Control Framework"@en ;
                                          rdfs:isDefinedBy <http://JP_ontology.org/nis2v> ;
                                          <http://www.w3.org/2004/02/skos/core#altLabel> "NIS2V Term"@en ;
                                          <http://www.w3.org/2004/02/skos/core#definition> "Obligations that an individual maintains following a change or the end of their employment, which can include confidentiality, returning property, and non-competition clauses."@en ;
                                          <http://www.w3.org/2004/02/skos/core#exactMatch> <http://JP_ontology.org/iso27001/ControlA.6.5> ;
                                          <http://www.w3.org/2004/02/skos/core#note> "This NIS2V Term aligns with Article 21.2i: Human resources security, access control policies and asset management."@en ;
                                          <http://www.w3.org/2004/02/skos/core#prefLabel> "Responsibilities after Termination or Change"@en .


:ReturnOfAssets <http://purl.org/dc/terms/contributor> "Jenni Parry" ;
                <http://purl.org/dc/terms/created> "2024-04-17"^^xsd:date ;
                <http://purl.org/dc/terms/source> "ISO 27001:2022 Control Framework"@en ;
                rdfs:isDefinedBy <http://JP_ontology.org/nis2v> ;
                <http://www.w3.org/2004/02/skos/core#altLabel> "NIS2V Term"@en ;
                <http://www.w3.org/2004/02/skos/core#definition> "The process of giving back property or resources to an organisation or individual after use or upon termination of employment or contract."@en ;
                <http://www.w3.org/2004/02/skos/core#exactMatch> <http://JP_ontology.org/iso27001/ControlA.5.11> ;
                <http://www.w3.org/2004/02/skos/core#note> "This NIS2V Term aligns with Article 21.2i: Human resources security, access control policies and asset management."@en ;
                <http://www.w3.org/2004/02/skos/core#prefLabel> "Return of Assets"@en .


:ScopeOfTheISMS <http://purl.org/dc/terms/contributor> "Jenni Parry" ;
                <http://purl.org/dc/terms/created> "2024-05-01"^^xsd:date ;
                <http://purl.org/dc/terms/source> "ENISA: Minimum Security Measures for Operators of Essentials Services, https://www.enisa.europa.eu/topics/cybersecurity-policy/nis-directive-new/minimum-security-measures-for-operators-of-essentials-services"@en ;
                rdfs:isDefinedBy <http://JP_ontology.org/nis2v> ;
                <http://www.w3.org/2004/02/skos/core#altLabel> "NIS2V Term"@en ;
                <http://www.w3.org/2004/02/skos/core#definition> "Defines the boundaries and applicability of an Information Security Management System (ISMS), specifying the assets, processes, and activities covered by the ISMS."@en ;
                <http://www.w3.org/2004/02/skos/core#exactMatch> <http://JP_ontology.org/iso27001/Control4.3> ;
                <http://www.w3.org/2004/02/skos/core#note> "This NIS2V Term aligns with Article 21.2a: Policies on risk analysis and information system security."@en ;
                <http://www.w3.org/2004/02/skos/core#prefLabel> "Scope of the ISMS"@en .


:Screening <http://purl.org/dc/terms/contributor> "Jenni Parry" ;
           <http://purl.org/dc/terms/created> "2024-04-17"^^xsd:date ;
           <http://purl.org/dc/terms/source> "ISO 27001:2022 Control Framework"@en ;
           rdfs:isDefinedBy <http://JP_ontology.org/nis2v> ;
           <http://www.w3.org/2004/02/skos/core#altLabel> "NIS2V Term"@en ;
           <http://www.w3.org/2004/02/skos/core#definition> "The process of evaluating or investigating something or someone for a specific purpose, often to determine eligibility or identify potential risks."@en ;
           <http://www.w3.org/2004/02/skos/core#exactMatch> <http://JP_ontology.org/iso27001/ControlA.6.1> ;
           <http://www.w3.org/2004/02/skos/core#note> "This NIS2V Term aligns with Article 21.2i: Human resources security, access control policies and asset management."@en ;
           <http://www.w3.org/2004/02/skos/core#prefLabel> "Screening"@en .


:SecureAuthenticationImplementation <http://purl.org/dc/terms/contributor> "Jenni Parry" ;
                                    <http://purl.org/dc/terms/created> "2024-06-04"^^xsd:date ;
                                    <http://purl.org/dc/terms/source> "ISO 27001:2022 Control Framework"@en ;
                                    rdfs:isDefinedBy <http://JP_ontology.org/nis2v> ;
                                    <http://www.w3.org/2004/02/skos/core#altLabel> "NIS2V Term"@en ;
                                    <http://www.w3.org/2004/02/skos/core#definition> "Secure Authentication Implementation: Implementation of secure authentication technologies and procedures, tailored to access restrictions and specific access control policies."@en ;
                                    <http://www.w3.org/2004/02/skos/core#exactMatch> <http://JP_ontology.org/iso27001/ControlA.8.5> ;
                                    <http://www.w3.org/2004/02/skos/core#note> "DPV Mapping Coverage: Complex Match"@en ,
                                                                               """ISO - DPV Mapping Assumptions / Commentary: Narrower/Directly Related: Authentication Protocols, Multi-Factor Authentication (MFA) and Password Authentication are specific authentication technologies that directly support the control's focus on secure authentication based on access restrictions.
Authentication Protocols - DPV: Protocols involving validation of identity i.e. authentication of a person or information
Multi-Factor Authentication (MFA) - DPV: 	An authentication system that uses two or more methods to authenticate
Password Authentication - DPV: Use of passwords to perform authentication"""@en ,
                                                                               "This NIS2V Term aligns with Article 21.2 i: Human resources security, access control policies and asset management;"@en ,
                                                                               "This NIS2V Term aligns with Article 21.2 j: The use of multi-factor authentication or continuous authentication solutions, secured voice, video and text communications and secured emergency communications systems within the entity, where appropriate"@en ;
                                    <http://www.w3.org/2004/02/skos/core#prefLabel> "Secure Authentication Implementation"@en ;
                                    <http://www.w3.org/2004/02/skos/core#related> <https://w3id.org/dpv#AuthenticationProtocols> ,
                                                                                  <https://w3id.org/dpv#MultiFactorAuthentication> ,
                                                                                  <https://w3id.org/dpv#PasswordAuthentication> .


:SecureDevelopmentLifeCycle <http://purl.org/dc/terms/contributor> "Jenni Parry" ;
                            <http://purl.org/dc/terms/created> "2024-05-01"^^xsd:date ;
                            <http://purl.org/dc/terms/source> "ENISA: Minimum Security Measures for Operators of Essentials Services, https://www.enisa.europa.eu/topics/cybersecurity-policy/nis-directive-new/minimum-security-measures-for-operators-of-essentials-services"@en ;
                            rdfs:isDefinedBy <http://JP_ontology.org/nis2v> ;
                            <http://www.w3.org/2004/02/skos/core#altLabel> "NIS2V Term"@en ;
                            <http://www.w3.org/2004/02/skos/core#definition> "The Secure Development Life Cycle (SDLC) is a systematic approach to integrating security considerations into every phase of the software development process, from initial design and coding to testing, deployment, and maintenance, aiming to identify and mitigate security vulnerabilities and threats early in the development lifecycle to build robust and secure software applications."@en ;
                            <http://www.w3.org/2004/02/skos/core#exactMatch> <http://JP_ontology.org/iso27001/ControlA.8.25> ;
                            <http://www.w3.org/2004/02/skos/core#note> "This NIS2V Term aligns with Article 21.2g: Basic computer hygiene practices and cybersecurity training."@en ;
                            <http://www.w3.org/2004/02/skos/core#prefLabel> "Secure Development Life Cycle"@en .


:SecureSoftwareInstallationManagement <http://purl.org/dc/terms/contributor> "Jenni Parry" ;
                                      <http://purl.org/dc/terms/created> "2024-06-04"^^xsd:date ;
                                      <http://purl.org/dc/terms/source> "ISO 27001:2022 Control Framework"@en ;
                                      rdfs:isDefinedBy <http://JP_ontology.org/nis2v> ;
                                      <http://www.w3.org/2004/02/skos/core#altLabel> "NIS2V Term"@en ;
                                      <http://www.w3.org/2004/02/skos/core#broader> <https://w3id.org/dpv#OperatingSystemSecurity> ;
                                      <http://www.w3.org/2004/02/skos/core#definition> "Secure Software Installation Management: Overseeing the installation, maintenance, and updating of software applications in an organisation."@en ;
                                      <http://www.w3.org/2004/02/skos/core#exactMatch> <http://JP_ontology.org/iso27001/ControlA.8.19> ;
                                      <http://www.w3.org/2004/02/skos/core#note> "DPV Mapping Coverage: Broader Match"@en ,
                                                                                 """ISO - DPV Mapping Assumptions / Commentary: The ISO Control emphasizes the need for implementing procedures and measures to securely manage software installation on operational systems. It focuses on the specific aspect of ensuring security during the software installation process.
Operating System Security is a broader concept that encompasses various measures and practices aimed at securing the operating systems of computer systems. DPV: Security implemented at or through operating systems"""@en ,
                                                                                 "This NIS2V Term aligns with Article 21.2 e: Security in network and information systems acquisition, development and maintenance, including vulnerability handling and disclosure"@en ,
                                                                                 "This NIS2V Term aligns with Article 21.2 g: Basic computer hygiene practices and cybersecurity training"@en ;
                                      <http://www.w3.org/2004/02/skos/core#prefLabel> "Secure Software Installation Management"@en .


:SecurityConfigurationOversight <http://purl.org/dc/terms/contributor> "Jenni Parry" ;
                                <http://purl.org/dc/terms/created> "2024-06-04"^^xsd:date ;
                                <http://purl.org/dc/terms/source> "ISO 27001:2022 Control Framework"@en ;
                                rdfs:isDefinedBy <http://JP_ontology.org/nis2v> ;
                                <http://www.w3.org/2004/02/skos/core#altLabel> "NIS2V Term"@en ;
                                <http://www.w3.org/2004/02/skos/core#definition> "Security Configuration Oversight: Establishment, documentation, implementation, and ongoing review of security configurations for all IT components."@en ;
                                <http://www.w3.org/2004/02/skos/core#exactMatch> <http://JP_ontology.org/iso27001/ControlA.8.9> ;
                                <http://www.w3.org/2004/02/skos/core#note> "DPV Mapping Coverage: Complex Match"@en ,
                                                                           """ISO - DPV Mapping Assumptions / Commentary: The ISO control addresses the establishment, documentation, implementation, monitoring, and review of configurations, including security configurations, of various elements such as hardware, software, services, and networks. It encompasses a broad range of configurations across different components within an organisation's infrastructure.
Each of the terms (Hardware Security Protocols and Network Security Protocols) refers to security protocols specific to different domains. These protocols are narrower in scope compared to the overall configurations addressed in the control. They focus on security measures and protocols relevant to specific technologies or communication mediums.
Hardware Security Protocols - DPV: Security protocols implemented at or within hardware
Network Security Protocols - DPV: Security implemented at or over networks protocols"""@en ,
                                                                           "This NIS2V Term aligns with Article 21.2 e: Security in network and information systems acquisition, development and maintenance, including vulnerability handling and disclosure"@en ,
                                                                           "This NIS2V Term aligns with Article 21.2 g: Basic computer hygiene practices and cybersecurity training"@en ;
                                <http://www.w3.org/2004/02/skos/core#prefLabel> "Security Configuration Oversight"@en ;
                                <http://www.w3.org/2004/02/skos/core#related> <https://w3id.org/dpv#HardwareSecurityProtocols> ,
                                                                              <https://w3id.org/dpv#NetworkSecurityProtocols> .


:SecurityEventReportingMechanism <http://purl.org/dc/terms/contributor> "Jenni Parry" ;
                                 <http://purl.org/dc/terms/created> "2024-06-04"^^xsd:date ;
                                 <http://purl.org/dc/terms/source> "ISO 27001:2022 Control Framework"@en ;
                                 rdfs:isDefinedBy <http://JP_ontology.org/nis2v> ;
                                 <http://www.w3.org/2004/02/skos/core#altLabel> "NIS2V Term"@en ;
                                 <http://www.w3.org/2004/02/skos/core#definition> "Security Event Reporting Mechanism: Establishment of protocols for personnel to report suspected or observed security events swiftly via appropriate channels."@en ;
                                 <http://www.w3.org/2004/02/skos/core#exactMatch> <http://JP_ontology.org/iso27001/ControlA.6.8> ,
                                                                                  <https://w3id.org/dpv#SecurityIncidentNotification> ;
                                 <http://www.w3.org/2004/02/skos/core#note> "DPV Mapping Coverage: Exact Match"@en ,
                                                                            """ISO - DPV Mapping Assumptions / Commentary: Security Incident Notification would be considered an exact match of the ISO control
DPV: Notification of information about security incident(s)"""@en ,
                                                                            "This NIS2V Term aligns with Article 21.2 b: Incident handling"@en ;
                                 <http://www.w3.org/2004/02/skos/core#prefLabel> "Security Event Reporting Mechanism"@en .


:SecurityIncidentCategorisation <http://purl.org/dc/terms/contributor> "Jenni Parry" ;
                                <http://purl.org/dc/terms/created> "2024-04-26"^^xsd:date ,
                                                                   "2024-05-01"^^xsd:date ;
                                <http://purl.org/dc/terms/source> "ENISA: Minimum Security Measures for Operators of Essentials Services, https://www.enisa.europa.eu/topics/cybersecurity-policy/nis-directive-new/minimum-security-measures-for-operators-of-essentials-services"@en ,
                                                                  "ISO 27001:2022 Control Framework"@en ;
                                rdfs:isDefinedBy <http://JP_ontology.org/nis2v> ;
                                <http://www.w3.org/2004/02/skos/core#altLabel> "NIS2V Term"@en ;
                                <http://www.w3.org/2004/02/skos/core#definition> "Assessment of security events by the organisation to determine if they qualify as security incidents."@en ;
                                <http://www.w3.org/2004/02/skos/core#exactMatch> <http://JP_ontology.org/iso27001/ControlA.5.25> ;
                                <http://www.w3.org/2004/02/skos/core#note> "This NIS2V Term aligns with Article 21.2b: Incident handling, such as the prevention, detection, and response to incidents."@en ;
                                <http://www.w3.org/2004/02/skos/core#prefLabel> "Security Incident Categorisation"@en .


:SecurityLoggingandAnalysis <http://purl.org/dc/terms/contributor> "Jenni Parry" ;
                            <http://purl.org/dc/terms/created> "2024-06-04"^^xsd:date ;
                            <http://purl.org/dc/terms/source> "ISO 27001:2022 Control Framework"@en ;
                            rdfs:isDefinedBy <http://JP_ontology.org/nis2v> ;
                            <http://www.w3.org/2004/02/skos/core#altLabel> "NIS2V Term"@en ;
                            <http://www.w3.org/2004/02/skos/core#broader> <https://w3id.org/dpv#LoggingPolicy> ;
                            <http://www.w3.org/2004/02/skos/core#definition> "Security Logging and Analysis: Production, storage, protection, and analysis of logs detailing activities, exceptions, and faults to maintain security oversight."@en ;
                            <http://www.w3.org/2004/02/skos/core#exactMatch> <http://JP_ontology.org/iso27001/ControlA.8.15> ;
                            <http://www.w3.org/2004/02/skos/core#note> "DPV Mapping Coverage: Broader Match"@en ,
                                                                       """ISO - DPV Mapping Assumptions / Commentary: The term Logging Policy closely matches the requirements outlined in the control statement but is broader. It encapsulates the governance aspect and the policy framework that would guide the specific actions required by the control (producing, storing, protecting, and analysing logs).
DPV: Policy for logging of information"""@en ,
                                                                       "This NIS2V Term aligns with Article 21.2 b: Incident handling"@en ;
                            <http://www.w3.org/2004/02/skos/core#prefLabel> "Security Logging and Analysis"@en .


:SecurityOfAssetsOffPremises <http://purl.org/dc/terms/contributor> "Jenni Parry" ;
                             <http://purl.org/dc/terms/created> "2024-04-17"^^xsd:date ;
                             <http://purl.org/dc/terms/source> "ISO 27001:2022 Control Framework"@en ;
                             rdfs:isDefinedBy <http://JP_ontology.org/nis2v> ;
                             <http://www.w3.org/2004/02/skos/core#altLabel> "NIS2V Term"@en ;
                             <http://www.w3.org/2004/02/skos/core#definition> "Measures taken to protect an organisation's property and information when they are located outside of the main business site."@en ;
                             <http://www.w3.org/2004/02/skos/core#exactMatch> <http://JP_ontology.org/iso27001/ControlA.7.9> ;
                             <http://www.w3.org/2004/02/skos/core#note> "This NIS2V Term aligns with Article 21.2i: Human resources security, access control policies and asset management."@en ;
                             <http://www.w3.org/2004/02/skos/core#prefLabel> "Security of Assets Off-Premises"@en .


:SecurityRolesResponsibilityAllocation <http://purl.org/dc/terms/contributor> "Jenni Parry" ;
                                       <http://purl.org/dc/terms/created> "2024-06-05"^^xsd:date ;
                                       <http://purl.org/dc/terms/source> "ISO 27001:2022 Control Framework"@en ;
                                       rdfs:isDefinedBy <http://JP_ontology.org/nis2v> ;
                                       <http://www.w3.org/2004/02/skos/core#altLabel> "NIS2V Term"@en ;
                                       <http://www.w3.org/2004/02/skos/core#definition> "Security Roles Responsibility Allocation: Allocation of information security roles and responsibilities tailored to the organisation's specific needs."@en ;
                                       <http://www.w3.org/2004/02/skos/core#exactMatch> <http://JP_ontology.org/iso27001/ControlA.5.2> ;
                                       <http://www.w3.org/2004/02/skos/core#note> "This NIS2V Term aligns with Article 21.2 a: Policies on risk analysis and information system security"@en ,
                                                                                  "This NIS2V Term aligns with Article 21.2 i: Human resources security, access control policies and asset management;"@en ;
                                       <http://www.w3.org/2004/02/skos/core#prefLabel> "Security Roles Responsibility Allocation"@en .


:SegregationOfDuties <http://purl.org/dc/terms/contributor> "Jenni Parry" ;
                     <http://purl.org/dc/terms/created> "2024-04-17"^^xsd:date ;
                     <http://purl.org/dc/terms/source> "ISO 27001:2022 Control Framework"@en ;
                     rdfs:isDefinedBy <http://JP_ontology.org/nis2v> ;
                     <http://www.w3.org/2004/02/skos/core#altLabel> "NIS2V Term"@en ;
                     <http://www.w3.org/2004/02/skos/core#definition> "A risk management practice that divides critical tasks among different people to prevent fraud and errors."@en ;
                     <http://www.w3.org/2004/02/skos/core#exactMatch> <http://JP_ontology.org/iso27001/ControlA.5.3> ;
                     <http://www.w3.org/2004/02/skos/core#note> "This NIS2V Term aligns with Article 21.2i: Human resources security, access control policies and asset management."@en ;
                     <http://www.w3.org/2004/02/skos/core#prefLabel> "Segregation of Duties"@en .


:SegregationOfNetworks <http://purl.org/dc/terms/contributor> "Jenni Parry" ;
                       <http://purl.org/dc/terms/created> "2024-05-01"^^xsd:date ;
                       <http://purl.org/dc/terms/source> "ISO 27001:2022 Control Framework"@en ;
                       rdfs:isDefinedBy <http://JP_ontology.org/nis2v> ;
                       <http://www.w3.org/2004/02/skos/core#altLabel> "NIS2V Term"@en ;
                       <http://www.w3.org/2004/02/skos/core#definition> "The practice of separating systems, networks, and information to reduce the risk of unauthorized access and improve security."@en ;
                       <http://www.w3.org/2004/02/skos/core#exactMatch> <http://JP_ontology.org/iso27001/ControlA.8.22> ;
                       <http://www.w3.org/2004/02/skos/core#note> "This NIS2V Term aligns with Article 21.2e: Security in network and information systems acquisition, development and maintenance, including vulnerability handling and disclosure."@en ;
                       <http://www.w3.org/2004/02/skos/core#prefLabel> "Segregation of Networks"@en .


:SeparationOfEnvironments <http://purl.org/dc/terms/contributor> "Jenni Parry" ;
                          <http://purl.org/dc/terms/created> "2024-05-01"^^xsd:date ;
                          <http://purl.org/dc/terms/source> "ENISA: Minimum Security Measures for Operators of Essentials Services, https://www.enisa.europa.eu/topics/cybersecurity-policy/nis-directive-new/minimum-security-measures-for-operators-of-essentials-services"@en ;
                          rdfs:isDefinedBy <http://JP_ontology.org/nis2v> ;
                          <http://www.w3.org/2004/02/skos/core#altLabel> "NIS2V Term"@en ;
                          <http://www.w3.org/2004/02/skos/core#definition> "Refers to the practice of maintaining distinct and segregated environments within an organisation's IT infrastructure to prevent interference and ensure security."@en ;
                          <http://www.w3.org/2004/02/skos/core#exactMatch> <http://JP_ontology.org/iso27001/ControlA.8.31> ;
                          <http://www.w3.org/2004/02/skos/core#note> "This NIS2V Term aligns with Article 21.2e: Security in network and information systems acquisition, development, and maintenance."@en ;
                          <http://www.w3.org/2004/02/skos/core#prefLabel> "Separation of Environments"@en .


:SourceCodeandDevelopmentAccessControl <http://purl.org/dc/terms/contributor> "Jenni Parry" ;
                                       <http://purl.org/dc/terms/created> "2024-06-05"^^xsd:date ;
                                       <http://purl.org/dc/terms/source> "ISO 27001:2022 Control Framework"@en ;
                                       rdfs:isDefinedBy <http://JP_ontology.org/nis2v> ;
                                       <http://www.w3.org/2004/02/skos/core#altLabel> "NIS2V Term"@en ;
                                       <http://www.w3.org/2004/02/skos/core#definition> "Source Code and Development Access Control: Management of read and write access to source code, development tools, and software libraries in a manner that aligns with appropriate security measures and controls."@en ;
                                       <http://www.w3.org/2004/02/skos/core#exactMatch> <http://JP_ontology.org/iso27001/ControlA.8.4> ;
                                       <http://www.w3.org/2004/02/skos/core#note> "This NIS2V Term aligns with Article 21.2 i: Human resources security, access control policies and asset management;"@en ;
                                       <http://www.w3.org/2004/02/skos/core#prefLabel> "Source Code and Development Access Control"@en .


:StorageMediaDisposalProtocol <http://purl.org/dc/terms/contributor> "Jenni Parry" ;
                              <http://purl.org/dc/terms/created> "2024-06-04"^^xsd:date ;
                              <http://purl.org/dc/terms/source> "ISO 27001:2022 Control Framework"@en ;
                              rdfs:isDefinedBy <http://JP_ontology.org/nis2v> ;
                              <http://www.w3.org/2004/02/skos/core#altLabel> "NIS2V Term"@en ;
                              <http://www.w3.org/2004/02/skos/core#definition> "Storage Media Disposal Protocol: Verification process to ensure removal or secure overwrite of sensitive data and licensed software from equipment containing storage media before disposal or reuse."@en ;
                              <http://www.w3.org/2004/02/skos/core#exactMatch> <http://JP_ontology.org/iso27001/ControlA.7.14> ;
                              <http://www.w3.org/2004/02/skos/core#narrower> <https://w3id.org/dpv#Erase> ;
                              <http://www.w3.org/2004/02/skos/core#note> "DPV Mapping Coverage: Narrower Match"@en ,
                                                                         """ISO - DPV Mapping Assumptions / Commentary: The control focuses on ensuring that sensitive data and licensed software are removed or securely overwritten on storage media within equipment before disposal or re-use.
Erase: This term is directly relevant but narrower, focusing on the action of removing data from storage media. Erase encompasses the processes involved in eliminating data to prevent its recovery. In the context of the control, it specifically addresses the requirement for data to be removed from equipment's storage media, which includes both the deletion of files and the secure wiping (overwriting) to ensure data cannot be retrieved.
DPV: to remove data from existence i.e. without the possibility of retrieval
"""@en ,
                                                                         "This NIS2V Term aligns with Article 21.2 i: Human resources security, access control policies and asset management;"@en ;
                              <http://www.w3.org/2004/02/skos/core#prefLabel> "Storage Media Disposal Protocol"@en .


:StorageMediaManagement <http://purl.org/dc/terms/contributor> "Jenni Parry" ;
                        <http://purl.org/dc/terms/created> "2024-06-04"^^xsd:date ;
                        <http://purl.org/dc/terms/source> "ISO 27001:2022 Control Framework"@en ;
                        rdfs:isDefinedBy <http://JP_ontology.org/nis2v> ;
                        <http://www.w3.org/2004/02/skos/core#altLabel> "NIS2V Term"@en ;
                        <http://www.w3.org/2004/02/skos/core#definition> """
Storage Media Management: Refers to the systematic and organized handling, maintenance, and administration of various types of storage devices or media used to store digital data. This includes activities such as inventory management, provisioning, data migration, backup and recovery, security measures, and disposal or recycling of storage media in accordance with relevant policies and regulations."""@en ;
                        <http://www.w3.org/2004/02/skos/core#exactMatch> <http://JP_ontology.org/iso27001/ControlA.7.10> ;
                        <http://www.w3.org/2004/02/skos/core#note> "DPV Mapping Coverage: Complex Match"@en ,
                                                                   """ISO - DPV Mapping Assumptions / Commentary: Narrower Aspects of Lifecycle Management: Storage Condition, Storage Deletion and Storage Duration are narrower terms that address specific aspects of the storage media lifecycle management process. Each term corresponds to important elements within the lifecycle stages but individually covers only part of the overall management process described in the control.
Storage Condition - DPV: Conditions required or followed regarding storage of data
Storage Deletion - DPV: Deletion or Erasure of data including any deletion guarantees
Storage Duration - DPV: Duration or temporal limitation on storage of data"""@en ,
                                                                   "This NIS2V Term aligns with Article 21.2 i: Human resources security, access control policies and asset management;"@en ;
                        <http://www.w3.org/2004/02/skos/core#prefLabel> "Storage Media Management"@en ;
                        <http://www.w3.org/2004/02/skos/core#related> <https://w3id.org/dpv#StorageCondition> ,
                                                                      <https://w3id.org/dpv#StorageDeletion> ,
                                                                      <https://w3id.org/dpv#StorageDuration> .


:SupplierSecurityRequirementsManagement <http://purl.org/dc/terms/contributor> "Jenni Parry" ;
                                        <http://purl.org/dc/terms/created> "2024-06-04"^^xsd:date ;
                                        <http://purl.org/dc/terms/source> "ISO 27001:2022 Control Framework"@en ;
                                        rdfs:isDefinedBy <http://JP_ontology.org/nis2v> ;
                                        <http://www.w3.org/2004/02/skos/core#altLabel> "NIS2V Term"@en ;
                                        <http://www.w3.org/2004/02/skos/core#definition> "Supplier Security Requirements Management: Establishment and agreement of specific information security requirements with suppliers, tailored to the nature of each supplier relationship."@en ;
                                        <http://www.w3.org/2004/02/skos/core#exactMatch> <http://JP_ontology.org/iso27001/ControlA.5.20> ;
                                        <http://www.w3.org/2004/02/skos/core#note> "DPV Mapping Coverage: Complex Match"@en ,
                                                                                   """ISO - DPV Mapping Assumptions / Commentary: Vendor Management is essential for the practical aspects of managing supply chain risks, focusing on the relationships with suppliers and the contractual mechanisms to control risks.
DPV: Purposes associated with manage orders, payment, evaluation, and prospecting related to vendors.
The ISO control would be considered broader compared to Third-Party Agreement and Third Party Contract.
As DPV is GDPR focused these terms are limited:
DPV - Third-Party Agreement: An agreement outlining conditions, criteria, obligations, responsibilities, and specifics for carrying out processing of data between a Data Controller or Processor and a Third Party
DPV - Third Party Contract: Creation, completion, fulfilment, or performance of a contract, with the Data Controller and Third Party as parties, and involving specified processing"""@en ,
                                                                                   "This NIS2V Term aligns with Article 21.2 d: Supply chain security, including security-related aspects concerning the relationships between each entity and its direct suppliers or service providers "@en ;
                                        <http://www.w3.org/2004/02/skos/core#prefLabel> "Supplier Security Requirements Management"@en ;
                                        <http://www.w3.org/2004/02/skos/core#related> <https://w3id.org/dpv#ThirdPartyAgreement> ,
                                                                                      <https://w3id.org/dpv#ThirdPartyContract> ,
                                                                                      <https://w3id.org/dpv#VendorManagement> .


:SupplyChainDiligence <http://purl.org/dc/terms/contributor> "Jenni Parry" ;
                      <http://purl.org/dc/terms/created> "2024-06-04"^^xsd:date ;
                      <http://purl.org/dc/terms/source> "ISO 27001:2022 Control Framework"@en ;
                      rdfs:isDefinedBy <http://JP_ontology.org/nis2v> ;
                      <http://www.w3.org/2004/02/skos/core#altLabel> "NIS2V Term"@en ;
                      <http://www.w3.org/2004/02/skos/core#definition> "Supply Chain Diligence: The careful and systematic examination, assessment, and verification of the components, processes, and practices within a supply chain to ensure compliance with security requirements and standards."@en ;
                      <http://www.w3.org/2004/02/skos/core#exactMatch> <http://JP_ontology.org/iso27001/ControlA.5.22> ,
                                                                       <https://w3id.org/dpv#VendorManagement> ;
                      <http://www.w3.org/2004/02/skos/core#note> "DPV Mapping Coverage: Exact Match"@en ,
                                                                 """ISO - DPV Mapping Assumptions / Commentary: Vendor Management aligns with the requirements of the control statement, covering the broad activities of overseeing suppliers and specifically monitoring their compliance with information security standards.
DPV: Purposes associated with manage orders, payment, evaluation, and prospecting related to vendors"""@en ,
                                                                 "This NIS2V Term aligns with Article 21.2 d: Supply chain security, including security-related aspects concerning the relationships between each entity and its direct suppliers or service providers "@en ;
                      <http://www.w3.org/2004/02/skos/core#prefLabel> "Supply Chain Diligence"@en .


:SupportingUtilities <http://purl.org/dc/terms/contributor> "Jenni Parry" ;
                     <http://purl.org/dc/terms/created> "2024-04-24"^^xsd:date ;
                     <http://purl.org/dc/terms/source> "ISO 27001:2022 Control Framework"@en ;
                     rdfs:isDefinedBy <http://JP_ontology.org/nis2v> ;
                     <http://www.w3.org/2004/02/skos/core#altLabel> "NIS2V Term"@en ;
                     <http://www.w3.org/2004/02/skos/core#definition> "Supporting Utilities: Strategies and actions designed to enhance a facility's ability to withstand and rapidly recover from disruptions, such as natural disasters or power failures."@en ;
                     <http://www.w3.org/2004/02/skos/core#exactMatch> <http://JP_ontology.org/iso27001/ControlA.7.11> ;
                     <http://www.w3.org/2004/02/skos/core#note> "This NIS2V Term aligns with Article 21.2c: Business continuity management, including backup management, crisis management and disaster recovery."@en ;
                     <http://www.w3.org/2004/02/skos/core#prefLabel> "Supporting Utilities"@en .


:TechnicalVulnerabilityManagement <http://purl.org/dc/terms/contributor> "Jenni Parry" ;
                                  <http://purl.org/dc/terms/created> "2024-06-04"^^xsd:date ;
                                  <http://purl.org/dc/terms/source> "ISO 27001:2022 Control Framework"@en ;
                                  rdfs:isDefinedBy <http://JP_ontology.org/nis2v> ;
                                  <http://www.w3.org/2004/02/skos/core#altLabel> "NIS2V Term"@en ;
                                  <http://www.w3.org/2004/02/skos/core#definition> "Technical Vulnerability Management: Acquisition and assessment of technical vulnerabilities in information systems, with appropriate mitigation measures implemented."@en ;
                                  <http://www.w3.org/2004/02/skos/core#exactMatch> <http://JP_ontology.org/iso27001/ControlA.8.8> ;
                                  <http://www.w3.org/2004/02/skos/core#narrower> <https://w3id.org/dpv#VulnerabilityTestingMethods> ;
                                  <http://www.w3.org/2004/02/skos/core#note> "DPV Mapping Coverage: Narrower Match"@en ,
                                                                             """ISO - DPV Mapping Assumptions / Commentary: Vulnerability Testing Methods represents a narrower concept compared to the ISO control. While vulnerability testing methods are used to identify vulnerabilities in information systems, the control encompasses a broader scope, including obtaining information about vulnerabilities, evaluating exposure, and taking appropriate measures.
DPV: Methods that assess or discover vulnerabilities in a system"""@en ,
                                                                             "This NIS2V Term aligns with Article 21.2 e: Security in network and information systems acquisition, development and maintenance, including vulnerability handling and disclosure"@en ,
                                                                             "This NIS2V Term aligns with Article 21.2 g: Basic computer hygiene practices and cybersecurity training"@en ;
                                  <http://www.w3.org/2004/02/skos/core#prefLabel> "Technical Vulnerability Management"@en .


:TermsAndConditionsOfEmployment <http://purl.org/dc/terms/contributor> "Jenni Parry" ;
                                <http://purl.org/dc/terms/created> "2024-04-17"^^xsd:date ;
                                <http://purl.org/dc/terms/source> "ISO 27001:2022 Control Framework"@en ;
                                rdfs:isDefinedBy <http://JP_ontology.org/nis2v> ;
                                <http://www.w3.org/2004/02/skos/core#altLabel> "NIS2V Term"@en ;
                                <http://www.w3.org/2004/02/skos/core#definition> "The rules, obligations, and expectations that constitute the agreement between an employer and employee regarding the job role and employment relationship."@en ;
                                <http://www.w3.org/2004/02/skos/core#exactMatch> <http://JP_ontology.org/iso27001/ControlA.6.2> ;
                                <http://www.w3.org/2004/02/skos/core#note> "This NIS2V Term aligns with Article 21.2i: Human resources security, access control policies and asset management."@en ;
                                <http://www.w3.org/2004/02/skos/core#prefLabel> "Terms and Conditions of Employment"@en .


:ThirdPartySecurityProcedures <http://purl.org/dc/terms/contributor> "Jenni Parry" ;
                              <http://purl.org/dc/terms/created> "2024-06-04"^^xsd:date ;
                              <http://purl.org/dc/terms/source> "ISO 27001:2022 Control Framework"@en ;
                              rdfs:isDefinedBy <http://JP_ontology.org/nis2v> ;
                              <http://www.w3.org/2004/02/skos/core#altLabel> "NIS2V Term"@en ;
                              <http://www.w3.org/2004/02/skos/core#definition> "Third Party Security Procedures: Security measures and protocols put in place to manage and mitigate the risks associated with the involvement of third-party vendors, contractors, or service providers in an organisation's operations, systems, or data handling processes."@en ;
                              <http://www.w3.org/2004/02/skos/core#exactMatch> <http://JP_ontology.org/iso27001/ControlA.5.19> ,
                                                                               <https://w3id.org/dpv#ThirdPartySecurityProcedures> ;
                              <http://www.w3.org/2004/02/skos/core#note> "DPV Mapping Coverage: Exact Match"@en ,
                                                                         "ISO - DPV Mapping Assumptions / Commentary: Third Party Security Procedures directly corresponds with the control's requirements for defining and implementing processes and procedures to manage information security risks from suppliers."@en ,
                                                                         "This NIS2V Term aligns with Article 21.2 d: Supply chain security, including security-related aspects concerning the relationships between each entity and its direct suppliers or service providers "@en ;
                              <http://www.w3.org/2004/02/skos/core#prefLabel> "Third Party Security Procedures"@en .


:ThreatIntelligence <http://purl.org/dc/terms/contributor> "Jenni Parry" ;
                    <http://purl.org/dc/terms/created> "2024-04-15"^^xsd:date ;
                    <http://purl.org/dc/terms/source> "ISO 27001:2022 Control Framework"@en ;
                    rdfs:isDefinedBy <http://JP_ontology.org/nis2v> ;
                    <http://www.w3.org/2004/02/skos/core#altLabel> "NIS2V Term"@en ;
                    <http://www.w3.org/2004/02/skos/core#definition> "Involves gathering and analysing information on potential cyber threats to help organisations pre-emptively identify and mitigate security risks."@en ;
                    <http://www.w3.org/2004/02/skos/core#exactMatch> <http://JP_ontology.org/iso27001/ControlA.5.7> ;
                    <http://www.w3.org/2004/02/skos/core#note> "This NIS2V Term aligns with Article 21.2a: Policies on risk analysis and information system security."@en ;
                    <http://www.w3.org/2004/02/skos/core#prefLabel> "Threat Intelligence"@en .


:UtilityProgramAccessRestrictions <http://purl.org/dc/terms/contributor> "Jenni Parry" ;
                                  <http://purl.org/dc/terms/created> "2024-06-04"^^xsd:date ;
                                  <http://purl.org/dc/terms/source> "ISO 27001:2022 Control Framework"@en ;
                                  rdfs:isDefinedBy <http://JP_ontology.org/nis2v> ;
                                  <http://www.w3.org/2004/02/skos/core#altLabel> "NIS2V Term"@en ;
                                  <http://www.w3.org/2004/02/skos/core#broader> <https://w3id.org/dpv#SecurityRoleProcedures> ;
                                  <http://www.w3.org/2004/02/skos/core#definition> "Utility Program Access Restrictions: Limitation and stringent control over the utilisation of utility programs capable of bypassing system and application controls to ensure security and integrity of operations."@en ;
                                  <http://www.w3.org/2004/02/skos/core#exactMatch> <http://JP_ontology.org/iso27001/ControlA.8.18> ;
                                  <http://www.w3.org/2004/02/skos/core#note> "DPV Mapping Coverage: Broader Match"@en ,
                                                                             """ISO - DPV Mapping Assumptions / Commentary: The ISO control addresses the control and restriction of utility programs capable of overriding system and application controls, which is a more specific aspect of security management.
Security Role Procedures, while important for overall security management, covers a broader range of security-related procedures beyond the specific control of utility programs.
DPV: Procedures related to security roles"""@en ,
                                                                             "This NIS2V Term aligns with Article 21.2 i: Human resources security, access control policies and asset management;"@en ;
                                  <http://www.w3.org/2004/02/skos/core#prefLabel> "Utility Program Access Restrictions"@en .


<http://JP_ontology.org/nis2v/Monitoring,Measurement,AnalysisandEvaluation> <http://purl.org/dc/terms/contributor> "Jenni Parry" ;
                                                                            <http://purl.org/dc/terms/created> "2024-06-04"^^xsd:date ;
                                                                            <http://purl.org/dc/terms/source> "ISO 27001:2022 Control Framework"@en ;
                                                                            rdfs:isDefinedBy <http://JP_ontology.org/nis2v> ;
                                                                            <http://www.w3.org/2004/02/skos/core#altLabel> "NIS2V Term"@en ;
                                                                            <http://www.w3.org/2004/02/skos/core#definition> "Monitoring, Measurement, Analysis, and Evaluation involves systematically observing, quantifying, examining, and assessing various aspects of an organisation's performance, processes, products, or services to ensure effectiveness, identify opportunities for improvement, and support informed decision-making."@en ;
                                                                            <http://www.w3.org/2004/02/skos/core#exactMatch> <http://JP_ontology.org/iso27001/Control9.1> ;
                                                                            <http://www.w3.org/2004/02/skos/core#narrower> <https://w3id.org/dpv#ActivityMonitoring> ;
                                                                            <http://www.w3.org/2004/02/skos/core#note> "DPV Mapping Coverage: Narrower Match"@en ,
                                                                                                                       """ISO - DPV Mapping Assumptions / Commentary: The ISO control outlines a comprehensive process for determining what needs to be monitored and measured within an organisation's information security management system. It includes specifying methods, timing, responsible parties, analysis, and evaluation of monitoring results.
Narrower Match: Activity monitoring is one element of the overall monitoring, measurement, analysis and evaluation processes.
DPV: Monitoring of activities including assessing whether they have been successfully initiated and completed"""@en ,
                                                                                                                       "This NIS2V Term aligns with Article 21.2 f: Policies and procedures to assess the effectiveness of cybersecurity risk management measures"@en ;
                                                                            <http://www.w3.org/2004/02/skos/core#prefLabel> "Monitoring, Measurement, Analysis and Evaluation"@en .


<http://JP_ontology.org/nis2v/Non-DisclosureAgreement(NDA)> <http://purl.org/dc/terms/contributor> "Jenni Parry" ;
                                                            <http://purl.org/dc/terms/created> "2024-06-04"^^xsd:date ;
                                                            <http://purl.org/dc/terms/source> "ISO 27001:2022 Control Framework"@en ;
                                                            rdfs:isDefinedBy <http://JP_ontology.org/nis2v> ;
                                                            <http://www.w3.org/2004/02/skos/core#altLabel> "NIS2V Term"@en ;
                                                            <http://www.w3.org/2004/02/skos/core#definition> "Non-Disclosure Agreement (NDA): A legal contract or agreement between parties, typically employees, contractors, or business partners, in which they agree to protect confidential information shared with them during the course of their engagement or employment, and to refrain from disclosing it to unauthorized parties."@en ;
                                                            <http://www.w3.org/2004/02/skos/core#exactMatch> <http://JP_ontology.org/iso27001/ControlA.6.6> ,
                                                                                                             <https://w3id.org/dpv#NDA> ;
                                                            <http://www.w3.org/2004/02/skos/core#note> "DPV Mapping Coverage: Exact Match"@en ,
                                                                                                       "ISO - DPV Mapping Assumptions / Commentary: Non-Disclosure Agreement (NDA) directly corresponds with the control's requirements. It represents a specific type of legal agreement focused on protecting confidential information."@en ,
                                                                                                       "This NIS2V Term aligns with Article 21.2 i: Human resources security, access control policies and asset management;"@en ;
                                                            <http://www.w3.org/2004/02/skos/core#prefLabel> "Non-Disclosure Agreement (NDA)"@en .


###  Generated by the OWL API (version 5.1.18) https://github.com/owlcs/owlapi/
